<?xml version="1.0"?>
<rdf:RDF xmlns="http://people.aifb.kit.edu/mu2771/step-nearly-all#"
     xml:base="http://people.aifb.kit.edu/mu2771/step-nearly-all"
     xmlns:qudt="http://qudt.org/schema/qudt#"
     xmlns:vaem="http://www.linkedmodel.org/schema/vaem#"
     xmlns:ns="http://www.w3.org/2003/06/sw-vocab-status/ns#"
     xmlns:owl="http://www.w3.org/2002/07/owl#"
     xmlns:org="http://www.w3.org/ns/org#"
     xmlns:part="https://www.w3.org/2001/sw/BestPractices/OEP/SimplePartWhole/part.owl#"
     xmlns:voag="http://voag.linkedmodel.org/schema/voag#"
     xmlns:xsd="http://www.w3.org/2001/XMLSchema#"
     xmlns:dtype="http://www.linkedmodel.org/schema/dtype#"
     xmlns:skos="http://www.w3.org/2004/02/skos/core#"
     xmlns:rdfs="http://www.w3.org/2000/01/rdf-schema#"
     xmlns:ns1="http://creativecommons.org/ns#"
     xmlns:rdf="http://www.w3.org/1999/02/22-rdf-syntax-ns#"
     xmlns:terms="http://purl.org/dc/terms/"
     xmlns:www="http://www.example.org/"
     xmlns:xml="http://www.w3.org/XML/1998/namespace"
     xmlns:iirds="http://iirds.tekom.de/iirds#"
     xmlns:wgs84_pos="http://www.w3.org/2003/01/geo/wgs84_pos#"
     xmlns:step="http://people.aifb.kit.edu/mu2771/step#"
     xmlns:time="http://www.w3.org/2006/time#"
     xmlns:foaf="http://xmlns.com/foaf/0.1/"
     xmlns:dc="http://purl.org/dc/elements/1.1/">
    <owl:Ontology rdf:about="http://people.aifb.kit.edu/mu2771/step-nearly-all">
        <owl:versionIRI rdf:resource="http://people.aifb.kit.edu/mu2771/step-nearly-all/0.1"/>
        <owl:imports rdf:resource="http://people.aifb.kit.edu/mu2771/extern/qudt-dimensionalunit.owl"/>
        <owl:imports rdf:resource="http://people.aifb.kit.edu/mu2771/extern/qudt-quantity.owl"/>
        <owl:imports rdf:resource="http://people.aifb.kit.edu/mu2771/extern/qudt-dimension.owl"/>
        <owl:imports rdf:resource="http://www.loa-cnr.it/ontologies/DUL.owl"/>
        <owl:imports rdf:resource="http://people.aifb.kit.edu/mu2771/extern/qudt-schema.owl"/>
        <owl:imports rdf:resource="http://people.aifb.kit.edu/mu2771/extern/qudt-unit.owl"/>
        <skos:changeNote>2017-02 - intervalIn, intervalDisjoint, monthOfYear added; TemporalUnit subclass of TemporalDuration</skos:changeNote>
        <rdfs:label xml:lang="it">Ontologia delle organizzazioni</rdfs:label>
        <rdfs:label xml:lang="en">Ontology for vCard</rdfs:label>
        <rdfs:seeAlso rdf:resource="http://www.w3.org/TR/owl-time"/>
        <terms:modified rdf:datatype="http://www.w3.org/2001/XMLSchema#date">2012-10-06</terms:modified>
        <terms:modified rdf:datatype="http://www.w3.org/2001/XMLSchema#date">2010-10-08</terms:modified>
        <rdfs:comment xml:lang="es">Vocabulario para describir organizaciones, adaptable a una amplia variedad de ellas.</rdfs:comment>
        <terms:license rdf:resource="http://www.opendatacommons.org/licenses/pddl/1.0/"/>
        <rdfs:label xml:lang="fr">Ontologie des organisations</rdfs:label>
        <rdfs:seeAlso rdf:resource="http://dx.doi.org/10.3233/SW-150187"/>
        <rdfs:label xml:lang="es">Ontología de organizaciones</rdfs:label>
        <rdfs:comment xml:lang="en">Module C of the STEP ontology</rdfs:comment>
        <skos:changeNote>2016-12-20 - restore time:Year and time:January which were present in the 2006 version of the ontology, but now marked &quot;deprecated&quot;. </skos:changeNote>
        <rdfs:comment rdf:datatype="http://www.w3.org/2001/XMLSchema#string">This ontology describes sensors and observations, and related concepts.  It does not describe domain concepts, time, locations, etc. these are intended to be included from other ontologies via OWL imports.</rdfs:comment>
        <rdfs:comment xml:lang="en">Ontology for vCard based on RFC6350</rdfs:comment>
        <owl:priorVersion rdf:resource="http://www.w3.org/2006/time#2006"/>
        <dc:creator rdf:datatype="http://www.w3.org/2001/XMLSchema#string">W3C Semantic Sensor Network Incubator Group</dc:creator>
        <terms:isVersionOf rdf:resource="http://www.w3.org/TR/owl-time"/>
        <terms:rights xml:lang="en">Copyright © 2006-2017 W3C, OGC. W3C and OGC liability, trademark and document use rules apply.</terms:rights>
        <terms:creator rdf:resource="https://en.wikipedia.org/wiki/Jerry_Hobbs"/>
        <terms:modified rdf:datatype="http://www.w3.org/2001/XMLSchema#date">2014-01-02</terms:modified>
        <dc:date rdf:datatype="http://www.w3.org/2001/XMLSchema#dateTime">2018-01-10T12:22:00+02:00</dc:date>
        <vaem:intent xml:lang="en">Provides a data model for describing machines, sensors and and sensor data</vaem:intent>
        <rdfs:label rdf:datatype="http://www.w3.org/2001/XMLSchema#string">STEP Ontology Module B - A Box</rdfs:label>
        <skos:historyNote xml:lang="en">Update of OWL-Time ontology, extended to support general temporal reference systems. 

Ontology engineering by Simon J D Cox</skos:historyNote>
        <owl:versionInfo>0.8</owl:versionInfo>
        <terms:creator rdf:resource="http://orcid.org/0000-0002-3884-3420"/>
        <rdfs:label xml:lang="en">Core organization ontology</rdfs:label>
        <rdfs:comment xml:lang="it">Vocabolario per descrivere strutture organizzative, le quali possono essere specializzate in una vasta varietà di tipi di organizzazione</rdfs:comment>
        <dc:author rdf:datatype="http://www.w3.org/2001/XMLSchema#string">Sebastian Bader (sebastian.bader@kit.edu)</dc:author>
        <terms:created rdf:datatype="http://www.w3.org/2001/XMLSchema#date">2006-09-27</terms:created>
        <rdfs:label xml:lang="en">OWL-Time</rdfs:label>
        <owl:versionInfo xml:lang="en">0.4.0</owl:versionInfo>
        <terms:title xml:lang="fr">Ontologie des organisations</terms:title>
        <terms:contributor>
            <rdf:Description>
                <foaf:name>Guadalupe Aguado de Cea</foaf:name>
                <foaf:mbox>lupe@fi.upm.es</foaf:mbox>
            </rdf:Description>
        </terms:contributor>
        <terms:contributor>
            <rdf:Description>
                <foaf:name>Dave Reynolds</foaf:name>
                <foaf:mbox>dave@epimorphics.com</foaf:mbox>
            </rdf:Description>
        </terms:contributor>
        <terms:modified rdf:datatype="http://www.w3.org/2001/XMLSchema#date">2014-02-05</terms:modified>
        <rdfs:label rdf:datatype="http://www.w3.org/2001/XMLSchema#string">STEP Ontology Part B</rdfs:label>
        <terms:contributor>
            <rdf:Description>
                <foaf:name>Elena Montiel Ponsoda</foaf:name>
                <foaf:mbox>emontiel@fi.upm.es</foaf:mbox>
            </rdf:Description>
        </terms:contributor>
        <terms:modified rdf:datatype="http://www.w3.org/2001/XMLSchema#date">2017-04-06</terms:modified>
        <terms:modified rdf:datatype="http://www.w3.org/2001/XMLSchema#date">2010-06-09</terms:modified>
        <terms:title xml:lang="es">Ontología de organizaciones</terms:title>
        <skos:changeNote>2016-06-15 - initial update of OWL-Time - modified to support arbitrary temporal reference systems. </skos:changeNote>
        <rdfs:comment xml:lang="en">Vocabulary for describing organizational structures, specializable to a broad variety of types of organization.</rdfs:comment>
        <terms:license rdf:resource="https://creativecommons.org/licenses/by/4.0/"/>
        <terms:modified rdf:datatype="http://www.w3.org/2001/XMLSchema#date">2012-09-30</terms:modified>
        <terms:creator rdf:resource="mailto:panfeng66@gmail.com"/>
        <terms:modified>2011-06-20</terms:modified>
        <owl:versionInfo xml:lang="en">Final</owl:versionInfo>
        <rdfs:seeAlso rdf:resource="http://www.w3.org/TR/vocab-org/"/>
        <terms:created rdf:datatype="http://www.w3.org/2001/XMLSchema#date">2010-05-28</terms:created>
        <dc:identifier>http://purl.oclc.org/NET/ssnx/ssn</dc:identifier>
        <rdfs:comment rdf:datatype="http://www.w3.org/2001/XMLSchema#string">This ontology is developed by the W3C Semantic Sensor Networks Incubator Group (SSN-XG). The concepts and structure of the ontology were discussed in the group&apos;s meetings and on the mailing list. For more information on the group&apos;s activities see: http://www.w3.org/2005/Incubator/ssn/</rdfs:comment>
        <dc:rights>Copyright 2009 - 2011 W3C.</dc:rights>
        <terms:contributor>
            <rdf:Description>
                <foaf:mbox>antonio.maccioni@agid.gov.it</foaf:mbox>
                <foaf:name>Antonio Maccioni</foaf:name>
            </rdf:Description>
        </terms:contributor>
        <terms:contributor>
            <rdf:Description>
                <foaf:name>Olga Ximena Giraldo</foaf:name>
                <foaf:mbox>ogiraldo@fi.upm.es</foaf:mbox>
            </rdf:Description>
        </terms:contributor>
        <terms:contributor>
            <rdf:Description>
                <foaf:name>María Poveda Villalón</foaf:name>
                <foaf:mbox>mpoveda@fi.upm.es</foaf:mbox>
            </rdf:Description>
        </terms:contributor>
        <terms:created>2009-12-02</terms:created>
        <terms:modified rdf:datatype="http://www.w3.org/2001/XMLSchema#date">2014-01-25</terms:modified>
        <terms:modified rdf:datatype="http://www.w3.org/2001/XMLSchema#date">2013-12-16</terms:modified>
        <terms:contributor>
            <rdf:Description>
                <foaf:name>Giorgia Lodi</foaf:name>
                <foaf:mbox>giorgia.lodi@agid.gov.it</foaf:mbox>
            </rdf:Description>
        </terms:contributor>
        <terms:contributor>
            <rdf:Description>
                <foaf:name>Dominique Guardiola</foaf:name>
                <foaf:mbox>dguardiola@quinode.fr</foaf:mbox>
            </rdf:Description>
        </terms:contributor>
        <terms:modified rdf:datatype="http://www.w3.org/2001/XMLSchema#date">2013-02-15</terms:modified>
        <owl:versionInfo>0.4.0</owl:versionInfo>
        <rdfs:comment rdf:datatype="http://www.w3.org/2001/XMLSchema#string"> Please report any errors to the Semantic Sensor Network Incubator Activity via the public W3C list public-xg-ssn@w3.org</rdfs:comment>
        <dc:title>Semantic Sensor Network Ontology</dc:title>
        <rdfs:seeAlso>http://www.w3.org/2005/Incubator/ssn/</rdfs:seeAlso>
        <terms:title xml:lang="en">Core organization ontology</terms:title>
        <owl:versionInfo>0.4.1</owl:versionInfo>
        <terms:contributor rdf:resource="mailto:chris.little@metoffice.gov.uk"/>
        <dc:author rdf:datatype="http://www.w3.org/2001/XMLSchema#string">Sebastian Bader</dc:author>
        <terms:title xml:lang="it">Ontologia delle organizzazioni</terms:title>
        <skos:changeNote>2016-12-20 - adjust range of time:timeZone to time:TimeZone, moved up from the tzont ontology.  </skos:changeNote>
        <ns1:license rdf:resource="http://www.w3.org/Consortium/Legal/2002/copyright-software-20021231.html"/>
        <vaem:revisionNumber rdf:datatype="http://www.w3.org/2001/XMLSchema#string">0.4.1</vaem:revisionNumber>
        <terms:modified rdf:datatype="http://www.w3.org/2001/XMLSchema#date">2014-04-12</terms:modified>
        <terms:contributor>
            <rdf:Description>
                <foaf:name>Shuji Kamitsuna</foaf:name>
                <foaf:homepage rdf:resource="http://www.asahi-net.or.jp/~ax2s-kmtn/"/>
            </rdf:Description>
        </terms:contributor>
        <rdfs:seeAlso rdf:resource="http://www.semantic-web-journal.net/content/time-ontology-extended-non-gregorian-calendar-applications"/>
        <skos:changeNote>2017-04-06 - hasTime, hasXSDDuration added; Number removed; all duration elements changed to xsd:decimal</skos:changeNote>
    </owl:Ontology>
    


    <!-- 
    ///////////////////////////////////////////////////////////////////////////////////////
    //
    // Annotation properties
    //
    ///////////////////////////////////////////////////////////////////////////////////////
     -->

    


    <!-- http://creativecommons.org/ns#license -->

    <owl:AnnotationProperty rdf:about="http://creativecommons.org/ns#license"/>
    


    <!-- http://iirds.tekom.de/iirds#Description -->

    <owl:AnnotationProperty rdf:about="http://iirds.tekom.de/iirds#Description">
        <rdfs:subPropertyOf rdf:resource="http://purl.org/dc/terms/description"/>
        <rdfs:range rdf:resource="http://www.w3.org/2001/XMLSchema#string"/>
        <rdfs:domain rdf:resource="http://iirds.tekom.de/iirds#iirdsDomainEntitiy"/>
    </owl:AnnotationProperty>
    


    <!-- http://iirds.tekom.de/iirds#Format -->

    <owl:AnnotationProperty rdf:about="http://iirds.tekom.de/iirds#Format">
        <rdfs:subPropertyOf rdf:resource="http://purl.org/dc/terms/format"/>
        <rdfs:range rdf:resource="http://www.w3.org/2001/XMLSchema#string"/>
        <rdfs:domain rdf:resource="http://iirds.tekom.de/iirds#InformationUnit"/>
    </owl:AnnotationProperty>
    


    <!-- http://iirds.tekom.de/iirds#Identifier -->

    <owl:AnnotationProperty rdf:about="http://iirds.tekom.de/iirds#Identifier">
        <rdfs:subPropertyOf rdf:resource="http://purl.org/dc/terms/identifier"/>
        <rdfs:range rdf:resource="http://www.w3.org/2001/XMLSchema#string"/>
        <rdfs:domain rdf:resource="http://iirds.tekom.de/iirds#InformationUnit"/>
    </owl:AnnotationProperty>
    


    <!-- http://iirds.tekom.de/iirds#Language -->

    <owl:AnnotationProperty rdf:about="http://iirds.tekom.de/iirds#Language">
        <rdfs:subPropertyOf rdf:resource="http://purl.org/dc/terms/language"/>
        <rdfs:range rdf:resource="http://www.w3.org/2001/XMLSchema#string"/>
        <rdfs:domain rdf:resource="http://iirds.tekom.de/iirds#InformationUnit"/>
    </owl:AnnotationProperty>
    


    <!-- http://iirds.tekom.de/iirds#Title -->

    <owl:AnnotationProperty rdf:about="http://iirds.tekom.de/iirds#Title">
        <rdfs:subPropertyOf rdf:resource="http://purl.org/dc/terms/title"/>
        <rdfs:range rdf:resource="http://www.w3.org/2001/XMLSchema#string"/>
        <rdfs:domain rdf:resource="http://iirds.tekom.de/iirds#InformationUnit"/>
    </owl:AnnotationProperty>
    


    <!-- http://iirds.tekom.de/iirds#has-author -->

    <owl:AnnotationProperty rdf:about="http://iirds.tekom.de/iirds#has-author">
        <rdfs:subPropertyOf rdf:resource="http://purl.org/dc/terms/creator"/>
        <rdfs:range rdf:resource="http://iirds.tekom.de/iirds#Agent"/>
    </owl:AnnotationProperty>
    


    <!-- http://iirds.tekom.de/iirds#has-contributor -->

    <owl:AnnotationProperty rdf:about="http://iirds.tekom.de/iirds#has-contributor">
        <rdfs:subPropertyOf rdf:resource="http://purl.org/dc/terms/contributor"/>
        <rdfs:range rdf:resource="http://iirds.tekom.de/iirds#Agent"/>
    </owl:AnnotationProperty>
    


    <!-- http://iirds.tekom.de/iirds#has-subject -->

    <owl:AnnotationProperty rdf:about="http://iirds.tekom.de/iirds#has-subject">
        <rdfs:subPropertyOf rdf:resource="http://purl.org/dc/terms/subject"/>
        <rdfs:range rdf:resource="http://iirds.tekom.de/iirds#InformationSubject"/>
    </owl:AnnotationProperty>
    


    <!-- http://iirds.tekom.de/iirds#has-version -->

    <owl:AnnotationProperty rdf:about="http://iirds.tekom.de/iirds#has-version">
        <rdfs:subPropertyOf rdf:resource="http://purl.org/dc/terms/hasVersion"/>
        <rdfs:range rdf:resource="http://iirds.tekom.de/iirds#InformationUnit"/>
    </owl:AnnotationProperty>
    


    <!-- http://iirds.tekom.de/iirds#is-version-of -->

    <owl:AnnotationProperty rdf:about="http://iirds.tekom.de/iirds#is-version-of">
        <rdfs:subPropertyOf rdf:resource="http://purl.org/dc/terms/isVersionOf"/>
        <rdfs:range rdf:resource="http://iirds.tekom.de/iirds#InformationUnit"/>
    </owl:AnnotationProperty>
    


    <!-- http://people.aifb.kit.edu/mu2771/step#hasExpertise -->

    <owl:AnnotationProperty rdf:about="http://people.aifb.kit.edu/mu2771/step#hasExpertise">
        <rdfs:range rdf:resource="http://people.aifb.kit.edu/mu2771/step#Expertise"/>
    </owl:AnnotationProperty>
    


    <!-- http://people.aifb.kit.edu/mu2771/step#sourceUri -->

    <owl:AnnotationProperty rdf:about="http://people.aifb.kit.edu/mu2771/step#sourceUri"/>
    


    <!-- http://purl.org/dc/elements/1.1/creator -->

    <owl:AnnotationProperty rdf:about="http://purl.org/dc/elements/1.1/creator"/>
    


    <!-- http://purl.org/dc/elements/1.1/date -->

    <owl:AnnotationProperty rdf:about="http://purl.org/dc/elements/1.1/date"/>
    


    <!-- http://purl.org/dc/elements/1.1/description -->

    <owl:AnnotationProperty rdf:about="http://purl.org/dc/elements/1.1/description"/>
    


    <!-- http://purl.org/dc/elements/1.1/identifier -->

    <owl:AnnotationProperty rdf:about="http://purl.org/dc/elements/1.1/identifier"/>
    


    <!-- http://purl.org/dc/elements/1.1/rights -->

    <owl:AnnotationProperty rdf:about="http://purl.org/dc/elements/1.1/rights"/>
    


    <!-- http://purl.org/dc/elements/1.1/source -->

    <owl:AnnotationProperty rdf:about="http://purl.org/dc/elements/1.1/source"/>
    


    <!-- http://purl.org/dc/elements/1.1/subject -->

    <rdf:Description rdf:about="http://purl.org/dc/elements/1.1/subject">
        <rdfs:range rdf:resource="http://people.aifb.kit.edu/mu2771/step#FinishedWorkOrder"/>
    </rdf:Description>
    


    <!-- http://purl.org/dc/elements/1.1/title -->

    <owl:AnnotationProperty rdf:about="http://purl.org/dc/elements/1.1/title"/>
    


    <!-- http://purl.org/dc/terms/contributor -->

    <owl:AnnotationProperty rdf:about="http://purl.org/dc/terms/contributor"/>
    


    <!-- http://purl.org/dc/terms/created -->

    <owl:AnnotationProperty rdf:about="http://purl.org/dc/terms/created"/>
    


    <!-- http://purl.org/dc/terms/creator -->

    <owl:AnnotationProperty rdf:about="http://purl.org/dc/terms/creator"/>
    


    <!-- http://purl.org/dc/terms/description -->

    <owl:AnnotationProperty rdf:about="http://purl.org/dc/terms/description"/>
    


    <!-- http://purl.org/dc/terms/format -->

    <owl:AnnotationProperty rdf:about="http://purl.org/dc/terms/format"/>
    


    <!-- http://purl.org/dc/terms/hasVersion -->

    <owl:AnnotationProperty rdf:about="http://purl.org/dc/terms/hasVersion"/>
    


    <!-- http://purl.org/dc/terms/identifier -->

    <owl:AnnotationProperty rdf:about="http://purl.org/dc/terms/identifier"/>
    


    <!-- http://purl.org/dc/terms/isVersionOf -->

    <owl:AnnotationProperty rdf:about="http://purl.org/dc/terms/isVersionOf"/>
    


    <!-- http://purl.org/dc/terms/language -->

    <owl:AnnotationProperty rdf:about="http://purl.org/dc/terms/language"/>
    


    <!-- http://purl.org/dc/terms/modified -->

    <owl:AnnotationProperty rdf:about="http://purl.org/dc/terms/modified"/>
    


    <!-- http://purl.org/dc/terms/subject -->

    <owl:AnnotationProperty rdf:about="http://purl.org/dc/terms/subject"/>
    


    <!-- http://purl.org/dc/terms/title -->

    <owl:AnnotationProperty rdf:about="http://purl.org/dc/terms/title"/>
    


    <!-- http://www.example.org/subClassOfInverted -->

    <owl:AnnotationProperty rdf:about="http://www.example.org/subClassOfInverted"/>
    


    <!-- http://www.w3.org/2000/01/rdf-schema#comment -->

    <owl:AnnotationProperty rdf:about="http://www.w3.org/2000/01/rdf-schema#comment"/>
    


    <!-- http://www.w3.org/2000/01/rdf-schema#isDefinedBy -->

    <owl:AnnotationProperty rdf:about="http://www.w3.org/2000/01/rdf-schema#isDefinedBy"/>
    


    <!-- http://www.w3.org/2000/01/rdf-schema#label -->

    <owl:AnnotationProperty rdf:about="http://www.w3.org/2000/01/rdf-schema#label"/>
    


    <!-- http://www.w3.org/2000/01/rdf-schema#seeAlso -->

    <owl:AnnotationProperty rdf:about="http://www.w3.org/2000/01/rdf-schema#seeAlso"/>
    


    <!-- http://www.w3.org/2001/XMLSchema#pattern -->

    <owl:AnnotationProperty rdf:about="http://www.w3.org/2001/XMLSchema#pattern"/>
    


    <!-- http://www.w3.org/2002/07/owl#minQualifiedCardinality -->

    <owl:AnnotationProperty rdf:about="http://www.w3.org/2002/07/owl#minQualifiedCardinality"/>
    


    <!-- http://www.w3.org/2003/01/geo/wgs84_pos#alt -->

    <owl:AnnotationProperty rdf:about="http://www.w3.org/2003/01/geo/wgs84_pos#alt">
        <rdfs:comment>The WGS84 altitude of a SpatialThing (decimal meters 
above the local reference ellipsoid).</rdfs:comment>
        <rdfs:label>altitude</rdfs:label>
        <rdfs:domain rdf:resource="http://www.w3.org/2003/01/geo/wgs84_pos#SpatialThing"/>
    </owl:AnnotationProperty>
    


    <!-- http://www.w3.org/2003/01/geo/wgs84_pos#lat -->

    <owl:AnnotationProperty rdf:about="http://www.w3.org/2003/01/geo/wgs84_pos#lat">
        <rdfs:comment>The WGS84 latitude of a SpatialThing (decimal degrees).</rdfs:comment>
        <rdfs:label>latitude</rdfs:label>
        <rdfs:domain rdf:resource="http://www.w3.org/2003/01/geo/wgs84_pos#SpatialThing"/>
    </owl:AnnotationProperty>
    


    <!-- http://www.w3.org/2003/01/geo/wgs84_pos#long -->

    <owl:AnnotationProperty rdf:about="http://www.w3.org/2003/01/geo/wgs84_pos#long">
        <rdfs:comment>The WGS84 longitude of a SpatialThing (decimal degrees).</rdfs:comment>
        <rdfs:label>longitude</rdfs:label>
        <rdfs:domain rdf:resource="http://www.w3.org/2003/01/geo/wgs84_pos#SpatialThing"/>
    </owl:AnnotationProperty>
    


    <!-- http://www.w3.org/2003/06/sw-vocab-status/ns#term_status -->

    <owl:AnnotationProperty rdf:about="http://www.w3.org/2003/06/sw-vocab-status/ns#term_status"/>
    


    <!-- http://www.w3.org/2004/02/skos/core#changeNote -->

    <owl:AnnotationProperty rdf:about="http://www.w3.org/2004/02/skos/core#changeNote"/>
    


    <!-- http://www.w3.org/2004/02/skos/core#definition -->

    <owl:AnnotationProperty rdf:about="http://www.w3.org/2004/02/skos/core#definition"/>
    


    <!-- http://www.w3.org/2004/02/skos/core#editorialNote -->

    <owl:AnnotationProperty rdf:about="http://www.w3.org/2004/02/skos/core#editorialNote"/>
    


    <!-- http://www.w3.org/2004/02/skos/core#historyNote -->

    <owl:AnnotationProperty rdf:about="http://www.w3.org/2004/02/skos/core#historyNote"/>
    


    <!-- http://www.w3.org/2004/02/skos/core#note -->

    <owl:AnnotationProperty rdf:about="http://www.w3.org/2004/02/skos/core#note"/>
    


    <!-- http://www.w3.org/2004/02/skos/core#prefLabel -->

    <owl:AnnotationProperty rdf:about="http://www.w3.org/2004/02/skos/core#prefLabel"/>
    


    <!-- http://www.w3.org/2004/02/skos/core#scopeNote -->

    <owl:AnnotationProperty rdf:about="http://www.w3.org/2004/02/skos/core#scopeNote"/>
    


    <!-- http://www.w3.org/ns/org#purpose -->

    <owl:AnnotationProperty rdf:about="http://www.w3.org/ns/org#purpose">
        <rdfs:comment xml:lang="es">Finalidad u objetivo de la organización. La organización puede tener muchos objetivos a diferentes niveles de abstracción, pero en la naturaleza de las organizaciones está el tener una razón para existir, y la finalidad de esta propiedad es documentar dicha razón. La organización podrá tener más de un objetivo. Se recomienda el uso de vocabularios controlados o listas de códigos para indicar el objetivo, preferentemente mediante el uso de un `skos:Concept`. Sin embargo, el rango no está predeterminado, de forma que otros tipos de esquemas descriptivos tiene cabida. Se espera que ciertas especializaciones de este vocabulario o ciertos perfiles de aplicaciones restrinjan el rango del objetivo. Denominaciones alternativas: área_ _jurisdicción_ _ responsabilidad _ (especialmente cuando se aplica a unidades tales como ministerios o divisiones administrativas de los gobiernos)</rdfs:comment>
        <rdfs:comment xml:lang="it">Indica l&apos;obiettivo di questa Organization. In generale, si possono esprimere gli obiettivi di un&apos;organizzazione secondo diversi livelli di astrazione, ma la natura stessa dell&apos;organizzazione ha una ragione d&apos;essere ed è proprio questa che deve essere catturata con tale proprietà. Inoltre, un&apos;Organization può avere obiettivi multipli. È raccomandabile che l&apos;obiettivo faccia parte di una code list, e che sia preferibilmente un `skos:Concept`. Ad ogni modo, il codominio della proprietà è lasciato aperto per consentire altri tipi di di descrizione. Conseguentemente, eventuali specializzazioni o profili applicativi possono utilizzare quel vocabolario come codominio della proprietà.</rdfs:comment>
        <rdfs:comment xml:lang="en">Indicates the purpose of this Organization. There can be many purposes at different levels of abstraction but the nature of an organization is to have a reason for existence and this property is a means to document that reason. An Organization may have multiple purposes. It is recommended that the purpose be denoted by a controlled term or code list, ideally a `skos:Concept`. However, the range is left open to allow for other types of descriptive schemes. It is expected that specializations or application profiles of this vocabulary will constrain the range of the purpose. Alternative names: _remit_ _responsibility_ (esp. if applied to OrganizationalUnits such as Government Departments).</rdfs:comment>
        <rdfs:comment xml:lang="fr">Indique le but de cette Organisation. Il peut exister plusieurs buts à différents niveaux d&apos;abstraction mais la nature d&apos;une organisation est d&apos;avoir une raison d&apos;exister et cette propriété doit servir à documenter cette raison d&apos;être. Une Organisation peut avoir plusieurs Buts. Il est recommandé que le but soit libellé à l&apos;aide d&apos;un vocabulaire contrôlé ou autre code établi, idéalement avec un concept `skos:Concept`. Toutefois, le champ de cette propriété est laissé ouvert et pourrait accepter d&apos;autres schémas de description. Il est préférable que les spécialisations ou les profils d&apos;applications de ce vocabulaire contraignent le champ de cette propriété.</rdfs:comment>
        <rdfs:comment xml:lang="ja">この組織の目的を示します。異なる抽象レベルの多くの目的がありえますが、組織の本質は存在理由を持つことであり、このプロパティーはその理由をドキュメント化する手段です。組織は、複数の目的を持っている可能性があります。</rdfs:comment>
        <rdfs:isDefinedBy rdf:resource="http://www.w3.org/ns/org"/>
        <rdfs:label xml:lang="fr">but</rdfs:label>
        <rdfs:label xml:lang="it">obiettivo</rdfs:label>
        <rdfs:label xml:lang="en">purpose</rdfs:label>
        <rdfs:label xml:lang="es">tiene objetivo</rdfs:label>
        <rdfs:domain rdf:resource="http://www.w3.org/ns/org#Organization"/>
    </owl:AnnotationProperty>
    


    <!-- http://www.w3.org/ns/org#roleProperty -->

    <owl:AnnotationProperty rdf:about="http://www.w3.org/ns/org#roleProperty">
        <rdfs:comment xml:lang="fr">Ceci est une méta-propriété utilisée pour annoter une instance de `org:Role` ayant une sous-propriété `org:memberOf` qui peut être utilisée pour indiquer directement le rôle et pouvoir faire des requêtes plus facilement. La sémantique visée est un Engagement impliquant l&apos;existence d&apos;une relation de propriété directe à travers d&apos;une règle d&apos;inférence de la forme:  `{ [] org:member ?p; org:organization ?o; org:role [org:roleProperty ?r] } -&gt; {?p ?r ?o}`.</rdfs:comment>
        <rdfs:comment xml:lang="es">Meta-propiedad que se utiliza para anotar una instancia de `org:Role` con una sub-propiedad de `org:memberOf`, que puede ser utilizada para indicar directamente la actividad a fin de facilitar las consultas a los datos. The intended semantics is that a Membership relation involving the Role implies the existence of a direct property relationship through an inference rule of the form: { [] org:member ?a; org:organization ?o; org:role [org:roleProperty ?r] } -&gt; {?a ?r ?o}</rdfs:comment>
        <rdfs:comment xml:lang="it">Questa è una meta-proprietà usata per annotare un&apos;istanza di `org:Role` con una sotto-proprietà di `org:memberOf` e può essere usata per indicare direttamente il ruolo per facilitare un&apos;interrogazione sui dati.</rdfs:comment>
        <rdfs:comment xml:lang="en">This is a metalevel property which is used to annotate an `org:Role` instance with a sub-property of `org:memberOf` that can be used to directly indicate the role for easy of query. The intended semantics is a Membership relation involving the Role implies the existence of a direct property relationship through an inference rule of the form:  `{ [] org:member ?p; org:organization ?o; org:role [org:roleProperty ?r] } -&gt; {?p ?r ?o}`.</rdfs:comment>
        <rdfs:comment xml:lang="ja">これは、クエリが容易になるように役割を直接的に示すために使用できるorg:memberOfのサブプロパティーでorg:Roleインスタンスを注釈するために用いられるメタレベルのプロパティーです。</rdfs:comment>
        <rdfs:isDefinedBy rdf:resource="http://www.w3.org/ns/org"/>
        <rdfs:label xml:lang="es">desempeña la actividad de (propiedad)</rdfs:label>
        <rdfs:label xml:lang="en">role (property)</rdfs:label>
        <rdfs:label xml:lang="it">ruolo (proprietà)</rdfs:label>
        <rdfs:label xml:lang="fr">rôle (propriété)</rdfs:label>
        <rdfs:range rdf:resource="http://www.w3.org/1999/02/22-rdf-syntax-ns#Property"/>
        <rdfs:domain rdf:resource="http://www.w3.org/ns/org#Role"/>
    </owl:AnnotationProperty>
    


    <!-- http://xmlns.com/foaf/0.1/homepage -->

    <owl:AnnotationProperty rdf:about="http://xmlns.com/foaf/0.1/homepage"/>
    


    <!-- http://xmlns.com/foaf/0.1/mbox -->

    <owl:AnnotationProperty rdf:about="http://xmlns.com/foaf/0.1/mbox"/>
    


    <!-- http://xmlns.com/foaf/0.1/name -->

    <owl:AnnotationProperty rdf:about="http://xmlns.com/foaf/0.1/name"/>
    


    <!-- https://www.w3.org/2001/sw/BestPractices/OEP/SimplePartWhole/part.owl#partOf -->

    <owl:AnnotationProperty rdf:about="https://www.w3.org/2001/sw/BestPractices/OEP/SimplePartWhole/part.owl#partOf"/>
    


    <!-- 
    ///////////////////////////////////////////////////////////////////////////////////////
    //
    // Datatypes
    //
    ///////////////////////////////////////////////////////////////////////////////////////
     -->

    


    <!-- http://www.w3.org/2001/XMLSchema#date -->

    <rdfs:Datatype rdf:about="http://www.w3.org/2001/XMLSchema#date"/>
    


    <!-- http://www.w3.org/2001/XMLSchema#dateTimeStamp -->

    <rdfs:Datatype rdf:about="http://www.w3.org/2001/XMLSchema#dateTimeStamp"/>
    


    <!-- http://www.w3.org/2001/XMLSchema#duration -->

    <rdfs:Datatype rdf:about="http://www.w3.org/2001/XMLSchema#duration"/>
    


    <!-- http://www.w3.org/2001/XMLSchema#gDay -->

    <rdfs:Datatype rdf:about="http://www.w3.org/2001/XMLSchema#gDay"/>
    


    <!-- http://www.w3.org/2001/XMLSchema#gMonth -->

    <rdfs:Datatype rdf:about="http://www.w3.org/2001/XMLSchema#gMonth"/>
    


    <!-- http://www.w3.org/2001/XMLSchema#gYear -->

    <rdfs:Datatype rdf:about="http://www.w3.org/2001/XMLSchema#gYear"/>
    


    <!-- http://www.w3.org/2001/XMLSchema#gYearMonth -->

    <rdfs:Datatype rdf:about="http://www.w3.org/2001/XMLSchema#gYearMonth"/>
    


    <!-- http://www.w3.org/2006/time#generalDay -->

    <rdfs:Datatype rdf:about="http://www.w3.org/2006/time#generalDay">
        <rdfs:comment xml:lang="en">Day of month - formulated as a text string with a pattern constraint to reproduce the same lexical form as gDay, except that values up to 99 are permitted, in order to support calendars with more than 31 days in a month. 
Note that the value-space is not defined, so a generic OWL2 processor cannot compute ordering relationships of values of this type.</rdfs:comment>
        <rdfs:label xml:lang="en">Generalized day</rdfs:label>
        <skos:definition xml:lang="en">Day of month - generalization of xsd:gDay, formulated as a text string with a pattern constraint to reproduce the same lexical form as gDay, except that values up to 99 are permitted, in order to support calendars with more than 31 days in a month. Note that the value-space is not defined, so a generic OWL2 processor cannot compute ordering relationships of values of this type. </skos:definition>
    </rdfs:Datatype>
    


    <!-- http://www.w3.org/2006/time#generalMonth -->

    <rdfs:Datatype rdf:about="http://www.w3.org/2006/time#generalMonth">
        <rdfs:comment xml:lang="en">Month of year - formulated as a text string with a pattern constraint to reproduce the same lexical form as gMonth, except that values up to 20 are permitted, in order to support calendars with more than 12 months in the year. 
Note that the value-space is not defined, so a generic OWL2 processor cannot compute ordering relationships of values of this type.</rdfs:comment>
        <rdfs:label xml:lang="en">Generalized month</rdfs:label>
        <skos:definition xml:lang="en">Month of year - generalization of xsd:gMonth, formulated as a text string with a pattern constraint to reproduce the same lexical form as gMonth, except that values up to 20 are permitted, in order to support calendars with more than 12 months in the year. Note that the value-space is not defined, so a generic OWL2 processor cannot compute ordering relationships of values of this type.</skos:definition>
    </rdfs:Datatype>
    


    <!-- http://www.w3.org/2006/time#generalYear -->

    <rdfs:Datatype rdf:about="http://www.w3.org/2006/time#generalYear"/>
    


    <!-- 
    ///////////////////////////////////////////////////////////////////////////////////////
    //
    // Object Properties
    //
    ///////////////////////////////////////////////////////////////////////////////////////
     -->

    


    <!-- _:genid-nodeid-genid-56a1b575ea1846ca84ca3b4cd567a37b-35ACB39B2C79FA9E1693206D302A5EC5 -->

    <owl:ObjectProperty rdf:about="_:genid-nodeid-genid-56a1b575ea1846ca84ca3b4cd567a37b-35ACB39B2C79FA9E1693206D302A5EC5"/>
    <rdf:Description>
        <owl:inverseOf rdf:resource="_:genid-nodeid-genid-56a1b575ea1846ca84ca3b4cd567a37b-35ACB39B2C79FA9E1693206D302A5EC5"/>
        <rdfs:range rdf:resource="http://www.w3.org/ns/org#Role"/>
    </rdf:Description>
    


    <!-- _:genid-nodeid-genid-56a1b575ea1846ca84ca3b4cd567a37b-3D9DAF7E819508C71FC07ED589F0B633 -->

    <owl:ObjectProperty rdf:about="_:genid-nodeid-genid-56a1b575ea1846ca84ca3b4cd567a37b-3D9DAF7E819508C71FC07ED589F0B633"/>
    <rdf:Description>
        <owl:inverseOf rdf:resource="_:genid-nodeid-genid-56a1b575ea1846ca84ca3b4cd567a37b-3D9DAF7E819508C71FC07ED589F0B633"/>
        <rdfs:range rdf:resource="http://www.w3.org/2006/time#TemporalUnit"/>
    </rdf:Description>
    


    <!-- _:genid-nodeid-genid-56a1b575ea1846ca84ca3b4cd567a37b-71DDAF06A1F28B2C32CCCB12BF968504 -->

    <owl:ObjectProperty rdf:about="_:genid-nodeid-genid-56a1b575ea1846ca84ca3b4cd567a37b-71DDAF06A1F28B2C32CCCB12BF968504"/>
    <rdf:Description>
        <owl:inverseOf rdf:resource="_:genid-nodeid-genid-56a1b575ea1846ca84ca3b4cd567a37b-71DDAF06A1F28B2C32CCCB12BF968504"/>
        <rdfs:range rdf:resource="http://www.w3.org/2006/time#TRS"/>
    </rdf:Description>
    


    <!-- _:genid-nodeid-genid-56a1b575ea1846ca84ca3b4cd567a37b-DA4F9AF98DB66B9E75D81CF27322D435 -->

    <owl:ObjectProperty rdf:about="_:genid-nodeid-genid-56a1b575ea1846ca84ca3b4cd567a37b-DA4F9AF98DB66B9E75D81CF27322D435"/>
    <rdf:Description>
        <owl:inverseOf rdf:resource="_:genid-nodeid-genid-56a1b575ea1846ca84ca3b4cd567a37b-DA4F9AF98DB66B9E75D81CF27322D435"/>
        <rdfs:range>
            <owl:Class>
                <owl:unionOf rdf:parseType="Collection">
                    <rdf:Description rdf:about="http://www.w3.org/ns/org#Post"/>
                    <rdf:Description rdf:about="http://xmlns.com/foaf/0.1/Agent"/>
                </owl:unionOf>
            </owl:Class>
        </rdfs:range>
    </rdf:Description>
    


    <!-- http://iirds.tekom.de/iirds#has-author -->

    <owl:ObjectProperty rdf:about="http://iirds.tekom.de/iirds#has-author">
        <rdfs:subPropertyOf rdf:resource="http://iirds.tekom.de/iirds#iirdsRelationConcept"/>
        <rdfs:domain rdf:resource="http://iirds.tekom.de/iirds#InformationUnit"/>
    </owl:ObjectProperty>
    


    <!-- http://iirds.tekom.de/iirds#has-contributor -->

    <owl:ObjectProperty rdf:about="http://iirds.tekom.de/iirds#has-contributor">
        <rdfs:subPropertyOf rdf:resource="http://iirds.tekom.de/iirds#iirdsRelationConcept"/>
        <rdfs:domain rdf:resource="http://iirds.tekom.de/iirds#InformationUnit"/>
    </owl:ObjectProperty>
    


    <!-- http://iirds.tekom.de/iirds#has-document-type -->

    <owl:ObjectProperty rdf:about="http://iirds.tekom.de/iirds#has-document-type">
        <rdfs:subPropertyOf rdf:resource="http://iirds.tekom.de/iirds#has-information-type"/>
        <rdfs:domain rdf:resource="http://iirds.tekom.de/iirds#Document"/>
        <rdfs:range rdf:resource="http://iirds.tekom.de/iirds#DocumentType"/>
    </owl:ObjectProperty>
    


    <!-- http://iirds.tekom.de/iirds#has-first-child -->

    <owl:ObjectProperty rdf:about="http://iirds.tekom.de/iirds#has-first-child">
        <rdfs:subPropertyOf rdf:resource="http://iirds.tekom.de/iirds#iirdsRelationConcept"/>
        <rdfs:domain rdf:resource="http://iirds.tekom.de/iirds#DirectoryNode"/>
        <rdfs:range rdf:resource="http://iirds.tekom.de/iirds#DirectoryNode"/>
        <rdfs:label xml:lang="en">has first child</rdfs:label>
        <rdfs:label xml:lang="de">hat als erstes Kindelement</rdfs:label>
    </owl:ObjectProperty>
    


    <!-- http://iirds.tekom.de/iirds#has-information-type -->

    <owl:ObjectProperty rdf:about="http://iirds.tekom.de/iirds#has-information-type">
        <rdfs:subPropertyOf rdf:resource="http://iirds.tekom.de/iirds#iirdsRelationConcept"/>
        <rdfs:domain rdf:resource="http://iirds.tekom.de/iirds#InformationUnit"/>
        <rdfs:range rdf:resource="http://iirds.tekom.de/iirds#InformationType"/>
    </owl:ObjectProperty>
    


    <!-- http://iirds.tekom.de/iirds#has-next-sibling -->

    <owl:ObjectProperty rdf:about="http://iirds.tekom.de/iirds#has-next-sibling">
        <rdfs:subPropertyOf rdf:resource="http://iirds.tekom.de/iirds#iirdsRelationConcept"/>
        <rdfs:domain rdf:resource="http://iirds.tekom.de/iirds#DirectoryNode"/>
        <rdfs:range rdf:resource="http://iirds.tekom.de/iirds#DirectoryNode"/>
        <rdfs:label xml:lang="en">has next sibling</rdfs:label>
        <rdfs:label xml:lang="de">hat als nächstes Element</rdfs:label>
    </owl:ObjectProperty>
    


    <!-- http://iirds.tekom.de/iirds#has-subject -->

    <owl:ObjectProperty rdf:about="http://iirds.tekom.de/iirds#has-subject">
        <rdfs:subPropertyOf rdf:resource="http://iirds.tekom.de/iirds#iirdsRelationConcept"/>
        <rdfs:domain rdf:resource="http://iirds.tekom.de/iirds#InformationUnit"/>
    </owl:ObjectProperty>
    


    <!-- http://iirds.tekom.de/iirds#has-topic-type -->

    <owl:ObjectProperty rdf:about="http://iirds.tekom.de/iirds#has-topic-type">
        <rdfs:subPropertyOf rdf:resource="http://iirds.tekom.de/iirds#has-information-type"/>
        <rdfs:domain rdf:resource="http://iirds.tekom.de/iirds#InformationUnit"/>
        <rdfs:range rdf:resource="http://iirds.tekom.de/iirds#TopicType"/>
    </owl:ObjectProperty>
    


    <!-- http://iirds.tekom.de/iirds#has-version -->

    <owl:ObjectProperty rdf:about="http://iirds.tekom.de/iirds#has-version">
        <rdfs:subPropertyOf rdf:resource="http://iirds.tekom.de/iirds#iirdsRelationConcept"/>
        <rdfs:domain rdf:resource="http://iirds.tekom.de/iirds#InformationUnit"/>
    </owl:ObjectProperty>
    


    <!-- http://iirds.tekom.de/iirds#iirdsRelationConcept -->

    <owl:ObjectProperty rdf:about="http://iirds.tekom.de/iirds#iirdsRelationConcept">
        <rdfs:domain rdf:resource="http://iirds.tekom.de/iirds#iirdsDomainEntitiy"/>
        <rdfs:range rdf:resource="http://iirds.tekom.de/iirds#iirdsDomainEntitiy"/>
        <rdfs:label xml:lang="de">iirdsRelationConcept</rdfs:label>
    </owl:ObjectProperty>
    


    <!-- http://iirds.tekom.de/iirds#is-version-of -->

    <owl:ObjectProperty rdf:about="http://iirds.tekom.de/iirds#is-version-of">
        <rdfs:subPropertyOf rdf:resource="http://iirds.tekom.de/iirds#iirdsRelationConcept"/>
        <rdfs:domain rdf:resource="http://iirds.tekom.de/iirds#InformationUnit"/>
    </owl:ObjectProperty>
    


    <!-- http://iirds.tekom.de/iirds#references-information-unit -->

    <owl:ObjectProperty rdf:about="http://iirds.tekom.de/iirds#references-information-unit">
        <rdfs:subPropertyOf rdf:resource="http://iirds.tekom.de/iirds#iirdsRelationConcept"/>
        <rdfs:domain rdf:resource="http://iirds.tekom.de/iirds#DirectoryNode"/>
        <rdfs:range rdf:resource="http://iirds.tekom.de/iirds#InformationUnit"/>
        <rdfs:label xml:lang="en">references information unit</rdfs:label>
        <rdfs:label xml:lang="de">referenziert Informationseinheit</rdfs:label>
    </owl:ObjectProperty>
    


    <!-- http://iirds.tekom.de/iirds#relates-to -->

    <owl:ObjectProperty rdf:about="http://iirds.tekom.de/iirds#relates-to">
        <rdfs:subPropertyOf rdf:resource="http://iirds.tekom.de/iirds#iirdsRelationConcept"/>
        <rdfs:domain rdf:resource="http://iirds.tekom.de/iirds#InformationUnit"/>
        <rdfs:range rdf:resource="http://iirds.tekom.de/iirds#DocumentationMetadata"/>
        <rdfs:label xml:lang="de">bezieht sich auf</rdfs:label>
        <rdfs:label xml:lang="en">relates to</rdfs:label>
    </owl:ObjectProperty>
    


    <!-- http://iirds.tekom.de/iirds#relates-to-event -->

    <owl:ObjectProperty rdf:about="http://iirds.tekom.de/iirds#relates-to-event">
        <rdfs:subPropertyOf rdf:resource="http://iirds.tekom.de/iirds#relates-to"/>
        <rdfs:domain rdf:resource="http://iirds.tekom.de/iirds#InformationUnit"/>
        <rdfs:range rdf:resource="http://iirds.tekom.de/iirds#Event"/>
        <rdfs:label xml:lang="de">bezieht sich auf Ereignis</rdfs:label>
        <rdfs:label xml:lang="en">relates to event</rdfs:label>
    </owl:ObjectProperty>
    


    <!-- http://iirds.tekom.de/iirds#relates-to-product-metadata -->

    <owl:ObjectProperty rdf:about="http://iirds.tekom.de/iirds#relates-to-product-metadata">
        <rdfs:subPropertyOf rdf:resource="http://iirds.tekom.de/iirds#relates-to"/>
        <rdfs:domain rdf:resource="http://iirds.tekom.de/iirds#InformationUnit"/>
        <rdfs:range rdf:resource="http://iirds.tekom.de/iirds#ProductMetadata"/>
        <rdfs:label xml:lang="de">bezieht sich auf Produkt</rdfs:label>
        <rdfs:label xml:lang="en">relates to product metadata</rdfs:label>
    </owl:ObjectProperty>
    


    <!-- http://iirds.tekom.de/iirds#requires -->

    <owl:ObjectProperty rdf:about="http://iirds.tekom.de/iirds#requires">
        <rdfs:subPropertyOf rdf:resource="http://iirds.tekom.de/iirds#iirdsRelationConcept"/>
        <rdfs:domain rdf:resource="http://iirds.tekom.de/iirds#InformationUnit"/>
        <rdfs:range rdf:resource="http://iirds.tekom.de/iirds#FunctionalMetadata"/>
        <rdfs:label xml:lang="de">erfordert</rdfs:label>
        <rdfs:label xml:lang="en">requires</rdfs:label>
    </owl:ObjectProperty>
    


    <!-- http://iirds.tekom.de/iirds#requires-qualification -->

    <owl:ObjectProperty rdf:about="http://iirds.tekom.de/iirds#requires-qualification">
        <rdfs:subPropertyOf rdf:resource="http://iirds.tekom.de/iirds#requires"/>
        <rdfs:domain rdf:resource="http://iirds.tekom.de/iirds#InformationUnit"/>
        <rdfs:range rdf:resource="http://iirds.tekom.de/iirds#Qualification"/>
        <rdfs:label xml:lang="de">erfordert Qualifikation</rdfs:label>
        <rdfs:label xml:lang="en">requires qualification</rdfs:label>
    </owl:ObjectProperty>
    


    <!-- http://iirds.tekom.de/iirds#requires-supply -->

    <owl:ObjectProperty rdf:about="http://iirds.tekom.de/iirds#requires-supply">
        <rdfs:subPropertyOf rdf:resource="http://iirds.tekom.de/iirds#requires"/>
        <rdfs:domain rdf:resource="http://iirds.tekom.de/iirds#InformationUnit"/>
        <rdfs:range rdf:resource="http://iirds.tekom.de/iirds#Supplies"/>
        <rdfs:label xml:lang="de">erfordert Hilfsmittel</rdfs:label>
        <rdfs:label xml:lang="en">requires supply</rdfs:label>
    </owl:ObjectProperty>
    


    <!-- http://iirds.tekom.de/iirds#requires-time -->

    <owl:ObjectProperty rdf:about="http://iirds.tekom.de/iirds#requires-time">
        <rdfs:subPropertyOf rdf:resource="http://iirds.tekom.de/iirds#requires"/>
        <rdfs:domain rdf:resource="http://iirds.tekom.de/iirds#InformationUnit"/>
        <rdfs:range rdf:resource="http://iirds.tekom.de/iirds#PlanningTime"/>
        <rdfs:label xml:lang="de">erfordert Zeit</rdfs:label>
        <rdfs:label xml:lang="en">requires time</rdfs:label>
    </owl:ObjectProperty>
    


    <!-- http://people.aifb.kit.edu/mu2771/step#date -->

    <owl:ObjectProperty rdf:about="http://people.aifb.kit.edu/mu2771/step#date">
        <rdfs:range rdf:resource="http://www.w3.org/2006/time#TemporalEntity"/>
        <rdfs:comment xml:lang="en">indicates that something happened/happens/will happen at a specific time</rdfs:comment>
        <rdfs:label xml:lang="en">date</rdfs:label>
    </owl:ObjectProperty>
    


    <!-- http://people.aifb.kit.edu/mu2771/step#expertiseOfSystem -->

    <owl:ObjectProperty rdf:about="http://people.aifb.kit.edu/mu2771/step#expertiseOfSystem">
        <rdfs:label xml:lang="en">expertise of system</rdfs:label>
    </owl:ObjectProperty>
    


    <!-- http://people.aifb.kit.edu/mu2771/step#hasExpertise -->

    <owl:ObjectProperty rdf:about="http://people.aifb.kit.edu/mu2771/step#hasExpertise"/>
    


    <!-- http://people.aifb.kit.edu/mu2771/step#hasPrediction -->

    <owl:ObjectProperty rdf:about="http://people.aifb.kit.edu/mu2771/step#hasPrediction">
        <rdfs:domain rdf:resource="http://purl.oclc.org/NET/ssnx/ssn#System"/>
        <rdfs:range rdf:resource="http://people.aifb.kit.edu/mu2771/step#Prediction"/>
    </owl:ObjectProperty>
    


    <!-- http://people.aifb.kit.edu/mu2771/step#hasPriority -->

    <owl:ObjectProperty rdf:about="http://people.aifb.kit.edu/mu2771/step#hasPriority">
        <rdfs:range rdf:resource="http://people.aifb.kit.edu/mu2771/step#Priority"/>
        <rdfs:comment xml:lang="en">specifies the priority or importance of a specific task</rdfs:comment>
        <rdfs:label xml:lang="en">has priority</rdfs:label>
        <rdfs:label xml:lang="de">hat Priorität</rdfs:label>
    </owl:ObjectProperty>
    


    <!-- http://people.aifb.kit.edu/mu2771/step#hasRoute -->

    <owl:ObjectProperty rdf:about="http://people.aifb.kit.edu/mu2771/step#hasRoute">
        <owl:inverseOf rdf:resource="http://people.aifb.kit.edu/mu2771/step#hasWorkOrder"/>
        <rdfs:domain rdf:resource="http://people.aifb.kit.edu/mu2771/step#ScheduledWorkOrder"/>
        <rdfs:range rdf:resource="http://people.aifb.kit.edu/mu2771/step#Route"/>
        <rdfs:label xml:lang="en">has route</rdfs:label>
    </owl:ObjectProperty>
    


    <!-- http://people.aifb.kit.edu/mu2771/step#hasType -->

    <owl:ObjectProperty rdf:about="http://people.aifb.kit.edu/mu2771/step#hasType">
        <rdfs:domain rdf:resource="http://purl.oclc.org/NET/ssnx/ssn#System"/>
        <rdfs:label xml:lang="en">hasType</rdfs:label>
    </owl:ObjectProperty>
    


    <!-- http://people.aifb.kit.edu/mu2771/step#hasWorkOrder -->

    <owl:ObjectProperty rdf:about="http://people.aifb.kit.edu/mu2771/step#hasWorkOrder">
        <rdfs:domain rdf:resource="http://people.aifb.kit.edu/mu2771/step#Route"/>
        <rdfs:range rdf:resource="http://people.aifb.kit.edu/mu2771/step#WorkOrder"/>
        <rdfs:label xml:lang="en">has work order</rdfs:label>
    </owl:ObjectProperty>
    


    <!-- http://people.aifb.kit.edu/mu2771/step#hasWorktimeAt -->

    <owl:ObjectProperty rdf:about="http://people.aifb.kit.edu/mu2771/step#hasWorktimeAt">
        <rdfs:domain rdf:resource="http://xmlns.com/foaf/0.1/Person"/>
        <rdfs:range rdf:resource="http://aifb.kit.edu/stepC#SpatialTemporalEntity"/>
        <owl:propertyDisjointWith rdf:resource="http://people.aifb.kit.edu/mu2771/step#isAvailableAt"/>
        <rdfs:comment xml:lang="en">the general work time of a foaf:Person, its overall capacity</rdfs:comment>
        <rdfs:label xml:lang="en">has work time at</rdfs:label>
    </owl:ObjectProperty>
    


    <!-- http://people.aifb.kit.edu/mu2771/step#isAvailableAt -->

    <owl:ObjectProperty rdf:about="http://people.aifb.kit.edu/mu2771/step#isAvailableAt">
        <rdfs:domain rdf:resource="http://xmlns.com/foaf/0.1/Person"/>
        <rdfs:range rdf:resource="http://aifb.kit.edu/stepC#SpatialTemporalEntity"/>
        <rdfs:comment xml:lang="en">the time interval where the foaf:Person is not busy yet</rdfs:comment>
        <rdfs:label xml:lang="en">is available at</rdfs:label>
    </owl:ObjectProperty>
    


    <!-- http://people.aifb.kit.edu/mu2771/step#isBusyAt -->

    <owl:ObjectProperty rdf:about="http://people.aifb.kit.edu/mu2771/step#isBusyAt">
        <rdfs:domain rdf:resource="http://xmlns.com/foaf/0.1/Person"/>
        <rdfs:range rdf:resource="http://aifb.kit.edu/stepC#SpatialTemporalEntity"/>
        <rdfs:comment xml:lang="en">the time interval where the foaf:Person already has a task</rdfs:comment>
        <rdfs:label xml:lang="en">is busy at</rdfs:label>
    </owl:ObjectProperty>
    


    <!-- http://people.aifb.kit.edu/mu2771/step#isExecutedBy -->

    <owl:ObjectProperty rdf:about="http://people.aifb.kit.edu/mu2771/step#isExecutedBy">
        <rdfs:domain rdf:resource="http://people.aifb.kit.edu/mu2771/step#WorkOrder"/>
        <rdfs:range rdf:resource="http://people.aifb.kit.edu/mu2771/step#Technician"/>
        <rdfs:comment xml:lang="en">a step:Plan needs one or more step:Technicians to handle it </rdfs:comment>
        <rdfs:comment xml:lang="en">is executed by</rdfs:comment>
    </owl:ObjectProperty>
    


    <!-- http://people.aifb.kit.edu/mu2771/step#memberOf -->

    <owl:ObjectProperty rdf:about="http://people.aifb.kit.edu/mu2771/step#memberOf">
        <owl:equivalentProperty rdf:resource="http://www.w3.org/ns/org#memberOf"/>
        <rdfs:domain rdf:resource="http://xmlns.com/foaf/0.1/Agent"/>
        <rdfs:range rdf:resource="http://www.w3.org/ns/org#Organization"/>
    </owl:ObjectProperty>
    


    <!-- http://people.aifb.kit.edu/mu2771/step#relatedTo -->

    <owl:ObjectProperty rdf:about="http://people.aifb.kit.edu/mu2771/step#relatedTo">
        <rdfs:range rdf:resource="http://purl.oclc.org/NET/ssnx/ssn#System"/>
        <rdfs:comment xml:lang="en">specifies which ssn:System is trageted</rdfs:comment>
        <rdfs:label xml:lang="en">related to</rdfs:label>
    </owl:ObjectProperty>
    


    <!-- http://people.aifb.kit.edu/mu2771/step#requieredExpertise -->

    <owl:ObjectProperty rdf:about="http://people.aifb.kit.edu/mu2771/step#requieredExpertise">
        <rdfs:domain rdf:resource="http://people.aifb.kit.edu/mu2771/step#WorkOrder"/>
        <rdfs:range rdf:resource="http://people.aifb.kit.edu/mu2771/step#Expertise"/>
        <rdfs:comment xml:lang="en">specifies which level of which expertise type is the required minimum</rdfs:comment>
        <rdfs:label xml:lang="en">required expertise</rdfs:label>
    </owl:ObjectProperty>
    


    <!-- http://people.aifb.kit.edu/mu2771/step#runBy -->

    <owl:ObjectProperty rdf:about="http://people.aifb.kit.edu/mu2771/step#runBy">
        <rdfs:domain rdf:resource="http://purl.oclc.org/NET/ssnx/ssn#System"/>
        <rdfs:range rdf:resource="http://www.w3.org/ns/org#Organization"/>
        <rdfs:comment xml:lang="en">the operating business entity of a ssn:System</rdfs:comment>
        <rdfs:label xml:lang="en">run by</rdfs:label>
    </owl:ObjectProperty>
    


    <!-- http://people.aifb.kit.edu/mu2771/step#usedModel -->

    <owl:ObjectProperty rdf:about="http://people.aifb.kit.edu/mu2771/step#usedModel">
        <rdfs:domain rdf:resource="http://people.aifb.kit.edu/mu2771/step#Prediction"/>
        <rdfs:comment>describes the type of algorithm used to produce the prediction</rdfs:comment>
        <rdfs:label>usedModel</rdfs:label>
    </owl:ObjectProperty>
    


    <!-- http://people.aifb.kit.edu/mu2771/step#wasFinishedWorkOrder -->

    <owl:ObjectProperty rdf:about="http://people.aifb.kit.edu/mu2771/step#wasFinishedWorkOrder">
        <rdfs:domain rdf:resource="http://people.aifb.kit.edu/mu2771/step#WorkOrder"/>
        <rdfs:range rdf:resource="http://people.aifb.kit.edu/mu2771/step#FinishedWorkOrder"/>
        <rdfs:label xml:lang="de">war Beendeter Auftrag</rdfs:label>
        <rdfs:label xml:lang="en">was finished work order</rdfs:label>
    </owl:ObjectProperty>
    


    <!-- http://people.aifb.kit.edu/mu2771/step#wasNewWorkOrder -->

    <owl:ObjectProperty rdf:about="http://people.aifb.kit.edu/mu2771/step#wasNewWorkOrder">
        <rdfs:domain rdf:resource="http://people.aifb.kit.edu/mu2771/step#WorkOrder"/>
        <rdfs:range rdf:resource="http://people.aifb.kit.edu/mu2771/step#NewWorkOrder"/>
        <rdfs:comment xml:lang="de">war Neuer Auftrag</rdfs:comment>
        <rdfs:label xml:lang="en">was new work order</rdfs:label>
    </owl:ObjectProperty>
    


    <!-- http://people.aifb.kit.edu/mu2771/step#wasScheduledWorkOrder -->

    <owl:ObjectProperty rdf:about="http://people.aifb.kit.edu/mu2771/step#wasScheduledWorkOrder">
        <rdfs:domain rdf:resource="http://people.aifb.kit.edu/mu2771/step#WorkOrder"/>
        <rdfs:range rdf:resource="http://people.aifb.kit.edu/mu2771/step#ScheduledWorkOrder"/>
        <rdfs:comment xml:lang="de">war Geplanter Auftrag</rdfs:comment>
        <rdfs:label xml:lang="en">was scheduled work order</rdfs:label>
    </owl:ObjectProperty>
    


    <!-- http://people.aifb.kit.edu/mu2771/step#wasUnplanedWorkOrder -->

    <owl:ObjectProperty rdf:about="http://people.aifb.kit.edu/mu2771/step#wasUnplanedWorkOrder">
        <rdfs:domain rdf:resource="http://people.aifb.kit.edu/mu2771/step#WorkOrder"/>
        <rdfs:range rdf:resource="http://people.aifb.kit.edu/mu2771/step#UnplannedWorkOrder"/>
        <rdfs:comment xml:lang="de">war Ungeplanter Auftrag</rdfs:comment>
        <rdfs:label xml:lang="en">was unplanned work order</rdfs:label>
    </owl:ObjectProperty>
    


    <!-- http://people.aifb.kit.edu/mu2771/step/0.2.0/moduleC#date -->

    <owl:ObjectProperty rdf:about="http://people.aifb.kit.edu/mu2771/step/0.2.0/moduleC#date">
        <rdfs:label>time:date</rdfs:label>
    </owl:ObjectProperty>
    


    <!-- http://purl.oclc.org/NET/ssnx/ssn#attachedSystem -->

    <owl:ObjectProperty rdf:about="http://purl.oclc.org/NET/ssnx/ssn#attachedSystem">
        <rdfs:subPropertyOf rdf:resource="http://www.loa-cnr.it/ontologies/DUL.owl#isLocationOf"/>
        <owl:inverseOf rdf:resource="http://purl.oclc.org/NET/ssnx/ssn#onPlatform"/>
        <rdfs:comment>Relation between a Platform and any Systems (e.g., Sensors) that are attached to the Platform.</rdfs:comment>
        <rdfs:isDefinedBy>http://purl.oclc.org/NET/ssnx/ssn</rdfs:isDefinedBy>
        <rdfs:label>attached system</rdfs:label>
        <rdfs:seeAlso>http://www.w3.org/2005/Incubator/ssn/wiki/SSN_Deploy#PlatformSite</rdfs:seeAlso>
    </owl:ObjectProperty>
    


    <!-- http://purl.oclc.org/NET/ssnx/ssn#deployedOnPlatform -->

    <owl:ObjectProperty rdf:about="http://purl.oclc.org/NET/ssnx/ssn#deployedOnPlatform">
        <rdfs:subPropertyOf rdf:resource="http://www.loa-cnr.it/ontologies/DUL.owl#hasParticipant"/>
        <owl:inverseOf rdf:resource="http://purl.oclc.org/NET/ssnx/ssn#inDeployment"/>
        <rdfs:comment>Relation between a deployment and the platform on which the system was deployed.</rdfs:comment>
        <rdfs:isDefinedBy>http://purl.oclc.org/NET/ssnx/ssn</rdfs:isDefinedBy>
        <rdfs:label>deployed on platform</rdfs:label>
        <rdfs:seeAlso>http://www.w3.org/2005/Incubator/ssn/wiki/SSN_Deploy#Deployment</rdfs:seeAlso>
    </owl:ObjectProperty>
    


    <!-- http://purl.oclc.org/NET/ssnx/ssn#deployedSystem -->

    <owl:ObjectProperty rdf:about="http://purl.oclc.org/NET/ssnx/ssn#deployedSystem">
        <rdfs:subPropertyOf rdf:resource="http://www.loa-cnr.it/ontologies/DUL.owl#hasParticipant"/>
        <owl:inverseOf rdf:resource="http://purl.oclc.org/NET/ssnx/ssn#hasDeployment"/>
        <rdfs:comment>Relation between a deployment and the deployed system.</rdfs:comment>
        <rdfs:isDefinedBy>http://purl.oclc.org/NET/ssnx/ssn</rdfs:isDefinedBy>
        <rdfs:label>deployed system</rdfs:label>
        <rdfs:seeAlso>http://www.w3.org/2005/Incubator/ssn/wiki/SSN_Deploy#Deployment</rdfs:seeAlso>
    </owl:ObjectProperty>
    


    <!-- http://purl.oclc.org/NET/ssnx/ssn#deploymentProcessPart -->

    <owl:ObjectProperty rdf:about="http://purl.oclc.org/NET/ssnx/ssn#deploymentProcessPart">
        <rdfs:subPropertyOf rdf:resource="http://www.loa-cnr.it/ontologies/DUL.owl#hasPart"/>
        <rdfs:comment>Has part relation between a deployment process and its constituent processes.</rdfs:comment>
        <rdfs:isDefinedBy>http://purl.oclc.org/NET/ssnx/ssn</rdfs:isDefinedBy>
        <rdfs:label>deployment process part</rdfs:label>
        <rdfs:seeAlso>http://www.w3.org/2005/Incubator/ssn/wiki/SSN_Deploy#Deployment</rdfs:seeAlso>
    </owl:ObjectProperty>
    


    <!-- http://purl.oclc.org/NET/ssnx/ssn#detects -->

    <owl:ObjectProperty rdf:about="http://purl.oclc.org/NET/ssnx/ssn#detects">
        <rdfs:comment>A relation from a sensor to the Stimulus that the sensor can detect.   
The Stimulus itself will be serving as a proxy for (see isProxyOf) some observable property.</rdfs:comment>
        <rdfs:isDefinedBy>http://purl.oclc.org/NET/ssnx/ssn</rdfs:isDefinedBy>
        <rdfs:label>detects</rdfs:label>
        <rdfs:seeAlso>http://www.w3.org/2005/Incubator/ssn/wiki/SSN_Skeleton#Skeleton</rdfs:seeAlso>
    </owl:ObjectProperty>
    


    <!-- http://purl.oclc.org/NET/ssnx/ssn#endTime -->

    <owl:ObjectProperty rdf:about="http://purl.oclc.org/NET/ssnx/ssn#endTime">
        <rdfs:subPropertyOf rdf:resource="http://www.loa-cnr.it/ontologies/DUL.owl#hasRegion"/>
        <rdfs:isDefinedBy>http://purl.oclc.org/NET/ssnx/ssn</rdfs:isDefinedBy>
        <rdfs:label>end time</rdfs:label>
        <rdfs:seeAlso>http://www.w3.org/2005/Incubator/ssn/wiki/SSN_Base#Time</rdfs:seeAlso>
    </owl:ObjectProperty>
    


    <!-- http://purl.oclc.org/NET/ssnx/ssn#featureOfInterest -->

    <owl:ObjectProperty rdf:about="http://purl.oclc.org/NET/ssnx/ssn#featureOfInterest">
        <rdfs:subPropertyOf rdf:resource="http://www.loa-cnr.it/ontologies/DUL.owl#isSettingFor"/>
        <dc:source>skos:exactMatch &apos;featureOfInterest&apos; [O&amp;M - ISO/DIS 19156] 
		                    http://portal.opengeospatial.org/files/?artifact_id=41579</dc:source>
        <rdfs:comment>A relation between an observation and the entity whose quality was observed.   For example, in an observation of the weight of a person, the feature of interest is the person and the quality is weight.</rdfs:comment>
        <rdfs:isDefinedBy>http://purl.oclc.org/NET/ssnx/ssn</rdfs:isDefinedBy>
        <rdfs:label>feature of interest</rdfs:label>
        <rdfs:seeAlso>http://www.w3.org/2005/Incubator/ssn/wiki/SSN_Skeleton#Skeleton</rdfs:seeAlso>
    </owl:ObjectProperty>
    


    <!-- http://purl.oclc.org/NET/ssnx/ssn#forProperty -->

    <owl:ObjectProperty rdf:about="http://purl.oclc.org/NET/ssnx/ssn#forProperty">
        <rdfs:comment>A relation between some aspect of a sensing entity and a property.  For example, from a sensor to the properties it can observe, or from a deployment to the properties it was installed to observe.  Also from a measurement capability to the property the capability is described for.  (Used in conjunction with ofFeature).</rdfs:comment>
        <rdfs:isDefinedBy>http://purl.oclc.org/NET/ssnx/ssn</rdfs:isDefinedBy>
        <rdfs:label>for property</rdfs:label>
        <rdfs:seeAlso>http://www.w3.org/2005/Incubator/ssn/wiki/SSN_Skeleton#Skeleton</rdfs:seeAlso>
    </owl:ObjectProperty>
    


    <!-- http://purl.oclc.org/NET/ssnx/ssn#hasDeployment -->

    <owl:ObjectProperty rdf:about="http://purl.oclc.org/NET/ssnx/ssn#hasDeployment">
        <rdfs:subPropertyOf rdf:resource="http://www.loa-cnr.it/ontologies/DUL.owl#isParticipantIn"/>
        <rdfs:comment>Relation between a System and a Deployment, recording that the System/Sensor was deployed in that Deployment.</rdfs:comment>
        <rdfs:isDefinedBy>http://purl.oclc.org/NET/ssnx/ssn</rdfs:isDefinedBy>
        <rdfs:label>has deployment</rdfs:label>
        <rdfs:seeAlso>http://www.w3.org/2005/Incubator/ssn/wiki/SSN_Deploy#Deployment</rdfs:seeAlso>
    </owl:ObjectProperty>
    


    <!-- http://purl.oclc.org/NET/ssnx/ssn#hasInput -->

    <owl:ObjectProperty rdf:about="http://purl.oclc.org/NET/ssnx/ssn#hasInput">
        <rdfs:isDefinedBy>http://purl.oclc.org/NET/ssnx/ssn</rdfs:isDefinedBy>
        <rdfs:label>has input</rdfs:label>
        <rdfs:seeAlso>http://www.w3.org/2005/Incubator/ssn/wiki/SSN_Model#Process</rdfs:seeAlso>
    </owl:ObjectProperty>
    


    <!-- http://purl.oclc.org/NET/ssnx/ssn#hasMeasurementCapability -->

    <owl:ObjectProperty rdf:about="http://purl.oclc.org/NET/ssnx/ssn#hasMeasurementCapability">
        <rdfs:subPropertyOf rdf:resource="http://purl.oclc.org/NET/ssnx/ssn#hasProperty"/>
        <rdfs:comment>Relation from a Sensor to a MeasurementCapability describing the measurement properties of the sensor.</rdfs:comment>
        <rdfs:isDefinedBy>http://purl.oclc.org/NET/ssnx/ssn</rdfs:isDefinedBy>
        <rdfs:label>has measurement  capability</rdfs:label>
        <rdfs:seeAlso>http://www.w3.org/2005/Incubator/ssn/wiki/SSN_Sensor#MeasuringCapability</rdfs:seeAlso>
    </owl:ObjectProperty>
    


    <!-- http://purl.oclc.org/NET/ssnx/ssn#hasMeasurementProperty -->

    <owl:ObjectProperty rdf:about="http://purl.oclc.org/NET/ssnx/ssn#hasMeasurementProperty">
        <rdfs:subPropertyOf rdf:resource="http://purl.oclc.org/NET/ssnx/ssn#hasProperty"/>
        <rdfs:comment>Relation from a MeasurementCapability to a MeasurementProperty.  For example, to an accuracy (see notes at MeasurementCapability).</rdfs:comment>
        <rdfs:isDefinedBy>http://purl.oclc.org/NET/ssnx/ssn</rdfs:isDefinedBy>
        <rdfs:label>has measurement property</rdfs:label>
        <rdfs:seeAlso>http://www.w3.org/2005/Incubator/ssn/wiki/SSN_Sensor#MeasuringCapability</rdfs:seeAlso>
    </owl:ObjectProperty>
    


    <!-- http://purl.oclc.org/NET/ssnx/ssn#hasOperatingProperty -->

    <owl:ObjectProperty rdf:about="http://purl.oclc.org/NET/ssnx/ssn#hasOperatingProperty">
        <rdfs:subPropertyOf rdf:resource="http://purl.oclc.org/NET/ssnx/ssn#hasProperty"/>
        <rdfs:comment>Relation from an OperatingRange to a Property.  For example, to a battery lifetime.</rdfs:comment>
        <rdfs:isDefinedBy>http://purl.oclc.org/NET/ssnx/ssn</rdfs:isDefinedBy>
        <rdfs:label>has operating property</rdfs:label>
        <rdfs:seeAlso>http://www.w3.org/2005/Incubator/ssn/wiki/SSN_Deploy#OperatingRestriction</rdfs:seeAlso>
    </owl:ObjectProperty>
    


    <!-- http://purl.oclc.org/NET/ssnx/ssn#hasOperatingRange -->

    <owl:ObjectProperty rdf:about="http://purl.oclc.org/NET/ssnx/ssn#hasOperatingRange">
        <rdfs:subPropertyOf rdf:resource="http://purl.oclc.org/NET/ssnx/ssn#hasProperty"/>
        <rdfs:comment>Relation from a System to an OperatingRange describing the normal operating environment of the System.</rdfs:comment>
        <rdfs:isDefinedBy>http://purl.oclc.org/NET/ssnx/ssn</rdfs:isDefinedBy>
        <rdfs:label>has operating range</rdfs:label>
        <rdfs:seeAlso>http://www.w3.org/2005/Incubator/ssn/wiki/SSN_Deploy#OperatingRestriction</rdfs:seeAlso>
    </owl:ObjectProperty>
    


    <!-- http://purl.oclc.org/NET/ssnx/ssn#hasOutput -->

    <owl:ObjectProperty rdf:about="http://purl.oclc.org/NET/ssnx/ssn#hasOutput">
        <rdfs:domain rdf:resource="http://purl.oclc.org/NET/ssnx/ssn#Process"/>
        <rdfs:range rdf:resource="http://purl.oclc.org/NET/ssnx/ssn#Output"/>
        <rdfs:isDefinedBy>http://purl.oclc.org/NET/ssnx/ssn</rdfs:isDefinedBy>
        <rdfs:label>has output</rdfs:label>
        <rdfs:seeAlso>http://www.w3.org/2005/Incubator/ssn/wiki/SSN_Model#Process</rdfs:seeAlso>
    </owl:ObjectProperty>
    


    <!-- http://purl.oclc.org/NET/ssnx/ssn#hasProperty -->

    <owl:ObjectProperty rdf:about="http://purl.oclc.org/NET/ssnx/ssn#hasProperty">
        <rdfs:subPropertyOf rdf:resource="http://www.loa-cnr.it/ontologies/DUL.owl#hasQuality"/>
        <owl:inverseOf rdf:resource="http://purl.oclc.org/NET/ssnx/ssn#isPropertyOf"/>
        <rdfs:comment>A relation between a FeatureOfInterest and a Property of that feature.</rdfs:comment>
        <rdfs:isDefinedBy>http://purl.oclc.org/NET/ssnx/ssn</rdfs:isDefinedBy>
        <rdfs:label>has property</rdfs:label>
        <rdfs:seeAlso>http://www.w3.org/2005/Incubator/ssn/wiki/SSN_Skeleton#Skeleton</rdfs:seeAlso>
    </owl:ObjectProperty>
    


    <!-- http://purl.oclc.org/NET/ssnx/ssn#hasSubSystem -->

    <owl:ObjectProperty rdf:about="http://purl.oclc.org/NET/ssnx/ssn#hasSubSystem">
        <rdfs:subPropertyOf rdf:resource="http://www.loa-cnr.it/ontologies/DUL.owl#hasPart"/>
        <rdfs:domain rdf:resource="http://purl.oclc.org/NET/ssnx/ssn#System"/>
        <rdfs:range rdf:resource="http://purl.oclc.org/NET/ssnx/ssn#System"/>
        <rdfs:comment>Haspart relation between a system and its parts.</rdfs:comment>
        <rdfs:isDefinedBy>http://purl.oclc.org/NET/ssnx/ssn</rdfs:isDefinedBy>
        <rdfs:label>has subsystem</rdfs:label>
        <rdfs:seeAlso>http://www.w3.org/2005/Incubator/ssn/wiki/SSN_Model#System</rdfs:seeAlso>
    </owl:ObjectProperty>
    


    <!-- http://purl.oclc.org/NET/ssnx/ssn#hasSurvivalProperty -->

    <owl:ObjectProperty rdf:about="http://purl.oclc.org/NET/ssnx/ssn#hasSurvivalProperty">
        <rdfs:subPropertyOf rdf:resource="http://purl.oclc.org/NET/ssnx/ssn#hasProperty"/>
        <rdfs:comment>Relation from a SurvivalRange to a Property describing the survial range of a system.  For example, to the temperature extreme that a system can withstand before being considered damaged.</rdfs:comment>
        <rdfs:isDefinedBy>http://purl.oclc.org/NET/ssnx/ssn</rdfs:isDefinedBy>
        <rdfs:label>has survival property</rdfs:label>
        <rdfs:seeAlso>http://www.w3.org/2005/Incubator/ssn/wiki/SSN_Deploy#OperatingRestriction</rdfs:seeAlso>
    </owl:ObjectProperty>
    


    <!-- http://purl.oclc.org/NET/ssnx/ssn#hasSurvivalRange -->

    <owl:ObjectProperty rdf:about="http://purl.oclc.org/NET/ssnx/ssn#hasSurvivalRange">
        <rdfs:subPropertyOf rdf:resource="http://purl.oclc.org/NET/ssnx/ssn#hasProperty"/>
        <rdfs:domain rdf:resource="http://purl.oclc.org/NET/ssnx/ssn#System"/>
        <rdfs:range rdf:resource="http://purl.oclc.org/NET/ssnx/ssn#SurvivalRange"/>
        <rdfs:comment>A Relation from a System to a SurvivalRange.</rdfs:comment>
        <rdfs:isDefinedBy>http://purl.oclc.org/NET/ssnx/ssn</rdfs:isDefinedBy>
        <rdfs:label>has survival range</rdfs:label>
        <rdfs:seeAlso>http://www.w3.org/2005/Incubator/ssn/wiki/SSN_Deploy#OperatingRestriction</rdfs:seeAlso>
    </owl:ObjectProperty>
    


    <!-- http://purl.oclc.org/NET/ssnx/ssn#hasValue -->

    <owl:ObjectProperty rdf:about="http://purl.oclc.org/NET/ssnx/ssn#hasValue">
        <rdfs:subPropertyOf rdf:resource="http://www.loa-cnr.it/ontologies/DUL.owl#hasRegion"/>
        <rdfs:domain rdf:resource="http://purl.oclc.org/NET/ssnx/ssn#SensorOutput"/>
        <rdfs:range rdf:resource="http://purl.oclc.org/NET/ssnx/ssn#ObservationValue"/>
        <rdfs:isDefinedBy>http://purl.oclc.org/NET/ssnx/ssn</rdfs:isDefinedBy>
        <rdfs:label>has value</rdfs:label>
        <rdfs:seeAlso>http://www.w3.org/2005/Incubator/ssn/wiki/SSN_Base#Data</rdfs:seeAlso>
    </owl:ObjectProperty>
    


    <!-- http://purl.oclc.org/NET/ssnx/ssn#implementedBy -->

    <owl:ObjectProperty rdf:about="http://purl.oclc.org/NET/ssnx/ssn#implementedBy">
        <rdfs:subPropertyOf rdf:resource="http://www.loa-cnr.it/ontologies/DUL.owl#describes"/>
        <owl:inverseOf rdf:resource="http://purl.oclc.org/NET/ssnx/ssn#implements"/>
        <rdfs:comment>A relation between the description of an algorithm, procedure or method and an entity that implements that method in some executable way.  For example, between a scientific measuring method and a sensor the senses via that method.</rdfs:comment>
        <rdfs:isDefinedBy>http://purl.oclc.org/NET/ssnx/ssn</rdfs:isDefinedBy>
        <rdfs:label>implemented by</rdfs:label>
        <rdfs:seeAlso>http://www.w3.org/2005/Incubator/ssn/wiki/SSN_Skeleton#Skeleton</rdfs:seeAlso>
    </owl:ObjectProperty>
    


    <!-- http://purl.oclc.org/NET/ssnx/ssn#implements -->

    <owl:ObjectProperty rdf:about="http://purl.oclc.org/NET/ssnx/ssn#implements">
        <rdfs:subPropertyOf rdf:resource="http://www.loa-cnr.it/ontologies/DUL.owl#isDescribedBy"/>
        <rdfs:comment>A relation between an entity that implements a method in some executable way and the description of an algorithm, procedure or method.  For example, between a Sensor and the scientific measuring method that the Sensor uses to observe a Property.</rdfs:comment>
        <rdfs:isDefinedBy>http://purl.oclc.org/NET/ssnx/ssn</rdfs:isDefinedBy>
        <rdfs:label>implements</rdfs:label>
        <rdfs:seeAlso>http://www.w3.org/2005/Incubator/ssn/wiki/SSN_Skeleton#Skeleton</rdfs:seeAlso>
    </owl:ObjectProperty>
    


    <!-- http://purl.oclc.org/NET/ssnx/ssn#inCondition -->

    <owl:ObjectProperty rdf:about="http://purl.oclc.org/NET/ssnx/ssn#inCondition">
        <rdfs:comment>Describes the prevailing environmental conditions for MeasurementCapabilites, OperatingConditions and SurvivalRanges.  Used for example to say that a sensor has a particular accuracy in particular conditions.  (see also MeasurementCapability)</rdfs:comment>
        <rdfs:isDefinedBy>http://purl.oclc.org/NET/ssnx/ssn</rdfs:isDefinedBy>
        <rdfs:label>in condition</rdfs:label>
        <rdfs:seeAlso>http://www.w3.org/2005/Incubator/ssn/wiki/SSN_Base#ConstraintBlock</rdfs:seeAlso>
    </owl:ObjectProperty>
    


    <!-- http://purl.oclc.org/NET/ssnx/ssn#inDeployment -->

    <owl:ObjectProperty rdf:about="http://purl.oclc.org/NET/ssnx/ssn#inDeployment">
        <rdfs:subPropertyOf rdf:resource="http://www.loa-cnr.it/ontologies/DUL.owl#isParticipantIn"/>
        <rdfs:comment>Relation between a Platform and a Deployment, recording that the object was used as a platform for a system/sensor for a particular deployment: as in this PhysicalObject is acting as a Platform inDeployment Deployment.</rdfs:comment>
        <rdfs:isDefinedBy>http://purl.oclc.org/NET/ssnx/ssn</rdfs:isDefinedBy>
        <rdfs:label>in deployment</rdfs:label>
        <rdfs:seeAlso>http://www.w3.org/2005/Incubator/ssn/wiki/SSN_Deploy#Deployment</rdfs:seeAlso>
    </owl:ObjectProperty>
    


    <!-- http://purl.oclc.org/NET/ssnx/ssn#isProducedBy -->

    <owl:ObjectProperty rdf:about="http://purl.oclc.org/NET/ssnx/ssn#isProducedBy">
        <rdfs:domain rdf:resource="http://purl.oclc.org/NET/ssnx/ssn#SensorOutput"/>
        <rdfs:range rdf:resource="http://purl.oclc.org/NET/ssnx/ssn#Sensor"/>
        <rdfs:comment>Relation between a producer and a produced entity: for example, between a sensor and the produced output.</rdfs:comment>
        <rdfs:isDefinedBy>http://purl.oclc.org/NET/ssnx/ssn</rdfs:isDefinedBy>
        <rdfs:label>is produced by</rdfs:label>
        <rdfs:seeAlso>http://www.w3.org/2005/Incubator/ssn/wiki/SSN_Model#Process</rdfs:seeAlso>
    </owl:ObjectProperty>
    


    <!-- http://purl.oclc.org/NET/ssnx/ssn#isPropertyOf -->

    <owl:ObjectProperty rdf:about="http://purl.oclc.org/NET/ssnx/ssn#isPropertyOf">
        <rdfs:subPropertyOf rdf:resource="http://www.loa-cnr.it/ontologies/DUL.owl#isQualityOf"/>
        <rdfs:comment>Relation between a FeatureOfInterest and a Property (a Quality observable by a sensor) of that feature.</rdfs:comment>
        <rdfs:isDefinedBy>http://purl.oclc.org/NET/ssnx/ssn</rdfs:isDefinedBy>
        <rdfs:label>is property of</rdfs:label>
        <rdfs:seeAlso>http://www.w3.org/2005/Incubator/ssn/wiki/SSN_Skeleton#Skeleton</rdfs:seeAlso>
    </owl:ObjectProperty>
    


    <!-- http://purl.oclc.org/NET/ssnx/ssn#isProxyFor -->

    <owl:ObjectProperty rdf:about="http://purl.oclc.org/NET/ssnx/ssn#isProxyFor">
        <rdfs:comment>A relation from a Stimulus to the Property that the Stimulus is serving as a proxy for.  For example, the expansion of the quicksilver is a stimulus that serves as a proxy for temperature, or an increase or decrease in the spinning of cups on a wind sensor is serving as a proxy for wind speed.</rdfs:comment>
        <rdfs:isDefinedBy>http://purl.oclc.org/NET/ssnx/ssn</rdfs:isDefinedBy>
        <rdfs:label>isProxyFor</rdfs:label>
        <rdfs:seeAlso>http://www.w3.org/2005/Incubator/ssn/wiki/SSN_Skeleton#Skeleton</rdfs:seeAlso>
    </owl:ObjectProperty>
    


    <!-- http://purl.oclc.org/NET/ssnx/ssn#madeObservation -->

    <owl:ObjectProperty rdf:about="http://purl.oclc.org/NET/ssnx/ssn#madeObservation">
        <rdfs:subPropertyOf rdf:resource="http://www.loa-cnr.it/ontologies/DUL.owl#isObjectIncludedIn"/>
        <owl:inverseOf rdf:resource="http://purl.oclc.org/NET/ssnx/ssn#observedBy"/>
        <rdfs:comment>Relation between a Sensor and Observations it has made.</rdfs:comment>
        <rdfs:isDefinedBy>http://purl.oclc.org/NET/ssnx/ssn</rdfs:isDefinedBy>
        <rdfs:label>made observation</rdfs:label>
        <rdfs:seeAlso>http://www.w3.org/2005/Incubator/ssn/wiki/SSN_Observation#Observation</rdfs:seeAlso>
    </owl:ObjectProperty>
    


    <!-- http://purl.oclc.org/NET/ssnx/ssn#observationResult -->

    <owl:ObjectProperty rdf:about="http://purl.oclc.org/NET/ssnx/ssn#observationResult">
        <rdfs:subPropertyOf rdf:resource="http://www.loa-cnr.it/ontologies/DUL.owl#isSettingFor"/>
        <dc:source>skos:closeMatch &apos;result&apos; [O&amp;M - ISO/DIS 19156] 
		                    http://portal.opengeospatial.org/files/?artifact_id=41579</dc:source>
        <rdfs:comment>Relation linking an Observation (i.e., a description of the context, the Situation, in which the observatioin was made) and a Result, which contains a value representing the value associated with the observed Property.</rdfs:comment>
        <rdfs:isDefinedBy>http://purl.oclc.org/NET/ssnx/ssn</rdfs:isDefinedBy>
        <rdfs:label>observation result</rdfs:label>
        <rdfs:seeAlso>http://www.w3.org/2005/Incubator/ssn/wiki/SSN_Skeleton#Skeleton</rdfs:seeAlso>
    </owl:ObjectProperty>
    


    <!-- http://purl.oclc.org/NET/ssnx/ssn#observationResultTime -->

    <owl:ObjectProperty rdf:about="http://purl.oclc.org/NET/ssnx/ssn#observationResultTime">
        <rdfs:subPropertyOf rdf:resource="http://www.loa-cnr.it/ontologies/DUL.owl#hasRegion"/>
        <dc:source>http://www.opengeospatial.org/standards/om</dc:source>
        <rdfs:comment>The result time is the time when the procedure associated with the observation act was applied.</rdfs:comment>
        <rdfs:comment>The result time shall describe the time when the result became available, typically when the procedure associated with the observation was completed For some observations this is identical to the phenomenonTime. However, there are important cases where they differ.[O&amp;M]</rdfs:comment>
        <rdfs:isDefinedBy>http://purl.oclc.org/NET/ssnx/ssn</rdfs:isDefinedBy>
        <rdfs:label>observation result time</rdfs:label>
        <rdfs:seeAlso>http://www.w3.org/2005/Incubator/ssn/wiki/SSN_Observation#Observation</rdfs:seeAlso>
    </owl:ObjectProperty>
    


    <!-- http://purl.oclc.org/NET/ssnx/ssn#observationSamplingTime -->

    <owl:ObjectProperty rdf:about="http://purl.oclc.org/NET/ssnx/ssn#observationSamplingTime">
        <rdfs:subPropertyOf rdf:resource="http://www.loa-cnr.it/ontologies/DUL.owl#hasRegion"/>
        <dc:source>http://www.opengeospatial.org/standards/om</dc:source>
        <rdfs:comment>Rebadged as phenomenon time in [O&amp;M]. The phenomenon time shall describe the time that the result applies to the property of the feature-of-interest. This is often the time of interaction by a sampling procedure or observation procedure with a real-world feature.</rdfs:comment>
        <rdfs:comment>The sampling time is the time that the result applies to the feature-of-interest. This is the time usually required for geospatial analysis of the result.</rdfs:comment>
        <rdfs:isDefinedBy>http://purl.oclc.org/NET/ssnx/ssn</rdfs:isDefinedBy>
        <rdfs:label>observation sampling time</rdfs:label>
        <rdfs:seeAlso>http://www.w3.org/2005/Incubator/ssn/wiki/SSN_Observation#Observation</rdfs:seeAlso>
    </owl:ObjectProperty>
    


    <!-- http://purl.oclc.org/NET/ssnx/ssn#observedBy -->

    <owl:ObjectProperty rdf:about="http://purl.oclc.org/NET/ssnx/ssn#observedBy">
        <rdfs:subPropertyOf rdf:resource="http://www.loa-cnr.it/ontologies/DUL.owl#includesObject"/>
        <rdfs:isDefinedBy>http://purl.oclc.org/NET/ssnx/ssn</rdfs:isDefinedBy>
        <rdfs:seeAlso>http://www.w3.org/2005/Incubator/ssn/wiki/SSN_Skeleton#Skeleton</rdfs:seeAlso>
    </owl:ObjectProperty>
    


    <!-- http://purl.oclc.org/NET/ssnx/ssn#observedProperty -->

    <owl:ObjectProperty rdf:about="http://purl.oclc.org/NET/ssnx/ssn#observedProperty">
        <rdfs:subPropertyOf rdf:resource="http://www.loa-cnr.it/ontologies/DUL.owl#isSettingFor"/>
        <dc:source>skos:exactMatch &apos;observedProperty&apos; [O&amp;M - ISO/DIS 19156] 
		                    http://portal.opengeospatial.org/files/?artifact_id=41579</dc:source>
        <rdfs:comment>Relation linking an Observation to the Property that was observed.  The observedProperty should be a Property (hasProperty) of the FeatureOfInterest (linked by featureOfInterest) of this observation.</rdfs:comment>
        <rdfs:isDefinedBy>http://purl.oclc.org/NET/ssnx/ssn</rdfs:isDefinedBy>
        <rdfs:label>observed property</rdfs:label>
        <rdfs:seeAlso>http://www.w3.org/2005/Incubator/ssn/wiki/SSN_Skeleton#Skeleton</rdfs:seeAlso>
    </owl:ObjectProperty>
    


    <!-- http://purl.oclc.org/NET/ssnx/ssn#observes -->

    <owl:ObjectProperty rdf:about="http://purl.oclc.org/NET/ssnx/ssn#observes">
        <owl:propertyChainAxiom rdf:parseType="Collection">
            <rdf:Description rdf:about="http://purl.oclc.org/NET/ssnx/ssn#hasMeasurementCapability"/>
            <rdf:Description rdf:about="http://purl.oclc.org/NET/ssnx/ssn#forProperty"/>
        </owl:propertyChainAxiom>
        <owl:propertyChainAxiom rdf:parseType="Collection">
            <rdf:Description rdf:about="http://purl.oclc.org/NET/ssnx/ssn#madeObservation"/>
            <rdf:Description rdf:about="http://purl.oclc.org/NET/ssnx/ssn#observedProperty"/>
        </owl:propertyChainAxiom>
        <rdfs:comment>Relation between a Sensor and a Property that the sensor can observe.

Note that, given the DUL modelling of Qualities, a sensor defined with &apos;observes only Windspeed&apos; technically links the sensor to particular instances of Windspeed, not to the concept itself - OWL can&apos;t express concept-concept relations, only individual-individual.  The property composition ensures that if an observation is made of a particular quality then one can infer that the sensor observes that quality.</rdfs:comment>
        <rdfs:isDefinedBy>http://purl.oclc.org/NET/ssnx/ssn</rdfs:isDefinedBy>
        <rdfs:label>observes</rdfs:label>
        <rdfs:seeAlso>http://www.w3.org/2005/Incubator/ssn/wiki/SSN_Sensor#Measuring</rdfs:seeAlso>
    </owl:ObjectProperty>
    


    <!-- http://purl.oclc.org/NET/ssnx/ssn#ofFeature -->

    <owl:ObjectProperty rdf:about="http://purl.oclc.org/NET/ssnx/ssn#ofFeature">
        <rdfs:comment>A relation between some aspect of a sensing entity and a feature.  For example, from a sensor to the features it can observe properties of, or from a deployment to the features it was installed to observe.  Also from a measurement capability to the feature the capability is described for.  (Used in conjunction with forProperty).</rdfs:comment>
        <rdfs:isDefinedBy>http://purl.oclc.org/NET/ssnx/ssn</rdfs:isDefinedBy>
        <rdfs:label>of feature</rdfs:label>
        <rdfs:seeAlso>http://www.w3.org/2005/Incubator/ssn/wiki/SSN_Skeleton#Skeleton</rdfs:seeAlso>
    </owl:ObjectProperty>
    


    <!-- http://purl.oclc.org/NET/ssnx/ssn#onPlatform -->

    <owl:ObjectProperty rdf:about="http://purl.oclc.org/NET/ssnx/ssn#onPlatform">
        <rdfs:subPropertyOf rdf:resource="http://www.loa-cnr.it/ontologies/DUL.owl#hasLocation"/>
        <rdfs:comment>Relation between a System (e.g., a Sensor) and a Platform.  The relation locates the sensor relative to other described entities entities: i.e., the Sensor s1&apos;s location is Platform p1.  More precise locations for sensors in space (relative to other entities, where attached to another entity, or in 3D space) are made using DOLCE&apos;s Regions (SpaceRegion).</rdfs:comment>
        <rdfs:isDefinedBy>http://purl.oclc.org/NET/ssnx/ssn</rdfs:isDefinedBy>
        <rdfs:label>on platform</rdfs:label>
        <rdfs:seeAlso>http://www.w3.org/2005/Incubator/ssn/wiki/SSN_Deploy#PlatformSite</rdfs:seeAlso>
    </owl:ObjectProperty>
    


    <!-- http://purl.oclc.org/NET/ssnx/ssn#qualityOfObservation -->

    <owl:ObjectProperty rdf:about="http://purl.oclc.org/NET/ssnx/ssn#qualityOfObservation">
        <rdfs:subPropertyOf rdf:resource="http://purl.oclc.org/NET/ssnx/ssn#hasProperty"/>
        <dc:source>skos:exactMatch &apos;resultQuality&apos; [O&amp;M - ISO/DIS 19156] 
		                    http://portal.opengeospatial.org/files/?artifact_id=41579</dc:source>
        <rdfs:comment>Relation linking an Observation to the adjudged quality of the result.  This is of course complimentary to the MeasurementCapability information recorded for the Sensor that made the Observation.</rdfs:comment>
        <rdfs:isDefinedBy>http://purl.oclc.org/NET/ssnx/ssn</rdfs:isDefinedBy>
        <rdfs:label>quality of observation</rdfs:label>
        <rdfs:seeAlso>http://www.w3.org/2005/Incubator/ssn/wiki/SSN_Observation#Observation</rdfs:seeAlso>
    </owl:ObjectProperty>
    


    <!-- http://purl.oclc.org/NET/ssnx/ssn#sensingMethodUsed -->

    <owl:ObjectProperty rdf:about="http://purl.oclc.org/NET/ssnx/ssn#sensingMethodUsed">
        <rdfs:subPropertyOf rdf:resource="http://www.loa-cnr.it/ontologies/DUL.owl#satisfies"/>
        <dc:source>http://www.bipm.org/en/committees/jc/jcgm/wg2.html</dc:source>
        <rdfs:comment>A (measurement) procedure is a detailed description of a measurement according to one or more measurement principles and to a given measurement method, based on a measurement model and including any calculation to obtain a measurement result [VIM 2.6]</rdfs:comment>
        <rdfs:isDefinedBy>http://purl.oclc.org/NET/ssnx/ssn</rdfs:isDefinedBy>
        <rdfs:label>sensing method used</rdfs:label>
        <rdfs:seeAlso>http://www.w3.org/2005/Incubator/ssn/wiki/SSN_Skeleton#Skeleton</rdfs:seeAlso>
    </owl:ObjectProperty>
    


    <!-- http://purl.oclc.org/NET/ssnx/ssn#startTime -->

    <owl:ObjectProperty rdf:about="http://purl.oclc.org/NET/ssnx/ssn#startTime">
        <rdfs:subPropertyOf rdf:resource="http://www.loa-cnr.it/ontologies/DUL.owl#hasRegion"/>
        <rdfs:isDefinedBy>http://purl.oclc.org/NET/ssnx/ssn</rdfs:isDefinedBy>
        <rdfs:label>start time</rdfs:label>
        <rdfs:seeAlso>http://www.w3.org/2005/Incubator/ssn/wiki/SSN_Base#Time</rdfs:seeAlso>
    </owl:ObjectProperty>
    


    <!-- http://purl.org/dc/elements/1.1/subject -->

    <owl:ObjectProperty rdf:about="http://purl.org/dc/elements/1.1/subject">
        <rdfs:domain rdf:resource="http://people.aifb.kit.edu/mu2771/step#Report"/>
    </owl:ObjectProperty>
    


    <!-- http://qudt.org/schema/qudt#unit -->

    <owl:ObjectProperty rdf:about="http://qudt.org/schema/qudt#unit">
        <rdfs:domain rdf:resource="http://purl.oclc.org/NET/ssnx/ssn#ObservationValue"/>
    </owl:ObjectProperty>
    


    <!-- http://qudt.org/schema/qudt#value -->

    <owl:ObjectProperty rdf:about="http://qudt.org/schema/qudt#value">
        <rdfs:domain rdf:resource="http://purl.oclc.org/NET/ssnx/ssn#ObservationValue"/>
    </owl:ObjectProperty>
    


    <!-- http://www.loa-cnr.it/ontologies/DUL.owl#describes -->

    <owl:ObjectProperty rdf:about="http://www.loa-cnr.it/ontologies/DUL.owl#describes"/>
    


    <!-- http://www.loa-cnr.it/ontologies/DUL.owl#hasLocation -->

    <owl:ObjectProperty rdf:about="http://www.loa-cnr.it/ontologies/DUL.owl#hasLocation"/>
    


    <!-- http://www.loa-cnr.it/ontologies/DUL.owl#hasPart -->

    <owl:ObjectProperty rdf:about="http://www.loa-cnr.it/ontologies/DUL.owl#hasPart"/>
    


    <!-- http://www.loa-cnr.it/ontologies/DUL.owl#hasParticipant -->

    <owl:ObjectProperty rdf:about="http://www.loa-cnr.it/ontologies/DUL.owl#hasParticipant"/>
    


    <!-- http://www.loa-cnr.it/ontologies/DUL.owl#hasQuality -->

    <owl:ObjectProperty rdf:about="http://www.loa-cnr.it/ontologies/DUL.owl#hasQuality"/>
    


    <!-- http://www.loa-cnr.it/ontologies/DUL.owl#hasRegion -->

    <owl:ObjectProperty rdf:about="http://www.loa-cnr.it/ontologies/DUL.owl#hasRegion"/>
    


    <!-- http://www.loa-cnr.it/ontologies/DUL.owl#includesEvent -->

    <owl:ObjectProperty rdf:about="http://www.loa-cnr.it/ontologies/DUL.owl#includesEvent"/>
    


    <!-- http://www.loa-cnr.it/ontologies/DUL.owl#includesObject -->

    <owl:ObjectProperty rdf:about="http://www.loa-cnr.it/ontologies/DUL.owl#includesObject"/>
    


    <!-- http://www.loa-cnr.it/ontologies/DUL.owl#isDescribedBy -->

    <owl:ObjectProperty rdf:about="http://www.loa-cnr.it/ontologies/DUL.owl#isDescribedBy"/>
    


    <!-- http://www.loa-cnr.it/ontologies/DUL.owl#isLocationOf -->

    <owl:ObjectProperty rdf:about="http://www.loa-cnr.it/ontologies/DUL.owl#isLocationOf"/>
    


    <!-- http://www.loa-cnr.it/ontologies/DUL.owl#isObjectIncludedIn -->

    <owl:ObjectProperty rdf:about="http://www.loa-cnr.it/ontologies/DUL.owl#isObjectIncludedIn"/>
    


    <!-- http://www.loa-cnr.it/ontologies/DUL.owl#isParticipantIn -->

    <owl:ObjectProperty rdf:about="http://www.loa-cnr.it/ontologies/DUL.owl#isParticipantIn"/>
    


    <!-- http://www.loa-cnr.it/ontologies/DUL.owl#isQualityOf -->

    <owl:ObjectProperty rdf:about="http://www.loa-cnr.it/ontologies/DUL.owl#isQualityOf"/>
    


    <!-- http://www.loa-cnr.it/ontologies/DUL.owl#isRegionFor -->

    <owl:ObjectProperty rdf:about="http://www.loa-cnr.it/ontologies/DUL.owl#isRegionFor"/>
    


    <!-- http://www.loa-cnr.it/ontologies/DUL.owl#isSettingFor -->

    <owl:ObjectProperty rdf:about="http://www.loa-cnr.it/ontologies/DUL.owl#isSettingFor"/>
    


    <!-- http://www.loa-cnr.it/ontologies/DUL.owl#satisfies -->

    <owl:ObjectProperty rdf:about="http://www.loa-cnr.it/ontologies/DUL.owl#satisfies"/>
    


    <!-- http://www.w3.org/2003/01/geo/wgs84_pos#location -->

    <owl:ObjectProperty rdf:about="http://www.w3.org/2003/01/geo/wgs84_pos#location">
        <rdfs:subPropertyOf rdf:resource="http://xmlns.com/foaf/0.1/based_near"/>
        <rdfs:range rdf:resource="http://www.w3.org/2003/01/geo/wgs84_pos#SpatialThing"/>
        <rdfs:range>
            <owl:Class>
                <owl:unionOf rdf:parseType="Collection">
                    <rdf:Description rdf:about="http://people.aifb.kit.edu/mu2771/step#SpatialTemporalEntity"/>
                    <rdf:Description rdf:about="http://www.w3.org/2003/01/geo/wgs84_pos#SpatialThing"/>
                </owl:unionOf>
            </owl:Class>
        </rdfs:range>
    </owl:ObjectProperty>
    


    <!-- http://www.w3.org/2006/time#after -->

    <owl:ObjectProperty rdf:about="http://www.w3.org/2006/time#after">
        <owl:inverseOf rdf:resource="http://www.w3.org/2006/time#before"/>
        <rdfs:domain rdf:resource="http://www.w3.org/2006/time#TemporalEntity"/>
        <rdfs:range rdf:resource="http://www.w3.org/2006/time#TemporalEntity"/>
        <rdfs:comment xml:lang="en">Gives directionality to time. If a temporal entity T1 is after another temporal entity T2, then the beginning of T1 is after the end of T2.</rdfs:comment>
        <rdfs:label xml:lang="en">after</rdfs:label>
        <skos:definition xml:lang="en">Gives directionality to time. If a temporal entity T1 is after another temporal entity T2, then the beginning of T1 is after the end of T2.</skos:definition>
    </owl:ObjectProperty>
    


    <!-- http://www.w3.org/2006/time#before -->

    <owl:ObjectProperty rdf:about="http://www.w3.org/2006/time#before">
        <rdf:type rdf:resource="http://www.w3.org/2002/07/owl#TransitiveProperty"/>
        <rdfs:domain rdf:resource="http://www.w3.org/2006/time#TemporalEntity"/>
        <rdfs:range rdf:resource="http://www.w3.org/2006/time#TemporalEntity"/>
        <rdfs:comment xml:lang="en">Gives directionality to time. If a temporal entity T1 is before another temporal entity T2, then the end of T1 is before the beginning of T2. Thus, &quot;before&quot; can be considered to be basic to instants and derived for intervals.</rdfs:comment>
        <rdfs:label xml:lang="en">before</rdfs:label>
        <skos:definition xml:lang="en">Gives directionality to time. If a temporal entity T1 is before another temporal entity T2, then the end of T1 is before the beginning of T2. Thus, &quot;before&quot; can be considered to be basic to instants and derived for intervals.</skos:definition>
    </owl:ObjectProperty>
    


    <!-- http://www.w3.org/2006/time#dayOfWeek -->

    <owl:ObjectProperty rdf:about="http://www.w3.org/2006/time#dayOfWeek">
        <rdfs:domain rdf:resource="http://www.w3.org/2006/time#GeneralDateTimeDescription"/>
        <rdfs:range rdf:resource="http://www.w3.org/2006/time#DayOfWeek"/>
        <rdfs:comment xml:lang="en">The day of week, whose value is a member of the class time:DayOfWeek</rdfs:comment>
        <rdfs:label xml:lang="en">day of week</rdfs:label>
        <skos:definition xml:lang="en">The day of week, whose value is a member of the class time:DayOfWeek</skos:definition>
    </owl:ObjectProperty>
    


    <!-- http://www.w3.org/2006/time#hasBeginning -->

    <owl:ObjectProperty rdf:about="http://www.w3.org/2006/time#hasBeginning">
        <rdfs:subPropertyOf rdf:resource="http://www.w3.org/2006/time#hasTime"/>
        <rdfs:domain rdf:resource="http://www.w3.org/2006/time#TemporalEntity"/>
        <rdfs:range rdf:resource="http://www.w3.org/2006/time#Instant"/>
        <rdfs:comment xml:lang="en">Beginning of a temporal entity</rdfs:comment>
        <rdfs:comment>inclusive start of an owl-time:Interval</rdfs:comment>
        <rdfs:label xml:lang="en">has beginning</rdfs:label>
        <skos:definition xml:lang="en">Beginning of a temporal entity.</skos:definition>
    </owl:ObjectProperty>
    


    <!-- http://www.w3.org/2006/time#hasDateTimeDescription -->

    <owl:ObjectProperty rdf:about="http://www.w3.org/2006/time#hasDateTimeDescription">
        <rdfs:domain rdf:resource="http://www.w3.org/2006/time#DateTimeInterval"/>
        <rdfs:range rdf:resource="http://www.w3.org/2006/time#GeneralDateTimeDescription"/>
        <rdfs:comment xml:lang="en">Value of DateTimeInterval expressed as a structured value. The beginning and end of the interval coincide with the limits of the shortest element in the description.</rdfs:comment>
        <rdfs:label xml:lang="en">has Date-Time description</rdfs:label>
        <skos:definition xml:lang="en">Value of DateTimeInterval expressed as a structured value. The beginning and end of the interval coincide with the limits of the shortest element in the description.</skos:definition>
    </owl:ObjectProperty>
    


    <!-- http://www.w3.org/2006/time#hasDuration -->

    <owl:ObjectProperty rdf:about="http://www.w3.org/2006/time#hasDuration">
        <rdfs:subPropertyOf rdf:resource="http://www.w3.org/2006/time#hasTemporalDuration"/>
        <rdfs:range rdf:resource="http://www.w3.org/2006/time#Duration"/>
        <rdfs:comment xml:lang="en">Duration of a temporal entity, expressed as a scaled value or nominal value</rdfs:comment>
        <rdfs:label xml:lang="en">has duration</rdfs:label>
        <skos:definition xml:lang="en">Duration of a temporal entity, event or activity, or thing, expressed as a scaled value</skos:definition>
    </owl:ObjectProperty>
    


    <!-- http://www.w3.org/2006/time#hasDurationDescription -->

    <owl:ObjectProperty rdf:about="http://www.w3.org/2006/time#hasDurationDescription">
        <rdfs:subPropertyOf rdf:resource="http://www.w3.org/2006/time#hasTemporalDuration"/>
        <rdfs:range rdf:resource="http://www.w3.org/2006/time#GeneralDurationDescription"/>
        <rdfs:comment xml:lang="en">Duration of a temporal entity, expressed using a structured description</rdfs:comment>
        <rdfs:label xml:lang="en">has duration description</rdfs:label>
        <skos:definition xml:lang="en">Duration of a temporal entity, expressed using a structured description</skos:definition>
    </owl:ObjectProperty>
    


    <!-- http://www.w3.org/2006/time#hasEnd -->

    <owl:ObjectProperty rdf:about="http://www.w3.org/2006/time#hasEnd">
        <rdfs:subPropertyOf rdf:resource="http://www.w3.org/2006/time#hasTime"/>
        <rdfs:domain rdf:resource="http://www.w3.org/2006/time#TemporalEntity"/>
        <rdfs:range rdf:resource="http://www.w3.org/2006/time#Instant"/>
        <rdfs:comment xml:lang="en">End of a temporal entity.</rdfs:comment>
        <rdfs:label xml:lang="en">has end</rdfs:label>
        <skos:definition xml:lang="en">End of a temporal entity.</skos:definition>
    </owl:ObjectProperty>
    


    <!-- http://www.w3.org/2006/time#hasTRS -->

    <owl:ObjectProperty rdf:about="http://www.w3.org/2006/time#hasTRS">
        <rdf:type rdf:resource="http://www.w3.org/2002/07/owl#FunctionalProperty"/>
        <rdfs:domain>
            <owl:Class>
                <owl:unionOf rdf:parseType="Collection">
                    <rdf:Description rdf:about="http://www.w3.org/2006/time#GeneralDurationDescription"/>
                    <rdf:Description rdf:about="http://www.w3.org/2006/time#TemporalPosition"/>
                </owl:unionOf>
            </owl:Class>
        </rdfs:domain>
    </owl:ObjectProperty>
    


    <!-- http://www.w3.org/2006/time#hasTemporalDuration -->

    <owl:ObjectProperty rdf:about="http://www.w3.org/2006/time#hasTemporalDuration">
        <rdfs:domain rdf:resource="http://www.w3.org/2006/time#TemporalEntity"/>
        <rdfs:range rdf:resource="http://www.w3.org/2006/time#TemporalDuration"/>
        <rdfs:comment xml:lang="en">Duration of a temporal entity.</rdfs:comment>
        <rdfs:label xml:lang="en">has temporal duration</rdfs:label>
        <skos:definition xml:lang="en">Duration of a temporal entity.</skos:definition>
    </owl:ObjectProperty>
    


    <!-- http://www.w3.org/2006/time#hasTime -->

    <owl:ObjectProperty rdf:about="http://www.w3.org/2006/time#hasTime">
        <rdfs:range rdf:resource="http://www.w3.org/2006/time#TemporalEntity"/>
        <rdfs:comment xml:lang="en">Supports the association of a temporal entity (instant or interval) to any thing</rdfs:comment>
        <rdfs:label xml:lang="en">has time</rdfs:label>
        <skos:definition xml:lang="en">Supports the association of a temporal entity (instant or interval) to any thing</skos:definition>
        <skos:editorialNote xml:lang="en">Feature at risk - added in 2017 revision, and not yet widely used. </skos:editorialNote>
    </owl:ObjectProperty>
    


    <!-- http://www.w3.org/2006/time#inDateTime -->

    <owl:ObjectProperty rdf:about="http://www.w3.org/2006/time#inDateTime">
        <rdfs:subPropertyOf rdf:resource="http://www.w3.org/2006/time#inTemporalPosition"/>
        <rdfs:domain rdf:resource="http://www.w3.org/2006/time#Instant"/>
        <rdfs:range rdf:resource="http://www.w3.org/2006/time#GeneralDateTimeDescription"/>
        <rdfs:comment xml:lang="en">Position of an instant, expressed using a structured description</rdfs:comment>
        <rdfs:label xml:lang="en">in date-time description</rdfs:label>
        <skos:definition xml:lang="en">Position of an instant, expressed using a structured description</skos:definition>
    </owl:ObjectProperty>
    


    <!-- http://www.w3.org/2006/time#inTemporalPosition -->

    <owl:ObjectProperty rdf:about="http://www.w3.org/2006/time#inTemporalPosition">
        <rdfs:domain rdf:resource="http://www.w3.org/2006/time#Instant"/>
        <rdfs:range rdf:resource="http://www.w3.org/2006/time#TemporalPosition"/>
        <rdfs:comment xml:lang="en">Position of a time instant</rdfs:comment>
        <rdfs:label xml:lang="en">Temporal position</rdfs:label>
        <skos:definition xml:lang="en">Position of a time instant</skos:definition>
    </owl:ObjectProperty>
    


    <!-- http://www.w3.org/2006/time#inTimePosition -->

    <owl:ObjectProperty rdf:about="http://www.w3.org/2006/time#inTimePosition">
        <rdfs:subPropertyOf rdf:resource="http://www.w3.org/2006/time#inTemporalPosition"/>
        <rdfs:domain rdf:resource="http://www.w3.org/2006/time#Instant"/>
        <rdfs:range rdf:resource="http://www.w3.org/2006/time#TimePosition"/>
        <rdfs:comment xml:lang="en">Position of an instant, expressed as a temporal coordinate or nominal value</rdfs:comment>
        <rdfs:label xml:lang="en">Time position</rdfs:label>
        <skos:definition xml:lang="en">Position of a time instant expressed as a TimePosition</skos:definition>
    </owl:ObjectProperty>
    


    <!-- http://www.w3.org/2006/time#inside -->

    <owl:ObjectProperty rdf:about="http://www.w3.org/2006/time#inside">
        <rdfs:domain rdf:resource="http://www.w3.org/2006/time#Interval"/>
        <rdfs:range rdf:resource="http://www.w3.org/2006/time#Instant"/>
        <rdfs:comment xml:lang="en">An instant that falls inside the interval. It is not intended to include beginnings and ends of intervals.</rdfs:comment>
        <rdfs:label xml:lang="en">has time instant inside</rdfs:label>
        <skos:definition xml:lang="en">An instant that falls inside the interval. It is not intended to include beginnings and ends of intervals.</skos:definition>
    </owl:ObjectProperty>
    


    <!-- http://www.w3.org/2006/time#intervalAfter -->

    <owl:ObjectProperty rdf:about="http://www.w3.org/2006/time#intervalAfter">
        <rdfs:subPropertyOf rdf:resource="http://www.w3.org/2006/time#after"/>
        <rdfs:subPropertyOf rdf:resource="http://www.w3.org/2006/time#intervalDisjoint"/>
        <owl:inverseOf rdf:resource="http://www.w3.org/2006/time#intervalBefore"/>
        <rdfs:domain rdf:resource="http://www.w3.org/2006/time#ProperInterval"/>
        <rdfs:range rdf:resource="http://www.w3.org/2006/time#ProperInterval"/>
        <rdfs:comment xml:lang="en">If a proper interval T1 is intervalAfter another proper interval T2, then the beginning of T1 is after the end of T2.</rdfs:comment>
        <rdfs:comment>shows that one instance of owl-time:Interval ends before another owl-time:Interval starts </rdfs:comment>
        <rdfs:label xml:lang="en">interval after</rdfs:label>
        <skos:definition xml:lang="en">If a proper interval T1 is intervalAfter another proper interval T2, then the beginning of T1 is after the end of T2.</skos:definition>
    </owl:ObjectProperty>
    


    <!-- http://www.w3.org/2006/time#intervalBefore -->

    <owl:ObjectProperty rdf:about="http://www.w3.org/2006/time#intervalBefore">
        <rdfs:subPropertyOf rdf:resource="http://www.w3.org/2006/time#before"/>
        <rdfs:subPropertyOf rdf:resource="http://www.w3.org/2006/time#intervalDisjoint"/>
        <rdfs:domain rdf:resource="http://www.w3.org/2006/time#ProperInterval"/>
        <rdfs:range rdf:resource="http://www.w3.org/2006/time#ProperInterval"/>
        <rdfs:comment xml:lang="en">If a proper interval T1 is intervalBefore another proper interval T2, then the end of T1 is before the beginning of T2.</rdfs:comment>
        <rdfs:label xml:lang="en">interval before</rdfs:label>
        <skos:definition xml:lang="en">If a proper interval T1 is intervalBefore another proper interval T2, then the end of T1 is before the beginning of T2.</skos:definition>
    </owl:ObjectProperty>
    


    <!-- http://www.w3.org/2006/time#intervalContains -->

    <owl:ObjectProperty rdf:about="http://www.w3.org/2006/time#intervalContains">
        <owl:inverseOf rdf:resource="http://www.w3.org/2006/time#intervalDuring"/>
        <rdfs:domain rdf:resource="http://www.w3.org/2006/time#ProperInterval"/>
        <rdfs:range rdf:resource="http://www.w3.org/2006/time#ProperInterval"/>
        <rdfs:comment xml:lang="en">If a proper interval T1 is intervalContains another proper interval T2, then the beginning of T1 is before the beginning of T2, and the end of T1 is after the end of T2.</rdfs:comment>
        <rdfs:label xml:lang="en">interval contains</rdfs:label>
        <skos:definition xml:lang="en">If a proper interval T1 is intervalContains another proper interval T2, then the beginning of T1 is before the beginning of T2, and the end of T1 is after the end of T2.</skos:definition>
    </owl:ObjectProperty>
    


    <!-- http://www.w3.org/2006/time#intervalDisjoint -->

    <owl:ObjectProperty rdf:about="http://www.w3.org/2006/time#intervalDisjoint">
        <rdfs:domain rdf:resource="http://www.w3.org/2006/time#ProperInterval"/>
        <rdfs:range rdf:resource="http://www.w3.org/2006/time#ProperInterval"/>
        <rdfs:comment xml:lang="en">If a proper interval T1 is intervalDisjoint another proper interval T2, then the beginning of T1 is after the end of T2, or the end of T1 is before the beginning of T2, i.e. the intervals do not overlap in any way, but their ordering relationship is not known.</rdfs:comment>
        <rdfs:label xml:lang="en">interval disjoint</rdfs:label>
        <skos:definition xml:lang="en">If a proper interval T1 is intervalDisjoint another proper interval T2, then the beginning of T1 is after the end of T2, or the end of T1 is before the beginning of T2, i.e. the intervals do not overlap in any way, but their ordering relationship is not known.</skos:definition>
        <skos:note xml:lang="en">This interval relation is not included in the 13 basic relationships defined in Allen (1984), but is defined in (T.3) as the union of :intervalDuring v :intervalStarts v :intervalFinishes</skos:note>
    </owl:ObjectProperty>
    


    <!-- http://www.w3.org/2006/time#intervalDuring -->

    <owl:ObjectProperty rdf:about="http://www.w3.org/2006/time#intervalDuring">
        <rdfs:subPropertyOf rdf:resource="http://www.w3.org/2006/time#intervalIn"/>
        <rdfs:domain rdf:resource="http://www.w3.org/2006/time#ProperInterval"/>
        <rdfs:range rdf:resource="http://www.w3.org/2006/time#ProperInterval"/>
        <rdfs:comment xml:lang="en">If a proper interval T1 is intervalDuring another proper interval T2, then the beginning of T1 is after the beginning of T2, and the end of T1 is before the end of T2.</rdfs:comment>
        <rdfs:label xml:lang="en">interval during</rdfs:label>
        <skos:definition xml:lang="en">If a proper interval T1 is intervalDuring another proper interval T2, then the beginning of T1 is after the beginning of T2, and the end of T1 is before the end of T2.</skos:definition>
    </owl:ObjectProperty>
    


    <!-- http://www.w3.org/2006/time#intervalEquals -->

    <owl:ObjectProperty rdf:about="http://www.w3.org/2006/time#intervalEquals">
        <rdfs:domain rdf:resource="http://www.w3.org/2006/time#ProperInterval"/>
        <rdfs:range rdf:resource="http://www.w3.org/2006/time#ProperInterval"/>
        <owl:propertyDisjointWith rdf:resource="http://www.w3.org/2006/time#intervalIn"/>
        <rdfs:comment xml:lang="en">If a proper interval T1 is intervalEquals another proper interval T2, then the beginning of T1 is coincident with the beginning of T2, and the end of T1 is coincident with the end of T2.</rdfs:comment>
        <rdfs:label xml:lang="en">interval equals</rdfs:label>
        <skos:definition xml:lang="en">If a proper interval T1 is intervalEquals another proper interval T2, then the beginning of T1 is coincident with the beginning of T2, and the end of T1 is coincident with the end of T2.</skos:definition>
    </owl:ObjectProperty>
    


    <!-- http://www.w3.org/2006/time#intervalFinishedBy -->

    <owl:ObjectProperty rdf:about="http://www.w3.org/2006/time#intervalFinishedBy">
        <owl:inverseOf rdf:resource="http://www.w3.org/2006/time#intervalFinishes"/>
        <rdfs:domain rdf:resource="http://www.w3.org/2006/time#ProperInterval"/>
        <rdfs:range rdf:resource="http://www.w3.org/2006/time#ProperInterval"/>
        <rdfs:comment xml:lang="en">If a proper interval T1 is intervalFinishedBy another proper interval T2, then the beginning of T1 is before the beginning of T2, and the end of T1 is coincident with the end of T2.</rdfs:comment>
        <rdfs:label xml:lang="en">interval finished by</rdfs:label>
        <skos:definition xml:lang="en">If a proper interval T1 is intervalFinishedBy another proper interval T2, then the beginning of T1 is before the beginning of T2, and the end of T1 is coincident with the end of T2.</skos:definition>
    </owl:ObjectProperty>
    


    <!-- http://www.w3.org/2006/time#intervalFinishes -->

    <owl:ObjectProperty rdf:about="http://www.w3.org/2006/time#intervalFinishes">
        <rdfs:subPropertyOf rdf:resource="http://www.w3.org/2006/time#intervalIn"/>
        <rdfs:domain rdf:resource="http://www.w3.org/2006/time#ProperInterval"/>
        <rdfs:range rdf:resource="http://www.w3.org/2006/time#ProperInterval"/>
        <rdfs:comment xml:lang="en">If a proper interval T1 is intervalFinishes another proper interval T2, then the beginning of T1 is after the beginning of T2, and the end of T1 is coincident with the end of T2.</rdfs:comment>
        <rdfs:label xml:lang="en">interval finishes</rdfs:label>
        <skos:definition xml:lang="en">If a proper interval T1 is intervalFinishes another proper interval T2, then the beginning of T1 is after the beginning of T2, and the end of T1 is coincident with the end of T2.</skos:definition>
    </owl:ObjectProperty>
    


    <!-- http://www.w3.org/2006/time#intervalIn -->

    <owl:ObjectProperty rdf:about="http://www.w3.org/2006/time#intervalIn">
        <rdfs:domain rdf:resource="http://www.w3.org/2006/time#ProperInterval"/>
        <rdfs:range rdf:resource="http://www.w3.org/2006/time#ProperInterval"/>
        <rdfs:comment xml:lang="en">If a proper interval T1 is intervalIn another proper interval T2, then the beginning of T1 is after the beginning of T2 or is coincident with the beginning of T2, and the end of T1 is before the end of T2, or is coincident with the end of T2, except that end of T1 may not be coincident with the end of T2 if the beginning of T1 is coincident with the beginning of T2.</rdfs:comment>
        <rdfs:label xml:lang="en">interval in</rdfs:label>
        <skos:definition xml:lang="en">If a proper interval T1 is intervalIn another proper interval T2, then the beginning of T1 is after the beginning of T2 or is coincident with the beginning of T2, and the end of T1 is before the end of T2, or is coincident with the end of T2, except that end of T1 may not be coincident with the end of T2 if the beginning of T1 is coincident with the beginning of T2.</skos:definition>
        <skos:note xml:lang="en">This interval relation is not included in the 13 basic relationships defined in Allen (1984), but is referred to as &apos;an important relationship&apos; in Allen and Ferguson (1997). It is the disjoint union of :intervalStarts v :intervalDuring v :intervalFinishes</skos:note>
    </owl:ObjectProperty>
    


    <!-- http://www.w3.org/2006/time#intervalMeets -->

    <owl:ObjectProperty rdf:about="http://www.w3.org/2006/time#intervalMeets">
        <owl:inverseOf rdf:resource="http://www.w3.org/2006/time#intervalMetBy"/>
        <rdfs:domain rdf:resource="http://www.w3.org/2006/time#ProperInterval"/>
        <rdfs:range rdf:resource="http://www.w3.org/2006/time#ProperInterval"/>
        <rdfs:comment xml:lang="en">If a proper interval T1 is intervalMeets another proper interval T2, then the end of T1 is coincident with the beginning of T2.</rdfs:comment>
        <rdfs:label xml:lang="en">interval meets</rdfs:label>
        <skos:definition xml:lang="en">If a proper interval T1 is intervalMeets another proper interval T2, then the end of T1 is coincident with the beginning of T2.</skos:definition>
    </owl:ObjectProperty>
    


    <!-- http://www.w3.org/2006/time#intervalMetBy -->

    <owl:ObjectProperty rdf:about="http://www.w3.org/2006/time#intervalMetBy">
        <rdfs:domain rdf:resource="http://www.w3.org/2006/time#ProperInterval"/>
        <rdfs:range rdf:resource="http://www.w3.org/2006/time#ProperInterval"/>
        <rdfs:comment xml:lang="en">If a proper interval T1 is intervalMetBy another proper interval T2, then the beginning of T1 is coincident with the end of T2.</rdfs:comment>
        <rdfs:label xml:lang="en">interval met by</rdfs:label>
        <skos:definition xml:lang="en">If a proper interval T1 is intervalMetBy another proper interval T2, then the beginning of T1 is coincident with the end of T2.</skos:definition>
    </owl:ObjectProperty>
    


    <!-- http://www.w3.org/2006/time#intervalOverlappedBy -->

    <owl:ObjectProperty rdf:about="http://www.w3.org/2006/time#intervalOverlappedBy">
        <owl:inverseOf rdf:resource="http://www.w3.org/2006/time#intervalOverlaps"/>
        <rdfs:domain rdf:resource="http://www.w3.org/2006/time#ProperInterval"/>
        <rdfs:range rdf:resource="http://www.w3.org/2006/time#ProperInterval"/>
        <rdfs:comment xml:lang="en">If a proper interval T1 is intervalOverlappedBy another proper interval T2, then the beginning of T1 is after the beginning of T2, the beginning of T1 is before the end of T2, and the end of T1 is after the end of T2.</rdfs:comment>
        <rdfs:label xml:lang="en">interval overlapped by</rdfs:label>
        <skos:definition xml:lang="en">If a proper interval T1 is intervalOverlappedBy another proper interval T2, then the beginning of T1 is after the beginning of T2, the beginning of T1 is before the end of T2, and the end of T1 is after the end of T2.</skos:definition>
    </owl:ObjectProperty>
    


    <!-- http://www.w3.org/2006/time#intervalOverlaps -->

    <owl:ObjectProperty rdf:about="http://www.w3.org/2006/time#intervalOverlaps">
        <rdfs:domain rdf:resource="http://www.w3.org/2006/time#ProperInterval"/>
        <rdfs:range rdf:resource="http://www.w3.org/2006/time#ProperInterval"/>
        <rdfs:comment xml:lang="en">If a proper interval T1 is intervalOverlaps another proper interval T2, then the beginning of T1 is before the beginning of T2, the end of T1 is after the beginning of T2, and the end of T1 is before the end of T2.</rdfs:comment>
        <rdfs:label xml:lang="en">interval overlaps</rdfs:label>
        <skos:definition xml:lang="en">If a proper interval T1 is intervalOverlaps another proper interval T2, then the beginning of T1 is before the beginning of T2, the end of T1 is after the beginning of T2, and the end of T1 is before the end of T2.</skos:definition>
    </owl:ObjectProperty>
    


    <!-- http://www.w3.org/2006/time#intervalStartedBy -->

    <owl:ObjectProperty rdf:about="http://www.w3.org/2006/time#intervalStartedBy">
        <owl:inverseOf rdf:resource="http://www.w3.org/2006/time#intervalStarts"/>
        <rdfs:domain rdf:resource="http://www.w3.org/2006/time#ProperInterval"/>
        <rdfs:range rdf:resource="http://www.w3.org/2006/time#ProperInterval"/>
        <rdfs:comment xml:lang="en">If a proper interval T1 is intervalStarted another proper interval T2, then the beginning of T1 is coincident with the beginning of T2, and the end of T1 is after the end of T2.</rdfs:comment>
        <rdfs:label xml:lang="en">interval started by</rdfs:label>
        <skos:definition xml:lang="en">If a proper interval T1 is intervalStarted another proper interval T2, then the beginning of T1 is coincident with the beginning of T2, and the end of T1 is after the end of T2.</skos:definition>
    </owl:ObjectProperty>
    


    <!-- http://www.w3.org/2006/time#intervalStarts -->

    <owl:ObjectProperty rdf:about="http://www.w3.org/2006/time#intervalStarts">
        <rdfs:subPropertyOf rdf:resource="http://www.w3.org/2006/time#intervalIn"/>
        <rdfs:domain rdf:resource="http://www.w3.org/2006/time#ProperInterval"/>
        <rdfs:range rdf:resource="http://www.w3.org/2006/time#ProperInterval"/>
        <rdfs:comment xml:lang="en">If a proper interval T1 is intervalStarts another proper interval T2, then the beginning of T1 is coincident with the beginning of T2, and the end of T1 is before the end of T2.</rdfs:comment>
        <rdfs:label xml:lang="en">interval starts</rdfs:label>
        <skos:definition xml:lang="en">If a proper interval T1 is intervalStarts another proper interval T2, then the beginning of T1 is coincident with the beginning of T2, and the end of T1 is before the end of T2.</skos:definition>
    </owl:ObjectProperty>
    


    <!-- http://www.w3.org/2006/time#monthOfYear -->

    <owl:ObjectProperty rdf:about="http://www.w3.org/2006/time#monthOfYear">
        <rdfs:domain rdf:resource="http://www.w3.org/2006/time#GeneralDateTimeDescription"/>
        <rdfs:range rdf:resource="http://www.w3.org/2006/time#MonthOfYear"/>
        <rdfs:comment xml:lang="en">The month of the year, whose value is a member of the class time:MonthOfYear</rdfs:comment>
        <rdfs:label xml:lang="en">month of year</rdfs:label>
        <skos:definition xml:lang="en">The month of the year, whose value is a member of the class time:MonthOfYear</skos:definition>
        <skos:editorialNote xml:lang="en">Feature at risk - added in 2017 revision, and not yet widely used. </skos:editorialNote>
    </owl:ObjectProperty>
    


    <!-- http://www.w3.org/2006/time#timeZone -->

    <owl:ObjectProperty rdf:about="http://www.w3.org/2006/time#timeZone">
        <rdfs:domain rdf:resource="http://www.w3.org/2006/time#GeneralDateTimeDescription"/>
        <rdfs:domain rdf:resource="http://www.w3.org/2006/time#TemporalEntity"/>
        <rdfs:range rdf:resource="http://www.w3.org/2006/time#TimeZone"/>
        <rdfs:range rdf:resource="http://www.w3.org/2006/timezone#TimeZone"/>
        <rdfs:comment xml:lang="en">The time zone for clock elements in the temporal position</rdfs:comment>
        <rdfs:label xml:lang="en">in time zone</rdfs:label>
        <skos:historyNote>In the original 2006 version of OWL-Time, the range of time:timeZone was a TimeZone class in a separate namespace &quot;http://www.w3.org/2006/timezone#&quot;. 
An alignment axiom 
	tzont:TimeZone rdfs:subClassOf time:TimeZone . 
allows data encoded according to the previous version to be consistent with the updated ontology. </skos:historyNote>
        <skos:note>IANA maintains a database of timezones. These are well maintained and generally considered authoritative, but individual items are not available at individual URIs, so cannot be used directly in data expressed using OWL-Time.

DBPedia provides a set of resources corresponding to the IANA timezones, with a URI for each (e.g. http://dbpedia.org/resource/Australia/Eucla). The World Clock service also provides a list of time zones with the description of each available as an individual webpage with a convenient individual URI (e.g. https://www.timeanddate.com/time/zones/acwst). These or other, similar, resources might be used as a value of the time:timeZone property.</skos:note>
    </owl:ObjectProperty>
    


    <!-- http://www.w3.org/2006/time#unitType -->

    <owl:ObjectProperty rdf:about="http://www.w3.org/2006/time#unitType">
        <rdfs:domain>
            <owl:Class>
                <owl:unionOf rdf:parseType="Collection">
                    <rdf:Description rdf:about="http://www.w3.org/2006/time#Duration"/>
                    <rdf:Description rdf:about="http://www.w3.org/2006/time#GeneralDateTimeDescription"/>
                </owl:unionOf>
            </owl:Class>
        </rdfs:domain>
    </owl:ObjectProperty>
    


    <!-- http://www.w3.org/2006/vcard/ns#adr -->

    <owl:ObjectProperty rdf:about="http://www.w3.org/2006/vcard/ns#adr">
        <owl:equivalentProperty rdf:resource="http://www.w3.org/2006/vcard/ns#hasAddress"/>
        <rdfs:comment xml:lang="en">This object property has been mapped</rdfs:comment>
        <rdfs:isDefinedBy rdf:resource="http://www.w3.org/2006/vcard/ns"/>
        <rdfs:label xml:lang="en">address</rdfs:label>
    </owl:ObjectProperty>
    


    <!-- http://www.w3.org/2006/vcard/ns#agent -->

    <owl:ObjectProperty rdf:about="http://www.w3.org/2006/vcard/ns#agent">
        <rdfs:comment xml:lang="en">This object property has been deprecated</rdfs:comment>
        <rdfs:isDefinedBy rdf:resource="http://www.w3.org/2006/vcard/ns"/>
        <rdfs:label xml:lang="en">agent</rdfs:label>
        <owl:deprecated rdf:datatype="http://www.w3.org/2001/XMLSchema#boolean">true</owl:deprecated>
    </owl:ObjectProperty>
    


    <!-- http://www.w3.org/2006/vcard/ns#email -->

    <owl:ObjectProperty rdf:about="http://www.w3.org/2006/vcard/ns#email">
        <owl:equivalentProperty rdf:resource="http://www.w3.org/2006/vcard/ns#hasEmail"/>
        <rdfs:comment xml:lang="en">This object property has been mapped</rdfs:comment>
        <rdfs:isDefinedBy rdf:resource="http://www.w3.org/2006/vcard/ns"/>
        <rdfs:label xml:lang="en">email</rdfs:label>
    </owl:ObjectProperty>
    


    <!-- http://www.w3.org/2006/vcard/ns#geo -->

    <owl:ObjectProperty rdf:about="http://www.w3.org/2006/vcard/ns#geo">
        <owl:equivalentProperty rdf:resource="http://www.w3.org/2006/vcard/ns#hasGeo"/>
        <rdfs:comment xml:lang="en">This object property has been mapped</rdfs:comment>
        <rdfs:isDefinedBy rdf:resource="http://www.w3.org/2006/vcard/ns"/>
        <rdfs:label xml:lang="en">geo</rdfs:label>
    </owl:ObjectProperty>
    


    <!-- http://www.w3.org/2006/vcard/ns#hasAdditionalName -->

    <owl:ObjectProperty rdf:about="http://www.w3.org/2006/vcard/ns#hasAdditionalName">
        <rdfs:comment xml:lang="en">Used to support property parameters for the additional name data property</rdfs:comment>
        <rdfs:isDefinedBy rdf:resource="http://www.w3.org/2006/vcard/ns"/>
        <rdfs:label xml:lang="en">has additional name</rdfs:label>
    </owl:ObjectProperty>
    


    <!-- http://www.w3.org/2006/vcard/ns#hasAddress -->

    <owl:ObjectProperty rdf:about="http://www.w3.org/2006/vcard/ns#hasAddress">
        <rdfs:subPropertyOf rdf:resource="http://www.w3.org/2003/01/geo/wgs84_pos#location"/>
        <rdfs:domain rdf:resource="http://purl.oclc.org/NET/ssnx/ssn#System"/>
        <rdfs:range rdf:resource="http://www.w3.org/2006/vcard/ns#Address"/>
        <rdfs:comment xml:lang="en">To specify the components of the delivery address for the object</rdfs:comment>
        <rdfs:isDefinedBy rdf:resource="http://www.w3.org/2006/vcard/ns"/>
        <rdfs:label xml:lang="en">has address</rdfs:label>
    </owl:ObjectProperty>
    


    <!-- http://www.w3.org/2006/vcard/ns#hasCalendarBusy -->

    <owl:ObjectProperty rdf:about="http://www.w3.org/2006/vcard/ns#hasCalendarBusy">
        <rdfs:comment xml:lang="en">To specify the busy time associated with the object. (Was called FBURL in RFC6350)</rdfs:comment>
        <rdfs:isDefinedBy rdf:resource="http://www.w3.org/2006/vcard/ns"/>
        <rdfs:label xml:lang="en">has calendar busy</rdfs:label>
    </owl:ObjectProperty>
    


    <!-- http://www.w3.org/2006/vcard/ns#hasCalendarLink -->

    <owl:ObjectProperty rdf:about="http://www.w3.org/2006/vcard/ns#hasCalendarLink">
        <rdfs:comment xml:lang="en">To specify the calendar associated with the object. (Was called CALURI in RFC6350)</rdfs:comment>
        <rdfs:isDefinedBy rdf:resource="http://www.w3.org/2006/vcard/ns"/>
        <rdfs:label xml:lang="en">has calendar link</rdfs:label>
    </owl:ObjectProperty>
    


    <!-- http://www.w3.org/2006/vcard/ns#hasCalendarRequest -->

    <owl:ObjectProperty rdf:about="http://www.w3.org/2006/vcard/ns#hasCalendarRequest">
        <rdfs:comment xml:lang="en">To specify the calendar user address to which a scheduling request be sent for the object. (Was called CALADRURI in RFC6350)</rdfs:comment>
        <rdfs:isDefinedBy rdf:resource="http://www.w3.org/2006/vcard/ns"/>
        <rdfs:label xml:lang="en">has calendar request</rdfs:label>
    </owl:ObjectProperty>
    


    <!-- http://www.w3.org/2006/vcard/ns#hasCategory -->

    <owl:ObjectProperty rdf:about="http://www.w3.org/2006/vcard/ns#hasCategory">
        <rdfs:comment xml:lang="en">Used to support property parameters for the category data property</rdfs:comment>
        <rdfs:isDefinedBy rdf:resource="http://www.w3.org/2006/vcard/ns"/>
        <rdfs:label xml:lang="en">has category</rdfs:label>
    </owl:ObjectProperty>
    


    <!-- http://www.w3.org/2006/vcard/ns#hasCountryName -->

    <owl:ObjectProperty rdf:about="http://www.w3.org/2006/vcard/ns#hasCountryName">
        <rdfs:comment xml:lang="en">Used to support property parameters for the country name data property</rdfs:comment>
        <rdfs:isDefinedBy rdf:resource="http://www.w3.org/2006/vcard/ns"/>
        <rdfs:label xml:lang="en">has country name</rdfs:label>
    </owl:ObjectProperty>
    


    <!-- http://www.w3.org/2006/vcard/ns#hasEmail -->

    <owl:ObjectProperty rdf:about="http://www.w3.org/2006/vcard/ns#hasEmail">
        <rdfs:range rdf:resource="http://www.w3.org/2006/vcard/ns#Email"/>
        <rdfs:comment xml:lang="en">To specify the electronic mail address for communication with the object</rdfs:comment>
        <rdfs:isDefinedBy rdf:resource="http://www.w3.org/2006/vcard/ns"/>
        <rdfs:label xml:lang="en">has email</rdfs:label>
    </owl:ObjectProperty>
    


    <!-- http://www.w3.org/2006/vcard/ns#hasFN -->

    <owl:ObjectProperty rdf:about="http://www.w3.org/2006/vcard/ns#hasFN">
        <rdfs:comment xml:lang="en">Used to support property parameters for the formatted name data property</rdfs:comment>
        <rdfs:isDefinedBy rdf:resource="http://www.w3.org/2006/vcard/ns"/>
        <rdfs:label xml:lang="en">has formatted name</rdfs:label>
    </owl:ObjectProperty>
    


    <!-- http://www.w3.org/2006/vcard/ns#hasFamilyName -->

    <owl:ObjectProperty rdf:about="http://www.w3.org/2006/vcard/ns#hasFamilyName">
        <rdfs:comment xml:lang="en">Used to support property parameters for the family name data property</rdfs:comment>
        <rdfs:isDefinedBy rdf:resource="http://www.w3.org/2006/vcard/ns"/>
        <rdfs:label xml:lang="en">has family name</rdfs:label>
    </owl:ObjectProperty>
    


    <!-- http://www.w3.org/2006/vcard/ns#hasGender -->

    <owl:ObjectProperty rdf:about="http://www.w3.org/2006/vcard/ns#hasGender">
        <rdfs:comment xml:lang="en">To specify  the sex or gender identity of the object. URIs are recommended to enable interoperable sex and gender codes to be used.</rdfs:comment>
        <rdfs:isDefinedBy rdf:resource="http://www.w3.org/2006/vcard/ns"/>
        <rdfs:label xml:lang="en">has gender</rdfs:label>
    </owl:ObjectProperty>
    


    <!-- http://www.w3.org/2006/vcard/ns#hasGeo -->

    <owl:ObjectProperty rdf:about="http://www.w3.org/2006/vcard/ns#hasGeo">
        <rdfs:comment xml:lang="en">To specify information related to the global positioning of the object. May also be used as a property parameter.</rdfs:comment>
        <rdfs:isDefinedBy rdf:resource="http://www.w3.org/2006/vcard/ns"/>
        <rdfs:label xml:lang="en">has geo</rdfs:label>
    </owl:ObjectProperty>
    


    <!-- http://www.w3.org/2006/vcard/ns#hasGivenName -->

    <owl:ObjectProperty rdf:about="http://www.w3.org/2006/vcard/ns#hasGivenName">
        <rdfs:comment xml:lang="en">Used to support property parameters for the given name data property</rdfs:comment>
        <rdfs:isDefinedBy rdf:resource="http://www.w3.org/2006/vcard/ns"/>
        <rdfs:label xml:lang="en">has given name</rdfs:label>
    </owl:ObjectProperty>
    


    <!-- http://www.w3.org/2006/vcard/ns#hasHonorificPrefix -->

    <owl:ObjectProperty rdf:about="http://www.w3.org/2006/vcard/ns#hasHonorificPrefix">
        <rdfs:comment xml:lang="en">Used to support property parameters for the honorific prefix data property</rdfs:comment>
        <rdfs:isDefinedBy rdf:resource="http://www.w3.org/2006/vcard/ns"/>
        <rdfs:label xml:lang="en">has honorific prefix</rdfs:label>
    </owl:ObjectProperty>
    


    <!-- http://www.w3.org/2006/vcard/ns#hasHonorificSuffix -->

    <owl:ObjectProperty rdf:about="http://www.w3.org/2006/vcard/ns#hasHonorificSuffix">
        <rdfs:comment xml:lang="en">Used to support property parameters for the honorific suffix data property</rdfs:comment>
        <rdfs:isDefinedBy rdf:resource="http://www.w3.org/2006/vcard/ns"/>
        <rdfs:label xml:lang="en">has honorific suffix</rdfs:label>
    </owl:ObjectProperty>
    


    <!-- http://www.w3.org/2006/vcard/ns#hasInstantMessage -->

    <owl:ObjectProperty rdf:about="http://www.w3.org/2006/vcard/ns#hasInstantMessage">
        <rdfs:comment xml:lang="en">To specify the instant messaging and presence protocol communications with the object. (Was called IMPP in RFC6350)</rdfs:comment>
        <rdfs:isDefinedBy rdf:resource="http://www.w3.org/2006/vcard/ns"/>
        <rdfs:label xml:lang="en">has messaging</rdfs:label>
    </owl:ObjectProperty>
    


    <!-- http://www.w3.org/2006/vcard/ns#hasKey -->

    <owl:ObjectProperty rdf:about="http://www.w3.org/2006/vcard/ns#hasKey">
        <owl:equivalentProperty rdf:resource="http://www.w3.org/2006/vcard/ns#key"/>
        <rdfs:comment xml:lang="en">To specify a public key or authentication certificate associated with the object</rdfs:comment>
        <rdfs:isDefinedBy rdf:resource="http://www.w3.org/2006/vcard/ns"/>
        <rdfs:label xml:lang="en">has key</rdfs:label>
    </owl:ObjectProperty>
    


    <!-- http://www.w3.org/2006/vcard/ns#hasLanguage -->

    <owl:ObjectProperty rdf:about="http://www.w3.org/2006/vcard/ns#hasLanguage">
        <rdfs:comment xml:lang="en">Used to support property parameters for the language data property</rdfs:comment>
        <rdfs:isDefinedBy rdf:resource="http://www.w3.org/2006/vcard/ns"/>
        <rdfs:label xml:lang="en">has language</rdfs:label>
    </owl:ObjectProperty>
    


    <!-- http://www.w3.org/2006/vcard/ns#hasLocality -->

    <owl:ObjectProperty rdf:about="http://www.w3.org/2006/vcard/ns#hasLocality">
        <rdfs:comment xml:lang="en">Used to support property parameters for the locality data property</rdfs:comment>
        <rdfs:isDefinedBy rdf:resource="http://www.w3.org/2006/vcard/ns"/>
        <rdfs:label xml:lang="en">has locality</rdfs:label>
    </owl:ObjectProperty>
    


    <!-- http://www.w3.org/2006/vcard/ns#hasLogo -->

    <owl:ObjectProperty rdf:about="http://www.w3.org/2006/vcard/ns#hasLogo">
        <owl:equivalentProperty rdf:resource="http://www.w3.org/2006/vcard/ns#logo"/>
        <rdfs:comment xml:lang="en">To specify a graphic image of a logo associated with the object </rdfs:comment>
        <rdfs:isDefinedBy rdf:resource="http://www.w3.org/2006/vcard/ns"/>
        <rdfs:label xml:lang="en">has logo</rdfs:label>
    </owl:ObjectProperty>
    


    <!-- http://www.w3.org/2006/vcard/ns#hasMember -->

    <owl:ObjectProperty rdf:about="http://www.w3.org/2006/vcard/ns#hasMember">
        <rdfs:domain rdf:resource="http://www.w3.org/2006/vcard/ns#Group"/>
        <rdfs:range rdf:resource="http://www.w3.org/2006/vcard/ns#Kind"/>
        <rdfs:comment xml:lang="en">To include a member in the group this object represents. (This property can only be used by Group individuals)</rdfs:comment>
        <rdfs:isDefinedBy rdf:resource="http://www.w3.org/2006/vcard/ns"/>
        <rdfs:label xml:lang="en">has member</rdfs:label>
    </owl:ObjectProperty>
    


    <!-- http://www.w3.org/2006/vcard/ns#hasName -->

    <owl:ObjectProperty rdf:about="http://www.w3.org/2006/vcard/ns#hasName">
        <owl:equivalentProperty rdf:resource="http://www.w3.org/2006/vcard/ns#n"/>
        <rdfs:range rdf:resource="http://www.w3.org/2006/vcard/ns#Name"/>
        <rdfs:comment xml:lang="en">To specify the components of the name of the object</rdfs:comment>
        <rdfs:isDefinedBy rdf:resource="http://www.w3.org/2006/vcard/ns"/>
        <rdfs:label xml:lang="en">has name</rdfs:label>
    </owl:ObjectProperty>
    


    <!-- http://www.w3.org/2006/vcard/ns#hasNickname -->

    <owl:ObjectProperty rdf:about="http://www.w3.org/2006/vcard/ns#hasNickname">
        <rdfs:comment xml:lang="en">Used to support property parameters for the nickname data property</rdfs:comment>
        <rdfs:isDefinedBy rdf:resource="http://www.w3.org/2006/vcard/ns"/>
        <rdfs:label xml:lang="en">has nickname</rdfs:label>
        <rdfs:seeAlso rdf:resource="http://www.w3.org/2006/vcard/ns#nickname"/>
    </owl:ObjectProperty>
    


    <!-- http://www.w3.org/2006/vcard/ns#hasNote -->

    <owl:ObjectProperty rdf:about="http://www.w3.org/2006/vcard/ns#hasNote">
        <rdfs:comment xml:lang="en">Used to support property parameters for the note data property</rdfs:comment>
        <rdfs:isDefinedBy rdf:resource="http://www.w3.org/2006/vcard/ns"/>
        <rdfs:label xml:lang="en">has note</rdfs:label>
    </owl:ObjectProperty>
    


    <!-- http://www.w3.org/2006/vcard/ns#hasOrganizationName -->

    <owl:ObjectProperty rdf:about="http://www.w3.org/2006/vcard/ns#hasOrganizationName">
        <rdfs:comment xml:lang="en">Used to support property parameters for the organization name data property</rdfs:comment>
        <rdfs:isDefinedBy rdf:resource="http://www.w3.org/2006/vcard/ns"/>
        <rdfs:label xml:lang="en">has organization name</rdfs:label>
    </owl:ObjectProperty>
    


    <!-- http://www.w3.org/2006/vcard/ns#hasOrganizationUnit -->

    <owl:ObjectProperty rdf:about="http://www.w3.org/2006/vcard/ns#hasOrganizationUnit">
        <rdfs:comment xml:lang="en">Used to support property parameters for the organization unit name data property</rdfs:comment>
        <rdfs:isDefinedBy rdf:resource="http://www.w3.org/2006/vcard/ns"/>
        <rdfs:label xml:lang="en">has organization unit name</rdfs:label>
    </owl:ObjectProperty>
    


    <!-- http://www.w3.org/2006/vcard/ns#hasPhoto -->

    <owl:ObjectProperty rdf:about="http://www.w3.org/2006/vcard/ns#hasPhoto">
        <owl:equivalentProperty rdf:resource="http://www.w3.org/2006/vcard/ns#photo"/>
        <rdfs:comment xml:lang="en">To specify an image or photograph information that annotates some aspect of the object</rdfs:comment>
        <rdfs:isDefinedBy rdf:resource="http://www.w3.org/2006/vcard/ns"/>
        <rdfs:label xml:lang="en">has photo</rdfs:label>
    </owl:ObjectProperty>
    


    <!-- http://www.w3.org/2006/vcard/ns#hasPostalCode -->

    <owl:ObjectProperty rdf:about="http://www.w3.org/2006/vcard/ns#hasPostalCode">
        <rdfs:comment xml:lang="en">Used to support property parameters for the postal code data property</rdfs:comment>
        <rdfs:isDefinedBy rdf:resource="http://www.w3.org/2006/vcard/ns"/>
        <rdfs:label xml:lang="en">has postal code</rdfs:label>
    </owl:ObjectProperty>
    


    <!-- http://www.w3.org/2006/vcard/ns#hasRegion -->

    <owl:ObjectProperty rdf:about="http://www.w3.org/2006/vcard/ns#hasRegion">
        <rdfs:comment xml:lang="en">Used to support property parameters for the region data property</rdfs:comment>
        <rdfs:isDefinedBy rdf:resource="http://www.w3.org/2006/vcard/ns"/>
        <rdfs:label xml:lang="en">has region</rdfs:label>
    </owl:ObjectProperty>
    


    <!-- http://www.w3.org/2006/vcard/ns#hasRelated -->

    <owl:ObjectProperty rdf:about="http://www.w3.org/2006/vcard/ns#hasRelated">
        <rdfs:comment xml:lang="en">To specify a relationship between another entity and the entity represented by this object</rdfs:comment>
        <rdfs:isDefinedBy rdf:resource="http://www.w3.org/2006/vcard/ns"/>
        <rdfs:label xml:lang="en">has related</rdfs:label>
    </owl:ObjectProperty>
    


    <!-- http://www.w3.org/2006/vcard/ns#hasRole -->

    <owl:ObjectProperty rdf:about="http://www.w3.org/2006/vcard/ns#hasRole">
        <rdfs:comment xml:lang="en">Used to support property parameters for the role data property</rdfs:comment>
        <rdfs:isDefinedBy rdf:resource="http://www.w3.org/2006/vcard/ns"/>
        <rdfs:label xml:lang="en">has role</rdfs:label>
    </owl:ObjectProperty>
    


    <!-- http://www.w3.org/2006/vcard/ns#hasSound -->

    <owl:ObjectProperty rdf:about="http://www.w3.org/2006/vcard/ns#hasSound">
        <owl:equivalentProperty rdf:resource="http://www.w3.org/2006/vcard/ns#sound"/>
        <rdfs:comment xml:lang="en">To specify a digital sound content information that annotates some aspect of the object</rdfs:comment>
        <rdfs:isDefinedBy rdf:resource="http://www.w3.org/2006/vcard/ns"/>
        <rdfs:label xml:lang="en">has sound</rdfs:label>
    </owl:ObjectProperty>
    


    <!-- http://www.w3.org/2006/vcard/ns#hasSource -->

    <owl:ObjectProperty rdf:about="http://www.w3.org/2006/vcard/ns#hasSource">
        <rdfs:comment xml:lang="en">To identify the source of directory information of the object</rdfs:comment>
        <rdfs:isDefinedBy rdf:resource="http://www.w3.org/2006/vcard/ns"/>
        <rdfs:label xml:lang="en">has source</rdfs:label>
    </owl:ObjectProperty>
    


    <!-- http://www.w3.org/2006/vcard/ns#hasStreetAddress -->

    <owl:ObjectProperty rdf:about="http://www.w3.org/2006/vcard/ns#hasStreetAddress">
        <rdfs:comment xml:lang="en">Used to support property parameters for the street address data property</rdfs:comment>
        <rdfs:isDefinedBy rdf:resource="http://www.w3.org/2006/vcard/ns"/>
        <rdfs:label xml:lang="en">has street address</rdfs:label>
    </owl:ObjectProperty>
    


    <!-- http://www.w3.org/2006/vcard/ns#hasTelephone -->

    <owl:ObjectProperty rdf:about="http://www.w3.org/2006/vcard/ns#hasTelephone">
        <owl:equivalentProperty rdf:resource="http://www.w3.org/2006/vcard/ns#tel"/>
        <rdfs:comment xml:lang="en">To specify the telephone number for telephony communication with the object</rdfs:comment>
        <rdfs:isDefinedBy rdf:resource="http://www.w3.org/2006/vcard/ns"/>
        <rdfs:label xml:lang="en">has telephone</rdfs:label>
    </owl:ObjectProperty>
    


    <!-- http://www.w3.org/2006/vcard/ns#hasTitle -->

    <owl:ObjectProperty rdf:about="http://www.w3.org/2006/vcard/ns#hasTitle">
        <rdfs:comment xml:lang="en">Used to support property parameters for the title data property</rdfs:comment>
        <rdfs:isDefinedBy rdf:resource="http://www.w3.org/2006/vcard/ns"/>
        <rdfs:label xml:lang="en">has title</rdfs:label>
    </owl:ObjectProperty>
    


    <!-- http://www.w3.org/2006/vcard/ns#hasUID -->

    <owl:ObjectProperty rdf:about="http://www.w3.org/2006/vcard/ns#hasUID">
        <rdfs:comment xml:lang="en">To specify a value that represents a globally unique identifier corresponding to the object</rdfs:comment>
        <rdfs:isDefinedBy rdf:resource="http://www.w3.org/2006/vcard/ns"/>
        <rdfs:label xml:lang="en">has uid</rdfs:label>
    </owl:ObjectProperty>
    


    <!-- http://www.w3.org/2006/vcard/ns#hasURL -->

    <owl:ObjectProperty rdf:about="http://www.w3.org/2006/vcard/ns#hasURL">
        <owl:equivalentProperty rdf:resource="http://www.w3.org/2006/vcard/ns#url"/>
        <rdfs:comment xml:lang="en">To specify a uniform resource locator associated with the object</rdfs:comment>
        <rdfs:isDefinedBy rdf:resource="http://www.w3.org/2006/vcard/ns"/>
        <rdfs:label xml:lang="en">has url</rdfs:label>
    </owl:ObjectProperty>
    


    <!-- http://www.w3.org/2006/vcard/ns#hasValue -->

    <owl:ObjectProperty rdf:about="http://www.w3.org/2006/vcard/ns#hasValue">
        <rdfs:comment xml:lang="en">Used to indicate the resource value of an object property that requires property parameters</rdfs:comment>
        <rdfs:isDefinedBy rdf:resource="http://www.w3.org/2006/vcard/ns"/>
        <rdfs:label xml:lang="en">has value</rdfs:label>
    </owl:ObjectProperty>
    


    <!-- http://www.w3.org/2006/vcard/ns#key -->

    <owl:ObjectProperty rdf:about="http://www.w3.org/2006/vcard/ns#key">
        <rdfs:comment xml:lang="en">This object property has been mapped</rdfs:comment>
        <rdfs:isDefinedBy rdf:resource="http://www.w3.org/2006/vcard/ns"/>
        <rdfs:label xml:lang="en">key</rdfs:label>
    </owl:ObjectProperty>
    


    <!-- http://www.w3.org/2006/vcard/ns#logo -->

    <owl:ObjectProperty rdf:about="http://www.w3.org/2006/vcard/ns#logo">
        <rdfs:comment xml:lang="en">This object property has been mapped</rdfs:comment>
        <rdfs:isDefinedBy rdf:resource="http://www.w3.org/2006/vcard/ns"/>
        <rdfs:label xml:lang="en">logo</rdfs:label>
    </owl:ObjectProperty>
    


    <!-- http://www.w3.org/2006/vcard/ns#n -->

    <owl:ObjectProperty rdf:about="http://www.w3.org/2006/vcard/ns#n">
        <rdfs:comment xml:lang="en">This object property has been mapped</rdfs:comment>
        <rdfs:isDefinedBy rdf:resource="http://www.w3.org/2006/vcard/ns"/>
        <rdfs:label xml:lang="en">name</rdfs:label>
    </owl:ObjectProperty>
    


    <!-- http://www.w3.org/2006/vcard/ns#org -->

    <owl:ObjectProperty rdf:about="http://www.w3.org/2006/vcard/ns#org">
        <rdfs:comment xml:lang="en">This object property has been mapped. Use the organization-name data property.</rdfs:comment>
        <rdfs:isDefinedBy rdf:resource="http://www.w3.org/2006/vcard/ns"/>
        <rdfs:label xml:lang="en">organization</rdfs:label>
    </owl:ObjectProperty>
    


    <!-- http://www.w3.org/2006/vcard/ns#photo -->

    <owl:ObjectProperty rdf:about="http://www.w3.org/2006/vcard/ns#photo">
        <rdfs:comment xml:lang="en">This object property has been mapped</rdfs:comment>
        <rdfs:isDefinedBy rdf:resource="http://www.w3.org/2006/vcard/ns"/>
        <rdfs:label xml:lang="en">photo</rdfs:label>
    </owl:ObjectProperty>
    


    <!-- http://www.w3.org/2006/vcard/ns#sound -->

    <owl:ObjectProperty rdf:about="http://www.w3.org/2006/vcard/ns#sound">
        <rdfs:comment xml:lang="en">This object property has been mapped</rdfs:comment>
        <rdfs:isDefinedBy rdf:resource="http://www.w3.org/2006/vcard/ns"/>
        <rdfs:label xml:lang="en">sound</rdfs:label>
    </owl:ObjectProperty>
    


    <!-- http://www.w3.org/2006/vcard/ns#tel -->

    <owl:ObjectProperty rdf:about="http://www.w3.org/2006/vcard/ns#tel">
        <rdfs:comment xml:lang="en">This object property has been mapped</rdfs:comment>
        <rdfs:isDefinedBy rdf:resource="http://www.w3.org/2006/vcard/ns"/>
        <rdfs:label xml:lang="en">telephone</rdfs:label>
    </owl:ObjectProperty>
    


    <!-- http://www.w3.org/2006/vcard/ns#url -->

    <owl:ObjectProperty rdf:about="http://www.w3.org/2006/vcard/ns#url">
        <rdfs:comment xml:lang="en">This object property has been mapped</rdfs:comment>
        <rdfs:isDefinedBy rdf:resource="http://www.w3.org/2006/vcard/ns"/>
        <rdfs:label xml:lang="en">url</rdfs:label>
    </owl:ObjectProperty>
    


    <!-- http://www.w3.org/ns/org#basedAt -->

    <owl:ObjectProperty rdf:about="http://www.w3.org/ns/org#basedAt">
        <rdfs:domain rdf:resource="http://xmlns.com/foaf/0.1/Person"/>
        <rdfs:range rdf:resource="http://www.w3.org/ns/org#Site"/>
        <rdfs:comment xml:lang="it">Indica la sede in cui una è stabilita una persona. Non esclude la possibilità che una persona sia allocata su più sedi.</rdfs:comment>
        <rdfs:comment xml:lang="en">Indicates the site at which a person is based. We do not restrict the possibility that a person is based at multiple sites.</rdfs:comment>
        <rdfs:comment xml:lang="fr">Indique le site sur lequel une personne est basée. Nous ne limitons pas le nombre de sites sur lesquels une personne peut être basée.</rdfs:comment>
        <rdfs:comment xml:lang="es">Lugar en el que trabaja una persona. No se restringe el hecho de que una persona pueda estar adscrita a múltiples ubicaciones.</rdfs:comment>
        <rdfs:comment xml:lang="ja">人が基礎としているサイトを示します。人が複数のサイトを基礎としている可能性を制限しません。</rdfs:comment>
        <rdfs:isDefinedBy rdf:resource="http://www.w3.org/ns/org"/>
        <rdfs:label xml:lang="it">basata a</rdfs:label>
        <rdfs:label xml:lang="en">based At</rdfs:label>
        <rdfs:label xml:lang="fr">basé à</rdfs:label>
        <rdfs:label xml:lang="es">trabaja en la sede</rdfs:label>
    </owl:ObjectProperty>
    


    <!-- http://www.w3.org/ns/org#changedBy -->

    <owl:ObjectProperty rdf:about="http://www.w3.org/ns/org#changedBy">
        <owl:inverseOf rdf:resource="http://www.w3.org/ns/org#originalOrganization"/>
        <rdfs:domain rdf:resource="http://www.w3.org/ns/org#Organization"/>
        <rdfs:range rdf:resource="http://www.w3.org/ns/org#ChangeEvent"/>
        <rdfs:comment xml:lang="es">Evento de cambio que resulta en una modificación en la organización. Dependiendo del evento, la organización puede dejar de existir tras el cambio. Es la relación inversa de `org:originalOrganization`.</rdfs:comment>
        <rdfs:comment xml:lang="it">Indica un evento che ha contribuito al cambiamento di questa organizzazione. A seconda dell&apos;evento, l&apos;organizzazione potrebbe essere esistente dopo l&apos;evento o aver cessato la propria esistenza. È l&apos;inverso di `org:originalOrganization`.</rdfs:comment>
        <rdfs:comment xml:lang="en">Indicates a change event which resulted in a change to this organization. Depending on the event the organization may or may not have continued to exist after the event. Inverse of `org:originalOrganization`.</rdfs:comment>
        <rdfs:comment xml:lang="fr">Indique un évènement qui a impliqué un changement dans l&apos;Organisation. Selon l&apos;évènement, l&apos;Organisation a continué à exister après l&apos;évènement, ou pas. Inverse de `org:originalOrganization`.</rdfs:comment>
        <rdfs:comment xml:lang="ja">この組織の変更のきっかけとなった出来事を示します。</rdfs:comment>
        <rdfs:isDefinedBy rdf:resource="http://www.w3.org/ns/org"/>
        <rdfs:label xml:lang="it">cambiata da</rdfs:label>
        <rdfs:label xml:lang="en">changed by</rdfs:label>
        <rdfs:label xml:lang="es">es modificada por</rdfs:label>
        <rdfs:label xml:lang="es">es modificado por</rdfs:label>
        <rdfs:label xml:lang="fr">modifiée par</rdfs:label>
    </owl:ObjectProperty>
    


    <!-- http://www.w3.org/ns/org#classification -->

    <owl:ObjectProperty rdf:about="http://www.w3.org/ns/org#classification">
        <rdfs:domain rdf:resource="http://www.w3.org/ns/org#Organization"/>
        <rdfs:range rdf:resource="http://www.w3.org/2004/02/skos/core#Concept"/>
        <rdfs:comment xml:lang="it">Indica una classificazione per questa Organization all&apos;interno di un qualche schema di classificazione. Alcuni vocabolari potrebbero voler specializzare questa proprietà per avere un codominio corrispondente a uno specifico `skos:ConceptScheme`. Si noti che la presenza di questa proprietà è ancora in fase di discussione e potrebbe  essere revisionata o rimossa.</rdfs:comment>
        <rdfs:comment xml:lang="en">Indicates a classification for this Organization within some classification scheme. Extension vocabularies may wish to specialize this property to have a range corresponding to a specific `skos:ConceptScheme`. This property is under discussion and may be revised or removed - in many cases organizations are best categorized by defining a sub-class hierarchy in an extension vocabulary.</rdfs:comment>
        <rdfs:comment xml:lang="fr">Indique une classification pour cette Organisation dans le cadre d&apos;un schéma de classification. Il est possible de spécialiser cette propriété en utilisant un vocabulaire spécialisé pour que le champ corresponde à un concept spécifique `skos:ConceptScheme`. Cette propriété est en discussion est pourrait être révisée ou supprimée - dans de nombreux cas, les organisations sont mieux catégorisées par une hiérarchie de sous-classe dans un vocabulaire externe.</rdfs:comment>
        <rdfs:comment xml:lang="es">Ordenación jerárquica que se hace de una organización dentro de un esquema de clasificación. Es posible que algunos vocabularios especifiquen esta propiedad de forma que el rango se corresponda con un `skos:ConceptScheme` específico. La conveniencia de incluir esta propiedad se está debatiendo y puede que se revise o elimine (en muchos casos las organizaciones se clasifican mejor si se define una jerarquía de subclases en un vocabulario aparte)</rdfs:comment>
        <rdfs:comment xml:lang="ja">ある分類表内のこの組織に対する分類を示します。
アプリケーションがorg:Organizationのサブクラスを組織的なカテゴリーを表わす手段として定義することも許容されることに注意してください。</rdfs:comment>
        <rdfs:isDefinedBy rdf:resource="http://www.w3.org/ns/org"/>
        <rdfs:label xml:lang="en">classification</rdfs:label>
        <rdfs:label xml:lang="fr">classification</rdfs:label>
        <rdfs:label xml:lang="it">classificazione</rdfs:label>
        <rdfs:label xml:lang="es">pertenece a la clasificación</rdfs:label>
    </owl:ObjectProperty>
    


    <!-- http://www.w3.org/ns/org#hasMember -->

    <owl:ObjectProperty rdf:about="http://www.w3.org/ns/org#hasMember">
        <owl:inverseOf rdf:resource="http://www.w3.org/ns/org#memberOf"/>
        <rdfs:domain rdf:resource="http://www.w3.org/ns/org#Organization"/>
        <rdfs:range rdf:resource="http://xmlns.com/foaf/0.1/Agent"/>
        <rdfs:comment xml:lang="it">Indica una persona che è membro della data Organization. È l&apos;inverso di `org:memberOf` ed è fornita per  compatibilità con `foaf:member`.</rdfs:comment>
        <rdfs:comment xml:lang="en">Indicates a person who is a member of the subject Organization. Inverse of `org:memberOf`, see that property for further clarification. Provided for compatibility with `foaf:member`.</rdfs:comment>
        <rdfs:comment xml:lang="fr">Indique une personne membre de l&apos;Organisation sujet. Inverse de `org:memberOf`, voyez la description de cette propriété pour plus de précisions. Fourni pour la compatibilité avec `foaf:member`.</rdfs:comment>
        <rdfs:comment xml:lang="es">Persona que es miembro de la organización en cuestión. Es la relación inversa de `org:memberOf`, véase la descripción de esa propiedad para más detalles. Se prevé compatibilidad con foaf:member`.</rdfs:comment>
        <rdfs:comment xml:lang="ja">対象組織のメンバーであるエージェント（人または他の組織）を示します。org:memberOfの逆。さらに明確な説明については、そのプロパティーを参照してください。</rdfs:comment>
        <rdfs:isDefinedBy rdf:resource="http://www.w3.org/ns/org"/>
        <rdfs:label xml:lang="it">ha membro</rdfs:label>
        <rdfs:label xml:lang="en">has member</rdfs:label>
        <rdfs:label xml:lang="fr">possède un membre</rdfs:label>
        <rdfs:label xml:lang="es">tiene miembro</rdfs:label>
    </owl:ObjectProperty>
    


    <!-- http://www.w3.org/ns/org#hasMembership -->

    <owl:ObjectProperty rdf:about="http://www.w3.org/ns/org#hasMembership">
        <owl:inverseOf rdf:resource="http://www.w3.org/ns/org#member"/>
        <rdfs:domain rdf:resource="http://xmlns.com/foaf/0.1/Agent"/>
        <rdfs:range rdf:resource="http://www.w3.org/ns/org#Membership"/>
        <rdfs:comment xml:lang="it">Indica una relazione di appartenenza che coinvolge un Agent. È l&apos;inverso di `org:member`.</rdfs:comment>
        <rdfs:comment xml:lang="en">Indicates a membership relationship that the Agent plays. Inverse of `org:member`.</rdfs:comment>
        <rdfs:comment xml:lang="fr">Indique pour cet Agent un engagement dans une Organisation. Inverse de `org:member`.</rdfs:comment>
        <rdfs:comment xml:lang="es">Relación de pertenencia o afiliación a una organización en la que el agente desempeña un cargo o función. Es la relación inversa de `org:member`.</rdfs:comment>
        <rdfs:comment xml:lang="ja">エージェントが担う構成員関係を示します。</rdfs:comment>
        <rdfs:isDefinedBy rdf:resource="http://www.w3.org/ns/org"/>
        <rdfs:label xml:lang="it">appartenenza</rdfs:label>
        <rdfs:label xml:lang="fr">engagement</rdfs:label>
        <rdfs:label xml:lang="en">membership</rdfs:label>
        <rdfs:label xml:lang="es">tiene membresía</rdfs:label>
    </owl:ObjectProperty>
    


    <!-- http://www.w3.org/ns/org#hasPost -->

    <owl:ObjectProperty rdf:about="http://www.w3.org/ns/org#hasPost">
        <owl:inverseOf rdf:resource="http://www.w3.org/ns/org#postIn"/>
        <rdfs:domain rdf:resource="http://www.w3.org/ns/org#Organization"/>
        <rdfs:range rdf:resource="http://www.w3.org/ns/org#Post"/>
        <rdfs:comment xml:lang="it">Indica il Post che è presente in una Organization.</rdfs:comment>
        <rdfs:comment xml:lang="fr">Indicate un Poste qui existe dans l&apos;Organisation.</rdfs:comment>
        <rdfs:comment xml:lang="en">Indicates a Post which exists within the Organization.</rdfs:comment>
        <rdfs:comment xml:lang="es">Posición que existe en una organización.</rdfs:comment>
        <rdfs:comment xml:lang="ja">組織内に存在するポストを示します。</rdfs:comment>
        <rdfs:isDefinedBy rdf:resource="http://www.w3.org/ns/org"/>
        <rdfs:label xml:lang="it">impiego</rdfs:label>
        <rdfs:label xml:lang="fr">possède un poste</rdfs:label>
        <rdfs:label xml:lang="en">post</rdfs:label>
        <rdfs:label xml:lang="es">tiene puesto</rdfs:label>
    </owl:ObjectProperty>
    


    <!-- http://www.w3.org/ns/org#hasPrimarySite -->

    <owl:ObjectProperty rdf:about="http://www.w3.org/ns/org#hasPrimarySite">
        <rdfs:subPropertyOf rdf:resource="http://www.w3.org/ns/org#hasSite"/>
        <rdfs:domain rdf:resource="http://www.w3.org/ns/org#Organization"/>
        <rdfs:range rdf:resource="http://www.w3.org/ns/org#Site"/>
        <rdfs:comment xml:lang="it">Indica la sede principale per l&apos;Organization. È da considerarsi come la sede di default in cui l&apos;Organization deve essere contattata pur non essendo necessariamente il quartier generale.</rdfs:comment>
        <rdfs:comment xml:lang="en">Indicates a primary site for the Organization, this is the default means by which an Organization can be contacted and is not necessarily the formal headquarters.</rdfs:comment>
        <rdfs:comment xml:lang="fr">Indique le site principal d&apos;une Organisation, le moyen par défaut par lequel l&apos;Organisation peut être contactée et pas nécessairement le siège social légal.</rdfs:comment>
        <rdfs:comment xml:lang="es">Oficina principal de la organización, la opción por defecto para ponerse en contacto con una organización, aunque no corresponde necesariamente con las oficinas centrales de la organización.</rdfs:comment>
        <rdfs:comment xml:lang="ja">組織の主要サイトを示します。組織の窓口となりえるデフォルトの手段ですが、正式な本部とは限りません。</rdfs:comment>
        <rdfs:isDefinedBy rdf:resource="http://www.w3.org/ns/org"/>
        <rdfs:label xml:lang="en">primary Site</rdfs:label>
        <rdfs:label xml:lang="it">sede principale</rdfs:label>
        <rdfs:label xml:lang="fr">site principal</rdfs:label>
        <rdfs:label xml:lang="es">tiene sede principal en</rdfs:label>
    </owl:ObjectProperty>
    


    <!-- http://www.w3.org/ns/org#hasRegisteredSite -->

    <owl:ObjectProperty rdf:about="http://www.w3.org/ns/org#hasRegisteredSite">
        <rdfs:subPropertyOf rdf:resource="http://www.w3.org/ns/org#hasPrimarySite"/>
        <rdfs:domain rdf:resource="http://www.w3.org/ns/org#FormalOrganization"/>
        <rdfs:range rdf:resource="http://www.w3.org/ns/org#Site"/>
        <rdfs:comment xml:lang="it">Indica la sede legale per l&apos;Organization. In molte giurisdizioni è richiesto che una FormalOrganization abbia una sede di questo tipo.</rdfs:comment>
        <rdfs:comment xml:lang="en">Indicates the legally registered site for the organization, in many legal jurisdictions there is a requirement that FormalOrganizations such as Companies or Charities have such a primary designed site. </rdfs:comment>
        <rdfs:comment xml:lang="fr">Indique l&apos;établissement principal légalement enregistré pour l&apos;Organisation. Dans de nombreuses juridictions existe l&apos;obligation pour une Organisation Formelle d&apos;avoir un tel site principal. </rdfs:comment>
        <rdfs:comment xml:lang="es">Oficina o sede legalmente registrada de la organización. En muchas jurisdicciones legales existe el requisito de que organizaciones formales tales como empresas u organizaciones de beneficencia tengan una sede principal de este tipo.</rdfs:comment>
        <rdfs:comment xml:lang="ja">組織の法律上登録されたサイトを示し、多くの法的管轄区域では、会社や慈善団体などのFormalOrganizations（正式な組織）がそのような主要サイトを持っているという要件があります。</rdfs:comment>
        <rdfs:isDefinedBy rdf:resource="http://www.w3.org/ns/org"/>
        <rdfs:label xml:lang="en">registered Site</rdfs:label>
        <rdfs:label xml:lang="it">sede legale</rdfs:label>
        <rdfs:label xml:lang="fr">siège social</rdfs:label>
        <rdfs:label xml:lang="es">tiene sede registrada en</rdfs:label>
    </owl:ObjectProperty>
    


    <!-- http://www.w3.org/ns/org#hasSite -->

    <owl:ObjectProperty rdf:about="http://www.w3.org/ns/org#hasSite">
        <owl:inverseOf rdf:resource="http://www.w3.org/ns/org#siteOf"/>
        <rdfs:domain rdf:resource="http://www.w3.org/ns/org#Organization"/>
        <rdfs:range rdf:resource="http://www.w3.org/ns/org#Site"/>
        <rdfs:comment xml:lang="it">Indica la sede in cui l&apos;Organization ha una qualche presenza anche in modo indiretto (ad esempio un ufficio virtuale). È l&apos;inverso di `org:siteOf`.</rdfs:comment>
        <rdfs:comment xml:lang="en">Indicates a site at which the Organization has some presence even if only indirect (e.g. virtual office or a professional service which is acting as the registered address for a company). Inverse of `org:siteOf`.</rdfs:comment>
        <rdfs:comment xml:lang="fr">Indique un site sur lequel l&apos;Organisation possède une présence, même indirecte (domiciliation, boite postale). Inverse de `org:siteOf`.</rdfs:comment>
        <rdfs:comment xml:lang="es">Lugar en donde la organización tiene algún tipo de presencia, incluso si es de forma indirecta (por ejemplo, una oficina virtual o servicio profesional que hagan la función de dirección registrada de la compañía). Es la relación inversa de `org:siteOf`.</rdfs:comment>
        <rdfs:comment xml:lang="ja">組織が、間接（例えば、会社の登録住所として機能しているバーチャル・オフィスやプロフェッショナル・サービス）のみであったとしても、ある存在感を持っているサイトを示します。</rdfs:comment>
        <rdfs:isDefinedBy rdf:resource="http://www.w3.org/ns/org"/>
        <rdfs:label xml:lang="fr">a un site</rdfs:label>
        <rdfs:label xml:lang="it">ha sede</rdfs:label>
        <rdfs:label xml:lang="en">has site</rdfs:label>
        <rdfs:label xml:lang="es">tiene sede en</rdfs:label>
    </owl:ObjectProperty>
    


    <!-- http://www.w3.org/ns/org#hasSubOrganization -->

    <owl:ObjectProperty rdf:about="http://www.w3.org/ns/org#hasSubOrganization">
        <owl:inverseOf rdf:resource="http://www.w3.org/ns/org#subOrganizationOf"/>
        <rdfs:domain rdf:resource="http://www.w3.org/ns/org#Organization"/>
        <rdfs:range rdf:resource="http://www.w3.org/ns/org#Organization"/>
        <rdfs:comment xml:lang="fr">Indique le statut de dépendance hiérarchique pour des Organisations ou des Unités Opérationnelles; indique une Organisation qui est une sous-partie ou une branche d&apos;une Organisation plus large. C&apos;est la propriété inverse de `org:subOrganizationOf`.</rdfs:comment>
        <rdfs:comment xml:lang="es">Organización jerárquica de organizaciones o unidades. Indica que una organización es parte de otra organización más amplia o pertenece a ella. Es la relación inversa de `org:subOrganizationOf`.</rdfs:comment>
        <rdfs:comment xml:lang="it">Rappresenta un contenimento gerarchico di una Organization o di una OrganizationalUnit. Indica una organizzazione che è parte di una organizzazione più grande. È l&apos;inverso di `org:subOrganizationOf`.</rdfs:comment>
        <rdfs:comment xml:lang="en">Represents hierarchical containment of Organizations or Organizational Units; indicates an organization which is a sub-part or child of this organization.  Inverse of `org:subOrganizationOf`.</rdfs:comment>
        <rdfs:comment xml:lang="ja">組織または組織単位の階層的包含を表わします。この組織のサブパートまたは子である組織を示します。</rdfs:comment>
        <rdfs:isDefinedBy rdf:resource="http://www.w3.org/ns/org"/>
        <rdfs:label xml:lang="fr">a une Sous-Organization</rdfs:label>
        <rdfs:label xml:lang="it">ha sotto-Organization</rdfs:label>
        <rdfs:label xml:lang="en">has SubOrganization</rdfs:label>
        <rdfs:label xml:lang="es">tiene suborganización</rdfs:label>
    </owl:ObjectProperty>
    


    <!-- http://www.w3.org/ns/org#hasUnit -->

    <owl:ObjectProperty rdf:about="http://www.w3.org/ns/org#hasUnit">
        <rdfs:subPropertyOf rdf:resource="http://www.w3.org/ns/org#hasSubOrganization"/>
        <owl:inverseOf rdf:resource="http://www.w3.org/ns/org#unitOf"/>
        <rdfs:domain rdf:resource="http://www.w3.org/ns/org#FormalOrganization"/>
        <rdfs:range rdf:resource="http://www.w3.org/ns/org#OrganizationalUnit"/>
        <rdfs:comment xml:lang="it">Indica un&apos;unità che è parte di questa Organization, come ad esempio un dipartimento facente parte di una più ampia FormalOrganization. È l&apos;inverso di `org:unitOf`.</rdfs:comment>
        <rdfs:comment xml:lang="en">Indicates a unit which is part of this Organization, e.g. a Department within a larger FormalOrganization. Inverse of `org:unitOf`.</rdfs:comment>
        <rdfs:comment xml:lang="fr">Indique une Unité qui fait partie d&apos;une Organisation, par exemple un Départment au sein d&apos;une Organisation Formelle plus large. Inverse de `org:unitOf`.</rdfs:comment>
        <rdfs:comment xml:lang="es">Unidad que es parte de la organización, como, por ejemplo, un departamento incluido en una organización formal más amplia.</rdfs:comment>
        <rdfs:comment xml:lang="ja">例えば、より大きな組織内の部局など、この組織の一部である単位を示します。</rdfs:comment>
        <rdfs:isDefinedBy rdf:resource="http://www.w3.org/ns/org"/>
        <rdfs:label xml:lang="es">contiene unidad</rdfs:label>
        <rdfs:label xml:lang="it">ha Unit</rdfs:label>
        <rdfs:label xml:lang="en">has Unit</rdfs:label>
        <rdfs:label xml:lang="fr">possède une Unité</rdfs:label>
    </owl:ObjectProperty>
    


    <!-- http://www.w3.org/ns/org#headOf -->

    <owl:ObjectProperty rdf:about="http://www.w3.org/ns/org#headOf">
        <rdfs:subPropertyOf rdf:resource="http://www.w3.org/ns/org#memberOf"/>
        <rdfs:domain rdf:resource="http://xmlns.com/foaf/0.1/Person"/>
        <rdfs:range rdf:resource="http://www.w3.org/ns/org#Organization"/>
        <rdfs:comment xml:lang="it">Indica che una persona è leader o responsabile formale di una Organization. Questo significa che la persona è alla radice del grafo (aciclico) creato dalle `org:reportsTo`, sebbene un&apos;organizzazione possa avere più di un responsabile.</rdfs:comment>
        <rdfs:comment xml:lang="en">Indicates that a person is the leader or formal head of the Organization. This will normally mean that they are the root of the `org:reportsTo` (acyclic) graph, though an organization may have more than one head.</rdfs:comment>
        <rdfs:comment xml:lang="fr">Indique qu&apos;une personne est le directeur ou le responsable formel d&apos;une Organisation. Ceci indique souvent qu&apos;il est au sommet de du graphe acyclique des `org:reportsTo`, même si une organisation peut avoir plus d&apos;un responsable.</rdfs:comment>
        <rdfs:comment xml:lang="es">Persona que es jefe o jefa, representante ,,director o directora de la organización. Esto significa que dicha persona es el rango de la relación `org:reportsTo` en el organigrama de la organización (acíclico), aunque una organización puede tener más de un jefe.</rdfs:comment>
        <rdfs:comment xml:lang="ja">人（または他のエージェント）が組織のリーダーや正式なトップであることを示します。</rdfs:comment>
        <rdfs:isDefinedBy rdf:resource="http://www.w3.org/ns/org"/>
        <rdfs:label xml:lang="es">es director ejecutivo de</rdfs:label>
        <rdfs:label xml:lang="en">head of</rdfs:label>
        <rdfs:label xml:lang="it">responsabile di</rdfs:label>
        <rdfs:label xml:lang="fr">responsable de</rdfs:label>
    </owl:ObjectProperty>
    


    <!-- http://www.w3.org/ns/org#heldBy -->

    <owl:ObjectProperty rdf:about="http://www.w3.org/ns/org#heldBy">
        <owl:inverseOf rdf:resource="http://www.w3.org/ns/org#holds"/>
        <rdfs:domain rdf:resource="http://www.w3.org/ns/org#Post"/>
        <rdfs:range rdf:resource="http://xmlns.com/foaf/0.1/Agent"/>
        <rdfs:comment xml:lang="es">Agente que ocupa un puesto.</rdfs:comment>
        <rdfs:comment xml:lang="it">Indica un Agent che ricopre un Post.</rdfs:comment>
        <rdfs:comment xml:lang="fr">Indicate un Agent qui occupe le Poste.</rdfs:comment>
        <rdfs:comment xml:lang="en">Indicates an Agent which holds a Post.</rdfs:comment>
        <rdfs:comment xml:lang="ja">ポストを保持するエージェントを示します。</rdfs:comment>
        <rdfs:isDefinedBy rdf:resource="http://www.w3.org/ns/org"/>
        <rdfs:label xml:lang="en">held by</rdfs:label>
        <rdfs:label xml:lang="fr">occupé par</rdfs:label>
        <rdfs:label xml:lang="es">ocupado por</rdfs:label>
        <rdfs:label xml:lang="it">ricoperto da</rdfs:label>
    </owl:ObjectProperty>
    


    <!-- http://www.w3.org/ns/org#holds -->

    <owl:ObjectProperty rdf:about="http://www.w3.org/ns/org#holds">
        <rdfs:domain rdf:resource="http://xmlns.com/foaf/0.1/Agent"/>
        <rdfs:range rdf:resource="http://www.w3.org/ns/org#Post"/>
        <rdfs:comment xml:lang="it">Indica un Impiego ricoperto da un Agent.</rdfs:comment>
        <rdfs:comment xml:lang="fr">Indicate un Poste occupé par un Agent.</rdfs:comment>
        <rdfs:comment xml:lang="en">Indicates a Post held by some Agent.</rdfs:comment>
        <rdfs:comment xml:lang="es">Puesto ocupado por algún agente.</rdfs:comment>
        <rdfs:comment xml:lang="ja">あるエージェントによって保持されているポストを示します。</rdfs:comment>
        <rdfs:isDefinedBy rdf:resource="http://www.w3.org/ns/org"/>
        <rdfs:label xml:lang="en">holds</rdfs:label>
        <rdfs:label xml:lang="fr">occupe</rdfs:label>
        <rdfs:label xml:lang="es">ocupa</rdfs:label>
        <rdfs:label xml:lang="it">ricopre</rdfs:label>
    </owl:ObjectProperty>
    


    <!-- http://www.w3.org/ns/org#linkedTo -->

    <owl:ObjectProperty rdf:about="http://www.w3.org/ns/org#linkedTo">
        <rdfs:domain rdf:resource="http://www.w3.org/ns/org#Organization"/>
        <rdfs:range rdf:resource="http://www.w3.org/ns/org#Organization"/>
        <rdfs:comment xml:lang="ja">2つの組織の任意の関係を示します。</rdfs:comment>
        <rdfs:comment xml:lang="it">Indica una relazione arbitraria tra due organizzazioni. Ad esempio, specializzazioni di questa proprietà possono essere usate per denotare relazioni particolari tipo il finanziamento o la fornitura.</rdfs:comment>
        <rdfs:comment xml:lang="en">Indicates an arbitrary relationship between two organizations. Specializations of this can be used to, for example, denote funding or supply chain relationships.</rdfs:comment>
        <rdfs:comment xml:lang="fr">Indique une relation arbitraire entre deux Organisations. Des spécialisations peuvent être utilisées pour, par exemple, qualifier une relation de fournisseur ou de financeur.</rdfs:comment>
        <rdfs:comment xml:lang="es">Relación arbitraria entre dos organizaciones. Las especializaciones de esta relación se pueden utilizar para denotar relaciones de financiación o suministro, entre otras.</rdfs:comment>
        <rdfs:isDefinedBy rdf:resource="http://www.w3.org/ns/org"/>
        <rdfs:label xml:lang="it">collegato a</rdfs:label>
        <rdfs:label xml:lang="es">está relacionada con</rdfs:label>
        <rdfs:label xml:lang="es">está relacionado con</rdfs:label>
        <rdfs:label xml:lang="en">linked to</rdfs:label>
        <rdfs:label xml:lang="fr">relié à</rdfs:label>
    </owl:ObjectProperty>
    


    <!-- http://www.w3.org/ns/org#member -->

    <owl:ObjectProperty rdf:about="http://www.w3.org/ns/org#member">
        <rdf:type rdf:resource="http://www.w3.org/2002/07/owl#FunctionalProperty"/>
        <rdfs:domain rdf:resource="http://www.w3.org/ns/org#Membership"/>
        <rdfs:range rdf:resource="http://xmlns.com/foaf/0.1/Agent"/>
        <rdfs:comment xml:lang="it">Indica la Person (o un altro Agent) coinvolto in una relazione di Membership. È l&apos;inverso di `org:hasMembership`.</rdfs:comment>
        <rdfs:comment xml:lang="en">Indicates the Person (or other Agent including Organization) involved in the Membership relationship. Inverse of `org:hasMembership`</rdfs:comment>
        <rdfs:comment xml:lang="fr">Indique une personne (ou tout autre Agent, y compris une Organisation) impliqué dans la relation d&apos;Engagement. Inverse de `org:hasMembership`</rdfs:comment>
        <rdfs:comment xml:lang="es">Persona (u otro agente, incluyendo una organización) que participa en la relación de membresía. Es la relación inversa de `org:hasMembership`.</rdfs:comment>
        <rdfs:comment xml:lang="ja">構成員関係に含まれている人（または、組織を含んでいる他のエージェント）を示します。</rdfs:comment>
        <rdfs:isDefinedBy rdf:resource="http://www.w3.org/ns/org"/>
        <rdfs:label xml:lang="es">es condición de miembro sobre agente</rdfs:label>
        <rdfs:label xml:lang="en">member</rdfs:label>
        <rdfs:label xml:lang="fr">membre</rdfs:label>
        <rdfs:label xml:lang="it">membro</rdfs:label>
    </owl:ObjectProperty>
    


    <!-- http://www.w3.org/ns/org#memberDuring -->

    <owl:ObjectProperty rdf:about="http://www.w3.org/ns/org#memberDuring">
        <rdfs:domain rdf:resource="http://www.w3.org/ns/org#Membership"/>
        <rdfs:range rdf:resource="http://aifb.kit.edu/stepC#SpatialTemporalEntity"/>
        <rdfs:comment xml:lang="en">Optional property to indicate the interval for which the membership is/was valid.</rdfs:comment>
        <rdfs:comment xml:lang="es">Propiedad opcional que indica el periodo durante el cual la relación de membresía o pertenencia a una organización se mantiene en vigencia.</rdfs:comment>
        <rdfs:comment xml:lang="it">Proprietà opzionale per indicare l&apos;intervallo per il quale l&apos;appartenenza è/è stata valida.</rdfs:comment>
        <rdfs:comment xml:lang="fr">Propriété optionnelle pour indiquer l&apos;intervalle durant lequel l&apos;engagemnet est ou était valide.</rdfs:comment>
        <rdfs:comment xml:lang="ja">構成員が有効である／であった期間を示すためのオプションのプロパティー。</rdfs:comment>
        <rdfs:isDefinedBy rdf:resource="http://www.w3.org/ns/org"/>
        <rdfs:label xml:lang="fr">durée d&apos;engagement</rdfs:label>
        <rdfs:label xml:lang="es">es miembro durante</rdfs:label>
        <rdfs:label xml:lang="en">member During</rdfs:label>
        <rdfs:label xml:lang="it">membro durante</rdfs:label>
    </owl:ObjectProperty>
    


    <!-- http://www.w3.org/ns/org#memberOf -->

    <owl:ObjectProperty rdf:about="http://www.w3.org/ns/org#memberOf">
        <rdf:type rdf:resource="http://www.w3.org/2002/07/owl#TransitiveProperty"/>
        <rdfs:domain rdf:resource="http://xmlns.com/foaf/0.1/Agent"/>
        <rdfs:range rdf:resource="http://www.w3.org/ns/org#Organization"/>
        <rdfs:comment xml:lang="it">Indica che una persona è membro di una Organization senza una precisa indicazione sulla natura di questa appartenenza e sul suo ruolo. Si noti che la scelta del nome di questa proprietà non intende limitarla alla sola  rappresentazione formalmente di un&apos;appartenenza. La proprietà può coprire anche altri coinvolgimenti nell&apos;organizzazione. Questa proprietà può essere specializzata per indicare ruoli all&apos;interno organizzazione o relazioni di diverse tipologie. Ha `org:hasmember` come proprietà inversa opzionale.</rdfs:comment>
        <rdfs:comment xml:lang="en">Indicates that a person is a member of the Organization with no indication of the nature of that membership or the role played. Note that the choice of property name is not meant to limit the property to only formal membership arrangements, it is also indended to cover related concepts such as affilliation or other involvement in the organization. Extensions can specialize this relationship to indicate particular roles within the organization or more nuanced relationships to the organization. Has an optional inverse, `org:hasmember`.</rdfs:comment>
        <rdfs:comment xml:lang="fr">Indique qu&apos;une personne est membre de l&apos;Organisation sans précision sur la nature de cet engagement ou du rôle joué. Notez que le choix du nom de cette propriété ne vise pas à la limiter aux seuls engagements formels, elle peut également couvrir des concepts reliés comme l&apos;affiliation ou le bénévolat. Des extensions peuvent spécialiser cette relation pour indiquer des rôles particuliers au sein de l&apos;Organisation or des relations plus nuancées avec elle. Possède une propriété inverse optionnelle, `org:hasmember`.</rdfs:comment>
        <rdfs:comment xml:lang="es">Persona que pertenece a la organización o es miembro de la misma, sin que conste la naturaleza de dicha pertenencia o el papel que desempeña. Se debe tener en cuenta que la elección de una denominación para esta propiedad no significa que la propiedad esté limitada a ciertos tipos de pertenencia formales, sino que pretende cubrir conceptos relacionados como el de afiliación u otras formas de participación en la organización. Se puede hacer uso de extensiones para especializar esta relación de forma que incluya tipos específicos de pertenencia a las organizaciones o relaciones especiales con la organización.</rdfs:comment>
        <rdfs:comment xml:lang="ja">エージェント（人または他の組織）が組織のメンバーであることを示します。ただし、その構成員の本質や担う役割は示しません。プロパティー名の選択は、プロパティーを正式な構成員配置のみに制限することが目的ではないことに注意してください。所属や組織へのその他の関与などの関連する概念をカバーすることも意図されています。拡張により、この関係を特殊化し、組織内の特定の役割やよりニュアンスを含んだ組織との関係を示すことができます。</rdfs:comment>
        <rdfs:isDefinedBy rdf:resource="http://www.w3.org/ns/org"/>
        <rdfs:label xml:lang="es">es miembro de</rdfs:label>
        <rdfs:label xml:lang="en">member of</rdfs:label>
        <rdfs:label xml:lang="fr">membre de</rdfs:label>
        <rdfs:label xml:lang="it">membro di</rdfs:label>
    </owl:ObjectProperty>
    


    <!-- http://www.w3.org/ns/org#organization -->

    <owl:ObjectProperty rdf:about="http://www.w3.org/ns/org#organization">
        <rdf:type rdf:resource="http://www.w3.org/2002/07/owl#FunctionalProperty"/>
        <rdfs:domain rdf:resource="http://www.w3.org/ns/org#Membership"/>
        <rdfs:range rdf:resource="http://www.w3.org/ns/org#Organization"/>
        <rdfs:comment xml:lang="it">Indica l&apos;Organization in cui l&apos;Agent è un membro.</rdfs:comment>
        <rdfs:comment xml:lang="en">Indicates Organization in which the Agent is a member.</rdfs:comment>
        <rdfs:comment xml:lang="fr">Indique l&apos;Organization dont l&apos;agent est membre.</rdfs:comment>
        <rdfs:comment xml:lang="es">Organización a la que pertenece el agente en calidad de miembro.</rdfs:comment>
        <rdfs:comment xml:lang="ja">エージェントがメンバーである組織を示します。</rdfs:comment>
        <rdfs:isDefinedBy rdf:resource="http://www.w3.org/ns/org"/>
        <rdfs:label xml:lang="es">es condición de miembro sobre organización</rdfs:label>
        <rdfs:label xml:lang="fr">organisation</rdfs:label>
        <rdfs:label xml:lang="en">organization</rdfs:label>
        <rdfs:label xml:lang="it">organizzazione</rdfs:label>
    </owl:ObjectProperty>
    


    <!-- http://www.w3.org/ns/org#originalOrganization -->

    <owl:ObjectProperty rdf:about="http://www.w3.org/ns/org#originalOrganization">
        <rdfs:subPropertyOf rdf:resource="http://www.w3.org/ns/prov#used"/>
        <rdfs:domain rdf:resource="http://www.w3.org/ns/org#ChangeEvent"/>
        <rdfs:range rdf:resource="http://www.w3.org/ns/org#Organization"/>
        <rdfs:comment xml:lang="it">Indica una o più organizzazioni pregresse rispetto a un evento di cambiamento. A seconda dell&apos;evento, queste organizzazioni potrebbero essere esistenti dopo l&apos;evento o  aver cessato la loro esistenza. È l&apos;inverso di `org:changedBy`.</rdfs:comment>
        <rdfs:comment xml:lang="en">Indicates one or more organizations that existed before the change event. Depending on the event they may or may not have continued to exist after the event. Inverse of `org:changedBy`.</rdfs:comment>
        <rdfs:comment xml:lang="fr">Indique une ou plusieurs organisations qui ont existé avant un évènement de changement. Selon l&apos;évènement, ces organisations ont pu continuer à exister ou non. Inverse de `org:changedBy`. </rdfs:comment>
        <rdfs:comment xml:lang="es">Una o más organizaciones que existían antes de que sucediera el cambio en la organización. Dependiendo del tipo de cambio, dichas organizaciones pueden haber dejado de existir o no. Es la relación inversa de `org:changedBy`.</rdfs:comment>
        <rdfs:comment xml:lang="ja">変更のきっかけとなった出来事以前に存在した1つ以上の組織を示します。出来事によって、出来事の後にそれらは存在し続けたかも、存在し続けなかったかもしれません。</rdfs:comment>
        <rdfs:isDefinedBy rdf:resource="http://www.w3.org/ns/org"/>
        <rdfs:label xml:lang="es">es organización original</rdfs:label>
        <rdfs:label xml:lang="fr">organisation originelle</rdfs:label>
        <rdfs:label xml:lang="it">organizzazione originale</rdfs:label>
        <rdfs:label xml:lang="en">original organization</rdfs:label>
    </owl:ObjectProperty>
    


    <!-- http://www.w3.org/ns/org#postIn -->

    <owl:ObjectProperty rdf:about="http://www.w3.org/ns/org#postIn">
        <rdfs:domain rdf:resource="http://www.w3.org/ns/org#Post"/>
        <rdfs:range rdf:resource="http://www.w3.org/ns/org#Organization"/>
        <rdfs:comment xml:lang="it">Indica l&apos;Organization in cui il Post è presente.</rdfs:comment>
        <rdfs:comment xml:lang="fr">Indicate l&apos;Organisation dans laquelle le Poste existe.</rdfs:comment>
        <rdfs:comment xml:lang="en">Indicates the Organization in which the Post exists.</rdfs:comment>
        <rdfs:comment xml:lang="es">Organización en la que existe el puesto.</rdfs:comment>
        <rdfs:comment xml:lang="ja">ポストが存在する組織を示します。</rdfs:comment>
        <rdfs:isDefinedBy rdf:resource="http://www.w3.org/ns/org"/>
        <rdfs:label xml:lang="es">es un puesto en</rdfs:label>
        <rdfs:label xml:lang="it">impiego in</rdfs:label>
        <rdfs:label xml:lang="en">post in</rdfs:label>
        <rdfs:label xml:lang="fr">poste chez</rdfs:label>
    </owl:ObjectProperty>
    


    <!-- http://www.w3.org/ns/org#remuneration -->

    <owl:ObjectProperty rdf:about="http://www.w3.org/ns/org#remuneration">
        <rdfs:domain rdf:resource="http://www.w3.org/ns/org#Role"/>
        <rdfs:comment xml:lang="it">Indica il salario o altra forma di remunerazione associata al ruolo. In genere, questo si denota usando uno schema di rappresentazione esistente come il `gr:PriceSpecification` ma il codominio è lasciato libero di essere specializzato a seconda delle applicazioni.</rdfs:comment>
        <rdfs:comment xml:lang="en">Indicates a salary or other reward associated with the role. Typically this will be denoted using an existing representation scheme such as `gr:PriceSpecification` but the range is left open to allow applications to specialize it (e.g. to remunerationInGBP).</rdfs:comment>
        <rdfs:comment xml:lang="fr">Indique un salaire ou tout autre compensation associée au Rôle. Typiquement, ceci sera annoté en utilisant un schéma existant comme  `gr:PriceSpecification` mais le champ de cette propriété est laissé ouvert afin de permettre aux applications de la spécialiser (par exemple remunerationEuro).</rdfs:comment>
        <rdfs:comment xml:lang="es">Salario o cualquier otra remuneración asociada con la actividad. La forma usual de referirse a dicha remuneración será utilizando un esquema de representación como el propuesto en la ontología GoodRelations `gr:PriceSpecification`, pero el rango se deja abierto a que las distintas aplicaciones lo especialicen (por ejemplo, remunerationInGBP)</rdfs:comment>
        <rdfs:comment xml:lang="ja">役割に関係する給料やその他の報酬を示します。</rdfs:comment>
        <rdfs:isDefinedBy rdf:resource="http://www.w3.org/ns/org"/>
        <rdfs:label xml:lang="es">recibe remuneración</rdfs:label>
        <rdfs:label xml:lang="en">remuneration</rdfs:label>
        <rdfs:label xml:lang="it">remunerazione</rdfs:label>
        <rdfs:label xml:lang="fr">rémuneration</rdfs:label>
    </owl:ObjectProperty>
    


    <!-- http://www.w3.org/ns/org#reportsTo -->

    <owl:ObjectProperty rdf:about="http://www.w3.org/ns/org#reportsTo">
        <rdfs:domain>
            <owl:Class>
                <owl:unionOf rdf:parseType="Collection">
                    <rdf:Description rdf:about="http://www.w3.org/ns/org#Post"/>
                    <rdf:Description rdf:about="http://xmlns.com/foaf/0.1/Agent"/>
                </owl:unionOf>
            </owl:Class>
        </rdfs:domain>
    </owl:ObjectProperty>
    


    <!-- http://www.w3.org/ns/org#resultedFrom -->

    <owl:ObjectProperty rdf:about="http://www.w3.org/ns/org#resultedFrom">
        <rdfs:subPropertyOf rdf:resource="http://www.w3.org/ns/prov#wasGeneratedBy"/>
        <owl:inverseOf rdf:resource="http://www.w3.org/ns/org#resultingOrganization"/>
        <rdfs:domain rdf:resource="http://www.w3.org/ns/org#Organization"/>
        <rdfs:range rdf:resource="http://www.w3.org/ns/org#ChangeEvent"/>
        <rdfs:comment xml:lang="es">Evento que tiene como resultado la creación de una organización.</rdfs:comment>
        <rdfs:comment xml:lang="it">Indica l&apos;evento che ha permesso all&apos;organizzazione di instaurarsi. È l&apos;inverso di `org:resultingOrganization`.</rdfs:comment>
        <rdfs:comment xml:lang="en">Indicates an event which resulted in this organization. Inverse of `org:resultingOrganization`.</rdfs:comment>
        <rdfs:comment xml:lang="fr">Indique un évènement dont est issue l&apos;Organisation. Inverse de `org:resultingOrganization`.</rdfs:comment>
        <rdfs:comment xml:lang="ja">この組織になった（導いた、作成された）きっかけとなった出来事を示します。</rdfs:comment>
        <rdfs:isDefinedBy rdf:resource="http://www.w3.org/ns/org"/>
        <rdfs:label xml:lang="es">es el resultado de</rdfs:label>
        <rdfs:label xml:lang="fr">issue de</rdfs:label>
        <rdfs:label xml:lang="en">resulted from</rdfs:label>
        <rdfs:label xml:lang="it">risultato da</rdfs:label>
    </owl:ObjectProperty>
    


    <!-- http://www.w3.org/ns/org#resultingOrganization -->

    <owl:ObjectProperty rdf:about="http://www.w3.org/ns/org#resultingOrganization">
        <rdfs:domain rdf:resource="http://www.w3.org/ns/org#ChangeEvent"/>
        <rdfs:range rdf:resource="http://www.w3.org/ns/org#Organization"/>
        <rdfs:comment xml:lang="it">Indica l&apos;organizzazione che è stata creata o mutata a seguito dell&apos;evento. È l&apos;inverso di `org:resultedFrom`.</rdfs:comment>
        <rdfs:comment xml:lang="en">Indicates an organization which was created or changed as a result of the event. Inverse of `org:resultedFrom`.</rdfs:comment>
        <rdfs:comment xml:lang="fr">Indique une organisation qui a été créée ou a été modifiée à la suite d&apos;un Évènement de changement. Inverse de `org:resultedFrom`.</rdfs:comment>
        <rdfs:comment xml:lang="es">Organización que ha sido creada o modificada tras un evento específico.  Es la relación inversa de `org:resultedFrom`.</rdfs:comment>
        <rdfs:comment xml:lang="ja">出来事の結果、作成、変更された組織を示します。</rdfs:comment>
        <rdfs:isDefinedBy rdf:resource="http://www.w3.org/ns/org"/>
        <rdfs:label xml:lang="fr">a donné naissance à</rdfs:label>
        <rdfs:label xml:lang="es">resulta en</rdfs:label>
        <rdfs:label xml:lang="en">resulted in</rdfs:label>
        <rdfs:label xml:lang="it">risultato in</rdfs:label>
    </owl:ObjectProperty>
    


    <!-- http://www.w3.org/ns/org#role -->

    <owl:ObjectProperty rdf:about="http://www.w3.org/ns/org#role">
        <rdfs:domain>
            <owl:Class>
                <owl:unionOf rdf:parseType="Collection">
                    <rdf:Description rdf:about="http://www.w3.org/ns/org#Membership"/>
                    <rdf:Description rdf:about="http://www.w3.org/ns/org#Post"/>
                </owl:unionOf>
            </owl:Class>
        </rdfs:domain>
    </owl:ObjectProperty>
    


    <!-- http://www.w3.org/ns/org#siteAddress -->

    <owl:ObjectProperty rdf:about="http://www.w3.org/ns/org#siteAddress">
        <rdfs:domain rdf:resource="http://www.w3.org/ns/org#Site"/>
        <rdfs:range rdf:resource="http://aifb.kit.edu/stepC#SpatialTemporalEntity"/>
        <rdfs:comment xml:lang="es">Dirección de la sede según una codificación adecuada. Se recomienda el uso de vCard (que utiliza el vocabulario en http://www.w3.org/TR/vcard-rdf/), pero el rango no se restringe únicamente al uso de este vocabulario sino que se permite el uso de otros códigos. La dirección puede constar de una dirección de correo electrónico, un número de teléfono o información de geo-localización, y no se limita a una dirección postal física.</rdfs:comment>
        <rdfs:comment xml:lang="it">Indica un indirizzo per la sede in una codifica appropriata. Il codominio è lasciato libero ma è consigliabile l&apos;uso del vocabolario vCard (http://www.w3.org/TR/vcard-rdf/). L&apos;indirizzo può includere email, numero di telefono e informazioni di geolocalizzazione e non è vincolato ad essere un indirizzo fisico.</rdfs:comment>
        <rdfs:comment xml:lang="en">Indicates an address for the site in a suitable encoding. Use of vCard (using the http://www.w3.org/TR/vcard-rdf/ vocabulary) is encouraged but the range is left open to allow other encodings to be used. The address may include email, telephone, and geo-location information and is not restricted to a physical address. </rdfs:comment>
        <rdfs:comment xml:lang="fr">Indique une adresse pour le site dans un encodage approprié. L&apos;usage du vocabulaire vCard ( http://www.w3.org/TR/vcard-rdf/) est encouragé, mais le range est ouvert pour permettre l&apos;utilisation d&apos;autres vocabulaires. L&apos;adresse peut comporter le courriel, le téléphone, et l&apos;information de géolocalisation; et n&apos;est donc pas seulement limitée à une adresse physique. </rdfs:comment>
        <rdfs:comment xml:lang="ja">適切にコード化されたサイトのアドレスを示します。vCard[vcard-rdf]語彙などの有名なアドレスのコード化の使用が奨励されますが、他の符号化の使用を可能とするために値域はオープンのままにされます。アドレスには、電子メール、電話およびジオロケーション情報を含むことができ、物理的なアドレスに制限されません。</rdfs:comment>
        <rdfs:isDefinedBy rdf:resource="http://www.w3.org/ns/org"/>
        <rdfs:label xml:lang="fr">adresse du Site</rdfs:label>
        <rdfs:label xml:lang="es">es la dirección de la sede</rdfs:label>
        <rdfs:label xml:lang="it">indirizzo della sede</rdfs:label>
        <rdfs:label xml:lang="en">site Address</rdfs:label>
    </owl:ObjectProperty>
    


    <!-- http://www.w3.org/ns/org#siteOf -->

    <owl:ObjectProperty rdf:about="http://www.w3.org/ns/org#siteOf">
        <rdfs:domain rdf:resource="http://www.w3.org/ns/org#Site"/>
        <rdfs:range rdf:resource="http://www.w3.org/ns/org#Organization"/>
        <rdfs:comment xml:lang="it">Indica un&apos;Organization che ha una qualche presenza nella data sede. È l&apos;inverso di `org:hasSite`.</rdfs:comment>
        <rdfs:comment xml:lang="en">Indicates an Organization which has some presence at the given site. This is the inverse of `org:hasSite`.</rdfs:comment>
        <rdfs:comment xml:lang="fr">Indique une Organisation qui a une présence sur le site en question. Inverse de `org:hasSite`.</rdfs:comment>
        <rdfs:comment xml:lang="es">Organización que tiene ubicación en un lugar. Es la relación inversa de `org:hasSite`.</rdfs:comment>
        <rdfs:comment xml:lang="ja">あるサイトである存在感を持っている組織を示します。</rdfs:comment>
        <rdfs:isDefinedBy rdf:resource="http://www.w3.org/ns/org"/>
        <rdfs:label xml:lang="es">es sede de</rdfs:label>
        <rdfs:label xml:lang="it">sede di</rdfs:label>
        <rdfs:label xml:lang="en">site Of</rdfs:label>
        <rdfs:label xml:lang="fr">site de</rdfs:label>
    </owl:ObjectProperty>
    


    <!-- http://www.w3.org/ns/org#subOrganizationOf -->

    <owl:ObjectProperty rdf:about="http://www.w3.org/ns/org#subOrganizationOf">
        <rdfs:subPropertyOf rdf:resource="http://www.w3.org/ns/org#transitiveSubOrganizationOf"/>
        <rdfs:domain rdf:resource="http://www.w3.org/ns/org#Organization"/>
        <rdfs:range rdf:resource="http://www.w3.org/ns/org#Organization"/>
        <rdfs:comment xml:lang="es">Distribución jerárquica de organizaciones o unidades. Indica que una organización contiene a otra organización. Es la relación inversa de `org:hasSubOrganization`</rdfs:comment>
        <rdfs:comment xml:lang="it">Rappresenta un contenimento gerarchico di una Organization o di una OrganizationalUnit. È l&apos;inverso di `org:hasSubOrganization`. Ha nome come nome alternativo hasSubOrg.</rdfs:comment>
        <rdfs:comment xml:lang="en">Represents hierarchical containment of Organizations or OrganizationalUnits; indicates an Organization which contains this Organization. Inverse of `org:hasSubOrganization`.</rdfs:comment>
        <rdfs:comment xml:lang="fr">Représente une relation hierarchique des Organisations ou des Unités Opérationnelles; indique une Organisation sujet qui contient cette Organisation. Inverse de `org:hasSubOrganization`.</rdfs:comment>
        <rdfs:comment xml:lang="ja">組織または組織単位の階層的包含を表わします。この組織を含む組織を示します。</rdfs:comment>
        <rdfs:isDefinedBy rdf:resource="http://www.w3.org/ns/org"/>
        <rdfs:label xml:lang="es">es suborganización de</rdfs:label>
        <rdfs:label xml:lang="it">sotto-Organization di</rdfs:label>
        <rdfs:label xml:lang="fr">sous-Organization de</rdfs:label>
        <rdfs:label xml:lang="en">subOrganization of</rdfs:label>
    </owl:ObjectProperty>
    


    <!-- http://www.w3.org/ns/org#transitiveSubOrganizationOf -->

    <owl:ObjectProperty rdf:about="http://www.w3.org/ns/org#transitiveSubOrganizationOf">
        <rdf:type rdf:resource="http://www.w3.org/2002/07/owl#TransitiveProperty"/>
        <rdfs:domain rdf:resource="http://www.w3.org/ns/org#Organization"/>
        <rdfs:range rdf:resource="http://www.w3.org/ns/org#Organization"/>
        <rdfs:comment xml:lang="fr">La version transitive de la propriété subOrganizationOf, renvoie une représentation de toutes les organisations qui contiennent celle-ci. Notez que ceci est une super-propriété de la relation transitive donc elle pourrait contenir des assertions additionnelles mais cet usage n&apos;est pas recommandé.</rdfs:comment>
        <rdfs:comment xml:lang="es">La versión transitiva de la propiedad “subOrganizationOf”, es decir, la representación de todas las organizaciones en las que esta está contenida. Téngase en cuenta que desde el punto de vista técnico esta es una propiedad que contiene a todas las propiedades transitivas, de forma que podría contener afirmaciones adicionales, aunque su uso no está aconsejado.</rdfs:comment>
        <rdfs:comment xml:lang="en">The transitive closure of subOrganizationOf, giving a representation of all organizations that contain this one. Note that technically this is a super property of the transitive closure so it could contain additional assertions but such usage is discouraged.</rdfs:comment>
        <rdfs:comment xml:lang="ja">subOrganizationOfの推移閉包で、これを含むすべての組織の表現を与える。技術的に、これが推移閉包のスーパープロパティーであるため、追加の言明を含むことができますが、そのような使用法はお勧めできないことに注意してください。</rdfs:comment>
        <rdfs:comment xml:lang="it">È la chiusura transitiva di subOrganizationOf, quindi rappresenta tutte le organizzazioni che la contengono. Tecnicamente, essendo una chiusura transitiva, può contenere asserzioni che non la riguardano e quindi il suo uso è sconsigliato.</rdfs:comment>
        <rdfs:isDefinedBy rdf:resource="http://www.w3.org/ns/org"/>
        <rdfs:label xml:lang="es">es suborganización de (transitiva)</rdfs:label>
        <rdfs:label xml:lang="es">es suborganización de manera transitiva de</rdfs:label>
        <rdfs:label xml:lang="it">sotto-Organization transitiva</rdfs:label>
        <rdfs:label xml:lang="fr">sous-Organization transitive de</rdfs:label>
        <rdfs:label xml:lang="en">transitive sub-organization</rdfs:label>
    </owl:ObjectProperty>
    


    <!-- http://www.w3.org/ns/org#unitOf -->

    <owl:ObjectProperty rdf:about="http://www.w3.org/ns/org#unitOf">
        <rdfs:subPropertyOf rdf:resource="http://www.w3.org/ns/org#subOrganizationOf"/>
        <rdfs:domain rdf:resource="http://www.w3.org/ns/org#OrganizationalUnit"/>
        <rdfs:range rdf:resource="http://www.w3.org/ns/org#FormalOrganization"/>
        <rdfs:comment xml:lang="it">Indica un Organization di cui questa Unit fa parte, come ad esempio un dipartimento all&apos;interno di una più vasta FormalOrganization. È l&apos;inverso di `org:hasUnit`.</rdfs:comment>
        <rdfs:comment xml:lang="en">Indicates an Organization of which this Unit is a part, e.g. a Department within a larger FormalOrganization. This is the inverse of `org:hasUnit`.</rdfs:comment>
        <rdfs:comment xml:lang="fr">Indique l&apos;Organisation dont cette Organisation ou Unité fait partie, par exemple un Départment au sein d&apos;une Organisation Formelle plus large. Inverse de `org:hasUnit`.</rdfs:comment>
        <rdfs:comment xml:lang="es">Organización de la que es parte esta unidad, por ejemplo, un departamento incluido en una organización formal más amplia.</rdfs:comment>
        <rdfs:comment xml:lang="ja">例えば、より大きな組織内の部局など、この単位がその一部分である組織を示します。</rdfs:comment>
        <rdfs:isDefinedBy rdf:resource="http://www.w3.org/ns/org"/>
        <rdfs:label xml:lang="es">es unidad de</rdfs:label>
        <rdfs:label xml:lang="en">unit Of</rdfs:label>
        <rdfs:label xml:lang="it">unità di</rdfs:label>
        <rdfs:label xml:lang="fr">unité de</rdfs:label>
    </owl:ObjectProperty>
    


    <!-- http://www.w3.org/ns/prov#used -->

    <owl:ObjectProperty rdf:about="http://www.w3.org/ns/prov#used"/>
    


    <!-- http://www.w3.org/ns/prov#wasDerivedFrom -->

    <owl:ObjectProperty rdf:about="http://www.w3.org/ns/prov#wasDerivedFrom">
        <owl:propertyChainAxiom rdf:parseType="Collection">
            <rdf:Description rdf:about="http://www.w3.org/ns/org#resultedFrom"/>
            <rdf:Description rdf:about="http://www.w3.org/ns/org#originalOrganization"/>
        </owl:propertyChainAxiom>
    </owl:ObjectProperty>
    


    <!-- http://www.w3.org/ns/prov#wasGeneratedBy -->

    <owl:ObjectProperty rdf:about="http://www.w3.org/ns/prov#wasGeneratedBy"/>
    


    <!-- http://xmlns.com/foaf/0.1/based_near -->

    <owl:ObjectProperty rdf:about="http://xmlns.com/foaf/0.1/based_near"/>
    


    <!-- http://xmlns.com/foaf/0.1/made -->

    <owl:ObjectProperty rdf:about="http://xmlns.com/foaf/0.1/made">
        <owl:inverseOf rdf:resource="http://xmlns.com/foaf/0.1/maker"/>
    </owl:ObjectProperty>
    


    <!-- http://xmlns.com/foaf/0.1/maker -->

    <owl:ObjectProperty rdf:about="http://xmlns.com/foaf/0.1/maker">
        <rdfs:domain rdf:resource="http://people.aifb.kit.edu/mu2771/step#Report"/>
        <rdfs:range rdf:resource="http://xmlns.com/foaf/0.1/Agent"/>
        <rdfs:comment>An agent that  made this thing.</rdfs:comment>
        <rdfs:isDefinedBy rdf:resource="http://xmlns.com/foaf/0.1/"/>
        <rdfs:label>maker</rdfs:label>
        <ns:term_status>stable</ns:term_status>
    </owl:ObjectProperty>
    


    <!-- 
    ///////////////////////////////////////////////////////////////////////////////////////
    //
    // Data properties
    //
    ///////////////////////////////////////////////////////////////////////////////////////
     -->

    


    <!-- http://iirds.tekom.de/iirds#Description -->

    <owl:DatatypeProperty rdf:about="http://iirds.tekom.de/iirds#Description">
        <rdfs:subPropertyOf rdf:resource="http://iirds.tekom.de/iirds#iirdsAttribute"/>
    </owl:DatatypeProperty>
    


    <!-- http://iirds.tekom.de/iirds#Duration -->

    <owl:DatatypeProperty rdf:about="http://iirds.tekom.de/iirds#Duration">
        <rdfs:subPropertyOf rdf:resource="http://iirds.tekom.de/iirds#iirdsAttribute"/>
        <rdfs:domain rdf:resource="http://iirds.tekom.de/iirds#PlanningTime"/>
        <rdfs:range rdf:resource="http://www.w3.org/2001/XMLSchema#string"/>
        <rdfs:label xml:lang="de">Dauer</rdfs:label>
        <rdfs:label xml:lang="en">Duration</rdfs:label>
    </owl:DatatypeProperty>
    


    <!-- http://iirds.tekom.de/iirds#EventCode -->

    <owl:DatatypeProperty rdf:about="http://iirds.tekom.de/iirds#EventCode">
        <rdfs:subPropertyOf rdf:resource="http://iirds.tekom.de/iirds#iirdsAttribute"/>
        <rdfs:domain rdf:resource="http://iirds.tekom.de/iirds#Event"/>
        <rdfs:range rdf:resource="http://www.w3.org/2001/XMLSchema#string"/>
        <rdfs:label xml:lang="de">EreignisCode</rdfs:label>
        <rdfs:label xml:lang="en">Event Code</rdfs:label>
    </owl:DatatypeProperty>
    


    <!-- http://iirds.tekom.de/iirds#EventType -->

    <owl:DatatypeProperty rdf:about="http://iirds.tekom.de/iirds#EventType">
        <rdfs:subPropertyOf rdf:resource="http://iirds.tekom.de/iirds#iirdsAttribute"/>
        <rdfs:domain rdf:resource="http://iirds.tekom.de/iirds#Event"/>
        <rdfs:range rdf:resource="http://www.w3.org/2001/XMLSchema#string"/>
        <rdfs:label xml:lang="de">EreignisTyp</rdfs:label>
        <rdfs:label xml:lang="en">Event Type</rdfs:label>
    </owl:DatatypeProperty>
    


    <!-- http://iirds.tekom.de/iirds#Format -->

    <owl:DatatypeProperty rdf:about="http://iirds.tekom.de/iirds#Format">
        <rdfs:subPropertyOf rdf:resource="http://iirds.tekom.de/iirds#iirdsAttribute"/>
    </owl:DatatypeProperty>
    


    <!-- http://iirds.tekom.de/iirds#FormatRestriction -->

    <owl:DatatypeProperty rdf:about="http://iirds.tekom.de/iirds#FormatRestriction">
        <rdfs:subPropertyOf rdf:resource="http://iirds.tekom.de/iirds#iirdsAttribute"/>
        <rdfs:domain rdf:resource="http://iirds.tekom.de/iirds#InformationUnit"/>
        <rdfs:range rdf:resource="http://www.w3.org/2001/XMLSchema#string"/>
        <rdfs:label xml:lang="de">Formateinschränkung</rdfs:label>
        <rdfs:label xml:lang="en">format restriction</rdfs:label>
    </owl:DatatypeProperty>
    


    <!-- http://iirds.tekom.de/iirds#Identifier -->

    <owl:DatatypeProperty rdf:about="http://iirds.tekom.de/iirds#Identifier">
        <rdfs:subPropertyOf rdf:resource="http://iirds.tekom.de/iirds#iirdsAttribute"/>
    </owl:DatatypeProperty>
    


    <!-- http://iirds.tekom.de/iirds#Language -->

    <owl:DatatypeProperty rdf:about="http://iirds.tekom.de/iirds#Language">
        <rdfs:subPropertyOf rdf:resource="http://iirds.tekom.de/iirds#iirdsAttribute"/>
    </owl:DatatypeProperty>
    


    <!-- http://iirds.tekom.de/iirds#Synonym -->

    <owl:DatatypeProperty rdf:about="http://iirds.tekom.de/iirds#Synonym">
        <rdfs:subPropertyOf rdf:resource="http://iirds.tekom.de/iirds#iirdsAttribute"/>
        <rdfs:domain rdf:resource="http://iirds.tekom.de/iirds#iirdsDomainEntitiy"/>
        <rdfs:range rdf:resource="http://www.w3.org/2001/XMLSchema#string"/>
        <rdfs:label xml:lang="de">Synonym</rdfs:label>
        <rdfs:label xml:lang="en">Synonym</rdfs:label>
    </owl:DatatypeProperty>
    


    <!-- http://iirds.tekom.de/iirds#Title -->

    <owl:DatatypeProperty rdf:about="http://iirds.tekom.de/iirds#Title">
        <rdfs:subPropertyOf rdf:resource="http://iirds.tekom.de/iirds#iirdsAttribute"/>
    </owl:DatatypeProperty>
    


    <!-- http://iirds.tekom.de/iirds#iiRDSVersion -->

    <owl:DatatypeProperty rdf:about="http://iirds.tekom.de/iirds#iiRDSVersion">
        <rdfs:subPropertyOf rdf:resource="http://iirds.tekom.de/iirds#iirdsAttribute"/>
        <rdfs:domain rdf:resource="http://iirds.tekom.de/iirds#Package"/>
        <rdfs:range rdf:resource="http://www.w3.org/2001/XMLSchema#string"/>
        <rdfs:label xml:lang="de">iiRDS Version</rdfs:label>
        <rdfs:label xml:lang="en">iiRDS version</rdfs:label>
    </owl:DatatypeProperty>
    


    <!-- http://iirds.tekom.de/iirds#iirdsAttribute -->

    <owl:DatatypeProperty rdf:about="http://iirds.tekom.de/iirds#iirdsAttribute">
        <rdfs:range rdf:resource="http://www.w3.org/2001/XMLSchema#string"/>
        <rdfs:label xml:lang="de">iirdsAttribute</rdfs:label>
        <rdfs:label xml:lang="en">iirdsAttribute</rdfs:label>
    </owl:DatatypeProperty>
    


    <!-- http://people.aifb.kit.edu/mu2771/step#differenceToUTC -->

    <owl:DatatypeProperty rdf:about="http://people.aifb.kit.edu/mu2771/step#differenceToUTC">
        <rdfs:comment>the amount of hours this timezone is different to Universal-Time-Coordinated (UTC)/Greenwich Mean Time (GMT)</rdfs:comment>
        <rdfs:isDefinedBy rdf:resource="http://aifb.kit.edu/stepC"/>
        <rdfs:label xml:lang="de">differenceToUTC</rdfs:label>
    </owl:DatatypeProperty>
    


    <!-- http://people.aifb.kit.edu/mu2771/step#failureProbability -->

    <owl:DatatypeProperty rdf:about="http://people.aifb.kit.edu/mu2771/step#failureProbability">
        <rdfs:domain rdf:resource="http://people.aifb.kit.edu/mu2771/step#Prediction"/>
        <rdfs:range rdf:resource="http://www.w3.org/2001/XMLSchema#double"/>
        <rdfs:label>failureProbability</rdfs:label>
    </owl:DatatypeProperty>
    


    <!-- http://people.aifb.kit.edu/mu2771/step#level -->

    <owl:DatatypeProperty rdf:about="http://people.aifb.kit.edu/mu2771/step#level">
        <rdfs:domain rdf:resource="http://people.aifb.kit.edu/mu2771/step#Expertise"/>
        <rdfs:range rdf:resource="http://www.w3.org/2001/XMLSchema#int"/>
        <rdfs:comment xml:lang="en">the level of expertise of a technician</rdfs:comment>
        <rdfs:label xml:lang="de">hat Qualifikationsstufe</rdfs:label>
        <rdfs:label xml:lang="en">level</rdfs:label>
    </owl:DatatypeProperty>
    


    <!-- http://people.aifb.kit.edu/mu2771/step#probability -->

    <owl:DatatypeProperty rdf:about="http://people.aifb.kit.edu/mu2771/step#probability">
        <rdfs:domain rdf:resource="http://people.aifb.kit.edu/mu2771/step#WorkOrder"/>
        <rdfs:range rdf:resource="http://www.w3.org/2001/XMLSchema#double"/>
        <rdfs:label xml:lang="de">hat Wahrscheinlichkeit</rdfs:label>
    </owl:DatatypeProperty>
    


    <!-- http://people.aifb.kit.edu/mu2771/step#reference -->

    <owl:DatatypeProperty rdf:about="http://people.aifb.kit.edu/mu2771/step#reference">
        <rdfs:subPropertyOf rdf:resource="http://www.w3.org/2002/07/owl#topDataProperty"/>
        <rdfs:domain rdf:resource="http://people.aifb.kit.edu/mu2771/step#Expertise"/>
        <rdfs:comment xml:lang="en">a reference proofing a specific expertise, a short text identifying a certificate or similar</rdfs:comment>
        <rdfs:label xml:lang="de">belegt durch Zertifikat</rdfs:label>
        <rdfs:label xml:lang="en">reference</rdfs:label>
    </owl:DatatypeProperty>
    


    <!-- http://people.aifb.kit.edu/mu2771/step#sourceURI -->

    <owl:DatatypeProperty rdf:about="http://people.aifb.kit.edu/mu2771/step#sourceURI">
        <rdfs:range rdf:resource="http://www.w3.org/2001/XMLSchema#anyURI"/>
        <rdfs:comment>identifies the resource which created/produced/made the domain instance</rdfs:comment>
        <rdfs:label>sourceURI</rdfs:label>
    </owl:DatatypeProperty>
    


    <!-- http://www.w3.org/2004/02/skos/core#notation -->

    <owl:DatatypeProperty rdf:about="http://www.w3.org/2004/02/skos/core#notation"/>
    


    <!-- http://www.w3.org/2006/time#day -->

    <owl:DatatypeProperty rdf:about="http://www.w3.org/2006/time#day">
        <rdfs:domain rdf:resource="http://www.w3.org/2006/time#GeneralDateTimeDescription"/>
        <rdfs:comment xml:lang="en">Day position in a calendar-clock system.

The range of this property is not specified, so can be replaced by any specific representation of a calendar day from any calendar. </rdfs:comment>
        <rdfs:label xml:lang="en">day</rdfs:label>
        <skos:definition xml:lang="en">Day position in a calendar-clock system.

The range of this property is not specified, so can be replaced by any specific representation of a calendar day from any calendar. </skos:definition>
    </owl:DatatypeProperty>
    


    <!-- http://www.w3.org/2006/time#dayOfYear -->

    <owl:DatatypeProperty rdf:about="http://www.w3.org/2006/time#dayOfYear">
        <rdfs:domain rdf:resource="http://www.w3.org/2006/time#GeneralDateTimeDescription"/>
        <rdfs:range rdf:resource="http://www.w3.org/2001/XMLSchema#nonNegativeInteger"/>
        <rdfs:comment xml:lang="en">The number of the day within the year</rdfs:comment>
        <rdfs:label xml:lang="en">day of year</rdfs:label>
        <skos:definition xml:lang="en">The number of the day within the year</skos:definition>
    </owl:DatatypeProperty>
    


    <!-- http://www.w3.org/2006/time#days -->

    <owl:DatatypeProperty rdf:about="http://www.w3.org/2006/time#days">
        <rdfs:domain rdf:resource="http://www.w3.org/2006/time#GeneralDurationDescription"/>
        <rdfs:range rdf:resource="http://www.w3.org/2001/XMLSchema#decimal"/>
        <rdfs:comment xml:lang="en">length of, or element of the length of, a temporal extent expressed in days</rdfs:comment>
        <rdfs:label xml:lang="en">days duration</rdfs:label>
        <skos:definition xml:lang="en">length of, or element of the length of, a temporal extent expressed in days</skos:definition>
    </owl:DatatypeProperty>
    


    <!-- http://www.w3.org/2006/time#hasXSDDuration -->

    <owl:DatatypeProperty rdf:about="http://www.w3.org/2006/time#hasXSDDuration">
        <rdfs:domain rdf:resource="http://www.w3.org/2006/time#TemporalEntity"/>
        <rdfs:range rdf:resource="http://www.w3.org/2001/XMLSchema#duration"/>
        <rdfs:comment xml:lang="en">Extent of a temporal entity, expressed using xsd:duration</rdfs:comment>
        <rdfs:label xml:lang="en">has XSD duration</rdfs:label>
        <skos:definition xml:lang="en">Extent of a temporal entity, expressed using xsd:duration</skos:definition>
        <skos:editorialNote xml:lang="en">Feature at risk - added in 2017 revision, and not yet widely used. </skos:editorialNote>
    </owl:DatatypeProperty>
    


    <!-- http://www.w3.org/2006/time#hour -->

    <owl:DatatypeProperty rdf:about="http://www.w3.org/2006/time#hour">
        <rdfs:domain rdf:resource="http://www.w3.org/2006/time#GeneralDateTimeDescription"/>
        <rdfs:domain rdf:resource="http://www.w3.org/2006/time#Instant"/>
        <rdfs:range rdf:resource="http://www.w3.org/2001/XMLSchema#nonNegativeInteger"/>
        <rdfs:comment xml:lang="en">Hour position in a calendar-clock system.</rdfs:comment>
        <rdfs:comment>the hours-of-a-day of a owl-time:Instant</rdfs:comment>
        <rdfs:label xml:lang="en">hour</rdfs:label>
        <skos:definition xml:lang="en">Hour position in a calendar-clock system.</skos:definition>
    </owl:DatatypeProperty>
    


    <!-- http://www.w3.org/2006/time#hours -->

    <owl:DatatypeProperty rdf:about="http://www.w3.org/2006/time#hours">
        <rdfs:domain rdf:resource="http://www.w3.org/2006/time#DurationDescription"/>
        <rdfs:domain rdf:resource="http://www.w3.org/2006/time#GeneralDurationDescription"/>
        <rdfs:range rdf:resource="http://www.w3.org/2001/XMLSchema#decimal"/>
        <rdfs:comment xml:lang="en">length of, or element of the length of, a temporal extent expressed in hours</rdfs:comment>
        <rdfs:label xml:lang="en">hours duration</rdfs:label>
        <skos:definition xml:lang="en">length of, or element of the length of, a temporal extent expressed in hours</skos:definition>
    </owl:DatatypeProperty>
    


    <!-- http://www.w3.org/2006/time#inXSDDate -->

    <owl:DatatypeProperty rdf:about="http://www.w3.org/2006/time#inXSDDate">
        <rdfs:domain rdf:resource="http://www.w3.org/2006/time#Instant"/>
        <rdfs:range rdf:resource="http://www.w3.org/2001/XMLSchema#date"/>
        <rdfs:comment xml:lang="en">Position of an instant, expressed using xsd:date</rdfs:comment>
        <rdfs:label xml:lang="en">in XSD date</rdfs:label>
        <skos:definition xml:lang="en">Position of an instant, expressed using xsd:date</skos:definition>
    </owl:DatatypeProperty>
    


    <!-- http://www.w3.org/2006/time#inXSDDateTime -->

    <owl:DatatypeProperty rdf:about="http://www.w3.org/2006/time#inXSDDateTime">
        <rdfs:domain rdf:resource="http://www.w3.org/2006/time#Instant"/>
        <rdfs:range rdf:resource="http://www.w3.org/2001/XMLSchema#dateTime"/>
        <rdfs:comment xml:lang="en">Position of an instant, expressed using xsd:dateTime</rdfs:comment>
        <rdfs:label xml:lang="en">in XSD Date-Time</rdfs:label>
        <owl:deprecated rdf:datatype="http://www.w3.org/2001/XMLSchema#boolean">true</owl:deprecated>
        <skos:definition xml:lang="en">Position of an instant, expressed using xsd:dateTime</skos:definition>
        <skos:note xml:lang="en">The property :inXSDDateTime is replaced by :inXSDDateTimeStamp which makes the time-zone field mandatory.</skos:note>
    </owl:DatatypeProperty>
    


    <!-- http://www.w3.org/2006/time#inXSDDateTimeStamp -->

    <owl:DatatypeProperty rdf:about="http://www.w3.org/2006/time#inXSDDateTimeStamp">
        <rdfs:domain rdf:resource="http://www.w3.org/2006/time#Instant"/>
        <rdfs:range rdf:resource="http://www.w3.org/2001/XMLSchema#dateTimeStamp"/>
        <rdfs:comment xml:lang="en">Position of an instant, expressed using xsd:dateTimeStamp</rdfs:comment>
        <rdfs:label xml:lang="en">in XSD Date-Time-Stamp</rdfs:label>
        <skos:definition xml:lang="en">Position of an instant, expressed using xsd:dateTimeStamp</skos:definition>
    </owl:DatatypeProperty>
    


    <!-- http://www.w3.org/2006/time#inXSDgYear -->

    <owl:DatatypeProperty rdf:about="http://www.w3.org/2006/time#inXSDgYear">
        <rdfs:domain rdf:resource="http://www.w3.org/2006/time#Instant"/>
        <rdfs:range rdf:resource="http://www.w3.org/2001/XMLSchema#gYear"/>
        <rdfs:comment xml:lang="en">Position of an instant, expressed using xsd:gYear</rdfs:comment>
        <rdfs:label xml:lang="en">in XSD g-Year</rdfs:label>
        <skos:definition xml:lang="en">Position of an instant, expressed using xsd:gYear</skos:definition>
    </owl:DatatypeProperty>
    


    <!-- http://www.w3.org/2006/time#inXSDgYearMonth -->

    <owl:DatatypeProperty rdf:about="http://www.w3.org/2006/time#inXSDgYearMonth">
        <rdfs:domain rdf:resource="http://www.w3.org/2006/time#Instant"/>
        <rdfs:range rdf:resource="http://www.w3.org/2001/XMLSchema#gYearMonth"/>
        <rdfs:comment xml:lang="en">Position of an instant, expressed using xsd:gYearMonth</rdfs:comment>
        <rdfs:label xml:lang="en">in XSD g-YearMonth</rdfs:label>
        <skos:definition xml:lang="en">Position of an instant, expressed using xsd:gYearMonth</skos:definition>
    </owl:DatatypeProperty>
    


    <!-- http://www.w3.org/2006/time#minute -->

    <owl:DatatypeProperty rdf:about="http://www.w3.org/2006/time#minute">
        <rdfs:domain rdf:resource="http://www.w3.org/2006/time#GeneralDateTimeDescription"/>
        <rdfs:domain rdf:resource="http://www.w3.org/2006/time#Instant"/>
        <rdfs:range rdf:resource="http://www.w3.org/2001/XMLSchema#nonNegativeInteger"/>
        <rdfs:comment xml:lang="en">Minute position in a calendar-clock system.</rdfs:comment>
        <rdfs:comment>the number of minutes-of-hour of an owl-time:Instance</rdfs:comment>
        <rdfs:label xml:lang="en">minute</rdfs:label>
        <skos:definition xml:lang="en">Minute position in a calendar-clock system.</skos:definition>
    </owl:DatatypeProperty>
    


    <!-- http://www.w3.org/2006/time#minutes -->

    <owl:DatatypeProperty rdf:about="http://www.w3.org/2006/time#minutes">
        <rdfs:domain rdf:resource="http://www.w3.org/2006/time#DurationDescription"/>
        <rdfs:domain rdf:resource="http://www.w3.org/2006/time#GeneralDurationDescription"/>
        <rdfs:range rdf:resource="http://www.w3.org/2001/XMLSchema#decimal"/>
        <rdfs:comment xml:lang="en">length, or element of, a temporal extent expressed in minutes</rdfs:comment>
        <rdfs:label xml:lang="en">minutes</rdfs:label>
        <skos:definition xml:lang="en">length, or element of, a temporal extent expressed in minutes</skos:definition>
    </owl:DatatypeProperty>
    


    <!-- http://www.w3.org/2006/time#month -->

    <owl:DatatypeProperty rdf:about="http://www.w3.org/2006/time#month">
        <rdfs:domain rdf:resource="http://www.w3.org/2006/time#GeneralDateTimeDescription"/>
        <rdfs:domain rdf:resource="http://www.w3.org/2006/time#Instant"/>
        <rdfs:range rdf:resource="http://www.w3.org/2001/XMLSchema#gMonth"/>
        <rdfs:comment xml:lang="en">Month position in a calendar-clock system.

The range of this property is not specified, so can be replaced by any specific representation of a calendar month from any calendar. </rdfs:comment>
        <rdfs:comment>the months-of-a-year of an owl-time:Instance</rdfs:comment>
        <rdfs:label xml:lang="en">month</rdfs:label>
        <skos:definition xml:lang="en">Month position in a calendar-clock system.

The range of this property is not specified, so can be replaced by any specific representation of a calendar month from any calendar. </skos:definition>
    </owl:DatatypeProperty>
    


    <!-- http://www.w3.org/2006/time#months -->

    <owl:DatatypeProperty rdf:about="http://www.w3.org/2006/time#months">
        <rdfs:domain rdf:resource="http://www.w3.org/2006/time#DurationDescription"/>
        <rdfs:domain rdf:resource="http://www.w3.org/2006/time#GeneralDurationDescription"/>
        <rdfs:range rdf:resource="http://www.w3.org/2001/XMLSchema#decimal"/>
        <rdfs:comment xml:lang="en">length of, or element of the length of, a temporal extent expressed in months</rdfs:comment>
        <rdfs:label xml:lang="en">months duration</rdfs:label>
        <skos:definition xml:lang="en">length of, or element of the length of, a temporal extent expressed in months</skos:definition>
    </owl:DatatypeProperty>
    


    <!-- http://www.w3.org/2006/time#nominalPosition -->

    <owl:DatatypeProperty rdf:about="http://www.w3.org/2006/time#nominalPosition">
        <rdfs:domain rdf:resource="http://www.w3.org/2006/time#TimePosition"/>
        <rdfs:range rdf:resource="http://www.w3.org/2001/XMLSchema#string"/>
        <rdfs:comment xml:lang="en">The (nominal) value indicating temporal position in an ordinal reference system </rdfs:comment>
        <rdfs:label xml:lang="en">Name of temporal position</rdfs:label>
        <skos:definition xml:lang="en">The (nominal) value indicating temporal position in an ordinal reference system </skos:definition>
    </owl:DatatypeProperty>
    


    <!-- http://www.w3.org/2006/time#numericDuration -->

    <owl:DatatypeProperty rdf:about="http://www.w3.org/2006/time#numericDuration">
        <rdfs:domain rdf:resource="http://www.w3.org/2006/time#Duration"/>
        <rdfs:range rdf:resource="http://www.w3.org/2001/XMLSchema#decimal"/>
        <rdfs:comment xml:lang="en">Value of a temporal extent expressed as a decimal number scaled by a temporal unit</rdfs:comment>
        <rdfs:label xml:lang="en">Numeric value of temporal duration</rdfs:label>
        <skos:definition xml:lang="en">Value of a temporal extent expressed as a decimal number scaled by a temporal unit</skos:definition>
    </owl:DatatypeProperty>
    


    <!-- http://www.w3.org/2006/time#numericPosition -->

    <owl:DatatypeProperty rdf:about="http://www.w3.org/2006/time#numericPosition">
        <rdfs:domain rdf:resource="http://www.w3.org/2006/time#TimePosition"/>
        <rdfs:range rdf:resource="http://www.w3.org/2001/XMLSchema#decimal"/>
        <rdfs:comment xml:lang="en">The (numeric) value indicating position within a temporal coordinate system </rdfs:comment>
        <rdfs:label xml:lang="en">Numeric value of temporal position</rdfs:label>
        <skos:definition xml:lang="en">The (numeric) value indicating position within a temporal coordinate system </skos:definition>
    </owl:DatatypeProperty>
    


    <!-- http://www.w3.org/2006/time#second -->

    <owl:DatatypeProperty rdf:about="http://www.w3.org/2006/time#second">
        <rdfs:domain rdf:resource="http://www.w3.org/2006/time#GeneralDateTimeDescription"/>
        <rdfs:range rdf:resource="http://www.w3.org/2001/XMLSchema#decimal"/>
        <rdfs:comment xml:lang="en">Second position in a calendar-clock system.</rdfs:comment>
        <rdfs:comment>the seconds-of-a-minute of an owl-time:Instance</rdfs:comment>
        <rdfs:label xml:lang="en">second</rdfs:label>
    </owl:DatatypeProperty>
    


    <!-- http://www.w3.org/2006/time#seconds -->

    <owl:DatatypeProperty rdf:about="http://www.w3.org/2006/time#seconds">
        <rdfs:domain rdf:resource="http://www.w3.org/2006/time#DurationDescription"/>
        <rdfs:domain rdf:resource="http://www.w3.org/2006/time#GeneralDurationDescription"/>
        <rdfs:range rdf:resource="http://www.w3.org/2001/XMLSchema#decimal"/>
        <rdfs:comment xml:lang="en">length of, or element of the length of, a temporal extent expressed in seconds</rdfs:comment>
        <rdfs:label xml:lang="en">seconds duration</rdfs:label>
        <rdfs:seeAlso rdf:resource="http://www.bipm.org/en/publications/si-brochure/second.html"/>
    </owl:DatatypeProperty>
    


    <!-- http://www.w3.org/2006/time#week -->

    <owl:DatatypeProperty rdf:about="http://www.w3.org/2006/time#week">
        <rdfs:domain rdf:resource="http://www.w3.org/2006/time#GeneralDateTimeDescription"/>
        <rdfs:range rdf:resource="http://www.w3.org/2001/XMLSchema#nonNegativeInteger"/>
        <rdfs:comment xml:lang="en">Week number within the year.</rdfs:comment>
        <rdfs:comment>the weeks-of-a-year of an owl-time:Instance</rdfs:comment>
        <rdfs:label xml:lang="en">week</rdfs:label>
        <skos:note xml:lang="en">Weeks are numbered differently depending on the calendar in use and the local language or cultural conventions (locale). ISO-8601 specifies that the first week of the year includes at least four days, and that Monday is the first day of the week. In that system, week 1 is the week that contains the first Thursday in the year.</skos:note>
    </owl:DatatypeProperty>
    


    <!-- http://www.w3.org/2006/time#weeks -->

    <owl:DatatypeProperty rdf:about="http://www.w3.org/2006/time#weeks">
        <rdfs:domain rdf:resource="http://www.w3.org/2006/time#DurationDescription"/>
        <rdfs:domain rdf:resource="http://www.w3.org/2006/time#GeneralDurationDescription"/>
        <rdfs:range rdf:resource="http://www.w3.org/2001/XMLSchema#decimal"/>
        <rdfs:comment xml:lang="en">length of, or element of the length of, a temporal extent expressed in weeks</rdfs:comment>
        <rdfs:label xml:lang="en">weeks duration</rdfs:label>
    </owl:DatatypeProperty>
    


    <!-- http://www.w3.org/2006/time#xsdDateTime -->

    <owl:DatatypeProperty rdf:about="http://www.w3.org/2006/time#xsdDateTime">
        <rdfs:domain rdf:resource="http://www.w3.org/2006/time#DateTimeInterval"/>
        <rdfs:range rdf:resource="http://www.w3.org/2001/XMLSchema#dateTime"/>
        <rdfs:comment xml:lang="en">Value of DateTimeInterval expressed as a compact value.</rdfs:comment>
        <rdfs:label xml:lang="en">has XSD date-time</rdfs:label>
        <owl:deprecated rdf:datatype="http://www.w3.org/2001/XMLSchema#boolean">true</owl:deprecated>
        <skos:note xml:lang="en">Using xsd:dateTime in this place means that the duration of the interval is implicit: it corresponds to the length of the smallest non-zero element of the date-time literal. However, this rule cannot be used for intervals whose duration is more than one rank smaller than the starting time - e.g. the first minute or second of a day, the first hour of a month, or the first day of a year. In these cases the desired interval cannot be distinguished from the interval corresponding to the next rank up. Because of this essential ambiguity, use of this property is not recommended and it is deprecated.</skos:note>
    </owl:DatatypeProperty>
    


    <!-- http://www.w3.org/2006/time#year -->

    <owl:DatatypeProperty rdf:about="http://www.w3.org/2006/time#year">
        <rdfs:domain rdf:resource="http://www.w3.org/2006/time#GeneralDateTimeDescription"/>
        <rdfs:range rdf:resource="http://www.w3.org/2001/XMLSchema#gYear"/>
        <rdfs:comment xml:lang="en">Year position in a calendar-clock system.

The range of this property is not specified, so can be replaced by any specific representation of a calendar year from any calendar. </rdfs:comment>
        <rdfs:comment>a year in the gregorian calendar</rdfs:comment>
        <rdfs:label xml:lang="en">year</rdfs:label>
    </owl:DatatypeProperty>
    


    <!-- http://www.w3.org/2006/time#years -->

    <owl:DatatypeProperty rdf:about="http://www.w3.org/2006/time#years">
        <rdfs:domain rdf:resource="http://www.w3.org/2006/time#DurationDescription"/>
        <rdfs:domain rdf:resource="http://www.w3.org/2006/time#GeneralDurationDescription"/>
        <rdfs:range rdf:resource="http://www.w3.org/2001/XMLSchema#decimal"/>
        <rdfs:comment xml:lang="en">length of, or element of the length of, a temporal extent expressed in years</rdfs:comment>
        <rdfs:label xml:lang="en">years duration</rdfs:label>
    </owl:DatatypeProperty>
    


    <!-- http://www.w3.org/2006/vcard/ns#additional-name -->

    <owl:DatatypeProperty rdf:about="http://www.w3.org/2006/vcard/ns#additional-name">
        <rdfs:range rdf:resource="http://www.w3.org/2001/XMLSchema#string"/>
        <rdfs:comment xml:lang="en">The additional name associated with the object</rdfs:comment>
        <rdfs:isDefinedBy rdf:resource="http://www.w3.org/2006/vcard/ns"/>
        <rdfs:label xml:lang="en">additional name</rdfs:label>
    </owl:DatatypeProperty>
    


    <!-- http://www.w3.org/2006/vcard/ns#anniversary -->

    <owl:DatatypeProperty rdf:about="http://www.w3.org/2006/vcard/ns#anniversary">
        <rdfs:range>
            <rdfs:Datatype>
                <owl:unionOf rdf:parseType="Collection">
                    <rdf:Description rdf:about="http://www.w3.org/2001/XMLSchema#dateTime"/>
                    <rdf:Description rdf:about="http://www.w3.org/2001/XMLSchema#gYear"/>
                </owl:unionOf>
            </rdfs:Datatype>
        </rdfs:range>
    </owl:DatatypeProperty>
    


    <!-- http://www.w3.org/2006/vcard/ns#bday -->

    <owl:DatatypeProperty rdf:about="http://www.w3.org/2006/vcard/ns#bday">
        <rdfs:range>
            <rdfs:Datatype>
                <owl:unionOf rdf:parseType="Collection">
                    <rdf:Description rdf:about="http://www.w3.org/2001/XMLSchema#dateTime"/>
                    <rdf:Description rdf:about="http://www.w3.org/2001/XMLSchema#dateTimeStamp"/>
                    <rdf:Description rdf:about="http://www.w3.org/2001/XMLSchema#gYear"/>
                </owl:unionOf>
            </rdfs:Datatype>
        </rdfs:range>
    </owl:DatatypeProperty>
    


    <!-- http://www.w3.org/2006/vcard/ns#category -->

    <owl:DatatypeProperty rdf:about="http://www.w3.org/2006/vcard/ns#category">
        <rdfs:range rdf:resource="http://www.w3.org/2001/XMLSchema#string"/>
        <rdfs:comment xml:lang="en">The category information about the object, also known as tags</rdfs:comment>
        <rdfs:isDefinedBy rdf:resource="http://www.w3.org/2006/vcard/ns"/>
        <rdfs:label xml:lang="en">category</rdfs:label>
    </owl:DatatypeProperty>
    


    <!-- http://www.w3.org/2006/vcard/ns#class -->

    <owl:DatatypeProperty rdf:about="http://www.w3.org/2006/vcard/ns#class">
        <rdfs:comment xml:lang="en">This data property has been deprecated</rdfs:comment>
        <rdfs:isDefinedBy rdf:resource="http://www.w3.org/2006/vcard/ns"/>
        <rdfs:label xml:lang="en">class</rdfs:label>
        <owl:deprecated rdf:datatype="http://www.w3.org/2001/XMLSchema#boolean">true</owl:deprecated>
    </owl:DatatypeProperty>
    


    <!-- http://www.w3.org/2006/vcard/ns#country-name -->

    <owl:DatatypeProperty rdf:about="http://www.w3.org/2006/vcard/ns#country-name">
        <rdfs:range rdf:resource="http://www.w3.org/2001/XMLSchema#string"/>
        <rdfs:comment xml:lang="en">The country name associated with the address of the object</rdfs:comment>
        <rdfs:isDefinedBy rdf:resource="http://www.w3.org/2006/vcard/ns"/>
        <rdfs:label xml:lang="en">country name</rdfs:label>
    </owl:DatatypeProperty>
    


    <!-- http://www.w3.org/2006/vcard/ns#extended-address -->

    <owl:DatatypeProperty rdf:about="http://www.w3.org/2006/vcard/ns#extended-address">
        <rdfs:comment xml:lang="en">This data property has been deprecated</rdfs:comment>
        <rdfs:isDefinedBy rdf:resource="http://www.w3.org/2006/vcard/ns"/>
        <rdfs:label xml:lang="en">extended address</rdfs:label>
        <owl:deprecated rdf:datatype="http://www.w3.org/2001/XMLSchema#boolean">true</owl:deprecated>
    </owl:DatatypeProperty>
    


    <!-- http://www.w3.org/2006/vcard/ns#family-name -->

    <owl:DatatypeProperty rdf:about="http://www.w3.org/2006/vcard/ns#family-name">
        <rdfs:range rdf:resource="http://www.w3.org/2001/XMLSchema#string"/>
        <rdfs:comment xml:lang="en">The family name associated with the object</rdfs:comment>
        <rdfs:isDefinedBy rdf:resource="http://www.w3.org/2006/vcard/ns"/>
        <rdfs:label xml:lang="en">family name</rdfs:label>
    </owl:DatatypeProperty>
    


    <!-- http://www.w3.org/2006/vcard/ns#fn -->

    <owl:DatatypeProperty rdf:about="http://www.w3.org/2006/vcard/ns#fn">
        <rdfs:range rdf:resource="http://www.w3.org/2001/XMLSchema#string"/>
        <rdfs:comment xml:lang="en">The formatted text corresponding to the name of the object</rdfs:comment>
        <rdfs:isDefinedBy rdf:resource="http://www.w3.org/2006/vcard/ns"/>
        <rdfs:label xml:lang="en">formatted name</rdfs:label>
    </owl:DatatypeProperty>
    


    <!-- http://www.w3.org/2006/vcard/ns#given-name -->

    <owl:DatatypeProperty rdf:about="http://www.w3.org/2006/vcard/ns#given-name">
        <rdfs:range rdf:resource="http://www.w3.org/2001/XMLSchema#string"/>
        <rdfs:comment xml:lang="en">The given name associated with the object</rdfs:comment>
        <rdfs:isDefinedBy rdf:resource="http://www.w3.org/2006/vcard/ns"/>
        <rdfs:label xml:lang="en">given name</rdfs:label>
    </owl:DatatypeProperty>
    


    <!-- http://www.w3.org/2006/vcard/ns#honorific-prefix -->

    <owl:DatatypeProperty rdf:about="http://www.w3.org/2006/vcard/ns#honorific-prefix">
        <rdfs:range rdf:resource="http://www.w3.org/2001/XMLSchema#string"/>
        <rdfs:comment xml:lang="en">The honorific prefix of the name associated with the object</rdfs:comment>
        <rdfs:isDefinedBy rdf:resource="http://www.w3.org/2006/vcard/ns"/>
        <rdfs:label xml:lang="en">honorific prefix</rdfs:label>
    </owl:DatatypeProperty>
    


    <!-- http://www.w3.org/2006/vcard/ns#honorific-suffix -->

    <owl:DatatypeProperty rdf:about="http://www.w3.org/2006/vcard/ns#honorific-suffix">
        <rdfs:range rdf:resource="http://www.w3.org/2001/XMLSchema#string"/>
        <rdfs:comment xml:lang="en">The honorific suffix of the name associated with the object</rdfs:comment>
        <rdfs:isDefinedBy rdf:resource="http://www.w3.org/2006/vcard/ns"/>
        <rdfs:label xml:lang="en">honorific suffix</rdfs:label>
    </owl:DatatypeProperty>
    


    <!-- http://www.w3.org/2006/vcard/ns#label -->

    <owl:DatatypeProperty rdf:about="http://www.w3.org/2006/vcard/ns#label">
        <rdfs:comment xml:lang="en">This data property has been deprecated</rdfs:comment>
        <rdfs:isDefinedBy rdf:resource="http://www.w3.org/2006/vcard/ns"/>
        <rdfs:label xml:lang="en">label</rdfs:label>
        <owl:deprecated rdf:datatype="http://www.w3.org/2001/XMLSchema#boolean">true</owl:deprecated>
    </owl:DatatypeProperty>
    


    <!-- http://www.w3.org/2006/vcard/ns#language -->

    <owl:DatatypeProperty rdf:about="http://www.w3.org/2006/vcard/ns#language">
        <rdfs:comment xml:lang="en">To specify the language that may be used for contacting the object. May also be used as a property parameter.</rdfs:comment>
        <rdfs:isDefinedBy rdf:resource="http://www.w3.org/2006/vcard/ns"/>
        <rdfs:label xml:lang="en">language</rdfs:label>
    </owl:DatatypeProperty>
    


    <!-- http://www.w3.org/2006/vcard/ns#latitude -->

    <owl:DatatypeProperty rdf:about="http://www.w3.org/2006/vcard/ns#latitude">
        <rdfs:comment xml:lang="en">This data property has been deprecated. See hasGeo</rdfs:comment>
        <rdfs:isDefinedBy rdf:resource="http://www.w3.org/2006/vcard/ns"/>
        <rdfs:label xml:lang="en">latitude</rdfs:label>
        <owl:deprecated rdf:datatype="http://www.w3.org/2001/XMLSchema#boolean">true</owl:deprecated>
    </owl:DatatypeProperty>
    


    <!-- http://www.w3.org/2006/vcard/ns#locality -->

    <owl:DatatypeProperty rdf:about="http://www.w3.org/2006/vcard/ns#locality">
        <rdfs:range rdf:resource="http://www.w3.org/2001/XMLSchema#string"/>
        <rdfs:comment xml:lang="en">The locality (e.g. city or town) associated with the address of the object</rdfs:comment>
        <rdfs:isDefinedBy rdf:resource="http://www.w3.org/2006/vcard/ns"/>
        <rdfs:label xml:lang="en">locality</rdfs:label>
    </owl:DatatypeProperty>
    


    <!-- http://www.w3.org/2006/vcard/ns#longitude -->

    <owl:DatatypeProperty rdf:about="http://www.w3.org/2006/vcard/ns#longitude">
        <rdfs:comment xml:lang="en">This data property has been deprecated. See hasGeo</rdfs:comment>
        <rdfs:isDefinedBy rdf:resource="http://www.w3.org/2006/vcard/ns"/>
        <rdfs:label xml:lang="en">longitude</rdfs:label>
        <owl:deprecated rdf:datatype="http://www.w3.org/2001/XMLSchema#boolean">true</owl:deprecated>
    </owl:DatatypeProperty>
    


    <!-- http://www.w3.org/2006/vcard/ns#mailer -->

    <owl:DatatypeProperty rdf:about="http://www.w3.org/2006/vcard/ns#mailer">
        <rdfs:comment xml:lang="en">This data property has been deprecated</rdfs:comment>
        <rdfs:isDefinedBy rdf:resource="http://www.w3.org/2006/vcard/ns"/>
        <rdfs:label xml:lang="en">mailer</rdfs:label>
        <owl:deprecated rdf:datatype="http://www.w3.org/2001/XMLSchema#boolean">true</owl:deprecated>
    </owl:DatatypeProperty>
    


    <!-- http://www.w3.org/2006/vcard/ns#nickname -->

    <owl:DatatypeProperty rdf:about="http://www.w3.org/2006/vcard/ns#nickname">
        <rdfs:range rdf:resource="http://www.w3.org/2001/XMLSchema#string"/>
        <rdfs:comment xml:lang="en">The nick name associated with the object</rdfs:comment>
        <rdfs:isDefinedBy rdf:resource="http://www.w3.org/2006/vcard/ns"/>
        <rdfs:label xml:lang="en">nickname</rdfs:label>
    </owl:DatatypeProperty>
    


    <!-- http://www.w3.org/2006/vcard/ns#note -->

    <owl:DatatypeProperty rdf:about="http://www.w3.org/2006/vcard/ns#note">
        <rdfs:range rdf:resource="http://www.w3.org/2001/XMLSchema#string"/>
        <rdfs:comment xml:lang="en">A note associated with the object</rdfs:comment>
        <rdfs:isDefinedBy rdf:resource="http://www.w3.org/2006/vcard/ns"/>
        <rdfs:label xml:lang="en">note</rdfs:label>
    </owl:DatatypeProperty>
    


    <!-- http://www.w3.org/2006/vcard/ns#organization-name -->

    <owl:DatatypeProperty rdf:about="http://www.w3.org/2006/vcard/ns#organization-name">
        <rdfs:range rdf:resource="http://www.w3.org/2001/XMLSchema#string"/>
        <rdfs:comment xml:lang="en">To specify the organizational name associated with the object</rdfs:comment>
        <rdfs:isDefinedBy rdf:resource="http://www.w3.org/2006/vcard/ns"/>
        <rdfs:label xml:lang="en">organization name</rdfs:label>
    </owl:DatatypeProperty>
    


    <!-- http://www.w3.org/2006/vcard/ns#organization-unit -->

    <owl:DatatypeProperty rdf:about="http://www.w3.org/2006/vcard/ns#organization-unit">
        <rdfs:subPropertyOf rdf:resource="http://www.w3.org/2006/vcard/ns#organization-name"/>
        <rdfs:range rdf:resource="http://www.w3.org/2001/XMLSchema#string"/>
        <rdfs:comment xml:lang="en">To specify the organizational unit name associated with the object</rdfs:comment>
        <rdfs:isDefinedBy rdf:resource="http://www.w3.org/2006/vcard/ns"/>
        <rdfs:label xml:lang="en">organizational unit name</rdfs:label>
    </owl:DatatypeProperty>
    


    <!-- http://www.w3.org/2006/vcard/ns#post-office-box -->

    <owl:DatatypeProperty rdf:about="http://www.w3.org/2006/vcard/ns#post-office-box">
        <rdfs:comment xml:lang="en">This data property has been deprecated</rdfs:comment>
        <rdfs:isDefinedBy rdf:resource="http://www.w3.org/2006/vcard/ns"/>
        <rdfs:label xml:lang="en">post office box</rdfs:label>
        <owl:deprecated rdf:datatype="http://www.w3.org/2001/XMLSchema#boolean">true</owl:deprecated>
    </owl:DatatypeProperty>
    


    <!-- http://www.w3.org/2006/vcard/ns#postal-code -->

    <owl:DatatypeProperty rdf:about="http://www.w3.org/2006/vcard/ns#postal-code">
        <rdfs:range rdf:resource="http://www.w3.org/2001/XMLSchema#string"/>
        <rdfs:comment xml:lang="en">The postal code associated with the address of the object</rdfs:comment>
        <rdfs:isDefinedBy rdf:resource="http://www.w3.org/2006/vcard/ns"/>
        <rdfs:label xml:lang="en">postal code</rdfs:label>
    </owl:DatatypeProperty>
    


    <!-- http://www.w3.org/2006/vcard/ns#prodid -->

    <owl:DatatypeProperty rdf:about="http://www.w3.org/2006/vcard/ns#prodid">
        <rdfs:range rdf:resource="http://www.w3.org/2001/XMLSchema#string"/>
        <rdfs:comment xml:lang="en">To specify the identifier for the product that created the object</rdfs:comment>
        <rdfs:isDefinedBy rdf:resource="http://www.w3.org/2006/vcard/ns"/>
        <rdfs:label xml:lang="en">product id</rdfs:label>
    </owl:DatatypeProperty>
    


    <!-- http://www.w3.org/2006/vcard/ns#region -->

    <owl:DatatypeProperty rdf:about="http://www.w3.org/2006/vcard/ns#region">
        <rdfs:range rdf:resource="http://www.w3.org/2001/XMLSchema#string"/>
        <rdfs:comment xml:lang="en">The region (e.g. state or province) associated with the address of the object</rdfs:comment>
        <rdfs:isDefinedBy rdf:resource="http://www.w3.org/2006/vcard/ns"/>
        <rdfs:label xml:lang="en">region</rdfs:label>
    </owl:DatatypeProperty>
    


    <!-- http://www.w3.org/2006/vcard/ns#rev -->

    <owl:DatatypeProperty rdf:about="http://www.w3.org/2006/vcard/ns#rev">
        <rdfs:range rdf:resource="http://www.w3.org/2001/XMLSchema#dateTime"/>
        <rdfs:comment xml:lang="en">To specify revision information about the object</rdfs:comment>
        <rdfs:isDefinedBy rdf:resource="http://www.w3.org/2006/vcard/ns"/>
        <rdfs:label xml:lang="en">revision</rdfs:label>
    </owl:DatatypeProperty>
    


    <!-- http://www.w3.org/2006/vcard/ns#role -->

    <owl:DatatypeProperty rdf:about="http://www.w3.org/2006/vcard/ns#role">
        <rdfs:range rdf:resource="http://www.w3.org/2001/XMLSchema#string"/>
        <rdfs:comment xml:lang="en">To specify the function or part played in a particular situation by the object</rdfs:comment>
        <rdfs:isDefinedBy rdf:resource="http://www.w3.org/2006/vcard/ns"/>
        <rdfs:label xml:lang="en">role</rdfs:label>
    </owl:DatatypeProperty>
    


    <!-- http://www.w3.org/2006/vcard/ns#sort-string -->

    <owl:DatatypeProperty rdf:about="http://www.w3.org/2006/vcard/ns#sort-string">
        <rdfs:range rdf:resource="http://www.w3.org/2001/XMLSchema#string"/>
        <rdfs:comment xml:lang="en">To specify the string to be used for national-language-specific sorting. Used as a property parameter only.</rdfs:comment>
        <rdfs:isDefinedBy rdf:resource="http://www.w3.org/2006/vcard/ns"/>
        <rdfs:label xml:lang="en">sort as</rdfs:label>
    </owl:DatatypeProperty>
    


    <!-- http://www.w3.org/2006/vcard/ns#street-address -->

    <owl:DatatypeProperty rdf:about="http://www.w3.org/2006/vcard/ns#street-address">
        <rdfs:range rdf:resource="http://www.w3.org/2001/XMLSchema#string"/>
        <rdfs:comment xml:lang="en">The street address associated with the address of the object</rdfs:comment>
        <rdfs:isDefinedBy rdf:resource="http://www.w3.org/2006/vcard/ns"/>
        <rdfs:label xml:lang="en">street address</rdfs:label>
    </owl:DatatypeProperty>
    


    <!-- http://www.w3.org/2006/vcard/ns#title -->

    <owl:DatatypeProperty rdf:about="http://www.w3.org/2006/vcard/ns#title">
        <rdfs:range rdf:resource="http://www.w3.org/2001/XMLSchema#string"/>
        <rdfs:comment xml:lang="en">To specify the position or job of the object</rdfs:comment>
        <rdfs:isDefinedBy rdf:resource="http://www.w3.org/2006/vcard/ns"/>
        <rdfs:label xml:lang="en">title</rdfs:label>
    </owl:DatatypeProperty>
    


    <!-- http://www.w3.org/2006/vcard/ns#tz -->

    <owl:DatatypeProperty rdf:about="http://www.w3.org/2006/vcard/ns#tz">
        <rdfs:range rdf:resource="http://www.w3.org/2001/XMLSchema#string"/>
        <rdfs:comment xml:lang="en">To indicate time zone information that is specific to the object. May also be used as a property parameter.</rdfs:comment>
        <rdfs:isDefinedBy rdf:resource="http://www.w3.org/2006/vcard/ns"/>
        <rdfs:label xml:lang="en">time zone</rdfs:label>
    </owl:DatatypeProperty>
    


    <!-- http://www.w3.org/2006/vcard/ns#value -->

    <owl:DatatypeProperty rdf:about="http://www.w3.org/2006/vcard/ns#value">
        <rdfs:comment xml:lang="en">Used to indicate the literal value of a data property that requires property parameters</rdfs:comment>
        <rdfs:isDefinedBy rdf:resource="http://www.w3.org/2006/vcard/ns"/>
        <rdfs:label xml:lang="en">value</rdfs:label>
    </owl:DatatypeProperty>
    


    <!-- http://www.w3.org/ns/org#identifier -->

    <owl:DatatypeProperty rdf:about="http://www.w3.org/ns/org#identifier">
        <rdfs:subPropertyOf rdf:resource="http://www.w3.org/2004/02/skos/core#notation"/>
        <rdfs:domain rdf:resource="http://www.w3.org/ns/org#Organization"/>
        <rdfs:comment xml:lang="es">Código o identificador, como por ejemplo el CIF de una empresa, que permite identificar de forma inequívoca a una organización. Existen muchos códigos de identificación tanto nacionales como internacionales. Esta ontología no obliga al uso de ningún esquema en concreto. Los códigos de identificación utilizados en cada caso se deberían indicar mediante el uso de la propiedad “datatype” del valor del identificador. El uso de la propiedad “datatype” para especificar el esquema de notación utilizado está en consonancia con las buenas prácticas recomendadas para el uso de la propiedad `skos:notation`, de la que esta propiedad es una especialización.</rdfs:comment>
        <rdfs:comment xml:lang="fr">Donne un identifiant, comme par exemple le numéro d&apos;enregistrement d&apos;une entreprise, qui peut être utilisé comme identifiant unique pour l&apos;Organisation. De nombreux schémas nationaux et internationaux sont disponibles. Cette ontologie reste neutre par rapport au schéma utilisé. Le schéma particulier utilisé devrait être indiqué par le `datatype` de la valeur de l&apos;identifiant. Utiliser les datatypes pour distinguer les schémas de notation est cohérent avec les bonnes pratiques pour `skos:notation` dont cette propriété est une spécialisation.</rdfs:comment>
        <rdfs:comment xml:lang="en">Gives an identifier, such as a company registration number, that can be used to used to uniquely identify the organization. Many different national and international identier schemes are available. The org ontology is neutral to which schemes are used. The particular identifier scheme should be indicated by the datatype of the identifier value.  Using datatypes to distinguish the notation scheme used is consistent with recommended best practice for `skos:notation` of which this property is a specialization.</rdfs:comment>
        <rdfs:comment xml:lang="it">Indica un identificatore univoco per l&apos;organizzazione, come ad esempio la partita IVA di un&apos;azienda. Molti schemi di identificazione a livello nazionale e internazionale sono disponibili allo scopo. L&apos;ontologia ORG è neutrale rispetto allo schema da utilizzare. Lo schema di identificazione dovrebbe essere indicato dal datatype del valore dell&apos;identificatore. L&apos;uso del datatype per distinguere lo schema di identificazione è coerente con le best practice per `skos:notation`, di cui questa proprietà è una specializzazione.</rdfs:comment>
        <rdfs:comment xml:lang="ja">組織を一意に識別するために使用できる会社登録番号などの識別子を与えます。</rdfs:comment>
        <rdfs:isDefinedBy rdf:resource="http://www.w3.org/ns/org"/>
        <rdfs:label xml:lang="fr">identifiant</rdfs:label>
        <rdfs:label xml:lang="it">identificatore</rdfs:label>
        <rdfs:label xml:lang="en">identifier</rdfs:label>
        <rdfs:label xml:lang="es">tiene identificador</rdfs:label>
    </owl:DatatypeProperty>
    


    <!-- http://www.w3.org/ns/org#location -->

    <owl:DatatypeProperty rdf:about="http://www.w3.org/ns/org#location">
        <rdfs:domain rdf:resource="http://xmlns.com/foaf/0.1/Person"/>
        <rdfs:range rdf:resource="http://www.w3.org/2001/XMLSchema#string"/>
        <rdfs:comment xml:lang="en">Gives a location description for a person within the organization, for example a _Mail Stop_ for internal posting purposes.</rdfs:comment>
        <rdfs:comment xml:lang="it">Indica la descrizione del luogo presso cui è possibile reperire una persona dell&apos;organizzazione.</rdfs:comment>
        <rdfs:comment xml:lang="fr">Indique la description de l&apos;endroit ou est basé une personne de l&apos;Organisation, par exemple pour des besoins de messagerie interne (Bureau 42).</rdfs:comment>
        <rdfs:comment xml:lang="es">Lugar o ubicación exacta de una persona en una organización con el objetivo de facilitar, por ejemplo, la entrega de correo.</rdfs:comment>
        <rdfs:comment xml:lang="ja">例えば、内部配送目的のメール・ストップ（Mail Stop）などの、組織内の人の位置記述を提供します。</rdfs:comment>
        <rdfs:isDefinedBy rdf:resource="http://www.w3.org/ns/org"/>
        <rdfs:label xml:lang="es">está ubicada en</rdfs:label>
        <rdfs:label xml:lang="es">está ubicado en</rdfs:label>
        <rdfs:label xml:lang="fr">localisation</rdfs:label>
        <rdfs:label xml:lang="en">location</rdfs:label>
        <rdfs:label xml:lang="it">luogo</rdfs:label>
    </owl:DatatypeProperty>
    


    <!-- 
    ///////////////////////////////////////////////////////////////////////////////////////
    //
    // Classes
    //
    ///////////////////////////////////////////////////////////////////////////////////////
     -->

    


    <!-- http://aifb.kit.edu/stepC#SpatialTemporalEntity -->

    <owl:Class rdf:about="http://aifb.kit.edu/stepC#SpatialTemporalEntity">
        <rdfs:label xml:lang="en">Geospatial Object</rdfs:label>
        <rdfs:label xml:lang="de">Räumlich-zeitliches Objekt</rdfs:label>
    </owl:Class>
    


    <!-- http://iirds.tekom.de/iirds#Agent -->

    <owl:Class rdf:about="http://iirds.tekom.de/iirds#Agent">
        <rdfs:subClassOf rdf:resource="http://iirds.tekom.de/iirds#iirdsDomainEntitiy"/>
        <rdfs:subClassOf rdf:resource="http://xmlns.com/foaf/0.1/Agent"/>
        <rdfs:label xml:lang="de">Agent</rdfs:label>
        <rdfs:label xml:lang="en">Agent</rdfs:label>
    </owl:Class>
    


    <!-- http://iirds.tekom.de/iirds#Component -->

    <owl:Class rdf:about="http://iirds.tekom.de/iirds#Component">
        <rdfs:subClassOf rdf:resource="http://iirds.tekom.de/iirds#ProductMetadata"/>
        <rdfs:subClassOf rdf:resource="http://purl.oclc.org/NET/ssnx/ssn#Device"/>
        <rdfs:label xml:lang="en">Component</rdfs:label>
        <rdfs:label xml:lang="de">Komponente</rdfs:label>
    </owl:Class>
    


    <!-- http://iirds.tekom.de/iirds#DirectoryNode -->

    <owl:Class rdf:about="http://iirds.tekom.de/iirds#DirectoryNode">
        <rdfs:subClassOf rdf:resource="http://iirds.tekom.de/iirds#iirdsDomainEntitiy"/>
        <www:subClassOfInverted rdf:resource="http://iirds.tekom.de/iirds#nil"/>
        <rdfs:comment xml:lang="en">English text for describing a navigation structure.</rdfs:comment>
        <rdfs:label xml:lang="en">Directory node</rdfs:label>
        <rdfs:label xml:lang="de">Verzeichnisstruktur</rdfs:label>
    </owl:Class>
    


    <!-- http://iirds.tekom.de/iirds#Document -->

    <owl:Class rdf:about="http://iirds.tekom.de/iirds#Document">
        <rdfs:subClassOf rdf:resource="http://iirds.tekom.de/iirds#InformationUnit"/>
    </owl:Class>
    


    <!-- http://iirds.tekom.de/iirds#DocumentType -->

    <owl:Class rdf:about="http://iirds.tekom.de/iirds#DocumentType">
        <rdfs:subClassOf rdf:resource="http://iirds.tekom.de/iirds#InformationType"/>
    </owl:Class>
    


    <!-- http://iirds.tekom.de/iirds#DocumentationMetadata -->

    <owl:Class rdf:about="http://iirds.tekom.de/iirds#DocumentationMetadata">
        <rdfs:subClassOf rdf:resource="http://iirds.tekom.de/iirds#iirdsDomainEntitiy"/>
    </owl:Class>
    


    <!-- http://iirds.tekom.de/iirds#Event -->

    <owl:Class rdf:about="http://iirds.tekom.de/iirds#Event">
        <rdfs:subClassOf rdf:resource="http://iirds.tekom.de/iirds#FunctionalMetadata"/>
        <rdfs:label xml:lang="de">Ereignis</rdfs:label>
        <rdfs:label xml:lang="en">Event</rdfs:label>
    </owl:Class>
    


    <!-- http://iirds.tekom.de/iirds#Fragment -->

    <owl:Class rdf:about="http://iirds.tekom.de/iirds#Fragment">
        <rdfs:subClassOf rdf:resource="http://iirds.tekom.de/iirds#InformationUnit"/>
    </owl:Class>
    


    <!-- http://iirds.tekom.de/iirds#FunctionalMetadata -->

    <owl:Class rdf:about="http://iirds.tekom.de/iirds#FunctionalMetadata">
        <rdfs:subClassOf rdf:resource="http://iirds.tekom.de/iirds#DocumentationMetadata"/>
        <www:subClassOfInverted rdf:resource="http://iirds.tekom.de/iirds#Event"/>
        <www:subClassOfInverted rdf:resource="http://iirds.tekom.de/iirds#PlanningTime"/>
        <www:subClassOfInverted rdf:resource="http://iirds.tekom.de/iirds#Qualification"/>
        <www:subClassOfInverted rdf:resource="http://iirds.tekom.de/iirds#Supplies"/>
        <rdfs:label xml:lang="en">Functional metadata</rdfs:label>
        <rdfs:label xml:lang="de">Funktionale Metadaten</rdfs:label>
    </owl:Class>
    


    <!-- http://iirds.tekom.de/iirds#InformationSubject -->

    <owl:Class rdf:about="http://iirds.tekom.de/iirds#InformationSubject">
        <rdfs:subClassOf rdf:resource="http://iirds.tekom.de/iirds#InformationType"/>
        <rdfs:label xml:lang="en">Information subject</rdfs:label>
        <rdfs:label xml:lang="de">Informationsthema</rdfs:label>
    </owl:Class>
    


    <!-- http://iirds.tekom.de/iirds#InformationType -->

    <owl:Class rdf:about="http://iirds.tekom.de/iirds#InformationType">
        <rdfs:subClassOf rdf:resource="http://iirds.tekom.de/iirds#iirdsDomainEntitiy"/>
    </owl:Class>
    


    <!-- http://iirds.tekom.de/iirds#InformationUnit -->

    <owl:Class rdf:about="http://iirds.tekom.de/iirds#InformationUnit">
        <rdfs:subClassOf rdf:resource="http://iirds.tekom.de/iirds#iirdsDomainEntitiy"/>
    </owl:Class>
    


    <!-- http://iirds.tekom.de/iirds#Package -->

    <owl:Class rdf:about="http://iirds.tekom.de/iirds#Package">
        <rdfs:subClassOf rdf:resource="http://iirds.tekom.de/iirds#InformationUnit"/>
    </owl:Class>
    


    <!-- http://iirds.tekom.de/iirds#PlanningTime -->

    <owl:Class rdf:about="http://iirds.tekom.de/iirds#PlanningTime">
        <rdfs:subClassOf rdf:resource="http://iirds.tekom.de/iirds#FunctionalMetadata"/>
        <rdfs:label xml:lang="en">Planning time</rdfs:label>
        <rdfs:label xml:lang="de">Planungszeit</rdfs:label>
    </owl:Class>
    


    <!-- http://iirds.tekom.de/iirds#Product -->

    <owl:Class rdf:about="http://iirds.tekom.de/iirds#Product">
        <rdfs:subClassOf rdf:resource="http://iirds.tekom.de/iirds#ProductMetadata"/>
    </owl:Class>
    


    <!-- http://iirds.tekom.de/iirds#ProductFeature -->

    <owl:Class rdf:about="http://iirds.tekom.de/iirds#ProductFeature">
        <rdfs:subClassOf rdf:resource="http://iirds.tekom.de/iirds#ProductMetadata"/>
        <rdfs:label xml:lang="en">Product feature</rdfs:label>
        <rdfs:label xml:lang="de">Produktmerkmal</rdfs:label>
    </owl:Class>
    


    <!-- http://iirds.tekom.de/iirds#ProductLifeCyclePhase -->

    <owl:Class rdf:about="http://iirds.tekom.de/iirds#ProductLifeCyclePhase">
        <rdfs:subClassOf rdf:resource="http://iirds.tekom.de/iirds#ProductMetadata"/>
        <rdfs:label xml:lang="en">Phase of product life cycle</rdfs:label>
        <rdfs:label xml:lang="de">Produktlebenszyklusphase</rdfs:label>
    </owl:Class>
    


    <!-- http://iirds.tekom.de/iirds#ProductMetadata -->

    <owl:Class rdf:about="http://iirds.tekom.de/iirds#ProductMetadata">
        <rdfs:subClassOf rdf:resource="http://iirds.tekom.de/iirds#DocumentationMetadata"/>
        <www:subClassOfInverted rdf:resource="http://iirds.tekom.de/iirds#Component"/>
        <www:subClassOfInverted rdf:resource="http://iirds.tekom.de/iirds#Product"/>
        <www:subClassOfInverted rdf:resource="http://iirds.tekom.de/iirds#ProductFeature"/>
        <www:subClassOfInverted rdf:resource="http://iirds.tekom.de/iirds#ProductLifeCyclePhase"/>
        <rdfs:label xml:lang="en">ProductMetadata</rdfs:label>
        <rdfs:label xml:lang="de">ProduktMetadaten</rdfs:label>
    </owl:Class>
    


    <!-- http://iirds.tekom.de/iirds#Qualification -->

    <owl:Class rdf:about="http://iirds.tekom.de/iirds#Qualification">
        <rdfs:subClassOf rdf:resource="http://iirds.tekom.de/iirds#FunctionalMetadata"/>
        <www:subClassOfInverted rdf:resource="http://iirds.tekom.de/iirds#Role"/>
        <www:subClassOfInverted rdf:resource="http://iirds.tekom.de/iirds#SkillLevel"/>
        <rdfs:label xml:lang="en">Qualification</rdfs:label>
        <rdfs:label xml:lang="de">Qualifikation</rdfs:label>
    </owl:Class>
    


    <!-- http://iirds.tekom.de/iirds#Role -->

    <owl:Class rdf:about="http://iirds.tekom.de/iirds#Role">
        <rdfs:subClassOf rdf:resource="http://iirds.tekom.de/iirds#Qualification"/>
        <rdfs:comment xml:lang="de">Menge von zusammenhängenden Verhaltensweisen, Berechtigungen und Verpflichtungen, die Nutzern (Menschen, Softwareprozesse oder Geräte) eines Systems zugeordnet sind</rdfs:comment>
        <rdfs:comment xml:lang="en">Set of connected behaviors, privileges and obligations associated with users (humans, software processes or devices) of a system</rdfs:comment>
        <rdfs:label xml:lang="en">Role</rdfs:label>
        <rdfs:label xml:lang="de">Rolle</rdfs:label>
    </owl:Class>
    


    <!-- http://iirds.tekom.de/iirds#SkillLevel -->

    <owl:Class rdf:about="http://iirds.tekom.de/iirds#SkillLevel">
        <rdfs:subClassOf rdf:resource="http://iirds.tekom.de/iirds#Qualification"/>
        <rdfs:label xml:lang="de">Kenntnisstufe</rdfs:label>
        <rdfs:label xml:lang="en">Skill level</rdfs:label>
    </owl:Class>
    


    <!-- http://iirds.tekom.de/iirds#Supplies -->

    <owl:Class rdf:about="http://iirds.tekom.de/iirds#Supplies">
        <rdfs:subClassOf rdf:resource="http://iirds.tekom.de/iirds#FunctionalMetadata"/>
        <rdfs:label xml:lang="de">Hilfsmittel</rdfs:label>
        <rdfs:label xml:lang="en">Supplies</rdfs:label>
    </owl:Class>
    


    <!-- http://iirds.tekom.de/iirds#Topic -->

    <owl:Class rdf:about="http://iirds.tekom.de/iirds#Topic">
        <rdfs:subClassOf rdf:resource="http://iirds.tekom.de/iirds#InformationUnit"/>
    </owl:Class>
    


    <!-- http://iirds.tekom.de/iirds#TopicType -->

    <owl:Class rdf:about="http://iirds.tekom.de/iirds#TopicType">
        <rdfs:subClassOf rdf:resource="http://iirds.tekom.de/iirds#InformationType"/>
    </owl:Class>
    


    <!-- http://iirds.tekom.de/iirds#iirdsDomainEntitiy -->

    <owl:Class rdf:about="http://iirds.tekom.de/iirds#iirdsDomainEntitiy">
        <rdfs:subClassOf rdf:resource="http://www.loa-cnr.it/ontologies/DUL.owl#InformationObject"/>
        <www:subClassOfInverted rdf:resource="http://iirds.tekom.de/iirds#Agent"/>
        <www:subClassOfInverted rdf:resource="http://iirds.tekom.de/iirds#DirectoryNode"/>
        <www:subClassOfInverted rdf:resource="http://iirds.tekom.de/iirds#DocumentationMetadata"/>
        <www:subClassOfInverted rdf:resource="http://iirds.tekom.de/iirds#InformationType"/>
        <www:subClassOfInverted rdf:resource="http://iirds.tekom.de/iirds#InformationUnit"/>
        <rdfs:label xml:lang="de">iirdsDomainEntitiy</rdfs:label>
        <rdfs:label xml:lang="en">iirdsDomainEntitiy</rdfs:label>
    </owl:Class>
    


    <!-- http://iirds.tekom.de/iirds#nil -->

    <owl:Class rdf:about="http://iirds.tekom.de/iirds#nil">
        <rdfs:subClassOf rdf:resource="http://iirds.tekom.de/iirds#DirectoryNode"/>
        <rdfs:comment xml:lang="en">English text for describing the end of a navigation structure.</rdfs:comment>
        <rdfs:label xml:lang="de">Ende einer Verzeichnisstruktur</rdfs:label>
        <rdfs:label xml:lang="en">end of a directory structure</rdfs:label>
    </owl:Class>
    


    <!-- http://ontology.tno.nl/saref/#OnState -->

    <owl:Class rdf:about="http://ontology.tno.nl/saref/#OnState"/>
    


    <!-- http://people.aifb.kit.edu/mu2771/step#Alarm -->

    <owl:Class rdf:about="http://people.aifb.kit.edu/mu2771/step#Alarm">
        <rdfs:subClassOf rdf:resource="http://www.loa-cnr.it/ontologies/DUL.owl#InformationObject"/>
        <rdfs:comment xml:lang="en">an alarm instance information about an urgent machine failure</rdfs:comment>
        <rdfs:label xml:lang="de">Alarm</rdfs:label>
        <rdfs:label xml:lang="en">alarm</rdfs:label>
    </owl:Class>
    


    <!-- http://people.aifb.kit.edu/mu2771/step#ElectronicMessage -->

    <owl:Class rdf:about="http://people.aifb.kit.edu/mu2771/step#ElectronicMessage">
        <rdfs:subClassOf rdf:resource="http://www.loa-cnr.it/ontologies/DUL.owl#InformationObject"/>
        <rdfs:comment xml:lang="en">an electronic message is sent automatically and informs the service organization about uncommon behaviour or breakdowns</rdfs:comment>
        <rdfs:label xml:lang="en">e call</rdfs:label>
        <rdfs:label xml:lang="en">electronic message</rdfs:label>
        <rdfs:label xml:lang="de">elektronische Nachricht</rdfs:label>
    </owl:Class>
    


    <!-- http://people.aifb.kit.edu/mu2771/step#Expertise -->

    <owl:Class rdf:about="http://people.aifb.kit.edu/mu2771/step#Expertise">
        <rdfs:comment xml:lang="en">experience and knowledge of a person (mainly technicians)</rdfs:comment>
        <rdfs:label xml:lang="en">Expertise</rdfs:label>
        <rdfs:label xml:lang="de">Qualifikation</rdfs:label>
    </owl:Class>
    


    <!-- http://people.aifb.kit.edu/mu2771/step#FinishedWorkOrder -->

    <owl:Class rdf:about="http://people.aifb.kit.edu/mu2771/step#FinishedWorkOrder">
        <rdfs:subClassOf rdf:resource="http://people.aifb.kit.edu/mu2771/step#WorkOrder"/>
        <rdfs:subClassOf>
            <owl:Class>
                <owl:intersectionOf rdf:parseType="Collection">
                    <owl:Restriction>
                        <owl:onProperty rdf:resource="http://people.aifb.kit.edu/mu2771/step#wasNewWorkOrder"/>
                        <owl:maxQualifiedCardinality rdf:datatype="http://www.w3.org/2001/XMLSchema#nonNegativeInteger">1</owl:maxQualifiedCardinality>
                        <owl:onClass rdf:resource="http://people.aifb.kit.edu/mu2771/step#NewWorkOrder"/>
                    </owl:Restriction>
                    <owl:Restriction>
                        <owl:onProperty rdf:resource="http://people.aifb.kit.edu/mu2771/step#wasScheduledWorkOrder"/>
                        <owl:maxQualifiedCardinality rdf:datatype="http://www.w3.org/2001/XMLSchema#nonNegativeInteger">1</owl:maxQualifiedCardinality>
                        <owl:onClass rdf:resource="http://people.aifb.kit.edu/mu2771/step#ScheduledWorkOrder"/>
                    </owl:Restriction>
                    <owl:Restriction>
                        <owl:onProperty rdf:resource="http://people.aifb.kit.edu/mu2771/step#wasUnplanedWorkOrder"/>
                        <owl:maxQualifiedCardinality rdf:datatype="http://www.w3.org/2001/XMLSchema#nonNegativeInteger">1</owl:maxQualifiedCardinality>
                        <owl:onClass rdf:resource="http://people.aifb.kit.edu/mu2771/step#UnplannedWorkOrder"/>
                    </owl:Restriction>
                </owl:intersectionOf>
            </owl:Class>
        </rdfs:subClassOf>
    </owl:Class>
    


    <!-- http://people.aifb.kit.edu/mu2771/step#NewWorkOrder -->

    <owl:Class rdf:about="http://people.aifb.kit.edu/mu2771/step#NewWorkOrder">
        <rdfs:subClassOf rdf:resource="http://people.aifb.kit.edu/mu2771/step#WorkOrder"/>
        <rdfs:subClassOf>
            <owl:Restriction>
                <owl:onProperty rdf:resource="http://people.aifb.kit.edu/mu2771/step#wasFinishedWorkOrder"/>
                <owl:maxQualifiedCardinality rdf:datatype="http://www.w3.org/2001/XMLSchema#nonNegativeInteger">1</owl:maxQualifiedCardinality>
                <owl:onClass rdf:resource="http://people.aifb.kit.edu/mu2771/step#FinishedWorkOrder"/>
            </owl:Restriction>
        </rdfs:subClassOf>
        <rdfs:label xml:lang="de">neuer Auftrag</rdfs:label>
        <rdfs:label xml:lang="en">new work order</rdfs:label>
    </owl:Class>
    


    <!-- http://people.aifb.kit.edu/mu2771/step#Prediction -->

    <owl:Class rdf:about="http://people.aifb.kit.edu/mu2771/step#Prediction">
        <rdfs:subClassOf rdf:resource="http://www.loa-cnr.it/ontologies/DUL.owl#InformationObject"/>
        <rdfs:comment xml:lang="en">a prediction instance has the information delivered by a predictive maintenance algortihm and describes the probability of a failure</rdfs:comment>
        <rdfs:label xml:lang="en">Prediction</rdfs:label>
        <rdfs:label xml:lang="de">Vorhersage</rdfs:label>
        <rdfs:label xml:lang="en">prediction</rdfs:label>
    </owl:Class>
    


    <!-- http://people.aifb.kit.edu/mu2771/step#Priority -->

    <owl:Class rdf:about="http://people.aifb.kit.edu/mu2771/step#Priority">
        <rdfs:comment xml:lang="en">Priority of some topic. Higher Priority values imply higher importance.</rdfs:comment>
        <rdfs:label xml:lang="en">Priority</rdfs:label>
        <rdfs:label xml:lang="de">Priorität</rdfs:label>
    </owl:Class>
    


    <!-- http://people.aifb.kit.edu/mu2771/step#Process -->

    <owl:Class rdf:about="http://people.aifb.kit.edu/mu2771/step#Process"/>
    


    <!-- http://people.aifb.kit.edu/mu2771/step#Product -->

    <owl:Class rdf:about="http://people.aifb.kit.edu/mu2771/step#Product"/>
    


    <!-- http://people.aifb.kit.edu/mu2771/step#Report -->

    <owl:Class rdf:about="http://people.aifb.kit.edu/mu2771/step#Report">
        <rdfs:subClassOf rdf:resource="http://www.loa-cnr.it/ontologies/DUL.owl#InformationObject"/>
        <rdfs:subClassOf>
            <owl:Restriction>
                <owl:onProperty rdf:resource="http://purl.oclc.org/NET/ssnx/ssn#hasValue"/>
                <owl:someValuesFrom rdf:resource="http://purl.oclc.org/NET/ssnx/ssn#ObservationValue"/>
            </owl:Restriction>
        </rdfs:subClassOf>
        <rdfs:subClassOf>
            <owl:Restriction>
                <owl:onProperty rdf:resource="http://purl.oclc.org/NET/ssnx/ssn#isProducedBy"/>
                <owl:someValuesFrom rdf:resource="http://purl.oclc.org/NET/ssnx/ssn#System"/>
            </owl:Restriction>
        </rdfs:subClassOf>
        <rdfs:comment xml:lang="en">a somehow aggregated form of sensor data. ssn:ObservationValues can be connected by using ssn:hasValue</rdfs:comment>
        <rdfs:label xml:lang="en">Activity Report</rdfs:label>
        <rdfs:label xml:lang="de">Tätigkeitsbericht</rdfs:label>
    </owl:Class>
    


    <!-- http://people.aifb.kit.edu/mu2771/step#Route -->

    <owl:Class rdf:about="http://people.aifb.kit.edu/mu2771/step#Route">
        <rdfs:subClassOf>
            <owl:Class>
                <owl:intersectionOf rdf:parseType="Collection">
                    <owl:Restriction>
                        <owl:onProperty rdf:resource="http://people.aifb.kit.edu/mu2771/step#hasWorkOrder"/>
                        <owl:someValuesFrom rdf:resource="http://people.aifb.kit.edu/mu2771/step#WorkOrder"/>
                    </owl:Restriction>
                    <owl:Restriction>
                        <owl:onProperty rdf:resource="http://people.aifb.kit.edu/mu2771/step#date"/>
                        <owl:minQualifiedCardinality rdf:datatype="http://www.w3.org/2001/XMLSchema#nonNegativeInteger">1</owl:minQualifiedCardinality>
                        <owl:onClass rdf:resource="http://www.w3.org/2006/time#Interval"/>
                    </owl:Restriction>
                    <owl:Restriction>
                        <owl:onProperty rdf:resource="http://people.aifb.kit.edu/mu2771/step#isExecutedBy"/>
                        <owl:minQualifiedCardinality rdf:datatype="http://www.w3.org/2001/XMLSchema#nonNegativeInteger">1</owl:minQualifiedCardinality>
                        <owl:onClass rdf:resource="http://people.aifb.kit.edu/mu2771/step#Technician"/>
                    </owl:Restriction>
                </owl:intersectionOf>
            </owl:Class>
        </rdfs:subClassOf>
    </owl:Class>
    


    <!-- http://people.aifb.kit.edu/mu2771/step#ScheduledWorkOrder -->

    <owl:Class rdf:about="http://people.aifb.kit.edu/mu2771/step#ScheduledWorkOrder">
        <rdfs:subClassOf rdf:resource="http://people.aifb.kit.edu/mu2771/step#WorkOrder"/>
        <rdfs:subClassOf>
            <owl:Class>
                <owl:intersectionOf rdf:parseType="Collection">
                    <owl:Restriction>
                        <owl:onProperty rdf:resource="http://people.aifb.kit.edu/mu2771/step#wasNewWorkOrder"/>
                        <owl:maxQualifiedCardinality rdf:datatype="http://www.w3.org/2001/XMLSchema#nonNegativeInteger">1</owl:maxQualifiedCardinality>
                        <owl:onClass rdf:resource="http://people.aifb.kit.edu/mu2771/step#NewWorkOrder"/>
                    </owl:Restriction>
                    <owl:Restriction>
                        <owl:onProperty rdf:resource="http://people.aifb.kit.edu/mu2771/step#wasUnplanedWorkOrder"/>
                        <owl:maxQualifiedCardinality rdf:datatype="http://www.w3.org/2001/XMLSchema#nonNegativeInteger">1</owl:maxQualifiedCardinality>
                        <owl:onClass rdf:resource="http://people.aifb.kit.edu/mu2771/step#UnplannedWorkOrder"/>
                    </owl:Restriction>
                </owl:intersectionOf>
            </owl:Class>
        </rdfs:subClassOf>
    </owl:Class>
    


    <!-- http://people.aifb.kit.edu/mu2771/step#Scheduler -->

    <owl:Class rdf:about="http://people.aifb.kit.edu/mu2771/step#Scheduler">
        <rdfs:subClassOf rdf:resource="http://xmlns.com/foaf/0.1/Person"/>
    </owl:Class>
    


    <!-- http://people.aifb.kit.edu/mu2771/step#Spare_Part -->

    <owl:Class rdf:about="http://people.aifb.kit.edu/mu2771/step#Spare_Part"/>
    


    <!-- http://people.aifb.kit.edu/mu2771/step#SpatialTemporalEntity -->

    <owl:Class rdf:about="http://people.aifb.kit.edu/mu2771/step#SpatialTemporalEntity">
        <rdfs:subClassOf rdf:resource="http://www.w3.org/2003/01/geo/wgs84_pos#SpatialThing"/>
        <rdfs:subClassOf rdf:resource="http://www.w3.org/2006/time#Instant"/>
        <rdfs:subClassOf>
            <owl:Restriction>
                <owl:onProperty rdf:resource="http://people.aifb.kit.edu/mu2771/step#date"/>
                <owl:qualifiedCardinality rdf:datatype="http://www.w3.org/2001/XMLSchema#nonNegativeInteger">1</owl:qualifiedCardinality>
                <owl:onClass rdf:resource="http://www.w3.org/2006/time#Instant"/>
            </owl:Restriction>
        </rdfs:subClassOf>
        <rdfs:subClassOf>
            <owl:Restriction>
                <owl:onProperty rdf:resource="http://www.w3.org/2003/01/geo/wgs84_pos#location"/>
                <owl:qualifiedCardinality rdf:datatype="http://www.w3.org/2001/XMLSchema#nonNegativeInteger">1</owl:qualifiedCardinality>
                <owl:onClass rdf:resource="http://www.w3.org/2003/01/geo/wgs84_pos#SpatialThing"/>
            </owl:Restriction>
        </rdfs:subClassOf>
        <rdfs:comment xml:lang="en">contains both a spatial and a temporal dimension and is a defined point in space and time in contrast to wgs84:SpatialThing or owl-time:TemporalEntity which only cover one of both by default</rdfs:comment>
    </owl:Class>
    


    <!-- http://people.aifb.kit.edu/mu2771/step#Technician -->

    <owl:Class rdf:about="http://people.aifb.kit.edu/mu2771/step#Technician">
        <rdfs:subClassOf rdf:resource="http://xmlns.com/foaf/0.1/Person"/>
        <rdfs:subClassOf>
            <owl:Class>
                <owl:unionOf rdf:parseType="Collection">
                    <owl:Restriction>
                        <owl:onProperty rdf:resource="http://people.aifb.kit.edu/mu2771/step#isAvailableAt"/>
                        <owl:minQualifiedCardinality rdf:datatype="http://www.w3.org/2001/XMLSchema#nonNegativeInteger">1</owl:minQualifiedCardinality>
                        <owl:onClass rdf:resource="http://www.w3.org/2003/01/geo/wgs84_pos#SpatialThing"/>
                    </owl:Restriction>
                    <owl:Restriction>
                        <owl:onProperty rdf:resource="http://www.w3.org/2006/vcard/ns#hasAddress"/>
                        <owl:minQualifiedCardinality rdf:datatype="http://www.w3.org/2001/XMLSchema#nonNegativeInteger">1</owl:minQualifiedCardinality>
                        <owl:onClass rdf:resource="http://www.w3.org/2006/vcard/ns#Address"/>
                    </owl:Restriction>
                </owl:unionOf>
            </owl:Class>
        </rdfs:subClassOf>
    </owl:Class>
    


    <!-- http://people.aifb.kit.edu/mu2771/step#Tool -->

    <owl:Class rdf:about="http://people.aifb.kit.edu/mu2771/step#Tool">
        <rdfs:subClassOf rdf:resource="http://purl.oclc.org/NET/ssnx/ssn#Device"/>
    </owl:Class>
    


    <!-- http://people.aifb.kit.edu/mu2771/step#UnplannedWorkOrder -->

    <owl:Class rdf:about="http://people.aifb.kit.edu/mu2771/step#UnplannedWorkOrder">
        <rdfs:subClassOf rdf:resource="http://people.aifb.kit.edu/mu2771/step#WorkOrder"/>
        <rdfs:subClassOf>
            <owl:Restriction>
                <owl:onProperty rdf:resource="http://people.aifb.kit.edu/mu2771/step#wasNewWorkOrder"/>
                <owl:maxQualifiedCardinality rdf:datatype="http://www.w3.org/2001/XMLSchema#nonNegativeInteger">1</owl:maxQualifiedCardinality>
                <owl:onClass rdf:resource="http://people.aifb.kit.edu/mu2771/step#NewWorkOrder"/>
            </owl:Restriction>
        </rdfs:subClassOf>
        <rdfs:label xml:lang="de">Ungeplanter Auftrag</rdfs:label>
        <rdfs:label xml:lang="en">unplanned work order</rdfs:label>
    </owl:Class>
    


    <!-- http://people.aifb.kit.edu/mu2771/step#WorkOrder -->

    <owl:Class rdf:about="http://people.aifb.kit.edu/mu2771/step#WorkOrder">
        <rdfs:subClassOf>
            <owl:Class>
                <owl:intersectionOf rdf:parseType="Collection">
                    <owl:Restriction>
                        <owl:onProperty rdf:resource="http://people.aifb.kit.edu/mu2771/step#requieredExpertise"/>
                        <owl:someValuesFrom rdf:resource="http://people.aifb.kit.edu/mu2771/step#Expertise"/>
                    </owl:Restriction>
                    <owl:Restriction>
                        <owl:onProperty rdf:resource="http://www.w3.org/2006/time#hasDuration"/>
                        <owl:minQualifiedCardinality rdf:datatype="http://www.w3.org/2001/XMLSchema#nonNegativeInteger">1</owl:minQualifiedCardinality>
                        <owl:onClass rdf:resource="http://www.w3.org/2006/time#Duration"/>
                    </owl:Restriction>
                    <owl:Restriction>
                        <owl:onProperty rdf:resource="http://www.w3.org/2006/time#hasTime"/>
                        <owl:minQualifiedCardinality rdf:datatype="http://www.w3.org/2001/XMLSchema#nonNegativeInteger">1</owl:minQualifiedCardinality>
                        <owl:onClass rdf:resource="http://www.w3.org/2006/time#Interval"/>
                    </owl:Restriction>
                    <owl:Restriction>
                        <owl:onProperty rdf:resource="http://www.w3.org/2003/01/geo/wgs84_pos#location"/>
                        <owl:qualifiedCardinality rdf:datatype="http://www.w3.org/2001/XMLSchema#nonNegativeInteger">1</owl:qualifiedCardinality>
                        <owl:onClass rdf:resource="http://www.w3.org/2003/01/geo/wgs84_pos#SpatialThing"/>
                    </owl:Restriction>
                    <owl:Restriction>
                        <owl:onProperty rdf:resource="http://people.aifb.kit.edu/mu2771/step#hasPriority"/>
                        <owl:maxQualifiedCardinality rdf:datatype="http://www.w3.org/2001/XMLSchema#nonNegativeInteger">1</owl:maxQualifiedCardinality>
                        <owl:onClass rdf:resource="http://people.aifb.kit.edu/mu2771/step#Priority"/>
                    </owl:Restriction>
                </owl:intersectionOf>
            </owl:Class>
        </rdfs:subClassOf>
        <www:subClassOfInverted rdf:resource="http://people.aifb.kit.edu/mu2771/step#FinishedWorkOrder"/>
        <www:subClassOfInverted rdf:resource="http://people.aifb.kit.edu/mu2771/step#NewWorkOrder"/>
        <www:subClassOfInverted rdf:resource="http://people.aifb.kit.edu/mu2771/step#ScheduledWorkOrder"/>
        <www:subClassOfInverted rdf:resource="http://people.aifb.kit.edu/mu2771/step#UnplannedWorkOrder"/>
    </owl:Class>
    


    <!-- http://purl.oclc.org/NET/ssnx/ssn#Accuracy -->

    <owl:Class rdf:about="http://purl.oclc.org/NET/ssnx/ssn#Accuracy">
        <rdfs:subClassOf rdf:resource="http://purl.oclc.org/NET/ssnx/ssn#MeasurementProperty"/>
        <dc:source>skos:exactMatch &apos;measurement accuracy/accuracy&apos; [VIM 2.13] 
		                    http://www.bipm.org/utils/common/documents/jcgm/JCGM_200_2008.pdf</dc:source>
        <rdfs:comment>The closeness of agreement between the value of an observation and the true value of the observed quality.</rdfs:comment>
        <rdfs:isDefinedBy>http://purl.oclc.org/NET/ssnx/ssn</rdfs:isDefinedBy>
        <rdfs:label>Accuracy</rdfs:label>
        <rdfs:seeAlso>http://www.w3.org/2005/Incubator/ssn/wiki/SSN_Sensor#MeasuringCapability</rdfs:seeAlso>
    </owl:Class>
    


    <!-- http://purl.oclc.org/NET/ssnx/ssn#BatteryLifetime -->

    <owl:Class rdf:about="http://purl.oclc.org/NET/ssnx/ssn#BatteryLifetime">
        <rdfs:subClassOf rdf:resource="http://purl.oclc.org/NET/ssnx/ssn#SurvivalProperty"/>
        <rdfs:comment>Total useful life of a battery.</rdfs:comment>
        <rdfs:isDefinedBy>http://purl.oclc.org/NET/ssnx/ssn</rdfs:isDefinedBy>
        <rdfs:label>Battery Lifetime</rdfs:label>
        <rdfs:seeAlso>http://www.w3.org/2005/Incubator/ssn/wiki/SSN_Energy#EnergyRestriction</rdfs:seeAlso>
    </owl:Class>
    


    <!-- http://purl.oclc.org/NET/ssnx/ssn#Condition -->

    <owl:Class rdf:about="http://purl.oclc.org/NET/ssnx/ssn#Condition">
        <rdfs:subClassOf rdf:resource="http://purl.oclc.org/NET/ssnx/ssn#Property"/>
        <rdfs:comment>Used to specify ranges for qualities that act as conditions on a system/sensor&apos;s operation.  For example, wind speed of 10-60m/s is expressed as a condition linking a quality, wind speed, a unit of measurement, metres per second, and a set of values, 10-60, and may be used as the condition on a MeasurementProperty, for example, to state that a sensor has a particular accuracy in that condition.</rdfs:comment>
        <rdfs:isDefinedBy>http://purl.oclc.org/NET/ssnx/ssn</rdfs:isDefinedBy>
        <rdfs:label>Condition</rdfs:label>
        <rdfs:seeAlso>http://www.w3.org/2005/Incubator/ssn/wiki/SSN_Base#ConstraintBlock</rdfs:seeAlso>
    </owl:Class>
    


    <!-- http://purl.oclc.org/NET/ssnx/ssn#Deployment -->

    <owl:Class rdf:about="http://purl.oclc.org/NET/ssnx/ssn#Deployment">
        <rdfs:subClassOf rdf:resource="http://purl.oclc.org/NET/ssnx/ssn#DeploymentRelatedProcess"/>
        <rdfs:subClassOf>
            <owl:Restriction>
                <owl:onProperty rdf:resource="http://purl.oclc.org/NET/ssnx/ssn#deployedOnPlatform"/>
                <owl:allValuesFrom rdf:resource="http://purl.oclc.org/NET/ssnx/ssn#Platform"/>
            </owl:Restriction>
        </rdfs:subClassOf>
        <rdfs:subClassOf>
            <owl:Restriction>
                <owl:onProperty rdf:resource="http://purl.oclc.org/NET/ssnx/ssn#deployedSystem"/>
                <owl:allValuesFrom rdf:resource="http://purl.oclc.org/NET/ssnx/ssn#System"/>
            </owl:Restriction>
        </rdfs:subClassOf>
        <dc:source>skos:closeMatch &apos;Deployment&apos; [MMI Dev]
                                 http://marinemetadata.org/community/teams/ontdevices</dc:source>
        <rdfs:comment>The ongoing Process of Entities (for the purposes of this ontology, mainly sensors) deployed for a particular purpose.  For example, a particular Sensor deployed on a Platform, or a whole network of Sensors deployed for an observation campaign.  The deployment may have sub processes, such as installation, maintenance, addition, and decomissioning and removal.</rdfs:comment>
        <rdfs:isDefinedBy>http://purl.oclc.org/NET/ssnx/ssn</rdfs:isDefinedBy>
        <rdfs:label>Deployment</rdfs:label>
        <rdfs:seeAlso>http://www.w3.org/2005/Incubator/ssn/wiki/SSN_Deploy#Deployment</rdfs:seeAlso>
    </owl:Class>
    


    <!-- http://purl.oclc.org/NET/ssnx/ssn#DeploymentRelatedProcess -->

    <owl:Class rdf:about="http://purl.oclc.org/NET/ssnx/ssn#DeploymentRelatedProcess">
        <rdfs:subClassOf rdf:resource="http://www.loa-cnr.it/ontologies/DUL.owl#Process"/>
        <rdfs:subClassOf>
            <owl:Restriction>
                <owl:onProperty rdf:resource="http://purl.oclc.org/NET/ssnx/ssn#deploymentProcessPart"/>
                <owl:allValuesFrom rdf:resource="http://purl.oclc.org/NET/ssnx/ssn#DeploymentRelatedProcess"/>
            </owl:Restriction>
        </rdfs:subClassOf>
        <dc:source>http://www.w3.org/2005/Incubator/ssn/</dc:source>
        <www:subClassOfInverted rdf:resource="http://purl.oclc.org/NET/ssnx/ssn#Deployment"/>
        <rdfs:comment>Place to group all the various Processes related to Deployment.  For example, as well as Deplyment, installation, maintenance, deployment of further sensors and the like would all be classified under DeploymentRelatedProcess.</rdfs:comment>
        <rdfs:isDefinedBy>http://purl.oclc.org/NET/ssnx/ssn</rdfs:isDefinedBy>
        <rdfs:label>Deployment-related Process</rdfs:label>
        <rdfs:seeAlso>http://www.w3.org/2005/Incubator/ssn/wiki/SSN_Deploy#Deployment</rdfs:seeAlso>
    </owl:Class>
    


    <!-- http://purl.oclc.org/NET/ssnx/ssn#DetectionLimit -->

    <owl:Class rdf:about="http://purl.oclc.org/NET/ssnx/ssn#DetectionLimit">
        <rdfs:subClassOf rdf:resource="http://purl.oclc.org/NET/ssnx/ssn#MeasurementProperty"/>
        <dc:source>skos:exactMatch &apos;detection limit&apos; [VIM 4.18] 
                                 http://www.bipm.org/utils/common/documents/jcgm/JCGM_200_2008.pdf</dc:source>
        <rdfs:comment>An observed value for which the probability of falsely claiming the absence of a component in a material is Î², given a probability Î± of falsely claiming its presence.</rdfs:comment>
        <rdfs:isDefinedBy>http://purl.oclc.org/NET/ssnx/ssn</rdfs:isDefinedBy>
        <rdfs:label>detection limit</rdfs:label>
        <rdfs:seeAlso>http://www.w3.org/2005/Incubator/ssn/wiki/SSN_Sensor#MeasuringCapability</rdfs:seeAlso>
    </owl:Class>
    


    <!-- http://purl.oclc.org/NET/ssnx/ssn#Device -->

    <owl:Class rdf:about="http://purl.oclc.org/NET/ssnx/ssn#Device">
        <rdfs:subClassOf rdf:resource="http://purl.oclc.org/NET/ssnx/ssn#System"/>
        <rdfs:subClassOf rdf:resource="http://www.loa-cnr.it/ontologies/DUL.owl#DesignedArtifact"/>
        <dc:source>http://www.w3.org/2005/Incubator/ssn/</dc:source>
        <www:subClassOfInverted rdf:resource="http://iirds.tekom.de/iirds#Component"/>
        <www:subClassOfInverted rdf:resource="http://people.aifb.kit.edu/mu2771/step#Tool"/>
        <www:subClassOfInverted rdf:resource="http://purl.oclc.org/NET/ssnx/ssn#SensingDevice"/>
        <rdfs:comment>A device is a physical piece of technology - a system in a box. Devices may of course be built of smaller devices and software components (i.e. systems have components).</rdfs:comment>
        <rdfs:isDefinedBy>http://purl.oclc.org/NET/ssnx/ssn</rdfs:isDefinedBy>
        <rdfs:label>Device</rdfs:label>
        <rdfs:label>ssn:Device</rdfs:label>
        <rdfs:seeAlso>http://www.w3.org/2005/Incubator/ssn/wiki/SSN_Device#Device</rdfs:seeAlso>
    </owl:Class>
    


    <!-- http://purl.oclc.org/NET/ssnx/ssn#Drift -->

    <owl:Class rdf:about="http://purl.oclc.org/NET/ssnx/ssn#Drift">
        <rdfs:subClassOf rdf:resource="http://purl.oclc.org/NET/ssnx/ssn#MeasurementProperty"/>
        <dc:source>skos:exactMatch &apos;instrumental drift&apos; [VIM 4.21]
                                  http://www.bipm.org/utils/common/documents/jcgm/JCGM_200_2008.pdf</dc:source>
        <rdfs:comment>A, continuous or incremental, change in the reported values of observations over time for an unchanging quality.</rdfs:comment>
        <rdfs:isDefinedBy>http://purl.oclc.org/NET/ssnx/ssn</rdfs:isDefinedBy>
        <rdfs:label>Drift</rdfs:label>
        <rdfs:seeAlso>http://www.w3.org/2005/Incubator/ssn/wiki/SSN_Sensor#MeasuringCapability</rdfs:seeAlso>
    </owl:Class>
    


    <!-- http://purl.oclc.org/NET/ssnx/ssn#FeatureOfInterest -->

    <owl:Class rdf:about="http://purl.oclc.org/NET/ssnx/ssn#FeatureOfInterest">
        <rdfs:subClassOf rdf:resource="http://www.w3.org/2002/07/owl#Thing"/>
        <rdfs:subClassOf>
            <owl:Class>
                <owl:unionOf rdf:parseType="Collection">
                    <rdf:Description rdf:about="http://www.loa-cnr.it/ontologies/DUL.owl#Event"/>
                    <rdf:Description rdf:about="http://www.loa-cnr.it/ontologies/DUL.owl#Object"/>
                </owl:unionOf>
            </owl:Class>
        </rdfs:subClassOf>
    </owl:Class>
    


    <!-- http://purl.oclc.org/NET/ssnx/ssn#Frequency -->

    <owl:Class rdf:about="http://purl.oclc.org/NET/ssnx/ssn#Frequency">
        <rdfs:subClassOf rdf:resource="http://purl.oclc.org/NET/ssnx/ssn#MeasurementProperty"/>
        <rdfs:comment>The smallest possible time between one observation and the next.</rdfs:comment>
        <rdfs:isDefinedBy>http://purl.oclc.org/NET/ssnx/ssn</rdfs:isDefinedBy>
        <rdfs:label>Frequency</rdfs:label>
        <rdfs:seeAlso>http://www.w3.org/2005/Incubator/ssn/wiki/SSN_Sensor#MeasuringCapability</rdfs:seeAlso>
    </owl:Class>
    


    <!-- http://purl.oclc.org/NET/ssnx/ssn#Input -->

    <owl:Class rdf:about="http://purl.oclc.org/NET/ssnx/ssn#Input">
        <rdfs:subClassOf rdf:resource="http://www.loa-cnr.it/ontologies/DUL.owl#InformationObject"/>
        <owl:disjointWith rdf:resource="http://purl.oclc.org/NET/ssnx/ssn#Output"/>
        <dc:source>http://marinemetadata.org/community/teams/ontdevices</dc:source>
        <rdfs:comment>Any information that is provided to a process for its use [MMI OntDev]</rdfs:comment>
        <rdfs:isDefinedBy>http://purl.oclc.org/NET/ssnx/ssn</rdfs:isDefinedBy>
        <rdfs:label>Input</rdfs:label>
        <rdfs:seeAlso>http://www.w3.org/2005/Incubator/ssn/wiki/SSN_Model#Process</rdfs:seeAlso>
    </owl:Class>
    


    <!-- http://purl.oclc.org/NET/ssnx/ssn#Latency -->

    <owl:Class rdf:about="http://purl.oclc.org/NET/ssnx/ssn#Latency">
        <rdfs:subClassOf rdf:resource="http://purl.oclc.org/NET/ssnx/ssn#MeasurementProperty"/>
        <rdfs:comment>The time between a request for an observation and the sensor providing a result.</rdfs:comment>
        <rdfs:isDefinedBy>http://purl.oclc.org/NET/ssnx/ssn</rdfs:isDefinedBy>
        <rdfs:label>Latency</rdfs:label>
        <rdfs:seeAlso>http://www.w3.org/2005/Incubator/ssn/wiki/SSN_Sensor#MeasuringCapability</rdfs:seeAlso>
    </owl:Class>
    


    <!-- http://purl.oclc.org/NET/ssnx/ssn#MaintenanceSchedule -->

    <owl:Class rdf:about="http://purl.oclc.org/NET/ssnx/ssn#MaintenanceSchedule">
        <rdfs:subClassOf rdf:resource="http://purl.oclc.org/NET/ssnx/ssn#OperatingProperty"/>
        <rdfs:comment>Schedule of maintenance for a system/sensor in the specified conditions.</rdfs:comment>
        <rdfs:isDefinedBy>http://purl.oclc.org/NET/ssnx/ssn</rdfs:isDefinedBy>
        <rdfs:label>Maintenance Schedule</rdfs:label>
        <rdfs:seeAlso>http://www.w3.org/2005/Incubator/ssn/wiki/SSN_Deploy#OperatingRestriction</rdfs:seeAlso>
    </owl:Class>
    


    <!-- http://purl.oclc.org/NET/ssnx/ssn#MeasurementCapability -->

    <owl:Class rdf:about="http://purl.oclc.org/NET/ssnx/ssn#MeasurementCapability">
        <rdfs:subClassOf rdf:resource="http://purl.oclc.org/NET/ssnx/ssn#Property"/>
        <rdfs:subClassOf>
            <owl:Restriction>
                <owl:onProperty rdf:resource="http://purl.oclc.org/NET/ssnx/ssn#forProperty"/>
                <owl:allValuesFrom rdf:resource="http://purl.oclc.org/NET/ssnx/ssn#Property"/>
            </owl:Restriction>
        </rdfs:subClassOf>
        <rdfs:subClassOf>
            <owl:Restriction>
                <owl:onProperty rdf:resource="http://purl.oclc.org/NET/ssnx/ssn#hasMeasurementProperty"/>
                <owl:allValuesFrom rdf:resource="http://purl.oclc.org/NET/ssnx/ssn#MeasurementProperty"/>
            </owl:Restriction>
        </rdfs:subClassOf>
        <rdfs:subClassOf>
            <owl:Restriction>
                <owl:onProperty rdf:resource="http://purl.oclc.org/NET/ssnx/ssn#inCondition"/>
                <owl:allValuesFrom rdf:resource="http://purl.oclc.org/NET/ssnx/ssn#Condition"/>
            </owl:Restriction>
        </rdfs:subClassOf>
        <dc:source>Similar idea to MeasurementCapability in MMI Device Ontology
                                  http://marinemetadata.org/community/teams/ontdevices

But the the two express the relationship between constraints and multiple measurement properties differently.

The conditions linked to a MeasurementCapability are skos:exactMatch to &apos;influence quantity&apos; [VIM 2.52]
http://www.bipm.org/utils/common/documents/jcgm/JCGM_200_2008.pdf</dc:source>
        <rdfs:comment>Collects together measurement properties (accuracy, range, precision, etc) and the environmental conditions in which those properties hold, representing a specification of a sensor&apos;s capability in those conditions.

The conditions specified here are those that affect the measurement properties, while those in OperatingRange represent the sensor&apos;s standard operating conditions, including conditions that don&apos;t affect the observations.</rdfs:comment>
        <rdfs:isDefinedBy>http://purl.oclc.org/NET/ssnx/ssn</rdfs:isDefinedBy>
        <rdfs:label>Measurement Capability</rdfs:label>
        <rdfs:seeAlso>http://www.w3.org/2005/Incubator/ssn/wiki/SSN_Sensor#MeasuringCapability</rdfs:seeAlso>
    </owl:Class>
    


    <!-- http://purl.oclc.org/NET/ssnx/ssn#MeasurementProperty -->

    <owl:Class rdf:about="http://purl.oclc.org/NET/ssnx/ssn#MeasurementProperty">
        <rdfs:subClassOf rdf:resource="http://purl.oclc.org/NET/ssnx/ssn#Property"/>
        <www:subClassOfInverted rdf:resource="http://purl.oclc.org/NET/ssnx/ssn#Accuracy"/>
        <www:subClassOfInverted rdf:resource="http://purl.oclc.org/NET/ssnx/ssn#DetectionLimit"/>
        <www:subClassOfInverted rdf:resource="http://purl.oclc.org/NET/ssnx/ssn#Drift"/>
        <www:subClassOfInverted rdf:resource="http://purl.oclc.org/NET/ssnx/ssn#Frequency"/>
        <www:subClassOfInverted rdf:resource="http://purl.oclc.org/NET/ssnx/ssn#Latency"/>
        <www:subClassOfInverted rdf:resource="http://purl.oclc.org/NET/ssnx/ssn#MeasurementRange"/>
        <www:subClassOfInverted rdf:resource="http://purl.oclc.org/NET/ssnx/ssn#Precision"/>
        <www:subClassOfInverted rdf:resource="http://purl.oclc.org/NET/ssnx/ssn#Resolution"/>
        <www:subClassOfInverted rdf:resource="http://purl.oclc.org/NET/ssnx/ssn#ResponseTime"/>
        <www:subClassOfInverted rdf:resource="http://purl.oclc.org/NET/ssnx/ssn#Selectivity"/>
        <www:subClassOfInverted rdf:resource="http://purl.oclc.org/NET/ssnx/ssn#Sensitivity"/>
        <rdfs:comment>An identifiable and observable characteristic of a sensor&apos;s observations or ability to make observations.</rdfs:comment>
        <rdfs:isDefinedBy>http://purl.oclc.org/NET/ssnx/ssn</rdfs:isDefinedBy>
        <rdfs:label>Measurement  Property</rdfs:label>
        <rdfs:seeAlso>http://www.w3.org/2005/Incubator/ssn/wiki/SSN_Sensor#MeasuringCapability</rdfs:seeAlso>
    </owl:Class>
    


    <!-- http://purl.oclc.org/NET/ssnx/ssn#MeasurementRange -->

    <owl:Class rdf:about="http://purl.oclc.org/NET/ssnx/ssn#MeasurementRange">
        <rdfs:subClassOf rdf:resource="http://purl.oclc.org/NET/ssnx/ssn#MeasurementProperty"/>
        <dc:source>skos:exactMatch &apos;measuring interval/measurement range&apos; [VIM 4.7]
                                  http://www.bipm.org/utils/common/documents/jcgm/JCGM_200_2008.pdf</dc:source>
        <rdfs:comment>The set of values that the sensor can return as the result of an observation under the defined conditions with the defined measurement properties.  (If no conditions are specified or the conditions do not specify a range for the observed qualities, the measurement range is to be taken as the condition for the observed qualities.)</rdfs:comment>
        <rdfs:isDefinedBy>http://purl.oclc.org/NET/ssnx/ssn</rdfs:isDefinedBy>
        <rdfs:label>Measurement  Range</rdfs:label>
        <rdfs:seeAlso>http://www.w3.org/2005/Incubator/ssn/wiki/SSN_Sensor#MeasuringCapability</rdfs:seeAlso>
    </owl:Class>
    


    <!-- http://purl.oclc.org/NET/ssnx/ssn#Observation -->

    <owl:Class rdf:about="http://purl.oclc.org/NET/ssnx/ssn#Observation">
        <rdfs:subClassOf rdf:resource="http://www.loa-cnr.it/ontologies/DUL.owl#Situation"/>
        <rdfs:subClassOf>
            <owl:Restriction>
                <owl:onProperty rdf:resource="http://www.loa-cnr.it/ontologies/DUL.owl#includesEvent"/>
                <owl:someValuesFrom rdf:resource="http://purl.oclc.org/NET/ssnx/ssn#Stimulus"/>
            </owl:Restriction>
        </rdfs:subClassOf>
        <rdfs:subClassOf>
            <owl:Restriction>
                <owl:onProperty rdf:resource="http://purl.oclc.org/NET/ssnx/ssn#featureOfInterest"/>
                <owl:allValuesFrom rdf:resource="http://purl.oclc.org/NET/ssnx/ssn#FeatureOfInterest"/>
            </owl:Restriction>
        </rdfs:subClassOf>
        <rdfs:subClassOf>
            <owl:Restriction>
                <owl:onProperty rdf:resource="http://purl.oclc.org/NET/ssnx/ssn#observationResult"/>
                <owl:allValuesFrom rdf:resource="http://purl.oclc.org/NET/ssnx/ssn#SensorOutput"/>
            </owl:Restriction>
        </rdfs:subClassOf>
        <rdfs:subClassOf>
            <owl:Restriction>
                <owl:onProperty rdf:resource="http://purl.oclc.org/NET/ssnx/ssn#observedBy"/>
                <owl:allValuesFrom rdf:resource="http://purl.oclc.org/NET/ssnx/ssn#Sensor"/>
            </owl:Restriction>
        </rdfs:subClassOf>
        <rdfs:subClassOf>
            <owl:Restriction>
                <owl:onProperty rdf:resource="http://purl.oclc.org/NET/ssnx/ssn#observedProperty"/>
                <owl:allValuesFrom rdf:resource="http://purl.oclc.org/NET/ssnx/ssn#Property"/>
            </owl:Restriction>
        </rdfs:subClassOf>
        <rdfs:subClassOf>
            <owl:Restriction>
                <owl:onProperty rdf:resource="http://purl.oclc.org/NET/ssnx/ssn#sensingMethodUsed"/>
                <owl:allValuesFrom rdf:resource="http://purl.oclc.org/NET/ssnx/ssn#Sensing"/>
            </owl:Restriction>
        </rdfs:subClassOf>
        <rdfs:subClassOf>
            <owl:Restriction>
                <owl:onProperty rdf:resource="http://purl.oclc.org/NET/ssnx/ssn#observationResultTime"/>
                <owl:minCardinality rdf:datatype="http://www.w3.org/2001/XMLSchema#nonNegativeInteger">0</owl:minCardinality>
            </owl:Restriction>
        </rdfs:subClassOf>
        <rdfs:subClassOf>
            <owl:Restriction>
                <owl:onProperty rdf:resource="http://purl.oclc.org/NET/ssnx/ssn#observationSamplingTime"/>
                <owl:minCardinality rdf:datatype="http://www.w3.org/2001/XMLSchema#nonNegativeInteger">0</owl:minCardinality>
            </owl:Restriction>
        </rdfs:subClassOf>
        <rdfs:subClassOf>
            <owl:Restriction>
                <owl:onProperty rdf:resource="http://purl.oclc.org/NET/ssnx/ssn#qualityOfObservation"/>
                <owl:minCardinality rdf:datatype="http://www.w3.org/2001/XMLSchema#nonNegativeInteger">0</owl:minCardinality>
            </owl:Restriction>
        </rdfs:subClassOf>
        <rdfs:subClassOf>
            <owl:Restriction>
                <owl:onProperty rdf:resource="http://purl.oclc.org/NET/ssnx/ssn#featureOfInterest"/>
                <owl:qualifiedCardinality rdf:datatype="http://www.w3.org/2001/XMLSchema#nonNegativeInteger">1</owl:qualifiedCardinality>
                <owl:onClass rdf:resource="http://purl.oclc.org/NET/ssnx/ssn#FeatureOfInterest"/>
            </owl:Restriction>
        </rdfs:subClassOf>
        <rdfs:subClassOf>
            <owl:Restriction>
                <owl:onProperty rdf:resource="http://purl.oclc.org/NET/ssnx/ssn#observedBy"/>
                <owl:qualifiedCardinality rdf:datatype="http://www.w3.org/2001/XMLSchema#nonNegativeInteger">1</owl:qualifiedCardinality>
                <owl:onClass rdf:resource="http://purl.oclc.org/NET/ssnx/ssn#Sensor"/>
            </owl:Restriction>
        </rdfs:subClassOf>
        <rdfs:subClassOf>
            <owl:Restriction>
                <owl:onProperty rdf:resource="http://purl.oclc.org/NET/ssnx/ssn#observedProperty"/>
                <owl:qualifiedCardinality rdf:datatype="http://www.w3.org/2001/XMLSchema#nonNegativeInteger">1</owl:qualifiedCardinality>
                <owl:onClass rdf:resource="http://purl.oclc.org/NET/ssnx/ssn#Property"/>
            </owl:Restriction>
        </rdfs:subClassOf>
        <rdfs:subClassOf>
            <owl:Restriction>
                <owl:onProperty rdf:resource="http://purl.oclc.org/NET/ssnx/ssn#sensingMethodUsed"/>
                <owl:qualifiedCardinality rdf:datatype="http://www.w3.org/2001/XMLSchema#nonNegativeInteger">1</owl:qualifiedCardinality>
                <owl:onClass rdf:resource="http://purl.oclc.org/NET/ssnx/ssn#Sensing"/>
            </owl:Restriction>
        </rdfs:subClassOf>
        <dc:source>skos:closeMatch &apos;observation&apos; [O&amp;M] 
		                    http://www.opengeospatial.org/standards/om 

Observation in this ontology and O&amp;M are described differently (O&amp;M records an observation as an act/event), but they record the same thing and are essentially interchangeable.  The difference is in the ontological structure of the two, not the data or use.

Observation here records a Situation (the estimation of the value of a Property) and a description of the method that was used (along with the participants), while O&amp;M interprets an Observation as the event itself; there must, however, have been an event that lead to our situation, so both are records of events.  The distinction is between the event itself and the record of what happened in that event.


skos:closeMatch &apos;measurement result&apos; [VIM 2.9] http://www.bipm.org/utils/common/documents/jcgm/JCGM_200_2008.pdf

Measurement result in VIM is the measured value plus any other relevant information, which means that measurement result and observation will often be associated to the same data (a value, a time, a property, etc.).</dc:source>
        <rdfs:comment>An Observation is a Situation in which a Sensing method has been used to estimate or calculate a value of a Property of a FeatureOfInterest.  Links to Sensing and Sensor describe what made the Observation and how; links to Property and Feature detail what was sensed; the result is the output of a Sensor; other metadata details times etc.</rdfs:comment>
        <rdfs:isDefinedBy>http://purl.oclc.org/NET/ssnx/ssn</rdfs:isDefinedBy>
        <rdfs:label>Observation</rdfs:label>
        <rdfs:label>ssn:Observation</rdfs:label>
        <rdfs:seeAlso>http://www.w3.org/2005/Incubator/ssn/wiki/SSN_Skeleton#Skeleton</rdfs:seeAlso>
    </owl:Class>
    


    <!-- http://purl.oclc.org/NET/ssnx/ssn#ObservationValue -->

    <owl:Class rdf:about="http://purl.oclc.org/NET/ssnx/ssn#ObservationValue">
        <rdfs:subClassOf rdf:resource="http://www.loa-cnr.it/ontologies/DUL.owl#InformationObject"/>
        <rdfs:subClassOf rdf:resource="http://www.loa-cnr.it/ontologies/DUL.owl#Region"/>
        <rdfs:subClassOf>
            <owl:Restriction>
                <owl:onProperty rdf:resource="http://www.loa-cnr.it/ontologies/DUL.owl#isRegionFor"/>
                <owl:someValuesFrom rdf:resource="http://purl.oclc.org/NET/ssnx/ssn#SensorOutput"/>
            </owl:Restriction>
        </rdfs:subClassOf>
        <rdfs:subClassOf>
            <owl:Restriction>
                <owl:onProperty rdf:resource="http://people.aifb.kit.edu/mu2771/step/0.2.0/moduleC#date"/>
                <owl:qualifiedCardinality rdf:datatype="http://www.w3.org/2001/XMLSchema#nonNegativeInteger">1</owl:qualifiedCardinality>
                <owl:onClass rdf:resource="http://www.w3.org/2006/time#Instant"/>
            </owl:Restriction>
        </rdfs:subClassOf>
        <rdfs:subClassOf>
            <owl:Restriction>
                <owl:onProperty rdf:resource="http://qudt.org/schema/qudt#unit"/>
                <owl:qualifiedCardinality rdf:datatype="http://www.w3.org/2001/XMLSchema#nonNegativeInteger">1</owl:qualifiedCardinality>
                <owl:onClass rdf:resource="http://qudt.org/schema/qudt#Unit"/>
            </owl:Restriction>
        </rdfs:subClassOf>
        <dc:source>skos:exactMatch &apos;measured quantity value&apos; [VIM 2.10]
                                  http://www.bipm.org/utils/common/documents/jcgm/JCGM_200_2008.pdf

skos:exactMatch &apos;observed value&apos; [SensorML OGC-0700]
http://www.opengeospatial.org/standards/sensorml 

skos:closeMatch &apos;observation result&apos; [O&amp;M]
http://www.opengeospatial.org/standards/om 

O&amp;M conflates what we have as SensorOutput and ObservationValue into observation result, though the OGC standard does say &quot;result contains a value&quot; and &quot;a result which has a value&quot;, which fits naturally with the model here.</dc:source>
        <rdfs:comment>The value of the result of an Observation.  An Observation has a result which is the output of some sensor, the result is an information object that encodes some value for a Feature.</rdfs:comment>
        <rdfs:isDefinedBy>http://purl.oclc.org/NET/ssnx/ssn</rdfs:isDefinedBy>
        <rdfs:label>Observation Value</rdfs:label>
        <rdfs:label>ssn:ObservationValue</rdfs:label>
        <rdfs:seeAlso>http://www.w3.org/2005/Incubator/ssn/wiki/SSN_Base#Data</rdfs:seeAlso>
    </owl:Class>
    


    <!-- http://purl.oclc.org/NET/ssnx/ssn#OperatingPowerRange -->

    <owl:Class rdf:about="http://purl.oclc.org/NET/ssnx/ssn#OperatingPowerRange">
        <rdfs:subClassOf rdf:resource="http://purl.oclc.org/NET/ssnx/ssn#OperatingProperty"/>
        <rdfs:comment>Power range in which system/sensor is expected to operate.</rdfs:comment>
        <rdfs:isDefinedBy>http://purl.oclc.org/NET/ssnx/ssn</rdfs:isDefinedBy>
        <rdfs:label>Operating Power Range</rdfs:label>
        <rdfs:seeAlso>http://www.w3.org/2005/Incubator/ssn/wiki/SSN_Energy#EnergyRestriction</rdfs:seeAlso>
    </owl:Class>
    


    <!-- http://purl.oclc.org/NET/ssnx/ssn#OperatingProperty -->

    <owl:Class rdf:about="http://purl.oclc.org/NET/ssnx/ssn#OperatingProperty">
        <rdfs:subClassOf rdf:resource="http://purl.oclc.org/NET/ssnx/ssn#Property"/>
        <www:subClassOfInverted rdf:resource="http://purl.oclc.org/NET/ssnx/ssn#MaintenanceSchedule"/>
        <www:subClassOfInverted rdf:resource="http://purl.oclc.org/NET/ssnx/ssn#OperatingPowerRange"/>
        <rdfs:comment>An identifiable characteristic of the environmental and other conditions in which the sensor is intended to operate.  May include power ranges, power sources, standard configurations, attachments and the like.</rdfs:comment>
        <rdfs:isDefinedBy>http://purl.oclc.org/NET/ssnx/ssn</rdfs:isDefinedBy>
        <rdfs:label>Operating Property</rdfs:label>
        <rdfs:seeAlso>http://www.w3.org/2005/Incubator/ssn/wiki/SSN_Deploy#OperatingRestriction</rdfs:seeAlso>
    </owl:Class>
    


    <!-- http://purl.oclc.org/NET/ssnx/ssn#OperatingRange -->

    <owl:Class rdf:about="http://purl.oclc.org/NET/ssnx/ssn#OperatingRange">
        <rdfs:subClassOf rdf:resource="http://purl.oclc.org/NET/ssnx/ssn#Property"/>
        <rdfs:subClassOf>
            <owl:Restriction>
                <owl:onProperty rdf:resource="http://purl.oclc.org/NET/ssnx/ssn#hasOperatingProperty"/>
                <owl:allValuesFrom rdf:resource="http://purl.oclc.org/NET/ssnx/ssn#OperatingProperty"/>
            </owl:Restriction>
        </rdfs:subClassOf>
        <rdfs:subClassOf>
            <owl:Restriction>
                <owl:onProperty rdf:resource="http://purl.oclc.org/NET/ssnx/ssn#inCondition"/>
                <owl:allValuesFrom rdf:resource="http://purl.oclc.org/NET/ssnx/ssn#Condition"/>
            </owl:Restriction>
        </rdfs:subClassOf>
        <dc:source>skos:broaderMatch &apos;reference operating condition&apos; [VIM 4.11]
                                  http://www.bipm.org/utils/common/documents/jcgm/JCGM_200_2008.pdf

The difference is that here we also allow for qualities that aren&apos;t VIM influence quantities [VIM 2.52] - for example, a quantity that alters the power requirements, but doesn&apos;t affect the measurement properties - conditions specified in MeasurementCapability should be influence quantities.</dc:source>
        <rdfs:comment>The environmental conditions and characteristics of a system/sensor&apos;s normal operating environment.  Can be used to specify for example the standard environmental conditions in which the sensor is expected to operate (a Condition with no OperatingProperty), or how the environmental and other operating properties relate: i.e., that the maintenance schedule or power requirements differ according to the conditions.</rdfs:comment>
        <rdfs:isDefinedBy>http://purl.oclc.org/NET/ssnx/ssn</rdfs:isDefinedBy>
        <rdfs:label>Operating Range</rdfs:label>
        <rdfs:seeAlso>http://www.w3.org/2005/Incubator/ssn/wiki/SSN_Deploy#OperatingRestriction</rdfs:seeAlso>
    </owl:Class>
    


    <!-- http://purl.oclc.org/NET/ssnx/ssn#Output -->

    <owl:Class rdf:about="http://purl.oclc.org/NET/ssnx/ssn#Output">
        <rdfs:subClassOf rdf:resource="http://www.loa-cnr.it/ontologies/DUL.owl#InformationObject"/>
        <dc:source>http://marinemetadata.org/community/teams/ontdevices</dc:source>
        <rdfs:comment>Any information that is reported from a process. [MMI OntDev]</rdfs:comment>
        <rdfs:isDefinedBy>http://purl.oclc.org/NET/ssnx/ssn</rdfs:isDefinedBy>
        <rdfs:label>Output</rdfs:label>
        <rdfs:seeAlso>http://www.w3.org/2005/Incubator/ssn/wiki/SSN_Model#Process</rdfs:seeAlso>
    </owl:Class>
    


    <!-- http://purl.oclc.org/NET/ssnx/ssn#Platform -->

    <owl:Class rdf:about="http://purl.oclc.org/NET/ssnx/ssn#Platform">
        <rdfs:subClassOf rdf:resource="http://www.loa-cnr.it/ontologies/DUL.owl#PhysicalObject"/>
        <rdfs:subClassOf>
            <owl:Restriction>
                <owl:onProperty rdf:resource="http://purl.oclc.org/NET/ssnx/ssn#attachedSystem"/>
                <owl:allValuesFrom rdf:resource="http://purl.oclc.org/NET/ssnx/ssn#System"/>
            </owl:Restriction>
        </rdfs:subClassOf>
        <rdfs:subClassOf>
            <owl:Restriction>
                <owl:onProperty rdf:resource="http://purl.oclc.org/NET/ssnx/ssn#inDeployment"/>
                <owl:allValuesFrom rdf:resource="http://purl.oclc.org/NET/ssnx/ssn#Deployment"/>
            </owl:Restriction>
        </rdfs:subClassOf>
        <dc:source>skos:exactMatch &apos;platform&apos; [SensorML OGC-0700]
                                  http://www.opengeospatial.org/standards/sensorml</dc:source>
        <rdfs:comment>An Entity to which other Entities can be attached - particuarly Sensors and other Platforms.  For example, a post might act as the Platform, a bouy might act as a Platform, or a fish might act as a Platform for an attached sensor.</rdfs:comment>
        <rdfs:isDefinedBy>http://purl.oclc.org/NET/ssnx/ssn</rdfs:isDefinedBy>
        <rdfs:label>Platform</rdfs:label>
        <rdfs:seeAlso>http://www.w3.org/2005/Incubator/ssn/wiki/SSN_Deploy#PlatformSite</rdfs:seeAlso>
    </owl:Class>
    


    <!-- http://purl.oclc.org/NET/ssnx/ssn#Precision -->

    <owl:Class rdf:about="http://purl.oclc.org/NET/ssnx/ssn#Precision">
        <rdfs:subClassOf rdf:resource="http://purl.oclc.org/NET/ssnx/ssn#MeasurementProperty"/>
        <dc:source>skos:exactMatch &apos;measurement precision/precision&apos; [VIM 2.15]
                                   http://www.bipm.org/utils/common/documents/jcgm/JCGM_200_2008.pdf</dc:source>
        <rdfs:comment>The closeness of agreement between replicate observations on an unchanged or similar quality value: i.e., a measure of a sensor&apos;s ability to consitently reproduce an observation.</rdfs:comment>
        <rdfs:isDefinedBy>http://purl.oclc.org/NET/ssnx/ssn</rdfs:isDefinedBy>
        <rdfs:label>Precision</rdfs:label>
        <rdfs:seeAlso>http://www.w3.org/2005/Incubator/ssn/wiki/SSN_Sensor#MeasuringCapability</rdfs:seeAlso>
    </owl:Class>
    


    <!-- http://purl.oclc.org/NET/ssnx/ssn#Process -->

    <owl:Class rdf:about="http://purl.oclc.org/NET/ssnx/ssn#Process">
        <rdfs:subClassOf rdf:resource="http://www.loa-cnr.it/ontologies/DUL.owl#Method"/>
        <rdfs:subClassOf>
            <owl:Restriction>
                <owl:onProperty rdf:resource="http://purl.oclc.org/NET/ssnx/ssn#hasOutput"/>
                <owl:someValuesFrom rdf:resource="http://purl.oclc.org/NET/ssnx/ssn#Output"/>
            </owl:Restriction>
        </rdfs:subClassOf>
        <rdfs:subClassOf>
            <owl:Restriction>
                <owl:onProperty rdf:resource="http://purl.oclc.org/NET/ssnx/ssn#hasInput"/>
                <owl:allValuesFrom rdf:resource="http://purl.oclc.org/NET/ssnx/ssn#Input"/>
            </owl:Restriction>
        </rdfs:subClassOf>
        <rdfs:subClassOf>
            <owl:Restriction>
                <owl:onProperty rdf:resource="http://purl.oclc.org/NET/ssnx/ssn#hasOutput"/>
                <owl:allValuesFrom rdf:resource="http://purl.oclc.org/NET/ssnx/ssn#Output"/>
            </owl:Restriction>
        </rdfs:subClassOf>
        <dc:source>http://www.w3.org/2005/Incubator/ssn/</dc:source>
        <www:subClassOfInverted rdf:resource="http://purl.oclc.org/NET/ssnx/ssn#Sensing"/>
        <rdfs:comment>A process has an output and possibly inputs and, for a composite process, describes the temporal and dataflow dependencies and relationships amongst its parts. [SSN XG]</rdfs:comment>
        <rdfs:isDefinedBy>http://purl.oclc.org/NET/ssnx/ssn</rdfs:isDefinedBy>
        <rdfs:label>Process</rdfs:label>
        <rdfs:seeAlso>http://www.w3.org/2005/Incubator/ssn/wiki/SSN_Model#Process</rdfs:seeAlso>
    </owl:Class>
    


    <!-- http://purl.oclc.org/NET/ssnx/ssn#Property -->

    <owl:Class rdf:about="http://purl.oclc.org/NET/ssnx/ssn#Property">
        <rdfs:subClassOf rdf:resource="http://www.loa-cnr.it/ontologies/DUL.owl#Quality"/>
        <rdfs:subClassOf>
            <owl:Restriction>
                <owl:onProperty rdf:resource="http://purl.oclc.org/NET/ssnx/ssn#isPropertyOf"/>
                <owl:someValuesFrom rdf:resource="http://purl.oclc.org/NET/ssnx/ssn#FeatureOfInterest"/>
            </owl:Restriction>
        </rdfs:subClassOf>
        <dc:source>skos:exactMatch &apos;property&apos; [O&amp;M] 
		                    http://www.opengeospatial.org/standards/om</dc:source>
        <www:subClassOfInverted rdf:resource="http://purl.oclc.org/NET/ssnx/ssn#Condition"/>
        <www:subClassOfInverted rdf:resource="http://purl.oclc.org/NET/ssnx/ssn#MeasurementCapability"/>
        <www:subClassOfInverted rdf:resource="http://purl.oclc.org/NET/ssnx/ssn#MeasurementProperty"/>
        <www:subClassOfInverted rdf:resource="http://purl.oclc.org/NET/ssnx/ssn#OperatingProperty"/>
        <www:subClassOfInverted rdf:resource="http://purl.oclc.org/NET/ssnx/ssn#OperatingRange"/>
        <www:subClassOfInverted rdf:resource="http://purl.oclc.org/NET/ssnx/ssn#SurvivalProperty"/>
        <www:subClassOfInverted rdf:resource="http://purl.oclc.org/NET/ssnx/ssn#SurvivalRange"/>
        <rdfs:comment>An observable Quality of an Event or Object.  That is, not a quality of an abstract entity as is also allowed by DUL&apos;s Quality, but rather an aspect of an entity that is intrinsic to and cannot exist without the entity and is observable by a sensor.</rdfs:comment>
        <rdfs:isDefinedBy>http://purl.oclc.org/NET/ssnx/ssn</rdfs:isDefinedBy>
        <rdfs:label>Property</rdfs:label>
        <rdfs:seeAlso>http://www.w3.org/2005/Incubator/ssn/wiki/SSN_Skeleton#Skeleton</rdfs:seeAlso>
    </owl:Class>
    


    <!-- http://purl.oclc.org/NET/ssnx/ssn#Resolution -->

    <owl:Class rdf:about="http://purl.oclc.org/NET/ssnx/ssn#Resolution">
        <rdfs:subClassOf rdf:resource="http://purl.oclc.org/NET/ssnx/ssn#MeasurementProperty"/>
        <dc:source>skos:exactMatch &apos;resolution&apos; [VIM 4.14]
                                  http://www.bipm.org/utils/common/documents/jcgm/JCGM_200_2008.pdf</dc:source>
        <rdfs:comment>The smallest difference in the value of a quality being observed that would result in perceptably different values of observation results.</rdfs:comment>
        <rdfs:isDefinedBy>http://purl.oclc.org/NET/ssnx/ssn</rdfs:isDefinedBy>
        <rdfs:label>Resolution</rdfs:label>
        <rdfs:seeAlso>http://www.w3.org/2005/Incubator/ssn/wiki/SSN_Sensor#MeasuringCapability</rdfs:seeAlso>
    </owl:Class>
    


    <!-- http://purl.oclc.org/NET/ssnx/ssn#ResponseTime -->

    <owl:Class rdf:about="http://purl.oclc.org/NET/ssnx/ssn#ResponseTime">
        <rdfs:subClassOf rdf:resource="http://purl.oclc.org/NET/ssnx/ssn#MeasurementProperty"/>
        <dc:source>skos:exactMatch &apos;step response time&apos; [VIM 4.23]
                                  http://www.bipm.org/utils/common/documents/jcgm/JCGM_200_2008.pdf</dc:source>
        <rdfs:comment>The time between a (step) change inthe value of an observed quality and a sensor (possibly with specified error) &apos;settling&apos; on an observed value.</rdfs:comment>
        <rdfs:isDefinedBy>http://purl.oclc.org/NET/ssnx/ssn</rdfs:isDefinedBy>
        <rdfs:label>Response time</rdfs:label>
        <rdfs:seeAlso>http://www.w3.org/2005/Incubator/ssn/wiki/SSN_Sensor#MeasuringCapability</rdfs:seeAlso>
    </owl:Class>
    


    <!-- http://purl.oclc.org/NET/ssnx/ssn#Selectivity -->

    <owl:Class rdf:about="http://purl.oclc.org/NET/ssnx/ssn#Selectivity">
        <rdfs:subClassOf rdf:resource="http://purl.oclc.org/NET/ssnx/ssn#MeasurementProperty"/>
        <dc:source>skos:exactMatch &apos;selectivity&apos; [VIM 4.13]
                                 http://www.bipm.org/utils/common/documents/jcgm/JCGM_200_2008.pdf</dc:source>
        <rdfs:comment>Selectivity is a property of a sensor whereby it provides observed values for one or more qualities such that the values of each quality are independent of other qualities in the phenomenon, body, or substance being investigated.</rdfs:comment>
        <rdfs:isDefinedBy>http://purl.oclc.org/NET/ssnx/ssn</rdfs:isDefinedBy>
        <rdfs:label>Selectivity</rdfs:label>
        <rdfs:seeAlso>http://www.w3.org/2005/Incubator/ssn/wiki/SSN_Sensor#MeasuringCapability</rdfs:seeAlso>
    </owl:Class>
    


    <!-- http://purl.oclc.org/NET/ssnx/ssn#Sensing -->

    <owl:Class rdf:about="http://purl.oclc.org/NET/ssnx/ssn#Sensing">
        <rdfs:subClassOf rdf:resource="http://purl.oclc.org/NET/ssnx/ssn#Process"/>
        <dc:source>http://www.w3.org/2005/Incubator/ssn/</dc:source>
        <rdfs:comment>Sensing is a process that results in the estimation, or calculation, of the value of a phenomenon.</rdfs:comment>
        <rdfs:isDefinedBy>http://purl.oclc.org/NET/ssnx/ssn</rdfs:isDefinedBy>
        <rdfs:label>Sensing</rdfs:label>
        <rdfs:seeAlso>http://www.w3.org/2005/Incubator/ssn/wiki/SSN_Skeleton#Skeleton</rdfs:seeAlso>
    </owl:Class>
    


    <!-- http://purl.oclc.org/NET/ssnx/ssn#SensingDevice -->

    <owl:Class rdf:about="http://purl.oclc.org/NET/ssnx/ssn#SensingDevice">
        <rdfs:subClassOf rdf:resource="http://purl.oclc.org/NET/ssnx/ssn#Device"/>
        <rdfs:subClassOf rdf:resource="http://purl.oclc.org/NET/ssnx/ssn#Sensor"/>
        <dc:source>http://www.w3.org/2005/Incubator/ssn/</dc:source>
        <rdfs:comment>A sensing device is a device that implements sensing.</rdfs:comment>
        <rdfs:isDefinedBy>http://purl.oclc.org/NET/ssnx/ssn</rdfs:isDefinedBy>
        <rdfs:label>Sensing Device</rdfs:label>
        <rdfs:label>ssn:SensingDevice</rdfs:label>
        <rdfs:seeAlso>http://www.w3.org/2005/Incubator/ssn/wiki/SSN_Sensor#Measuring</rdfs:seeAlso>
    </owl:Class>
    


    <!-- http://purl.oclc.org/NET/ssnx/ssn#Sensitivity -->

    <owl:Class rdf:about="http://purl.oclc.org/NET/ssnx/ssn#Sensitivity">
        <rdfs:subClassOf rdf:resource="http://purl.oclc.org/NET/ssnx/ssn#MeasurementProperty"/>
        <dc:source>skos:exactMatch &apos;sensitivity&apos; [VIM 4.12]
                                  http://www.bipm.org/utils/common/documents/jcgm/JCGM_200_2008.pdf</dc:source>
        <rdfs:comment>Sensitivity is the quotient of the change in a result of sensor and the corresponding change in a value of a quality being observed.</rdfs:comment>
        <rdfs:isDefinedBy>http://purl.oclc.org/NET/ssnx/ssn</rdfs:isDefinedBy>
        <rdfs:label>Sensitivity</rdfs:label>
        <rdfs:seeAlso>http://www.w3.org/2005/Incubator/ssn/wiki/SSN_Sensor#MeasuringCapability</rdfs:seeAlso>
    </owl:Class>
    


    <!-- http://purl.oclc.org/NET/ssnx/ssn#Sensor -->

    <owl:Class rdf:about="http://purl.oclc.org/NET/ssnx/ssn#Sensor">
        <rdfs:subClassOf rdf:resource="http://www.loa-cnr.it/ontologies/DUL.owl#PhysicalObject"/>
        <rdfs:subClassOf>
            <owl:Restriction>
                <owl:onProperty rdf:resource="http://purl.oclc.org/NET/ssnx/ssn#implements"/>
                <owl:someValuesFrom rdf:resource="http://purl.oclc.org/NET/ssnx/ssn#Sensing"/>
            </owl:Restriction>
        </rdfs:subClassOf>
        <rdfs:subClassOf>
            <owl:Restriction>
                <owl:onProperty rdf:resource="http://purl.oclc.org/NET/ssnx/ssn#detects"/>
                <owl:allValuesFrom rdf:resource="http://purl.oclc.org/NET/ssnx/ssn#Stimulus"/>
            </owl:Restriction>
        </rdfs:subClassOf>
        <rdfs:subClassOf>
            <owl:Restriction>
                <owl:onProperty rdf:resource="http://purl.oclc.org/NET/ssnx/ssn#hasMeasurementCapability"/>
                <owl:allValuesFrom rdf:resource="http://purl.oclc.org/NET/ssnx/ssn#MeasurementCapability"/>
            </owl:Restriction>
        </rdfs:subClassOf>
        <rdfs:subClassOf>
            <owl:Restriction>
                <owl:onProperty rdf:resource="http://purl.oclc.org/NET/ssnx/ssn#observes"/>
                <owl:allValuesFrom rdf:resource="http://purl.oclc.org/NET/ssnx/ssn#Property"/>
            </owl:Restriction>
        </rdfs:subClassOf>
        <dc:source>skos:exactMatch &apos;sensor&apos; [SensorML OGC-0700]
		                    http://www.opengeospatial.org/standards/sensorml 

                                skos:closeMatch &apos;observation procedure&apos; [O&amp;M] 
                                http://www.opengeospatial.org/standards/om 

O&amp;M allows sensors, methods, instruments, systems, algorithms and process chains as the processUsed of an observation; this ontology allows a similar range of things (any thing that can do sensing), just they are all grouped under the term sensor (which is thus wider than the O&amp;M concept).</dc:source>
        <www:subClassOfInverted rdf:resource="http://purl.oclc.org/NET/ssnx/ssn#SensingDevice"/>
        <rdfs:comment>A sensor can do (implements) sensing: that is, a sensor is any entity that can follow a sensing method and thus observe some Property of a FeatureOfInterest.  Sensors may be physical devices, computational methods, a laboratory setup with a person following a method, or any other thing that can follow a Sensing Method to observe a Property.</rdfs:comment>
        <rdfs:isDefinedBy>http://purl.oclc.org/NET/ssnx/ssn</rdfs:isDefinedBy>
        <rdfs:label>Sensor</rdfs:label>
        <rdfs:label>ssn:Sensor</rdfs:label>
        <rdfs:seeAlso>http://www.w3.org/2005/Incubator/ssn/wiki/SSN_Skeleton#Skeleton</rdfs:seeAlso>
    </owl:Class>
    


    <!-- http://purl.oclc.org/NET/ssnx/ssn#SensorDataSheet -->

    <owl:Class rdf:about="http://purl.oclc.org/NET/ssnx/ssn#SensorDataSheet">
        <rdfs:subClassOf rdf:resource="http://www.loa-cnr.it/ontologies/DUL.owl#InformationObject"/>
        <dc:source>http://www.w3.org/2005/Incubator/ssn/</dc:source>
        <rdfs:comment>A data sheet records properties of a sensor.  A data sheet might describe for example the accuracy in various conditions, the power use, the types of connectors that the sensor has, etc.  

Generally a sensor&apos;s properties are recorded directly (with hasMeasurementCapability, for example), but the data sheet can be used for example to record the manufacturers specifications verses observed capabilites, or if more is known than the manufacturer specifies, etc.  The data sheet is an information object about the sensor&apos;s properties, rather than a direct link to the actual properties themselves.</rdfs:comment>
        <rdfs:isDefinedBy>http://purl.oclc.org/NET/ssnx/ssn</rdfs:isDefinedBy>
        <rdfs:label>Sensor Data Sheet</rdfs:label>
        <rdfs:seeAlso>http://www.w3.org/2005/Incubator/ssn/wiki/SSN_Sensor#Measuring</rdfs:seeAlso>
    </owl:Class>
    


    <!-- http://purl.oclc.org/NET/ssnx/ssn#SensorInput -->

    <owl:Class rdf:about="http://purl.oclc.org/NET/ssnx/ssn#SensorInput">
        <owl:equivalentClass rdf:resource="http://purl.oclc.org/NET/ssnx/ssn#Stimulus"/>
        <rdfs:subClassOf rdf:resource="http://www.loa-cnr.it/ontologies/DUL.owl#Event"/>
        <rdfs:subClassOf>
            <owl:Restriction>
                <owl:onProperty rdf:resource="http://purl.oclc.org/NET/ssnx/ssn#isProxyFor"/>
                <owl:allValuesFrom rdf:resource="http://purl.oclc.org/NET/ssnx/ssn#Property"/>
            </owl:Restriction>
        </rdfs:subClassOf>
        <dc:source>http://www.w3.org/2005/Incubator/ssn/</dc:source>
        <rdfs:comment>An Event in the real world that &apos;triggers&apos; the sensor.  The properties associated to the stimulus may be different to eventual observed property.  It is the event, not the object that triggers the sensor.</rdfs:comment>
        <rdfs:isDefinedBy>http://purl.oclc.org/NET/ssnx/ssn</rdfs:isDefinedBy>
        <rdfs:label>Sensor Input</rdfs:label>
        <rdfs:label>ssn:SensorInput</rdfs:label>
        <rdfs:seeAlso>http://www.w3.org/2005/Incubator/ssn/wiki/SSN_Skeleton#Skeleton</rdfs:seeAlso>
    </owl:Class>
    


    <!-- http://purl.oclc.org/NET/ssnx/ssn#SensorOutput -->

    <owl:Class rdf:about="http://purl.oclc.org/NET/ssnx/ssn#SensorOutput">
        <rdfs:subClassOf rdf:resource="http://www.loa-cnr.it/ontologies/DUL.owl#InformationObject"/>
        <rdfs:subClassOf>
            <owl:Restriction>
                <owl:onProperty rdf:resource="http://purl.oclc.org/NET/ssnx/ssn#hasValue"/>
                <owl:someValuesFrom rdf:resource="http://purl.oclc.org/NET/ssnx/ssn#ObservationValue"/>
            </owl:Restriction>
        </rdfs:subClassOf>
        <rdfs:subClassOf>
            <owl:Restriction>
                <owl:onProperty rdf:resource="http://purl.oclc.org/NET/ssnx/ssn#isProducedBy"/>
                <owl:someValuesFrom rdf:resource="http://purl.oclc.org/NET/ssnx/ssn#Sensor"/>
            </owl:Restriction>
        </rdfs:subClassOf>
        <dc:source>http://www.w3.org/2005/Incubator/ssn/

                                  skos:closeMatch &apos;observation result&apos; [O&amp;M] 
                                  http://www.opengeospatial.org/standards/om 

See comments at ObservationValue.</dc:source>
        <rdfs:comment>A sensor outputs a piece of information (an observed value), the value itself being represented by an ObservationValue.</rdfs:comment>
        <rdfs:isDefinedBy>http://purl.oclc.org/NET/ssnx/ssn</rdfs:isDefinedBy>
        <rdfs:label>Sensor Output</rdfs:label>
        <rdfs:label>ssn:SensorOutput</rdfs:label>
        <rdfs:seeAlso>http://www.w3.org/2005/Incubator/ssn/wiki/SSN_Skeleton#Skeleton</rdfs:seeAlso>
    </owl:Class>
    


    <!-- http://purl.oclc.org/NET/ssnx/ssn#Stimulus -->

    <owl:Class rdf:about="http://purl.oclc.org/NET/ssnx/ssn#Stimulus">
        <rdfs:subClassOf rdf:resource="http://www.loa-cnr.it/ontologies/DUL.owl#Event"/>
        <dc:source>http://www.w3.org/2005/Incubator/ssn/</dc:source>
        <rdfs:comment>An Event in the real world that &apos;triggers&apos; the sensor.  The properties associated to the stimulus may be different to eventual observed property.  It is the event, not the object that triggers the sensor.</rdfs:comment>
        <rdfs:isDefinedBy>http://purl.oclc.org/NET/ssnx/ssn</rdfs:isDefinedBy>
        <rdfs:label>Stimulus</rdfs:label>
        <rdfs:label>ssn:Stimulus</rdfs:label>
        <rdfs:seeAlso>http://www.w3.org/2005/Incubator/ssn/wiki/SSN_Skeleton#Skeleton</rdfs:seeAlso>
    </owl:Class>
    


    <!-- http://purl.oclc.org/NET/ssnx/ssn#SurvivalProperty -->

    <owl:Class rdf:about="http://purl.oclc.org/NET/ssnx/ssn#SurvivalProperty">
        <rdfs:subClassOf rdf:resource="http://purl.oclc.org/NET/ssnx/ssn#Property"/>
        <www:subClassOfInverted rdf:resource="http://purl.oclc.org/NET/ssnx/ssn#BatteryLifetime"/>
        <www:subClassOfInverted rdf:resource="http://purl.oclc.org/NET/ssnx/ssn#SystemLifetime"/>
        <rdfs:comment>An identifiable characteristic that represents the extent of the sensors useful life.  Might include for example total battery life or number of recharges, or, for sensors that are used only a fixed number of times, the number of observations that can be made before the sensing capability is depleted.</rdfs:comment>
        <rdfs:isDefinedBy>http://purl.oclc.org/NET/ssnx/ssn</rdfs:isDefinedBy>
        <rdfs:label>Survival Property</rdfs:label>
        <rdfs:seeAlso>http://www.w3.org/2005/Incubator/ssn/wiki/SSN_Deploy#OperatingRestriction</rdfs:seeAlso>
    </owl:Class>
    


    <!-- http://purl.oclc.org/NET/ssnx/ssn#SurvivalRange -->

    <owl:Class rdf:about="http://purl.oclc.org/NET/ssnx/ssn#SurvivalRange">
        <rdfs:subClassOf rdf:resource="http://purl.oclc.org/NET/ssnx/ssn#Property"/>
        <rdfs:subClassOf>
            <owl:Restriction>
                <owl:onProperty rdf:resource="http://purl.oclc.org/NET/ssnx/ssn#hasSurvivalProperty"/>
                <owl:allValuesFrom rdf:resource="http://purl.oclc.org/NET/ssnx/ssn#SurvivalProperty"/>
            </owl:Restriction>
        </rdfs:subClassOf>
        <rdfs:subClassOf>
            <owl:Restriction>
                <owl:onProperty rdf:resource="http://purl.oclc.org/NET/ssnx/ssn#inCondition"/>
                <owl:allValuesFrom rdf:resource="http://purl.oclc.org/NET/ssnx/ssn#Condition"/>
            </owl:Restriction>
        </rdfs:subClassOf>
        <dc:source>skos:narrowerMatch &apos;limiting operating condition&apos; [VIM 4.10]
                                  http://www.bipm.org/utils/common/documents/jcgm/JCGM_200_2008.pdf</dc:source>
        <rdfs:comment>The conditions a sensor can be exposed to without damage: i.e., the sensor continues to operate as defined using MeasurementCapability.  If, however, the SurvivalRange is exceeded, the sensor is &apos;damaged&apos; and MeasurementCapability specifications may no longer hold.</rdfs:comment>
        <rdfs:isDefinedBy>http://purl.oclc.org/NET/ssnx/ssn</rdfs:isDefinedBy>
        <rdfs:label>Survival Range</rdfs:label>
        <rdfs:label>ssn:SurvivalRange</rdfs:label>
        <rdfs:seeAlso>http://www.w3.org/2005/Incubator/ssn/wiki/SSN_Deploy#OperatingRestriction</rdfs:seeAlso>
    </owl:Class>
    


    <!-- http://purl.oclc.org/NET/ssnx/ssn#System -->

    <owl:Class rdf:about="http://purl.oclc.org/NET/ssnx/ssn#System">
        <rdfs:subClassOf rdf:resource="http://www.loa-cnr.it/ontologies/DUL.owl#PhysicalObject"/>
        <rdfs:subClassOf>
            <owl:Restriction>
                <owl:onProperty rdf:resource="http://people.aifb.kit.edu/mu2771/step#runBy"/>
                <owl:someValuesFrom rdf:resource="http://www.w3.org/ns/org#Organization"/>
            </owl:Restriction>
        </rdfs:subClassOf>
        <rdfs:subClassOf>
            <owl:Restriction>
                <owl:onProperty rdf:resource="http://purl.oclc.org/NET/ssnx/ssn#hasSubSystem"/>
                <owl:someValuesFrom rdf:resource="http://purl.oclc.org/NET/ssnx/ssn#System"/>
            </owl:Restriction>
        </rdfs:subClassOf>
        <rdfs:subClassOf>
            <owl:Restriction>
                <owl:onProperty rdf:resource="http://purl.oclc.org/NET/ssnx/ssn#hasDeployment"/>
                <owl:allValuesFrom rdf:resource="http://purl.oclc.org/NET/ssnx/ssn#Deployment"/>
            </owl:Restriction>
        </rdfs:subClassOf>
        <rdfs:subClassOf>
            <owl:Restriction>
                <owl:onProperty rdf:resource="http://purl.oclc.org/NET/ssnx/ssn#hasOperatingRange"/>
                <owl:allValuesFrom rdf:resource="http://purl.oclc.org/NET/ssnx/ssn#OperatingRange"/>
            </owl:Restriction>
        </rdfs:subClassOf>
        <rdfs:subClassOf>
            <owl:Restriction>
                <owl:onProperty rdf:resource="http://purl.oclc.org/NET/ssnx/ssn#hasSubSystem"/>
                <owl:allValuesFrom rdf:resource="http://purl.oclc.org/NET/ssnx/ssn#System"/>
            </owl:Restriction>
        </rdfs:subClassOf>
        <rdfs:subClassOf>
            <owl:Restriction>
                <owl:onProperty rdf:resource="http://purl.oclc.org/NET/ssnx/ssn#hasSurvivalRange"/>
                <owl:allValuesFrom rdf:resource="http://purl.oclc.org/NET/ssnx/ssn#SurvivalRange"/>
            </owl:Restriction>
        </rdfs:subClassOf>
        <rdfs:subClassOf>
            <owl:Restriction>
                <owl:onProperty rdf:resource="http://purl.oclc.org/NET/ssnx/ssn#onPlatform"/>
                <owl:allValuesFrom rdf:resource="http://purl.oclc.org/NET/ssnx/ssn#Platform"/>
            </owl:Restriction>
        </rdfs:subClassOf>
        <dc:source>http://www.w3.org/2005/Incubator/ssn/</dc:source>
        <www:subClassOfInverted rdf:resource="http://purl.oclc.org/NET/ssnx/ssn#Device"/>
        <rdfs:comment>System is a unit of abstraction for pieces of infrastructure (and we largely care that they are) for sensing. A system has components, its subsystems, which are other systems.</rdfs:comment>
        <rdfs:isDefinedBy>http://purl.oclc.org/NET/ssnx/ssn</rdfs:isDefinedBy>
        <rdfs:label>System</rdfs:label>
        <rdfs:label>ssn:System</rdfs:label>
        <rdfs:seeAlso>http://www.w3.org/2005/Incubator/ssn/wiki/SSN_Model#System</rdfs:seeAlso>
    </owl:Class>
    


    <!-- http://purl.oclc.org/NET/ssnx/ssn#SystemLifetime -->

    <owl:Class rdf:about="http://purl.oclc.org/NET/ssnx/ssn#SystemLifetime">
        <rdfs:subClassOf rdf:resource="http://purl.oclc.org/NET/ssnx/ssn#SurvivalProperty"/>
        <rdfs:comment>Total useful life of a sensor/system (expressed as total life since manufacture, time in use, number of operations, etc.).</rdfs:comment>
        <rdfs:isDefinedBy>http://purl.oclc.org/NET/ssnx/ssn</rdfs:isDefinedBy>
        <rdfs:label>System Lifetime</rdfs:label>
        <rdfs:seeAlso>http://www.w3.org/2005/Incubator/ssn/wiki/SSN_Deploy#OperatingRestriction</rdfs:seeAlso>
    </owl:Class>
    


    <!-- http://purl.org/dc/terms/SizeOrDuration -->

    <owl:Class rdf:about="http://purl.org/dc/terms/SizeOrDuration"/>
    


    <!-- http://purl.org/goodrelations/v1#BusinessEntity -->

    <owl:Class rdf:about="http://purl.org/goodrelations/v1#BusinessEntity">
        <rdfs:subClassOf rdf:resource="http://www.w3.org/ns/org#FormalOrganization"/>
    </owl:Class>
    


    <!-- http://purl.org/ontology/mo/produced_signal -->

    <owl:Class rdf:about="http://purl.org/ontology/mo/produced_signal"/>
    


    <!-- http://qudt.org/schema/qudt#AtomicPhysicsQuantityKind -->

    <rdf:Description rdf:about="http://qudt.org/schema/qudt#AtomicPhysicsQuantityKind">
        <rdfs:subClassOf rdf:resource="http://qudt.org/schema/qudt#QuantityKind"/>
    </rdf:Description>
    


    <!-- http://qudt.org/schema/qudt#BiologyQuantityKind -->

    <rdf:Description rdf:about="http://qudt.org/schema/qudt#BiologyQuantityKind">
        <rdfs:subClassOf rdf:resource="http://qudt.org/schema/qudt#QuantityKind"/>
    </rdf:Description>
    


    <!-- http://qudt.org/schema/qudt#ChemistryQuantityKind -->

    <rdf:Description rdf:about="http://qudt.org/schema/qudt#ChemistryQuantityKind">
        <rdfs:subClassOf rdf:resource="http://qudt.org/schema/qudt#QuantityKind"/>
    </rdf:Description>
    


    <!-- http://qudt.org/schema/qudt#CommunicationsQuantityKind -->

    <rdf:Description rdf:about="http://qudt.org/schema/qudt#CommunicationsQuantityKind">
        <rdfs:subClassOf rdf:resource="http://qudt.org/schema/qudt#QuantityKind"/>
    </rdf:Description>
    


    <!-- http://qudt.org/schema/qudt#ElectricityAndMagnetismQuantityKind -->

    <rdf:Description rdf:about="http://qudt.org/schema/qudt#ElectricityAndMagnetismQuantityKind">
        <rdfs:subClassOf rdf:resource="http://qudt.org/schema/qudt#QuantityKind"/>
    </rdf:Description>
    


    <!-- http://qudt.org/schema/qudt#FinancialQuantityKind -->

    <rdf:Description rdf:about="http://qudt.org/schema/qudt#FinancialQuantityKind">
        <rdfs:subClassOf rdf:resource="http://qudt.org/schema/qudt#QuantityKind"/>
    </rdf:Description>
    


    <!-- http://qudt.org/schema/qudt#FluidMechanicsQuantityKind -->

    <rdf:Description rdf:about="http://qudt.org/schema/qudt#FluidMechanicsQuantityKind">
        <rdfs:subClassOf rdf:resource="http://qudt.org/schema/qudt#QuantityKind"/>
    </rdf:Description>
    


    <!-- http://qudt.org/schema/qudt#InformationQuantityKind -->

    <rdf:Description rdf:about="http://qudt.org/schema/qudt#InformationQuantityKind">
        <rdfs:subClassOf rdf:resource="http://qudt.org/schema/qudt#QuantityKind"/>
    </rdf:Description>
    


    <!-- http://qudt.org/schema/qudt#MechanicsQuantityKind -->

    <rdf:Description rdf:about="http://qudt.org/schema/qudt#MechanicsQuantityKind">
        <rdfs:subClassOf rdf:resource="http://qudt.org/schema/qudt#QuantityKind"/>
    </rdf:Description>
    


    <!-- http://qudt.org/schema/qudt#PhotometryQuantityKind -->

    <rdf:Description rdf:about="http://qudt.org/schema/qudt#PhotometryQuantityKind">
        <rdfs:subClassOf rdf:resource="http://qudt.org/schema/qudt#QuantityKind"/>
    </rdf:Description>
    


    <!-- http://qudt.org/schema/qudt#QuantityKind -->

    <rdf:Description rdf:about="http://qudt.org/schema/qudt#QuantityKind">
        <www:subClassOfInverted rdf:resource="http://qudt.org/schema/qudt#AtomicPhysicsQuantityKind"/>
        <www:subClassOfInverted rdf:resource="http://qudt.org/schema/qudt#BiologyQuantityKind"/>
        <www:subClassOfInverted rdf:resource="http://qudt.org/schema/qudt#ChemistryQuantityKind"/>
        <www:subClassOfInverted rdf:resource="http://qudt.org/schema/qudt#CommunicationsQuantityKind"/>
        <www:subClassOfInverted rdf:resource="http://qudt.org/schema/qudt#ElectricityAndMagnetismQuantityKind"/>
        <www:subClassOfInverted rdf:resource="http://qudt.org/schema/qudt#FinancialQuantityKind"/>
        <www:subClassOfInverted rdf:resource="http://qudt.org/schema/qudt#FluidMechanicsQuantityKind"/>
        <www:subClassOfInverted rdf:resource="http://qudt.org/schema/qudt#InformationQuantityKind"/>
        <www:subClassOfInverted rdf:resource="http://qudt.org/schema/qudt#MechanicsQuantityKind"/>
        <www:subClassOfInverted rdf:resource="http://qudt.org/schema/qudt#PhotometryQuantityKind"/>
        <www:subClassOfInverted rdf:resource="http://qudt.org/schema/qudt#QuantumMechanicsQuantityKind"/>
        <www:subClassOfInverted rdf:resource="http://qudt.org/schema/qudt#RadiologyQuantityKind"/>
        <www:subClassOfInverted rdf:resource="http://qudt.org/schema/qudt#RadiometryQuantityKind"/>
        <www:subClassOfInverted rdf:resource="http://qudt.org/schema/qudt#SolidMechanicsQuantityKind"/>
        <www:subClassOfInverted rdf:resource="http://qudt.org/schema/qudt#SpaceAndTimeQuantityKind"/>
        <www:subClassOfInverted rdf:resource="http://qudt.org/schema/qudt#ThermodynamicsQuantityKind"/>
    </rdf:Description>
    


    <!-- http://qudt.org/schema/qudt#QuantumMechanicsQuantityKind -->

    <rdf:Description rdf:about="http://qudt.org/schema/qudt#QuantumMechanicsQuantityKind">
        <rdfs:subClassOf rdf:resource="http://qudt.org/schema/qudt#QuantityKind"/>
    </rdf:Description>
    


    <!-- http://qudt.org/schema/qudt#RadiologyQuantityKind -->

    <rdf:Description rdf:about="http://qudt.org/schema/qudt#RadiologyQuantityKind">
        <rdfs:subClassOf rdf:resource="http://qudt.org/schema/qudt#QuantityKind"/>
    </rdf:Description>
    


    <!-- http://qudt.org/schema/qudt#RadiometryQuantityKind -->

    <rdf:Description rdf:about="http://qudt.org/schema/qudt#RadiometryQuantityKind">
        <rdfs:subClassOf rdf:resource="http://qudt.org/schema/qudt#QuantityKind"/>
    </rdf:Description>
    


    <!-- http://qudt.org/schema/qudt#SolidMechanicsQuantityKind -->

    <rdf:Description rdf:about="http://qudt.org/schema/qudt#SolidMechanicsQuantityKind">
        <rdfs:subClassOf rdf:resource="http://qudt.org/schema/qudt#QuantityKind"/>
    </rdf:Description>
    


    <!-- http://qudt.org/schema/qudt#SpaceAndTimeQuantityKind -->

    <rdf:Description rdf:about="http://qudt.org/schema/qudt#SpaceAndTimeQuantityKind">
        <rdfs:subClassOf rdf:resource="http://qudt.org/schema/qudt#QuantityKind"/>
    </rdf:Description>
    


    <!-- http://qudt.org/schema/qudt#ThermodynamicsQuantityKind -->

    <rdf:Description rdf:about="http://qudt.org/schema/qudt#ThermodynamicsQuantityKind">
        <rdfs:subClassOf rdf:resource="http://qudt.org/schema/qudt#QuantityKind"/>
    </rdf:Description>
    


    <!-- http://qudt.org/schema/qudt#Unit -->

    <owl:Class rdf:about="http://qudt.org/schema/qudt#Unit">
        <www:subClassOfInverted>
            <rdf:Description rdf:nodeID="_:genid135">
                <rdfs:comment xml:lang="en">A standard duration, which provides a scale factor for a time extent, or the granularity or precision for a time position.</rdfs:comment>
                <rdfs:comment>any common used unit of time</rdfs:comment>
                <rdfs:label xml:lang="en">Temporal unit</rdfs:label>
                <rdfs:label>time:TemporalUnit</rdfs:label>
                <skos:changeNote xml:lang="en">Remove enumeration from definition, in order to allow other units to be used when required in other coordinate systems. 
NOTE: existing units are still present as members of the class, but the class membership is now open. 

In the original OWL-Time the following constraint appeared: 
  owl:oneOf (
      time:unitSecond
      time:unitMinute
      time:unitHour
      time:unitDay
      time:unitWeek
      time:unitMonth
      time:unitYear
    ) ;</skos:changeNote>
                <skos:definition xml:lang="en">A standard duration, which provides a scale factor for a time extent, or the granularity or precision for a time position.</skos:definition>
                <skos:note xml:lang="en">Membership of the class TemporalUnit is open, to allow for other temporal units used in some technical applications (e.g. millions of years, Baha&apos;i month).</skos:note>
            </rdf:Description>
        </www:subClassOfInverted>
        <rdfs:label>qudt:Unit</rdfs:label>
    </owl:Class>
    


    <!-- http://vocab.datex.org/terms#equipmentOrSystemFaultType -->

    <owl:Class rdf:about="http://vocab.datex.org/terms#equipmentOrSystemFaultType"/>
    


    <!-- http://www.loa-cnr.it/ontologies/DUL.owl#DesignedArtifact -->

    <owl:Class rdf:about="http://www.loa-cnr.it/ontologies/DUL.owl#DesignedArtifact">
        <www:subClassOfInverted rdf:resource="http://purl.oclc.org/NET/ssnx/ssn#Device"/>
        <rdfs:label>dul:DesignedArtifact</rdfs:label>
    </owl:Class>
    


    <!-- http://www.loa-cnr.it/ontologies/DUL.owl#Event -->

    <owl:Class rdf:about="http://www.loa-cnr.it/ontologies/DUL.owl#Event">
        <www:subClassOfInverted rdf:resource="http://purl.oclc.org/NET/ssnx/ssn#SensorInput"/>
        <www:subClassOfInverted rdf:resource="http://purl.oclc.org/NET/ssnx/ssn#Stimulus"/>
    </owl:Class>
    


    <!-- http://www.loa-cnr.it/ontologies/DUL.owl#InformationObject -->

    <owl:Class rdf:about="http://www.loa-cnr.it/ontologies/DUL.owl#InformationObject">
        <rdfs:subClassOf rdf:resource="http://www.loa-cnr.it/ontologies/DUL.owl#Object"/>
        <www:subClassOfInverted rdf:resource="http://iirds.tekom.de/iirds#iirdsDomainEntitiy"/>
        <www:subClassOfInverted rdf:resource="http://people.aifb.kit.edu/mu2771/step#Alarm"/>
        <www:subClassOfInverted rdf:resource="http://people.aifb.kit.edu/mu2771/step#ElectronicMessage"/>
        <www:subClassOfInverted rdf:resource="http://people.aifb.kit.edu/mu2771/step#Prediction"/>
        <www:subClassOfInverted rdf:resource="http://people.aifb.kit.edu/mu2771/step#Report"/>
        <www:subClassOfInverted rdf:resource="http://purl.oclc.org/NET/ssnx/ssn#Input"/>
        <www:subClassOfInverted rdf:resource="http://purl.oclc.org/NET/ssnx/ssn#ObservationValue"/>
        <www:subClassOfInverted rdf:resource="http://purl.oclc.org/NET/ssnx/ssn#Output"/>
        <www:subClassOfInverted rdf:resource="http://purl.oclc.org/NET/ssnx/ssn#SensorDataSheet"/>
        <www:subClassOfInverted rdf:resource="http://purl.oclc.org/NET/ssnx/ssn#SensorOutput"/>
    </owl:Class>
    


    <!-- http://www.loa-cnr.it/ontologies/DUL.owl#Method -->

    <owl:Class rdf:about="http://www.loa-cnr.it/ontologies/DUL.owl#Method">
        <www:subClassOfInverted rdf:resource="http://purl.oclc.org/NET/ssnx/ssn#Process"/>
    </owl:Class>
    


    <!-- http://www.loa-cnr.it/ontologies/DUL.owl#Object -->

    <owl:Class rdf:about="http://www.loa-cnr.it/ontologies/DUL.owl#Object">
        <www:subClassOfInverted rdf:resource="http://www.loa-cnr.it/ontologies/DUL.owl#InformationObject"/>
        <www:subClassOfInverted rdf:resource="http://www.loa-cnr.it/ontologies/DUL.owl#PhysicalObject"/>
    </owl:Class>
    


    <!-- http://www.loa-cnr.it/ontologies/DUL.owl#PhysicalObject -->

    <owl:Class rdf:about="http://www.loa-cnr.it/ontologies/DUL.owl#PhysicalObject">
        <rdfs:subClassOf rdf:resource="http://www.loa-cnr.it/ontologies/DUL.owl#Object"/>
        <www:subClassOfInverted rdf:resource="http://purl.oclc.org/NET/ssnx/ssn#Platform"/>
        <www:subClassOfInverted rdf:resource="http://purl.oclc.org/NET/ssnx/ssn#Sensor"/>
        <www:subClassOfInverted rdf:resource="http://purl.oclc.org/NET/ssnx/ssn#System"/>
    </owl:Class>
    


    <!-- http://www.loa-cnr.it/ontologies/DUL.owl#Process -->

    <owl:Class rdf:about="http://www.loa-cnr.it/ontologies/DUL.owl#Process">
        <www:subClassOfInverted rdf:resource="http://purl.oclc.org/NET/ssnx/ssn#DeploymentRelatedProcess"/>
    </owl:Class>
    


    <!-- http://www.loa-cnr.it/ontologies/DUL.owl#Quality -->

    <owl:Class rdf:about="http://www.loa-cnr.it/ontologies/DUL.owl#Quality">
        <www:subClassOfInverted rdf:resource="http://purl.oclc.org/NET/ssnx/ssn#Property"/>
    </owl:Class>
    


    <!-- http://www.loa-cnr.it/ontologies/DUL.owl#Region -->

    <owl:Class rdf:about="http://www.loa-cnr.it/ontologies/DUL.owl#Region">
        <www:subClassOfInverted rdf:resource="http://purl.oclc.org/NET/ssnx/ssn#ObservationValue"/>
    </owl:Class>
    


    <!-- http://www.loa-cnr.it/ontologies/DUL.owl#Situation -->

    <owl:Class rdf:about="http://www.loa-cnr.it/ontologies/DUL.owl#Situation">
        <www:subClassOfInverted rdf:resource="http://purl.oclc.org/NET/ssnx/ssn#Observation"/>
    </owl:Class>
    


    <!-- http://www.w3.org/2000/01/rdf-schema#Resource -->

    <owl:Class rdf:about="http://www.w3.org/2000/01/rdf-schema#Resource">
        <www:subClassOfInverted rdf:resource="http://www.w3.org/2006/time#generalYear"/>
    </owl:Class>
    


    <!-- http://www.w3.org/2001/XMLSchema#dateTimeStamp -->

    <owl:Class rdf:about="http://www.w3.org/2001/XMLSchema#dateTimeStamp">
        <rdfs:subClassOf rdf:resource="http://www.w3.org/2000/01/rdf-schema#Literal"/>
    </owl:Class>
    


    <!-- http://www.w3.org/2002/07/owl#Thing -->

    <rdf:Description rdf:about="http://www.w3.org/2002/07/owl#Thing">
        <www:subClassOfInverted rdf:resource="http://purl.oclc.org/NET/ssnx/ssn#FeatureOfInterest"/>
        <www:subClassOfInverted rdf:resource="http://www.w3.org/2006/time#DayOfWeek"/>
        <www:subClassOfInverted>
            <rdf:Description>
                <rdfs:comment xml:lang="en">A temporal interval or instant.</rdfs:comment>
                <rdfs:comment rdf:datatype="http://www.w3.org/2001/XMLSchema#string">defines a time concept based on the gregorian calendar </rdfs:comment>
                <rdfs:label xml:lang="en">Temporal entity</rdfs:label>
                <rdfs:label>time:TemporalEntity</rdfs:label>
                <skos:definition xml:lang="en">A temporal interval or instant.</skos:definition>
            </rdf:Description>
        </www:subClassOfInverted>
    </rdf:Description>
    


    <!-- http://www.w3.org/2003/01/geo/wgs84_pos#Point -->

    <owl:Class rdf:about="http://www.w3.org/2003/01/geo/wgs84_pos#Point">
        <rdfs:subClassOf rdf:resource="http://www.w3.org/2003/01/geo/wgs84_pos#SpatialThing"/>
        <rdfs:comment> 
Uniquely identified by lat/long/alt. i.e.

spaciallyIntersects(P1, P2) :- lat(P1, LAT), long(P1, LONG), alt(P1, ALT),
  lat(P2, LAT), long(P2, LONG), alt(P2, ALT).

sameThing(P1, P2) :- type(P1, Point), type(P2, Point), spaciallyIntersects(P1, P2).
  </rdfs:comment>
        <rdfs:comment>A point, typically described using a coordinate system relative to Earth, such as WGS84.
  </rdfs:comment>
        <rdfs:label>point</rdfs:label>
    </owl:Class>
    


    <!-- http://www.w3.org/2003/01/geo/wgs84_pos#SpatialThing -->

    <owl:Class rdf:about="http://www.w3.org/2003/01/geo/wgs84_pos#SpatialThing">
        <owl:equivalentClass rdf:resource="http://www.w3.org/2006/vcard/ns#Location"/>
        <www:subClassOfInverted rdf:resource="http://people.aifb.kit.edu/mu2771/step#SpatialTemporalEntity"/>
        <www:subClassOfInverted rdf:resource="http://www.w3.org/2003/01/geo/wgs84_pos#Point"/>
        <www:subClassOfInverted>
            <rdf:Description>
                <rdfs:comment xml:lang="en">To specify the components of the delivery address for the  object</rdfs:comment>
                <rdfs:isDefinedBy rdf:resource="http://www.w3.org/2006/vcard/ns"/>
                <rdfs:label xml:lang="en">Address</rdfs:label>
            </rdf:Description>
        </www:subClassOfInverted>
        <rdfs:comment>Anything with spatial extent, i.e. size, shape, or position.
 e.g. people, places, bowling balls, as well as abstract areas like cubes.
</rdfs:comment>
        <rdfs:comment>SpatialThing</rdfs:comment>
        <rdfs:label>SpatialThing</rdfs:label>
    </owl:Class>
    


    <!-- http://www.w3.org/2004/02/skos/core#Concept -->

    <owl:Class rdf:about="http://www.w3.org/2004/02/skos/core#Concept">
        <www:subClassOfInverted rdf:resource="http://www.w3.org/ns/org#Role"/>
    </owl:Class>
    


    <!-- http://www.w3.org/2006/time#DateTimeDescription -->

    <owl:Class rdf:about="http://www.w3.org/2006/time#DateTimeDescription">
        <rdfs:subClassOf rdf:resource="http://www.w3.org/2006/time#GeneralDateTimeDescription"/>
        <rdfs:subClassOf>
            <owl:Restriction>
                <owl:onProperty rdf:resource="http://www.w3.org/2006/time#hasTRS"/>
                <owl:hasValue rdf:resource="http://www.opengis.net/def/uom/ISO-8601/0/Gregorian"/>
            </owl:Restriction>
        </rdfs:subClassOf>
        <rdfs:subClassOf>
            <owl:Restriction>
                <owl:onProperty rdf:resource="http://www.w3.org/2006/time#day"/>
                <owl:allValuesFrom rdf:resource="http://www.w3.org/2001/XMLSchema#gDay"/>
            </owl:Restriction>
        </rdfs:subClassOf>
        <rdfs:subClassOf>
            <owl:Restriction>
                <owl:onProperty rdf:resource="http://www.w3.org/2006/time#month"/>
                <owl:allValuesFrom rdf:resource="http://www.w3.org/2001/XMLSchema#gMonth"/>
            </owl:Restriction>
        </rdfs:subClassOf>
        <rdfs:subClassOf>
            <owl:Restriction>
                <owl:onProperty rdf:resource="http://www.w3.org/2006/time#year"/>
                <owl:allValuesFrom rdf:resource="http://www.w3.org/2001/XMLSchema#gYear"/>
            </owl:Restriction>
        </rdfs:subClassOf>
        <www:subClassOfInverted rdf:resource="http://www.w3.org/2006/time#January"/>
        <www:subClassOfInverted rdf:resource="http://www.w3.org/2006/time#MonthOfYear"/>
        <rdfs:comment xml:lang="en">Description of date and time structured with separate values for the various elements of a calendar-clock system. The temporal reference system is fixed to Gregorian Calendar, and the range of year, month, day properties restricted to corresponding XML Schema types xsd:gYear, xsd:gMonth and xsd:gDay, respectively.</rdfs:comment>
        <rdfs:label xml:lang="en">Date-Time description</rdfs:label>
        <skos:definition xml:lang="en">Description of date and time structured with separate values for the various elements of a calendar-clock system. The temporal reference system is fixed to Gregorian Calendar, and the range of year, month, day properties restricted to corresponding XML Schema types xsd:gYear, xsd:gMonth and xsd:gDay, respectively.</skos:definition>
    </owl:Class>
    


    <!-- http://www.w3.org/2006/time#DateTimeInterval -->

    <owl:Class rdf:about="http://www.w3.org/2006/time#DateTimeInterval">
        <rdfs:subClassOf rdf:resource="http://www.w3.org/2006/time#ProperInterval"/>
        <rdfs:comment xml:lang="en">DateTimeInterval is a subclass of ProperInterval, defined using the multi-element DateTimeDescription.</rdfs:comment>
        <rdfs:label xml:lang="en">Date-time interval</rdfs:label>
        <skos:definition xml:lang="en">DateTimeInterval is a subclass of ProperInterval, defined using the multi-element DateTimeDescription.</skos:definition>
        <skos:note xml:lang="en">:DateTimeInterval can only be used for an interval whose limits coincide with a date-time element aligned to the calendar and timezone indicated. For example, while both have a duration of one day, the 24-hour interval beginning at midnight at the beginning of 8 May in Central Europe can be expressed as a :DateTimeInterval, but the 24-hour interval starting at 1:30pm cannot.</skos:note>
    </owl:Class>
    


    <!-- http://www.w3.org/2006/time#DayOfWeek -->

    <owl:Class rdf:about="http://www.w3.org/2006/time#DayOfWeek">
        <rdfs:subClassOf rdf:resource="http://www.w3.org/2002/07/owl#Thing"/>
        <rdfs:subClassOf rdf:resource="http://www.w3.org/2006/time#TemporalEntity"/>
        <rdfs:comment xml:lang="en">The day of week</rdfs:comment>
        <rdfs:label xml:lang="en">Day of week</rdfs:label>
        <skos:changeNote xml:lang="en">Remove enumeration from definition, in order to allow other days to be used when required in other calendars. 
NOTE: existing days are still present as members of the class, but the class membership is now open. 

In the original OWL-Time the following constraint appeared: 
  owl:oneOf (
      time:Monday
      time:Tuesday
      time:Wednesday
      time:Thursday
      time:Friday
      time:Saturday
      time:Sunday
    ) ;</skos:changeNote>
        <skos:definition xml:lang="en">The day of week</skos:definition>
        <skos:note xml:lang="en">Membership of the class :DayOfWeek is open, to allow for alternative week lengths and different day names.</skos:note>
    </owl:Class>
    


    <!-- http://www.w3.org/2006/time#Duration -->

    <owl:Class rdf:about="http://www.w3.org/2006/time#Duration">
        <rdfs:subClassOf rdf:resource="http://www.w3.org/2006/time#TemporalDuration"/>
        <rdfs:subClassOf>
            <owl:Restriction>
                <owl:onProperty rdf:resource="http://www.w3.org/2006/time#unitType"/>
                <owl:cardinality rdf:datatype="http://www.w3.org/2001/XMLSchema#nonNegativeInteger">1</owl:cardinality>
            </owl:Restriction>
        </rdfs:subClassOf>
        <rdfs:subClassOf>
            <owl:Restriction>
                <owl:onProperty rdf:resource="http://www.w3.org/2006/time#numericDuration"/>
                <owl:cardinality rdf:datatype="http://www.w3.org/2001/XMLSchema#nonNegativeInteger">1</owl:cardinality>
            </owl:Restriction>
        </rdfs:subClassOf>
        <rdfs:comment xml:lang="en">Duration of a temporal extent expressed as a number scaled by a temporal unit</rdfs:comment>
        <rdfs:label xml:lang="en">Time duration</rdfs:label>
        <skos:definition xml:lang="en">Duration of a temporal extent expressed as a number scaled by a temporal unit</skos:definition>
        <skos:note xml:lang="en">Alternative to time:DurationDescription to support description of a temporal duration other than using a calendar/clock system.</skos:note>
    </owl:Class>
    


    <!-- http://www.w3.org/2006/time#DurationDescription -->

    <owl:Class rdf:about="http://www.w3.org/2006/time#DurationDescription">
        <rdfs:subClassOf rdf:resource="http://www.w3.org/2006/time#GeneralDurationDescription"/>
        <rdfs:subClassOf>
            <owl:Restriction>
                <owl:onProperty rdf:resource="http://www.w3.org/2006/time#hasTRS"/>
                <owl:hasValue rdf:resource="http://www.opengis.net/def/uom/ISO-8601/0/Gregorian"/>
            </owl:Restriction>
        </rdfs:subClassOf>
        <rdfs:subClassOf>
            <owl:Restriction>
                <owl:onProperty rdf:resource="http://www.w3.org/2006/time#days"/>
                <owl:allValuesFrom rdf:resource="http://www.w3.org/2001/XMLSchema#decimal"/>
            </owl:Restriction>
        </rdfs:subClassOf>
        <rdfs:subClassOf>
            <owl:Restriction>
                <owl:onProperty rdf:resource="http://www.w3.org/2006/time#hours"/>
                <owl:allValuesFrom rdf:resource="http://www.w3.org/2001/XMLSchema#decimal"/>
            </owl:Restriction>
        </rdfs:subClassOf>
        <rdfs:subClassOf>
            <owl:Restriction>
                <owl:onProperty rdf:resource="http://www.w3.org/2006/time#minutes"/>
                <owl:allValuesFrom rdf:resource="http://www.w3.org/2001/XMLSchema#decimal"/>
            </owl:Restriction>
        </rdfs:subClassOf>
        <rdfs:subClassOf>
            <owl:Restriction>
                <owl:onProperty rdf:resource="http://www.w3.org/2006/time#months"/>
                <owl:allValuesFrom rdf:resource="http://www.w3.org/2001/XMLSchema#decimal"/>
            </owl:Restriction>
        </rdfs:subClassOf>
        <rdfs:subClassOf>
            <owl:Restriction>
                <owl:onProperty rdf:resource="http://www.w3.org/2006/time#seconds"/>
                <owl:allValuesFrom rdf:resource="http://www.w3.org/2001/XMLSchema#decimal"/>
            </owl:Restriction>
        </rdfs:subClassOf>
        <rdfs:subClassOf>
            <owl:Restriction>
                <owl:onProperty rdf:resource="http://www.w3.org/2006/time#weeks"/>
                <owl:allValuesFrom rdf:resource="http://www.w3.org/2001/XMLSchema#decimal"/>
            </owl:Restriction>
        </rdfs:subClassOf>
        <rdfs:subClassOf>
            <owl:Restriction>
                <owl:onProperty rdf:resource="http://www.w3.org/2006/time#years"/>
                <owl:allValuesFrom rdf:resource="http://www.w3.org/2001/XMLSchema#decimal"/>
            </owl:Restriction>
        </rdfs:subClassOf>
        <rdfs:subClassOf>
            <owl:Restriction>
                <owl:onProperty rdf:resource="http://www.w3.org/2006/time#hours"/>
                <owl:maxCardinality rdf:datatype="http://www.w3.org/2001/XMLSchema#nonNegativeInteger">1</owl:maxCardinality>
            </owl:Restriction>
        </rdfs:subClassOf>
        <rdfs:subClassOf>
            <owl:Restriction>
                <owl:onProperty rdf:resource="http://www.w3.org/2006/time#minutes"/>
                <owl:maxCardinality rdf:datatype="http://www.w3.org/2001/XMLSchema#nonNegativeInteger">1</owl:maxCardinality>
            </owl:Restriction>
        </rdfs:subClassOf>
        <rdfs:subClassOf>
            <owl:Restriction>
                <owl:onProperty rdf:resource="http://www.w3.org/2006/time#months"/>
                <owl:maxCardinality rdf:datatype="http://www.w3.org/2001/XMLSchema#nonNegativeInteger">1</owl:maxCardinality>
            </owl:Restriction>
        </rdfs:subClassOf>
        <rdfs:subClassOf>
            <owl:Restriction>
                <owl:onProperty rdf:resource="http://www.w3.org/2006/time#seconds"/>
                <owl:maxCardinality rdf:datatype="http://www.w3.org/2001/XMLSchema#nonNegativeInteger">1</owl:maxCardinality>
            </owl:Restriction>
        </rdfs:subClassOf>
        <rdfs:subClassOf>
            <owl:Restriction>
                <owl:onProperty rdf:resource="http://www.w3.org/2006/time#weeks"/>
                <owl:maxCardinality rdf:datatype="http://www.w3.org/2001/XMLSchema#nonNegativeInteger">1</owl:maxCardinality>
            </owl:Restriction>
        </rdfs:subClassOf>
        <rdfs:subClassOf>
            <owl:Restriction>
                <owl:onProperty rdf:resource="http://www.w3.org/2006/time#years"/>
                <owl:maxCardinality rdf:datatype="http://www.w3.org/2001/XMLSchema#nonNegativeInteger">1</owl:maxCardinality>
            </owl:Restriction>
        </rdfs:subClassOf>
        <www:subClassOfInverted rdf:resource="http://www.w3.org/2006/time#Year"/>
        <rdfs:comment xml:lang="en">Description of temporal extent structured with separate values for the various elements of a calendar-clock system. The temporal reference system is fixed to Gregorian Calendar, and the range of each of the numeric properties is restricted to xsd:decimal</rdfs:comment>
        <rdfs:label xml:lang="en">Duration description</rdfs:label>
        <rdfs:label>time:DurationDescription</rdfs:label>
        <skos:definition xml:lang="en">Description of temporal extent structured with separate values for the various elements of a calendar-clock system. The temporal reference system is fixed to Gregorian Calendar, and the range of each of the numeric properties is restricted to xsd:decimal</skos:definition>
        <skos:note xml:lang="en">In the Gregorian calendar the length of the month is not fixed. Therefore, a value like &quot;2.5 months&quot; cannot be exactly compared with a similar duration expressed in terms of weeks or days.</skos:note>
    </owl:Class>
    


    <!-- http://www.w3.org/2006/time#GeneralDateTimeDescription -->

    <owl:Class rdf:about="http://www.w3.org/2006/time#GeneralDateTimeDescription">
        <rdfs:subClassOf rdf:resource="http://www.w3.org/2006/time#TemporalPosition"/>
        <rdfs:subClassOf>
            <owl:Restriction>
                <owl:onProperty rdf:resource="http://www.w3.org/2006/time#unitType"/>
                <owl:cardinality rdf:datatype="http://www.w3.org/2001/XMLSchema#nonNegativeInteger">1</owl:cardinality>
            </owl:Restriction>
        </rdfs:subClassOf>
        <rdfs:subClassOf>
            <owl:Restriction>
                <owl:onProperty rdf:resource="http://www.w3.org/2006/time#dayOfWeek"/>
                <owl:maxCardinality rdf:datatype="http://www.w3.org/2001/XMLSchema#nonNegativeInteger">1</owl:maxCardinality>
            </owl:Restriction>
        </rdfs:subClassOf>
        <rdfs:subClassOf>
            <owl:Restriction>
                <owl:onProperty rdf:resource="http://www.w3.org/2006/time#monthOfYear"/>
                <owl:maxCardinality rdf:datatype="http://www.w3.org/2001/XMLSchema#nonNegativeInteger">1</owl:maxCardinality>
            </owl:Restriction>
        </rdfs:subClassOf>
        <rdfs:subClassOf>
            <owl:Restriction>
                <owl:onProperty rdf:resource="http://www.w3.org/2006/time#timeZone"/>
                <owl:maxCardinality rdf:datatype="http://www.w3.org/2001/XMLSchema#nonNegativeInteger">1</owl:maxCardinality>
            </owl:Restriction>
        </rdfs:subClassOf>
        <rdfs:subClassOf>
            <owl:Restriction>
                <owl:onProperty rdf:resource="http://www.w3.org/2006/time#day"/>
                <owl:maxCardinality rdf:datatype="http://www.w3.org/2001/XMLSchema#nonNegativeInteger">1</owl:maxCardinality>
            </owl:Restriction>
        </rdfs:subClassOf>
        <rdfs:subClassOf>
            <owl:Restriction>
                <owl:onProperty rdf:resource="http://www.w3.org/2006/time#dayOfYear"/>
                <owl:maxCardinality rdf:datatype="http://www.w3.org/2001/XMLSchema#nonNegativeInteger">1</owl:maxCardinality>
            </owl:Restriction>
        </rdfs:subClassOf>
        <rdfs:subClassOf>
            <owl:Restriction>
                <owl:onProperty rdf:resource="http://www.w3.org/2006/time#hour"/>
                <owl:maxCardinality rdf:datatype="http://www.w3.org/2001/XMLSchema#nonNegativeInteger">1</owl:maxCardinality>
            </owl:Restriction>
        </rdfs:subClassOf>
        <rdfs:subClassOf>
            <owl:Restriction>
                <owl:onProperty rdf:resource="http://www.w3.org/2006/time#minute"/>
                <owl:maxCardinality rdf:datatype="http://www.w3.org/2001/XMLSchema#nonNegativeInteger">1</owl:maxCardinality>
            </owl:Restriction>
        </rdfs:subClassOf>
        <rdfs:subClassOf>
            <owl:Restriction>
                <owl:onProperty rdf:resource="http://www.w3.org/2006/time#month"/>
                <owl:maxCardinality rdf:datatype="http://www.w3.org/2001/XMLSchema#nonNegativeInteger">1</owl:maxCardinality>
            </owl:Restriction>
        </rdfs:subClassOf>
        <rdfs:subClassOf>
            <owl:Restriction>
                <owl:onProperty rdf:resource="http://www.w3.org/2006/time#second"/>
                <owl:maxCardinality rdf:datatype="http://www.w3.org/2001/XMLSchema#nonNegativeInteger">1</owl:maxCardinality>
            </owl:Restriction>
        </rdfs:subClassOf>
        <rdfs:subClassOf>
            <owl:Restriction>
                <owl:onProperty rdf:resource="http://www.w3.org/2006/time#week"/>
                <owl:maxCardinality rdf:datatype="http://www.w3.org/2001/XMLSchema#nonNegativeInteger">1</owl:maxCardinality>
            </owl:Restriction>
        </rdfs:subClassOf>
        <rdfs:subClassOf>
            <owl:Restriction>
                <owl:onProperty rdf:resource="http://www.w3.org/2006/time#year"/>
                <owl:maxCardinality rdf:datatype="http://www.w3.org/2001/XMLSchema#nonNegativeInteger">1</owl:maxCardinality>
            </owl:Restriction>
        </rdfs:subClassOf>
        <www:subClassOfInverted rdf:resource="http://www.w3.org/2006/time#DateTimeDescription"/>
        <rdfs:comment xml:lang="en">Description of date and time structured with separate values for the various elements of a calendar-clock system</rdfs:comment>
        <rdfs:label xml:lang="en">Generalized date-time description</rdfs:label>
        <skos:definition xml:lang="en">Description of date and time structured with separate values for the various elements of a calendar-clock system</skos:definition>
        <skos:note>Some combinations of properties are redundant - for example, within a specified :year if :dayOfYear is provided then :day and :month can be computed, and vice versa. Individual values should be consistent with each other and the calendar, indicated through the value of the :hasTRS property.</skos:note>
    </owl:Class>
    


    <!-- http://www.w3.org/2006/time#GeneralDurationDescription -->

    <owl:Class rdf:about="http://www.w3.org/2006/time#GeneralDurationDescription">
        <rdfs:subClassOf rdf:resource="http://www.w3.org/2006/time#TemporalDuration"/>
        <rdfs:subClassOf>
            <owl:Restriction>
                <owl:onProperty rdf:resource="http://www.w3.org/2006/time#hasTRS"/>
                <owl:cardinality rdf:datatype="http://www.w3.org/2001/XMLSchema#nonNegativeInteger">1</owl:cardinality>
            </owl:Restriction>
        </rdfs:subClassOf>
        <rdfs:subClassOf>
            <owl:Restriction>
                <owl:onProperty rdf:resource="http://www.w3.org/2006/time#days"/>
                <owl:maxCardinality rdf:datatype="http://www.w3.org/2001/XMLSchema#nonNegativeInteger">1</owl:maxCardinality>
            </owl:Restriction>
        </rdfs:subClassOf>
        <rdfs:subClassOf>
            <owl:Restriction>
                <owl:onProperty rdf:resource="http://www.w3.org/2006/time#hours"/>
                <owl:maxCardinality rdf:datatype="http://www.w3.org/2001/XMLSchema#nonNegativeInteger">1</owl:maxCardinality>
            </owl:Restriction>
        </rdfs:subClassOf>
        <rdfs:subClassOf>
            <owl:Restriction>
                <owl:onProperty rdf:resource="http://www.w3.org/2006/time#minutes"/>
                <owl:maxCardinality rdf:datatype="http://www.w3.org/2001/XMLSchema#nonNegativeInteger">1</owl:maxCardinality>
            </owl:Restriction>
        </rdfs:subClassOf>
        <rdfs:subClassOf>
            <owl:Restriction>
                <owl:onProperty rdf:resource="http://www.w3.org/2006/time#months"/>
                <owl:maxCardinality rdf:datatype="http://www.w3.org/2001/XMLSchema#nonNegativeInteger">1</owl:maxCardinality>
            </owl:Restriction>
        </rdfs:subClassOf>
        <rdfs:subClassOf>
            <owl:Restriction>
                <owl:onProperty rdf:resource="http://www.w3.org/2006/time#seconds"/>
                <owl:maxCardinality rdf:datatype="http://www.w3.org/2001/XMLSchema#nonNegativeInteger">1</owl:maxCardinality>
            </owl:Restriction>
        </rdfs:subClassOf>
        <rdfs:subClassOf>
            <owl:Restriction>
                <owl:onProperty rdf:resource="http://www.w3.org/2006/time#weeks"/>
                <owl:maxCardinality rdf:datatype="http://www.w3.org/2001/XMLSchema#nonNegativeInteger">1</owl:maxCardinality>
            </owl:Restriction>
        </rdfs:subClassOf>
        <rdfs:subClassOf>
            <owl:Restriction>
                <owl:onProperty rdf:resource="http://www.w3.org/2006/time#years"/>
                <owl:maxCardinality rdf:datatype="http://www.w3.org/2001/XMLSchema#nonNegativeInteger">1</owl:maxCardinality>
            </owl:Restriction>
        </rdfs:subClassOf>
        <www:subClassOfInverted rdf:resource="http://www.w3.org/2006/time#DurationDescription"/>
        <rdfs:comment xml:lang="en">Description of temporal extent structured with separate values for the various elements of a calendar-clock system.</rdfs:comment>
        <rdfs:label xml:lang="en">Generalized duration description</rdfs:label>
        <skos:definition xml:lang="en">Description of temporal extent structured with separate values for the various elements of a calendar-clock system.</skos:definition>
        <skos:note xml:lang="en">The extent of a time duration expressed as a GeneralDurationDescription depends on the Temporal Reference System. In some calendars the length of the week or month is not constant within the year. Therefore, a value like &quot;2.5 months&quot; may not necessarily be exactly compared with a similar duration expressed in terms of weeks or days. When non-earth-based calendars are considered even more care must be taken in comparing durations.</skos:note>
    </owl:Class>
    


    <!-- http://www.w3.org/2006/time#Instant -->

    <owl:Class rdf:about="http://www.w3.org/2006/time#Instant">
        <rdfs:subClassOf rdf:resource="http://www.w3.org/2006/time#TemporalEntity"/>
        <owl:disjointWith rdf:resource="http://www.w3.org/2006/time#ProperInterval"/>
        <www:subClassOfInverted rdf:resource="http://people.aifb.kit.edu/mu2771/step#SpatialTemporalEntity"/>
        <rdfs:comment xml:lang="en">A temporal entity with zero extent or duration</rdfs:comment>
        <rdfs:comment rdf:datatype="http://www.w3.org/2001/XMLSchema#string">a single point in time</rdfs:comment>
        <rdfs:label xml:lang="en">Time instant</rdfs:label>
        <rdfs:label>time:Instant</rdfs:label>
        <skos:definition xml:lang="en">A temporal entity with zero extent or duration</skos:definition>
    </owl:Class>
    


    <!-- http://www.w3.org/2006/time#Interval -->

    <owl:Class rdf:about="http://www.w3.org/2006/time#Interval">
        <rdfs:subClassOf rdf:resource="http://www.w3.org/2006/time#TemporalEntity"/>
        <www:subClassOfInverted rdf:resource="http://www.w3.org/2006/time#ProperInterval"/>
        <rdfs:comment xml:lang="en">A temporal entity with an extent or duration</rdfs:comment>
        <rdfs:comment rdf:datatype="http://www.w3.org/2001/XMLSchema#string">time interval with an inclusive start and end</rdfs:comment>
        <rdfs:label xml:lang="en">Time interval</rdfs:label>
        <rdfs:label>time:Interval</rdfs:label>
        <skos:definition xml:lang="en">A temporal entity with an extent or duration</skos:definition>
    </owl:Class>
    


    <!-- http://www.w3.org/2006/time#January -->

    <owl:Class rdf:about="http://www.w3.org/2006/time#January">
        <rdfs:subClassOf rdf:resource="http://www.w3.org/2006/time#DateTimeDescription"/>
        <rdfs:subClassOf>
            <owl:Restriction>
                <owl:onProperty rdf:resource="http://www.w3.org/2006/time#unitType"/>
                <owl:hasValue rdf:resource="http://www.w3.org/2006/time#unitMonth"/>
            </owl:Restriction>
        </rdfs:subClassOf>
        <rdfs:subClassOf>
            <owl:Restriction>
                <owl:onProperty rdf:resource="http://www.w3.org/2006/time#month"/>
                <owl:hasValue>--01</owl:hasValue>
            </owl:Restriction>
        </rdfs:subClassOf>
        <rdfs:label>January</rdfs:label>
        <owl:deprecated rdf:datatype="http://www.w3.org/2001/XMLSchema#boolean">true</owl:deprecated>
        <skos:historyNote>This class was present in the 2006 version of OWL-Time. It was presented as an example of how DateTimeDescription could be specialized, but does not belong in the revised ontology. </skos:historyNote>
    </owl:Class>
    


    <!-- http://www.w3.org/2006/time#MonthOfYear -->

    <owl:Class rdf:about="http://www.w3.org/2006/time#MonthOfYear">
        <rdfs:subClassOf rdf:resource="http://www.w3.org/2006/time#DateTimeDescription"/>
        <rdfs:subClassOf>
            <owl:Restriction>
                <owl:onProperty rdf:resource="http://www.w3.org/2006/time#unitType"/>
                <owl:hasValue rdf:resource="http://www.w3.org/2006/time#unitMonth"/>
            </owl:Restriction>
        </rdfs:subClassOf>
        <rdfs:subClassOf>
            <owl:Restriction>
                <owl:onProperty rdf:resource="http://www.w3.org/2006/time#day"/>
                <owl:cardinality rdf:datatype="http://www.w3.org/2001/XMLSchema#nonNegativeInteger">0</owl:cardinality>
            </owl:Restriction>
        </rdfs:subClassOf>
        <rdfs:subClassOf>
            <owl:Restriction>
                <owl:onProperty rdf:resource="http://www.w3.org/2006/time#hour"/>
                <owl:cardinality rdf:datatype="http://www.w3.org/2001/XMLSchema#nonNegativeInteger">0</owl:cardinality>
            </owl:Restriction>
        </rdfs:subClassOf>
        <rdfs:subClassOf>
            <owl:Restriction>
                <owl:onProperty rdf:resource="http://www.w3.org/2006/time#minute"/>
                <owl:cardinality rdf:datatype="http://www.w3.org/2001/XMLSchema#nonNegativeInteger">0</owl:cardinality>
            </owl:Restriction>
        </rdfs:subClassOf>
        <rdfs:subClassOf>
            <owl:Restriction>
                <owl:onProperty rdf:resource="http://www.w3.org/2006/time#month"/>
                <owl:cardinality rdf:datatype="http://www.w3.org/2001/XMLSchema#nonNegativeInteger">1</owl:cardinality>
            </owl:Restriction>
        </rdfs:subClassOf>
        <rdfs:subClassOf>
            <owl:Restriction>
                <owl:onProperty rdf:resource="http://www.w3.org/2006/time#second"/>
                <owl:cardinality rdf:datatype="http://www.w3.org/2001/XMLSchema#nonNegativeInteger">0</owl:cardinality>
            </owl:Restriction>
        </rdfs:subClassOf>
        <rdfs:subClassOf>
            <owl:Restriction>
                <owl:onProperty rdf:resource="http://www.w3.org/2006/time#week"/>
                <owl:cardinality rdf:datatype="http://www.w3.org/2001/XMLSchema#nonNegativeInteger">0</owl:cardinality>
            </owl:Restriction>
        </rdfs:subClassOf>
        <rdfs:subClassOf>
            <owl:Restriction>
                <owl:onProperty rdf:resource="http://www.w3.org/2006/time#year"/>
                <owl:cardinality rdf:datatype="http://www.w3.org/2001/XMLSchema#nonNegativeInteger">0</owl:cardinality>
            </owl:Restriction>
        </rdfs:subClassOf>
        <rdfs:comment xml:lang="en">The month of the year</rdfs:comment>
        <rdfs:label xml:lang="en">Month of year</rdfs:label>
        <skos:definition xml:lang="en">The month of the year</skos:definition>
        <skos:editorialNote xml:lang="en">Feature at risk - added in 2017 revision, and not yet widely used. </skos:editorialNote>
        <skos:note xml:lang="en">Membership of the class :MonthOfYear is open, to allow for alternative annual calendars and different month names.</skos:note>
    </owl:Class>
    


    <!-- http://www.w3.org/2006/time#ProperInterval -->

    <owl:Class rdf:about="http://www.w3.org/2006/time#ProperInterval">
        <rdfs:subClassOf rdf:resource="http://www.w3.org/2006/time#Interval"/>
        <www:subClassOfInverted rdf:resource="http://www.w3.org/2006/time#DateTimeInterval"/>
        <rdfs:comment xml:lang="en">A temporal entity with non-zero extent or duration, i.e. for which the value of the beginning and end are different</rdfs:comment>
        <rdfs:comment rdf:datatype="http://www.w3.org/2001/XMLSchema#string">a finite time interval</rdfs:comment>
        <rdfs:label xml:lang="en">Proper interval</rdfs:label>
        <skos:definition xml:lang="en">A temporal entity with non-zero extent or duration, i.e. for which the value of the beginning and end are different</skos:definition>
    </owl:Class>
    


    <!-- http://www.w3.org/2006/time#TRS -->

    <owl:Class rdf:about="http://www.w3.org/2006/time#TRS">
        <rdfs:subClassOf rdf:resource="http://www.w3.org/2006/time#TemporalEntity"/>
        <www:subClassOfInverted rdf:resource="http://www.w3.org/2006/time#TimeZone"/>
        <rdfs:comment xml:lang="en">A temporal reference system, such as a temporal coordinate system (with an origin, direction, and scale), a calendar-clock combination, or a (possibly hierarchical) ordinal system. 

This is a stub class, representing the set of all temporal reference systems.</rdfs:comment>
        <rdfs:label xml:lang="en">Temporal Reference System</rdfs:label>
        <skos:definition xml:lang="en">A temporal reference system, such as a temporal coordinate system (with an origin, direction, and scale), a calendar-clock combination, or a (possibly hierarchical) ordinal system. 

This is a stub class, representing the set of all temporal reference systems.</skos:definition>
        <skos:note xml:lang="en">A taxonomy of temporal reference systems is provided in ISO 19108:2002 [ISO19108], including (a) calendar + clock systems; (b) temporal coordinate systems (i.e. numeric offset from an epoch); (c) temporal ordinal reference systems (i.e. ordered sequence of named intervals, not necessarily of equal duration).</skos:note>
    </owl:Class>
    


    <!-- http://www.w3.org/2006/time#TemporalDuration -->

    <owl:Class rdf:about="http://www.w3.org/2006/time#TemporalDuration">
        <rdfs:subClassOf rdf:resource="http://www.w3.org/2006/time#TemporalEntity"/>
        <www:subClassOfInverted rdf:resource="http://www.w3.org/2006/time#Duration"/>
        <www:subClassOfInverted rdf:resource="http://www.w3.org/2006/time#GeneralDurationDescription"/>
        <www:subClassOfInverted>
            <rdf:Description rdf:nodeID="_:genid188">
                <rdfs:comment xml:lang="en">A standard duration, which provides a scale factor for a time extent, or the granularity or precision for a time position.</rdfs:comment>
                <rdfs:comment>any common used unit of time</rdfs:comment>
                <rdfs:label xml:lang="en">Temporal unit</rdfs:label>
                <rdfs:label>time:TemporalUnit</rdfs:label>
                <skos:changeNote xml:lang="en">Remove enumeration from definition, in order to allow other units to be used when required in other coordinate systems. 
NOTE: existing units are still present as members of the class, but the class membership is now open. 

In the original OWL-Time the following constraint appeared: 
  owl:oneOf (
      time:unitSecond
      time:unitMinute
      time:unitHour
      time:unitDay
      time:unitWeek
      time:unitMonth
      time:unitYear
    ) ;</skos:changeNote>
                <skos:definition xml:lang="en">A standard duration, which provides a scale factor for a time extent, or the granularity or precision for a time position.</skos:definition>
                <skos:note xml:lang="en">Membership of the class TemporalUnit is open, to allow for other temporal units used in some technical applications (e.g. millions of years, Baha&apos;i month).</skos:note>
            </rdf:Description>
        </www:subClassOfInverted>
        <rdfs:comment xml:lang="en">Time extent; duration of a time interval separate from its particular start position</rdfs:comment>
        <rdfs:label xml:lang="en">Temporal duration</rdfs:label>
        <skos:definition xml:lang="en">Time extent; duration of a time interval separate from its particular start position</skos:definition>
    </owl:Class>
    


    <!-- http://www.w3.org/2006/time#TemporalEntity -->

    <owl:Class rdf:about="http://www.w3.org/2006/time#TemporalEntity">
        <owl:equivalentClass>
            <owl:Class>
                <owl:unionOf rdf:parseType="Collection">
                    <rdf:Description rdf:about="http://www.w3.org/2006/time#Instant"/>
                    <rdf:Description rdf:about="http://www.w3.org/2006/time#Interval"/>
                </owl:unionOf>
            </owl:Class>
        </owl:equivalentClass>
        <www:subClassOfInverted rdf:resource="http://www.w3.org/2006/time#DayOfWeek"/>
        <www:subClassOfInverted rdf:resource="http://www.w3.org/2006/time#Instant"/>
        <www:subClassOfInverted rdf:resource="http://www.w3.org/2006/time#Interval"/>
        <www:subClassOfInverted rdf:resource="http://www.w3.org/2006/time#TRS"/>
        <www:subClassOfInverted rdf:resource="http://www.w3.org/2006/time#TemporalDuration"/>
        <www:subClassOfInverted rdf:resource="http://www.w3.org/2006/time#TemporalPosition"/>
    </owl:Class>
    


    <!-- http://www.w3.org/2006/time#TemporalPosition -->

    <owl:Class rdf:about="http://www.w3.org/2006/time#TemporalPosition">
        <rdfs:subClassOf rdf:resource="http://www.w3.org/2006/time#TemporalEntity"/>
        <rdfs:subClassOf>
            <owl:Restriction>
                <owl:onProperty rdf:resource="http://www.w3.org/2006/time#hasTRS"/>
                <owl:cardinality rdf:datatype="http://www.w3.org/2001/XMLSchema#nonNegativeInteger">1</owl:cardinality>
            </owl:Restriction>
        </rdfs:subClassOf>
        <www:subClassOfInverted rdf:resource="http://www.w3.org/2006/time#GeneralDateTimeDescription"/>
        <www:subClassOfInverted rdf:resource="http://www.w3.org/2006/time#TimePosition"/>
        <rdfs:comment xml:lang="en">A position on a time-line</rdfs:comment>
        <rdfs:label xml:lang="en">Temporal position</rdfs:label>
        <skos:definition xml:lang="en">A position on a time-line</skos:definition>
    </owl:Class>
    


    <!-- http://www.w3.org/2006/time#TemporalUnit -->

    <owl:Class rdf:about="http://www.w3.org/2006/time#TemporalUnit">
        <owl:equivalentClass>
            <owl:Class>
                <owl:oneOf rdf:parseType="Collection">
                    <rdf:Description rdf:about="http://www.w3.org/2006/time#unitDay"/>
                    <rdf:Description rdf:about="http://www.w3.org/2006/time#unitHour"/>
                    <rdf:Description rdf:about="http://www.w3.org/2006/time#unitMinute"/>
                    <rdf:Description rdf:about="http://www.w3.org/2006/time#unitMonth"/>
                    <rdf:Description rdf:about="http://www.w3.org/2006/time#unitSecond"/>
                    <rdf:Description rdf:about="http://www.w3.org/2006/time#unitWeek"/>
                    <rdf:Description rdf:about="http://www.w3.org/2006/time#unitYear"/>
                </owl:oneOf>
            </owl:Class>
        </owl:equivalentClass>
    </owl:Class>
    


    <!-- http://www.w3.org/2006/time#TimePosition -->

    <owl:Class rdf:about="http://www.w3.org/2006/time#TimePosition">
        <rdfs:subClassOf rdf:resource="http://www.w3.org/2006/time#TemporalPosition"/>
        <rdfs:subClassOf>
            <owl:Class>
                <owl:unionOf rdf:parseType="Collection">
                    <owl:Restriction>
                        <owl:onProperty rdf:resource="http://www.w3.org/2006/time#nominalPosition"/>
                        <owl:cardinality rdf:datatype="http://www.w3.org/2001/XMLSchema#nonNegativeInteger">1</owl:cardinality>
                    </owl:Restriction>
                    <owl:Restriction>
                        <owl:onProperty rdf:resource="http://www.w3.org/2006/time#numericPosition"/>
                        <owl:cardinality rdf:datatype="http://www.w3.org/2001/XMLSchema#nonNegativeInteger">1</owl:cardinality>
                    </owl:Restriction>
                </owl:unionOf>
            </owl:Class>
        </rdfs:subClassOf>
    </owl:Class>
    


    <!-- http://www.w3.org/2006/time#TimeZone -->

    <owl:Class rdf:about="http://www.w3.org/2006/time#TimeZone">
        <owl:equivalentClass rdf:resource="http://www.w3.org/2006/timezone#TimeZone"/>
        <rdfs:subClassOf rdf:resource="http://www.w3.org/2006/time#TRS"/>
        <rdfs:comment xml:lang="en">A Time Zone specifies the amount by which the local time is offset from UTC. 
	A time zone is usually denoted geographically (e.g. Australian Eastern Daylight Time), with a constant value in a given region. 
The region where it applies and the offset from UTC are specified by a locally recognised governing authority.</rdfs:comment>
        <rdfs:label xml:lang="en">Time Zone</rdfs:label>
        <skos:definition xml:lang="en">A Time Zone specifies the amount by which the local time is offset from UTC. 
	A time zone is usually denoted geographically (e.g. Australian Eastern Daylight Time), with a constant value in a given region. 
The region where it applies and the offset from UTC are specified by a locally recognised governing authority.</skos:definition>
        <skos:historyNote>In the original 2006 version of OWL-Time, the TimeZone class, with several properties corresponding to a specific model of time-zones, was defined in a separate namespace &quot;http://www.w3.org/2006/timezone#&quot;. 

In the current version a class with same local name is put into the main OWL-Time namespace, removing the dependency on the external namespace. 

An alignment axiom 
	tzont:TimeZone rdfs:subClassOf time:TimeZone . 
allows data encoded according to the previous version to be consistent with the updated ontology. </skos:historyNote>
        <skos:note xml:lang="en">A designated timezone is associated with a geographic region. However, for a particular region the offset from UTC often varies seasonally, and the dates of the changes may vary from year to year. The timezone designation usually changes for the different seasons (e.g. Australian Eastern Standard Time vs. Australian Eastern Daylight Time). Furthermore, the offset for a timezone may change over longer timescales, though its designation might not.  

Detailed guidance about working with time zones is given in http://www.w3.org/TR/timezone/ .</skos:note>
        <skos:note xml:lang="en">An ontology for time zone descriptions was described in [owl-time-20060927] and provided as RDF in a separate namespace tzont:. However, that ontology was incomplete in scope, and the example datasets were selective. Furthermore, since the use of a class from an external ontology as the range of an ObjectProperty in OWL-Time creates a dependency, reference to the time zone class has been replaced with the &apos;stub&apos; class in the normative part of this version of OWL-Time.</skos:note>
        <skos:scopeNote>In this implementation TimeZone has no properties defined. It should be thought of as an &apos;abstract&apos; superclass of all specific timezone implementations.</skos:scopeNote>
    </owl:Class>
    


    <!-- http://www.w3.org/2006/time#Year -->

    <owl:Class rdf:about="http://www.w3.org/2006/time#Year">
        <rdfs:subClassOf rdf:resource="http://www.w3.org/2006/time#DurationDescription"/>
        <rdfs:subClassOf>
            <owl:Restriction>
                <owl:onProperty rdf:resource="http://www.w3.org/2006/time#days"/>
                <owl:cardinality rdf:datatype="http://www.w3.org/2001/XMLSchema#nonNegativeInteger">0</owl:cardinality>
            </owl:Restriction>
        </rdfs:subClassOf>
        <rdfs:subClassOf>
            <owl:Restriction>
                <owl:onProperty rdf:resource="http://www.w3.org/2006/time#hours"/>
                <owl:cardinality rdf:datatype="http://www.w3.org/2001/XMLSchema#nonNegativeInteger">0</owl:cardinality>
            </owl:Restriction>
        </rdfs:subClassOf>
        <rdfs:subClassOf>
            <owl:Restriction>
                <owl:onProperty rdf:resource="http://www.w3.org/2006/time#minutes"/>
                <owl:cardinality rdf:datatype="http://www.w3.org/2001/XMLSchema#nonNegativeInteger">0</owl:cardinality>
            </owl:Restriction>
        </rdfs:subClassOf>
        <rdfs:subClassOf>
            <owl:Restriction>
                <owl:onProperty rdf:resource="http://www.w3.org/2006/time#months"/>
                <owl:cardinality rdf:datatype="http://www.w3.org/2001/XMLSchema#nonNegativeInteger">0</owl:cardinality>
            </owl:Restriction>
        </rdfs:subClassOf>
        <rdfs:subClassOf>
            <owl:Restriction>
                <owl:onProperty rdf:resource="http://www.w3.org/2006/time#seconds"/>
                <owl:cardinality rdf:datatype="http://www.w3.org/2001/XMLSchema#nonNegativeInteger">0</owl:cardinality>
            </owl:Restriction>
        </rdfs:subClassOf>
        <rdfs:subClassOf>
            <owl:Restriction>
                <owl:onProperty rdf:resource="http://www.w3.org/2006/time#weeks"/>
                <owl:cardinality rdf:datatype="http://www.w3.org/2001/XMLSchema#nonNegativeInteger">0</owl:cardinality>
            </owl:Restriction>
        </rdfs:subClassOf>
        <rdfs:subClassOf>
            <owl:Restriction>
                <owl:onProperty rdf:resource="http://www.w3.org/2006/time#years"/>
                <owl:cardinality rdf:datatype="http://www.w3.org/2001/XMLSchema#nonNegativeInteger">1</owl:cardinality>
            </owl:Restriction>
        </rdfs:subClassOf>
        <rdfs:comment>Year duration</rdfs:comment>
        <rdfs:label xml:lang="en">Year</rdfs:label>
        <owl:deprecated rdf:datatype="http://www.w3.org/2001/XMLSchema#boolean">true</owl:deprecated>
        <skos:definition>Year duration</skos:definition>
        <skos:historyNote>Year was proposed in the 2006 version of OWL-Time as an example of how DurationDescription could be specialized to allow for a duration to be restricted to a number of years. 

It is deprecated in this edition of OWL-Time. </skos:historyNote>
        <skos:prefLabel xml:lang="it">Anno</skos:prefLabel>
        <skos:prefLabel xml:lang="fr">Année (calendrier)</skos:prefLabel>
        <skos:prefLabel xml:lang="pt">Ano</skos:prefLabel>
        <skos:prefLabel xml:lang="es">Año</skos:prefLabel>
        <skos:prefLabel xml:lang="nl">Jaar</skos:prefLabel>
        <skos:prefLabel xml:lang="de">Jahr</skos:prefLabel>
        <skos:prefLabel xml:lang="pl">Rok</skos:prefLabel>
        <skos:prefLabel xml:lang="en">Year</skos:prefLabel>
        <skos:prefLabel xml:lang="ru">Год</skos:prefLabel>
        <skos:prefLabel xml:lang="ar">سنة</skos:prefLabel>
        <skos:prefLabel xml:lang="ja">年</skos:prefLabel>
        <skos:prefLabel xml:lang="zh">年</skos:prefLabel>
    </owl:Class>
    


    <!-- http://www.w3.org/2006/time#generalYear -->

    <owl:Class rdf:about="http://www.w3.org/2006/time#generalYear">
        <rdfs:subClassOf rdf:resource="http://www.w3.org/2000/01/rdf-schema#Resource"/>
    </owl:Class>
    


    <!-- http://www.w3.org/2006/timezone#TimeZone -->

    <owl:Class rdf:about="http://www.w3.org/2006/timezone#TimeZone">
        <rdfs:label>timezone:TimeZone</rdfs:label>
    </owl:Class>
    


    <!-- http://www.w3.org/2006/vcard/ns#Acquaintance -->

    <owl:Class rdf:about="http://www.w3.org/2006/vcard/ns#Acquaintance">
        <rdfs:subClassOf rdf:resource="http://www.w3.org/2006/vcard/ns#RelatedType"/>
        <rdfs:isDefinedBy rdf:resource="http://www.w3.org/2006/vcard/ns"/>
        <rdfs:label xml:lang="en">Acquaintance</rdfs:label>
    </owl:Class>
    


    <!-- http://www.w3.org/2006/vcard/ns#Address -->

    <owl:Class rdf:about="http://www.w3.org/2006/vcard/ns#Address">
        <owl:equivalentClass>
            <owl:Class>
                <owl:unionOf rdf:parseType="Collection">
                    <owl:Class>
                        <owl:intersectionOf rdf:parseType="Collection">
                            <owl:Restriction>
                                <owl:onProperty rdf:resource="http://www.w3.org/2006/vcard/ns#country-name"/>
                                <owl:someValuesFrom rdf:resource="http://www.w3.org/2001/XMLSchema#string"/>
                            </owl:Restriction>
                            <owl:Restriction>
                                <owl:onProperty rdf:resource="http://www.w3.org/2006/vcard/ns#country-name"/>
                                <owl:maxCardinality rdf:datatype="http://www.w3.org/2001/XMLSchema#nonNegativeInteger">1</owl:maxCardinality>
                            </owl:Restriction>
                        </owl:intersectionOf>
                    </owl:Class>
                    <owl:Class>
                        <owl:intersectionOf rdf:parseType="Collection">
                            <owl:Restriction>
                                <owl:onProperty rdf:resource="http://www.w3.org/2006/vcard/ns#locality"/>
                                <owl:someValuesFrom rdf:resource="http://www.w3.org/2001/XMLSchema#string"/>
                            </owl:Restriction>
                            <owl:Restriction>
                                <owl:onProperty rdf:resource="http://www.w3.org/2006/vcard/ns#locality"/>
                                <owl:maxCardinality rdf:datatype="http://www.w3.org/2001/XMLSchema#nonNegativeInteger">1</owl:maxCardinality>
                            </owl:Restriction>
                        </owl:intersectionOf>
                    </owl:Class>
                    <owl:Class>
                        <owl:intersectionOf rdf:parseType="Collection">
                            <owl:Restriction>
                                <owl:onProperty rdf:resource="http://www.w3.org/2006/vcard/ns#postal-code"/>
                                <owl:someValuesFrom rdf:resource="http://www.w3.org/2001/XMLSchema#string"/>
                            </owl:Restriction>
                            <owl:Restriction>
                                <owl:onProperty rdf:resource="http://www.w3.org/2006/vcard/ns#postal-code"/>
                                <owl:maxCardinality rdf:datatype="http://www.w3.org/2001/XMLSchema#nonNegativeInteger">1</owl:maxCardinality>
                            </owl:Restriction>
                        </owl:intersectionOf>
                    </owl:Class>
                    <owl:Class>
                        <owl:intersectionOf rdf:parseType="Collection">
                            <owl:Restriction>
                                <owl:onProperty rdf:resource="http://www.w3.org/2006/vcard/ns#region"/>
                                <owl:someValuesFrom rdf:resource="http://www.w3.org/2001/XMLSchema#string"/>
                            </owl:Restriction>
                            <owl:Restriction>
                                <owl:onProperty rdf:resource="http://www.w3.org/2006/vcard/ns#region"/>
                                <owl:maxCardinality rdf:datatype="http://www.w3.org/2001/XMLSchema#nonNegativeInteger">1</owl:maxCardinality>
                            </owl:Restriction>
                        </owl:intersectionOf>
                    </owl:Class>
                    <owl:Class>
                        <owl:intersectionOf rdf:parseType="Collection">
                            <owl:Restriction>
                                <owl:onProperty rdf:resource="http://www.w3.org/2006/vcard/ns#street-address"/>
                                <owl:someValuesFrom rdf:resource="http://www.w3.org/2001/XMLSchema#string"/>
                            </owl:Restriction>
                            <owl:Restriction>
                                <owl:onProperty rdf:resource="http://www.w3.org/2006/vcard/ns#street-address"/>
                                <owl:maxCardinality rdf:datatype="http://www.w3.org/2001/XMLSchema#nonNegativeInteger">1</owl:maxCardinality>
                            </owl:Restriction>
                        </owl:intersectionOf>
                    </owl:Class>
                </owl:unionOf>
            </owl:Class>
        </owl:equivalentClass>
    </owl:Class>
    


    <!-- http://www.w3.org/2006/vcard/ns#Agent -->

    <owl:Class rdf:about="http://www.w3.org/2006/vcard/ns#Agent">
        <rdfs:subClassOf rdf:resource="http://www.w3.org/2006/vcard/ns#RelatedType"/>
        <rdfs:isDefinedBy rdf:resource="http://www.w3.org/2006/vcard/ns"/>
        <rdfs:label xml:lang="en">Agent</rdfs:label>
    </owl:Class>
    


    <!-- http://www.w3.org/2006/vcard/ns#BBS -->

    <owl:Class rdf:about="http://www.w3.org/2006/vcard/ns#BBS">
        <rdfs:subClassOf rdf:resource="http://www.w3.org/2006/vcard/ns#TelephoneType"/>
        <rdfs:comment xml:lang="en">This class is deprecated</rdfs:comment>
        <rdfs:isDefinedBy rdf:resource="http://www.w3.org/2006/vcard/ns"/>
        <rdfs:label xml:lang="en">BBS</rdfs:label>
        <owl:deprecated rdf:datatype="http://www.w3.org/2001/XMLSchema#boolean">true</owl:deprecated>
    </owl:Class>
    


    <!-- http://www.w3.org/2006/vcard/ns#Car -->

    <owl:Class rdf:about="http://www.w3.org/2006/vcard/ns#Car">
        <rdfs:subClassOf rdf:resource="http://www.w3.org/2006/vcard/ns#TelephoneType"/>
        <rdfs:comment xml:lang="en">This class is deprecated</rdfs:comment>
        <rdfs:isDefinedBy rdf:resource="http://www.w3.org/2006/vcard/ns"/>
        <rdfs:label xml:lang="en">Car</rdfs:label>
        <owl:deprecated rdf:datatype="http://www.w3.org/2001/XMLSchema#boolean">true</owl:deprecated>
    </owl:Class>
    


    <!-- http://www.w3.org/2006/vcard/ns#Cell -->

    <owl:Class rdf:about="http://www.w3.org/2006/vcard/ns#Cell">
        <rdfs:subClassOf rdf:resource="http://www.w3.org/2006/vcard/ns#TelephoneType"/>
        <rdfs:comment xml:lang="en">Also called mobile telephone</rdfs:comment>
        <rdfs:isDefinedBy rdf:resource="http://www.w3.org/2006/vcard/ns"/>
        <rdfs:label xml:lang="en">Cell</rdfs:label>
    </owl:Class>
    


    <!-- http://www.w3.org/2006/vcard/ns#Child -->

    <owl:Class rdf:about="http://www.w3.org/2006/vcard/ns#Child">
        <rdfs:subClassOf rdf:resource="http://www.w3.org/2006/vcard/ns#RelatedType"/>
        <rdfs:isDefinedBy rdf:resource="http://www.w3.org/2006/vcard/ns"/>
        <rdfs:label xml:lang="en">Child</rdfs:label>
    </owl:Class>
    


    <!-- http://www.w3.org/2006/vcard/ns#Colleague -->

    <owl:Class rdf:about="http://www.w3.org/2006/vcard/ns#Colleague">
        <rdfs:subClassOf rdf:resource="http://www.w3.org/2006/vcard/ns#RelatedType"/>
        <rdfs:isDefinedBy rdf:resource="http://www.w3.org/2006/vcard/ns"/>
        <rdfs:label xml:lang="en">Colleague</rdfs:label>
    </owl:Class>
    


    <!-- http://www.w3.org/2006/vcard/ns#Contact -->

    <owl:Class rdf:about="http://www.w3.org/2006/vcard/ns#Contact">
        <rdfs:subClassOf rdf:resource="http://www.w3.org/2006/vcard/ns#RelatedType"/>
        <rdfs:isDefinedBy rdf:resource="http://www.w3.org/2006/vcard/ns"/>
        <rdfs:label xml:lang="en">Contact</rdfs:label>
    </owl:Class>
    


    <!-- http://www.w3.org/2006/vcard/ns#Coresident -->

    <owl:Class rdf:about="http://www.w3.org/2006/vcard/ns#Coresident">
        <rdfs:subClassOf rdf:resource="http://www.w3.org/2006/vcard/ns#RelatedType"/>
        <rdfs:isDefinedBy rdf:resource="http://www.w3.org/2006/vcard/ns"/>
        <rdfs:label xml:lang="en">Coresident</rdfs:label>
    </owl:Class>
    


    <!-- http://www.w3.org/2006/vcard/ns#Coworker -->

    <owl:Class rdf:about="http://www.w3.org/2006/vcard/ns#Coworker">
        <rdfs:subClassOf rdf:resource="http://www.w3.org/2006/vcard/ns#RelatedType"/>
        <rdfs:isDefinedBy rdf:resource="http://www.w3.org/2006/vcard/ns"/>
        <rdfs:label xml:lang="en">Coworker</rdfs:label>
    </owl:Class>
    


    <!-- http://www.w3.org/2006/vcard/ns#Crush -->

    <owl:Class rdf:about="http://www.w3.org/2006/vcard/ns#Crush">
        <rdfs:subClassOf rdf:resource="http://www.w3.org/2006/vcard/ns#RelatedType"/>
        <rdfs:isDefinedBy rdf:resource="http://www.w3.org/2006/vcard/ns"/>
        <rdfs:label xml:lang="en">Crush</rdfs:label>
    </owl:Class>
    


    <!-- http://www.w3.org/2006/vcard/ns#Date -->

    <owl:Class rdf:about="http://www.w3.org/2006/vcard/ns#Date">
        <rdfs:subClassOf rdf:resource="http://www.w3.org/2006/vcard/ns#RelatedType"/>
        <rdfs:isDefinedBy rdf:resource="http://www.w3.org/2006/vcard/ns"/>
        <rdfs:label xml:lang="en">Date</rdfs:label>
    </owl:Class>
    


    <!-- http://www.w3.org/2006/vcard/ns#Dom -->

    <owl:Class rdf:about="http://www.w3.org/2006/vcard/ns#Dom">
        <rdfs:subClassOf rdf:resource="http://www.w3.org/2006/vcard/ns#Type"/>
        <rdfs:comment xml:lang="en">This class is deprecated</rdfs:comment>
        <rdfs:isDefinedBy rdf:resource="http://www.w3.org/2006/vcard/ns"/>
        <rdfs:label xml:lang="en">Dom</rdfs:label>
        <owl:deprecated rdf:datatype="http://www.w3.org/2001/XMLSchema#boolean">true</owl:deprecated>
    </owl:Class>
    


    <!-- http://www.w3.org/2006/vcard/ns#Email -->

    <owl:Class rdf:about="http://www.w3.org/2006/vcard/ns#Email">
        <rdfs:comment xml:lang="en">To specify the electronic mail address for communication with the object the vCard represents. Use the hasEmail object property.</rdfs:comment>
        <rdfs:isDefinedBy rdf:resource="http://www.w3.org/2006/vcard/ns"/>
        <rdfs:label xml:lang="en">Email</rdfs:label>
        <owl:deprecated rdf:datatype="http://www.w3.org/2001/XMLSchema#boolean">true</owl:deprecated>
    </owl:Class>
    


    <!-- http://www.w3.org/2006/vcard/ns#Emergency -->

    <owl:Class rdf:about="http://www.w3.org/2006/vcard/ns#Emergency">
        <rdfs:subClassOf rdf:resource="http://www.w3.org/2006/vcard/ns#RelatedType"/>
        <rdfs:isDefinedBy rdf:resource="http://www.w3.org/2006/vcard/ns"/>
        <rdfs:label xml:lang="en">Emergency</rdfs:label>
    </owl:Class>
    


    <!-- http://www.w3.org/2006/vcard/ns#Fax -->

    <owl:Class rdf:about="http://www.w3.org/2006/vcard/ns#Fax">
        <rdfs:subClassOf rdf:resource="http://www.w3.org/2006/vcard/ns#TelephoneType"/>
        <rdfs:isDefinedBy rdf:resource="http://www.w3.org/2006/vcard/ns"/>
        <rdfs:label xml:lang="en">Fax</rdfs:label>
    </owl:Class>
    


    <!-- http://www.w3.org/2006/vcard/ns#Female -->

    <owl:Class rdf:about="http://www.w3.org/2006/vcard/ns#Female">
        <rdfs:subClassOf rdf:resource="http://www.w3.org/2006/vcard/ns#Gender"/>
        <rdfs:isDefinedBy rdf:resource="http://www.w3.org/2006/vcard/ns"/>
        <rdfs:label xml:lang="en">Female</rdfs:label>
    </owl:Class>
    


    <!-- http://www.w3.org/2006/vcard/ns#Friend -->

    <owl:Class rdf:about="http://www.w3.org/2006/vcard/ns#Friend">
        <rdfs:subClassOf rdf:resource="http://www.w3.org/2006/vcard/ns#RelatedType"/>
        <rdfs:isDefinedBy rdf:resource="http://www.w3.org/2006/vcard/ns"/>
        <rdfs:label xml:lang="en">Friend</rdfs:label>
    </owl:Class>
    


    <!-- http://www.w3.org/2006/vcard/ns#Gender -->

    <owl:Class rdf:about="http://www.w3.org/2006/vcard/ns#Gender">
        <www:subClassOfInverted rdf:resource="http://www.w3.org/2006/vcard/ns#Female"/>
        <www:subClassOfInverted rdf:resource="http://www.w3.org/2006/vcard/ns#Male"/>
        <www:subClassOfInverted rdf:resource="http://www.w3.org/2006/vcard/ns#None"/>
        <www:subClassOfInverted rdf:resource="http://www.w3.org/2006/vcard/ns#Other"/>
        <www:subClassOfInverted rdf:resource="http://www.w3.org/2006/vcard/ns#Unknown"/>
        <rdfs:comment xml:lang="en">Used for gender codes. The URI of the gender code must be used as the value for Gender.</rdfs:comment>
        <rdfs:isDefinedBy rdf:resource="http://www.w3.org/2006/vcard/ns"/>
        <rdfs:label xml:lang="en">Gender</rdfs:label>
    </owl:Class>
    


    <!-- http://www.w3.org/2006/vcard/ns#Group -->

    <owl:Class rdf:about="http://www.w3.org/2006/vcard/ns#Group">
        <owl:equivalentClass>
            <owl:Class>
                <owl:intersectionOf rdf:parseType="Collection">
                    <owl:Restriction>
                        <owl:onProperty rdf:resource="http://www.w3.org/2006/vcard/ns#hasMember"/>
                        <owl:someValuesFrom rdf:resource="http://www.w3.org/2006/vcard/ns#Kind"/>
                    </owl:Restriction>
                    <owl:Restriction>
                        <owl:onProperty rdf:resource="http://www.w3.org/2006/vcard/ns#hasMember"/>
                        <owl:minQualifiedCardinality rdf:datatype="http://www.w3.org/2001/XMLSchema#nonNegativeInteger">1</owl:minQualifiedCardinality>
                        <owl:onClass rdf:resource="http://www.w3.org/2006/vcard/ns#Kind"/>
                    </owl:Restriction>
                </owl:intersectionOf>
            </owl:Class>
        </owl:equivalentClass>
    </owl:Class>
    


    <!-- http://www.w3.org/2006/vcard/ns#Home -->

    <owl:Class rdf:about="http://www.w3.org/2006/vcard/ns#Home">
        <rdfs:subClassOf rdf:resource="http://www.w3.org/2006/vcard/ns#Type"/>
        <rdfs:comment xml:lang="en">This implies that the property is related to an individual&apos;s personal life</rdfs:comment>
        <rdfs:isDefinedBy rdf:resource="http://www.w3.org/2006/vcard/ns"/>
        <rdfs:label xml:lang="en">Home</rdfs:label>
    </owl:Class>
    


    <!-- http://www.w3.org/2006/vcard/ns#ISDN -->

    <owl:Class rdf:about="http://www.w3.org/2006/vcard/ns#ISDN">
        <rdfs:subClassOf rdf:resource="http://www.w3.org/2006/vcard/ns#Type"/>
        <rdfs:comment xml:lang="en">This class is deprecated</rdfs:comment>
        <rdfs:isDefinedBy rdf:resource="http://www.w3.org/2006/vcard/ns"/>
        <rdfs:label xml:lang="en">ISDN</rdfs:label>
        <owl:deprecated rdf:datatype="http://www.w3.org/2001/XMLSchema#boolean">true</owl:deprecated>
    </owl:Class>
    


    <!-- http://www.w3.org/2006/vcard/ns#Individual -->

    <owl:Class rdf:about="http://www.w3.org/2006/vcard/ns#Individual">
        <rdfs:subClassOf rdf:resource="http://www.w3.org/2006/vcard/ns#Kind"/>
        <owl:disjointWith rdf:resource="http://www.w3.org/2006/vcard/ns#Location"/>
        <owl:disjointWith rdf:resource="http://www.w3.org/2006/vcard/ns#Organization"/>
        <owl:disjointWith>
            <owl:Class>
                <owl:intersectionOf rdf:parseType="Collection">
                    <owl:Restriction>
                        <owl:onProperty rdf:resource="http://www.w3.org/2006/vcard/ns#hasMember"/>
                        <owl:someValuesFrom rdf:resource="http://www.w3.org/2006/vcard/ns#Kind"/>
                    </owl:Restriction>
                    <owl:Restriction>
                        <owl:onProperty rdf:resource="http://www.w3.org/2006/vcard/ns#hasMember"/>
                        <owl:minQualifiedCardinality rdf:datatype="http://www.w3.org/2001/XMLSchema#nonNegativeInteger">1</owl:minQualifiedCardinality>
                        <owl:onClass rdf:resource="http://www.w3.org/2006/vcard/ns#Kind"/>
                    </owl:Restriction>
                </owl:intersectionOf>
            </owl:Class>
        </owl:disjointWith>
        <rdfs:comment xml:lang="en">An object representing a single person or entity</rdfs:comment>
        <rdfs:isDefinedBy rdf:resource="http://www.w3.org/2006/vcard/ns"/>
        <rdfs:label xml:lang="en">Individual</rdfs:label>
    </owl:Class>
    


    <!-- http://www.w3.org/2006/vcard/ns#Internet -->

    <owl:Class rdf:about="http://www.w3.org/2006/vcard/ns#Internet">
        <rdfs:subClassOf rdf:resource="http://www.w3.org/2006/vcard/ns#Type"/>
        <rdfs:comment xml:lang="en">This class is deprecated</rdfs:comment>
        <rdfs:isDefinedBy rdf:resource="http://www.w3.org/2006/vcard/ns"/>
        <rdfs:label xml:lang="en">Internet</rdfs:label>
        <owl:deprecated rdf:datatype="http://www.w3.org/2001/XMLSchema#boolean">true</owl:deprecated>
    </owl:Class>
    


    <!-- http://www.w3.org/2006/vcard/ns#Intl -->

    <owl:Class rdf:about="http://www.w3.org/2006/vcard/ns#Intl">
        <rdfs:subClassOf rdf:resource="http://www.w3.org/2006/vcard/ns#Type"/>
        <rdfs:comment xml:lang="en">This class is deprecated</rdfs:comment>
        <rdfs:isDefinedBy rdf:resource="http://www.w3.org/2006/vcard/ns"/>
        <rdfs:label xml:lang="en">Intl</rdfs:label>
        <owl:deprecated rdf:datatype="http://www.w3.org/2001/XMLSchema#boolean">true</owl:deprecated>
    </owl:Class>
    


    <!-- http://www.w3.org/2006/vcard/ns#Kin -->

    <owl:Class rdf:about="http://www.w3.org/2006/vcard/ns#Kin">
        <rdfs:subClassOf rdf:resource="http://www.w3.org/2006/vcard/ns#RelatedType"/>
        <rdfs:isDefinedBy rdf:resource="http://www.w3.org/2006/vcard/ns"/>
        <rdfs:label xml:lang="en">Kin</rdfs:label>
    </owl:Class>
    


    <!-- http://www.w3.org/2006/vcard/ns#Kind -->

    <owl:Class rdf:about="http://www.w3.org/2006/vcard/ns#Kind">
        <owl:equivalentClass rdf:resource="http://www.w3.org/2006/vcard/ns#VCard"/>
        <owl:equivalentClass>
            <owl:Restriction>
                <owl:onProperty rdf:resource="http://www.w3.org/2006/vcard/ns#fn"/>
                <owl:minQualifiedCardinality rdf:datatype="http://www.w3.org/2001/XMLSchema#nonNegativeInteger">1</owl:minQualifiedCardinality>
                <owl:onDataRange rdf:resource="http://www.w3.org/2001/XMLSchema#string"/>
            </owl:Restriction>
        </owl:equivalentClass>
        <www:subClassOfInverted rdf:resource="http://www.w3.org/2006/vcard/ns#Individual"/>
        <www:subClassOfInverted rdf:resource="http://www.w3.org/2006/vcard/ns#Location"/>
        <www:subClassOfInverted rdf:resource="http://www.w3.org/2006/vcard/ns#Organization"/>
        <www:subClassOfInverted>
            <rdf:Description>
                <rdfs:comment xml:lang="en">Object representing a group of persons or entities.  A group object will usually contain hasMember properties to specify the members of the group.</rdfs:comment>
                <rdfs:isDefinedBy rdf:resource="http://www.w3.org/2006/vcard/ns"/>
                <rdfs:label xml:lang="en">Group</rdfs:label>
            </rdf:Description>
        </www:subClassOfInverted>
        <rdfs:comment xml:lang="en">The parent class for all objects</rdfs:comment>
        <rdfs:isDefinedBy rdf:resource="http://www.w3.org/2006/vcard/ns"/>
        <rdfs:label xml:lang="en">Kind</rdfs:label>
    </owl:Class>
    


    <!-- http://www.w3.org/2006/vcard/ns#Label -->

    <owl:Class rdf:about="http://www.w3.org/2006/vcard/ns#Label">
        <rdfs:subClassOf rdf:resource="http://www.w3.org/2006/vcard/ns#Type"/>
        <rdfs:comment xml:lang="en">This class is deprecated</rdfs:comment>
        <rdfs:isDefinedBy rdf:resource="http://www.w3.org/2006/vcard/ns"/>
        <rdfs:label xml:lang="en">Label</rdfs:label>
        <owl:deprecated rdf:datatype="http://www.w3.org/2001/XMLSchema#boolean">true</owl:deprecated>
    </owl:Class>
    


    <!-- http://www.w3.org/2006/vcard/ns#Location -->

    <owl:Class rdf:about="http://www.w3.org/2006/vcard/ns#Location">
        <rdfs:subClassOf rdf:resource="http://www.w3.org/2006/vcard/ns#Kind"/>
        <owl:disjointWith rdf:resource="http://www.w3.org/2006/vcard/ns#Organization"/>
        <owl:disjointWith>
            <owl:Class>
                <owl:intersectionOf rdf:parseType="Collection">
                    <owl:Restriction>
                        <owl:onProperty rdf:resource="http://www.w3.org/2006/vcard/ns#hasMember"/>
                        <owl:someValuesFrom rdf:resource="http://www.w3.org/2006/vcard/ns#Kind"/>
                    </owl:Restriction>
                    <owl:Restriction>
                        <owl:onProperty rdf:resource="http://www.w3.org/2006/vcard/ns#hasMember"/>
                        <owl:minQualifiedCardinality rdf:datatype="http://www.w3.org/2001/XMLSchema#nonNegativeInteger">1</owl:minQualifiedCardinality>
                        <owl:onClass rdf:resource="http://www.w3.org/2006/vcard/ns#Kind"/>
                    </owl:Restriction>
                </owl:intersectionOf>
            </owl:Class>
        </owl:disjointWith>
        <rdfs:comment xml:lang="en">An object representing a named geographical place</rdfs:comment>
        <rdfs:isDefinedBy rdf:resource="http://www.w3.org/2006/vcard/ns"/>
        <rdfs:label xml:lang="en">Location</rdfs:label>
    </owl:Class>
    


    <!-- http://www.w3.org/2006/vcard/ns#Male -->

    <owl:Class rdf:about="http://www.w3.org/2006/vcard/ns#Male">
        <rdfs:subClassOf rdf:resource="http://www.w3.org/2006/vcard/ns#Gender"/>
        <rdfs:isDefinedBy rdf:resource="http://www.w3.org/2006/vcard/ns"/>
        <rdfs:label xml:lang="en">Male</rdfs:label>
    </owl:Class>
    


    <!-- http://www.w3.org/2006/vcard/ns#Me -->

    <owl:Class rdf:about="http://www.w3.org/2006/vcard/ns#Me">
        <rdfs:subClassOf rdf:resource="http://www.w3.org/2006/vcard/ns#RelatedType"/>
        <rdfs:isDefinedBy rdf:resource="http://www.w3.org/2006/vcard/ns"/>
        <rdfs:label xml:lang="en">Me</rdfs:label>
    </owl:Class>
    


    <!-- http://www.w3.org/2006/vcard/ns#Met -->

    <owl:Class rdf:about="http://www.w3.org/2006/vcard/ns#Met">
        <rdfs:subClassOf rdf:resource="http://www.w3.org/2006/vcard/ns#RelatedType"/>
        <rdfs:isDefinedBy rdf:resource="http://www.w3.org/2006/vcard/ns"/>
        <rdfs:label xml:lang="en">Met</rdfs:label>
    </owl:Class>
    


    <!-- http://www.w3.org/2006/vcard/ns#Modem -->

    <owl:Class rdf:about="http://www.w3.org/2006/vcard/ns#Modem">
        <rdfs:subClassOf rdf:resource="http://www.w3.org/2006/vcard/ns#TelephoneType"/>
        <rdfs:comment xml:lang="en">This class is deprecated</rdfs:comment>
        <rdfs:isDefinedBy rdf:resource="http://www.w3.org/2006/vcard/ns"/>
        <rdfs:label xml:lang="en">Modem</rdfs:label>
        <owl:deprecated rdf:datatype="http://www.w3.org/2001/XMLSchema#boolean">true</owl:deprecated>
    </owl:Class>
    


    <!-- http://www.w3.org/2006/vcard/ns#Msg -->

    <owl:Class rdf:about="http://www.w3.org/2006/vcard/ns#Msg">
        <rdfs:subClassOf rdf:resource="http://www.w3.org/2006/vcard/ns#TelephoneType"/>
        <rdfs:comment xml:lang="en">This class is deprecated</rdfs:comment>
        <rdfs:isDefinedBy rdf:resource="http://www.w3.org/2006/vcard/ns"/>
        <rdfs:label xml:lang="en">Msg</rdfs:label>
        <owl:deprecated rdf:datatype="http://www.w3.org/2001/XMLSchema#boolean">true</owl:deprecated>
    </owl:Class>
    


    <!-- http://www.w3.org/2006/vcard/ns#Muse -->

    <owl:Class rdf:about="http://www.w3.org/2006/vcard/ns#Muse">
        <rdfs:subClassOf rdf:resource="http://www.w3.org/2006/vcard/ns#RelatedType"/>
        <rdfs:isDefinedBy rdf:resource="http://www.w3.org/2006/vcard/ns"/>
        <rdfs:label xml:lang="en">Muse</rdfs:label>
    </owl:Class>
    


    <!-- http://www.w3.org/2006/vcard/ns#Name -->

    <owl:Class rdf:about="http://www.w3.org/2006/vcard/ns#Name">
        <owl:equivalentClass>
            <owl:Class>
                <owl:unionOf rdf:parseType="Collection">
                    <owl:Class>
                        <owl:intersectionOf rdf:parseType="Collection">
                            <owl:Restriction>
                                <owl:onProperty rdf:resource="http://www.w3.org/2006/vcard/ns#additional-name"/>
                                <owl:someValuesFrom rdf:resource="http://www.w3.org/2001/XMLSchema#string"/>
                            </owl:Restriction>
                            <owl:Restriction>
                                <owl:onProperty rdf:resource="http://www.w3.org/2006/vcard/ns#additional-name"/>
                                <owl:minCardinality rdf:datatype="http://www.w3.org/2001/XMLSchema#nonNegativeInteger">0</owl:minCardinality>
                            </owl:Restriction>
                        </owl:intersectionOf>
                    </owl:Class>
                    <owl:Class>
                        <owl:intersectionOf rdf:parseType="Collection">
                            <owl:Restriction>
                                <owl:onProperty rdf:resource="http://www.w3.org/2006/vcard/ns#family-name"/>
                                <owl:someValuesFrom rdf:resource="http://www.w3.org/2001/XMLSchema#string"/>
                            </owl:Restriction>
                            <owl:Restriction>
                                <owl:onProperty rdf:resource="http://www.w3.org/2006/vcard/ns#family-name"/>
                                <owl:maxCardinality rdf:datatype="http://www.w3.org/2001/XMLSchema#nonNegativeInteger">1</owl:maxCardinality>
                            </owl:Restriction>
                        </owl:intersectionOf>
                    </owl:Class>
                    <owl:Class>
                        <owl:intersectionOf rdf:parseType="Collection">
                            <owl:Restriction>
                                <owl:onProperty rdf:resource="http://www.w3.org/2006/vcard/ns#given-name"/>
                                <owl:someValuesFrom rdf:resource="http://www.w3.org/2001/XMLSchema#string"/>
                            </owl:Restriction>
                            <owl:Restriction>
                                <owl:onProperty rdf:resource="http://www.w3.org/2006/vcard/ns#given-name"/>
                                <owl:maxCardinality rdf:datatype="http://www.w3.org/2001/XMLSchema#nonNegativeInteger">1</owl:maxCardinality>
                            </owl:Restriction>
                        </owl:intersectionOf>
                    </owl:Class>
                    <owl:Class>
                        <owl:intersectionOf rdf:parseType="Collection">
                            <owl:Restriction>
                                <owl:onProperty rdf:resource="http://www.w3.org/2006/vcard/ns#honorific-prefix"/>
                                <owl:someValuesFrom rdf:resource="http://www.w3.org/2001/XMLSchema#string"/>
                            </owl:Restriction>
                            <owl:Restriction>
                                <owl:onProperty rdf:resource="http://www.w3.org/2006/vcard/ns#honorific-prefix"/>
                                <owl:minCardinality rdf:datatype="http://www.w3.org/2001/XMLSchema#nonNegativeInteger">0</owl:minCardinality>
                            </owl:Restriction>
                        </owl:intersectionOf>
                    </owl:Class>
                    <owl:Class>
                        <owl:intersectionOf rdf:parseType="Collection">
                            <owl:Restriction>
                                <owl:onProperty rdf:resource="http://www.w3.org/2006/vcard/ns#honorific-suffix"/>
                                <owl:someValuesFrom rdf:resource="http://www.w3.org/2001/XMLSchema#string"/>
                            </owl:Restriction>
                            <owl:Restriction>
                                <owl:onProperty rdf:resource="http://www.w3.org/2006/vcard/ns#honorific-suffix"/>
                                <owl:minCardinality rdf:datatype="http://www.w3.org/2001/XMLSchema#nonNegativeInteger">0</owl:minCardinality>
                            </owl:Restriction>
                        </owl:intersectionOf>
                    </owl:Class>
                </owl:unionOf>
            </owl:Class>
        </owl:equivalentClass>
    </owl:Class>
    


    <!-- http://www.w3.org/2006/vcard/ns#Neighbor -->

    <owl:Class rdf:about="http://www.w3.org/2006/vcard/ns#Neighbor">
        <rdfs:subClassOf rdf:resource="http://www.w3.org/2006/vcard/ns#RelatedType"/>
        <rdfs:isDefinedBy rdf:resource="http://www.w3.org/2006/vcard/ns"/>
        <rdfs:label xml:lang="en">Neighbor</rdfs:label>
    </owl:Class>
    


    <!-- http://www.w3.org/2006/vcard/ns#None -->

    <owl:Class rdf:about="http://www.w3.org/2006/vcard/ns#None">
        <rdfs:subClassOf rdf:resource="http://www.w3.org/2006/vcard/ns#Gender"/>
        <rdfs:isDefinedBy rdf:resource="http://www.w3.org/2006/vcard/ns"/>
        <rdfs:label xml:lang="en">None</rdfs:label>
    </owl:Class>
    


    <!-- http://www.w3.org/2006/vcard/ns#Organization -->

    <owl:Class rdf:about="http://www.w3.org/2006/vcard/ns#Organization">
        <rdfs:subClassOf rdf:resource="http://www.w3.org/2006/vcard/ns#Kind"/>
        <owl:disjointWith>
            <owl:Class>
                <owl:intersectionOf rdf:parseType="Collection">
                    <owl:Restriction>
                        <owl:onProperty rdf:resource="http://www.w3.org/2006/vcard/ns#hasMember"/>
                        <owl:someValuesFrom rdf:resource="http://www.w3.org/2006/vcard/ns#Kind"/>
                    </owl:Restriction>
                    <owl:Restriction>
                        <owl:onProperty rdf:resource="http://www.w3.org/2006/vcard/ns#hasMember"/>
                        <owl:minQualifiedCardinality rdf:datatype="http://www.w3.org/2001/XMLSchema#nonNegativeInteger">1</owl:minQualifiedCardinality>
                        <owl:onClass rdf:resource="http://www.w3.org/2006/vcard/ns#Kind"/>
                    </owl:Restriction>
                </owl:intersectionOf>
            </owl:Class>
        </owl:disjointWith>
        <rdfs:comment xml:lang="en">An object representing an organization.  An organization is a single entity, and might represent a business or government, a department or division within a business or government, a club, an association, or the like.
</rdfs:comment>
        <rdfs:isDefinedBy rdf:resource="http://www.w3.org/2006/vcard/ns"/>
        <rdfs:label xml:lang="en">Organization</rdfs:label>
    </owl:Class>
    


    <!-- http://www.w3.org/2006/vcard/ns#Other -->

    <owl:Class rdf:about="http://www.w3.org/2006/vcard/ns#Other">
        <rdfs:subClassOf rdf:resource="http://www.w3.org/2006/vcard/ns#Gender"/>
        <rdfs:isDefinedBy rdf:resource="http://www.w3.org/2006/vcard/ns"/>
        <rdfs:label xml:lang="en">Other</rdfs:label>
    </owl:Class>
    


    <!-- http://www.w3.org/2006/vcard/ns#PCS -->

    <owl:Class rdf:about="http://www.w3.org/2006/vcard/ns#PCS">
        <rdfs:subClassOf rdf:resource="http://www.w3.org/2006/vcard/ns#TelephoneType"/>
        <rdfs:comment xml:lang="en">This class is deprecated</rdfs:comment>
        <rdfs:isDefinedBy rdf:resource="http://www.w3.org/2006/vcard/ns"/>
        <rdfs:label xml:lang="en">PCS</rdfs:label>
        <owl:deprecated rdf:datatype="http://www.w3.org/2001/XMLSchema#boolean">true</owl:deprecated>
    </owl:Class>
    


    <!-- http://www.w3.org/2006/vcard/ns#Pager -->

    <owl:Class rdf:about="http://www.w3.org/2006/vcard/ns#Pager">
        <rdfs:subClassOf rdf:resource="http://www.w3.org/2006/vcard/ns#TelephoneType"/>
        <rdfs:isDefinedBy rdf:resource="http://www.w3.org/2006/vcard/ns"/>
        <rdfs:label xml:lang="en">Pager</rdfs:label>
    </owl:Class>
    


    <!-- http://www.w3.org/2006/vcard/ns#Parcel -->

    <owl:Class rdf:about="http://www.w3.org/2006/vcard/ns#Parcel">
        <rdfs:subClassOf rdf:resource="http://www.w3.org/2006/vcard/ns#Type"/>
        <rdfs:comment xml:lang="en">This class is deprecated</rdfs:comment>
        <rdfs:isDefinedBy rdf:resource="http://www.w3.org/2006/vcard/ns"/>
        <rdfs:label xml:lang="en">Parcel</rdfs:label>
        <owl:deprecated rdf:datatype="http://www.w3.org/2001/XMLSchema#boolean">true</owl:deprecated>
    </owl:Class>
    


    <!-- http://www.w3.org/2006/vcard/ns#Parent -->

    <owl:Class rdf:about="http://www.w3.org/2006/vcard/ns#Parent">
        <rdfs:subClassOf rdf:resource="http://www.w3.org/2006/vcard/ns#RelatedType"/>
        <rdfs:isDefinedBy rdf:resource="http://www.w3.org/2006/vcard/ns"/>
        <rdfs:label xml:lang="en">Parent</rdfs:label>
    </owl:Class>
    


    <!-- http://www.w3.org/2006/vcard/ns#Postal -->

    <owl:Class rdf:about="http://www.w3.org/2006/vcard/ns#Postal">
        <rdfs:subClassOf rdf:resource="http://www.w3.org/2006/vcard/ns#Type"/>
        <rdfs:comment xml:lang="en">This class is deprecated</rdfs:comment>
        <rdfs:isDefinedBy rdf:resource="http://www.w3.org/2006/vcard/ns"/>
        <rdfs:label xml:lang="en">Postal</rdfs:label>
        <owl:deprecated rdf:datatype="http://www.w3.org/2001/XMLSchema#boolean">true</owl:deprecated>
    </owl:Class>
    


    <!-- http://www.w3.org/2006/vcard/ns#Pref -->

    <owl:Class rdf:about="http://www.w3.org/2006/vcard/ns#Pref">
        <rdfs:subClassOf rdf:resource="http://www.w3.org/2006/vcard/ns#Type"/>
        <rdfs:comment xml:lang="en">This class is deprecated</rdfs:comment>
        <rdfs:isDefinedBy rdf:resource="http://www.w3.org/2006/vcard/ns"/>
        <rdfs:label xml:lang="en">Pref</rdfs:label>
        <owl:deprecated rdf:datatype="http://www.w3.org/2001/XMLSchema#boolean">true</owl:deprecated>
    </owl:Class>
    


    <!-- http://www.w3.org/2006/vcard/ns#RelatedType -->

    <owl:Class rdf:about="http://www.w3.org/2006/vcard/ns#RelatedType">
        <www:subClassOfInverted rdf:resource="http://www.w3.org/2006/vcard/ns#Acquaintance"/>
        <www:subClassOfInverted rdf:resource="http://www.w3.org/2006/vcard/ns#Agent"/>
        <www:subClassOfInverted rdf:resource="http://www.w3.org/2006/vcard/ns#Child"/>
        <www:subClassOfInverted rdf:resource="http://www.w3.org/2006/vcard/ns#Colleague"/>
        <www:subClassOfInverted rdf:resource="http://www.w3.org/2006/vcard/ns#Contact"/>
        <www:subClassOfInverted rdf:resource="http://www.w3.org/2006/vcard/ns#Coresident"/>
        <www:subClassOfInverted rdf:resource="http://www.w3.org/2006/vcard/ns#Coworker"/>
        <www:subClassOfInverted rdf:resource="http://www.w3.org/2006/vcard/ns#Crush"/>
        <www:subClassOfInverted rdf:resource="http://www.w3.org/2006/vcard/ns#Date"/>
        <www:subClassOfInverted rdf:resource="http://www.w3.org/2006/vcard/ns#Emergency"/>
        <www:subClassOfInverted rdf:resource="http://www.w3.org/2006/vcard/ns#Friend"/>
        <www:subClassOfInverted rdf:resource="http://www.w3.org/2006/vcard/ns#Kin"/>
        <www:subClassOfInverted rdf:resource="http://www.w3.org/2006/vcard/ns#Me"/>
        <www:subClassOfInverted rdf:resource="http://www.w3.org/2006/vcard/ns#Met"/>
        <www:subClassOfInverted rdf:resource="http://www.w3.org/2006/vcard/ns#Muse"/>
        <www:subClassOfInverted rdf:resource="http://www.w3.org/2006/vcard/ns#Neighbor"/>
        <www:subClassOfInverted rdf:resource="http://www.w3.org/2006/vcard/ns#Parent"/>
        <www:subClassOfInverted rdf:resource="http://www.w3.org/2006/vcard/ns#Sibling"/>
        <www:subClassOfInverted rdf:resource="http://www.w3.org/2006/vcard/ns#Spouse"/>
        <www:subClassOfInverted rdf:resource="http://www.w3.org/2006/vcard/ns#Sweetheart"/>
        <rdfs:comment xml:lang="en">Used for relation type codes. The URI of the relation type code must be used as the value for the Relation Type.</rdfs:comment>
        <rdfs:isDefinedBy rdf:resource="http://www.w3.org/2006/vcard/ns"/>
        <rdfs:label xml:lang="en">Relation Type</rdfs:label>
    </owl:Class>
    


    <!-- http://www.w3.org/2006/vcard/ns#Sibling -->

    <owl:Class rdf:about="http://www.w3.org/2006/vcard/ns#Sibling">
        <rdfs:subClassOf rdf:resource="http://www.w3.org/2006/vcard/ns#RelatedType"/>
        <rdfs:isDefinedBy rdf:resource="http://www.w3.org/2006/vcard/ns"/>
        <rdfs:label xml:lang="en">Sibling</rdfs:label>
    </owl:Class>
    


    <!-- http://www.w3.org/2006/vcard/ns#Spouse -->

    <owl:Class rdf:about="http://www.w3.org/2006/vcard/ns#Spouse">
        <rdfs:subClassOf rdf:resource="http://www.w3.org/2006/vcard/ns#RelatedType"/>
        <rdfs:isDefinedBy rdf:resource="http://www.w3.org/2006/vcard/ns"/>
        <rdfs:label xml:lang="en">Spouse</rdfs:label>
    </owl:Class>
    


    <!-- http://www.w3.org/2006/vcard/ns#Sweetheart -->

    <owl:Class rdf:about="http://www.w3.org/2006/vcard/ns#Sweetheart">
        <rdfs:subClassOf rdf:resource="http://www.w3.org/2006/vcard/ns#RelatedType"/>
        <rdfs:isDefinedBy rdf:resource="http://www.w3.org/2006/vcard/ns"/>
        <rdfs:label xml:lang="en">Sweetheart</rdfs:label>
    </owl:Class>
    


    <!-- http://www.w3.org/2006/vcard/ns#Tel -->

    <owl:Class rdf:about="http://www.w3.org/2006/vcard/ns#Tel">
        <rdfs:comment xml:lang="en">This class is deprecated. Use the hasTelephone object property.</rdfs:comment>
        <rdfs:isDefinedBy rdf:resource="http://www.w3.org/2006/vcard/ns"/>
        <rdfs:label xml:lang="en">Tel</rdfs:label>
        <owl:deprecated rdf:datatype="http://www.w3.org/2001/XMLSchema#boolean">true</owl:deprecated>
    </owl:Class>
    


    <!-- http://www.w3.org/2006/vcard/ns#TelephoneType -->

    <owl:Class rdf:about="http://www.w3.org/2006/vcard/ns#TelephoneType">
        <www:subClassOfInverted rdf:resource="http://www.w3.org/2006/vcard/ns#BBS"/>
        <www:subClassOfInverted rdf:resource="http://www.w3.org/2006/vcard/ns#Car"/>
        <www:subClassOfInverted rdf:resource="http://www.w3.org/2006/vcard/ns#Cell"/>
        <www:subClassOfInverted rdf:resource="http://www.w3.org/2006/vcard/ns#Fax"/>
        <www:subClassOfInverted rdf:resource="http://www.w3.org/2006/vcard/ns#Modem"/>
        <www:subClassOfInverted rdf:resource="http://www.w3.org/2006/vcard/ns#Msg"/>
        <www:subClassOfInverted rdf:resource="http://www.w3.org/2006/vcard/ns#PCS"/>
        <www:subClassOfInverted rdf:resource="http://www.w3.org/2006/vcard/ns#Pager"/>
        <www:subClassOfInverted rdf:resource="http://www.w3.org/2006/vcard/ns#Text"/>
        <www:subClassOfInverted rdf:resource="http://www.w3.org/2006/vcard/ns#TextPhone"/>
        <www:subClassOfInverted rdf:resource="http://www.w3.org/2006/vcard/ns#Video"/>
        <www:subClassOfInverted rdf:resource="http://www.w3.org/2006/vcard/ns#Voice"/>
        <rdfs:comment xml:lang="en">Used for telephone type codes. The URI of the telephone type code must be used as the value for the Telephone Type.</rdfs:comment>
        <rdfs:isDefinedBy rdf:resource="http://www.w3.org/2006/vcard/ns"/>
        <rdfs:label xml:lang="en">Phone</rdfs:label>
    </owl:Class>
    


    <!-- http://www.w3.org/2006/vcard/ns#Text -->

    <owl:Class rdf:about="http://www.w3.org/2006/vcard/ns#Text">
        <rdfs:subClassOf rdf:resource="http://www.w3.org/2006/vcard/ns#TelephoneType"/>
        <rdfs:comment xml:lang="en">Also called sms telephone</rdfs:comment>
        <rdfs:isDefinedBy rdf:resource="http://www.w3.org/2006/vcard/ns"/>
        <rdfs:label xml:lang="en">Text</rdfs:label>
    </owl:Class>
    


    <!-- http://www.w3.org/2006/vcard/ns#TextPhone -->

    <owl:Class rdf:about="http://www.w3.org/2006/vcard/ns#TextPhone">
        <rdfs:subClassOf rdf:resource="http://www.w3.org/2006/vcard/ns#TelephoneType"/>
        <rdfs:isDefinedBy rdf:resource="http://www.w3.org/2006/vcard/ns"/>
        <rdfs:label xml:lang="en">Text phone</rdfs:label>
    </owl:Class>
    


    <!-- http://www.w3.org/2006/vcard/ns#Type -->

    <owl:Class rdf:about="http://www.w3.org/2006/vcard/ns#Type">
        <www:subClassOfInverted rdf:resource="http://www.w3.org/2006/vcard/ns#Dom"/>
        <www:subClassOfInverted rdf:resource="http://www.w3.org/2006/vcard/ns#Home"/>
        <www:subClassOfInverted rdf:resource="http://www.w3.org/2006/vcard/ns#ISDN"/>
        <www:subClassOfInverted rdf:resource="http://www.w3.org/2006/vcard/ns#Internet"/>
        <www:subClassOfInverted rdf:resource="http://www.w3.org/2006/vcard/ns#Intl"/>
        <www:subClassOfInverted rdf:resource="http://www.w3.org/2006/vcard/ns#Label"/>
        <www:subClassOfInverted rdf:resource="http://www.w3.org/2006/vcard/ns#Parcel"/>
        <www:subClassOfInverted rdf:resource="http://www.w3.org/2006/vcard/ns#Postal"/>
        <www:subClassOfInverted rdf:resource="http://www.w3.org/2006/vcard/ns#Pref"/>
        <www:subClassOfInverted rdf:resource="http://www.w3.org/2006/vcard/ns#Work"/>
        <www:subClassOfInverted rdf:resource="http://www.w3.org/2006/vcard/ns#X400"/>
        <rdfs:comment xml:lang="en">Used for type codes. The URI of the type code must be used as the value for Type.</rdfs:comment>
        <rdfs:isDefinedBy rdf:resource="http://www.w3.org/2006/vcard/ns"/>
        <rdfs:label xml:lang="en">Type</rdfs:label>
    </owl:Class>
    


    <!-- http://www.w3.org/2006/vcard/ns#Unknown -->

    <owl:Class rdf:about="http://www.w3.org/2006/vcard/ns#Unknown">
        <rdfs:subClassOf rdf:resource="http://www.w3.org/2006/vcard/ns#Gender"/>
        <rdfs:isDefinedBy rdf:resource="http://www.w3.org/2006/vcard/ns"/>
        <rdfs:label xml:lang="en">Unknown</rdfs:label>
    </owl:Class>
    


    <!-- http://www.w3.org/2006/vcard/ns#VCard -->

    <owl:Class rdf:about="http://www.w3.org/2006/vcard/ns#VCard">
        <rdfs:comment xml:lang="en">The vCard class is  equivalent to the new Kind class, which is the parent for the four explicit types of vCards (Individual, Organization, Location, Group)</rdfs:comment>
        <rdfs:isDefinedBy rdf:resource="http://www.w3.org/2006/vcard/ns"/>
        <rdfs:label xml:lang="en">VCard</rdfs:label>
    </owl:Class>
    


    <!-- http://www.w3.org/2006/vcard/ns#Video -->

    <owl:Class rdf:about="http://www.w3.org/2006/vcard/ns#Video">
        <rdfs:subClassOf rdf:resource="http://www.w3.org/2006/vcard/ns#TelephoneType"/>
        <rdfs:isDefinedBy rdf:resource="http://www.w3.org/2006/vcard/ns"/>
        <rdfs:label xml:lang="en">Video</rdfs:label>
    </owl:Class>
    


    <!-- http://www.w3.org/2006/vcard/ns#Voice -->

    <owl:Class rdf:about="http://www.w3.org/2006/vcard/ns#Voice">
        <rdfs:subClassOf rdf:resource="http://www.w3.org/2006/vcard/ns#TelephoneType"/>
        <rdfs:isDefinedBy rdf:resource="http://www.w3.org/2006/vcard/ns"/>
        <rdfs:label xml:lang="en">Voice</rdfs:label>
    </owl:Class>
    


    <!-- http://www.w3.org/2006/vcard/ns#Work -->

    <owl:Class rdf:about="http://www.w3.org/2006/vcard/ns#Work">
        <rdfs:subClassOf rdf:resource="http://www.w3.org/2006/vcard/ns#Type"/>
        <rdfs:comment xml:lang="en">This implies that the property is related to an individual&apos;s work place</rdfs:comment>
        <rdfs:isDefinedBy rdf:resource="http://www.w3.org/2006/vcard/ns"/>
        <rdfs:label xml:lang="en">Work</rdfs:label>
    </owl:Class>
    


    <!-- http://www.w3.org/2006/vcard/ns#X400 -->

    <owl:Class rdf:about="http://www.w3.org/2006/vcard/ns#X400">
        <rdfs:subClassOf rdf:resource="http://www.w3.org/2006/vcard/ns#Type"/>
        <rdfs:comment xml:lang="en">This class is deprecated</rdfs:comment>
        <rdfs:isDefinedBy rdf:resource="http://www.w3.org/2006/vcard/ns"/>
        <rdfs:label xml:lang="en">X400</rdfs:label>
        <owl:deprecated rdf:datatype="http://www.w3.org/2001/XMLSchema#boolean">true</owl:deprecated>
    </owl:Class>
    


    <!-- http://www.w3.org/ns/org#ChangeEvent -->

    <owl:Class rdf:about="http://www.w3.org/ns/org#ChangeEvent">
        <rdfs:subClassOf rdf:resource="http://www.w3.org/ns/prov#Activity"/>
        <owl:disjointWith rdf:resource="http://www.w3.org/ns/org#Membership"/>
        <owl:disjointWith rdf:resource="http://www.w3.org/ns/org#Organization"/>
        <owl:disjointWith rdf:resource="http://www.w3.org/ns/org#Role"/>
        <owl:disjointWith rdf:resource="http://www.w3.org/ns/org#Site"/>
        <rdfs:comment xml:lang="es">Evento que da como resultado un cambio sustancial en la organización, por ejemplo, una fusión o una reestructuración total. Está pensado para situaciones en las que la organización resultante es lo suficientemente distinta de las organizaciones originales, tiene una identidad distinta y una URI también distinta. Se deberían definir subtipos de eventos mediante vocabularios específicos (Extension vocabularies) para referirse a categorías de eventos específicos. El momento o periodo en el que el evento ocurre se debería expresar mediante las propiedades `prov:startAtTime` y `prov:endedAtTime`, y una descripción del mismo se debería incluir mediante el uso de la propiedad `dct:description`.</rdfs:comment>
        <rdfs:comment xml:lang="it">Rappresenta un evento risultato essere un importante cambiamento per un&apos;organizzazione come ad esempio una fusione o una riorganizzazione. È pensato per quelle situazioni in cui l&apos;organizzazione risultante si distingue da quella originale sufficientemente da essere rappresentata con una URI differente. Le estensioni del vocabolario dovrebbero definire le sotto-classi per esprimere particolari categorie di eventi. L&apos;istante o l&apos;intervallo in cui l&apos;evento accade dovrebbe essere espresso tramite `prov:startAtTime` e`prov:endedAtTime`. Una descrizione dovrebbe essere fornita attraverso `dct:description`.</rdfs:comment>
        <rdfs:comment xml:lang="en">Represents an event which resulted in a major change to an organization such as a merger or complete restructuring. It is intended for situations where the resulting organization is sufficient distinct from the original organizations that it has a distinct identity and distinct URI. Extension vocabularies should define sub-classes of this to denote particular categories of event. The instant or interval at which the event occurred should be given by `prov:startAtTime` and `prov:endedAtTime`, a description should be given by `dct:description`. </rdfs:comment>
        <rdfs:comment xml:lang="fr">Représente un Évènement impliquant un changement majeur dans l&apos;Organisation, comme une fusion ou une restructuration. Prévu pour des situations ou l&apos;organisation finale est suffisamment différente des Organisations originales pour qu&apos;elle ait une identité et une URI distinctes. Des vocabulaires d&apos;extension devraient définir des sous-classes de celle-ci pour annoter les différentes catégories d&apos;Évènemenents. Le moment ou l&apos;intervalle de l&apos;Évènement devrait être indiqué avec `prov:startAtTime` et `prov:endedAtTime`, et une description avec la classe `dct:description`. </rdfs:comment>
        <rdfs:comment xml:lang="ja">合併や完全な再編などの組織に大きな変化をもたらした出来事を表わします。これは、結果として作成される組織と元の組織とが、別のアイデンティティーと別のURIを持つに足るほど異なる状況を対象としています。</rdfs:comment>
        <rdfs:isDefinedBy rdf:resource="http://www.w3.org/ns/org"/>
        <rdfs:label xml:lang="en">Change Event</rdfs:label>
        <rdfs:label xml:lang="it">Evento di cambiamento</rdfs:label>
        <rdfs:label xml:lang="es">evento de cambio</rdfs:label>
        <rdfs:label xml:lang="fr">Évènement</rdfs:label>
    </owl:Class>
    


    <!-- http://www.w3.org/ns/org#FormalOrganization -->

    <owl:Class rdf:about="http://www.w3.org/ns/org#FormalOrganization">
        <rdfs:subClassOf rdf:resource="http://www.w3.org/ns/org#Organization"/>
        <rdfs:subClassOf rdf:resource="http://xmlns.com/foaf/0.1/Organization"/>
        <www:subClassOfInverted rdf:resource="http://purl.org/goodrelations/v1#BusinessEntity"/>
        <rdfs:comment xml:lang="en">An Organization which is recognized in the world at large, in particular in legal jurisdictions, with associated rights and responsibilities. Examples include a Corporation, Charity, Government or Church. Note that this is a super class of `gr:BusinessEntity` and it is recommended to use the GoodRelations vocabulary to denote Business classifications such as DUNS or NAICS.</rdfs:comment>
        <rdfs:comment xml:lang="es">Organización reconocida a nivel mundial, en particular en jurisdicciones legales, con derechos y responsabilidades asociadas. Algunos ejemplos son: organización corporativa, organización benéfica, organización gubernamental, organización religiosa. Se debe tener en cuenta que ésta es una superclase de `gr:BusinessEntity` y que se recomienda el uso del vocabulario GoodRelations para referirse a clasificaciones de negocios tales como DUNS o NAICS.</rdfs:comment>
        <rdfs:comment xml:lang="it">Un&apos;organizzazione che è riconosciuta a livello mondiale o, in generale, all&apos;interno di una qualche giurisdizione, e che quindi possiede diritti e responsabilità. Ad esempio aziende, enti governativi, associazioni di volontariato. Si noti che questa è una superclasse di `gr:BusinessEntity` e che quindi è raccomandabile usare il vocabolario GoodRelations per esprimere classificazioni di tipo industriale e commerciale come DUNS e NAICS.</rdfs:comment>
        <rdfs:comment xml:lang="fr">Une Organisation reconnue, en particulier par les juridictions locales, ayant des droits et des responsabilités. Exemples : entreprises, association à but non-lucratif, collectivité, église. Notez que c&apos;est une super-classe de `gr:BusinessEntity` et qu&apos;il est recommandé d&apos;utiliser le vocabulaire GoodRelations pour indiquer les classifications économiques comme le code NACE.</rdfs:comment>
        <rdfs:comment xml:lang="ja">関連する権利と責任を有する（特に法的管轄区域において）世界中に広く認識されている組織。例には、企業、慈善団体、政府や教会が含まれます。</rdfs:comment>
        <rdfs:isDefinedBy rdf:resource="http://www.w3.org/ns/org"/>
        <rdfs:label xml:lang="en">Formal Organization</rdfs:label>
        <rdfs:label xml:lang="fr">Organisation Formelle</rdfs:label>
        <rdfs:label xml:lang="it">Organizzazione formale</rdfs:label>
        <rdfs:label xml:lang="es">organización formal</rdfs:label>
    </owl:Class>
    


    <!-- http://www.w3.org/ns/org#Membership -->

    <owl:Class rdf:about="http://www.w3.org/ns/org#Membership">
        <owl:disjointWith rdf:resource="http://www.w3.org/ns/org#Organization"/>
        <owl:disjointWith rdf:resource="http://www.w3.org/ns/org#Role"/>
        <owl:disjointWith rdf:resource="http://www.w3.org/ns/org#Site"/>
        <rdfs:comment xml:lang="it">Indica la natura della relazione di appartenenza di un Agent in un&apos;organizzazione. Rappresenta una relazione n-aria tra un&apos;Agent, un Organization e un Role. È possibile indicare direttamente la membership, indipendentemente dallo specifico Role, attraverso l&apos;uso della proprietà `org:memberOf`</rdfs:comment>
        <rdfs:comment xml:lang="en">Indicates the nature of an Agent&apos;s membership of an organization. Represents an n-ary relation between an Agent, an Organization and a Role. It is possible to directly indicate membership, independent of the specific Role, through use of the `org:memberOf` property.</rdfs:comment>
        <rdfs:comment xml:lang="fr">Indique la nature de l&apos;engagement d&apos;un Agent dans une Organisation. Représente une relation n-aire entre un Agent, une Organisation et un Role. Il est possible d&apos;indiquer directement l&apos;appartenance à une organisation, independemment d&apos;un rôle spécifique, à travers l&apos;usage de la propriété `org:memberOf`.</rdfs:comment>
        <rdfs:comment xml:lang="es">Pertenencia o afiliación de un agente a una organización. Es una relación n-aria entre un agente, una organización y una actividad. Es posible indicar pertenencia mediante el uso de la propiedad `org:memberOf`, independientemente de la actividad específica que se desempeñe.</rdfs:comment>
        <rdfs:comment xml:lang="ja">組織のエージェントの構成員の本質を示します。</rdfs:comment>
        <rdfs:isDefinedBy rdf:resource="http://www.w3.org/ns/org"/>
        <rdfs:label xml:lang="it">Appartenenza</rdfs:label>
        <rdfs:label xml:lang="fr">Engagement</rdfs:label>
        <rdfs:label xml:lang="en">Membership</rdfs:label>
        <rdfs:label xml:lang="es">membresía</rdfs:label>
    </owl:Class>
    


    <!-- http://www.w3.org/ns/org#Organization -->

    <owl:Class rdf:about="http://www.w3.org/ns/org#Organization">
        <owl:equivalentClass rdf:resource="http://xmlns.com/foaf/0.1/Organization"/>
        <rdfs:subClassOf rdf:resource="http://xmlns.com/foaf/0.1/Agent"/>
        <owl:disjointWith rdf:resource="http://www.w3.org/ns/org#Role"/>
        <owl:disjointWith rdf:resource="http://www.w3.org/ns/org#Site"/>
        <owl:hasKey rdf:parseType="Collection">
            <rdf:Description rdf:about="http://www.w3.org/ns/org#identifier"/>
        </owl:hasKey>
        <www:subClassOfInverted rdf:resource="http://www.w3.org/ns/org#FormalOrganization"/>
        <www:subClassOfInverted rdf:resource="http://www.w3.org/ns/org#OrganizationalUnit"/>
        <www:subClassOfInverted>
            <rdf:Description>
                <rdfs:comment xml:lang="en">A collaboration between two or more Organizations such as a project. It meets the criteria for being an Organization in that it has an identity and defining purpose independent of its particular members but is neither a formally recognized legal entity nor a sub-unit within some larger organization. Might typically have a shorter lifetime than the Organizations within it, but not necessarily. All members are `org:Organization`s rather than individuals and those Organizations can play particular roles within the venture. Alternative names: _Project_ _Venture_  _Endeavour_ _Consortium_ _Endeavour_</rdfs:comment>
                <rdfs:comment xml:lang="es">Colaboración determinada entre dos o más organizaciones, como en el caso de un proyecto común. Cumple con los criterios de ser una organización en sí misma, en la medida en que tiene una identidad y un propósito definido independiente de sus miembros en particular, pero no es una entidad legal formalmente reconocida ni una sub-unidad dentro de una organización más grande. La duración suele ser más corta que la de las organizaciones que lo componen, pero no necesariamente. Todos sus miembros son de tipo `org:Organization` en vez de individuos, y desempeñan una actividad concreta en el marco del proyecto de cooperación.</rdfs:comment>
                <rdfs:comment xml:lang="fr">Une collaboration entre deux ou plusieurs Organisations, telle qu&apos;un projet commun. Un partenariat peut être considéré comme Organisation dans le sens ou il possède une identité et un But propre indépendant de ceux de ses membres, mais ce n&apos;est ni une entité légale ni une sous-unité d&apos;une Organisation plus grande. Typiquement, elle peut avoir une durée de vie plus courte que les Organisations qui la composent, mais pas nécessairement. Tous les membres sont des `org:Organization`s plutôt que des individus et ces Organisations peuvent jouer des Rôles particuliers au sein du Partenariat. </rdfs:comment>
                <rdfs:comment xml:lang="it">È una collaborazione tra due o più Organization come ad esempio un progetto. Consente di rappresentare alcune identità dell&apos;Organization che sono fuori dallo scopo principale e non sono formalmente riconosciute. Potrebbe anche avere un ciclo di vita limitato.</rdfs:comment>
                <rdfs:comment xml:lang="ja">プロジェクトなどの2つ以上の組織間のコラボレーション。それは、アイデンティティを有し、その特定のメンバーとは無関係に目的を定めているという点で、組織としての基準を満たしますが、正式に認識された法的実体でも、あるより大きな組織内のサブユニットでもありません。一般的には、その内部の組織よりも存続期間が短いかもしれませんが、必ずしもそうとは限りません。</rdfs:comment>
                <rdfs:isDefinedBy rdf:resource="http://www.w3.org/ns/org"/>
                <rdfs:label xml:lang="it">Collaborazione</rdfs:label>
                <rdfs:label xml:lang="en">Endeavour</rdfs:label>
                <rdfs:label xml:lang="fr">Partenariat</rdfs:label>
                <rdfs:label xml:lang="es">proyecto de cooperación empresarial</rdfs:label>
            </rdf:Description>
        </www:subClassOfInverted>
        <rdfs:comment xml:lang="es">Grupo de personas que se organiza en una comunidad u otro tipo de estructura social, comercial o política. Dicho grupo tiene un objetivo o motivo común para su existencia que va más allá del conjunto de personas que lo forman y que puede actuar como “agente”. A menudo las organizaciones se pueden agrupar en estructuras jerárquicas. Se recomienda el uso de etiquetas de SKOS para denominar a cada “organización”. En concreto, `skos:prefLabel` para la denominación principal o recomendada (aquella reconocida legalmente, siempre que sea posible), `skos:altLabel` para denominaciones alternativas (nombre comercial, sigla, denominación por la que se conoce a la organización coloquialmente) y `skos:notation` para referirse al código que identifique a la organización en una lista de códigos. Denominaciones alternativas: _colectivo_ _corporación_ _grupo_</rdfs:comment>
        <rdfs:comment xml:lang="it">Rappresenta una collezione di persone organizzate all&apos;interno di una communità o di una qualche struttura sociale, commerciale o politica. Il gruppo condivide un obiettivo o una ragione d&apos;essere che va oltre gli stessi membri appartenenti al gruppo e  può agire come un Agent. Le organizzazioni si possono spesso suddividere in strutture gerarchiche. Si raccomanda di usare le label per l&apos;Organization mediante le proprietà di SKOS. In particolare, `skos:prefLabel` per il nome principale (possibilmente un nome legalmente riconosciuto)”, `skos:altLabel` come nome alternativo (denominazione commerciale, denominazione colloquiale) e `skos:notation` per indicare un codice di una lista di codici.</rdfs:comment>
        <rdfs:comment xml:lang="en">Represents a collection of people organized together into a community or other social, commercial or political structure. The group has some common purpose or reason for existence which goes beyond the set of people belonging to it and can act as an Agent. Organizations are often decomposable into hierarchical structures.  It is recommended that SKOS lexical labels should be used to label the Organization. In particular `skos:prefLabel` for the primary (possibly legally recognized name), `skos:altLabel` for alternative names (trading names, colloquial names) and `skos:notation` to denote a code from a code list. Alternative names: _Collective_ _Body_ _Org_ _Group_</rdfs:comment>
        <rdfs:comment xml:lang="fr">Représente un groupe de personnes organisées en communauté où tout autre forme de structure sociale, commerciale ou politique. Le groupe a un but commun ou une raison d&apos;être qui va au-delà de la somme des personnes qui en font partie et peut agir en tant que &quot;Agent&quot;. Les organisations sont souvent décomposables en structures hiérarchisées. Il est recommandé que des labels lexicaux SKOS soient utilisés pour nommer l&apos;Organisation. En particulier `skos:prefLabel` pour le nom principal (en général le nom légal), `skos:altLabel` pour les noms alternatifs (marques, sigles, appellations familières) et `skos:notation` pour indiquer un code provenant d&apos;une liste de code.</rdfs:comment>
        <rdfs:comment xml:lang="ja">コミュニティー、その他の社会、商業、政治的な構造に共に編入された人々の集合を表わします。グループには、そこに属する人々を超えた、存在に対するある共通の目的や理由があり、エージェント（代理）を務めることができます。組織は、多くの場合、階層構造に分割できます。</rdfs:comment>
        <rdfs:isDefinedBy rdf:resource="http://www.w3.org/ns/org"/>
        <rdfs:label xml:lang="fr">Organisation</rdfs:label>
        <rdfs:label xml:lang="en">Organization</rdfs:label>
        <rdfs:label xml:lang="it">Organizzazione</rdfs:label>
        <rdfs:label>org:Organization</rdfs:label>
        <rdfs:label xml:lang="es">organización</rdfs:label>
    </owl:Class>
    


    <!-- http://www.w3.org/ns/org#OrganizationalCollaboration -->

    <owl:Class rdf:about="http://www.w3.org/ns/org#OrganizationalCollaboration">
        <owl:equivalentClass>
            <owl:Class>
                <owl:intersectionOf rdf:parseType="Collection">
                    <rdf:Description rdf:about="http://www.w3.org/ns/org#Organization"/>
                    <owl:Restriction>
                        <owl:onProperty rdf:resource="http://www.w3.org/ns/org#hasMember"/>
                        <owl:allValuesFrom rdf:resource="http://www.w3.org/ns/org#Organization"/>
                    </owl:Restriction>
                </owl:intersectionOf>
            </owl:Class>
        </owl:equivalentClass>
    </owl:Class>
    


    <!-- http://www.w3.org/ns/org#OrganizationalUnit -->

    <owl:Class rdf:about="http://www.w3.org/ns/org#OrganizationalUnit">
        <rdfs:subClassOf rdf:resource="http://www.w3.org/ns/org#Organization"/>
        <rdfs:comment xml:lang="en">An Organization such as a University Support Unit which is part of some larger FormalOrganization and only has full recognition within the context of that FormalOrganization, it is not a Legal Entity in its own right. Units can be large and complex containing other Units and even FormalOrganizations. Alternative names: _OU_ _Unit_ _Department_</rdfs:comment>
        <rdfs:comment xml:lang="es">Organización que forma parte de una organización formal más amplia, como el servicio de informática o centro de cálculo de una universidad, y que sólo tiene reconocimiento pleno en el contexto de dicha organización formal, pero que no es una entidad legal propiamente dicha. Estas unidades pueden ser amplias y complejas, e incluir a otras unidades o incluso a otras organizaciones formales. Denominaciones alternativas: departamento.</rdfs:comment>
        <rdfs:comment xml:lang="it">Un&apos;organizzazione come ad esempio l&apos;unità dei sistemi informativi che è parte di una più grande FormalOrganization e che, pur essendo riconosciuta nel contesto della propria organizzazione di riferimento, non è legalmente riconosciuta come entità a sé stante. Le unità possono essere ampie e complesse e contenere al loro interno sia altre unità che addirittura FormalOrganization.</rdfs:comment>
        <rdfs:comment xml:lang="fr">Une organisation telle que le support informatique d&apos;une université, qui fait partie d&apos;une Organisation Formelle plus importante et qui ne peut être reconnue qu&apos;en tant que membre de cette organisation supérieure, ce n&apos;est pas une entité légale en elle-même. Les unités opérationnelles peuvent être étendues, complexes et inclure elles-mêmes d&apos;autres branches ou Unités Opérationnelles, voire des Organisations Formelles.</rdfs:comment>
        <rdfs:comment xml:lang="ja">あるより大きな組織の一部であり、その組織の中においてのみ完全に認識される部局や支援部署などの組織です。特に、その単位はそれ自体では法的実体と見なされません。</rdfs:comment>
        <rdfs:isDefinedBy rdf:resource="http://www.w3.org/ns/org"/>
        <rdfs:label xml:lang="en">OrganizationalUnit</rdfs:label>
        <rdfs:label xml:lang="it">Unità Organizzativa</rdfs:label>
        <rdfs:label xml:lang="fr">Unité opérationnelle</rdfs:label>
        <rdfs:label xml:lang="es">unidad organizativa</rdfs:label>
    </owl:Class>
    


    <!-- http://www.w3.org/ns/org#Post -->

    <owl:Class rdf:about="http://www.w3.org/ns/org#Post">
        <rdfs:comment xml:lang="en">A Post represents some position within an organization that exists independently of the person or persons filling it. Posts may be used to represent situations where a person is a member of an organization ex officio (for example the Secretary of State for Scotland is part of UK Cabinet by virtue of being Secretary of State for Scotland, not as an individual person). A post can be held by multiple people and hence can be treated as a organization in its own right.</rdfs:comment>
        <rdfs:comment xml:lang="es">Puesto o posición que representa algún tipo de empleo dentro de una organización, que existe independientemente de la persona o personas que lo desempeñan. Esta clase puede utilizarse para representar situaciones en las que una persona es miembro de una organización ex oficio (por ejemplo, el Secretario de Estado escocés es parte del Gabinete del gobierno británico por virtud de ser Secretario de Estado en Escocia, y no como individuo). Un puesto puede ser desempeñado por múltiples individuos y de aquí que sea tratado como una organización en sí misma.</rdfs:comment>
        <rdfs:comment xml:lang="it">Un Impiego rappresenta una posizione all&apos;interno dell&apos;organizzazione che esiste indipendentemente dalla persona che la ricopre. Gli impieghi possono essere utilizzati per le situazioni in cui una persona è membro di un&apos;organizzazione o di un ufficio (ad esempio un segretario di stato). Un Impiego può essere ricoperto da più persone.</rdfs:comment>
        <rdfs:comment xml:lang="fr">Un Poste représente une position au sein d&apos;une Organisation qui existe indépendamment de la personne ou des personnes qui le remplissent. Les postes peuvent être utilisés pour représenter des situations où une personne est membre d&apos;une Organisation d&apos;office (par exemple, le Secrétaire d&apos;Etat pour l&apos;Ecosse fait partie du Cabinet du Royaume-Uni du fait d&apos;être Secrétaire d&apos;Etat pour l&apos;Ecosse, non pas comme une personne physique). Un poste après peut être occupé par plusieurs personnes et peut donc être considéré comme une Organisation à part entière.</rdfs:comment>
        <rdfs:comment xml:lang="ja">ポストは、それを埋める人（人々）とは無関係に存在する組織内のある位置を表わします。ポストは、人が職権上、組織のメンバーである状況を表わすために使用できます（例えば、スコットランド大臣は、個人としてではなく、スコットランド大臣であることにより、英国内閣の一部です）。ポストは、複数の人々によって保持されることが可能だあるため、それ自体を組織として扱うことができます。</rdfs:comment>
        <rdfs:isDefinedBy rdf:resource="http://www.w3.org/ns/org"/>
        <rdfs:label xml:lang="it">Impiego</rdfs:label>
        <rdfs:label xml:lang="en">Post</rdfs:label>
        <rdfs:label xml:lang="fr">Poste</rdfs:label>
        <rdfs:label xml:lang="es">puesto</rdfs:label>
    </owl:Class>
    


    <!-- http://www.w3.org/ns/org#Role -->

    <owl:Class rdf:about="http://www.w3.org/ns/org#Role">
        <rdfs:subClassOf rdf:resource="http://www.w3.org/2004/02/skos/core#Concept"/>
        <owl:disjointWith rdf:resource="http://www.w3.org/ns/org#Site"/>
        <rdfs:comment xml:lang="en">Denotes a role that a Person or other Agent can take in an organization. Instances of this class describe the abstract role; to denote a specific instance of a person playing that role in a specific organization use an instance of `org:Membership`. It is common for roles to be arranged in some taxonomic structure and we use SKOS to represent that. The normal SKOS lexical properties should be used when labelling the Role. Additional descriptive properties for the Role, such as a Salary band, may be added by extension vocabularies.</rdfs:comment>
        <rdfs:comment xml:lang="es">Función que una persona o agente desempeña en el seno de una organización. Las instancias de esta clase describen la actividad en abstracto; si lo que se pretende es incluir una instancia que refleje la función o actividad que desempeña una persona en concreto en una organización específica, se indica el uso de instancias de la clase `org:Membership`. Es común que dichas actividades se representen en una estructura taxonómica mediante SKOS. Las propiedades léxicas de SKOS deberían utilizarse a la hora de denominar o etiquetar la actividad desempeñada. Para añadir propiedades descriptivas adicionales, como rango salarial, se tendrá que recurrir a vocabularios externos.</rdfs:comment>
        <rdfs:comment xml:lang="it">Indica il ruolo che una Person o un altro Agent può assumere in un&apos;organizzazione. Le istanze di questa classe descrivono un ruolo astratto; per esprimere il ruolo che una precisa persona ricopre in un&apos;organizzazione si usi un&apos;istanza di `org:Membership`. È comune organizzare i ruoli in una qualche struttura tassonomica e quindi si raccomanda SKOS per questo. Altre proprietà descrittive per il Role, come salario, possono essere aggiunte mediante l&apos;uso di altri vocabolari.</rdfs:comment>
        <rdfs:comment xml:lang="fr">Indique le rôle qu&apos;une Personne ou un autre Agent peut avoir dans une Organisation. Les instances de cette classe décrivent le rôle dans l&apos;absolu; pour indiquer une personne ayant ce rôle spécifique dans une Organisation, utilisez une instance de `org:Membership`. Il est courant que les rôles soient organisés dans une sorte de taxonomie, ce qui peut être représenté avec SKOS. Les propriétés de libellés standards de SKOS devraient être utilisées pour libeller le Rôle. D&apos;autres propriétés additionnelles pour ce rôle, comme une fourchette de Salaire peuvent être ajoutées par une extension de ce vocabulaire.</rdfs:comment>
        <rdfs:comment xml:lang="ja">人またはその他のエージェントが組織で担うことができる役割を表わします。この種のインスタンスは、抽象的な役割を記述します。特定の組織でその役割を担っている人の特定のインスタンスを示すためには、org:Membershipのインスタンスを使用します。</rdfs:comment>
        <rdfs:isDefinedBy rdf:resource="http://www.w3.org/ns/org"/>
        <rdfs:label xml:lang="en">Role</rdfs:label>
        <rdfs:label xml:lang="it">Ruolo</rdfs:label>
        <rdfs:label xml:lang="fr">Rôle</rdfs:label>
        <rdfs:label xml:lang="es">actividad</rdfs:label>
    </owl:Class>
    


    <!-- http://www.w3.org/ns/org#Site -->

    <owl:Class rdf:about="http://www.w3.org/ns/org#Site">
        <rdfs:comment xml:lang="en">An office or other premise at which the organization is located. Many organizations are spread across multiple sites and many sites will host multiple locations. In most cases a Site will be a physical location. However, we don&apos;t exclude the possibility of non-physical sites such as a virtual office with an associated post box and phone reception service. Extensions may provide subclasses to denote particular types of site.</rdfs:comment>
        <rdfs:comment xml:lang="es">Oficina, local o cualquier otro lugar en el que se encuentra una organización. Muchas organizaciones están distribuidas en varias sedes, que a su vez están repartidas en distintas ubicaciones. En muchos casos una sede será un sitio o local físico. Sin embargo, no se excluye la posibilidad de lugares no físicos como oficinas virtuales con los correspondientes apartados de correo y servicio de atención telefónica. Se pueden añadir más subtipos mediante extensiones para incluir tipos especiales de lugares.</rdfs:comment>
        <rdfs:comment xml:lang="it">Un ufficio o altra sede dovei l&apos;organizzazione è situata. Molte organizzazione sono distribuite su più sedi e molte sedi ospitano più ubicazioni. Nella maggior parte dei casi un Site è una locazione fisica. Non si esclude la possibilità di indicare sedi non fisiche come ad esempio gli uffici virtuali. Le estensioni dell&apos;ontologia potrebbero usare delle sottoclassi per rappresentare i tipi particolari di sede.</rdfs:comment>
        <rdfs:comment xml:lang="fr">Un établissement ou tout autre lieu dans lequel une Organisation est localisé. Beaucoup d&apos;organisations sont dispersées à travers plusieurs sites. Dans la plupart des cas un Site sera un lieu physique. Toutefois, nous n&apos;excluons pas la possibilité de sites non-physiques comme un bureau virtuel avec une boîte postale et un service de secrétariat mutualisé. Des extensions pourraient fournir des sous-classes pour décrire des types de sites particuliers.</rdfs:comment>
        <rdfs:comment xml:lang="ja">組織が位置するオフィスやその他の敷地。多くの組織が複数のサイトに散在しており、多くのサイトが多数の場所を持つでしょう。</rdfs:comment>
        <rdfs:isDefinedBy rdf:resource="http://www.w3.org/ns/org"/>
        <rdfs:label xml:lang="it">Sede</rdfs:label>
        <rdfs:label xml:lang="en">Site</rdfs:label>
        <rdfs:label xml:lang="fr">Site</rdfs:label>
        <rdfs:label xml:lang="es">sede</rdfs:label>
    </owl:Class>
    


    <!-- http://www.w3.org/ns/prov#Activity -->

    <owl:Class rdf:about="http://www.w3.org/ns/prov#Activity">
        <www:subClassOfInverted rdf:resource="http://www.w3.org/ns/org#ChangeEvent"/>
    </owl:Class>
    


    <!-- http://xmlns.com/foaf/0.1/Agent -->

    <owl:Class rdf:about="http://xmlns.com/foaf/0.1/Agent">
        <www:subClassOfInverted rdf:resource="http://iirds.tekom.de/iirds#Agent"/>
        <www:subClassOfInverted rdf:resource="http://www.w3.org/ns/org#Organization"/>
        <www:subClassOfInverted rdf:resource="http://xmlns.com/foaf/0.1/Person"/>
    </owl:Class>
    


    <!-- http://xmlns.com/foaf/0.1/Organization -->

    <owl:Class rdf:about="http://xmlns.com/foaf/0.1/Organization">
        <www:subClassOfInverted rdf:resource="http://www.w3.org/ns/org#FormalOrganization"/>
    </owl:Class>
    


    <!-- http://xmlns.com/foaf/0.1/Person -->

    <owl:Class rdf:about="http://xmlns.com/foaf/0.1/Person">
        <rdfs:subClassOf rdf:resource="http://xmlns.com/foaf/0.1/Agent"/>
        <www:subClassOfInverted rdf:resource="http://people.aifb.kit.edu/mu2771/step#Scheduler"/>
        <www:subClassOfInverted rdf:resource="http://people.aifb.kit.edu/mu2771/step#Technician"/>
        <rdfs:label xml:lang="de">Person</rdfs:label>
    </owl:Class>
    


    <!-- 
    ///////////////////////////////////////////////////////////////////////////////////////
    //
    // Individuals
    //
    ///////////////////////////////////////////////////////////////////////////////////////
     -->

    


    <!-- http://iirds.tekom.de/iirds#AdministratorGuide -->

    <owl:NamedIndividual rdf:about="http://iirds.tekom.de/iirds#AdministratorGuide">
        <rdf:type rdf:resource="http://iirds.tekom.de/iirds#DocumentType"/>
        <iirds:Description rdf:datatype="http://www.w3.org/2001/XMLSchema#string">Shall only be assigned to information units of type &quot;Document&quot;</iirds:Description>
        <rdfs:comment xml:lang="en">Type of document. Contains instructions for the administration of a technical system.</rdfs:comment>
        <rdfs:label xml:lang="de">Administrationsanleitung</rdfs:label>
        <rdfs:label xml:lang="en">Administrator guide</rdfs:label>
    </owl:NamedIndividual>
    


    <!-- http://iirds.tekom.de/iirds#Architecture -->

    <owl:NamedIndividual rdf:about="http://iirds.tekom.de/iirds#Architecture">
        <rdf:type rdf:resource="http://iirds.tekom.de/iirds#InformationSubject"/>
        <iirds:Description rdf:datatype="http://www.w3.org/2001/XMLSchema#string">InstanceDescription</iirds:Description>
        <rdfs:label xml:lang="en">Architecture</rdfs:label>
        <rdfs:label xml:lang="de">Architektur</rdfs:label>
    </owl:NamedIndividual>
    


    <!-- http://iirds.tekom.de/iirds#AssemblyInstructions -->

    <owl:NamedIndividual rdf:about="http://iirds.tekom.de/iirds#AssemblyInstructions">
        <rdf:type rdf:resource="http://iirds.tekom.de/iirds#DocumentType"/>
        <iirds:Description rdf:datatype="http://www.w3.org/2001/XMLSchema#string">Shall only be assigned to information units of type &quot;Document&quot;</iirds:Description>
        <rdfs:comment xml:lang="de">Dokumentenart. Enthält Anleitungen, die den Anwender dazu befähigen, ein physisches Produkt so zusammenzubauen, dass es die bestimmungsgemäße Verwendung erfüllt und die Sicherheit und Gesundheit von Personen nicht beeinträchtigt wird.</rdfs:comment>
        <rdfs:comment xml:lang="en">Type of document. Contains instructions enabling the operator to assemble a physical product so that it fulfills its intended use and does not endanger the health and safety of persons.</rdfs:comment>
        <rdfs:label xml:lang="en">Assembly instructions</rdfs:label>
        <rdfs:label xml:lang="de">Montageanleitung</rdfs:label>
    </owl:NamedIndividual>
    


    <!-- http://iirds.tekom.de/iirds#CEDeclarationOfConformity -->

    <owl:NamedIndividual rdf:about="http://iirds.tekom.de/iirds#CEDeclarationOfConformity">
        <rdf:type rdf:resource="http://iirds.tekom.de/iirds#DocumentType"/>
        <iirds:Description rdf:datatype="http://www.w3.org/2001/XMLSchema#string">Shall only be assigned to information units of type &quot;Document&quot;</iirds:Description>
        <rdfs:comment xml:lang="de">Bestätigung des Hersteller (bzw. falls dieser seinen Sitz außerhalb der EU hat, sein Bevollmächtigter mit Sitz in der EU), dass ein von ihm in Verkehr gebrachtes Produkt den grundlegenden Gesundheits- und Sicherheitsanforderungen aller relevanten europäischen Richtlinien entspricht, also mit ihnen konform ist.</rdfs:comment>
        <rdfs:comment xml:lang="en">Type of document. Created as a result of a procedure whereby the manufacture or authorized representative &quot;ensures and declares&quot; that the products concerned satisfy the requirements of the directives that apply to them.</rdfs:comment>
        <rdfs:label xml:lang="en">CE declaration of conformity</rdfs:label>
        <rdfs:label xml:lang="de">CE-Konformitätserklärung</rdfs:label>
    </owl:NamedIndividual>
    


    <!-- http://iirds.tekom.de/iirds#CircuitDiagram -->

    <owl:NamedIndividual rdf:about="http://iirds.tekom.de/iirds#CircuitDiagram">
        <rdf:type rdf:resource="http://iirds.tekom.de/iirds#InformationSubject"/>
        <rdfs:comment xml:lang="en">In Electrical engineering common type of representation for an electric circuit</rdfs:comment>
        <rdfs:label xml:lang="en">Circuit diagram</rdfs:label>
        <rdfs:label xml:lang="de">Schaltplan</rdfs:label>
    </owl:NamedIndividual>
    


    <!-- http://iirds.tekom.de/iirds#CodeSample -->

    <owl:NamedIndividual rdf:about="http://iirds.tekom.de/iirds#CodeSample">
        <rdf:type rdf:resource="http://iirds.tekom.de/iirds#InformationSubject"/>
        <rdfs:label xml:lang="en">Code sample</rdfs:label>
        <rdfs:label xml:lang="de">Codebeispiel</rdfs:label>
    </owl:NamedIndividual>
    


    <!-- http://iirds.tekom.de/iirds#Commissioning -->

    <owl:NamedIndividual rdf:about="http://iirds.tekom.de/iirds#Commissioning">
        <rdf:type rdf:resource="http://iirds.tekom.de/iirds#ProductLifeCyclePhase"/>
        <rdfs:comment xml:lang="en">Life cycle phase of a product containing procedures prior, or related, to the handing over of a product ready for putting into service, including final acceptance testing, the handing over of all documentation relevant to the use of the product and, if necessary, instructing personnel.</rdfs:comment>
        <rdfs:label xml:lang="en">Commissioning</rdfs:label>
        <rdfs:label xml:lang="de">Inbetriebnahme</rdfs:label>
    </owl:NamedIndividual>
    


    <!-- http://iirds.tekom.de/iirds#Concept -->

    <owl:NamedIndividual rdf:about="http://iirds.tekom.de/iirds#Concept">
        <rdf:type rdf:resource="http://iirds.tekom.de/iirds#TopicType"/>
        <iirds:Description rdf:datatype="http://www.w3.org/2001/XMLSchema#string">Conceptual information helps users to map their existing knowledge to tasks and other essential information about a product or system.
Shall only be assigned to information units of type &quot;Topic&quot;.</iirds:Description>
        <rdfs:comment xml:lang="en">Topic type that provides background that helps readers understand essential information about a product, interface, or task.</rdfs:comment>
        <rdfs:label xml:lang="en">Concept</rdfs:label>
        <rdfs:label xml:lang="de">Konzept</rdfs:label>
    </owl:NamedIndividual>
    


    <!-- http://iirds.tekom.de/iirds#ConsumableSupply -->

    <owl:NamedIndividual rdf:about="http://iirds.tekom.de/iirds#ConsumableSupply">
        <rdf:type rdf:resource="http://iirds.tekom.de/iirds#Supplies"/>
        <rdfs:label xml:lang="en">Consumable supply</rdfs:label>
        <rdfs:label xml:lang="de">Verbrauchsmaterial</rdfs:label>
    </owl:NamedIndividual>
    


    <!-- http://iirds.tekom.de/iirds#ContactInformation -->

    <owl:NamedIndividual rdf:about="http://iirds.tekom.de/iirds#ContactInformation">
        <rdf:type rdf:resource="http://iirds.tekom.de/iirds#InformationSubject"/>
        <rdfs:comment xml:lang="en">Data under which someone can come in contact with another person, company, institution or similar</rdfs:comment>
        <rdfs:label xml:lang="en">Contact information</rdfs:label>
        <rdfs:label xml:lang="de">Kontaktdaten</rdfs:label>
    </owl:NamedIndividual>
    


    <!-- http://iirds.tekom.de/iirds#Customization -->

    <owl:NamedIndividual rdf:about="http://iirds.tekom.de/iirds#Customization">
        <rdf:type rdf:resource="http://iirds.tekom.de/iirds#ProductLifeCyclePhase"/>
        <rdfs:comment xml:lang="en">Reworking of a standard product (device or even software) to the special requirements of individual customers.</rdfs:comment>
        <rdfs:label xml:lang="en">Customization</rdfs:label>
        <rdfs:label xml:lang="de">Kundenspezifische Anpassung</rdfs:label>
    </owl:NamedIndividual>
    


    <!-- http://iirds.tekom.de/iirds#DataPrivacy -->

    <owl:NamedIndividual rdf:about="http://iirds.tekom.de/iirds#DataPrivacy">
        <rdf:type rdf:resource="http://iirds.tekom.de/iirds#InformationSubject"/>
        <rdfs:comment xml:lang="en">Protection of individuals against their right to privacy being impaired through the handling of their personal data.</rdfs:comment>
        <rdfs:comment xml:lang="de">Schutz der allgemeinen Persönlichkeitsrechte von natürlichen Personen (Menschen), insbesondere den Anspruch auf Achtung der Privatsphäre, vor einer missbräuchlichen Datenverarbeitung</rdfs:comment>
        <rdfs:label xml:lang="en">Data protection</rdfs:label>
        <rdfs:label xml:lang="de">Datenschutz</rdfs:label>
    </owl:NamedIndividual>
    


    <!-- http://iirds.tekom.de/iirds#Decommissioning -->

    <owl:NamedIndividual rdf:about="http://iirds.tekom.de/iirds#Decommissioning">
        <rdf:type rdf:resource="http://iirds.tekom.de/iirds#ProductLifeCyclePhase"/>
        <rdfs:comment xml:lang="en">Life cycle phase of a product describing the shut-down and transfer into a safe state.</rdfs:comment>
        <rdfs:label xml:lang="de">Außerbetriebnahme</rdfs:label>
        <rdfs:label xml:lang="en">Decommissioning</rdfs:label>
    </owl:NamedIndividual>
    


    <!-- http://iirds.tekom.de/iirds#Design -->

    <owl:NamedIndividual rdf:about="http://iirds.tekom.de/iirds#Design">
        <rdf:type rdf:resource="http://iirds.tekom.de/iirds#ProductLifeCyclePhase"/>
        <rdfs:comment xml:lang="en">Life cycle phase of a product comprising planning and developing the product&apos;s technical design.</rdfs:comment>
        <rdfs:label xml:lang="en">Design</rdfs:label>
        <rdfs:label xml:lang="de">Entwurf</rdfs:label>
    </owl:NamedIndividual>
    


    <!-- http://iirds.tekom.de/iirds#Development -->

    <owl:NamedIndividual rdf:about="http://iirds.tekom.de/iirds#Development">
        <rdf:type rdf:resource="http://iirds.tekom.de/iirds#ProductLifeCyclePhase"/>
        <rdfs:comment xml:lang="en">Life cycle phase of a product progressing from detailed design to prototyping through pilot release to full product launch.</rdfs:comment>
        <rdfs:label xml:lang="en">Development</rdfs:label>
        <rdfs:label xml:lang="de">Entwicklung</rdfs:label>
    </owl:NamedIndividual>
    


    <!-- http://iirds.tekom.de/iirds#Diagnosis -->

    <owl:NamedIndividual rdf:about="http://iirds.tekom.de/iirds#Diagnosis">
        <rdf:type rdf:resource="http://iirds.tekom.de/iirds#ProductLifeCyclePhase"/>
        <rdfs:label xml:lang="de">Diagnose</rdfs:label>
        <rdfs:label xml:lang="en">Diagnosis</rdfs:label>
    </owl:NamedIndividual>
    


    <!-- http://iirds.tekom.de/iirds#Disposal -->

    <owl:NamedIndividual rdf:about="http://iirds.tekom.de/iirds#Disposal">
        <rdf:type rdf:resource="http://iirds.tekom.de/iirds#ProductLifeCyclePhase"/>
        <rdfs:comment xml:lang="en">Life cycle phase of a product describing the elimination of components, mounted parts and lubricant considering the country-specific current law.</rdfs:comment>
        <rdfs:label xml:lang="en">Disposal</rdfs:label>
        <rdfs:label xml:lang="de">Entsorgung</rdfs:label>
    </owl:NamedIndividual>
    


    <!-- http://iirds.tekom.de/iirds#Document -->

    <owl:NamedIndividual rdf:about="http://iirds.tekom.de/iirds#Document"/>
    


    <!-- http://iirds.tekom.de/iirds#DocumentType -->

    <owl:NamedIndividual rdf:about="http://iirds.tekom.de/iirds#DocumentType"/>
    


    <!-- http://iirds.tekom.de/iirds#DocumentationMetadata -->

    <owl:NamedIndividual rdf:about="http://iirds.tekom.de/iirds#DocumentationMetadata"/>
    


    <!-- http://iirds.tekom.de/iirds#DownTime -->

    <owl:NamedIndividual rdf:about="http://iirds.tekom.de/iirds#DownTime">
        <rdf:type rdf:resource="http://iirds.tekom.de/iirds#PlanningTime"/>
        <rdfs:label xml:lang="en">Down time</rdfs:label>
        <rdfs:label xml:lang="de">Stillstandszeit</rdfs:label>
    </owl:NamedIndividual>
    


    <!-- http://iirds.tekom.de/iirds#FAQ -->

    <owl:NamedIndividual rdf:about="http://iirds.tekom.de/iirds#FAQ">
        <rdf:type rdf:resource="http://iirds.tekom.de/iirds#InformationSubject"/>
        <rdfs:label xml:lang="de">FAQ</rdfs:label>
        <rdfs:label xml:lang="en">FAQ</rdfs:label>
    </owl:NamedIndividual>
    


    <!-- http://iirds.tekom.de/iirds#Fragment -->

    <owl:NamedIndividual rdf:about="http://iirds.tekom.de/iirds#Fragment"/>
    


    <!-- http://iirds.tekom.de/iirds#HazardStatement -->

    <owl:NamedIndividual rdf:about="http://iirds.tekom.de/iirds#HazardStatement">
        <rdf:type rdf:resource="http://iirds.tekom.de/iirds#InformationSubject"/>
        <rdfs:label xml:lang="de">Gefahrenhinweis</rdfs:label>
        <rdfs:label xml:lang="en">Hazard statement</rdfs:label>
    </owl:NamedIndividual>
    


    <!-- http://iirds.tekom.de/iirds#InformationType -->

    <owl:NamedIndividual rdf:about="http://iirds.tekom.de/iirds#InformationType"/>
    


    <!-- http://iirds.tekom.de/iirds#InformationUnit -->

    <owl:NamedIndividual rdf:about="http://iirds.tekom.de/iirds#InformationUnit"/>
    


    <!-- http://iirds.tekom.de/iirds#Installation -->

    <owl:NamedIndividual rdf:about="http://iirds.tekom.de/iirds#Installation">
        <rdf:type rdf:resource="http://iirds.tekom.de/iirds#ProductLifeCyclePhase"/>
        <rdfs:comment xml:lang="en">Life cycle phase of a product containing procedures for installing and setting up a software or IT system.</rdfs:comment>
        <rdfs:label xml:lang="de">Installation</rdfs:label>
        <rdfs:label xml:lang="en">Installation</rdfs:label>
    </owl:NamedIndividual>
    


    <!-- http://iirds.tekom.de/iirds#InstallationGuide -->

    <owl:NamedIndividual rdf:about="http://iirds.tekom.de/iirds#InstallationGuide">
        <rdf:type rdf:resource="http://iirds.tekom.de/iirds#DocumentType"/>
        <iirds:Description rdf:datatype="http://www.w3.org/2001/XMLSchema#string">For physical products: Instructions enabling the operator to assemble and electrically connect a physical product so that it does not endanger the health and safety of persons. For IT products: Instructions enabling the administrator to set up and potentially configure a program or new version on a computer so that does not endanger data security. Shall only be assigned to information units of type &quot;Document&quot;.</iirds:Description>
        <rdfs:comment xml:lang="en">Type of document. Contains instructions enabling the operator or administrator to assemble or install a physical product or software so that it fulfills its intended use.</rdfs:comment>
        <rdfs:label xml:lang="en">Installation instructions</rdfs:label>
        <rdfs:label xml:lang="de">Installationsanleitung</rdfs:label>
    </owl:NamedIndividual>
    


    <!-- http://iirds.tekom.de/iirds#Integration -->

    <owl:NamedIndividual rdf:about="http://iirds.tekom.de/iirds#Integration">
        <rdf:type rdf:resource="http://iirds.tekom.de/iirds#ProductLifeCyclePhase"/>
        <rdfs:label xml:lang="de">Integration</rdfs:label>
        <rdfs:label xml:lang="en">Integration</rdfs:label>
    </owl:NamedIndividual>
    


    <!-- http://iirds.tekom.de/iirds#Interface -->

    <owl:NamedIndividual rdf:about="http://iirds.tekom.de/iirds#Interface">
        <rdf:type rdf:resource="http://iirds.tekom.de/iirds#InformationSubject"/>
        <iirds:Description rdf:datatype="http://www.w3.org/2001/XMLSchema#string">As an exchange between SW modules or between different software manufacturers or databases</iirds:Description>
        <rdfs:comment xml:lang="en">Serves the communication between systems, mostly used in software</rdfs:comment>
        <rdfs:label xml:lang="en">Interface</rdfs:label>
        <rdfs:label xml:lang="de">Schnittstelle</rdfs:label>
    </owl:NamedIndividual>
    


    <!-- http://iirds.tekom.de/iirds#Learning -->

    <owl:NamedIndividual rdf:about="http://iirds.tekom.de/iirds#Learning">
        <rdf:type rdf:resource="http://iirds.tekom.de/iirds#TopicType"/>
        <iirds:Description rdf:datatype="http://www.w3.org/2001/XMLSchema#string">Learning content may comprise learning plans, learning objectives, learning content details, summaries, and assessments.
Shall only be assigned to information units of type &quot;Topic&quot;.</iirds:Description>
        <rdfs:comment xml:lang="en">Topic type that provides learning content.</rdfs:comment>
        <rdfs:label xml:lang="en">Learning</rdfs:label>
        <rdfs:label xml:lang="de">Lernen</rdfs:label>
    </owl:NamedIndividual>
    


    <!-- http://iirds.tekom.de/iirds#Licensing -->

    <owl:NamedIndividual rdf:about="http://iirds.tekom.de/iirds#Licensing">
        <rdf:type rdf:resource="http://iirds.tekom.de/iirds#InformationSubject"/>
        <rdfs:label xml:lang="en">Licensing</rdfs:label>
        <rdfs:label xml:lang="de">Lizenzierung</rdfs:label>
    </owl:NamedIndividual>
    


    <!-- http://iirds.tekom.de/iirds#LifecycleSpecification -->

    <owl:NamedIndividual rdf:about="http://iirds.tekom.de/iirds#LifecycleSpecification">
        <rdf:type rdf:resource="http://iirds.tekom.de/iirds#ProductLifeCyclePhase"/>
        <rdfs:comment xml:lang="en">Life cycle phase of a product describing acitivities for defining the requirements on a product or technical system as well as the properties and qualities of the product/system to be built or manufactured.</rdfs:comment>
        <rdfs:label xml:lang="en">Lifecycle Specification</rdfs:label>
        <rdfs:label xml:lang="de">Spezifikation</rdfs:label>
    </owl:NamedIndividual>
    


    <!-- http://iirds.tekom.de/iirds#Lubricant -->

    <owl:NamedIndividual rdf:about="http://iirds.tekom.de/iirds#Lubricant">
        <rdf:type rdf:resource="http://iirds.tekom.de/iirds#Supplies"/>
        <rdfs:label xml:lang="en">Lubricant</rdfs:label>
        <rdfs:label xml:lang="de">Schmierstoff</rdfs:label>
    </owl:NamedIndividual>
    


    <!-- http://iirds.tekom.de/iirds#Maintenance -->

    <owl:NamedIndividual rdf:about="http://iirds.tekom.de/iirds#Maintenance">
        <rdf:type rdf:resource="http://iirds.tekom.de/iirds#ProductLifeCyclePhase"/>
        <iirds:Description rdf:datatype="http://www.w3.org/2001/XMLSchema#string">Maintenance is carried out according to technical rules or manufacturing regulations, e.g. after a certain mileage or duration</iirds:Description>
        <rdfs:comment xml:lang="de">Lebenszyklusphase eines Produkts, in der Maßnahmen ausgeführt werden, die den Sollzustand von technischen Arbeitsmitteln und Anlagen zur Vermeidung von Störungen des Produktionsablaufs bewahren.</rdfs:comment>
        <rdfs:comment xml:lang="en">Life cycle phase of a product containing actions which keep the device in working order or prevent trouble from arising.</rdfs:comment>
        <rdfs:label xml:lang="en">Maintenance</rdfs:label>
        <rdfs:label xml:lang="de">Wartung</rdfs:label>
    </owl:NamedIndividual>
    


    <!-- http://iirds.tekom.de/iirds#MaintenanceInstructions -->

    <owl:NamedIndividual rdf:about="http://iirds.tekom.de/iirds#MaintenanceInstructions">
        <rdf:type rdf:resource="http://iirds.tekom.de/iirds#DocumentType"/>
        <iirds:Description rdf:datatype="http://www.w3.org/2001/XMLSchema#string">Shall only be assigned to information units of type &quot;Document&quot;</iirds:Description>
        <rdfs:comment xml:lang="en">Type of document. Contains instructions for retaining or restoring a piece of equipment, machine, or system to the specified operable condition.</rdfs:comment>
        <rdfs:label xml:lang="en">Maintenance instructions</rdfs:label>
        <rdfs:label xml:lang="de">Wartungsanleitung</rdfs:label>
    </owl:NamedIndividual>
    


    <!-- http://iirds.tekom.de/iirds#MaintenanceInterval -->

    <owl:NamedIndividual rdf:about="http://iirds.tekom.de/iirds#MaintenanceInterval">
        <rdf:type rdf:resource="http://iirds.tekom.de/iirds#PlanningTime"/>
        <rdfs:label xml:lang="en">Maintenance interval</rdfs:label>
        <rdfs:label xml:lang="de">Wartungsintervall</rdfs:label>
    </owl:NamedIndividual>
    


    <!-- http://iirds.tekom.de/iirds#MaintenancePlan -->

    <owl:NamedIndividual rdf:about="http://iirds.tekom.de/iirds#MaintenancePlan">
        <rdf:type rdf:resource="http://iirds.tekom.de/iirds#InformationSubject"/>
        <rdfs:comment xml:lang="en">Timely overview of individual maintenance; What must be done when and in which order</rdfs:comment>
        <rdfs:label xml:lang="en">Maintenance plan</rdfs:label>
        <rdfs:label xml:lang="de">Wartungsplan</rdfs:label>
    </owl:NamedIndividual>
    


    <!-- http://iirds.tekom.de/iirds#OccupationalSafety -->

    <owl:NamedIndividual rdf:about="http://iirds.tekom.de/iirds#OccupationalSafety">
        <rdf:type rdf:resource="http://iirds.tekom.de/iirds#InformationSubject"/>
        <rdfs:comment xml:lang="en">Maintenance of a work environment that is relatively free from actual or potential hazards that can injure employees.</rdfs:comment>
        <rdfs:comment xml:lang="de">Maßnahmen zur Verhütung von Unfällen bei der Arbeit und arbeitsbedingten Gesundheitsgefahren einschließlich Maßnahmen der menschengerechten Gestaltung der Arbeit</rdfs:comment>
        <rdfs:label xml:lang="de">Arbeitsschutz</rdfs:label>
        <rdfs:label xml:lang="en">Occupational safety and health</rdfs:label>
    </owl:NamedIndividual>
    


    <!-- http://iirds.tekom.de/iirds#OperatingInstructions -->

    <owl:NamedIndividual rdf:about="http://iirds.tekom.de/iirds#OperatingInstructions">
        <rdf:type rdf:resource="http://iirds.tekom.de/iirds#DocumentType"/>
        <iirds:Description rdf:datatype="http://www.w3.org/2001/XMLSchema#string">Anleitung, die den Anwender dazu befähigt, ein Gerät, eine Maschine oder eine Software so zu betreiben, dass das Gerät oder die Maschine die bestimmungsgemäße Verwendung erfüllt und die Sicherheit und Gesundheit von Personen nicht beeinträchtigt wird.</iirds:Description>
        <iirds:Description rdf:datatype="http://www.w3.org/2001/XMLSchema#string">The instructions in this document type shall enable the user to operate a device, machine, or software considering the reference use as well as the safety and health regulations for the product. Shall only be assigned to information units of type &quot;Document&quot;.</iirds:Description>
        <rdfs:comment xml:lang="en">Type of document. Contains instructions for operation and use of a technical system.</rdfs:comment>
        <rdfs:label xml:lang="de">Betriebsanleitung</rdfs:label>
        <rdfs:label xml:lang="en">Operation instructions</rdfs:label>
    </owl:NamedIndividual>
    


    <!-- http://iirds.tekom.de/iirds#OperatingSupply -->

    <owl:NamedIndividual rdf:about="http://iirds.tekom.de/iirds#OperatingSupply">
        <rdf:type rdf:resource="http://iirds.tekom.de/iirds#Supplies"/>
        <rdfs:label xml:lang="de">Betriebsstoff</rdfs:label>
        <rdfs:label xml:lang="en">Operating supply</rdfs:label>
    </owl:NamedIndividual>
    


    <!-- http://iirds.tekom.de/iirds#Operation -->

    <owl:NamedIndividual rdf:about="http://iirds.tekom.de/iirds#Operation">
        <rdf:type rdf:resource="http://iirds.tekom.de/iirds#ProductLifeCyclePhase"/>
        <rdfs:comment xml:lang="en">Life cycle phase of a product comprising all technical, administrative and managerial actions, other than maintenance actions, that result in the system being in use</rdfs:comment>
        <rdfs:label xml:lang="de">Betrieb</rdfs:label>
        <rdfs:label xml:lang="en">Operation</rdfs:label>
    </owl:NamedIndividual>
    


    <!-- http://iirds.tekom.de/iirds#Package -->

    <owl:NamedIndividual rdf:about="http://iirds.tekom.de/iirds#Package"/>
    


    <!-- http://iirds.tekom.de/iirds#PartsCatalog -->

    <owl:NamedIndividual rdf:about="http://iirds.tekom.de/iirds#PartsCatalog">
        <rdf:type rdf:resource="http://iirds.tekom.de/iirds#DocumentType"/>
        <rdfs:comment xml:lang="en">Type of document. Contains listings of product names and their part numbers and graphics which are necessary for the aftersales service, but do not include prices or availabilities.</rdfs:comment>
        <rdfs:label xml:lang="en">Parts catalog</rdfs:label>
        <rdfs:label xml:lang="de">Teilekatalog</rdfs:label>
    </owl:NamedIndividual>
    


    <!-- http://iirds.tekom.de/iirds#Planning -->

    <owl:NamedIndividual rdf:about="http://iirds.tekom.de/iirds#Planning">
        <rdf:type rdf:resource="http://iirds.tekom.de/iirds#ProductLifeCyclePhase"/>
        <rdfs:comment xml:lang="en">Life cycle phase of a product containing activities for planning resources, priorities, and time schedules for the development of a product.</rdfs:comment>
        <rdfs:label xml:lang="en">Planning</rdfs:label>
        <rdfs:label xml:lang="de">Planung</rdfs:label>
    </owl:NamedIndividual>
    


    <!-- http://iirds.tekom.de/iirds#Product -->

    <owl:NamedIndividual rdf:about="http://iirds.tekom.de/iirds#Product"/>
    


    <!-- http://iirds.tekom.de/iirds#QuickGuide -->

    <owl:NamedIndividual rdf:about="http://iirds.tekom.de/iirds#QuickGuide">
        <rdf:type rdf:resource="http://iirds.tekom.de/iirds#DocumentType"/>
        <iirds:Description rdf:datatype="http://www.w3.org/2001/XMLSchema#string">Shall only be assigned to information units of type &quot;Document&quot;</iirds:Description>
        <rdfs:comment xml:lang="en">Type of document. Describes a short document that contains selected instructions for a specific user group or purpose.</rdfs:comment>
        <rdfs:label xml:lang="de">Kurzanleitung</rdfs:label>
        <rdfs:label xml:lang="en">Quick guide</rdfs:label>
    </owl:NamedIndividual>
    


    <!-- http://iirds.tekom.de/iirds#Reference -->

    <owl:NamedIndividual rdf:about="http://iirds.tekom.de/iirds#Reference">
        <rdf:type rdf:resource="http://iirds.tekom.de/iirds#TopicType"/>
        <iirds:Description rdf:datatype="http://www.w3.org/2001/XMLSchema#string">Examples are parameter lists, tables with technical data, UI control overviews, and parts lists. 
Shall only be assigned to information units of type &quot;Topic&quot;.</iirds:Description>
        <rdfs:comment xml:lang="en">Topic type that contains information that supports users as they perform a task, meaning data that is looked up rather than memorized.</rdfs:comment>
        <rdfs:label xml:lang="en">Reference</rdfs:label>
        <rdfs:label xml:lang="de">Referenz</rdfs:label>
    </owl:NamedIndividual>
    


    <!-- http://iirds.tekom.de/iirds#Repair -->

    <owl:NamedIndividual rdf:about="http://iirds.tekom.de/iirds#Repair">
        <rdf:type rdf:resource="http://iirds.tekom.de/iirds#ProductLifeCyclePhase"/>
        <rdfs:comment xml:lang="en">Life cycle phase of a product that describes activities for restoring the product to a working and sound condition after damage or wear and tear.</rdfs:comment>
        <rdfs:label xml:lang="en">Repair</rdfs:label>
        <rdfs:label xml:lang="de">Reparatur</rdfs:label>
    </owl:NamedIndividual>
    


    <!-- http://iirds.tekom.de/iirds#RepairInstructions -->

    <owl:NamedIndividual rdf:about="http://iirds.tekom.de/iirds#RepairInstructions">
        <rdf:type rdf:resource="http://iirds.tekom.de/iirds#DocumentType"/>
        <iirds:Description rdf:datatype="http://www.w3.org/2001/XMLSchema#string">Anleitung, die den Anwender dazu befähigt, ein Gerät oder eine Maschine so instandzusetzen, dass das Gerät oder die Maschine die bestimmungsgemäße Verwendung erfüllt und die Sicherheit und Gesundheit von Personen nicht beeinträchtigt wird.</iirds:Description>
        <iirds:Description rdf:datatype="http://www.w3.org/2001/XMLSchema#string">The instructions in this document type shall enable the user to repair a device, machine, or system considering the reference use as well as the safety and health regulations for the product. Shall only be assigned to information units of type &quot;Document&quot;</iirds:Description>
        <rdfs:comment xml:lang="en">Type of document. Contains instructions for restoring a product to a working condition.</rdfs:comment>
        <rdfs:label xml:lang="en">Repair instructions</rdfs:label>
        <rdfs:label xml:lang="de">Reparaturanleitung</rdfs:label>
    </owl:NamedIndividual>
    


    <!-- http://iirds.tekom.de/iirds#Safety -->

    <owl:NamedIndividual rdf:about="http://iirds.tekom.de/iirds#Safety">
        <rdf:type rdf:resource="http://iirds.tekom.de/iirds#ProductLifeCyclePhase"/>
        <iirds:Description rdf:datatype="http://www.w3.org/2001/XMLSchema#string">Applies primarily to equipment / machines. Users should be able to work safely with the products (without injuries)</iirds:Description>
        <rdfs:comment xml:lang="en">Safety is a condition in which there are no unacceptable risks or which is free of hazards</rdfs:comment>
        <rdfs:label xml:lang="en">Safety</rdfs:label>
        <rdfs:label xml:lang="de">Sicherheit</rdfs:label>
    </owl:NamedIndividual>
    


    <!-- http://iirds.tekom.de/iirds#SalesCatalog -->

    <owl:NamedIndividual rdf:about="http://iirds.tekom.de/iirds#SalesCatalog">
        <rdf:type rdf:resource="http://iirds.tekom.de/iirds#DocumentType"/>
        <iirds:Description rdf:datatype="http://www.w3.org/2001/XMLSchema#string">Shall only be assigned to information units of type &quot;Document&quot;</iirds:Description>
        <rdfs:comment xml:lang="en">Type of document. Contains listings of available products of a producing company with consumers as the target group.</rdfs:comment>
        <rdfs:label xml:lang="en">Sales catalog</rdfs:label>
        <rdfs:label xml:lang="de">Verkaufskatalog</rdfs:label>
    </owl:NamedIndividual>
    


    <!-- http://iirds.tekom.de/iirds#ScopeOfSupply -->

    <owl:NamedIndividual rdf:about="http://iirds.tekom.de/iirds#ScopeOfSupply">
        <rdf:type rdf:resource="http://iirds.tekom.de/iirds#InformationSubject"/>
        <iirds:Description rdf:datatype="http://www.w3.org/2001/XMLSchema#string">Applies to product &amp; software</iirds:Description>
        <rdfs:comment xml:lang="en">Overview of all parts of the entire (supplied) system</rdfs:comment>
        <rdfs:label xml:lang="de">Lieferumfang</rdfs:label>
        <rdfs:label xml:lang="en">Scope of supply</rdfs:label>
    </owl:NamedIndividual>
    


    <!-- http://iirds.tekom.de/iirds#SetupTime -->

    <owl:NamedIndividual rdf:about="http://iirds.tekom.de/iirds#SetupTime">
        <rdf:type rdf:resource="http://iirds.tekom.de/iirds#PlanningTime"/>
        <rdfs:label xml:lang="de">Rüstzeit</rdfs:label>
        <rdfs:label xml:lang="en">Set-up time</rdfs:label>
    </owl:NamedIndividual>
    


    <!-- http://iirds.tekom.de/iirds#SparePart -->

    <owl:NamedIndividual rdf:about="http://iirds.tekom.de/iirds#SparePart">
        <rdf:type rdf:resource="http://iirds.tekom.de/iirds#Supplies"/>
        <rdfs:label xml:lang="de">Ersatzteil</rdfs:label>
        <rdfs:label xml:lang="en">Spare part</rdfs:label>
    </owl:NamedIndividual>
    


    <!-- http://iirds.tekom.de/iirds#Specification -->

    <owl:NamedIndividual rdf:about="http://iirds.tekom.de/iirds#Specification">
        <rdf:type rdf:resource="http://iirds.tekom.de/iirds#DocumentType"/>
        <iirds:Description rdf:datatype="http://www.w3.org/2001/XMLSchema#string">Shall only be assigned to information units of type &quot;Document&quot;</iirds:Description>
        <rdfs:comment xml:lang="en">Type of document. Contains requirements and/or statements describing properties and qualities of a product to be built or manufactured.</rdfs:comment>
        <rdfs:label xml:lang="en">Specification</rdfs:label>
        <rdfs:label xml:lang="de">Spezifikation</rdfs:label>
    </owl:NamedIndividual>
    


    <!-- http://iirds.tekom.de/iirds#Storage -->

    <owl:NamedIndividual rdf:about="http://iirds.tekom.de/iirds#Storage">
        <rdf:type rdf:resource="http://iirds.tekom.de/iirds#ProductLifeCyclePhase"/>
        <rdfs:comment xml:lang="en">Life cycle phase of a product that describes the process of keeping physical products available or in an adequate environment in order to tide over the time between arrival and use.</rdfs:comment>
        <rdfs:label xml:lang="de">Lagerung</rdfs:label>
        <rdfs:label xml:lang="en">Storage</rdfs:label>
    </owl:NamedIndividual>
    


    <!-- http://iirds.tekom.de/iirds#Task -->

    <owl:NamedIndividual rdf:about="http://iirds.tekom.de/iirds#Task">
        <rdf:type rdf:resource="http://iirds.tekom.de/iirds#TopicType"/>
        <iirds:Description rdf:datatype="http://www.w3.org/2001/XMLSchema#string">Tasks provide instructions and may contain information on other aspects, such as requirements that must be fulfilled or safety instructions.
Shall only be assigned to information units of type &quot;Topic&quot;.</iirds:Description>
        <rdfs:comment xml:lang="en">Topic type that contains procedural information for work activities.</rdfs:comment>
        <rdfs:label xml:lang="de">Aufgabe</rdfs:label>
        <rdfs:label xml:lang="en">Task</rdfs:label>
    </owl:NamedIndividual>
    


    <!-- http://iirds.tekom.de/iirds#TechnicalData -->

    <owl:NamedIndividual rdf:about="http://iirds.tekom.de/iirds#TechnicalData">
        <rdf:type rdf:resource="http://iirds.tekom.de/iirds#InformationSubject"/>
        <rdfs:label xml:lang="en">Technical data</rdfs:label>
        <rdfs:label xml:lang="de">Technische Daten</rdfs:label>
    </owl:NamedIndividual>
    


    <!-- http://iirds.tekom.de/iirds#Tool -->

    <owl:NamedIndividual rdf:about="http://iirds.tekom.de/iirds#Tool">
        <rdf:type rdf:resource="http://iirds.tekom.de/iirds#Supplies"/>
        <rdfs:label xml:lang="en">Tool</rdfs:label>
        <rdfs:label xml:lang="de">Werkzeug</rdfs:label>
    </owl:NamedIndividual>
    


    <!-- http://iirds.tekom.de/iirds#Topic -->

    <owl:NamedIndividual rdf:about="http://iirds.tekom.de/iirds#Topic"/>
    


    <!-- http://iirds.tekom.de/iirds#TopicType -->

    <owl:NamedIndividual rdf:about="http://iirds.tekom.de/iirds#TopicType"/>
    


    <!-- http://iirds.tekom.de/iirds#Transport -->

    <owl:NamedIndividual rdf:about="http://iirds.tekom.de/iirds#Transport">
        <rdf:type rdf:resource="http://iirds.tekom.de/iirds#ProductLifeCyclePhase"/>
        <rdfs:comment xml:lang="en">Life cycle phase of a product that describes activities for moving or conveying the product from one place to another.</rdfs:comment>
        <rdfs:label xml:lang="de">Transport</rdfs:label>
        <rdfs:label xml:lang="en">Transport</rdfs:label>
    </owl:NamedIndividual>
    


    <!-- http://iirds.tekom.de/iirds#TransportInstructions -->

    <owl:NamedIndividual rdf:about="http://iirds.tekom.de/iirds#TransportInstructions">
        <rdf:type rdf:resource="http://iirds.tekom.de/iirds#DocumentType"/>
        <iirds:Description rdf:datatype="http://www.w3.org/2001/XMLSchema#string">Shall only be assigned to information units of type &quot;Document&quot;</iirds:Description>
        <rdfs:comment xml:lang="en">Type of document. Contains instructions for transporting the product or its components from one place to another.</rdfs:comment>
        <rdfs:label xml:lang="en">Transport instructions</rdfs:label>
        <rdfs:label xml:lang="de">Transportanleitung</rdfs:label>
    </owl:NamedIndividual>
    


    <!-- http://iirds.tekom.de/iirds#Troubleshooting -->

    <owl:NamedIndividual rdf:about="http://iirds.tekom.de/iirds#Troubleshooting">
        <rdf:type rdf:resource="http://iirds.tekom.de/iirds#TopicType"/>
        <rdfs:comment xml:lang="en">Eliminate a fault by means of appropriate remedial measures</rdfs:comment>
        <rdfs:label xml:lang="de">Störungsbeseitigung</rdfs:label>
        <rdfs:label xml:lang="en">Troubleshooting</rdfs:label>
    </owl:NamedIndividual>
    


    <!-- http://iirds.tekom.de/iirds#Warranty -->

    <owl:NamedIndividual rdf:about="http://iirds.tekom.de/iirds#Warranty">
        <rdf:type rdf:resource="http://iirds.tekom.de/iirds#ProductLifeCyclePhase"/>
        <iirds:Description rdf:datatype="http://www.w3.org/2001/XMLSchema#string">(Written) assurance by the manufacturer that he will be responsible for the cost of remedying defects for a certain period after the purchase of a product.</iirds:Description>
        <rdfs:comment xml:lang="en">Assurance of functionality (usually of products, consumer goods) for a defined time</rdfs:comment>
        <rdfs:label xml:lang="de">Garantie</rdfs:label>
        <rdfs:label xml:lang="en">Warranty</rdfs:label>
    </owl:NamedIndividual>
    


    <!-- http://iirds.tekom.de/iirds#WhatsNew -->

    <owl:NamedIndividual rdf:about="http://iirds.tekom.de/iirds#WhatsNew">
        <rdf:type rdf:resource="http://iirds.tekom.de/iirds#InformationSubject"/>
        <rdfs:label xml:lang="en">What&apos;s new</rdfs:label>
        <rdfs:label xml:lang="de">Änderungen</rdfs:label>
    </owl:NamedIndividual>
    


    <!-- http://iirds.tekom.de/iirds#WorkingTime -->

    <owl:NamedIndividual rdf:about="http://iirds.tekom.de/iirds#WorkingTime">
        <rdf:type rdf:resource="http://iirds.tekom.de/iirds#PlanningTime"/>
        <rdfs:label xml:lang="de">Arbeitszeit</rdfs:label>
        <rdfs:label xml:lang="en">Working time</rdfs:label>
    </owl:NamedIndividual>
    


    <!-- http://iirds.tekom.de/iirds#has-contributor -->

    <owl:NamedIndividual rdf:about="http://iirds.tekom.de/iirds#has-contributor"/>
    


    <!-- http://iirds.tekom.de/iirds#has-document-type -->

    <owl:NamedIndividual rdf:about="http://iirds.tekom.de/iirds#has-document-type"/>
    


    <!-- http://iirds.tekom.de/iirds#has-information-type -->

    <owl:NamedIndividual rdf:about="http://iirds.tekom.de/iirds#has-information-type"/>
    


    <!-- http://iirds.tekom.de/iirds#has-topic-type -->

    <owl:NamedIndividual rdf:about="http://iirds.tekom.de/iirds#has-topic-type"/>
    


    <!-- http://iirds.tekom.de/iirds#has-version -->

    <owl:NamedIndividual rdf:about="http://iirds.tekom.de/iirds#has-version"/>
    


    <!-- http://iirds.tekom.de/iirds#is-version-of -->

    <owl:NamedIndividual rdf:about="http://iirds.tekom.de/iirds#is-version-of"/>
    


    <!-- http://people.aifb.kit.edu/mu2771/step#A4 -->

    <owl:NamedIndividual rdf:about="http://people.aifb.kit.edu/mu2771/step#A4">
        <rdf:type rdf:resource="http://purl.org/dc/terms/SizeOrDuration"/>
        <dc:creator rdf:resource="http://www.aifb.kit.edu/web/Sebastian_Bader"/>
        <rdfs:label xml:lang="de">A4</rdfs:label>
        <rdfs:label xml:lang="en">A4</rdfs:label>
    </owl:NamedIndividual>
    


    <!-- http://people.aifb.kit.edu/mu2771/step#AIFB -->

    <owl:NamedIndividual rdf:about="http://people.aifb.kit.edu/mu2771/step#AIFB">
        <rdf:type rdf:resource="http://www.w3.org/ns/org#FormalOrganization"/>
        <rdfs:label xml:lang="de">AIFB GmbH und Ko. KG</rdfs:label>
    </owl:NamedIndividual>
    


    <!-- http://people.aifb.kit.edu/mu2771/step#AVXTechnology -->

    <owl:NamedIndividual rdf:about="http://people.aifb.kit.edu/mu2771/step#AVXTechnology">
        <rdf:type rdf:resource="http://www.w3.org/ns/org#FormalOrganization"/>
        <rdfs:label xml:lang="en">AVX Technology</rdfs:label>
    </owl:NamedIndividual>
    


    <!-- http://people.aifb.kit.edu/mu2771/step#B0-B4-48-BF-B4-82 -->

    <owl:NamedIndividual rdf:about="http://people.aifb.kit.edu/mu2771/step#B0-B4-48-BF-B4-82">
        <rdf:type rdf:resource="http://purl.oclc.org/NET/ssnx/ssn#SensingDevice"/>
        <rdfs:comment xml:lang="en">A Texas Instrument sensor of type CC2650</rdfs:comment>
        <rdfs:label>B0:B4:48:BF:B4:82</rdfs:label>
    </owl:NamedIndividual>
    


    <!-- http://people.aifb.kit.edu/mu2771/step#BlechGmbH -->

    <owl:NamedIndividual rdf:about="http://people.aifb.kit.edu/mu2771/step#BlechGmbH">
        <rdf:type rdf:resource="http://www.w3.org/ns/org#FormalOrganization"/>
        <rdfs:label xml:lang="de">Blech GmbH</rdfs:label>
    </owl:NamedIndividual>
    


    <!-- http://people.aifb.kit.edu/mu2771/step#CeramStahl -->

    <owl:NamedIndividual rdf:about="http://people.aifb.kit.edu/mu2771/step#CeramStahl">
        <rdf:type rdf:resource="http://www.w3.org/ns/org#FormalOrganization"/>
        <rdfs:label xml:lang="de">CeramStahl</rdfs:label>
    </owl:NamedIndividual>
    


    <!-- http://people.aifb.kit.edu/mu2771/step#Customer1 -->

    <owl:NamedIndividual rdf:about="http://people.aifb.kit.edu/mu2771/step#Customer1">
        <rdf:type rdf:resource="http://www.w3.org/ns/org#FormalOrganization"/>
        <rdfs:label xml:lang="en">Customer no 1</rdfs:label>
        <rdfs:label xml:lang="de">Kunde Nr. 1</rdfs:label>
    </owl:NamedIndividual>
    


    <!-- http://people.aifb.kit.edu/mu2771/step#Ditzingen -->

    <owl:NamedIndividual rdf:about="http://people.aifb.kit.edu/mu2771/step#Ditzingen">
        <rdf:type rdf:resource="http://www.w3.org/2003/01/geo/wgs84_pos#SpatialThing"/>
        <rdfs:label xml:lang="de">Ditzingen</rdfs:label>
    </owl:NamedIndividual>
    


    <!-- http://people.aifb.kit.edu/mu2771/step#Esslingen -->

    <owl:NamedIndividual rdf:about="http://people.aifb.kit.edu/mu2771/step#Esslingen">
        <rdf:type rdf:resource="http://www.w3.org/2003/01/geo/wgs84_pos#SpatialThing"/>
        <rdfs:label xml:lang="de">Esslingen</rdfs:label>
    </owl:NamedIndividual>
    


    <!-- http://people.aifb.kit.edu/mu2771/step#Fall1 -->

    <owl:NamedIndividual rdf:about="http://people.aifb.kit.edu/mu2771/step#Fall1">
        <rdf:type rdf:resource="http://people.aifb.kit.edu/mu2771/step#NewWorkOrder"/>
        <step:level rdf:datatype="http://www.w3.org/2001/XMLSchema#int">2</step:level>
        <step:probability rdf:datatype="http://www.w3.org/2001/XMLSchema#double">1.0</step:probability>
        <rdfs:comment>a dummy event which requires some action by a random technician</rdfs:comment>
        <rdfs:label xml:lang="de">Servicefall Nummer 1</rdfs:label>
        <rdfs:label xml:lang="en">Ticket no. 1</rdfs:label>
    </owl:NamedIndividual>
    


    <!-- http://people.aifb.kit.edu/mu2771/step#Garage -->

    <owl:NamedIndividual rdf:about="http://people.aifb.kit.edu/mu2771/step#Garage">
        <rdf:type rdf:resource="http://www.w3.org/ns/org#Site"/>
        <rdfs:label xml:lang="en">Mario&apos;s garage</rdfs:label>
        <rdfs:label xml:lang="de">Marios Garage</rdfs:label>
    </owl:NamedIndividual>
    


    <!-- http://people.aifb.kit.edu/mu2771/step#Groundskeeping -->

    <owl:NamedIndividual rdf:about="http://people.aifb.kit.edu/mu2771/step#Groundskeeping">
        <rdf:type rdf:resource="http://people.aifb.kit.edu/mu2771/step#Expertise"/>
        <step:level rdf:datatype="http://www.w3.org/2001/XMLSchema#integer">4</step:level>
    </owl:NamedIndividual>
    


    <!-- http://people.aifb.kit.edu/mu2771/step#Gustav_Gans -->

    <owl:NamedIndividual rdf:about="http://people.aifb.kit.edu/mu2771/step#Gustav_Gans">
        <rdf:type rdf:resource="http://people.aifb.kit.edu/mu2771/step#Technician"/>
        <rdfs:label xml:lang="de">Gustav Gans</rdfs:label>
    </owl:NamedIndividual>
    


    <!-- http://people.aifb.kit.edu/mu2771/step#HansaVerlagsgruppe -->

    <owl:NamedIndividual rdf:about="http://people.aifb.kit.edu/mu2771/step#HansaVerlagsgruppe">
        <rdf:type rdf:resource="http://www.w3.org/ns/org#FormalOrganization"/>
        <rdfs:label xml:lang="de">Hansa Verlagsgruppe</rdfs:label>
    </owl:NamedIndividual>
    


    <!-- http://people.aifb.kit.edu/mu2771/step#Heidenheim -->

    <owl:NamedIndividual rdf:about="http://people.aifb.kit.edu/mu2771/step#Heidenheim">
        <rdf:type rdf:resource="http://www.w3.org/2003/01/geo/wgs84_pos#SpatialThing"/>
        <rdfs:label xml:lang="de">Heidenheim</rdfs:label>
    </owl:NamedIndividual>
    


    <!-- http://people.aifb.kit.edu/mu2771/step#HeinzMueller -->

    <owl:NamedIndividual rdf:about="http://people.aifb.kit.edu/mu2771/step#HeinzMueller">
        <rdf:type rdf:resource="http://people.aifb.kit.edu/mu2771/step#Technician"/>
        <rdfs:label xml:lang="de">Heinz Müller</rdfs:label>
    </owl:NamedIndividual>
    


    <!-- http://people.aifb.kit.edu/mu2771/step#HenrikMueller -->

    <owl:NamedIndividual rdf:about="http://people.aifb.kit.edu/mu2771/step#HenrikMueller">
        <rdf:type rdf:resource="http://people.aifb.kit.edu/mu2771/step#Technician"/>
        <rdfs:label xml:lang="de">Henrik Müller</rdfs:label>
    </owl:NamedIndividual>
    


    <!-- http://people.aifb.kit.edu/mu2771/step#Herbert_Feuerstein -->

    <owl:NamedIndividual rdf:about="http://people.aifb.kit.edu/mu2771/step#Herbert_Feuerstein">
        <rdf:type rdf:resource="http://people.aifb.kit.edu/mu2771/step#Technician"/>
        <rdfs:label xml:lang="de">Herbert Feuerstein</rdfs:label>
    </owl:NamedIndividual>
    


    <!-- http://people.aifb.kit.edu/mu2771/step#HäfeleAG -->

    <owl:NamedIndividual rdf:about="http://people.aifb.kit.edu/mu2771/step#HäfeleAG">
        <rdf:type rdf:resource="http://www.w3.org/ns/org#FormalOrganization"/>
        <rdfs:label xml:lang="de">Häfele</rdfs:label>
    </owl:NamedIndividual>
    


    <!-- http://people.aifb.kit.edu/mu2771/step#JuergenTKork -->

    <owl:NamedIndividual rdf:about="http://people.aifb.kit.edu/mu2771/step#JuergenTKork">
        <rdf:type rdf:resource="http://people.aifb.kit.edu/mu2771/step#Technician"/>
        <rdfs:label xml:lang="de">Jürgen T. Kork</rdfs:label>
    </owl:NamedIndividual>
    


    <!-- http://people.aifb.kit.edu/mu2771/step#KIT000012 -->

    <owl:NamedIndividual rdf:about="http://people.aifb.kit.edu/mu2771/step#KIT000012">
        <rdf:type rdf:resource="http://people.aifb.kit.edu/mu2771/step#Alarm"/>
        <rdfs:label xml:lang="de">Alarmcode 12</rdfs:label>
        <rdfs:label xml:lang="en">KIT000012</rdfs:label>
        <rdfs:label xml:lang="en">alarm code 12</rdfs:label>
    </owl:NamedIndividual>
    


    <!-- http://people.aifb.kit.edu/mu2771/step#KIT000088 -->

    <owl:NamedIndividual rdf:about="http://people.aifb.kit.edu/mu2771/step#KIT000088">
        <rdf:type rdf:resource="http://people.aifb.kit.edu/mu2771/step#Alarm"/>
        <rdfs:label xml:lang="de">Alarmcode 88</rdfs:label>
        <rdfs:label xml:lang="en">KIT000088</rdfs:label>
        <rdfs:label xml:lang="en">alarm code 88</rdfs:label>
    </owl:NamedIndividual>
    


    <!-- http://people.aifb.kit.edu/mu2771/step#KITE00034 -->

    <owl:NamedIndividual rdf:about="http://people.aifb.kit.edu/mu2771/step#KITE00034">
        <rdf:type rdf:resource="http://people.aifb.kit.edu/mu2771/step#ElectronicMessage"/>
        <rdfs:label xml:lang="de">Elektronischer Fehlercode 34</rdfs:label>
        <rdfs:label xml:lang="en">KITE00034</rdfs:label>
        <rdfs:label xml:lang="en">electronic error code 34</rdfs:label>
    </owl:NamedIndividual>
    


    <!-- http://people.aifb.kit.edu/mu2771/step#KITE00046 -->

    <owl:NamedIndividual rdf:about="http://people.aifb.kit.edu/mu2771/step#KITE00046">
        <rdf:type rdf:resource="http://people.aifb.kit.edu/mu2771/step#ElectronicMessage"/>
        <rdfs:label xml:lang="de">Elektronischer Fehlercode 46</rdfs:label>
        <rdfs:label xml:lang="en">KITE00046</rdfs:label>
        <rdfs:label xml:lang="en">electronic error code 46</rdfs:label>
    </owl:NamedIndividual>
    


    <!-- http://people.aifb.kit.edu/mu2771/step#KITE00075 -->

    <owl:NamedIndividual rdf:about="http://people.aifb.kit.edu/mu2771/step#KITE00075">
        <rdf:type rdf:resource="http://people.aifb.kit.edu/mu2771/step#ElectronicMessage"/>
        <rdfs:label xml:lang="de">Elektronischer Fehlercode 75</rdfs:label>
        <rdfs:label xml:lang="en">KITE00075</rdfs:label>
        <rdfs:label xml:lang="en">electronic error code 75</rdfs:label>
    </owl:NamedIndividual>
    


    <!-- http://people.aifb.kit.edu/mu2771/step#KITP00043 -->

    <owl:NamedIndividual rdf:about="http://people.aifb.kit.edu/mu2771/step#KITP00043">
        <rdf:type rdf:resource="http://people.aifb.kit.edu/mu2771/step#Prediction"/>
        <rdfs:label xml:lang="en">KITP00043</rdfs:label>
        <rdfs:label xml:lang="en">predictive message code 43</rdfs:label>
        <rdfs:label xml:lang="de">prädiktive Fehlermeldung 43</rdfs:label>
    </owl:NamedIndividual>
    


    <!-- http://people.aifb.kit.edu/mu2771/step#KITP00142 -->

    <owl:NamedIndividual rdf:about="http://people.aifb.kit.edu/mu2771/step#KITP00142">
        <rdf:type rdf:resource="http://people.aifb.kit.edu/mu2771/step#Prediction"/>
        <rdfs:label xml:lang="en">KITP00142</rdfs:label>
        <rdfs:label xml:lang="en">predictive message code 142</rdfs:label>
        <rdfs:label xml:lang="de">prädiktive Fehlermeldung 142</rdfs:label>
    </owl:NamedIndividual>
    


    <!-- http://people.aifb.kit.edu/mu2771/step#KITP00304 -->

    <owl:NamedIndividual rdf:about="http://people.aifb.kit.edu/mu2771/step#KITP00304">
        <rdf:type rdf:resource="http://people.aifb.kit.edu/mu2771/step#Prediction"/>
        <rdfs:label xml:lang="en">KITP00304</rdfs:label>
        <rdfs:label xml:lang="en">predictive message code 304</rdfs:label>
        <rdfs:label xml:lang="de">prädiktive Fehlermeldung 304</rdfs:label>
    </owl:NamedIndividual>
    


    <!-- http://people.aifb.kit.edu/mu2771/step#KITP00764 -->

    <owl:NamedIndividual rdf:about="http://people.aifb.kit.edu/mu2771/step#KITP00764">
        <rdf:type rdf:resource="http://people.aifb.kit.edu/mu2771/step#Prediction"/>
        <rdfs:label xml:lang="en">KITP00764</rdfs:label>
        <rdfs:label xml:lang="en">predictive message code 764</rdfs:label>
        <rdfs:label xml:lang="de">prädiktive Fehlermeldung 764</rdfs:label>
    </owl:NamedIndividual>
    


    <!-- http://people.aifb.kit.edu/mu2771/step#KSRI -->

    <owl:NamedIndividual rdf:about="http://people.aifb.kit.edu/mu2771/step#KSRI">
        <rdf:type rdf:resource="http://www.w3.org/ns/org#FormalOrganization"/>
        <rdfs:label xml:lang="de">KSRI</rdfs:label>
        <rdfs:label xml:lang="en">Karlsruhe Service Research Insitute</rdfs:label>
    </owl:NamedIndividual>
    


    <!-- http://people.aifb.kit.edu/mu2771/step#Karlsruhe -->

    <owl:NamedIndividual rdf:about="http://people.aifb.kit.edu/mu2771/step#Karlsruhe">
        <rdf:type rdf:resource="http://www.w3.org/2003/01/geo/wgs84_pos#SpatialThing"/>
        <rdfs:label xml:lang="de">Karlsruhe</rdfs:label>
    </owl:NamedIndividual>
    


    <!-- http://people.aifb.kit.edu/mu2771/step#Konstanz -->

    <owl:NamedIndividual rdf:about="http://people.aifb.kit.edu/mu2771/step#Konstanz">
        <rdf:type rdf:resource="http://www.w3.org/2003/01/geo/wgs84_pos#SpatialThing"/>
        <rdfs:label xml:lang="de">Konstanz</rdfs:label>
    </owl:NamedIndividual>
    


    <!-- http://people.aifb.kit.edu/mu2771/step#MaierAG -->

    <owl:NamedIndividual rdf:about="http://people.aifb.kit.edu/mu2771/step#MaierAG">
        <rdf:type rdf:resource="http://www.w3.org/ns/org#FormalOrganization"/>
        <rdfs:label xml:lang="de">Maier AG</rdfs:label>
    </owl:NamedIndividual>
    


    <!-- http://people.aifb.kit.edu/mu2771/step#MaintainanceCompany -->

    <owl:NamedIndividual rdf:about="http://people.aifb.kit.edu/mu2771/step#MaintainanceCompany">
        <rdf:type rdf:resource="http://www.w3.org/ns/org#FormalOrganization"/>
        <rdfs:label xml:lang="de">Wartungsanbieter</rdfs:label>
        <rdfs:label xml:lang="en">maintenance provider</rdfs:label>
    </owl:NamedIndividual>
    


    <!-- http://people.aifb.kit.edu/mu2771/step#MaintanencePlan -->

    <owl:NamedIndividual rdf:about="http://people.aifb.kit.edu/mu2771/step#MaintanencePlan">
        <rdf:type rdf:resource="http://iirds.tekom.de/iirds#TopicType"/>
        <rdfs:label xml:lang="de">Wartungsplan</rdfs:label>
        <rdfs:label xml:lang="en">maintanence plan</rdfs:label>
    </owl:NamedIndividual>
    


    <!-- http://people.aifb.kit.edu/mu2771/step#MaintenanceIntervall -->

    <owl:NamedIndividual rdf:about="http://people.aifb.kit.edu/mu2771/step#MaintenanceIntervall">
        <rdf:type rdf:resource="http://iirds.tekom.de/iirds#TopicType"/>
        <rdfs:label xml:lang="de">Wartungsintervall</rdfs:label>
        <rdfs:label xml:lang="en">maintenance intervall</rdfs:label>
    </owl:NamedIndividual>
    


    <!-- http://people.aifb.kit.edu/mu2771/step#Malte_Frisch -->

    <owl:NamedIndividual rdf:about="http://people.aifb.kit.edu/mu2771/step#Malte_Frisch">
        <rdf:type rdf:resource="http://people.aifb.kit.edu/mu2771/step#Technician"/>
        <rdfs:label xml:lang="de">Malte Frisch</rdfs:label>
    </owl:NamedIndividual>
    


    <!-- http://people.aifb.kit.edu/mu2771/step#MaxMustermann -->

    <owl:NamedIndividual rdf:about="http://people.aifb.kit.edu/mu2771/step#MaxMustermann">
        <rdf:type rdf:resource="http://people.aifb.kit.edu/mu2771/step#Technician"/>
        <rdfs:label rdf:datatype="http://www.w3.org/2001/XMLSchema#string">Max Mustermann</rdfs:label>
        <foaf:name rdf:datatype="http://www.w3.org/2001/XMLSchema#string">Max Mustermann</foaf:name>
    </owl:NamedIndividual>
    


    <!-- http://people.aifb.kit.edu/mu2771/step#Michael_Wolff -->

    <owl:NamedIndividual rdf:about="http://people.aifb.kit.edu/mu2771/step#Michael_Wolff">
        <rdf:type rdf:resource="http://people.aifb.kit.edu/mu2771/step#Technician"/>
        <rdfs:label xml:lang="de">Michael Wolff</rdfs:label>
    </owl:NamedIndividual>
    


    <!-- http://people.aifb.kit.edu/mu2771/step#Micheal_Mann -->

    <owl:NamedIndividual rdf:about="http://people.aifb.kit.edu/mu2771/step#Micheal_Mann">
        <rdf:type rdf:resource="http://people.aifb.kit.edu/mu2771/step#Technician"/>
        <rdfs:label xml:lang="de">Micheal Mann</rdfs:label>
    </owl:NamedIndividual>
    


    <!-- http://people.aifb.kit.edu/mu2771/step#Munich -->

    <owl:NamedIndividual rdf:about="http://people.aifb.kit.edu/mu2771/step#Munich">
        <rdf:type rdf:resource="http://www.w3.org/2003/01/geo/wgs84_pos#SpatialThing"/>
        <rdfs:label xml:lang="de">Munich</rdfs:label>
        <rdfs:label xml:lang="de">München</rdfs:label>
    </owl:NamedIndividual>
    


    <!-- http://people.aifb.kit.edu/mu2771/step#Preface -->

    <owl:NamedIndividual rdf:about="http://people.aifb.kit.edu/mu2771/step#Preface">
        <rdf:type rdf:resource="http://iirds.tekom.de/iirds#TopicType"/>
        <rdfs:label xml:lang="de">Vorwort</rdfs:label>
        <rdfs:label xml:lang="en">preface</rdfs:label>
    </owl:NamedIndividual>
    


    <!-- http://people.aifb.kit.edu/mu2771/step#PrintTechnologies -->

    <owl:NamedIndividual rdf:about="http://people.aifb.kit.edu/mu2771/step#PrintTechnologies">
        <rdf:type rdf:resource="http://www.w3.org/ns/org#FormalOrganization"/>
        <rdfs:label xml:lang="en">Print Technologies</rdfs:label>
    </owl:NamedIndividual>
    


    <!-- http://people.aifb.kit.edu/mu2771/step#Priority1 -->

    <owl:NamedIndividual rdf:about="http://people.aifb.kit.edu/mu2771/step#Priority1">
        <rdf:type rdf:resource="http://people.aifb.kit.edu/mu2771/step#Priority"/>
        <rdfs:label xml:lang="de">Priorität 1</rdfs:label>
        <rdfs:label xml:lang="de">priority 1</rdfs:label>
    </owl:NamedIndividual>
    


    <!-- http://people.aifb.kit.edu/mu2771/step#Priority2 -->

    <owl:NamedIndividual rdf:about="http://people.aifb.kit.edu/mu2771/step#Priority2">
        <rdf:type rdf:resource="http://people.aifb.kit.edu/mu2771/step#Priority"/>
        <rdfs:label xml:lang="de">Priorität 2</rdfs:label>
        <rdfs:label xml:lang="de">priority 2</rdfs:label>
    </owl:NamedIndividual>
    


    <!-- http://people.aifb.kit.edu/mu2771/step#Priority3 -->

    <owl:NamedIndividual rdf:about="http://people.aifb.kit.edu/mu2771/step#Priority3">
        <rdf:type rdf:resource="http://people.aifb.kit.edu/mu2771/step#Priority"/>
        <rdfs:label xml:lang="de">Priorität 3</rdfs:label>
        <rdfs:label xml:lang="de">priority 3</rdfs:label>
    </owl:NamedIndividual>
    


    <!-- http://people.aifb.kit.edu/mu2771/step#Rainer_Bowden -->

    <owl:NamedIndividual rdf:about="http://people.aifb.kit.edu/mu2771/step#Rainer_Bowden">
        <rdf:type rdf:resource="http://people.aifb.kit.edu/mu2771/step#Technician"/>
        <rdfs:label xml:lang="de">Rainer Bowden</rdfs:label>
    </owl:NamedIndividual>
    


    <!-- http://people.aifb.kit.edu/mu2771/step#Report_2016-06-22 -->

    <owl:NamedIndividual rdf:about="http://people.aifb.kit.edu/mu2771/step#Report_2016-06-22">
        <rdf:type rdf:resource="http://people.aifb.kit.edu/mu2771/step#Report"/>
        <rdfs:comment xml:lang="de">Technikerbericht vom Einsatz am 22. Juni 2016 am KIT</rdfs:comment>
        <rdfs:label xml:lang="de">Technikerbericht 22.06.2016</rdfs:label>
    </owl:NamedIndividual>
    


    <!-- http://people.aifb.kit.edu/mu2771/step#Reutlingen -->

    <owl:NamedIndividual rdf:about="http://people.aifb.kit.edu/mu2771/step#Reutlingen">
        <rdf:type rdf:resource="http://www.w3.org/2003/01/geo/wgs84_pos#SpatialThing"/>
        <rdfs:label xml:lang="de">Reutlingen</rdfs:label>
    </owl:NamedIndividual>
    


    <!-- http://people.aifb.kit.edu/mu2771/step#Roger_Federer -->

    <owl:NamedIndividual rdf:about="http://people.aifb.kit.edu/mu2771/step#Roger_Federer">
        <rdf:type rdf:resource="http://xmlns.com/foaf/0.1/Person"/>
        <rdfs:label xml:lang="de">Roger Federer</rdfs:label>
    </owl:NamedIndividual>
    


    <!-- http://people.aifb.kit.edu/mu2771/step#SchmidtPapierdruck -->

    <owl:NamedIndividual rdf:about="http://people.aifb.kit.edu/mu2771/step#SchmidtPapierdruck">
        <rdf:type rdf:resource="http://www.w3.org/ns/org#FormalOrganization"/>
        <rdfs:label xml:lang="de">Schmidt Papierdruck</rdfs:label>
    </owl:NamedIndividual>
    


    <!-- http://people.aifb.kit.edu/mu2771/step#Stuttgart -->

    <owl:NamedIndividual rdf:about="http://people.aifb.kit.edu/mu2771/step#Stuttgart">
        <rdf:type rdf:resource="http://www.w3.org/2003/01/geo/wgs84_pos#SpatialThing"/>
        <rdfs:label xml:lang="de">Stuttgart</rdfs:label>
    </owl:NamedIndividual>
    


    <!-- http://people.aifb.kit.edu/mu2771/step#TaskNo1 -->

    <owl:NamedIndividual rdf:about="http://people.aifb.kit.edu/mu2771/step#TaskNo1">
        <rdf:type rdf:resource="http://people.aifb.kit.edu/mu2771/step#ScheduledWorkOrder"/>
        <rdfs:label xml:lang="de">Geplanter Einsatz Nr. 1</rdfs:label>
    </owl:NamedIndividual>
    


    <!-- http://people.aifb.kit.edu/mu2771/step#Thorsten_Meier -->

    <owl:NamedIndividual rdf:about="http://people.aifb.kit.edu/mu2771/step#Thorsten_Meier">
        <rdf:type rdf:resource="http://people.aifb.kit.edu/mu2771/step#Technician"/>
        <rdfs:label xml:lang="de">Thorsten Meier</rdfs:label>
    </owl:NamedIndividual>
    


    <!-- http://people.aifb.kit.edu/mu2771/step#Tuttlingen -->

    <owl:NamedIndividual rdf:about="http://people.aifb.kit.edu/mu2771/step#Tuttlingen">
        <rdf:type rdf:resource="http://www.w3.org/2003/01/geo/wgs84_pos#SpatialThing"/>
    </owl:NamedIndividual>
    


    <!-- http://people.aifb.kit.edu/mu2771/step#U-clamp -->

    <owl:NamedIndividual rdf:about="http://people.aifb.kit.edu/mu2771/step#U-clamp">
        <rdf:type rdf:resource="http://purl.oclc.org/NET/ssnx/ssn#Device"/>
        <step:sourceUri rdf:resource="http://people.aifb.kit.edu/mu2771/step#"/>
        <rdfs:label xml:lang="de">Bogenaufspannklaue</rdfs:label>
        <rdfs:label xml:lang="en">U-clamp</rdfs:label>
        <part:partOf rdf:resource="http://people.aifb.kit.edu/mu2771/step#caliper_detector"/>
        <part:partOf rdf:resource="http://people.aifb.kit.edu/mu2771/step#no-sheet_detector"/>
    </owl:NamedIndividual>
    


    <!-- http://people.aifb.kit.edu/mu2771/step#Ueberschiessbogen -->

    <owl:NamedIndividual rdf:about="http://people.aifb.kit.edu/mu2771/step#Ueberschiessbogen">
        <rdf:type rdf:resource="http://purl.oclc.org/NET/ssnx/ssn#Device"/>
        <dc:creator rdf:resource="http://www.aifb.kit.edu/web/Sebastian_Bader"/>
        <rdfs:label xml:lang="de">Ueberschiessbogen</rdfs:label>
        <part:partOf rdf:resource="http://people.aifb.kit.edu/mu2771/step#rotary-valve"/>
    </owl:NamedIndividual>
    


    <!-- http://people.aifb.kit.edu/mu2771/step#UnplannedTaskNo1 -->

    <owl:NamedIndividual rdf:about="http://people.aifb.kit.edu/mu2771/step#UnplannedTaskNo1">
        <rdf:type rdf:resource="http://people.aifb.kit.edu/mu2771/step#UnplannedWorkOrder"/>
        <rdfs:label xml:lang="de">Ungeplanter Einsatz Nr 1</rdfs:label>
    </owl:NamedIndividual>
    


    <!-- http://people.aifb.kit.edu/mu2771/step#adjustment -->

    <owl:NamedIndividual rdf:about="http://people.aifb.kit.edu/mu2771/step#adjustment">
        <rdf:type rdf:resource="http://purl.oclc.org/NET/ssnx/ssn#Process"/>
        <dc:creator rdf:resource="http://www.aifb.kit.edu/web/Sebastian_Bader"/>
        <rdfs:label xml:lang="de">Anpassung</rdfs:label>
        <rdfs:label xml:lang="de">Justage</rdfs:label>
        <rdfs:label xml:lang="en">adjustment</rdfs:label>
    </owl:NamedIndividual>
    


    <!-- http://people.aifb.kit.edu/mu2771/step#blanket -->

    <owl:NamedIndividual rdf:about="http://people.aifb.kit.edu/mu2771/step#blanket">
        <rdf:type rdf:resource="http://people.aifb.kit.edu/mu2771/step#Tool"/>
        <dc:creator rdf:resource="http://www.heidelberg.com/"/>
        <rdfs:label xml:lang="de">Gummituch</rdfs:label>
        <rdfs:label xml:lang="en">blanket</rdfs:label>
    </owl:NamedIndividual>
    


    <!-- http://people.aifb.kit.edu/mu2771/step#caliper_detector -->

    <owl:NamedIndividual rdf:about="http://people.aifb.kit.edu/mu2771/step#caliper_detector">
        <rdf:type rdf:resource="http://purl.oclc.org/NET/ssnx/ssn#System"/>
        <owl:sameAs rdf:resource="http://people.aifb.kit.edu/mu2771/step#no-sheet_detector"/>
        <step:sourceUri rdf:resource="http://people.aifb.kit.edu/mu2771/step#"/>
        <rdfs:label xml:lang="de">Fehlbogenkontrolle</rdfs:label>
        <rdfs:label xml:lang="en">caliper detector</rdfs:label>
        <part:partOf rdf:resource="http://people.aifb.kit.edu/mu2771/step#printing_press"/>
    </owl:NamedIndividual>
    


    <!-- http://people.aifb.kit.edu/mu2771/step#central_control_cabinet -->

    <owl:NamedIndividual rdf:about="http://people.aifb.kit.edu/mu2771/step#central_control_cabinet">
        <rdf:type rdf:resource="http://purl.oclc.org/NET/ssnx/ssn#Device"/>
        <dc:creator rdf:resource="http://www.heidelberg.com/"/>
        <rdfs:label xml:lang="de">Zentralschaltgerät</rdfs:label>
        <rdfs:label xml:lang="en">central control cabinet</rdfs:label>
        <part:partOf rdf:resource="http://people.aifb.kit.edu/mu2771/step#printing_press"/>
    </owl:NamedIndividual>
    


    <!-- http://people.aifb.kit.edu/mu2771/step#circumferential_register -->

    <owl:NamedIndividual rdf:about="http://people.aifb.kit.edu/mu2771/step#circumferential_register">
        <rdf:type rdf:resource="http://purl.oclc.org/NET/ssnx/ssn#System"/>
        <step:sourceUri rdf:resource="http://people.aifb.kit.edu/mu2771/step#"/>
        <rdfs:label xml:lang="de">Umfangregister</rdfs:label>
        <rdfs:label xml:lang="de">Umfangsregister</rdfs:label>
        <rdfs:label xml:lang="en">circumferential register</rdfs:label>
        <part:partOf rdf:resource="http://people.aifb.kit.edu/mu2771/step#caliper_detector"/>
        <part:partOf rdf:resource="http://people.aifb.kit.edu/mu2771/step#no-sheet_detector"/>
    </owl:NamedIndividual>
    


    <!-- http://people.aifb.kit.edu/mu2771/step#clamp -->

    <owl:NamedIndividual rdf:about="http://people.aifb.kit.edu/mu2771/step#clamp">
        <rdf:type rdf:resource="http://purl.oclc.org/NET/ssnx/ssn#Process"/>
        <dc:creator rdf:resource="http://www.aifb.kit.edu/web/Sebastian_Bader"/>
        <rdfs:label xml:lang="en">clamp</rdfs:label>
        <rdfs:label xml:lang="de">einspannen</rdfs:label>
    </owl:NamedIndividual>
    


    <!-- http://people.aifb.kit.edu/mu2771/step#cleaning -->

    <owl:NamedIndividual rdf:about="http://people.aifb.kit.edu/mu2771/step#cleaning">
        <rdf:type rdf:resource="http://purl.oclc.org/NET/ssnx/ssn#Process"/>
        <dc:creator rdf:resource="http://www.aifb.kit.edu/web/Sebastian_Bader"/>
        <rdfs:label xml:lang="de">Reinigung</rdfs:label>
        <rdfs:label xml:lang="en">cleaning</rdfs:label>
    </owl:NamedIndividual>
    


    <!-- http://people.aifb.kit.edu/mu2771/step#color -->

    <owl:NamedIndividual rdf:about="http://people.aifb.kit.edu/mu2771/step#color">
        <rdf:type rdf:resource="http://qudt.org/schema/qudt#Dimension"/>
        <dc:creator rdf:resource="http://www.heidelberg.com/"/>
        <rdfs:label xml:lang="de">Farbe</rdfs:label>
        <rdfs:label xml:lang="en">color</rdfs:label>
    </owl:NamedIndividual>
    


    <!-- http://people.aifb.kit.edu/mu2771/step#color_separation -->

    <owl:NamedIndividual rdf:about="http://people.aifb.kit.edu/mu2771/step#color_separation">
        <rdf:type rdf:resource="http://purl.oclc.org/NET/ssnx/ssn#System"/>
        <dc:creator rdf:resource="http://www.heidelberg.com/"/>
        <rdfs:label xml:lang="de">Farbauszug</rdfs:label>
        <rdfs:label xml:lang="en">color separation</rdfs:label>
    </owl:NamedIndividual>
    


    <!-- http://people.aifb.kit.edu/mu2771/step#color_strip -->

    <owl:NamedIndividual rdf:about="http://people.aifb.kit.edu/mu2771/step#color_strip">
        <rdf:type rdf:resource="http://people.aifb.kit.edu/mu2771/step#Tool"/>
        <dc:creator rdf:resource="http://www.heidelberg.com/"/>
        <rdfs:label xml:lang="de">Messstreifen</rdfs:label>
        <rdfs:label xml:lang="en">color strip</rdfs:label>
    </owl:NamedIndividual>
    


    <!-- http://people.aifb.kit.edu/mu2771/step#colour_console -->

    <owl:NamedIndividual rdf:about="http://people.aifb.kit.edu/mu2771/step#colour_console">
        <rdf:type rdf:resource="http://purl.oclc.org/NET/ssnx/ssn#Device"/>
        <owl:sameAs rdf:resource="http://people.aifb.kit.edu/mu2771/step#print_color_desk"/>
        <step:sourceUri rdf:resource="http://people.aifb.kit.edu/mu2771/step#"/>
        <rdfs:label xml:lang="de">Colorpult</rdfs:label>
        <rdfs:label xml:lang="de">Colorsteuerpult</rdfs:label>
        <rdfs:label xml:lang="de">Farbpult</rdfs:label>
        <rdfs:label xml:lang="de">Farbsteuerpult</rdfs:label>
        <rdfs:label xml:lang="en">colour console</rdfs:label>
        <part:partOf rdf:resource="http://people.aifb.kit.edu/mu2771/step#printing_press"/>
    </owl:NamedIndividual>
    


    <!-- http://people.aifb.kit.edu/mu2771/step#control_console -->

    <owl:NamedIndividual rdf:about="http://people.aifb.kit.edu/mu2771/step#control_console">
        <rdf:type rdf:resource="http://purl.oclc.org/NET/ssnx/ssn#System"/>
        <dc:creator rdf:resource="http://www.heidelberg.com/"/>
        <rdfs:label xml:lang="de">Bedienpult</rdfs:label>
        <rdfs:label xml:lang="en">control console</rdfs:label>
        <part:partOf rdf:resource="http://people.aifb.kit.edu/mu2771/step#printing_press"/>
    </owl:NamedIndividual>
    


    <!-- http://people.aifb.kit.edu/mu2771/step#coupling -->

    <owl:NamedIndividual rdf:about="http://people.aifb.kit.edu/mu2771/step#coupling">
        <rdf:type rdf:resource="http://purl.oclc.org/NET/ssnx/ssn#Device"/>
        <dc:creator rdf:resource="http://www.heidelberg.com/"/>
        <rdfs:label xml:lang="de">Kupplung</rdfs:label>
        <rdfs:label xml:lang="en">coupling</rdfs:label>
        <part:partOf rdf:resource="http://people.aifb.kit.edu/mu2771/step#dampening_system"/>
        <part:partOf rdf:resource="http://people.aifb.kit.edu/mu2771/step#dampening_unit"/>
        <part:partOf rdf:resource="http://people.aifb.kit.edu/mu2771/step#damping_unit"/>
        <part:partOf rdf:resource="http://people.aifb.kit.edu/mu2771/step#moistener"/>
        <part:partOf rdf:resource="http://people.aifb.kit.edu/mu2771/step#print_dampener"/>
    </owl:NamedIndividual>
    


    <!-- http://people.aifb.kit.edu/mu2771/step#dampener-roller -->

    <owl:NamedIndividual rdf:about="http://people.aifb.kit.edu/mu2771/step#dampener-roller">
        <rdf:type rdf:resource="http://purl.oclc.org/NET/ssnx/ssn#Device"/>
        <step:sourceUri rdf:resource="http://people.aifb.kit.edu/mu2771/step#"/>
        <rdfs:label xml:lang="de">Feuchtauftragwalze</rdfs:label>
        <rdfs:label xml:lang="en">dampener-roller</rdfs:label>
        <part:partOf rdf:resource="http://people.aifb.kit.edu/mu2771/step#dampening_system"/>
        <part:partOf rdf:resource="http://people.aifb.kit.edu/mu2771/step#dampening_unit"/>
        <part:partOf rdf:resource="http://people.aifb.kit.edu/mu2771/step#damping_unit"/>
        <part:partOf rdf:resource="http://people.aifb.kit.edu/mu2771/step#moistener"/>
        <part:partOf rdf:resource="http://people.aifb.kit.edu/mu2771/step#print_dampener"/>
    </owl:NamedIndividual>
    


    <!-- http://people.aifb.kit.edu/mu2771/step#dampener_circulator -->

    <owl:NamedIndividual rdf:about="http://people.aifb.kit.edu/mu2771/step#dampener_circulator">
        <rdf:type rdf:resource="http://purl.oclc.org/NET/ssnx/ssn#Device"/>
        <step:sourceUri rdf:resource="http://people.aifb.kit.edu/mu2771/step#"/>
        <rdfs:label xml:lang="de">Wasserumwälzanlage</rdfs:label>
        <rdfs:label xml:lang="en">dampener circulator</rdfs:label>
        <part:partOf rdf:resource="http://people.aifb.kit.edu/mu2771/step#dampening_fountain"/>
        <part:partOf rdf:resource="http://people.aifb.kit.edu/mu2771/step#water_fountain"/>
        <part:partOf rdf:resource="http://people.aifb.kit.edu/mu2771/step#water_pan"/>
    </owl:NamedIndividual>
    


    <!-- http://people.aifb.kit.edu/mu2771/step#dampener_roll -->

    <owl:NamedIndividual rdf:about="http://people.aifb.kit.edu/mu2771/step#dampener_roll">
        <rdf:type rdf:resource="http://purl.oclc.org/NET/ssnx/ssn#Device"/>
        <owl:sameAs rdf:resource="http://people.aifb.kit.edu/mu2771/step#dampening_form_roller"/>
        <step:sourceUri rdf:resource="http://people.aifb.kit.edu/mu2771/step#"/>
        <rdfs:label xml:lang="de">Feuchtauftragwalze</rdfs:label>
        <rdfs:label xml:lang="de">Feuchtwalze</rdfs:label>
        <rdfs:label xml:lang="en">dampener roll</rdfs:label>
        <part:partOf rdf:resource="http://people.aifb.kit.edu/mu2771/step#dampening_system"/>
        <part:partOf rdf:resource="http://people.aifb.kit.edu/mu2771/step#dampening_unit"/>
        <part:partOf rdf:resource="http://people.aifb.kit.edu/mu2771/step#damping_unit"/>
        <part:partOf rdf:resource="http://people.aifb.kit.edu/mu2771/step#moistener"/>
        <part:partOf rdf:resource="http://people.aifb.kit.edu/mu2771/step#print_dampener"/>
    </owl:NamedIndividual>
    


    <!-- http://people.aifb.kit.edu/mu2771/step#dampening_distributor_cylinder -->

    <owl:NamedIndividual rdf:about="http://people.aifb.kit.edu/mu2771/step#dampening_distributor_cylinder">
        <rdf:type rdf:resource="http://purl.oclc.org/NET/ssnx/ssn#Device"/>
        <step:sourceUri rdf:resource="http://people.aifb.kit.edu/mu2771/step#"/>
        <rdfs:label xml:lang="de">Verreiberzylinder</rdfs:label>
        <rdfs:label xml:lang="en">dampening distributor cylinder</rdfs:label>
        <part:partOf rdf:resource="http://people.aifb.kit.edu/mu2771/step#dampening_system"/>
        <part:partOf rdf:resource="http://people.aifb.kit.edu/mu2771/step#dampening_unit"/>
        <part:partOf rdf:resource="http://people.aifb.kit.edu/mu2771/step#damping_unit"/>
        <part:partOf rdf:resource="http://people.aifb.kit.edu/mu2771/step#moistener"/>
        <part:partOf rdf:resource="http://people.aifb.kit.edu/mu2771/step#print_dampener"/>
    </owl:NamedIndividual>
    


    <!-- http://people.aifb.kit.edu/mu2771/step#dampening_form_roller -->

    <owl:NamedIndividual rdf:about="http://people.aifb.kit.edu/mu2771/step#dampening_form_roller">
        <rdf:type rdf:resource="http://purl.oclc.org/NET/ssnx/ssn#Device"/>
        <step:sourceUri rdf:resource="http://people.aifb.kit.edu/mu2771/step#"/>
        <rdfs:label xml:lang="de">Feuchtauftragswalze</rdfs:label>
        <rdfs:label xml:lang="de">Feuchtauftragwalze</rdfs:label>
        <rdfs:label xml:lang="de">Feuchtwalze</rdfs:label>
        <rdfs:label xml:lang="en">dampener roll</rdfs:label>
        <rdfs:label xml:lang="en">dampening form roller</rdfs:label>
        <part:partOf rdf:resource="http://people.aifb.kit.edu/mu2771/step#dampening_system"/>
        <part:partOf rdf:resource="http://people.aifb.kit.edu/mu2771/step#dampening_unit"/>
        <part:partOf rdf:resource="http://people.aifb.kit.edu/mu2771/step#damping_unit"/>
        <part:partOf rdf:resource="http://people.aifb.kit.edu/mu2771/step#moistener"/>
        <part:partOf rdf:resource="http://people.aifb.kit.edu/mu2771/step#print_dampener"/>
    </owl:NamedIndividual>
    


    <!-- http://people.aifb.kit.edu/mu2771/step#dampening_fountain -->

    <owl:NamedIndividual rdf:about="http://people.aifb.kit.edu/mu2771/step#dampening_fountain">
        <rdf:type rdf:resource="http://purl.oclc.org/NET/ssnx/ssn#Device"/>
        <owl:sameAs rdf:resource="http://people.aifb.kit.edu/mu2771/step#water_fountain"/>
        <owl:sameAs rdf:resource="http://people.aifb.kit.edu/mu2771/step#water_pan"/>
        <step:sourceUri rdf:resource="http://people.aifb.kit.edu/mu2771/step#"/>
        <rdfs:label xml:lang="de">Wasserkasten</rdfs:label>
        <rdfs:label xml:lang="en">dampening fountain</rdfs:label>
        <part:partOf rdf:resource="http://people.aifb.kit.edu/mu2771/step#dampening_form_roller"/>
    </owl:NamedIndividual>
    


    <!-- http://people.aifb.kit.edu/mu2771/step#dampening_fountain_roller -->

    <owl:NamedIndividual rdf:about="http://people.aifb.kit.edu/mu2771/step#dampening_fountain_roller">
        <rdf:type rdf:resource="http://purl.oclc.org/NET/ssnx/ssn#Device"/>
        <owl:sameAs rdf:resource="http://people.aifb.kit.edu/mu2771/step#water-duct_roller"/>
        <owl:sameAs rdf:resource="http://people.aifb.kit.edu/mu2771/step#water_duct_roller"/>
        <owl:sameAs rdf:resource="http://people.aifb.kit.edu/mu2771/step#water_fountain_roller"/>
        <step:sourceUri rdf:resource="http://people.aifb.kit.edu/mu2771/step#"/>
        <rdfs:label xml:lang="de">Feuchtduktor</rdfs:label>
        <rdfs:label xml:lang="en">dampening fountain roller</rdfs:label>
        <part:partOf rdf:resource="http://people.aifb.kit.edu/mu2771/step#dampening_system"/>
        <part:partOf rdf:resource="http://people.aifb.kit.edu/mu2771/step#dampening_unit"/>
        <part:partOf rdf:resource="http://people.aifb.kit.edu/mu2771/step#damping_unit"/>
        <part:partOf rdf:resource="http://people.aifb.kit.edu/mu2771/step#moistener"/>
        <part:partOf rdf:resource="http://people.aifb.kit.edu/mu2771/step#print_dampener"/>
    </owl:NamedIndividual>
    


    <!-- http://people.aifb.kit.edu/mu2771/step#dampening_shutter -->

    <owl:NamedIndividual rdf:about="http://people.aifb.kit.edu/mu2771/step#dampening_shutter">
        <rdf:type rdf:resource="http://purl.oclc.org/NET/ssnx/ssn#Device"/>
        <step:sourceUri rdf:resource="http://people.aifb.kit.edu/mu2771/step#"/>
        <rdfs:label xml:lang="de">Feuchtwerkblende</rdfs:label>
        <rdfs:label xml:lang="en">dampening shutter</rdfs:label>
        <part:partOf rdf:resource="http://people.aifb.kit.edu/mu2771/step#dampening_system"/>
        <part:partOf rdf:resource="http://people.aifb.kit.edu/mu2771/step#dampening_unit"/>
        <part:partOf rdf:resource="http://people.aifb.kit.edu/mu2771/step#damping_unit"/>
        <part:partOf rdf:resource="http://people.aifb.kit.edu/mu2771/step#moistener"/>
        <part:partOf rdf:resource="http://people.aifb.kit.edu/mu2771/step#print_dampener"/>
    </owl:NamedIndividual>
    


    <!-- http://people.aifb.kit.edu/mu2771/step#dampening_system -->

    <owl:NamedIndividual rdf:about="http://people.aifb.kit.edu/mu2771/step#dampening_system">
        <rdf:type rdf:resource="http://purl.oclc.org/NET/ssnx/ssn#Device"/>
        <owl:sameAs rdf:resource="http://people.aifb.kit.edu/mu2771/step#dampening_unit"/>
        <owl:sameAs rdf:resource="http://people.aifb.kit.edu/mu2771/step#damping_unit"/>
        <owl:sameAs rdf:resource="http://people.aifb.kit.edu/mu2771/step#moistener"/>
        <owl:sameAs rdf:resource="http://people.aifb.kit.edu/mu2771/step#print_dampener"/>
        <step:sourceUri rdf:resource="http://people.aifb.kit.edu/mu2771/step#"/>
        <rdfs:label xml:lang="de">Feuchtwerk</rdfs:label>
        <rdfs:label xml:lang="en">dampening system</rdfs:label>
        <part:partOf rdf:resource="http://people.aifb.kit.edu/mu2771/step#printing_press"/>
    </owl:NamedIndividual>
    


    <!-- http://people.aifb.kit.edu/mu2771/step#dampening_unit -->

    <owl:NamedIndividual rdf:about="http://people.aifb.kit.edu/mu2771/step#dampening_unit">
        <rdf:type rdf:resource="http://purl.oclc.org/NET/ssnx/ssn#Device"/>
        <rdf:type rdf:resource="http://purl.oclc.org/NET/ssnx/ssn#System"/>
        <owl:sameAs rdf:resource="http://people.aifb.kit.edu/mu2771/step#damping_unit"/>
        <owl:sameAs rdf:resource="http://people.aifb.kit.edu/mu2771/step#moistener"/>
        <owl:sameAs rdf:resource="http://people.aifb.kit.edu/mu2771/step#print_dampener"/>
        <step:sourceUri rdf:resource="http://people.aifb.kit.edu/mu2771/step#"/>
        <rdfs:label xml:lang="de">Feuchtauftragwalze</rdfs:label>
        <rdfs:label xml:lang="de">Feuchtwalze</rdfs:label>
        <rdfs:label xml:lang="de">Feuchtwerk</rdfs:label>
        <rdfs:label xml:lang="en">dampening system</rdfs:label>
        <rdfs:label xml:lang="en">dampening unit</rdfs:label>
        <rdfs:label xml:lang="en">damping unit</rdfs:label>
        <rdfs:label xml:lang="en">moistener</rdfs:label>
        <rdfs:label xml:lang="en">print dampener</rdfs:label>
        <part:partOf rdf:resource="http://people.aifb.kit.edu/mu2771/step#printing_press"/>
    </owl:NamedIndividual>
    


    <!-- http://people.aifb.kit.edu/mu2771/step#dampening_vibrator -->

    <owl:NamedIndividual rdf:about="http://people.aifb.kit.edu/mu2771/step#dampening_vibrator">
        <rdf:type rdf:resource="http://purl.oclc.org/NET/ssnx/ssn#Device"/>
        <step:sourceUri rdf:resource="http://people.aifb.kit.edu/mu2771/step#"/>
        <rdfs:label xml:lang="de">Feuchtheber</rdfs:label>
        <rdfs:label xml:lang="en">dampening vibrator</rdfs:label>
        <part:partOf rdf:resource="http://people.aifb.kit.edu/mu2771/step#dampening_system"/>
        <part:partOf rdf:resource="http://people.aifb.kit.edu/mu2771/step#dampening_unit"/>
        <part:partOf rdf:resource="http://people.aifb.kit.edu/mu2771/step#damping_unit"/>
        <part:partOf rdf:resource="http://people.aifb.kit.edu/mu2771/step#moistener"/>
        <part:partOf rdf:resource="http://people.aifb.kit.edu/mu2771/step#print_dampener"/>
    </owl:NamedIndividual>
    


    <!-- http://people.aifb.kit.edu/mu2771/step#damper -->

    <owl:NamedIndividual rdf:about="http://people.aifb.kit.edu/mu2771/step#damper">
        <owl:sameAs rdf:resource="http://people.aifb.kit.edu/mu2771/step#damping_roller"/>
    </owl:NamedIndividual>
    


    <!-- http://people.aifb.kit.edu/mu2771/step#damper-roller -->

    <owl:NamedIndividual rdf:about="http://people.aifb.kit.edu/mu2771/step#damper-roller">
        <rdf:type rdf:resource="http://purl.oclc.org/NET/ssnx/ssn#Device"/>
        <owl:sameAs rdf:resource="http://people.aifb.kit.edu/mu2771/step#water_roller"/>
        <step:sourceUri rdf:resource="http://people.aifb.kit.edu/mu2771/step#"/>
        <rdfs:label xml:lang="de">Feuchtwalze</rdfs:label>
        <rdfs:label xml:lang="en">damper-roller</rdfs:label>
        <part:partOf rdf:resource="http://people.aifb.kit.edu/mu2771/step#dampening_system"/>
        <part:partOf rdf:resource="http://people.aifb.kit.edu/mu2771/step#dampening_unit"/>
        <part:partOf rdf:resource="http://people.aifb.kit.edu/mu2771/step#damping_unit"/>
        <part:partOf rdf:resource="http://people.aifb.kit.edu/mu2771/step#moistener"/>
        <part:partOf rdf:resource="http://people.aifb.kit.edu/mu2771/step#print_dampener"/>
    </owl:NamedIndividual>
    


    <!-- http://people.aifb.kit.edu/mu2771/step#damping_fountain_roller -->

    <owl:NamedIndividual rdf:about="http://people.aifb.kit.edu/mu2771/step#damping_fountain_roller">
        <rdf:type rdf:resource="http://purl.oclc.org/NET/ssnx/ssn#Device"/>
        <step:sourceUri rdf:resource="http://people.aifb.kit.edu/mu2771/step#"/>
        <rdfs:label xml:lang="de">Wasserkastenwalze</rdfs:label>
        <rdfs:label xml:lang="en">damping fountain roller</rdfs:label>
        <part:partOf rdf:resource="http://people.aifb.kit.edu/mu2771/step#dampening_fountain"/>
        <part:partOf rdf:resource="http://people.aifb.kit.edu/mu2771/step#water_fountain"/>
        <part:partOf rdf:resource="http://people.aifb.kit.edu/mu2771/step#water_pan"/>
    </owl:NamedIndividual>
    


    <!-- http://people.aifb.kit.edu/mu2771/step#damping_roller -->

    <owl:NamedIndividual rdf:about="http://people.aifb.kit.edu/mu2771/step#damping_roller">
        <rdf:type rdf:resource="http://purl.oclc.org/NET/ssnx/ssn#Device"/>
        <step:sourceUri rdf:resource="http://people.aifb.kit.edu/mu2771/step#"/>
        <rdfs:label xml:lang="de">Feuchtauftragwalze</rdfs:label>
        <rdfs:label xml:lang="de">Feuchtwalze</rdfs:label>
        <rdfs:label xml:lang="en">damping roller</rdfs:label>
    </owl:NamedIndividual>
    


    <!-- http://people.aifb.kit.edu/mu2771/step#damping_unit -->

    <owl:NamedIndividual rdf:about="http://people.aifb.kit.edu/mu2771/step#damping_unit">
        <rdf:type rdf:resource="http://purl.oclc.org/NET/ssnx/ssn#Device"/>
        <rdf:type rdf:resource="http://purl.oclc.org/NET/ssnx/ssn#System"/>
        <owl:sameAs rdf:resource="http://people.aifb.kit.edu/mu2771/step#moistener"/>
        <owl:sameAs rdf:resource="http://people.aifb.kit.edu/mu2771/step#print_dampener"/>
        <step:sourceUri rdf:resource="http://people.aifb.kit.edu/mu2771/step#"/>
        <rdfs:label xml:lang="de">Feuchtauftragwalze</rdfs:label>
        <rdfs:label xml:lang="de">Feuchtwalze</rdfs:label>
        <rdfs:label xml:lang="de">Feuchtwerk</rdfs:label>
        <rdfs:label xml:lang="en">dampening system</rdfs:label>
        <rdfs:label xml:lang="en">dampening unit</rdfs:label>
        <rdfs:label xml:lang="en">damping unit</rdfs:label>
        <rdfs:label xml:lang="en">moistener</rdfs:label>
        <rdfs:label xml:lang="en">print dampener</rdfs:label>
        <part:partOf rdf:resource="http://people.aifb.kit.edu/mu2771/step#printing_press"/>
    </owl:NamedIndividual>
    


    <!-- http://people.aifb.kit.edu/mu2771/step#damping_vibrator -->

    <owl:NamedIndividual rdf:about="http://people.aifb.kit.edu/mu2771/step#damping_vibrator">
        <rdf:type rdf:resource="http://purl.oclc.org/NET/ssnx/ssn#Device"/>
        <owl:sameAs rdf:resource="http://people.aifb.kit.edu/mu2771/step#vibrating_dampening_roller"/>
        <step:sourceUri rdf:resource="http://people.aifb.kit.edu/mu2771/step#"/>
        <rdfs:label xml:lang="de">Feuchtheber</rdfs:label>
        <rdfs:label xml:lang="en">damping vibrator</rdfs:label>
        <part:partOf rdf:resource="http://people.aifb.kit.edu/mu2771/step#dampening_system"/>
        <part:partOf rdf:resource="http://people.aifb.kit.edu/mu2771/step#dampening_unit"/>
        <part:partOf rdf:resource="http://people.aifb.kit.edu/mu2771/step#damping_unit"/>
        <part:partOf rdf:resource="http://people.aifb.kit.edu/mu2771/step#moistener"/>
        <part:partOf rdf:resource="http://people.aifb.kit.edu/mu2771/step#print_dampener"/>
    </owl:NamedIndividual>
    


    <!-- http://people.aifb.kit.edu/mu2771/step#de-electrification -->

    <owl:NamedIndividual rdf:about="http://people.aifb.kit.edu/mu2771/step#de-electrification">
        <rdf:type rdf:resource="http://purl.oclc.org/NET/ssnx/ssn#Process"/>
        <step:sourceUri rdf:resource="http://people.aifb.kit.edu/mu2771/step#"/>
        <rdfs:label xml:lang="de">Entelektrisierung</rdfs:label>
        <rdfs:label xml:lang="en">de-electrification</rdfs:label>
    </owl:NamedIndividual>
    


    <!-- http://people.aifb.kit.edu/mu2771/step#delivery_table -->

    <owl:NamedIndividual rdf:about="http://people.aifb.kit.edu/mu2771/step#delivery_table">
        <rdf:type rdf:resource="http://purl.oclc.org/NET/ssnx/ssn#Device"/>
        <step:sourceUri rdf:resource="http://people.aifb.kit.edu/mu2771/step#"/>
        <rdfs:label xml:lang="de">Auslegetisch</rdfs:label>
        <rdfs:label xml:lang="en">delivery table</rdfs:label>
        <part:partOf rdf:resource="http://people.aifb.kit.edu/mu2771/step#printing_press"/>
    </owl:NamedIndividual>
    


    <!-- http://people.aifb.kit.edu/mu2771/step#distributing_roller -->

    <owl:NamedIndividual rdf:about="http://people.aifb.kit.edu/mu2771/step#distributing_roller">
        <rdf:type rdf:resource="http://purl.oclc.org/NET/ssnx/ssn#Device"/>
        <owl:sameAs rdf:resource="http://people.aifb.kit.edu/mu2771/step#distributor_roll"/>
        <owl:sameAs rdf:resource="http://people.aifb.kit.edu/mu2771/step#distributor_roller"/>
        <step:sourceUri rdf:resource="http://people.aifb.kit.edu/mu2771/step#"/>
        <rdfs:label xml:lang="de">Reibwalze</rdfs:label>
        <rdfs:label xml:lang="de">Verreibwalze</rdfs:label>
        <rdfs:label xml:lang="en">distributing roller</rdfs:label>
        <part:partOf rdf:resource="http://people.aifb.kit.edu/mu2771/step#printing_press"/>
    </owl:NamedIndividual>
    


    <!-- http://people.aifb.kit.edu/mu2771/step#distributor_roll -->

    <owl:NamedIndividual rdf:about="http://people.aifb.kit.edu/mu2771/step#distributor_roll">
        <rdf:type rdf:resource="http://purl.oclc.org/NET/ssnx/ssn#Device"/>
        <owl:sameAs rdf:resource="http://people.aifb.kit.edu/mu2771/step#distributor_roller"/>
        <step:sourceUri rdf:resource="http://people.aifb.kit.edu/mu2771/step#"/>
        <rdfs:label xml:lang="de">Reiber</rdfs:label>
        <rdfs:label xml:lang="de">Reibwalze</rdfs:label>
        <rdfs:label xml:lang="de">Verreibwalze</rdfs:label>
        <rdfs:label xml:lang="en">distributing roller</rdfs:label>
        <rdfs:label xml:lang="en">distributor</rdfs:label>
        <rdfs:label xml:lang="en">distributor (roll)</rdfs:label>
        <rdfs:label xml:lang="en">distributor roll</rdfs:label>
        <rdfs:label xml:lang="en">distributor roller</rdfs:label>
        <part:partOf rdf:resource="http://people.aifb.kit.edu/mu2771/step#printing_press"/>
    </owl:NamedIndividual>
    


    <!-- http://people.aifb.kit.edu/mu2771/step#distributor_roller -->

    <owl:NamedIndividual rdf:about="http://people.aifb.kit.edu/mu2771/step#distributor_roller">
        <rdf:type rdf:resource="http://purl.oclc.org/NET/ssnx/ssn#Device"/>
        <step:sourceUri rdf:resource="http://people.aifb.kit.edu/mu2771/step#"/>
        <rdfs:label xml:lang="de">Reiber</rdfs:label>
        <rdfs:label xml:lang="de">Reibwalze</rdfs:label>
        <rdfs:label xml:lang="de">Verreibwalze</rdfs:label>
        <rdfs:label xml:lang="en">distributing roller</rdfs:label>
        <rdfs:label xml:lang="en">distributor</rdfs:label>
        <rdfs:label xml:lang="en">distributor (roll)</rdfs:label>
        <rdfs:label xml:lang="en">distributor roll</rdfs:label>
        <rdfs:label xml:lang="en">distributor roller</rdfs:label>
        <part:partOf rdf:resource="http://people.aifb.kit.edu/mu2771/step#printing_press"/>
    </owl:NamedIndividual>
    


    <!-- http://people.aifb.kit.edu/mu2771/step#doctor_knife -->

    <owl:NamedIndividual rdf:about="http://people.aifb.kit.edu/mu2771/step#doctor_knife">
        <rdf:type rdf:resource="http://purl.oclc.org/NET/ssnx/ssn#Device"/>
        <owl:sameAs rdf:resource="http://people.aifb.kit.edu/mu2771/step#fountain_blade"/>
        <owl:sameAs rdf:resource="http://people.aifb.kit.edu/mu2771/step#print_ink_blade"/>
        <step:sourceUri rdf:resource="http://people.aifb.kit.edu/mu2771/step#"/>
        <rdfs:label xml:lang="de">Farbmesser</rdfs:label>
        <rdfs:label xml:lang="en">doctor knife</rdfs:label>
        <part:partOf rdf:resource="http://people.aifb.kit.edu/mu2771/step#printing_press"/>
    </owl:NamedIndividual>
    


    <!-- http://people.aifb.kit.edu/mu2771/step#double_sheet_control -->

    <owl:NamedIndividual rdf:about="http://people.aifb.kit.edu/mu2771/step#double_sheet_control">
        <rdf:type rdf:resource="http://purl.oclc.org/NET/ssnx/ssn#System"/>
        <owl:sameAs rdf:resource="http://people.aifb.kit.edu/mu2771/step#double_sheet_detector"/>
        <owl:sameAs rdf:resource="http://people.aifb.kit.edu/mu2771/step#doubles_detector"/>
        <step:sourceUri rdf:resource="http://people.aifb.kit.edu/mu2771/step#"/>
        <rdfs:label xml:lang="de">Doppelbogenabfühlung</rdfs:label>
        <rdfs:label xml:lang="de">Doppelbogenkontrolle</rdfs:label>
        <rdfs:label xml:lang="en">double sheet control</rdfs:label>
        <part:partOf rdf:resource="http://people.aifb.kit.edu/mu2771/step#printing_press"/>
    </owl:NamedIndividual>
    


    <!-- http://people.aifb.kit.edu/mu2771/step#double_sheet_detector -->

    <owl:NamedIndividual rdf:about="http://people.aifb.kit.edu/mu2771/step#double_sheet_detector">
        <rdf:type rdf:resource="http://purl.oclc.org/NET/ssnx/ssn#System"/>
        <owl:sameAs rdf:resource="http://people.aifb.kit.edu/mu2771/step#doubles_detector"/>
        <step:sourceUri rdf:resource="http://people.aifb.kit.edu/mu2771/step#"/>
        <rdfs:label xml:lang="de">Doppelbogenabfühlung</rdfs:label>
        <rdfs:label xml:lang="de">Doppelbogenkontrolle</rdfs:label>
        <rdfs:label xml:lang="en">double sheet control</rdfs:label>
        <rdfs:label xml:lang="en">double sheet detector</rdfs:label>
        <rdfs:label xml:lang="en">doubles detector</rdfs:label>
        <part:partOf rdf:resource="http://people.aifb.kit.edu/mu2771/step#printing_press"/>
    </owl:NamedIndividual>
    


    <!-- http://people.aifb.kit.edu/mu2771/step#doubles_detector -->

    <owl:NamedIndividual rdf:about="http://people.aifb.kit.edu/mu2771/step#doubles_detector">
        <rdf:type rdf:resource="http://purl.oclc.org/NET/ssnx/ssn#System"/>
        <step:sourceUri rdf:resource="http://people.aifb.kit.edu/mu2771/step#"/>
        <rdfs:label xml:lang="de">Doppelbogenabfühlung</rdfs:label>
        <rdfs:label xml:lang="de">Doppelbogenkontrolle</rdfs:label>
        <rdfs:label xml:lang="en">double sheet control</rdfs:label>
        <rdfs:label xml:lang="en">double sheet detector</rdfs:label>
        <rdfs:label xml:lang="en">doubles detector</rdfs:label>
        <part:partOf rdf:resource="http://people.aifb.kit.edu/mu2771/step#printing_press"/>
    </owl:NamedIndividual>
    


    <!-- http://people.aifb.kit.edu/mu2771/step#dryer -->

    <owl:NamedIndividual rdf:about="http://people.aifb.kit.edu/mu2771/step#dryer">
        <rdf:type rdf:resource="http://purl.oclc.org/NET/ssnx/ssn#Device"/>
        <dc:creator rdf:resource="http://www.heidelberg.com/"/>
        <rdfs:label xml:lang="de">Trockner</rdfs:label>
        <rdfs:label xml:lang="en">dryer</rdfs:label>
    </owl:NamedIndividual>
    


    <!-- http://people.aifb.kit.edu/mu2771/step#dryer_control_cabinet -->

    <owl:NamedIndividual rdf:about="http://people.aifb.kit.edu/mu2771/step#dryer_control_cabinet">
        <rdf:type rdf:resource="http://purl.oclc.org/NET/ssnx/ssn#System"/>
        <dc:creator rdf:resource="http://www.heidelberg.com/"/>
        <rdfs:label xml:lang="de">Trocknerschaltschrank</rdfs:label>
        <rdfs:label xml:lang="en">dryer control cabinet</rdfs:label>
        <part:partOf rdf:resource="http://people.aifb.kit.edu/mu2771/step#dryer"/>
    </owl:NamedIndividual>
    


    <!-- http://people.aifb.kit.edu/mu2771/step#duct-adjusting_screw -->

    <owl:NamedIndividual rdf:about="http://people.aifb.kit.edu/mu2771/step#duct-adjusting_screw">
        <rdf:type rdf:resource="http://purl.oclc.org/NET/ssnx/ssn#Device"/>
        <owl:sameAs rdf:resource="http://people.aifb.kit.edu/mu2771/step#ink_fountain_key"/>
        <step:sourceUri rdf:resource="http://people.aifb.kit.edu/mu2771/step#"/>
        <rdfs:label xml:lang="de">Farbzonenschraube</rdfs:label>
        <rdfs:label xml:lang="de">Zonenschraube</rdfs:label>
        <rdfs:label xml:lang="en">duct-adjusting screw</rdfs:label>
        <part:partOf rdf:resource="http://people.aifb.kit.edu/mu2771/step#printing_press"/>
    </owl:NamedIndividual>
    


    <!-- http://people.aifb.kit.edu/mu2771/step#ductor -->

    <owl:NamedIndividual rdf:about="http://people.aifb.kit.edu/mu2771/step#ductor">
        <rdf:type rdf:resource="http://purl.oclc.org/NET/ssnx/ssn#Device"/>
        <owl:sameAs rdf:resource="http://people.aifb.kit.edu/mu2771/step#ink_duct_roller"/>
        <owl:sameAs rdf:resource="http://people.aifb.kit.edu/mu2771/step#print_ink_ductor"/>
        <step:sourceUri rdf:resource="http://people.aifb.kit.edu/mu2771/step#"/>
        <rdfs:label xml:lang="de">Farbkastenwalze</rdfs:label>
        <rdfs:label xml:lang="en">ductor</rdfs:label>
        <part:partOf rdf:resource="http://people.aifb.kit.edu/mu2771/step#printing_press"/>
    </owl:NamedIndividual>
    


    <!-- http://people.aifb.kit.edu/mu2771/step#dwba -->

    <owl:NamedIndividual rdf:about="http://people.aifb.kit.edu/mu2771/step#dwba">
        <rdf:type rdf:resource="http://purl.oclc.org/NET/ssnx/ssn#Sensing"/>
        <dc:creator rdf:resource="http://www.aifb.kit.edu/web/Sebastian_Bader"/>
        <rdfs:label xml:lang="de">Bornsche Näherung mit gestörten Wellen</rdfs:label>
        <rdfs:label xml:lang="en">DWBA</rdfs:label>
        <rdfs:label xml:lang="en">distorted-wave born approximation</rdfs:label>
    </owl:NamedIndividual>
    


    <!-- http://people.aifb.kit.edu/mu2771/step#engine_delivery_wheel -->

    <owl:NamedIndividual rdf:about="http://people.aifb.kit.edu/mu2771/step#engine_delivery_wheel">
        <rdf:type rdf:resource="http://purl.oclc.org/NET/ssnx/ssn#Device"/>
        <step:sourceUri rdf:resource="http://people.aifb.kit.edu/mu2771/step#"/>
        <rdfs:label xml:lang="de">Auslegerrad</rdfs:label>
        <rdfs:label xml:lang="en">engine delivery wheel</rdfs:label>
        <part:partOf rdf:resource="http://people.aifb.kit.edu/mu2771/step#printing_press"/>
    </owl:NamedIndividual>
    


    <!-- http://people.aifb.kit.edu/mu2771/step#fan -->

    <owl:NamedIndividual rdf:about="http://people.aifb.kit.edu/mu2771/step#fan">
        <rdf:type rdf:resource="http://purl.oclc.org/NET/ssnx/ssn#Device"/>
        <dc:creator rdf:resource="http://www.heidelberg.com/"/>
        <rdfs:label xml:lang="de">Lüfter</rdfs:label>
        <rdfs:label xml:lang="de">Ventilator</rdfs:label>
        <rdfs:label xml:lang="en">fan</rdfs:label>
        <part:partOf rdf:resource="http://people.aifb.kit.edu/mu2771/step#dryer"/>
    </owl:NamedIndividual>
    


    <!-- http://people.aifb.kit.edu/mu2771/step#forwarding_roller -->

    <owl:NamedIndividual rdf:about="http://people.aifb.kit.edu/mu2771/step#forwarding_roller">
        <rdf:type rdf:resource="http://purl.oclc.org/NET/ssnx/ssn#Device"/>
        <dc:creator rdf:resource="http://www.heidelberg.com/"/>
        <rdfs:label xml:lang="de">Taktrolle</rdfs:label>
        <rdfs:label xml:lang="en">forwarding roller</rdfs:label>
        <part:partOf rdf:resource="http://people.aifb.kit.edu/mu2771/step#dampener_roll"/>
        <part:partOf rdf:resource="http://people.aifb.kit.edu/mu2771/step#dampening_form_roller"/>
    </owl:NamedIndividual>
    


    <!-- http://people.aifb.kit.edu/mu2771/step#fountain_blade -->

    <owl:NamedIndividual rdf:about="http://people.aifb.kit.edu/mu2771/step#fountain_blade">
        <rdf:type rdf:resource="http://purl.oclc.org/NET/ssnx/ssn#Device"/>
        <owl:sameAs rdf:resource="http://people.aifb.kit.edu/mu2771/step#print_ink_blade"/>
        <step:sourceUri rdf:resource="http://people.aifb.kit.edu/mu2771/step#"/>
        <rdfs:label xml:lang="de">Farbmesser</rdfs:label>
        <rdfs:label xml:lang="en">doctor knife</rdfs:label>
        <rdfs:label xml:lang="en">fountain blade</rdfs:label>
        <rdfs:label xml:lang="en">print ink blade</rdfs:label>
        <part:partOf rdf:resource="http://people.aifb.kit.edu/mu2771/step#printing_press"/>
    </owl:NamedIndividual>
    


    <!-- http://people.aifb.kit.edu/mu2771/step#front_lay -->

    <owl:NamedIndividual rdf:about="http://people.aifb.kit.edu/mu2771/step#front_lay">
        <rdf:type rdf:resource="http://purl.oclc.org/NET/ssnx/ssn#System"/>
        <step:sourceUri rdf:resource="http://people.aifb.kit.edu/mu2771/step#"/>
        <rdfs:label xml:lang="de">Vordermarke</rdfs:label>
        <rdfs:label xml:lang="en">front lay</rdfs:label>
        <part:partOf rdf:resource="http://people.aifb.kit.edu/mu2771/step#printing_press"/>
    </owl:NamedIndividual>
    


    <!-- http://people.aifb.kit.edu/mu2771/step#grammage -->

    <owl:NamedIndividual rdf:about="http://people.aifb.kit.edu/mu2771/step#grammage">
        <rdf:type rdf:resource="http://purl.oclc.org/NET/ssnx/ssn#System"/>
        <owl:sameAs rdf:resource="http://people.aifb.kit.edu/mu2771/step#print_color_desk"/>
        <dc:creator rdf:resource="http://www.heidelberg.com/"/>
        <rdfs:label xml:lang="de">Grammatur</rdfs:label>
        <rdfs:label xml:lang="en">grammage</rdfs:label>
    </owl:NamedIndividual>
    


    <!-- http://people.aifb.kit.edu/mu2771/step#gripper_operating_shaft -->

    <owl:NamedIndividual rdf:about="http://people.aifb.kit.edu/mu2771/step#gripper_operating_shaft">
        <rdf:type rdf:resource="http://purl.oclc.org/NET/ssnx/ssn#Device"/>
        <dc:creator rdf:resource="http://www.heidelberg.com/"/>
        <rdfs:label xml:lang="de">Greiferwelle</rdfs:label>
        <rdfs:label xml:lang="en">gripper operating shaft</rdfs:label>
        <part:partOf rdf:resource="http://people.aifb.kit.edu/mu2771/step#printing_press"/>
    </owl:NamedIndividual>
    


    <!-- http://people.aifb.kit.edu/mu2771/step#guide -->

    <owl:NamedIndividual rdf:about="http://people.aifb.kit.edu/mu2771/step#guide">
        <rdf:type rdf:resource="http://purl.oclc.org/NET/ssnx/ssn#Device"/>
        <dc:creator rdf:resource="http://www.aifb.kit.edu/web/Sebastian_Bader"/>
        <rdfs:label xml:lang="de">Leiteinrichtung</rdfs:label>
        <rdfs:label xml:lang="en">guide</rdfs:label>
        <part:partOf rdf:resource="http://people.aifb.kit.edu/mu2771/step#indent"/>
    </owl:NamedIndividual>
    


    <!-- http://people.aifb.kit.edu/mu2771/step#heat_transfer_compound -->

    <owl:NamedIndividual rdf:about="http://people.aifb.kit.edu/mu2771/step#heat_transfer_compound">
        <rdf:type rdf:resource="http://people.aifb.kit.edu/mu2771/step#Spare_Part"/>
        <dc:creator rdf:resource="http://www.heidelberg.com/"/>
        <rdfs:label xml:lang="de">Wärmeleitpaste</rdfs:label>
        <rdfs:label xml:lang="en">heat transfer compound</rdfs:label>
    </owl:NamedIndividual>
    


    <!-- http://people.aifb.kit.edu/mu2771/step#impression_cylinder -->

    <owl:NamedIndividual rdf:about="http://people.aifb.kit.edu/mu2771/step#impression_cylinder">
        <rdf:type rdf:resource="http://purl.oclc.org/NET/ssnx/ssn#System"/>
        <owl:sameAs rdf:resource="http://people.aifb.kit.edu/mu2771/step#print_counter-pressure_cylinder_"/>
        <owl:sameAs rdf:resource="http://people.aifb.kit.edu/mu2771/step#print_counterpressure_cylinder_"/>
        <owl:sameAs rdf:resource="http://people.aifb.kit.edu/mu2771/step#printing_cylinder"/>
        <step:sourceUri rdf:resource="http://people.aifb.kit.edu/mu2771/step#"/>
        <rdfs:label xml:lang="de">Gegendruckzylinder</rdfs:label>
        <rdfs:label xml:lang="en">impression cylinder</rdfs:label>
        <part:partOf rdf:resource="http://people.aifb.kit.edu/mu2771/step#ink_train"/>
        <part:partOf rdf:resource="http://people.aifb.kit.edu/mu2771/step#inking_station"/>
        <part:partOf rdf:resource="http://people.aifb.kit.edu/mu2771/step#inking_system"/>
        <part:partOf rdf:resource="http://people.aifb.kit.edu/mu2771/step#inking_unit"/>
        <part:partOf rdf:resource="http://people.aifb.kit.edu/mu2771/step#take-up_roller"/>
    </owl:NamedIndividual>
    


    <!-- http://people.aifb.kit.edu/mu2771/step#indent -->

    <owl:NamedIndividual rdf:about="http://people.aifb.kit.edu/mu2771/step#indent">
        <rdf:type rdf:resource="http://purl.oclc.org/NET/ssnx/ssn#Device"/>
        <dc:creator rdf:resource="http://www.aifb.kit.edu/web/Sebastian_Bader"/>
        <rdfs:label xml:lang="de">Einzug</rdfs:label>
        <rdfs:label xml:lang="en">indent</rdfs:label>
        <part:partOf rdf:resource="http://people.aifb.kit.edu/mu2771/step#printing_press"/>
    </owl:NamedIndividual>
    


    <!-- http://people.aifb.kit.edu/mu2771/step#ink_density -->

    <owl:NamedIndividual rdf:about="http://people.aifb.kit.edu/mu2771/step#ink_density">
        <rdf:type rdf:resource="http://qudt.org/schema/qudt#Dimension"/>
        <dc:creator rdf:resource="http://www.heidelberg.com/"/>
        <rdfs:label xml:lang="de">Farbdichte</rdfs:label>
        <rdfs:label xml:lang="en">ink density</rdfs:label>
    </owl:NamedIndividual>
    


    <!-- http://people.aifb.kit.edu/mu2771/step#ink_duct_roller -->

    <owl:NamedIndividual rdf:about="http://people.aifb.kit.edu/mu2771/step#ink_duct_roller">
        <rdf:type rdf:resource="http://purl.oclc.org/NET/ssnx/ssn#Device"/>
        <owl:sameAs rdf:resource="http://people.aifb.kit.edu/mu2771/step#print_ink_ductor"/>
        <step:sourceUri rdf:resource="http://people.aifb.kit.edu/mu2771/step#"/>
        <rdfs:label xml:lang="en">(ink) duct roller</rdfs:label>
        <rdfs:label xml:lang="de">Farbduktor</rdfs:label>
        <rdfs:label xml:lang="de">Farbduktorwalze</rdfs:label>
        <rdfs:label xml:lang="de">Farbduktorzylinder</rdfs:label>
        <rdfs:label xml:lang="de">Farbkastenwalze</rdfs:label>
        <rdfs:label xml:lang="en">duct roller</rdfs:label>
        <rdfs:label xml:lang="en">ductor</rdfs:label>
        <rdfs:label xml:lang="en">ink duct roller</rdfs:label>
        <rdfs:label xml:lang="en">print ink ductor</rdfs:label>
        <part:partOf rdf:resource="http://people.aifb.kit.edu/mu2771/step#printing_press"/>
    </owl:NamedIndividual>
    


    <!-- http://people.aifb.kit.edu/mu2771/step#ink_ductor -->

    <owl:NamedIndividual rdf:about="http://people.aifb.kit.edu/mu2771/step#ink_ductor">
        <rdf:type rdf:resource="http://purl.oclc.org/NET/ssnx/ssn#Device"/>
        <owl:sameAs rdf:resource="http://people.aifb.kit.edu/mu2771/step#ink_fountain_roller"/>
        <step:sourceUri rdf:resource="http://people.aifb.kit.edu/mu2771/step#"/>
        <rdfs:label xml:lang="de">Farbduktor</rdfs:label>
        <rdfs:label xml:lang="de">Farbduktorwalze</rdfs:label>
        <rdfs:label xml:lang="de">Farbduktorzylinder</rdfs:label>
        <rdfs:label xml:lang="en">ink ductor</rdfs:label>
        <part:partOf rdf:resource="http://people.aifb.kit.edu/mu2771/step#ink_train"/>
        <part:partOf rdf:resource="http://people.aifb.kit.edu/mu2771/step#inking_station"/>
        <part:partOf rdf:resource="http://people.aifb.kit.edu/mu2771/step#inking_system"/>
        <part:partOf rdf:resource="http://people.aifb.kit.edu/mu2771/step#inking_unit"/>
        <part:partOf rdf:resource="http://people.aifb.kit.edu/mu2771/step#take-up_roller"/>
    </owl:NamedIndividual>
    


    <!-- http://people.aifb.kit.edu/mu2771/step#ink_feed_roller -->

    <owl:NamedIndividual rdf:about="http://people.aifb.kit.edu/mu2771/step#ink_feed_roller">
        <rdf:type rdf:resource="http://purl.oclc.org/NET/ssnx/ssn#Device"/>
        <step:sourceUri rdf:resource="http://people.aifb.kit.edu/mu2771/step#"/>
        <rdfs:label xml:lang="de">Farbheberwalze</rdfs:label>
        <rdfs:label xml:lang="en">ink feed roller</rdfs:label>
        <part:partOf rdf:resource="http://people.aifb.kit.edu/mu2771/step#ink_train"/>
        <part:partOf rdf:resource="http://people.aifb.kit.edu/mu2771/step#inking_station"/>
        <part:partOf rdf:resource="http://people.aifb.kit.edu/mu2771/step#inking_system"/>
        <part:partOf rdf:resource="http://people.aifb.kit.edu/mu2771/step#inking_unit"/>
        <part:partOf rdf:resource="http://people.aifb.kit.edu/mu2771/step#take-up_roller"/>
    </owl:NamedIndividual>
    


    <!-- http://people.aifb.kit.edu/mu2771/step#ink_fountain_key -->

    <owl:NamedIndividual rdf:about="http://people.aifb.kit.edu/mu2771/step#ink_fountain_key">
        <rdf:type rdf:resource="http://purl.oclc.org/NET/ssnx/ssn#Device"/>
        <step:sourceUri rdf:resource="http://people.aifb.kit.edu/mu2771/step#"/>
        <rdfs:label xml:lang="de">Farbzonenschraube</rdfs:label>
        <rdfs:label xml:lang="de">Zonenschraube</rdfs:label>
        <rdfs:label xml:lang="en">duct-adjusting screw</rdfs:label>
        <rdfs:label xml:lang="en">ink (fountain) key</rdfs:label>
        <rdfs:label xml:lang="en">ink fountain key</rdfs:label>
        <rdfs:label xml:lang="en">ink key</rdfs:label>
        <part:partOf rdf:resource="http://people.aifb.kit.edu/mu2771/step#printing_press"/>
    </owl:NamedIndividual>
    


    <!-- http://people.aifb.kit.edu/mu2771/step#ink_fountain_roller -->

    <owl:NamedIndividual rdf:about="http://people.aifb.kit.edu/mu2771/step#ink_fountain_roller">
        <rdf:type rdf:resource="http://purl.oclc.org/NET/ssnx/ssn#Device"/>
        <step:sourceUri rdf:resource="http://people.aifb.kit.edu/mu2771/step#"/>
        <rdfs:label xml:lang="de">Farbduktor</rdfs:label>
        <rdfs:label xml:lang="de">Farbduktorwalze</rdfs:label>
        <rdfs:label xml:lang="de">Farbduktorzylinder</rdfs:label>
        <rdfs:label xml:lang="de">Farbkastenwalze</rdfs:label>
        <rdfs:label xml:lang="en">ink ductor</rdfs:label>
        <rdfs:label xml:lang="en">ink fountain roller</rdfs:label>
        <part:partOf rdf:resource="http://people.aifb.kit.edu/mu2771/step#ink_train"/>
        <part:partOf rdf:resource="http://people.aifb.kit.edu/mu2771/step#inking_station"/>
        <part:partOf rdf:resource="http://people.aifb.kit.edu/mu2771/step#inking_system"/>
        <part:partOf rdf:resource="http://people.aifb.kit.edu/mu2771/step#inking_unit"/>
        <part:partOf rdf:resource="http://people.aifb.kit.edu/mu2771/step#take-up_roller"/>
    </owl:NamedIndividual>
    


    <!-- http://people.aifb.kit.edu/mu2771/step#ink_roller -->

    <owl:NamedIndividual rdf:about="http://people.aifb.kit.edu/mu2771/step#ink_roller">
        <rdf:type rdf:resource="http://purl.oclc.org/NET/ssnx/ssn#Device"/>
        <owl:sameAs rdf:resource="http://people.aifb.kit.edu/mu2771/step#inker"/>
        <owl:sameAs rdf:resource="http://people.aifb.kit.edu/mu2771/step#inking_roller"/>
        <step:sourceUri rdf:resource="http://people.aifb.kit.edu/mu2771/step#"/>
        <rdfs:label xml:lang="de">Farbwalze</rdfs:label>
        <rdfs:label xml:lang="de">Farbzylinder</rdfs:label>
        <rdfs:label xml:lang="en">ink roller</rdfs:label>
        <part:partOf rdf:resource="http://people.aifb.kit.edu/mu2771/step#ink_train"/>
        <part:partOf rdf:resource="http://people.aifb.kit.edu/mu2771/step#inking_station"/>
        <part:partOf rdf:resource="http://people.aifb.kit.edu/mu2771/step#inking_system"/>
        <part:partOf rdf:resource="http://people.aifb.kit.edu/mu2771/step#inking_unit"/>
        <part:partOf rdf:resource="http://people.aifb.kit.edu/mu2771/step#take-up_roller"/>
    </owl:NamedIndividual>
    


    <!-- http://people.aifb.kit.edu/mu2771/step#ink_train -->

    <owl:NamedIndividual rdf:about="http://people.aifb.kit.edu/mu2771/step#ink_train">
        <rdf:type rdf:resource="http://purl.oclc.org/NET/ssnx/ssn#System"/>
        <owl:sameAs rdf:resource="http://people.aifb.kit.edu/mu2771/step#inking_station"/>
        <owl:sameAs rdf:resource="http://people.aifb.kit.edu/mu2771/step#inking_system"/>
        <owl:sameAs rdf:resource="http://people.aifb.kit.edu/mu2771/step#inking_unit"/>
        <owl:sameAs rdf:resource="http://people.aifb.kit.edu/mu2771/step#take-up_roller"/>
        <step:sourceUri rdf:resource="http://people.aifb.kit.edu/mu2771/step#"/>
        <rdfs:label xml:lang="de">Farbwerk</rdfs:label>
        <rdfs:label xml:lang="en">ink train</rdfs:label>
        <part:partOf rdf:resource="http://people.aifb.kit.edu/mu2771/step#printing_press"/>
    </owl:NamedIndividual>
    


    <!-- http://people.aifb.kit.edu/mu2771/step#ink_vibrator -->

    <owl:NamedIndividual rdf:about="http://people.aifb.kit.edu/mu2771/step#ink_vibrator">
        <rdf:type rdf:resource="http://purl.oclc.org/NET/ssnx/ssn#Device"/>
        <step:sourceUri rdf:resource="http://people.aifb.kit.edu/mu2771/step#"/>
        <rdfs:label xml:lang="de">Farbheber</rdfs:label>
        <rdfs:label xml:lang="de">Farbheberwalze</rdfs:label>
        <rdfs:label xml:lang="en">ink vibrator</rdfs:label>
        <part:partOf rdf:resource="http://people.aifb.kit.edu/mu2771/step#ink_train"/>
        <part:partOf rdf:resource="http://people.aifb.kit.edu/mu2771/step#inking_station"/>
        <part:partOf rdf:resource="http://people.aifb.kit.edu/mu2771/step#inking_system"/>
        <part:partOf rdf:resource="http://people.aifb.kit.edu/mu2771/step#inking_unit"/>
        <part:partOf rdf:resource="http://people.aifb.kit.edu/mu2771/step#take-up_roller"/>
    </owl:NamedIndividual>
    


    <!-- http://people.aifb.kit.edu/mu2771/step#ink_zone_key -->

    <owl:NamedIndividual rdf:about="http://people.aifb.kit.edu/mu2771/step#ink_zone_key">
        <rdf:type rdf:resource="http://purl.oclc.org/NET/ssnx/ssn#Device"/>
        <step:sourceUri rdf:resource="http://people.aifb.kit.edu/mu2771/step#"/>
        <rdfs:label xml:lang="de">Farbzonenschraube</rdfs:label>
        <rdfs:label xml:lang="de">Zonenschraube</rdfs:label>
        <rdfs:label xml:lang="en">ink zone key</rdfs:label>
        <part:partOf rdf:resource="http://people.aifb.kit.edu/mu2771/step#ink_train"/>
        <part:partOf rdf:resource="http://people.aifb.kit.edu/mu2771/step#inking_station"/>
        <part:partOf rdf:resource="http://people.aifb.kit.edu/mu2771/step#inking_system"/>
        <part:partOf rdf:resource="http://people.aifb.kit.edu/mu2771/step#inking_unit"/>
        <part:partOf rdf:resource="http://people.aifb.kit.edu/mu2771/step#take-up_roller"/>
    </owl:NamedIndividual>
    


    <!-- http://people.aifb.kit.edu/mu2771/step#inker -->

    <owl:NamedIndividual rdf:about="http://people.aifb.kit.edu/mu2771/step#inker">
        <rdf:type rdf:resource="http://purl.oclc.org/NET/ssnx/ssn#Device"/>
        <owl:sameAs rdf:resource="http://people.aifb.kit.edu/mu2771/step#inking_roller"/>
        <step:sourceUri rdf:resource="http://people.aifb.kit.edu/mu2771/step#"/>
        <rdfs:label xml:lang="de">Farbwalze</rdfs:label>
        <rdfs:label xml:lang="de">Farbzylinder</rdfs:label>
        <rdfs:label xml:lang="en">ink roller</rdfs:label>
        <rdfs:label xml:lang="en">inker</rdfs:label>
        <rdfs:label xml:lang="en">inking roller</rdfs:label>
        <part:partOf rdf:resource="http://people.aifb.kit.edu/mu2771/step#ink_train"/>
        <part:partOf rdf:resource="http://people.aifb.kit.edu/mu2771/step#inking_station"/>
        <part:partOf rdf:resource="http://people.aifb.kit.edu/mu2771/step#inking_system"/>
        <part:partOf rdf:resource="http://people.aifb.kit.edu/mu2771/step#inking_unit"/>
        <part:partOf rdf:resource="http://people.aifb.kit.edu/mu2771/step#printing_press"/>
        <part:partOf rdf:resource="http://people.aifb.kit.edu/mu2771/step#take-up_roller"/>
    </owl:NamedIndividual>
    


    <!-- http://people.aifb.kit.edu/mu2771/step#inking-unit_drive -->

    <owl:NamedIndividual rdf:about="http://people.aifb.kit.edu/mu2771/step#inking-unit_drive">
        <rdf:type rdf:resource="http://purl.oclc.org/NET/ssnx/ssn#Device"/>
        <step:sourceUri rdf:resource="http://people.aifb.kit.edu/mu2771/step#"/>
        <rdfs:label xml:lang="de">Farbwerkantrieb</rdfs:label>
        <rdfs:label xml:lang="en">inking-unit drive</rdfs:label>
        <part:partOf rdf:resource="http://people.aifb.kit.edu/mu2771/step#ink_train"/>
        <part:partOf rdf:resource="http://people.aifb.kit.edu/mu2771/step#inking_station"/>
        <part:partOf rdf:resource="http://people.aifb.kit.edu/mu2771/step#inking_system"/>
        <part:partOf rdf:resource="http://people.aifb.kit.edu/mu2771/step#inking_unit"/>
        <part:partOf rdf:resource="http://people.aifb.kit.edu/mu2771/step#take-up_roller"/>
    </owl:NamedIndividual>
    


    <!-- http://people.aifb.kit.edu/mu2771/step#inking_form_roller -->

    <owl:NamedIndividual rdf:about="http://people.aifb.kit.edu/mu2771/step#inking_form_roller">
        <rdf:type rdf:resource="http://purl.oclc.org/NET/ssnx/ssn#Device"/>
        <dc:creator rdf:resource="http://www.heidelberg.com/"/>
        <rdfs:label xml:lang="de">Farbauftragwalze</rdfs:label>
        <rdfs:label xml:lang="en">inking form roller</rdfs:label>
        <part:partOf rdf:resource="http://people.aifb.kit.edu/mu2771/step#ink_duct_roller"/>
        <part:partOf rdf:resource="http://people.aifb.kit.edu/mu2771/step#print_ink_ductor"/>
    </owl:NamedIndividual>
    


    <!-- http://people.aifb.kit.edu/mu2771/step#inking_roller -->

    <owl:NamedIndividual rdf:about="http://people.aifb.kit.edu/mu2771/step#inking_roller">
        <rdf:type rdf:resource="http://purl.oclc.org/NET/ssnx/ssn#Device"/>
        <step:sourceUri rdf:resource="http://people.aifb.kit.edu/mu2771/step#"/>
        <rdfs:label xml:lang="de">Farbwalze</rdfs:label>
        <rdfs:label xml:lang="de">Farbzylinder</rdfs:label>
        <rdfs:label xml:lang="en">ink roller</rdfs:label>
        <rdfs:label xml:lang="en">inker</rdfs:label>
        <rdfs:label xml:lang="en">inking roller</rdfs:label>
        <part:partOf rdf:resource="http://people.aifb.kit.edu/mu2771/step#ink_train"/>
        <part:partOf rdf:resource="http://people.aifb.kit.edu/mu2771/step#inking_station"/>
        <part:partOf rdf:resource="http://people.aifb.kit.edu/mu2771/step#inking_system"/>
        <part:partOf rdf:resource="http://people.aifb.kit.edu/mu2771/step#inking_unit"/>
        <part:partOf rdf:resource="http://people.aifb.kit.edu/mu2771/step#printing_press"/>
        <part:partOf rdf:resource="http://people.aifb.kit.edu/mu2771/step#take-up_roller"/>
    </owl:NamedIndividual>
    


    <!-- http://people.aifb.kit.edu/mu2771/step#inking_station -->

    <owl:NamedIndividual rdf:about="http://people.aifb.kit.edu/mu2771/step#inking_station">
        <rdf:type rdf:resource="http://purl.oclc.org/NET/ssnx/ssn#Device"/>
        <rdf:type rdf:resource="http://purl.oclc.org/NET/ssnx/ssn#System"/>
        <owl:sameAs rdf:resource="http://people.aifb.kit.edu/mu2771/step#inking_system"/>
        <owl:sameAs rdf:resource="http://people.aifb.kit.edu/mu2771/step#inking_unit"/>
        <owl:sameAs rdf:resource="http://people.aifb.kit.edu/mu2771/step#take-up_roller"/>
        <step:sourceUri rdf:resource="http://people.aifb.kit.edu/mu2771/step#"/>
        <rdfs:label xml:lang="de">Farbheber</rdfs:label>
        <rdfs:label xml:lang="de">Farbwerk</rdfs:label>
        <rdfs:label xml:lang="en">ink train</rdfs:label>
        <rdfs:label xml:lang="en">inking station</rdfs:label>
        <rdfs:label xml:lang="en">inking system</rdfs:label>
        <rdfs:label xml:lang="en">inking unit</rdfs:label>
        <rdfs:label xml:lang="en">take-up roller</rdfs:label>
        <part:partOf rdf:resource="http://people.aifb.kit.edu/mu2771/step#printing_press"/>
    </owl:NamedIndividual>
    


    <!-- http://people.aifb.kit.edu/mu2771/step#inking_system -->

    <owl:NamedIndividual rdf:about="http://people.aifb.kit.edu/mu2771/step#inking_system">
        <rdf:type rdf:resource="http://purl.oclc.org/NET/ssnx/ssn#Device"/>
        <rdf:type rdf:resource="http://purl.oclc.org/NET/ssnx/ssn#System"/>
        <owl:sameAs rdf:resource="http://people.aifb.kit.edu/mu2771/step#inking_unit"/>
        <owl:sameAs rdf:resource="http://people.aifb.kit.edu/mu2771/step#take-up_roller"/>
        <step:sourceUri rdf:resource="http://people.aifb.kit.edu/mu2771/step#"/>
        <rdfs:label xml:lang="de">Farbheber</rdfs:label>
        <rdfs:label xml:lang="de">Farbwerk</rdfs:label>
        <rdfs:label xml:lang="en">ink train</rdfs:label>
        <rdfs:label xml:lang="en">inking station</rdfs:label>
        <rdfs:label xml:lang="en">inking system</rdfs:label>
        <rdfs:label xml:lang="en">inking unit</rdfs:label>
        <rdfs:label xml:lang="en">take-up roller</rdfs:label>
        <part:partOf rdf:resource="http://people.aifb.kit.edu/mu2771/step#printing_press"/>
    </owl:NamedIndividual>
    


    <!-- http://people.aifb.kit.edu/mu2771/step#inking_unit -->

    <owl:NamedIndividual rdf:about="http://people.aifb.kit.edu/mu2771/step#inking_unit">
        <rdf:type rdf:resource="http://purl.oclc.org/NET/ssnx/ssn#Device"/>
        <rdf:type rdf:resource="http://purl.oclc.org/NET/ssnx/ssn#System"/>
        <owl:sameAs rdf:resource="http://people.aifb.kit.edu/mu2771/step#take-up_roller"/>
        <step:sourceUri rdf:resource="http://people.aifb.kit.edu/mu2771/step#"/>
        <rdfs:label xml:lang="de">Farbheber</rdfs:label>
        <rdfs:label xml:lang="de">Farbwerk</rdfs:label>
        <rdfs:label xml:lang="en">ink train</rdfs:label>
        <rdfs:label xml:lang="en">inking station</rdfs:label>
        <rdfs:label xml:lang="en">inking system</rdfs:label>
        <rdfs:label xml:lang="en">inking unit</rdfs:label>
        <rdfs:label xml:lang="en">take-up roller</rdfs:label>
        <part:partOf rdf:resource="http://people.aifb.kit.edu/mu2771/step#printing_press"/>
    </owl:NamedIndividual>
    


    <!-- http://people.aifb.kit.edu/mu2771/step#installation -->

    <owl:NamedIndividual rdf:about="http://people.aifb.kit.edu/mu2771/step#installation">
        <rdf:type rdf:resource="http://people.aifb.kit.edu/mu2771/step#Process"/>
        <dc:creator rdf:resource="http://www.heidelberg.com/"/>
        <rdfs:label xml:lang="de">Installation</rdfs:label>
        <rdfs:label xml:lang="en">installation</rdfs:label>
    </owl:NamedIndividual>
    


    <!-- http://people.aifb.kit.edu/mu2771/step#interface -->

    <owl:Thing rdf:about="http://people.aifb.kit.edu/mu2771/step#interface">
        <rdf:type rdf:resource="http://www.w3.org/2002/07/owl#NamedIndividual"/>
        <dc:creator rdf:resource="http://www.heidelberg.com/"/>
        <rdfs:label xml:lang="de">Interface</rdfs:label>
        <rdfs:label xml:lang="en">interface</rdfs:label>
    </owl:Thing>
    


    <!-- http://people.aifb.kit.edu/mu2771/step#keyboard -->

    <owl:NamedIndividual rdf:about="http://people.aifb.kit.edu/mu2771/step#keyboard">
        <rdf:type rdf:resource="http://purl.oclc.org/NET/ssnx/ssn#Device"/>
        <dc:creator rdf:resource="http://www.heidelberg.com/"/>
        <rdfs:label xml:lang="de">Tastatur</rdfs:label>
        <rdfs:label xml:lang="en">keyboard</rdfs:label>
        <part:partOf rdf:resource="http://people.aifb.kit.edu/mu2771/step#control_console"/>
    </owl:NamedIndividual>
    


    <!-- http://people.aifb.kit.edu/mu2771/step#light-barrier -->

    <owl:NamedIndividual rdf:about="http://people.aifb.kit.edu/mu2771/step#light-barrier">
        <rdf:type rdf:resource="http://purl.oclc.org/NET/ssnx/ssn#Device"/>
        <dc:creator rdf:resource="http://www.aifb.kit.edu/web/Sebastian_Bader"/>
        <rdfs:label xml:lang="de">Lichtschranke</rdfs:label>
        <rdfs:label xml:lang="en">light barrier</rdfs:label>
        <rdfs:label xml:lang="en">photoelectric barrier</rdfs:label>
        <part:partOf rdf:resource="http://people.aifb.kit.edu/mu2771/step#indent"/>
    </owl:NamedIndividual>
    


    <!-- http://people.aifb.kit.edu/mu2771/step#main_connection -->

    <owl:NamedIndividual rdf:about="http://people.aifb.kit.edu/mu2771/step#main_connection">
        <rdf:type rdf:resource="http://purl.oclc.org/NET/ssnx/ssn#Device"/>
        <dc:creator rdf:resource="http://www.heidelberg.com/"/>
        <rdfs:label xml:lang="de">Netzanschluss</rdfs:label>
        <rdfs:label xml:lang="en">main connection</rdfs:label>
        <part:partOf rdf:resource="http://people.aifb.kit.edu/mu2771/step#central_control_cabinet"/>
        <part:partOf rdf:resource="http://people.aifb.kit.edu/mu2771/step#dryer_control_cabinet"/>
    </owl:NamedIndividual>
    


    <!-- http://people.aifb.kit.edu/mu2771/step#main_pile -->

    <owl:NamedIndividual rdf:about="http://people.aifb.kit.edu/mu2771/step#main_pile">
        <rdf:type rdf:resource="http://people.aifb.kit.edu/mu2771/step#Product"/>
        <dc:creator rdf:resource="http://www.heidelberg.com/"/>
        <rdfs:label xml:lang="de">Hauptstapel</rdfs:label>
        <rdfs:label xml:lang="en">main pile</rdfs:label>
        <part:partOf rdf:resource="http://people.aifb.kit.edu/mu2771/step#"/>
    </owl:NamedIndividual>
    


    <!-- http://people.aifb.kit.edu/mu2771/step#maintenance_work -->

    <owl:NamedIndividual rdf:about="http://people.aifb.kit.edu/mu2771/step#maintenance_work">
        <rdf:type rdf:resource="http://people.aifb.kit.edu/mu2771/step#Process"/>
        <dc:creator rdf:resource="http://www.heidelberg.com/"/>
        <rdfs:label xml:lang="de">Wartungstätigkeit</rdfs:label>
        <rdfs:label xml:lang="en">maintenance</rdfs:label>
        <rdfs:label xml:lang="en">maintenance work</rdfs:label>
        <part:partOf rdf:resource="http://people.aifb.kit.edu/mu2771/step#preloading_device"/>
    </owl:NamedIndividual>
    


    <!-- http://people.aifb.kit.edu/mu2771/step#makeready -->

    <owl:NamedIndividual rdf:about="http://people.aifb.kit.edu/mu2771/step#makeready">
        <rdf:type rdf:resource="http://people.aifb.kit.edu/mu2771/step#Process"/>
        <dc:creator rdf:resource="http://www.heidelberg.com/"/>
        <rdfs:label xml:lang="de">Einrichten</rdfs:label>
        <rdfs:label xml:lang="en">make ready</rdfs:label>
        <rdfs:label xml:lang="en">makeready</rdfs:label>
    </owl:NamedIndividual>
    


    <!-- http://people.aifb.kit.edu/mu2771/step#malfunction -->

    <owl:NamedIndividual rdf:about="http://people.aifb.kit.edu/mu2771/step#malfunction">
        <rdf:type rdf:resource="http://vocab.datex.org/terms#equipmentOrSystemFaultType"/>
        <dc:creator rdf:resource="http://www.aifb.kit.edu/web/Sebastian_Bader"/>
        <rdfs:label xml:lang="de">Ausfall</rdfs:label>
        <rdfs:label xml:lang="de">Fehlfunktion</rdfs:label>
        <rdfs:label xml:lang="en">malfunction</rdfs:label>
    </owl:NamedIndividual>
    


    <!-- http://people.aifb.kit.edu/mu2771/step#matt_coated -->

    <owl:NamedIndividual rdf:about="http://people.aifb.kit.edu/mu2771/step#matt_coated">
        <dc:creator rdf:resource="http://www.heidelberg.com/"/>
        <rdfs:label xml:lang="en">matt coated</rdfs:label>
        <rdfs:label xml:lang="de">matt gestrichen</rdfs:label>
    </owl:NamedIndividual>
    


    <!-- http://people.aifb.kit.edu/mu2771/step#measured_value -->

    <owl:Thing rdf:about="http://people.aifb.kit.edu/mu2771/step#measured_value">
        <rdf:type rdf:resource="http://www.w3.org/2002/07/owl#NamedIndividual"/>
        <dc:creator rdf:resource="http://www.heidelberg.com/"/>
        <rdfs:label xml:lang="de">Messwert</rdfs:label>
        <rdfs:label xml:lang="en">measured value</rdfs:label>
    </owl:Thing>
    


    <!-- http://people.aifb.kit.edu/mu2771/step#moistener -->

    <owl:NamedIndividual rdf:about="http://people.aifb.kit.edu/mu2771/step#moistener">
        <rdf:type rdf:resource="http://purl.oclc.org/NET/ssnx/ssn#Device"/>
        <rdf:type rdf:resource="http://purl.oclc.org/NET/ssnx/ssn#System"/>
        <owl:sameAs rdf:resource="http://people.aifb.kit.edu/mu2771/step#print_dampener"/>
        <step:sourceUri rdf:resource="http://people.aifb.kit.edu/mu2771/step#"/>
        <rdfs:label xml:lang="de">Feuchtauftragwalze</rdfs:label>
        <rdfs:label xml:lang="de">Feuchtwalze</rdfs:label>
        <rdfs:label xml:lang="de">Feuchtwerk</rdfs:label>
        <rdfs:label xml:lang="en">dampening system</rdfs:label>
        <rdfs:label xml:lang="en">dampening unit</rdfs:label>
        <rdfs:label xml:lang="en">damping unit</rdfs:label>
        <rdfs:label xml:lang="en">moistener</rdfs:label>
        <rdfs:label xml:lang="en">print dampener</rdfs:label>
        <part:partOf rdf:resource="http://people.aifb.kit.edu/mu2771/step#printing_press"/>
    </owl:NamedIndividual>
    


    <!-- http://people.aifb.kit.edu/mu2771/step#mounting -->

    <owl:NamedIndividual rdf:about="http://people.aifb.kit.edu/mu2771/step#mounting">
        <rdf:type rdf:resource="http://purl.oclc.org/NET/ssnx/ssn#Process"/>
        <dc:creator rdf:resource="http://www.aifb.kit.edu/web/Sebastian_Bader"/>
        <rdfs:label xml:lang="de">Montage</rdfs:label>
        <rdfs:label xml:lang="en">mounting</rdfs:label>
    </owl:NamedIndividual>
    


    <!-- http://people.aifb.kit.edu/mu2771/step#mounting_device -->

    <owl:NamedIndividual rdf:about="http://people.aifb.kit.edu/mu2771/step#mounting_device">
        <rdf:type rdf:resource="http://people.aifb.kit.edu/mu2771/step#Tool"/>
        <rdf:type rdf:resource="http://purl.oclc.org/NET/ssnx/ssn#Device"/>
        <dc:creator rdf:resource="http://www.heidelberg.com/"/>
        <rdfs:label xml:lang="de">Montagevorrichtung</rdfs:label>
        <rdfs:label xml:lang="en">mounting device</rdfs:label>
    </owl:NamedIndividual>
    


    <!-- http://people.aifb.kit.edu/mu2771/step#no-sheet_detector -->

    <owl:NamedIndividual rdf:about="http://people.aifb.kit.edu/mu2771/step#no-sheet_detector">
        <rdf:type rdf:resource="http://purl.oclc.org/NET/ssnx/ssn#Device"/>
        <rdf:type rdf:resource="http://purl.oclc.org/NET/ssnx/ssn#System"/>
        <step:sourceUri rdf:resource="http://people.aifb.kit.edu/mu2771/step#"/>
        <rdfs:label xml:lang="de">Fehlbogenkontrolle</rdfs:label>
        <rdfs:label xml:lang="en">caliper detector</rdfs:label>
        <rdfs:label xml:lang="en">no-sheet detector</rdfs:label>
        <part:partOf rdf:resource="http://people.aifb.kit.edu/mu2771/step#printing_press"/>
    </owl:NamedIndividual>
    


    <!-- http://people.aifb.kit.edu/mu2771/step#nominal_current -->

    <owl:NamedIndividual rdf:about="http://people.aifb.kit.edu/mu2771/step#nominal_current">
        <rdf:type rdf:resource="http://qudt.org/schema/qudt#ElectricityAndMagnetismQuantityKind"/>
        <dc:creator rdf:resource="http://www.heidelberg.com/"/>
        <rdfs:label xml:lang="de">Nennstrom</rdfs:label>
        <rdfs:label xml:lang="en">nominal current</rdfs:label>
    </owl:NamedIndividual>
    


    <!-- http://people.aifb.kit.edu/mu2771/step#nominal_voltage -->

    <owl:NamedIndividual rdf:about="http://people.aifb.kit.edu/mu2771/step#nominal_voltage">
        <rdf:type rdf:resource="http://qudt.org/schema/qudt#ElectricityAndMagnetismQuantityKind"/>
        <dc:creator rdf:resource="http://www.heidelberg.com/"/>
        <rdfs:label xml:lang="de">Nennspannung</rdfs:label>
        <rdfs:label xml:lang="en">nominal voltage</rdfs:label>
    </owl:NamedIndividual>
    


    <!-- http://people.aifb.kit.edu/mu2771/step#offset_unit -->

    <owl:NamedIndividual rdf:about="http://people.aifb.kit.edu/mu2771/step#offset_unit">
        <rdf:type rdf:resource="http://purl.oclc.org/NET/ssnx/ssn#System"/>
        <dc:creator rdf:resource="http://www.heidelberg.com/"/>
        <rdfs:label xml:lang="de">Offset-Werk</rdfs:label>
        <rdfs:label xml:lang="en">offset unit</rdfs:label>
        <part:partOf rdf:resource="http://people.aifb.kit.edu/mu2771/step#printing_press"/>
    </owl:NamedIndividual>
    


    <!-- http://people.aifb.kit.edu/mu2771/step#oil_collecting_pan -->

    <owl:NamedIndividual rdf:about="http://people.aifb.kit.edu/mu2771/step#oil_collecting_pan">
        <rdf:type rdf:resource="http://purl.oclc.org/NET/ssnx/ssn#Device"/>
        <dc:creator rdf:resource="http://www.heidelberg.com/"/>
        <rdfs:label xml:lang="en">oil collecting pan</rdfs:label>
        <rdfs:label xml:lang="de">Ölauffangwanne</rdfs:label>
        <part:partOf rdf:resource="http://people.aifb.kit.edu/mu2771/step#printing_press"/>
    </owl:NamedIndividual>
    


    <!-- http://people.aifb.kit.edu/mu2771/step#oil_reservoir -->

    <owl:NamedIndividual rdf:about="http://people.aifb.kit.edu/mu2771/step#oil_reservoir">
        <rdf:type rdf:resource="http://purl.oclc.org/NET/ssnx/ssn#Device"/>
        <dc:creator rdf:resource="http://www.heidelberg.com/"/>
        <rdfs:label xml:lang="en">oil reservoir</rdfs:label>
        <rdfs:label xml:lang="de">Ölbehälter</rdfs:label>
        <part:partOf rdf:resource="http://people.aifb.kit.edu/mu2771/step#oil_collecting_pan"/>
    </owl:NamedIndividual>
    


    <!-- http://people.aifb.kit.edu/mu2771/step#on -->

    <owl:NamedIndividual rdf:about="http://people.aifb.kit.edu/mu2771/step#on">
        <rdf:type rdf:resource="http://ontology.tno.nl/saref/#OnState"/>
        <dc:creator rdf:resource="http://www.aifb.kit.edu/web/Sebastian_Bader"/>
        <rdfs:label xml:lang="de">ein</rdfs:label>
        <rdfs:label xml:lang="en">on</rdfs:label>
    </owl:NamedIndividual>
    


    <!-- http://people.aifb.kit.edu/mu2771/step#oscillating_dampening_roller -->

    <owl:NamedIndividual rdf:about="http://people.aifb.kit.edu/mu2771/step#oscillating_dampening_roller">
        <rdf:type rdf:resource="http://purl.oclc.org/NET/ssnx/ssn#Device"/>
        <step:sourceUri rdf:resource="http://people.aifb.kit.edu/mu2771/step#"/>
        <rdfs:label xml:lang="de">Verreiberzylinder</rdfs:label>
        <rdfs:label xml:lang="en">oscillating dampening roller</rdfs:label>
        <part:partOf rdf:resource="http://people.aifb.kit.edu/mu2771/step#inking_station"/>
        <part:partOf rdf:resource="http://people.aifb.kit.edu/mu2771/step#inking_system"/>
        <part:partOf rdf:resource="http://people.aifb.kit.edu/mu2771/step#inking_unit"/>
        <part:partOf rdf:resource="http://people.aifb.kit.edu/mu2771/step#take-up_roller"/>
    </owl:NamedIndividual>
    


    <!-- http://people.aifb.kit.edu/mu2771/step#oscillating_ink_roller -->

    <owl:NamedIndividual rdf:about="http://people.aifb.kit.edu/mu2771/step#oscillating_ink_roller">
        <rdf:type rdf:resource="http://purl.oclc.org/NET/ssnx/ssn#Device"/>
        <owl:sameAs rdf:resource="http://people.aifb.kit.edu/mu2771/step#oscillator"/>
        <step:sourceUri rdf:resource="http://people.aifb.kit.edu/mu2771/step#"/>
        <rdfs:label xml:lang="de">Verreiberzylinder</rdfs:label>
        <rdfs:label xml:lang="en">oscillating ink roller</rdfs:label>
        <part:partOf rdf:resource="http://people.aifb.kit.edu/mu2771/step#inking_station"/>
        <part:partOf rdf:resource="http://people.aifb.kit.edu/mu2771/step#inking_system"/>
        <part:partOf rdf:resource="http://people.aifb.kit.edu/mu2771/step#inking_unit"/>
        <part:partOf rdf:resource="http://people.aifb.kit.edu/mu2771/step#take-up_roller"/>
    </owl:NamedIndividual>
    


    <!-- http://people.aifb.kit.edu/mu2771/step#oscillator -->

    <owl:NamedIndividual rdf:about="http://people.aifb.kit.edu/mu2771/step#oscillator">
        <rdf:type rdf:resource="http://purl.oclc.org/NET/ssnx/ssn#Device"/>
        <step:sourceUri rdf:resource="http://people.aifb.kit.edu/mu2771/step#"/>
        <rdfs:label xml:lang="de">Verreiberzylinder</rdfs:label>
        <rdfs:label xml:lang="en">oscillating ink roller</rdfs:label>
        <rdfs:label xml:lang="en">oscillator</rdfs:label>
        <part:partOf rdf:resource="http://people.aifb.kit.edu/mu2771/step#inking_station"/>
        <part:partOf rdf:resource="http://people.aifb.kit.edu/mu2771/step#inking_system"/>
        <part:partOf rdf:resource="http://people.aifb.kit.edu/mu2771/step#inking_unit"/>
        <part:partOf rdf:resource="http://people.aifb.kit.edu/mu2771/step#take-up_roller"/>
    </owl:NamedIndividual>
    


    <!-- http://people.aifb.kit.edu/mu2771/step#overdampening -->

    <owl:NamedIndividual rdf:about="http://people.aifb.kit.edu/mu2771/step#overdampening">
        <rdf:type rdf:resource="http://people.aifb.kit.edu/mu2771/step#Process"/>
        <dc:creator rdf:resource="http://www.heidelberg.com/"/>
        <rdfs:label xml:lang="en">overdampening</rdfs:label>
        <rdfs:label xml:lang="de">Überfeuchten</rdfs:label>
    </owl:NamedIndividual>
    


    <!-- http://people.aifb.kit.edu/mu2771/step#overinking -->

    <owl:NamedIndividual rdf:about="http://people.aifb.kit.edu/mu2771/step#overinking">
        <rdf:type rdf:resource="http://people.aifb.kit.edu/mu2771/step#Process"/>
        <dc:creator rdf:resource="http://www.heidelberg.com/"/>
        <rdfs:label xml:lang="en">overinking</rdfs:label>
        <rdfs:label xml:lang="de">Überfärben</rdfs:label>
    </owl:NamedIndividual>
    


    <!-- http://people.aifb.kit.edu/mu2771/step#overvoltage_limiter -->

    <owl:NamedIndividual rdf:about="http://people.aifb.kit.edu/mu2771/step#overvoltage_limiter">
        <rdf:type rdf:resource="http://purl.oclc.org/NET/ssnx/ssn#Device"/>
        <dc:creator rdf:resource="http://www.heidelberg.com/"/>
        <rdfs:label xml:lang="en">overvoltage limiter</rdfs:label>
        <rdfs:label xml:lang="de">Überspannungsbegrenzer</rdfs:label>
        <part:partOf rdf:resource="http://people.aifb.kit.edu/mu2771/step#main_connection"/>
    </owl:NamedIndividual>
    


    <!-- http://people.aifb.kit.edu/mu2771/step#package-unit -->

    <owl:NamedIndividual rdf:about="http://people.aifb.kit.edu/mu2771/step#package-unit">
        <rdf:type rdf:resource="http://purl.oclc.org/NET/ssnx/ssn#System"/>
        <dc:creator rdf:resource="http://www.aifb.kit.edu/web/Sebastian_Bader"/>
        <rdfs:label xml:lang="de">PU</rdfs:label>
        <rdfs:label xml:lang="en">package unit</rdfs:label>
        <part:partOf rdf:resource="http://people.aifb.kit.edu/mu2771/step#printing_press"/>
    </owl:NamedIndividual>
    


    <!-- http://people.aifb.kit.edu/mu2771/step#pallet -->

    <owl:NamedIndividual rdf:about="http://people.aifb.kit.edu/mu2771/step#pallet">
        <rdf:type rdf:resource="http://people.aifb.kit.edu/mu2771/step#Product"/>
        <dc:creator rdf:resource="http://www.heidelberg.com/"/>
        <rdfs:label xml:lang="de">Palette</rdfs:label>
        <rdfs:label xml:lang="en">pallet</rdfs:label>
    </owl:NamedIndividual>
    


    <!-- http://people.aifb.kit.edu/mu2771/step#paper -->

    <owl:NamedIndividual rdf:about="http://people.aifb.kit.edu/mu2771/step#paper">
        <rdf:type rdf:resource="http://people.aifb.kit.edu/mu2771/step#Product"/>
        <dc:creator rdf:resource="http://www.heidelberg.com/"/>
        <rdfs:label xml:lang="de">Papier</rdfs:label>
        <rdfs:label xml:lang="en">paper</rdfs:label>
    </owl:NamedIndividual>
    


    <!-- http://people.aifb.kit.edu/mu2771/step#perfecting -->

    <owl:NamedIndividual rdf:about="http://people.aifb.kit.edu/mu2771/step#perfecting">
        <rdf:type rdf:resource="http://people.aifb.kit.edu/mu2771/step#Process"/>
        <dc:creator rdf:resource="http://www.heidelberg.com/"/>
        <rdfs:label xml:lang="de">Schoendruck</rdfs:label>
        <rdfs:label xml:lang="de">Schön-/Widerdruck</rdfs:label>
        <rdfs:label xml:lang="de">Schöndruck</rdfs:label>
        <rdfs:label xml:lang="de">Widerdruck</rdfs:label>
        <rdfs:label xml:lang="en">perfecting</rdfs:label>
    </owl:NamedIndividual>
    


    <!-- http://people.aifb.kit.edu/mu2771/step#perforating -->

    <owl:NamedIndividual rdf:about="http://people.aifb.kit.edu/mu2771/step#perforating">
        <rdf:type rdf:resource="http://people.aifb.kit.edu/mu2771/step#Process"/>
        <dc:creator rdf:resource="http://www.heidelberg.com/"/>
        <rdfs:label xml:lang="de">Perforieren</rdfs:label>
        <rdfs:label xml:lang="en">perforating</rdfs:label>
    </owl:NamedIndividual>
    


    <!-- http://people.aifb.kit.edu/mu2771/step#plate-detection -->

    <owl:NamedIndividual rdf:about="http://people.aifb.kit.edu/mu2771/step#plate-detection">
        <rdf:type rdf:resource="http://purl.oclc.org/NET/ssnx/ssn#SensingDevice"/>
        <dc:creator rdf:resource="http://www.aifb.kit.edu/web/Sebastian_Bader"/>
        <rdfs:label xml:lang="de">Plattenerkennung</rdfs:label>
        <rdfs:label xml:lang="en">plate detection</rdfs:label>
        <part:partOf rdf:resource="http://people.aifb.kit.edu/mu2771/step#control_console"/>
    </owl:NamedIndividual>
    


    <!-- http://people.aifb.kit.edu/mu2771/step#pneumatic_pressure -->

    <owl:NamedIndividual rdf:about="http://people.aifb.kit.edu/mu2771/step#pneumatic_pressure">
        <rdf:type rdf:resource="http://qudt.org/schema/qudt#Dimension"/>
        <dc:creator rdf:resource="http://www.heidelberg.com/"/>
        <rdfs:label xml:lang="de">Pneumatikdruck</rdfs:label>
        <rdfs:label xml:lang="en">pneumatic pressure</rdfs:label>
    </owl:NamedIndividual>
    


    <!-- http://people.aifb.kit.edu/mu2771/step#powder_spray -->

    <owl:NamedIndividual rdf:about="http://people.aifb.kit.edu/mu2771/step#powder_spray">
        <rdf:type rdf:resource="http://purl.oclc.org/NET/ssnx/ssn#Device"/>
        <owl:sameAs rdf:resource="http://people.aifb.kit.edu/mu2771/step#powder_spray_device"/>
        <owl:sameAs rdf:resource="http://people.aifb.kit.edu/mu2771/step#powder_spray_system"/>
        <owl:sameAs rdf:resource="http://people.aifb.kit.edu/mu2771/step#powder_spray_unit"/>
        <step:sourceUri rdf:resource="http://people.aifb.kit.edu/mu2771/step#"/>
        <rdfs:label xml:lang="de">Puderdruckbestäuber</rdfs:label>
        <rdfs:label xml:lang="en">powder spray</rdfs:label>
        <part:partOf rdf:resource="http://people.aifb.kit.edu/mu2771/step#inking_station"/>
        <part:partOf rdf:resource="http://people.aifb.kit.edu/mu2771/step#inking_system"/>
        <part:partOf rdf:resource="http://people.aifb.kit.edu/mu2771/step#inking_unit"/>
        <part:partOf rdf:resource="http://people.aifb.kit.edu/mu2771/step#take-up_roller"/>
    </owl:NamedIndividual>
    


    <!-- http://people.aifb.kit.edu/mu2771/step#powder_spray_device -->

    <owl:NamedIndividual rdf:about="http://people.aifb.kit.edu/mu2771/step#powder_spray_device">
        <rdf:type rdf:resource="http://purl.oclc.org/NET/ssnx/ssn#Device"/>
        <owl:sameAs rdf:resource="http://people.aifb.kit.edu/mu2771/step#powder_spray_system"/>
        <owl:sameAs rdf:resource="http://people.aifb.kit.edu/mu2771/step#powder_spray_unit"/>
        <step:sourceUri rdf:resource="http://people.aifb.kit.edu/mu2771/step#"/>
        <rdfs:label xml:lang="de">Puderapparat</rdfs:label>
        <rdfs:label xml:lang="de">Puderdruckbestäuber</rdfs:label>
        <rdfs:label xml:lang="en">powder spray</rdfs:label>
        <rdfs:label xml:lang="en">powder spray (device)</rdfs:label>
        <rdfs:label xml:lang="en">powder spray device</rdfs:label>
        <rdfs:label xml:lang="en">powder spray system</rdfs:label>
        <rdfs:label xml:lang="en">powder spray unit</rdfs:label>
        <part:partOf rdf:resource="http://people.aifb.kit.edu/mu2771/step#inking_station"/>
        <part:partOf rdf:resource="http://people.aifb.kit.edu/mu2771/step#inking_system"/>
        <part:partOf rdf:resource="http://people.aifb.kit.edu/mu2771/step#inking_unit"/>
        <part:partOf rdf:resource="http://people.aifb.kit.edu/mu2771/step#take-up_roller"/>
    </owl:NamedIndividual>
    


    <!-- http://people.aifb.kit.edu/mu2771/step#powder_spray_system -->

    <owl:NamedIndividual rdf:about="http://people.aifb.kit.edu/mu2771/step#powder_spray_system">
        <rdf:type rdf:resource="http://purl.oclc.org/NET/ssnx/ssn#Device"/>
        <owl:sameAs rdf:resource="http://people.aifb.kit.edu/mu2771/step#powder_spray_unit"/>
        <step:sourceUri rdf:resource="http://people.aifb.kit.edu/mu2771/step#"/>
        <rdfs:label xml:lang="de">Puderapparat</rdfs:label>
        <rdfs:label xml:lang="de">Puderdruckbestäuber</rdfs:label>
        <rdfs:label xml:lang="en">powder spray</rdfs:label>
        <rdfs:label xml:lang="en">powder spray (device)</rdfs:label>
        <rdfs:label xml:lang="en">powder spray device</rdfs:label>
        <rdfs:label xml:lang="en">powder spray system</rdfs:label>
        <rdfs:label xml:lang="en">powder spray unit</rdfs:label>
        <part:partOf rdf:resource="http://people.aifb.kit.edu/mu2771/step#inking_station"/>
        <part:partOf rdf:resource="http://people.aifb.kit.edu/mu2771/step#inking_system"/>
        <part:partOf rdf:resource="http://people.aifb.kit.edu/mu2771/step#inking_unit"/>
        <part:partOf rdf:resource="http://people.aifb.kit.edu/mu2771/step#take-up_roller"/>
    </owl:NamedIndividual>
    


    <!-- http://people.aifb.kit.edu/mu2771/step#powder_spray_unit -->

    <owl:NamedIndividual rdf:about="http://people.aifb.kit.edu/mu2771/step#powder_spray_unit">
        <rdf:type rdf:resource="http://purl.oclc.org/NET/ssnx/ssn#Device"/>
        <step:sourceUri rdf:resource="http://people.aifb.kit.edu/mu2771/step#"/>
        <rdfs:label xml:lang="de">Puderapparat</rdfs:label>
        <rdfs:label xml:lang="de">Puderdruckbestäuber</rdfs:label>
        <rdfs:label xml:lang="en">powder spray</rdfs:label>
        <rdfs:label xml:lang="en">powder spray (device)</rdfs:label>
        <rdfs:label xml:lang="en">powder spray device</rdfs:label>
        <rdfs:label xml:lang="en">powder spray system</rdfs:label>
        <rdfs:label xml:lang="en">powder spray unit</rdfs:label>
        <part:partOf rdf:resource="http://people.aifb.kit.edu/mu2771/step#inking_station"/>
        <part:partOf rdf:resource="http://people.aifb.kit.edu/mu2771/step#inking_system"/>
        <part:partOf rdf:resource="http://people.aifb.kit.edu/mu2771/step#inking_unit"/>
        <part:partOf rdf:resource="http://people.aifb.kit.edu/mu2771/step#take-up_roller"/>
    </owl:NamedIndividual>
    


    <!-- http://people.aifb.kit.edu/mu2771/step#pre-gripper -->

    <owl:NamedIndividual rdf:about="http://people.aifb.kit.edu/mu2771/step#pre-gripper">
        <rdf:type rdf:resource="http://purl.oclc.org/NET/ssnx/ssn#Device"/>
        <step:sourceUri rdf:resource="http://people.aifb.kit.edu/mu2771/step#"/>
        <rdfs:label xml:lang="de">Vorgreifer</rdfs:label>
        <rdfs:label xml:lang="en">pre-gripper</rdfs:label>
        <part:partOf rdf:resource="http://people.aifb.kit.edu/mu2771/step#printing_press"/>
    </owl:NamedIndividual>
    


    <!-- http://people.aifb.kit.edu/mu2771/step#preinking -->

    <owl:NamedIndividual rdf:about="http://people.aifb.kit.edu/mu2771/step#preinking">
        <rdf:type rdf:resource="http://purl.oclc.org/NET/ssnx/ssn#System"/>
        <dc:creator rdf:resource="http://www.heidelberg.com/"/>
        <rdfs:label xml:lang="de">Farbeinlauf</rdfs:label>
        <rdfs:label xml:lang="en">preinking</rdfs:label>
        <part:partOf rdf:resource="http://people.aifb.kit.edu/mu2771/step#ink_ductor"/>
        <part:partOf rdf:resource="http://people.aifb.kit.edu/mu2771/step#ink_fountain_roller"/>
    </owl:NamedIndividual>
    


    <!-- http://people.aifb.kit.edu/mu2771/step#preloading_device -->

    <owl:NamedIndividual rdf:about="http://people.aifb.kit.edu/mu2771/step#preloading_device">
        <rdf:type rdf:resource="http://purl.oclc.org/NET/ssnx/ssn#Device"/>
        <dc:creator rdf:resource="http://www.heidelberg.com/"/>
        <rdfs:label xml:lang="de">Vorstapeleinrichtung</rdfs:label>
        <rdfs:label xml:lang="en">preloading device</rdfs:label>
        <part:partOf rdf:resource="http://people.aifb.kit.edu/mu2771/step#main_pile"/>
    </owl:NamedIndividual>
    


    <!-- http://people.aifb.kit.edu/mu2771/step#press_configuration -->

    <owl:Thing rdf:about="http://people.aifb.kit.edu/mu2771/step#press_configuration">
        <rdf:type rdf:resource="http://www.w3.org/2002/07/owl#NamedIndividual"/>
        <dc:creator rdf:resource="http://www.heidelberg.com/"/>
        <rdfs:label xml:lang="de">Maschinenkonfiguration</rdfs:label>
        <rdfs:label xml:lang="en">press configuration</rdfs:label>
    </owl:Thing>
    


    <!-- http://people.aifb.kit.edu/mu2771/step#press_sheet_size -->

    <owl:Thing rdf:about="http://people.aifb.kit.edu/mu2771/step#press_sheet_size">
        <rdf:type rdf:resource="http://www.w3.org/2002/07/owl#NamedIndividual"/>
        <dc:creator rdf:resource="http://www.heidelberg.com/"/>
        <rdfs:label xml:lang="de">Maschinenformat</rdfs:label>
        <rdfs:label xml:lang="en">press sheet size</rdfs:label>
    </owl:Thing>
    


    <!-- http://people.aifb.kit.edu/mu2771/step#press_speed -->

    <owl:Thing rdf:about="http://people.aifb.kit.edu/mu2771/step#press_speed">
        <rdf:type rdf:resource="http://www.w3.org/2002/07/owl#NamedIndividual"/>
        <dc:creator rdf:resource="http://www.heidelberg.com/"/>
        <rdfs:label xml:lang="de">Maschinengeschwindigkeit</rdfs:label>
        <rdfs:label xml:lang="en">press speed</rdfs:label>
    </owl:Thing>
    


    <!-- http://people.aifb.kit.edu/mu2771/step#pressure_tank -->

    <owl:NamedIndividual rdf:about="http://people.aifb.kit.edu/mu2771/step#pressure_tank">
        <rdf:type rdf:resource="http://purl.oclc.org/NET/ssnx/ssn#Device"/>
        <dc:creator rdf:resource="http://www.heidelberg.com/"/>
        <rdfs:label xml:lang="de">Druckbehälter</rdfs:label>
        <rdfs:label xml:lang="en">pressure tank</rdfs:label>
        <part:partOf rdf:resource="http://people.aifb.kit.edu/mu2771/step#powder_spray_device"/>
        <part:partOf rdf:resource="http://people.aifb.kit.edu/mu2771/step#powder_spray_system"/>
        <part:partOf rdf:resource="http://people.aifb.kit.edu/mu2771/step#powder_spray_unit"/>
    </owl:NamedIndividual>
    


    <!-- http://people.aifb.kit.edu/mu2771/step#print_bearer-to-bearer_printing_press -->

    <owl:NamedIndividual rdf:about="http://people.aifb.kit.edu/mu2771/step#print_bearer-to-bearer_printing_press">
        <rdf:type rdf:resource="http://purl.oclc.org/NET/ssnx/ssn#Device"/>
        <step:sourceUri rdf:resource="http://people.aifb.kit.edu/mu2771/step#"/>
        <rdfs:label xml:lang="de">Schmitzringläufer</rdfs:label>
        <rdfs:label xml:lang="en">print bearer-to-bearer printing press</rdfs:label>
        <part:partOf rdf:resource="http://people.aifb.kit.edu/mu2771/step#printing_press"/>
    </owl:NamedIndividual>
    


    <!-- http://people.aifb.kit.edu/mu2771/step#print_color_desk -->

    <owl:NamedIndividual rdf:about="http://people.aifb.kit.edu/mu2771/step#print_color_desk">
        <rdf:type rdf:resource="http://purl.oclc.org/NET/ssnx/ssn#Device"/>
        <rdf:type rdf:resource="http://purl.oclc.org/NET/ssnx/ssn#System"/>
        <step:sourceUri rdf:resource="http://people.aifb.kit.edu/mu2771/step#"/>
        <dc:creator rdf:resource="http://www.heidelberg.com/"/>
        <rdfs:label xml:lang="de">Colorpult</rdfs:label>
        <rdfs:label xml:lang="de">Colorsteuerpult</rdfs:label>
        <rdfs:label xml:lang="de">Farbpult</rdfs:label>
        <rdfs:label xml:lang="de">Farbsteuerpult</rdfs:label>
        <rdfs:label xml:lang="de">Grammatur</rdfs:label>
        <rdfs:label xml:lang="en">colour console</rdfs:label>
        <rdfs:label xml:lang="en">grammage</rdfs:label>
        <rdfs:label xml:lang="en">print color desk</rdfs:label>
        <part:partOf rdf:resource="http://people.aifb.kit.edu/mu2771/step#printing_press"/>
    </owl:NamedIndividual>
    


    <!-- http://people.aifb.kit.edu/mu2771/step#print_counter-pressure_cylinder_ -->

    <owl:NamedIndividual rdf:about="http://people.aifb.kit.edu/mu2771/step#print_counter-pressure_cylinder_">
        <rdf:type rdf:resource="http://purl.oclc.org/NET/ssnx/ssn#Device"/>
        <rdf:type rdf:resource="http://purl.oclc.org/NET/ssnx/ssn#System"/>
        <owl:sameAs rdf:resource="http://people.aifb.kit.edu/mu2771/step#print_counterpressure_cylinder_"/>
        <owl:sameAs rdf:resource="http://people.aifb.kit.edu/mu2771/step#printing_cylinder"/>
        <step:sourceUri rdf:resource="http://people.aifb.kit.edu/mu2771/step#"/>
        <rdfs:label xml:lang="de">Druckzylinder</rdfs:label>
        <rdfs:label xml:lang="de">Gegendruckzylinder</rdfs:label>
        <rdfs:label xml:lang="en">impression cylinder</rdfs:label>
        <rdfs:label xml:lang="en">print counter-pressure cylinder </rdfs:label>
        <rdfs:label xml:lang="en">print counterpressure cylinder </rdfs:label>
        <rdfs:label xml:lang="en">printing cylinder</rdfs:label>
        <part:partOf rdf:resource="http://people.aifb.kit.edu/mu2771/step#ink_train"/>
        <part:partOf rdf:resource="http://people.aifb.kit.edu/mu2771/step#inking_station"/>
        <part:partOf rdf:resource="http://people.aifb.kit.edu/mu2771/step#inking_system"/>
        <part:partOf rdf:resource="http://people.aifb.kit.edu/mu2771/step#inking_unit"/>
        <part:partOf rdf:resource="http://people.aifb.kit.edu/mu2771/step#printing_press"/>
        <part:partOf rdf:resource="http://people.aifb.kit.edu/mu2771/step#take-up_roller"/>
    </owl:NamedIndividual>
    


    <!-- http://people.aifb.kit.edu/mu2771/step#print_counterpressure_cylinder_ -->

    <owl:NamedIndividual rdf:about="http://people.aifb.kit.edu/mu2771/step#print_counterpressure_cylinder_">
        <rdf:type rdf:resource="http://purl.oclc.org/NET/ssnx/ssn#Device"/>
        <rdf:type rdf:resource="http://purl.oclc.org/NET/ssnx/ssn#System"/>
        <owl:sameAs rdf:resource="http://people.aifb.kit.edu/mu2771/step#printing_cylinder"/>
        <step:sourceUri rdf:resource="http://people.aifb.kit.edu/mu2771/step#"/>
        <rdfs:label xml:lang="de">Druckzylinder</rdfs:label>
        <rdfs:label xml:lang="de">Gegendruckzylinder</rdfs:label>
        <rdfs:label xml:lang="en">impression cylinder</rdfs:label>
        <rdfs:label xml:lang="en">print counter-pressure cylinder </rdfs:label>
        <rdfs:label xml:lang="en">print counterpressure cylinder </rdfs:label>
        <rdfs:label xml:lang="en">printing cylinder</rdfs:label>
        <part:partOf rdf:resource="http://people.aifb.kit.edu/mu2771/step#ink_train"/>
        <part:partOf rdf:resource="http://people.aifb.kit.edu/mu2771/step#inking_station"/>
        <part:partOf rdf:resource="http://people.aifb.kit.edu/mu2771/step#inking_system"/>
        <part:partOf rdf:resource="http://people.aifb.kit.edu/mu2771/step#inking_unit"/>
        <part:partOf rdf:resource="http://people.aifb.kit.edu/mu2771/step#printing_press"/>
        <part:partOf rdf:resource="http://people.aifb.kit.edu/mu2771/step#take-up_roller"/>
    </owl:NamedIndividual>
    


    <!-- http://people.aifb.kit.edu/mu2771/step#print_dampener -->

    <owl:NamedIndividual rdf:about="http://people.aifb.kit.edu/mu2771/step#print_dampener">
        <rdf:type rdf:resource="http://purl.oclc.org/NET/ssnx/ssn#Device"/>
        <rdf:type rdf:resource="http://purl.oclc.org/NET/ssnx/ssn#System"/>
        <step:sourceUri rdf:resource="http://people.aifb.kit.edu/mu2771/step#"/>
        <rdfs:label xml:lang="de">Feuchtauftragwalze</rdfs:label>
        <rdfs:label xml:lang="de">Feuchtwalze</rdfs:label>
        <rdfs:label xml:lang="de">Feuchtwerk</rdfs:label>
        <rdfs:label xml:lang="en">dampening system</rdfs:label>
        <rdfs:label xml:lang="en">dampening unit</rdfs:label>
        <rdfs:label xml:lang="en">damping unit</rdfs:label>
        <rdfs:label xml:lang="en">moistener</rdfs:label>
        <rdfs:label xml:lang="en">print dampener</rdfs:label>
        <part:partOf rdf:resource="http://people.aifb.kit.edu/mu2771/step#printing_press"/>
    </owl:NamedIndividual>
    


    <!-- http://people.aifb.kit.edu/mu2771/step#print_feed_guide -->

    <owl:NamedIndividual rdf:about="http://people.aifb.kit.edu/mu2771/step#print_feed_guide">
        <rdf:type rdf:resource="http://purl.oclc.org/NET/ssnx/ssn#System"/>
        <step:sourceUri rdf:resource="http://people.aifb.kit.edu/mu2771/step#"/>
        <rdfs:label xml:lang="de">Anlage</rdfs:label>
        <rdfs:label xml:lang="en">print feed guide</rdfs:label>
        <part:partOf rdf:resource="http://people.aifb.kit.edu/mu2771/step#printing_press"/>
    </owl:NamedIndividual>
    


    <!-- http://people.aifb.kit.edu/mu2771/step#print_impression_cylinder -->

    <owl:NamedIndividual rdf:about="http://people.aifb.kit.edu/mu2771/step#print_impression_cylinder">
        <rdf:type rdf:resource="http://purl.oclc.org/NET/ssnx/ssn#Device"/>
        <step:sourceUri rdf:resource="http://people.aifb.kit.edu/mu2771/step#"/>
        <rdfs:label xml:lang="de">Druckzylinder</rdfs:label>
        <rdfs:label xml:lang="en">print impression cylinder</rdfs:label>
        <part:partOf rdf:resource="http://people.aifb.kit.edu/mu2771/step#print_feed_guide"/>
    </owl:NamedIndividual>
    


    <!-- http://people.aifb.kit.edu/mu2771/step#print_ink_blade -->

    <owl:NamedIndividual rdf:about="http://people.aifb.kit.edu/mu2771/step#print_ink_blade">
        <rdf:type rdf:resource="http://purl.oclc.org/NET/ssnx/ssn#Device"/>
        <step:sourceUri rdf:resource="http://people.aifb.kit.edu/mu2771/step#"/>
        <rdfs:label xml:lang="de">Farbmesser</rdfs:label>
        <rdfs:label xml:lang="en">doctor knife</rdfs:label>
        <rdfs:label xml:lang="en">fountain blade</rdfs:label>
        <rdfs:label xml:lang="en">print ink blade</rdfs:label>
        <part:partOf rdf:resource="http://people.aifb.kit.edu/mu2771/step#printing_press"/>
    </owl:NamedIndividual>
    


    <!-- http://people.aifb.kit.edu/mu2771/step#print_ink_delivery_system -->

    <owl:NamedIndividual rdf:about="http://people.aifb.kit.edu/mu2771/step#print_ink_delivery_system">
        <rdf:type rdf:resource="http://purl.oclc.org/NET/ssnx/ssn#System"/>
        <owl:sameAs rdf:resource="http://people.aifb.kit.edu/mu2771/step#print_ink_feed"/>
        <owl:sameAs rdf:resource="http://people.aifb.kit.edu/mu2771/step#print_ink_feeding"/>
        <step:sourceUri rdf:resource="http://people.aifb.kit.edu/mu2771/step#"/>
        <rdfs:label xml:lang="de">Farbzuführung</rdfs:label>
        <rdfs:label xml:lang="en">print ink delivery system</rdfs:label>
        <part:partOf rdf:resource="http://people.aifb.kit.edu/mu2771/step#printing_press"/>
    </owl:NamedIndividual>
    


    <!-- http://people.aifb.kit.edu/mu2771/step#print_ink_duct -->

    <owl:NamedIndividual rdf:about="http://people.aifb.kit.edu/mu2771/step#print_ink_duct">
        <rdf:type rdf:resource="http://purl.oclc.org/NET/ssnx/ssn#Device"/>
        <owl:sameAs rdf:resource="http://people.aifb.kit.edu/mu2771/step#print_ink_fountain"/>
        <owl:sameAs rdf:resource="http://people.aifb.kit.edu/mu2771/step#print_ink_supply"/>
        <owl:sameAs rdf:resource="http://people.aifb.kit.edu/mu2771/step#print_ink_well"/>
        <step:sourceUri rdf:resource="http://people.aifb.kit.edu/mu2771/step#"/>
        <rdfs:label xml:lang="de">Farbkasten</rdfs:label>
        <rdfs:label xml:lang="en">print (ink) duct</rdfs:label>
        <rdfs:label xml:lang="en">print duct</rdfs:label>
        <rdfs:label xml:lang="en">print ink duct</rdfs:label>
    </owl:NamedIndividual>
    


    <!-- http://people.aifb.kit.edu/mu2771/step#print_ink_ductor -->

    <owl:NamedIndividual rdf:about="http://people.aifb.kit.edu/mu2771/step#print_ink_ductor">
        <rdf:type rdf:resource="http://purl.oclc.org/NET/ssnx/ssn#Device"/>
        <step:sourceUri rdf:resource="http://people.aifb.kit.edu/mu2771/step#"/>
        <rdfs:label xml:lang="en">(ink) duct roller</rdfs:label>
        <rdfs:label xml:lang="de">Farbduktor</rdfs:label>
        <rdfs:label xml:lang="de">Farbduktorwalze</rdfs:label>
        <rdfs:label xml:lang="de">Farbduktorzylinder</rdfs:label>
        <rdfs:label xml:lang="de">Farbkastenwalze</rdfs:label>
        <rdfs:label xml:lang="en">duct roller</rdfs:label>
        <rdfs:label xml:lang="en">ductor</rdfs:label>
        <rdfs:label xml:lang="en">ink duct roller</rdfs:label>
        <rdfs:label xml:lang="en">print ink ductor</rdfs:label>
        <part:partOf rdf:resource="http://people.aifb.kit.edu/mu2771/step#printing_press"/>
    </owl:NamedIndividual>
    


    <!-- http://people.aifb.kit.edu/mu2771/step#print_ink_feed -->

    <owl:NamedIndividual rdf:about="http://people.aifb.kit.edu/mu2771/step#print_ink_feed">
        <rdf:type rdf:resource="http://purl.oclc.org/NET/ssnx/ssn#System"/>
        <owl:sameAs rdf:resource="http://people.aifb.kit.edu/mu2771/step#print_ink_feeding"/>
        <step:sourceUri rdf:resource="http://people.aifb.kit.edu/mu2771/step#"/>
        <rdfs:label xml:lang="de">Farbzuführung</rdfs:label>
        <rdfs:label xml:lang="en">print ink delivery system</rdfs:label>
        <rdfs:label xml:lang="en">print ink feed</rdfs:label>
        <rdfs:label xml:lang="en">print ink feeding</rdfs:label>
        <part:partOf rdf:resource="http://people.aifb.kit.edu/mu2771/step#printing_press"/>
    </owl:NamedIndividual>
    


    <!-- http://people.aifb.kit.edu/mu2771/step#print_ink_feeding -->

    <owl:NamedIndividual rdf:about="http://people.aifb.kit.edu/mu2771/step#print_ink_feeding">
        <rdf:type rdf:resource="http://purl.oclc.org/NET/ssnx/ssn#System"/>
        <step:sourceUri rdf:resource="http://people.aifb.kit.edu/mu2771/step#"/>
        <rdfs:label xml:lang="de">Farbzuführung</rdfs:label>
        <rdfs:label xml:lang="en">print ink delivery system</rdfs:label>
        <rdfs:label xml:lang="en">print ink feed</rdfs:label>
        <rdfs:label xml:lang="en">print ink feeding</rdfs:label>
        <part:partOf rdf:resource="http://people.aifb.kit.edu/mu2771/step#printing_press"/>
    </owl:NamedIndividual>
    


    <!-- http://people.aifb.kit.edu/mu2771/step#print_ink_form_roller -->

    <owl:NamedIndividual rdf:about="http://people.aifb.kit.edu/mu2771/step#print_ink_form_roller">
        <rdf:type rdf:resource="http://purl.oclc.org/NET/ssnx/ssn#Device"/>
        <step:sourceUri rdf:resource="http://people.aifb.kit.edu/mu2771/step#"/>
        <rdfs:label xml:lang="de">Farbauftragwalze</rdfs:label>
        <rdfs:label xml:lang="en">print ink form roller</rdfs:label>
        <part:partOf rdf:resource="http://people.aifb.kit.edu/mu2771/step#print_ink_delivery_system"/>
        <part:partOf rdf:resource="http://people.aifb.kit.edu/mu2771/step#print_ink_feed"/>
        <part:partOf rdf:resource="http://people.aifb.kit.edu/mu2771/step#print_ink_feeding"/>
    </owl:NamedIndividual>
    


    <!-- http://people.aifb.kit.edu/mu2771/step#print_ink_fountain -->

    <owl:NamedIndividual rdf:about="http://people.aifb.kit.edu/mu2771/step#print_ink_fountain">
        <rdf:type rdf:resource="http://purl.oclc.org/NET/ssnx/ssn#Device"/>
        <owl:sameAs rdf:resource="http://people.aifb.kit.edu/mu2771/step#print_ink_supply"/>
        <owl:sameAs rdf:resource="http://people.aifb.kit.edu/mu2771/step#print_ink_well"/>
        <step:sourceUri rdf:resource="http://people.aifb.kit.edu/mu2771/step#"/>
        <rdfs:label xml:lang="de">Farbkasten</rdfs:label>
        <rdfs:label xml:lang="en">print (ink) duct</rdfs:label>
        <rdfs:label xml:lang="en">print duct</rdfs:label>
        <rdfs:label xml:lang="en">print ink duct</rdfs:label>
        <rdfs:label xml:lang="en">print ink fountain</rdfs:label>
        <rdfs:label xml:lang="en">print ink supply</rdfs:label>
        <rdfs:label xml:lang="en">print ink well</rdfs:label>
        <part:partOf rdf:resource="http://people.aifb.kit.edu/mu2771/step#ink_train"/>
        <part:partOf rdf:resource="http://people.aifb.kit.edu/mu2771/step#inking_station"/>
        <part:partOf rdf:resource="http://people.aifb.kit.edu/mu2771/step#inking_system"/>
        <part:partOf rdf:resource="http://people.aifb.kit.edu/mu2771/step#inking_unit"/>
        <part:partOf rdf:resource="http://people.aifb.kit.edu/mu2771/step#take-up_roller"/>
    </owl:NamedIndividual>
    


    <!-- http://people.aifb.kit.edu/mu2771/step#print_ink_supply -->

    <owl:NamedIndividual rdf:about="http://people.aifb.kit.edu/mu2771/step#print_ink_supply">
        <rdf:type rdf:resource="http://purl.oclc.org/NET/ssnx/ssn#Device"/>
        <owl:sameAs rdf:resource="http://people.aifb.kit.edu/mu2771/step#print_ink_well"/>
        <step:sourceUri rdf:resource="http://people.aifb.kit.edu/mu2771/step#"/>
        <rdfs:label xml:lang="de">Farbkasten</rdfs:label>
        <rdfs:label xml:lang="en">print (ink) duct</rdfs:label>
        <rdfs:label xml:lang="en">print duct</rdfs:label>
        <rdfs:label xml:lang="en">print ink duct</rdfs:label>
        <rdfs:label xml:lang="en">print ink fountain</rdfs:label>
        <rdfs:label xml:lang="en">print ink supply</rdfs:label>
        <rdfs:label xml:lang="en">print ink well</rdfs:label>
        <part:partOf rdf:resource="http://people.aifb.kit.edu/mu2771/step#ink_train"/>
        <part:partOf rdf:resource="http://people.aifb.kit.edu/mu2771/step#inking_station"/>
        <part:partOf rdf:resource="http://people.aifb.kit.edu/mu2771/step#inking_system"/>
        <part:partOf rdf:resource="http://people.aifb.kit.edu/mu2771/step#inking_unit"/>
        <part:partOf rdf:resource="http://people.aifb.kit.edu/mu2771/step#take-up_roller"/>
    </owl:NamedIndividual>
    


    <!-- http://people.aifb.kit.edu/mu2771/step#print_ink_transfer_roller -->

    <owl:NamedIndividual rdf:about="http://people.aifb.kit.edu/mu2771/step#print_ink_transfer_roller">
        <rdf:type rdf:resource="http://purl.oclc.org/NET/ssnx/ssn#Device"/>
        <owl:sameAs rdf:resource="http://people.aifb.kit.edu/mu2771/step#print_inking_roller"/>
        <step:sourceUri rdf:resource="http://people.aifb.kit.edu/mu2771/step#"/>
        <rdfs:label xml:lang="de">Farbübertragungswalze</rdfs:label>
        <rdfs:label xml:lang="de">Farbübertragwalze</rdfs:label>
        <rdfs:label xml:lang="en">print ink transfer roller</rdfs:label>
        <part:partOf rdf:resource="http://people.aifb.kit.edu/mu2771/step#print_ink_fountain"/>
        <part:partOf rdf:resource="http://people.aifb.kit.edu/mu2771/step#print_ink_supply"/>
        <part:partOf rdf:resource="http://people.aifb.kit.edu/mu2771/step#print_ink_well"/>
    </owl:NamedIndividual>
    


    <!-- http://people.aifb.kit.edu/mu2771/step#print_ink_well -->

    <owl:NamedIndividual rdf:about="http://people.aifb.kit.edu/mu2771/step#print_ink_well">
        <rdf:type rdf:resource="http://purl.oclc.org/NET/ssnx/ssn#Device"/>
        <step:sourceUri rdf:resource="http://people.aifb.kit.edu/mu2771/step#"/>
        <rdfs:label xml:lang="de">Farbkasten</rdfs:label>
        <rdfs:label xml:lang="en">print (ink) duct</rdfs:label>
        <rdfs:label xml:lang="en">print duct</rdfs:label>
        <rdfs:label xml:lang="en">print ink duct</rdfs:label>
        <rdfs:label xml:lang="en">print ink fountain</rdfs:label>
        <rdfs:label xml:lang="en">print ink supply</rdfs:label>
        <rdfs:label xml:lang="en">print ink well</rdfs:label>
        <part:partOf rdf:resource="http://people.aifb.kit.edu/mu2771/step#ink_train"/>
        <part:partOf rdf:resource="http://people.aifb.kit.edu/mu2771/step#inking_station"/>
        <part:partOf rdf:resource="http://people.aifb.kit.edu/mu2771/step#inking_system"/>
        <part:partOf rdf:resource="http://people.aifb.kit.edu/mu2771/step#inking_unit"/>
        <part:partOf rdf:resource="http://people.aifb.kit.edu/mu2771/step#take-up_roller"/>
    </owl:NamedIndividual>
    


    <!-- http://people.aifb.kit.edu/mu2771/step#print_inking_roller -->

    <owl:NamedIndividual rdf:about="http://people.aifb.kit.edu/mu2771/step#print_inking_roller">
        <rdf:type rdf:resource="http://purl.oclc.org/NET/ssnx/ssn#Device"/>
        <step:sourceUri rdf:resource="http://people.aifb.kit.edu/mu2771/step#"/>
        <rdfs:label xml:lang="de">Farbauftragwalze</rdfs:label>
        <rdfs:label xml:lang="de">Farbübertragungswalze</rdfs:label>
        <rdfs:label xml:lang="de">Farbübertragwalze</rdfs:label>
        <rdfs:label xml:lang="en">print ink transfer roller</rdfs:label>
        <rdfs:label xml:lang="en">print inking roller</rdfs:label>
        <part:partOf rdf:resource="http://people.aifb.kit.edu/mu2771/step#print_ink_fountain"/>
        <part:partOf rdf:resource="http://people.aifb.kit.edu/mu2771/step#print_ink_supply"/>
        <part:partOf rdf:resource="http://people.aifb.kit.edu/mu2771/step#print_ink_well"/>
        <part:partOf rdf:resource="http://people.aifb.kit.edu/mu2771/step#printing_press"/>
    </owl:NamedIndividual>
    


    <!-- http://people.aifb.kit.edu/mu2771/step#print_job -->

    <owl:NamedIndividual rdf:about="http://people.aifb.kit.edu/mu2771/step#print_job">
        <rdf:type rdf:resource="http://people.aifb.kit.edu/mu2771/step#Process"/>
        <dc:creator rdf:resource="http://www.heidelberg.com/"/>
        <rdfs:label xml:lang="de">Druckauftrag</rdfs:label>
        <rdfs:label xml:lang="en">print job</rdfs:label>
    </owl:NamedIndividual>
    


    <!-- http://people.aifb.kit.edu/mu2771/step#print_press_bed -->

    <owl:NamedIndividual rdf:about="http://people.aifb.kit.edu/mu2771/step#print_press_bed">
        <rdf:type rdf:resource="http://purl.oclc.org/NET/ssnx/ssn#Device"/>
        <step:sourceUri rdf:resource="http://people.aifb.kit.edu/mu2771/step#"/>
        <rdfs:label xml:lang="de">Drucktisch</rdfs:label>
        <rdfs:label xml:lang="en">print press bed</rdfs:label>
        <part:partOf rdf:resource="http://people.aifb.kit.edu/mu2771/step#printing_press"/>
    </owl:NamedIndividual>
    


    <!-- http://people.aifb.kit.edu/mu2771/step#print_sheet -->

    <owl:NamedIndividual rdf:about="http://people.aifb.kit.edu/mu2771/step#print_sheet">
        <rdf:type rdf:resource="http://people.aifb.kit.edu/mu2771/step#Product"/>
        <dc:creator rdf:resource="http://www.heidelberg.com/"/>
        <rdfs:label xml:lang="de">Druckbogen</rdfs:label>
        <rdfs:label xml:lang="en">print sheet</rdfs:label>
    </owl:NamedIndividual>
    


    <!-- http://people.aifb.kit.edu/mu2771/step#print_start -->

    <owl:NamedIndividual rdf:about="http://people.aifb.kit.edu/mu2771/step#print_start">
        <rdf:type rdf:resource="http://www.w3.org/2006/time#Instant"/>
        <dc:creator rdf:resource="http://www.heidelberg.com/"/>
        <rdfs:label xml:lang="de">Druckbeginn</rdfs:label>
        <rdfs:label xml:lang="en">print start</rdfs:label>
    </owl:NamedIndividual>
    


    <!-- http://people.aifb.kit.edu/mu2771/step#print_tech_delivery_chain -->

    <owl:NamedIndividual rdf:about="http://people.aifb.kit.edu/mu2771/step#print_tech_delivery_chain">
        <rdf:type rdf:resource="http://purl.oclc.org/NET/ssnx/ssn#Device"/>
        <step:sourceUri rdf:resource="http://people.aifb.kit.edu/mu2771/step#"/>
        <rdfs:label xml:lang="de">Auslegerkette</rdfs:label>
        <rdfs:label xml:lang="en">print tech. delivery chain</rdfs:label>
        <part:partOf rdf:resource="http://people.aifb.kit.edu/mu2771/step#print_press_bed"/>
    </owl:NamedIndividual>
    


    <!-- http://people.aifb.kit.edu/mu2771/step#print_tech_distributing_cylinder -->

    <owl:NamedIndividual rdf:about="http://people.aifb.kit.edu/mu2771/step#print_tech_distributing_cylinder">
        <rdf:type rdf:resource="http://purl.oclc.org/NET/ssnx/ssn#Device"/>
        <step:sourceUri rdf:resource="http://people.aifb.kit.edu/mu2771/step#"/>
        <rdfs:label xml:lang="de">Verreiberzylinder</rdfs:label>
        <rdfs:label xml:lang="en">print tech. distributing cylinder</rdfs:label>
        <part:partOf rdf:resource="http://people.aifb.kit.edu/mu2771/step#print_tech_perfecting_drum"/>
        <part:partOf rdf:resource="http://people.aifb.kit.edu/mu2771/step#turning_drum"/>
    </owl:NamedIndividual>
    


    <!-- http://people.aifb.kit.edu/mu2771/step#print_tech_perfecting_drum -->

    <owl:NamedIndividual rdf:about="http://people.aifb.kit.edu/mu2771/step#print_tech_perfecting_drum">
        <rdf:type rdf:resource="http://purl.oclc.org/NET/ssnx/ssn#Device"/>
        <owl:sameAs rdf:resource="http://people.aifb.kit.edu/mu2771/step#turning_drum"/>
        <step:sourceUri rdf:resource="http://people.aifb.kit.edu/mu2771/step#"/>
        <rdfs:label xml:lang="de">Wendetrommel</rdfs:label>
        <rdfs:label xml:lang="en">print tech. perfecting drum</rdfs:label>
        <part:partOf rdf:resource="http://people.aifb.kit.edu/mu2771/step#printing_press"/>
    </owl:NamedIndividual>
    


    <!-- http://people.aifb.kit.edu/mu2771/step#printing_cylinder -->

    <owl:NamedIndividual rdf:about="http://people.aifb.kit.edu/mu2771/step#printing_cylinder">
        <rdf:type rdf:resource="http://purl.oclc.org/NET/ssnx/ssn#Device"/>
        <rdf:type rdf:resource="http://purl.oclc.org/NET/ssnx/ssn#System"/>
        <step:sourceUri rdf:resource="http://people.aifb.kit.edu/mu2771/step#"/>
        <rdfs:label xml:lang="de">Druckzylinder</rdfs:label>
        <rdfs:label xml:lang="de">Gegendruckzylinder</rdfs:label>
        <rdfs:label xml:lang="en">impression cylinder</rdfs:label>
        <rdfs:label xml:lang="en">print counter-pressure cylinder </rdfs:label>
        <rdfs:label xml:lang="en">print counterpressure cylinder </rdfs:label>
        <rdfs:label xml:lang="en">printing cylinder</rdfs:label>
        <part:partOf rdf:resource="http://people.aifb.kit.edu/mu2771/step#ink_train"/>
        <part:partOf rdf:resource="http://people.aifb.kit.edu/mu2771/step#inking_station"/>
        <part:partOf rdf:resource="http://people.aifb.kit.edu/mu2771/step#inking_system"/>
        <part:partOf rdf:resource="http://people.aifb.kit.edu/mu2771/step#inking_unit"/>
        <part:partOf rdf:resource="http://people.aifb.kit.edu/mu2771/step#printing_press"/>
        <part:partOf rdf:resource="http://people.aifb.kit.edu/mu2771/step#take-up_roller"/>
    </owl:NamedIndividual>
    


    <!-- http://people.aifb.kit.edu/mu2771/step#printing_material -->

    <owl:NamedIndividual rdf:about="http://people.aifb.kit.edu/mu2771/step#printing_material">
        <rdf:type rdf:resource="http://people.aifb.kit.edu/mu2771/step#Product"/>
        <dc:creator rdf:resource="http://www.heidelberg.com/"/>
        <rdfs:label xml:lang="de">Bedruckstoff</rdfs:label>
        <rdfs:label xml:lang="en">printing material</rdfs:label>
    </owl:NamedIndividual>
    


    <!-- http://people.aifb.kit.edu/mu2771/step#printing_material_length -->

    <owl:NamedIndividual rdf:about="http://people.aifb.kit.edu/mu2771/step#printing_material_length">
        <rdf:type rdf:resource="http://qudt.org/schema/qudt#LengthUnit"/>
        <dc:creator rdf:resource="http://www.heidelberg.com/"/>
        <rdfs:label xml:lang="de">Bedruckstofflänge</rdfs:label>
        <rdfs:label xml:lang="en">printing material length</rdfs:label>
    </owl:NamedIndividual>
    


    <!-- http://people.aifb.kit.edu/mu2771/step#printing_material_width -->

    <owl:NamedIndividual rdf:about="http://people.aifb.kit.edu/mu2771/step#printing_material_width">
        <rdf:type rdf:resource="http://qudt.org/schema/qudt#LengthUnit"/>
        <dc:creator rdf:resource="http://www.heidelberg.com/"/>
        <rdfs:label xml:lang="de">Bedruckstoffbreite</rdfs:label>
        <rdfs:label xml:lang="en">printing material width</rdfs:label>
    </owl:NamedIndividual>
    


    <!-- http://people.aifb.kit.edu/mu2771/step#printing_press -->

    <owl:NamedIndividual rdf:about="http://people.aifb.kit.edu/mu2771/step#printing_press">
        <rdf:type rdf:resource="http://purl.oclc.org/NET/ssnx/ssn#System"/>
        <step:sourceUri rdf:resource="http://people.aifb.kit.edu/mu2771/step#"/>
        <rdfs:label xml:lang="de">Druckmaschine</rdfs:label>
        <rdfs:label xml:lang="en">printing press</rdfs:label>
    </owl:NamedIndividual>
    


    <!-- http://people.aifb.kit.edu/mu2771/step#pull_lay -->

    <owl:NamedIndividual rdf:about="http://people.aifb.kit.edu/mu2771/step#pull_lay">
        <rdf:type rdf:resource="http://people.aifb.kit.edu/mu2771/step#Product"/>
        <dc:creator rdf:resource="http://www.heidelberg.com/"/>
        <rdfs:label xml:lang="de">Ziehmarke</rdfs:label>
        <rdfs:label xml:lang="en">pull lay</rdfs:label>
    </owl:NamedIndividual>
    


    <!-- http://people.aifb.kit.edu/mu2771/step#pump -->

    <owl:NamedIndividual rdf:about="http://people.aifb.kit.edu/mu2771/step#pump">
        <rdf:type rdf:resource="http://purl.oclc.org/NET/ssnx/ssn#Device"/>
        <dc:creator rdf:resource="http://www.heidelberg.com/"/>
        <rdfs:label xml:lang="de">Pumpe</rdfs:label>
        <rdfs:label xml:lang="en">pump</rdfs:label>
        <part:partOf rdf:resource="http://people.aifb.kit.edu/mu2771/step#washing_fluid_container"/>
    </owl:NamedIndividual>
    


    <!-- http://people.aifb.kit.edu/mu2771/step#pwm-signal -->

    <owl:NamedIndividual rdf:about="http://people.aifb.kit.edu/mu2771/step#pwm-signal">
        <rdf:type rdf:resource="http://purl.org/ontology/mo/produced_signal"/>
        <dc:creator rdf:resource="http://www.aifb.kit.edu/web/Sebastian_Bader"/>
        <rdfs:label xml:lang="de">PW-Signal</rdfs:label>
        <rdfs:label xml:lang="de">PW-Signale</rdfs:label>
        <rdfs:label xml:lang="de">PWM-Signal</rdfs:label>
        <rdfs:label xml:lang="de">PWM-Signale</rdfs:label>
        <rdfs:label xml:lang="en">pwm signal</rdfs:label>
    </owl:NamedIndividual>
    


    <!-- http://people.aifb.kit.edu/mu2771/step#rated_output -->

    <owl:NamedIndividual rdf:about="http://people.aifb.kit.edu/mu2771/step#rated_output">
        <rdf:type rdf:resource="http://qudt.org/schema/qudt#ElectricityAndMagnetismQuantityKind"/>
        <dc:creator rdf:resource="http://www.heidelberg.com/"/>
        <rdfs:label xml:lang="de">Nennleistung</rdfs:label>
        <rdfs:label xml:lang="en">rated output</rdfs:label>
    </owl:NamedIndividual>
    


    <!-- http://people.aifb.kit.edu/mu2771/step#register -->

    <owl:NamedIndividual rdf:about="http://people.aifb.kit.edu/mu2771/step#register">
        <rdf:type rdf:resource="http://purl.oclc.org/NET/ssnx/ssn#System"/>
        <dc:creator rdf:resource="http://www.heidelberg.com/"/>
        <rdfs:label xml:lang="de">Register</rdfs:label>
        <rdfs:label xml:lang="en">register</rdfs:label>
        <part:partOf rdf:resource="http://people.aifb.kit.edu/mu2771/step#printing_press"/>
    </owl:NamedIndividual>
    


    <!-- http://people.aifb.kit.edu/mu2771/step#ribbon_feeding_feature -->

    <owl:NamedIndividual rdf:about="http://people.aifb.kit.edu/mu2771/step#ribbon_feeding_feature">
        <rdf:type rdf:resource="http://purl.oclc.org/NET/ssnx/ssn#Device"/>
        <step:sourceUri rdf:resource="http://people.aifb.kit.edu/mu2771/step#"/>
        <rdfs:label xml:lang="de">Farbtuchantrieb</rdfs:label>
        <rdfs:label xml:lang="en">ribbon feeding feature</rdfs:label>
        <part:partOf rdf:resource="http://people.aifb.kit.edu/mu2771/step#print_tech_perfecting_drum"/>
        <part:partOf rdf:resource="http://people.aifb.kit.edu/mu2771/step#turning_drum"/>
    </owl:NamedIndividual>
    


    <!-- http://people.aifb.kit.edu/mu2771/step#rotary-valve -->

    <owl:NamedIndividual rdf:about="http://people.aifb.kit.edu/mu2771/step#rotary-valve">
        <rdf:type rdf:resource="http://purl.oclc.org/NET/ssnx/ssn#Device"/>
        <dc:creator rdf:resource="http://www.aifb.kit.edu/web/Sebastian_Bader"/>
        <rdfs:label xml:lang="de">Drehventil</rdfs:label>
        <rdfs:label xml:lang="en">rotary valve</rdfs:label>
        <part:partOf rdf:resource="http://people.aifb.kit.edu/mu2771/step#dampening_shutter"/>
        <part:partOf rdf:resource="http://people.aifb.kit.edu/mu2771/step#indent"/>
        <part:partOf rdf:resource="http://people.aifb.kit.edu/mu2771/step#pre-gripper"/>
        <part:partOf rdf:resource="http://people.aifb.kit.edu/mu2771/step#print_counter-pressure_cylinder"/>
    </owl:NamedIndividual>
    


    <!-- http://people.aifb.kit.edu/mu2771/step#rubber_blanket_cylinder -->

    <owl:NamedIndividual rdf:about="http://people.aifb.kit.edu/mu2771/step#rubber_blanket_cylinder">
        <rdf:type rdf:resource="http://purl.oclc.org/NET/ssnx/ssn#Device"/>
        <step:sourceUri rdf:resource="http://people.aifb.kit.edu/mu2771/step#"/>
        <rdfs:label xml:lang="en">(rubber) blanket cylinder</rdfs:label>
        <rdfs:label xml:lang="de">Farbtuchzylinder</rdfs:label>
        <rdfs:label xml:lang="en">blanket cylinder</rdfs:label>
        <rdfs:label xml:lang="en">rubber blanket cylinder</rdfs:label>
        <part:partOf rdf:resource="http://people.aifb.kit.edu/mu2771/step#ribbon_feeding_feature"/>
    </owl:NamedIndividual>
    


    <!-- http://people.aifb.kit.edu/mu2771/step#rubber_blanket_plate -->

    <owl:NamedIndividual rdf:about="http://people.aifb.kit.edu/mu2771/step#rubber_blanket_plate">
        <rdf:type rdf:resource="http://purl.oclc.org/NET/ssnx/ssn#Device"/>
        <step:sourceUri rdf:resource="http://people.aifb.kit.edu/mu2771/step#"/>
        <rdfs:label xml:lang="de">Gummituchplatte</rdfs:label>
        <rdfs:label xml:lang="en">rubber blanket plate</rdfs:label>
        <part:partOf rdf:resource="http://people.aifb.kit.edu/mu2771/step#print_tech_perfecting_drum"/>
        <part:partOf rdf:resource="http://people.aifb.kit.edu/mu2771/step#turning_drum"/>
    </owl:NamedIndividual>
    


    <!-- http://people.aifb.kit.edu/mu2771/step#rubber_underpacking -->

    <owl:NamedIndividual rdf:about="http://people.aifb.kit.edu/mu2771/step#rubber_underpacking">
        <rdf:type rdf:resource="http://purl.oclc.org/NET/ssnx/ssn#Device"/>
        <step:sourceUri rdf:resource="http://people.aifb.kit.edu/mu2771/step#"/>
        <rdfs:label xml:lang="de">Gummituchunterlage</rdfs:label>
        <rdfs:label xml:lang="en">rubber underpacking</rdfs:label>
        <part:partOf rdf:resource="http://people.aifb.kit.edu/mu2771/step#rubber_blanket_plate"/>
    </owl:NamedIndividual>
    


    <!-- http://people.aifb.kit.edu/mu2771/step#sample_sheet -->

    <owl:NamedIndividual rdf:about="http://people.aifb.kit.edu/mu2771/step#sample_sheet">
        <rdf:type rdf:resource="http://people.aifb.kit.edu/mu2771/step#Product"/>
        <dc:creator rdf:resource="http://www.heidelberg.com/"/>
        <rdfs:label xml:lang="de">Probebogen</rdfs:label>
        <rdfs:label xml:lang="en">sample sheet</rdfs:label>
    </owl:NamedIndividual>
    


    <!-- http://people.aifb.kit.edu/mu2771/step#sample_sheet_removal -->

    <owl:NamedIndividual rdf:about="http://people.aifb.kit.edu/mu2771/step#sample_sheet_removal">
        <rdf:type rdf:resource="http://people.aifb.kit.edu/mu2771/step#Process"/>
        <dc:creator rdf:resource="http://www.heidelberg.com/"/>
        <rdfs:label xml:lang="de">Probebogenentnahme</rdfs:label>
        <rdfs:label xml:lang="en">sample sheet removal</rdfs:label>
    </owl:NamedIndividual>
    


    <!-- http://people.aifb.kit.edu/mu2771/step#screen -->

    <owl:NamedIndividual rdf:about="http://people.aifb.kit.edu/mu2771/step#screen">
        <rdf:type rdf:resource="http://purl.oclc.org/NET/ssnx/ssn#System"/>
        <dc:creator rdf:resource="http://www.heidelberg.com/"/>
        <rdfs:label xml:lang="de">Raster</rdfs:label>
        <rdfs:label xml:lang="en">screen</rdfs:label>
        <part:partOf rdf:resource="http://people.aifb.kit.edu/mu2771/step#register"/>
    </owl:NamedIndividual>
    


    <!-- http://people.aifb.kit.edu/mu2771/step#screening_settings -->

    <owl:Thing rdf:about="http://people.aifb.kit.edu/mu2771/step#screening_settings">
        <rdf:type rdf:resource="http://www.w3.org/2002/07/owl#NamedIndividual"/>
        <dc:creator rdf:resource="http://www.heidelberg.com/"/>
        <rdfs:label xml:lang="de">Rastereinstellung</rdfs:label>
        <rdfs:label xml:lang="en">screening settings</rdfs:label>
    </owl:Thing>
    


    <!-- http://people.aifb.kit.edu/mu2771/step#service_display -->

    <owl:NamedIndividual rdf:about="http://people.aifb.kit.edu/mu2771/step#service_display">
        <rdf:type rdf:resource="http://purl.oclc.org/NET/ssnx/ssn#Device"/>
        <dc:creator rdf:resource="http://www.heidelberg.com/"/>
        <rdfs:label xml:lang="de">Serviceanzeige</rdfs:label>
        <rdfs:label xml:lang="en">service display</rdfs:label>
        <part:partOf rdf:resource="http://people.aifb.kit.edu/mu2771/step#control_console"/>
    </owl:NamedIndividual>
    


    <!-- http://people.aifb.kit.edu/mu2771/step#sheet_counter -->

    <owl:NamedIndividual rdf:about="http://people.aifb.kit.edu/mu2771/step#sheet_counter">
        <rdf:type rdf:resource="http://purl.oclc.org/NET/ssnx/ssn#Device"/>
        <step:sourceUri rdf:resource="http://people.aifb.kit.edu/mu2771/step#"/>
        <rdfs:label xml:lang="de">Bogenzähler</rdfs:label>
        <rdfs:label xml:lang="en">sheet counter</rdfs:label>
        <part:partOf rdf:resource="http://people.aifb.kit.edu/mu2771/step#indent"/>
    </owl:NamedIndividual>
    


    <!-- http://people.aifb.kit.edu/mu2771/step#sheet_front_edge -->

    <owl:Thing rdf:about="http://people.aifb.kit.edu/mu2771/step#sheet_front_edge">
        <rdf:type rdf:resource="http://www.w3.org/2002/07/owl#NamedIndividual"/>
        <dc:creator rdf:resource="http://www.heidelberg.com/"/>
        <rdfs:label xml:lang="de">Papieranfang</rdfs:label>
        <rdfs:label xml:lang="en">sheet front edge</rdfs:label>
    </owl:Thing>
    


    <!-- http://people.aifb.kit.edu/mu2771/step#sheet_jogger -->

    <owl:NamedIndividual rdf:about="http://people.aifb.kit.edu/mu2771/step#sheet_jogger">
        <rdf:type rdf:resource="http://purl.oclc.org/NET/ssnx/ssn#Device"/>
        <step:sourceUri rdf:resource="http://people.aifb.kit.edu/mu2771/step#"/>
        <rdfs:label xml:lang="en">(sheet) jogger</rdfs:label>
        <rdfs:label xml:lang="de">Bogengeradstoßer</rdfs:label>
        <rdfs:label xml:lang="en">jogger</rdfs:label>
        <rdfs:label xml:lang="en">sheet jogger</rdfs:label>
        <part:partOf rdf:resource="http://people.aifb.kit.edu/mu2771/step#sheet_monitoring"/>
    </owl:NamedIndividual>
    


    <!-- http://people.aifb.kit.edu/mu2771/step#sheet_monitoring -->

    <owl:NamedIndividual rdf:about="http://people.aifb.kit.edu/mu2771/step#sheet_monitoring">
        <rdf:type rdf:resource="http://purl.oclc.org/NET/ssnx/ssn#Device"/>
        <dc:creator rdf:resource="http://www.heidelberg.com/"/>
        <rdfs:label xml:lang="de">Bogenüberwachung</rdfs:label>
        <rdfs:label xml:lang="en">sheet monitoring</rdfs:label>
        <part:partOf rdf:resource="http://people.aifb.kit.edu/mu2771/step#indent"/>
    </owl:NamedIndividual>
    


    <!-- http://people.aifb.kit.edu/mu2771/step#sheet_reversal -->

    <owl:Thing rdf:about="http://people.aifb.kit.edu/mu2771/step#sheet_reversal">
        <rdf:type rdf:resource="http://www.w3.org/2002/07/owl#NamedIndividual"/>
        <dc:creator rdf:resource="http://www.heidelberg.com/"/>
        <rdfs:label xml:lang="de">Wendung</rdfs:label>
        <rdfs:label xml:lang="en">sheet reversal</rdfs:label>
    </owl:Thing>
    


    <!-- http://people.aifb.kit.edu/mu2771/step#sheet_size -->

    <owl:Thing rdf:about="http://people.aifb.kit.edu/mu2771/step#sheet_size">
        <rdf:type rdf:resource="http://www.w3.org/2002/07/owl#NamedIndividual"/>
        <dc:creator rdf:resource="http://www.heidelberg.com/"/>
        <rdfs:label xml:lang="de">Druckbogenformat</rdfs:label>
        <rdfs:label xml:lang="en">sheet size</rdfs:label>
    </owl:Thing>
    


    <!-- http://people.aifb.kit.edu/mu2771/step#sheet_stop -->

    <owl:NamedIndividual rdf:about="http://people.aifb.kit.edu/mu2771/step#sheet_stop">
        <rdf:type rdf:resource="http://purl.oclc.org/NET/ssnx/ssn#Device"/>
        <dc:creator rdf:resource="http://www.heidelberg.com/"/>
        <rdfs:label xml:lang="de">Papieranschlag</rdfs:label>
        <rdfs:label xml:lang="en">sheet stop</rdfs:label>
        <part:partOf rdf:resource="http://people.aifb.kit.edu/mu2771/step#indent"/>
    </owl:NamedIndividual>
    


    <!-- http://people.aifb.kit.edu/mu2771/step#sidelay -->

    <owl:NamedIndividual rdf:about="http://people.aifb.kit.edu/mu2771/step#sidelay">
        <rdf:type rdf:resource="http://purl.oclc.org/NET/ssnx/ssn#Device"/>
        <step:sourceUri rdf:resource="http://people.aifb.kit.edu/mu2771/step#"/>
        <rdfs:label xml:lang="de">Seitenmarke</rdfs:label>
        <rdfs:label xml:lang="en">sidelay</rdfs:label>
        <part:partOf rdf:resource="http://people.aifb.kit.edu/mu2771/step#indent"/>
    </owl:NamedIndividual>
    


    <!-- http://people.aifb.kit.edu/mu2771/step#signal_device -->

    <owl:NamedIndividual rdf:about="http://people.aifb.kit.edu/mu2771/step#signal_device">
        <rdf:type rdf:resource="http://purl.oclc.org/NET/ssnx/ssn#Device"/>
        <dc:creator rdf:resource="http://www.heidelberg.com/"/>
        <rdfs:label xml:lang="de">Signalgeber</rdfs:label>
        <rdfs:label xml:lang="en">signal device</rdfs:label>
        <part:partOf rdf:resource="http://people.aifb.kit.edu/mu2771/step#service_display"/>
    </owl:NamedIndividual>
    


    <!-- http://people.aifb.kit.edu/mu2771/step#single_sheet_feeder -->

    <owl:NamedIndividual rdf:about="http://people.aifb.kit.edu/mu2771/step#single_sheet_feeder">
        <rdf:type rdf:resource="http://purl.oclc.org/NET/ssnx/ssn#Device"/>
        <step:sourceUri rdf:resource="http://people.aifb.kit.edu/mu2771/step#"/>
        <rdfs:label xml:lang="de">Saugstangenanleger</rdfs:label>
        <rdfs:label xml:lang="en">single sheet feeder</rdfs:label>
        <part:partOf rdf:resource="http://people.aifb.kit.edu/mu2771/step#printing_press"/>
    </owl:NamedIndividual>
    


    <!-- http://people.aifb.kit.edu/mu2771/step#slide-in_dryer -->

    <owl:NamedIndividual rdf:about="http://people.aifb.kit.edu/mu2771/step#slide-in_dryer">
        <rdf:type rdf:resource="http://purl.oclc.org/NET/ssnx/ssn#Device"/>
        <dc:creator rdf:resource="http://www.heidelberg.com/"/>
        <rdfs:label xml:lang="de">Trocknereinschub</rdfs:label>
        <rdfs:label xml:lang="en">slide-in dryer</rdfs:label>
        <part:partOf rdf:resource="http://people.aifb.kit.edu/mu2771/step#indent"/>
    </owl:NamedIndividual>
    


    <!-- http://people.aifb.kit.edu/mu2771/step#speed -->

    <owl:Thing rdf:about="http://people.aifb.kit.edu/mu2771/step#speed">
        <rdf:type rdf:resource="http://www.w3.org/2002/07/owl#NamedIndividual"/>
        <dc:creator rdf:resource="http://www.heidelberg.com/"/>
        <rdfs:label xml:lang="de">Geschwindigkeit</rdfs:label>
        <rdfs:label xml:lang="en">speed</rdfs:label>
    </owl:Thing>
    


    <!-- http://people.aifb.kit.edu/mu2771/step#speed_control -->

    <owl:NamedIndividual rdf:about="http://people.aifb.kit.edu/mu2771/step#speed_control">
        <rdf:type rdf:resource="http://people.aifb.kit.edu/mu2771/step#Process"/>
        <dc:creator rdf:resource="http://www.heidelberg.com/"/>
        <rdfs:label xml:lang="de">Geschwindigkeitsregulierung</rdfs:label>
        <rdfs:label xml:lang="en">speed control</rdfs:label>
    </owl:NamedIndividual>
    


    <!-- http://people.aifb.kit.edu/mu2771/step#square-wave-signal -->

    <owl:NamedIndividual rdf:about="http://people.aifb.kit.edu/mu2771/step#square-wave-signal">
        <rdf:type rdf:resource="http://purl.org/ontology/mo/produced_signal"/>
        <dc:creator rdf:resource="http://www.aifb.kit.edu/web/Sebastian_Bader"/>
        <rdfs:label xml:lang="de">Rechtecksignale</rdfs:label>
        <rdfs:label xml:lang="en">square wave signal</rdfs:label>
        <rdfs:label xml:lang="en">square-wave signal</rdfs:label>
    </owl:NamedIndividual>
    


    <!-- http://people.aifb.kit.edu/mu2771/step#steel_distributor_roller -->

    <owl:NamedIndividual rdf:about="http://people.aifb.kit.edu/mu2771/step#steel_distributor_roller">
        <rdf:type rdf:resource="http://purl.oclc.org/NET/ssnx/ssn#System"/>
        <step:sourceUri rdf:resource="http://people.aifb.kit.edu/mu2771/step#"/>
        <rdfs:label xml:lang="de">Stahlreiber</rdfs:label>
        <rdfs:label xml:lang="en">steel distributor</rdfs:label>
        <rdfs:label xml:lang="en">steel distributor (roller)</rdfs:label>
        <rdfs:label xml:lang="en">steel distributor roller</rdfs:label>
        <part:partOf rdf:resource="http://people.aifb.kit.edu/mu2771/step#print_press_bed"/>
    </owl:NamedIndividual>
    


    <!-- http://people.aifb.kit.edu/mu2771/step#straight_printing -->

    <owl:Thing rdf:about="http://people.aifb.kit.edu/mu2771/step#straight_printing">
        <rdf:type rdf:resource="http://www.w3.org/2002/07/owl#NamedIndividual"/>
        <dc:creator rdf:resource="http://www.heidelberg.com/"/>
        <rdfs:label xml:lang="de">Schöndruck</rdfs:label>
        <rdfs:label xml:lang="en">straight printing</rdfs:label>
    </owl:Thing>
    


    <!-- http://people.aifb.kit.edu/mu2771/step#suction_head -->

    <owl:NamedIndividual rdf:about="http://people.aifb.kit.edu/mu2771/step#suction_head">
        <rdf:type rdf:resource="http://purl.oclc.org/NET/ssnx/ssn#Device"/>
        <dc:creator rdf:resource="http://www.heidelberg.com/"/>
        <rdfs:label xml:lang="de">Saugkopf</rdfs:label>
        <rdfs:label xml:lang="en">suction head</rdfs:label>
        <part:partOf rdf:resource="http://people.aifb.kit.edu/mu2771/step#dampening_system"/>
        <part:partOf rdf:resource="http://people.aifb.kit.edu/mu2771/step#dampening_unit"/>
        <part:partOf rdf:resource="http://people.aifb.kit.edu/mu2771/step#damping_unit"/>
        <part:partOf rdf:resource="http://people.aifb.kit.edu/mu2771/step#moistener"/>
        <part:partOf rdf:resource="http://people.aifb.kit.edu/mu2771/step#print_dampener"/>
    </owl:NamedIndividual>
    


    <!-- http://people.aifb.kit.edu/mu2771/step#suction_head_drive -->

    <owl:NamedIndividual rdf:about="http://people.aifb.kit.edu/mu2771/step#suction_head_drive">
        <rdf:type rdf:resource="http://purl.oclc.org/NET/ssnx/ssn#Device"/>
        <dc:creator rdf:resource="http://www.heidelberg.com/"/>
        <rdfs:label xml:lang="de">Saugkopfantrieb</rdfs:label>
        <rdfs:label xml:lang="en">suction head drive</rdfs:label>
        <part:partOf rdf:resource="http://people.aifb.kit.edu/mu2771/step#suction_head"/>
    </owl:NamedIndividual>
    


    <!-- http://people.aifb.kit.edu/mu2771/step#suction_pile_feeder -->

    <owl:NamedIndividual rdf:about="http://people.aifb.kit.edu/mu2771/step#suction_pile_feeder">
        <rdf:type rdf:resource="http://purl.oclc.org/NET/ssnx/ssn#Device"/>
        <step:sourceUri rdf:resource="http://people.aifb.kit.edu/mu2771/step#"/>
        <rdfs:label xml:lang="de">Saugstapelanleger</rdfs:label>
        <rdfs:label xml:lang="en">suction pile feeder</rdfs:label>
        <part:partOf rdf:resource="http://people.aifb.kit.edu/mu2771/step#Saugstangenanleger"/>
    </owl:NamedIndividual>
    


    <!-- http://people.aifb.kit.edu/mu2771/step#suction_pressure -->

    <owl:Thing rdf:about="http://people.aifb.kit.edu/mu2771/step#suction_pressure">
        <rdf:type rdf:resource="http://www.w3.org/2002/07/owl#NamedIndividual"/>
        <dc:creator rdf:resource="http://www.heidelberg.com/"/>
        <rdfs:label xml:lang="de">Saugdruck</rdfs:label>
        <rdfs:label xml:lang="en">suction pressure</rdfs:label>
    </owl:Thing>
    


    <!-- http://people.aifb.kit.edu/mu2771/step#suction_tape -->

    <owl:NamedIndividual rdf:about="http://people.aifb.kit.edu/mu2771/step#suction_tape">
        <rdf:type rdf:resource="http://purl.oclc.org/NET/ssnx/ssn#Device"/>
        <dc:creator rdf:resource="http://www.heidelberg.com/"/>
        <rdfs:label xml:lang="de">Saugband</rdfs:label>
        <rdfs:label xml:lang="en">suction tape</rdfs:label>
        <part:partOf rdf:resource="http://people.aifb.kit.edu/mu2771/step#suction_head"/>
    </owl:NamedIndividual>
    


    <!-- http://people.aifb.kit.edu/mu2771/step#swing_gripper -->

    <owl:NamedIndividual rdf:about="http://people.aifb.kit.edu/mu2771/step#swing_gripper">
        <rdf:type rdf:resource="http://purl.oclc.org/NET/ssnx/ssn#Device"/>
        <step:sourceUri rdf:resource="http://people.aifb.kit.edu/mu2771/step#"/>
        <rdfs:label xml:lang="de">Schwunggreifer</rdfs:label>
        <rdfs:label xml:lang="en">swing gripper</rdfs:label>
        <part:partOf rdf:resource="http://people.aifb.kit.edu/mu2771/step#printing_press"/>
    </owl:NamedIndividual>
    


    <!-- http://people.aifb.kit.edu/mu2771/step#take-up_roller -->

    <owl:NamedIndividual rdf:about="http://people.aifb.kit.edu/mu2771/step#take-up_roller">
        <rdf:type rdf:resource="http://purl.oclc.org/NET/ssnx/ssn#Device"/>
        <rdf:type rdf:resource="http://purl.oclc.org/NET/ssnx/ssn#System"/>
        <step:sourceUri rdf:resource="http://people.aifb.kit.edu/mu2771/step#"/>
        <rdfs:label xml:lang="de">Farbheber</rdfs:label>
        <rdfs:label xml:lang="de">Farbwerk</rdfs:label>
        <rdfs:label xml:lang="en">ink train</rdfs:label>
        <rdfs:label xml:lang="en">inking station</rdfs:label>
        <rdfs:label xml:lang="en">inking system</rdfs:label>
        <rdfs:label xml:lang="en">inking unit</rdfs:label>
        <rdfs:label xml:lang="en">take-up roller</rdfs:label>
        <part:partOf rdf:resource="http://people.aifb.kit.edu/mu2771/step#printing_press"/>
    </owl:NamedIndividual>
    


    <!-- http://people.aifb.kit.edu/mu2771/step#tech_bearer_ring -->

    <owl:NamedIndividual rdf:about="http://people.aifb.kit.edu/mu2771/step#tech_bearer_ring">
        <rdf:type rdf:resource="http://purl.oclc.org/NET/ssnx/ssn#Device"/>
        <step:sourceUri rdf:resource="http://people.aifb.kit.edu/mu2771/step#"/>
        <rdfs:label xml:lang="de">Schmitzring</rdfs:label>
        <rdfs:label xml:lang="en">tech. bearer ring</rdfs:label>
        <part:partOf rdf:resource="http://people.aifb.kit.edu/mu2771/step#print_impression_cylinder"/>
    </owl:NamedIndividual>
    


    <!-- http://people.aifb.kit.edu/mu2771/step#temperature_setting -->

    <owl:Thing rdf:about="http://people.aifb.kit.edu/mu2771/step#temperature_setting">
        <rdf:type rdf:resource="http://www.w3.org/2002/07/owl#NamedIndividual"/>
        <dc:creator rdf:resource="http://www.heidelberg.com/"/>
        <rdfs:label xml:lang="de">Temperatureinstellung</rdfs:label>
        <rdfs:label xml:lang="en">temperature setting</rdfs:label>
    </owl:Thing>
    


    <!-- http://people.aifb.kit.edu/mu2771/step#transfer_roll -->

    <owl:NamedIndividual rdf:about="http://people.aifb.kit.edu/mu2771/step#transfer_roll">
        <rdf:type rdf:resource="http://purl.oclc.org/NET/ssnx/ssn#Device"/>
        <owl:sameAs rdf:resource="http://people.aifb.kit.edu/mu2771/step#transfer_roller"/>
        <step:sourceUri rdf:resource="http://people.aifb.kit.edu/mu2771/step#"/>
        <rdfs:label xml:lang="en">transfer roll</rdfs:label>
        <rdfs:label xml:lang="de">Übertragwalze</rdfs:label>
        <part:partOf rdf:resource="http://people.aifb.kit.edu/mu2771/step#print_ink_transfer_roller"/>
        <part:partOf rdf:resource="http://people.aifb.kit.edu/mu2771/step#print_inking_roller"/>
    </owl:NamedIndividual>
    


    <!-- http://people.aifb.kit.edu/mu2771/step#transfer_roller -->

    <owl:NamedIndividual rdf:about="http://people.aifb.kit.edu/mu2771/step#transfer_roller">
        <rdf:type rdf:resource="http://purl.oclc.org/NET/ssnx/ssn#Device"/>
        <step:sourceUri rdf:resource="http://people.aifb.kit.edu/mu2771/step#"/>
        <rdfs:label xml:lang="en">transfer roll</rdfs:label>
        <rdfs:label xml:lang="en">transfer roller</rdfs:label>
        <rdfs:label xml:lang="de">Übertragwalze</rdfs:label>
        <part:partOf rdf:resource="http://people.aifb.kit.edu/mu2771/step#print_ink_transfer_roller"/>
        <part:partOf rdf:resource="http://people.aifb.kit.edu/mu2771/step#print_inking_roller"/>
    </owl:NamedIndividual>
    


    <!-- http://people.aifb.kit.edu/mu2771/step#turning_drum -->

    <owl:NamedIndividual rdf:about="http://people.aifb.kit.edu/mu2771/step#turning_drum">
        <rdf:type rdf:resource="http://purl.oclc.org/NET/ssnx/ssn#Device"/>
        <step:sourceUri rdf:resource="http://people.aifb.kit.edu/mu2771/step#"/>
        <rdfs:label xml:lang="de">Wendetrommel</rdfs:label>
        <rdfs:label xml:lang="en">print tech. perfecting drum</rdfs:label>
        <rdfs:label xml:lang="en">turning drum</rdfs:label>
        <part:partOf rdf:resource="http://people.aifb.kit.edu/mu2771/step#printing_press"/>
    </owl:NamedIndividual>
    


    <!-- http://people.aifb.kit.edu/mu2771/step#user_interface -->

    <owl:NamedIndividual rdf:about="http://people.aifb.kit.edu/mu2771/step#user_interface">
        <rdf:type rdf:resource="http://purl.oclc.org/NET/ssnx/ssn#System"/>
        <dc:creator rdf:resource="http://www.heidelberg.com/"/>
        <rdfs:label xml:lang="de">Bedienoberfläche</rdfs:label>
        <rdfs:label xml:lang="en">user interface</rdfs:label>
        <part:partOf rdf:resource="http://people.aifb.kit.edu/mu2771/step#control_console"/>
    </owl:NamedIndividual>
    


    <!-- http://people.aifb.kit.edu/mu2771/step#valve -->

    <owl:NamedIndividual rdf:about="http://people.aifb.kit.edu/mu2771/step#valve">
        <rdf:type rdf:resource="http://purl.oclc.org/NET/ssnx/ssn#Device"/>
        <dc:creator rdf:resource="http://www.heidelberg.com/"/>
        <rdfs:label xml:lang="de">Ventil</rdfs:label>
        <rdfs:label xml:lang="en">valve</rdfs:label>
        <part:partOf rdf:resource="http://people.aifb.kit.edu/mu2771/step#dampening_system"/>
        <part:partOf rdf:resource="http://people.aifb.kit.edu/mu2771/step#dampening_unit"/>
        <part:partOf rdf:resource="http://people.aifb.kit.edu/mu2771/step#damping_unit"/>
        <part:partOf rdf:resource="http://people.aifb.kit.edu/mu2771/step#moistener"/>
        <part:partOf rdf:resource="http://people.aifb.kit.edu/mu2771/step#print_dampener"/>
        <part:partOf rdf:resource="http://people.aifb.kit.edu/mu2771/step#suction_head"/>
        <part:partOf rdf:resource="http://people.aifb.kit.edu/mu2771/step#suction_pile_feeder"/>
    </owl:NamedIndividual>
    


    <!-- http://people.aifb.kit.edu/mu2771/step#varnish -->

    <owl:NamedIndividual rdf:about="http://people.aifb.kit.edu/mu2771/step#varnish">
        <rdf:type rdf:resource="http://people.aifb.kit.edu/mu2771/step#Product"/>
        <dc:creator rdf:resource="http://www.heidelberg.com/"/>
        <rdfs:label xml:lang="de">Lack</rdfs:label>
        <rdfs:label xml:lang="en">varnish</rdfs:label>
    </owl:NamedIndividual>
    


    <!-- http://people.aifb.kit.edu/mu2771/step#varnish_metering -->

    <owl:Thing rdf:about="http://people.aifb.kit.edu/mu2771/step#varnish_metering">
        <rdf:type rdf:resource="http://www.w3.org/2002/07/owl#NamedIndividual"/>
        <dc:creator rdf:resource="http://www.heidelberg.com/"/>
        <rdfs:label xml:lang="de">Lackdosierung</rdfs:label>
        <rdfs:label xml:lang="en">varnish metering</rdfs:label>
    </owl:Thing>
    


    <!-- http://people.aifb.kit.edu/mu2771/step#varnish_metering_roller -->

    <owl:Thing rdf:about="http://people.aifb.kit.edu/mu2771/step#varnish_metering_roller">
        <rdf:type rdf:resource="http://www.w3.org/2002/07/owl#NamedIndividual"/>
        <dc:creator rdf:resource="http://www.heidelberg.com/"/>
        <rdfs:label xml:lang="de">Lackdosierwalze</rdfs:label>
        <rdfs:label xml:lang="en">varnish metering roller</rdfs:label>
        <part:partOf rdf:resource="http://people.aifb.kit.edu/mu2771/step#dampening_system"/>
        <part:partOf rdf:resource="http://people.aifb.kit.edu/mu2771/step#dampening_unit"/>
        <part:partOf rdf:resource="http://people.aifb.kit.edu/mu2771/step#damping_unit"/>
        <part:partOf rdf:resource="http://people.aifb.kit.edu/mu2771/step#moistener"/>
        <part:partOf rdf:resource="http://people.aifb.kit.edu/mu2771/step#print_dampener"/>
    </owl:Thing>
    


    <!-- http://people.aifb.kit.edu/mu2771/step#varnish_tank -->

    <owl:NamedIndividual rdf:about="http://people.aifb.kit.edu/mu2771/step#varnish_tank">
        <rdf:type rdf:resource="http://purl.oclc.org/NET/ssnx/ssn#Device"/>
        <dc:creator rdf:resource="http://www.heidelberg.com/"/>
        <rdfs:label xml:lang="de">Lackbehälter</rdfs:label>
        <rdfs:label xml:lang="en">varnish tank</rdfs:label>
        <part:partOf rdf:resource="http://people.aifb.kit.edu/mu2771/step#varnish_metering_roller"/>
    </owl:NamedIndividual>
    


    <!-- http://people.aifb.kit.edu/mu2771/step#vibrating_dampening_roller -->

    <owl:NamedIndividual rdf:about="http://people.aifb.kit.edu/mu2771/step#vibrating_dampening_roller">
        <rdf:type rdf:resource="http://purl.oclc.org/NET/ssnx/ssn#Device"/>
        <step:sourceUri rdf:resource="http://people.aifb.kit.edu/mu2771/step#"/>
        <rdfs:label xml:lang="de">Feuchtheber</rdfs:label>
        <rdfs:label xml:lang="en">damping vibrator</rdfs:label>
        <rdfs:label xml:lang="en">vibrating dampening roller</rdfs:label>
        <part:partOf rdf:resource="http://people.aifb.kit.edu/mu2771/step#dampening_system"/>
        <part:partOf rdf:resource="http://people.aifb.kit.edu/mu2771/step#dampening_unit"/>
        <part:partOf rdf:resource="http://people.aifb.kit.edu/mu2771/step#damping_unit"/>
        <part:partOf rdf:resource="http://people.aifb.kit.edu/mu2771/step#moistener"/>
        <part:partOf rdf:resource="http://people.aifb.kit.edu/mu2771/step#print_dampener"/>
    </owl:NamedIndividual>
    


    <!-- http://people.aifb.kit.edu/mu2771/step#vibrator_drive -->

    <owl:NamedIndividual rdf:about="http://people.aifb.kit.edu/mu2771/step#vibrator_drive">
        <rdf:type rdf:resource="http://purl.oclc.org/NET/ssnx/ssn#Device"/>
        <dc:creator rdf:resource="http://www.heidelberg.com/"/>
        <rdfs:label xml:lang="de">Heberantrieb</rdfs:label>
        <rdfs:label xml:lang="en">vibrator drive</rdfs:label>
        <part:partOf rdf:resource="http://people.aifb.kit.edu/mu2771/step#ink_train"/>
        <part:partOf rdf:resource="http://people.aifb.kit.edu/mu2771/step#inking_station"/>
        <part:partOf rdf:resource="http://people.aifb.kit.edu/mu2771/step#inking_system"/>
        <part:partOf rdf:resource="http://people.aifb.kit.edu/mu2771/step#inking_unit"/>
        <part:partOf rdf:resource="http://people.aifb.kit.edu/mu2771/step#take-up_roller"/>
    </owl:NamedIndividual>
    


    <!-- http://people.aifb.kit.edu/mu2771/step#warning_signal -->

    <owl:Thing rdf:about="http://people.aifb.kit.edu/mu2771/step#warning_signal">
        <rdf:type rdf:resource="http://www.w3.org/2002/07/owl#NamedIndividual"/>
        <dc:creator rdf:resource="http://www.heidelberg.com/"/>
        <rdfs:label xml:lang="de">Warnsignal</rdfs:label>
        <rdfs:label xml:lang="en">warning signal</rdfs:label>
    </owl:Thing>
    


    <!-- http://people.aifb.kit.edu/mu2771/step#washing_fluid -->

    <owl:NamedIndividual rdf:about="http://people.aifb.kit.edu/mu2771/step#washing_fluid">
        <rdf:type rdf:resource="http://people.aifb.kit.edu/mu2771/step#Product"/>
        <dc:creator rdf:resource="http://www.heidelberg.com/"/>
        <rdfs:label xml:lang="de">Waschmittel</rdfs:label>
        <rdfs:label xml:lang="en">washing fluid</rdfs:label>
    </owl:NamedIndividual>
    


    <!-- http://people.aifb.kit.edu/mu2771/step#washing_fluid_container -->

    <owl:NamedIndividual rdf:about="http://people.aifb.kit.edu/mu2771/step#washing_fluid_container">
        <rdf:type rdf:resource="http://purl.oclc.org/NET/ssnx/ssn#Device"/>
        <dc:creator rdf:resource="http://www.heidelberg.com/"/>
        <rdfs:label xml:lang="de">Waschmittelbehälter</rdfs:label>
        <rdfs:label xml:lang="en">washing fluid container</rdfs:label>
        <part:partOf rdf:resource="http://people.aifb.kit.edu/mu2771/step#washup_device"/>
    </owl:NamedIndividual>
    


    <!-- http://people.aifb.kit.edu/mu2771/step#washup_device -->

    <owl:NamedIndividual rdf:about="http://people.aifb.kit.edu/mu2771/step#washup_device">
        <rdf:type rdf:resource="http://purl.oclc.org/NET/ssnx/ssn#Device"/>
        <dc:creator rdf:resource="http://www.heidelberg.com/"/>
        <rdfs:label xml:lang="de">Wascheinrichtung</rdfs:label>
        <rdfs:label xml:lang="en">washup device</rdfs:label>
        <part:partOf rdf:resource="http://people.aifb.kit.edu/mu2771/step#printing_press"/>
    </owl:NamedIndividual>
    


    <!-- http://people.aifb.kit.edu/mu2771/step#washup_speed -->

    <owl:Thing rdf:about="http://people.aifb.kit.edu/mu2771/step#washup_speed">
        <rdf:type rdf:resource="http://www.w3.org/2002/07/owl#NamedIndividual"/>
        <dc:creator rdf:resource="http://www.heidelberg.com/"/>
        <rdfs:label xml:lang="de">Waschgeschwindigkeit</rdfs:label>
        <rdfs:label xml:lang="en">washup speed</rdfs:label>
    </owl:Thing>
    


    <!-- http://people.aifb.kit.edu/mu2771/step#waste-sheet_counter -->

    <owl:NamedIndividual rdf:about="http://people.aifb.kit.edu/mu2771/step#waste-sheet_counter">
        <rdf:type rdf:resource="http://purl.oclc.org/NET/ssnx/ssn#Device"/>
        <dc:creator rdf:resource="http://www.heidelberg.com/"/>
        <rdfs:label xml:lang="de">Makulaturzähler</rdfs:label>
        <rdfs:label xml:lang="en">waste-sheet counter</rdfs:label>
        <part:partOf rdf:resource="http://people.aifb.kit.edu/mu2771/step#control_console"/>
    </owl:NamedIndividual>
    


    <!-- http://people.aifb.kit.edu/mu2771/step#waste_sheet -->

    <owl:NamedIndividual rdf:about="http://people.aifb.kit.edu/mu2771/step#waste_sheet">
        <rdf:type rdf:resource="http://people.aifb.kit.edu/mu2771/step#Product"/>
        <dc:creator rdf:resource="http://www.heidelberg.com/"/>
        <rdfs:label xml:lang="de">Makulaturbogen</rdfs:label>
        <rdfs:label xml:lang="en">waste sheet</rdfs:label>
    </owl:NamedIndividual>
    


    <!-- http://people.aifb.kit.edu/mu2771/step#water-duct_roller -->

    <owl:NamedIndividual rdf:about="http://people.aifb.kit.edu/mu2771/step#water-duct_roller">
        <rdf:type rdf:resource="http://purl.oclc.org/NET/ssnx/ssn#Device"/>
        <owl:sameAs rdf:resource="http://people.aifb.kit.edu/mu2771/step#water_duct_roller"/>
        <owl:sameAs rdf:resource="http://people.aifb.kit.edu/mu2771/step#water_fountain_roller"/>
        <step:sourceUri rdf:resource="http://people.aifb.kit.edu/mu2771/step#"/>
        <rdfs:label xml:lang="en">(water) fountain roller</rdfs:label>
        <rdfs:label xml:lang="de">Feuchtduktor</rdfs:label>
        <rdfs:label xml:lang="de">Feuchtwerkswalze</rdfs:label>
        <rdfs:label xml:lang="de">Feuchtwerkwalze</rdfs:label>
        <rdfs:label xml:lang="en">dampening fountain roller</rdfs:label>
        <rdfs:label xml:lang="en">fountain roller</rdfs:label>
        <rdfs:label xml:lang="en">water duct roller</rdfs:label>
        <rdfs:label xml:lang="en">water fountain roller</rdfs:label>
        <rdfs:label xml:lang="en">water-duct roller</rdfs:label>
        <part:partOf rdf:resource="http://people.aifb.kit.edu/mu2771/step#dampening_system"/>
        <part:partOf rdf:resource="http://people.aifb.kit.edu/mu2771/step#dampening_unit"/>
        <part:partOf rdf:resource="http://people.aifb.kit.edu/mu2771/step#damping_unit"/>
        <part:partOf rdf:resource="http://people.aifb.kit.edu/mu2771/step#moistener"/>
        <part:partOf rdf:resource="http://people.aifb.kit.edu/mu2771/step#print_dampener"/>
    </owl:NamedIndividual>
    


    <!-- http://people.aifb.kit.edu/mu2771/step#water_duct_roller -->

    <owl:NamedIndividual rdf:about="http://people.aifb.kit.edu/mu2771/step#water_duct_roller">
        <rdf:type rdf:resource="http://purl.oclc.org/NET/ssnx/ssn#Device"/>
        <owl:sameAs rdf:resource="http://people.aifb.kit.edu/mu2771/step#water_fountain_roller"/>
        <step:sourceUri rdf:resource="http://people.aifb.kit.edu/mu2771/step#"/>
        <rdfs:label xml:lang="en">(water) fountain roller</rdfs:label>
        <rdfs:label xml:lang="de">Feuchtduktor</rdfs:label>
        <rdfs:label xml:lang="de">Feuchtwerkswalze</rdfs:label>
        <rdfs:label xml:lang="de">Feuchtwerkwalze</rdfs:label>
        <rdfs:label xml:lang="en">dampening fountain roller</rdfs:label>
        <rdfs:label xml:lang="en">fountain roller</rdfs:label>
        <rdfs:label xml:lang="en">water duct roller</rdfs:label>
        <rdfs:label xml:lang="en">water fountain roller</rdfs:label>
        <rdfs:label xml:lang="en">water-duct roller</rdfs:label>
        <part:partOf rdf:resource="http://people.aifb.kit.edu/mu2771/step#dampening_system"/>
        <part:partOf rdf:resource="http://people.aifb.kit.edu/mu2771/step#dampening_unit"/>
        <part:partOf rdf:resource="http://people.aifb.kit.edu/mu2771/step#damping_unit"/>
        <part:partOf rdf:resource="http://people.aifb.kit.edu/mu2771/step#moistener"/>
        <part:partOf rdf:resource="http://people.aifb.kit.edu/mu2771/step#print_dampener"/>
    </owl:NamedIndividual>
    


    <!-- http://people.aifb.kit.edu/mu2771/step#water_fountain -->

    <owl:NamedIndividual rdf:about="http://people.aifb.kit.edu/mu2771/step#water_fountain">
        <rdf:type rdf:resource="http://purl.oclc.org/NET/ssnx/ssn#Device"/>
        <owl:sameAs rdf:resource="http://people.aifb.kit.edu/mu2771/step#water_pan"/>
        <step:sourceUri rdf:resource="http://people.aifb.kit.edu/mu2771/step#"/>
        <rdfs:label xml:lang="de">Wasserkasten</rdfs:label>
        <rdfs:label xml:lang="en">dampening fountain</rdfs:label>
        <rdfs:label xml:lang="en">water fountain</rdfs:label>
        <rdfs:label xml:lang="en">water pan</rdfs:label>
        <part:partOf rdf:resource="http://people.aifb.kit.edu/mu2771/step#dampening_form_roller"/>
    </owl:NamedIndividual>
    


    <!-- http://people.aifb.kit.edu/mu2771/step#water_fountain_roller -->

    <owl:NamedIndividual rdf:about="http://people.aifb.kit.edu/mu2771/step#water_fountain_roller">
        <rdf:type rdf:resource="http://purl.oclc.org/NET/ssnx/ssn#Device"/>
        <step:sourceUri rdf:resource="http://people.aifb.kit.edu/mu2771/step#"/>
        <rdfs:label xml:lang="en">(water) fountain roller</rdfs:label>
        <rdfs:label xml:lang="de">Feuchtduktor</rdfs:label>
        <rdfs:label xml:lang="de">Feuchtwerkswalze</rdfs:label>
        <rdfs:label xml:lang="de">Feuchtwerkwalze</rdfs:label>
        <rdfs:label xml:lang="en">dampening fountain roller</rdfs:label>
        <rdfs:label xml:lang="en">fountain roller</rdfs:label>
        <rdfs:label xml:lang="en">water duct roller</rdfs:label>
        <rdfs:label xml:lang="en">water fountain roller</rdfs:label>
        <rdfs:label xml:lang="en">water-duct roller</rdfs:label>
        <part:partOf rdf:resource="http://people.aifb.kit.edu/mu2771/step#dampening_system"/>
        <part:partOf rdf:resource="http://people.aifb.kit.edu/mu2771/step#dampening_unit"/>
        <part:partOf rdf:resource="http://people.aifb.kit.edu/mu2771/step#damping_unit"/>
        <part:partOf rdf:resource="http://people.aifb.kit.edu/mu2771/step#moistener"/>
        <part:partOf rdf:resource="http://people.aifb.kit.edu/mu2771/step#print_dampener"/>
    </owl:NamedIndividual>
    


    <!-- http://people.aifb.kit.edu/mu2771/step#water_pan -->

    <owl:NamedIndividual rdf:about="http://people.aifb.kit.edu/mu2771/step#water_pan">
        <rdf:type rdf:resource="http://purl.oclc.org/NET/ssnx/ssn#Device"/>
        <step:sourceUri rdf:resource="http://people.aifb.kit.edu/mu2771/step#"/>
        <rdfs:label xml:lang="de">Wasserkasten</rdfs:label>
        <rdfs:label xml:lang="en">dampening fountain</rdfs:label>
        <rdfs:label xml:lang="en">water fountain</rdfs:label>
        <rdfs:label xml:lang="en">water pan</rdfs:label>
        <part:partOf rdf:resource="http://people.aifb.kit.edu/mu2771/step#dampening_form_roller"/>
    </owl:NamedIndividual>
    


    <!-- http://people.aifb.kit.edu/mu2771/step#water_pan_roller -->

    <owl:NamedIndividual rdf:about="http://people.aifb.kit.edu/mu2771/step#water_pan_roller">
        <rdf:type rdf:resource="http://purl.oclc.org/NET/ssnx/ssn#Device"/>
        <dc:creator rdf:resource="http://www.heidelberg.com/"/>
        <rdfs:label xml:lang="de">Tauchwalze</rdfs:label>
        <rdfs:label xml:lang="en">water pan roller</rdfs:label>
        <part:partOf rdf:resource="http://people.aifb.kit.edu/mu2771/step#dampening_fountain"/>
        <part:partOf rdf:resource="http://people.aifb.kit.edu/mu2771/step#water_fountain"/>
        <part:partOf rdf:resource="http://people.aifb.kit.edu/mu2771/step#water_pan"/>
    </owl:NamedIndividual>
    


    <!-- http://people.aifb.kit.edu/mu2771/step#water_roller -->

    <owl:NamedIndividual rdf:about="http://people.aifb.kit.edu/mu2771/step#water_roller">
        <rdf:type rdf:resource="http://purl.oclc.org/NET/ssnx/ssn#Device"/>
        <step:sourceUri rdf:resource="http://people.aifb.kit.edu/mu2771/step#"/>
        <rdfs:label xml:lang="de">Feuchtauftragwalze</rdfs:label>
        <rdfs:label xml:lang="de">Feuchtwalze</rdfs:label>
        <rdfs:label xml:lang="en">damper-roller</rdfs:label>
        <rdfs:label xml:lang="en">water roller</rdfs:label>
        <part:partOf rdf:resource="http://people.aifb.kit.edu/mu2771/step#dampening_system"/>
        <part:partOf rdf:resource="http://people.aifb.kit.edu/mu2771/step#dampening_unit"/>
        <part:partOf rdf:resource="http://people.aifb.kit.edu/mu2771/step#damping_unit"/>
        <part:partOf rdf:resource="http://people.aifb.kit.edu/mu2771/step#moistener"/>
        <part:partOf rdf:resource="http://people.aifb.kit.edu/mu2771/step#print_dampener"/>
    </owl:NamedIndividual>
    


    <!-- http://people.aifb.kit.edu/mu2771/step#zufuehrzeit -->

    <owl:NamedIndividual rdf:about="http://people.aifb.kit.edu/mu2771/step#zufuehrzeit">
        <rdf:type rdf:resource="http://www.w3.org/2006/time#DurationDescription"/>
        <dc:creator rdf:resource="http://www.aifb.kit.edu/web/Sebastian_Bader"/>
        <rdfs:label xml:lang="de">Zufuehrzeit</rdfs:label>
        <rdfs:label xml:lang="de">Zuführzeit</rdfs:label>
    </owl:NamedIndividual>
    


    <!-- http://people.aifb.kit.edu/mu2771/step#2-sheet_detector -->

    <owl:NamedIndividual rdf:about="http://people.aifb.kit.edu/mu2771/step#2-sheet_detector">
        <rdf:type rdf:resource="http://purl.oclc.org/NET/ssnx/ssn#System"/>
        <step:sourceUri rdf:resource="http://people.aifb.kit.edu/mu2771/step#"/>
        <rdfs:label xml:lang="en">2 sheet detector</rdfs:label>
        <rdfs:label xml:lang="en">2-sheet detector</rdfs:label>
        <rdfs:label xml:lang="de">Doppelbogenabfühlung</rdfs:label>
        <rdfs:label xml:lang="de">Doppelbogenkontrolle</rdfs:label>
        <rdfs:label xml:lang="en">two sheet detector</rdfs:label>
        <rdfs:label xml:lang="en">two-sheet detector</rdfs:label>
        <part:partOf rdf:resource="http://people.aifb.kit.edu/mu2771/step#printing_press"/>
    </owl:NamedIndividual>
    


    <!-- http://people.aifb.kit.edu/mu2771/step#blanket/impression_cylinder_washup_device -->

    <owl:NamedIndividual rdf:about="http://people.aifb.kit.edu/mu2771/step#blanket/impression_cylinder_washup_device">
        <rdf:type rdf:resource="http://purl.oclc.org/NET/ssnx/ssn#Device"/>
        <dc:creator rdf:resource="http://www.heidelberg.com/"/>
        <rdfs:label xml:lang="de">Druckzylinder Wascheinrichtung</rdfs:label>
        <rdfs:label xml:lang="de">Druckzylinder-Wascheinrichtung</rdfs:label>
        <rdfs:label xml:lang="de">Druckzylinderwascheinrichtung</rdfs:label>
        <rdfs:label xml:lang="de">Gummituch Wascheinrichtung</rdfs:label>
        <rdfs:label xml:lang="de">Gummituch-/Druckzylinder-Wascheinrichtung</rdfs:label>
        <rdfs:label xml:lang="de">Gummituch-Wascheinrichtung</rdfs:label>
        <rdfs:label xml:lang="de">Gummituchwascheinrichtung</rdfs:label>
        <rdfs:label xml:lang="en">blanket cylinder washup device</rdfs:label>
        <rdfs:label xml:lang="en">blanket/impression cylinder washup device</rdfs:label>
        <rdfs:label xml:lang="en">impression cylinder washup device</rdfs:label>
        <part:partOf rdf:resource="http://people.aifb.kit.edu/mu2771/step#washing_fluid_container"/>
    </owl:NamedIndividual>
    


    <!-- http://www.opengis.net/def/uom/ISO-8601/0/Gregorian -->

    <owl:NamedIndividual rdf:about="http://www.opengis.net/def/uom/ISO-8601/0/Gregorian"/>
    


    <!-- http://www.w3.org/2006/time#Friday -->

    <owl:NamedIndividual rdf:about="http://www.w3.org/2006/time#Friday">
        <rdf:type rdf:resource="http://www.w3.org/2006/time#DayOfWeek"/>
        <rdfs:label xml:lang="en">Friday</rdfs:label>
        <skos:prefLabel xml:lang="de">Freitag</skos:prefLabel>
        <skos:prefLabel xml:lang="en">Friday</skos:prefLabel>
        <skos:prefLabel xml:lang="pl">Piątek</skos:prefLabel>
        <skos:prefLabel xml:lang="pt">Sexta-feira</skos:prefLabel>
        <skos:prefLabel xml:lang="fr">Vendredi</skos:prefLabel>
        <skos:prefLabel xml:lang="it">Venerdì</skos:prefLabel>
        <skos:prefLabel xml:lang="es">Viernes</skos:prefLabel>
        <skos:prefLabel xml:lang="nl">Vrijdag</skos:prefLabel>
        <skos:prefLabel xml:lang="ru">Пятница</skos:prefLabel>
        <skos:prefLabel xml:lang="ar">الجمعة</skos:prefLabel>
        <skos:prefLabel xml:lang="zh">星期五</skos:prefLabel>
        <skos:prefLabel xml:lang="ja">金曜日</skos:prefLabel>
    </owl:NamedIndividual>
    


    <!-- http://www.w3.org/2006/time#Monday -->

    <owl:NamedIndividual rdf:about="http://www.w3.org/2006/time#Monday">
        <rdf:type rdf:resource="http://www.w3.org/2006/time#DayOfWeek"/>
        <rdfs:label xml:lang="en">Monday</rdfs:label>
        <skos:prefLabel xml:lang="fr">Lundi</skos:prefLabel>
        <skos:prefLabel xml:lang="it">Lunedì</skos:prefLabel>
        <skos:prefLabel xml:lang="es">Lunes</skos:prefLabel>
        <skos:prefLabel xml:lang="nl">Maandag</skos:prefLabel>
        <skos:prefLabel xml:lang="en">Monday</skos:prefLabel>
        <skos:prefLabel xml:lang="de">Montag</skos:prefLabel>
        <skos:prefLabel xml:lang="pl">Poniedziałek</skos:prefLabel>
        <skos:prefLabel xml:lang="pt">Segunda-feira</skos:prefLabel>
        <skos:prefLabel xml:lang="ru">Понедельник</skos:prefLabel>
        <skos:prefLabel xml:lang="ar">الاثنين</skos:prefLabel>
        <skos:prefLabel xml:lang="zh">星期一</skos:prefLabel>
        <skos:prefLabel xml:lang="ja">月曜日</skos:prefLabel>
    </owl:NamedIndividual>
    


    <!-- http://www.w3.org/2006/time#Saturday -->

    <owl:NamedIndividual rdf:about="http://www.w3.org/2006/time#Saturday">
        <rdf:type rdf:resource="http://www.w3.org/2006/time#DayOfWeek"/>
        <rdfs:label xml:lang="en">Saturday</rdfs:label>
        <skos:prefLabel xml:lang="it">Sabato</skos:prefLabel>
        <skos:prefLabel xml:lang="fr">Samedi</skos:prefLabel>
        <skos:prefLabel xml:lang="de">Samstag</skos:prefLabel>
        <skos:prefLabel xml:lang="en">Saturday</skos:prefLabel>
        <skos:prefLabel xml:lang="pl">Sobota</skos:prefLabel>
        <skos:prefLabel xml:lang="es">Sábado</skos:prefLabel>
        <skos:prefLabel xml:lang="pt">Sábado</skos:prefLabel>
        <skos:prefLabel xml:lang="nl">Zaterdag</skos:prefLabel>
        <skos:prefLabel xml:lang="ru">Суббота</skos:prefLabel>
        <skos:prefLabel xml:lang="ar">السبت</skos:prefLabel>
        <skos:prefLabel xml:lang="ja">土曜日</skos:prefLabel>
        <skos:prefLabel xml:lang="zh">星期六</skos:prefLabel>
    </owl:NamedIndividual>
    


    <!-- http://www.w3.org/2006/time#Sunday -->

    <owl:NamedIndividual rdf:about="http://www.w3.org/2006/time#Sunday">
        <rdf:type rdf:resource="http://www.w3.org/2006/time#DayOfWeek"/>
        <rdfs:label xml:lang="en">Sunday</rdfs:label>
        <skos:prefLabel xml:lang="fr">Dimanche</skos:prefLabel>
        <skos:prefLabel xml:lang="it">Domenica</skos:prefLabel>
        <skos:prefLabel xml:lang="es">Domingo</skos:prefLabel>
        <skos:prefLabel xml:lang="pt">Domingo</skos:prefLabel>
        <skos:prefLabel xml:lang="pl">Niedziela</skos:prefLabel>
        <skos:prefLabel xml:lang="de">Sonntag</skos:prefLabel>
        <skos:prefLabel xml:lang="en">Sunday</skos:prefLabel>
        <skos:prefLabel xml:lang="nl">Zondag</skos:prefLabel>
        <skos:prefLabel xml:lang="ru">Воскресенье</skos:prefLabel>
        <skos:prefLabel xml:lang="ar">الأحد (يوم)</skos:prefLabel>
        <skos:prefLabel xml:lang="ja">日曜日</skos:prefLabel>
        <skos:prefLabel xml:lang="zh">星期日</skos:prefLabel>
    </owl:NamedIndividual>
    


    <!-- http://www.w3.org/2006/time#Thursday -->

    <owl:NamedIndividual rdf:about="http://www.w3.org/2006/time#Thursday">
        <rdf:type rdf:resource="http://www.w3.org/2006/time#DayOfWeek"/>
        <rdfs:label xml:lang="en">Thursday</rdfs:label>
        <skos:prefLabel xml:lang="pl">Czwartek</skos:prefLabel>
        <skos:prefLabel xml:lang="nl">Donderdag</skos:prefLabel>
        <skos:prefLabel xml:lang="de">Donnerstag</skos:prefLabel>
        <skos:prefLabel xml:lang="it">Giovedì</skos:prefLabel>
        <skos:prefLabel xml:lang="fr">Jeudi</skos:prefLabel>
        <skos:prefLabel xml:lang="es">Jueves</skos:prefLabel>
        <skos:prefLabel xml:lang="pt">Quinta-feira</skos:prefLabel>
        <skos:prefLabel xml:lang="en">Thursday</skos:prefLabel>
        <skos:prefLabel xml:lang="ru">Четверг</skos:prefLabel>
        <skos:prefLabel xml:lang="ar">الخميس</skos:prefLabel>
        <skos:prefLabel xml:lang="zh">星期四</skos:prefLabel>
        <skos:prefLabel xml:lang="ja">木曜日</skos:prefLabel>
    </owl:NamedIndividual>
    


    <!-- http://www.w3.org/2006/time#Tuesday -->

    <owl:NamedIndividual rdf:about="http://www.w3.org/2006/time#Tuesday">
        <rdf:type rdf:resource="http://www.w3.org/2006/time#DayOfWeek"/>
        <rdfs:label xml:lang="en">Tuesday</rdfs:label>
        <skos:prefLabel xml:lang="de">Dienstag</skos:prefLabel>
        <skos:prefLabel xml:lang="nl">Dinsdag</skos:prefLabel>
        <skos:prefLabel xml:lang="fr">Mardi</skos:prefLabel>
        <skos:prefLabel xml:lang="it">Martedì</skos:prefLabel>
        <skos:prefLabel xml:lang="es">Martes</skos:prefLabel>
        <skos:prefLabel xml:lang="pt">Terça-feira</skos:prefLabel>
        <skos:prefLabel xml:lang="en">Tuesday</skos:prefLabel>
        <skos:prefLabel xml:lang="pl">Wtorek</skos:prefLabel>
        <skos:prefLabel xml:lang="ru">Вторник</skos:prefLabel>
        <skos:prefLabel xml:lang="ar">الثلاثاء</skos:prefLabel>
        <skos:prefLabel xml:lang="zh">星期二</skos:prefLabel>
        <skos:prefLabel xml:lang="ja">火曜日</skos:prefLabel>
    </owl:NamedIndividual>
    


    <!-- http://www.w3.org/2006/time#Wednesday -->

    <owl:NamedIndividual rdf:about="http://www.w3.org/2006/time#Wednesday">
        <rdf:type rdf:resource="http://www.w3.org/2006/time#DayOfWeek"/>
        <rdfs:label xml:lang="en">Wednesday</rdfs:label>
        <skos:prefLabel xml:lang="it">Mercoledì</skos:prefLabel>
        <skos:prefLabel xml:lang="fr">Mercredi</skos:prefLabel>
        <skos:prefLabel xml:lang="de">Mittwoch</skos:prefLabel>
        <skos:prefLabel xml:lang="es">Miércoles</skos:prefLabel>
        <skos:prefLabel xml:lang="pt">Quarta-feira</skos:prefLabel>
        <skos:prefLabel xml:lang="en">Wednesday</skos:prefLabel>
        <skos:prefLabel xml:lang="nl">Woensdag</skos:prefLabel>
        <skos:prefLabel xml:lang="pl">Środa</skos:prefLabel>
        <skos:prefLabel xml:lang="ru">Среда</skos:prefLabel>
        <skos:prefLabel xml:lang="ar">الأربعاء</skos:prefLabel>
        <skos:prefLabel xml:lang="zh">星期三</skos:prefLabel>
        <skos:prefLabel xml:lang="ja">水曜日</skos:prefLabel>
    </owl:NamedIndividual>
    


    <!-- http://www.w3.org/2006/time#unitDay -->

    <owl:NamedIndividual rdf:about="http://www.w3.org/2006/time#unitDay">
        <rdf:type rdf:resource="http://www.w3.org/2006/time#TemporalUnit"/>
        <time:days rdf:datatype="http://www.w3.org/2001/XMLSchema#decimal">1</time:days>
        <time:hours rdf:datatype="http://www.w3.org/2001/XMLSchema#decimal">0</time:hours>
        <time:minutes rdf:datatype="http://www.w3.org/2001/XMLSchema#decimal">0</time:minutes>
        <time:months rdf:datatype="http://www.w3.org/2001/XMLSchema#decimal">0</time:months>
        <time:seconds rdf:datatype="http://www.w3.org/2001/XMLSchema#decimal">0</time:seconds>
        <time:weeks rdf:datatype="http://www.w3.org/2001/XMLSchema#decimal">0</time:weeks>
        <time:years rdf:datatype="http://www.w3.org/2001/XMLSchema#decimal">0</time:years>
        <rdfs:label xml:lang="en">Day (unit of temporal duration)</rdfs:label>
        <skos:prefLabel xml:lang="de">Tag</skos:prefLabel>
        <skos:prefLabel xml:lang="nl">dag</skos:prefLabel>
        <skos:prefLabel xml:lang="en">day</skos:prefLabel>
        <skos:prefLabel xml:lang="pt">dia</skos:prefLabel>
        <skos:prefLabel xml:lang="pl">doba</skos:prefLabel>
        <skos:prefLabel xml:lang="es">día</skos:prefLabel>
        <skos:prefLabel xml:lang="it">giorno</skos:prefLabel>
        <skos:prefLabel xml:lang="fr">jour</skos:prefLabel>
        <skos:prefLabel xml:lang="ar">يوماً ما</skos:prefLabel>
        <skos:prefLabel xml:lang="jp">ある日</skos:prefLabel>
        <skos:prefLabel xml:lang="zh">一天</skos:prefLabel>
        <skos:prefLabel xml:lang="kr">언젠가</skos:prefLabel>
    </owl:NamedIndividual>
    


    <!-- http://www.w3.org/2006/time#unitHour -->

    <owl:NamedIndividual rdf:about="http://www.w3.org/2006/time#unitHour">
        <rdf:type rdf:resource="http://www.w3.org/2006/time#TemporalUnit"/>
        <time:days rdf:datatype="http://www.w3.org/2001/XMLSchema#decimal">0</time:days>
        <time:hours rdf:datatype="http://www.w3.org/2001/XMLSchema#decimal">1</time:hours>
        <time:minutes rdf:datatype="http://www.w3.org/2001/XMLSchema#decimal">0</time:minutes>
        <time:months rdf:datatype="http://www.w3.org/2001/XMLSchema#decimal">0</time:months>
        <time:seconds rdf:datatype="http://www.w3.org/2001/XMLSchema#decimal">0</time:seconds>
        <time:weeks rdf:datatype="http://www.w3.org/2001/XMLSchema#decimal">0</time:weeks>
        <time:years rdf:datatype="http://www.w3.org/2001/XMLSchema#decimal">0</time:years>
        <rdfs:label xml:lang="en">Hour (unit of temporal duration)</rdfs:label>
        <skos:prefLabel xml:lang="de">Stunde</skos:prefLabel>
        <skos:prefLabel xml:lang="pl">godzina</skos:prefLabel>
        <skos:prefLabel xml:lang="fr">heure</skos:prefLabel>
        <skos:prefLabel xml:lang="es">hora</skos:prefLabel>
        <skos:prefLabel xml:lang="pt">hora</skos:prefLabel>
        <skos:prefLabel xml:lang="en">hour</skos:prefLabel>
        <skos:prefLabel xml:lang="it">ora</skos:prefLabel>
        <skos:prefLabel xml:lang="nl">uur</skos:prefLabel>
        <skos:prefLabel>один час&quot;@ru</skos:prefLabel>
        <skos:prefLabel xml:lang="ar">ساعة واحدة</skos:prefLabel>
        <skos:prefLabel xml:lang="zh">一小時</skos:prefLabel>
        <skos:prefLabel xml:lang="jp">一時間</skos:prefLabel>
        <skos:prefLabel xml:lang="kr">한 시간</skos:prefLabel>
    </owl:NamedIndividual>
    


    <!-- http://www.w3.org/2006/time#unitMinute -->

    <owl:NamedIndividual rdf:about="http://www.w3.org/2006/time#unitMinute">
        <rdf:type rdf:resource="http://www.w3.org/2006/time#TemporalUnit"/>
        <time:days rdf:datatype="http://www.w3.org/2001/XMLSchema#decimal">0</time:days>
        <time:hours rdf:datatype="http://www.w3.org/2001/XMLSchema#decimal">0</time:hours>
        <time:minutes rdf:datatype="http://www.w3.org/2001/XMLSchema#decimal">1</time:minutes>
        <time:months rdf:datatype="http://www.w3.org/2001/XMLSchema#decimal">0</time:months>
        <time:seconds rdf:datatype="http://www.w3.org/2001/XMLSchema#decimal">0</time:seconds>
        <time:weeks rdf:datatype="http://www.w3.org/2001/XMLSchema#decimal">0</time:weeks>
        <time:years rdf:datatype="http://www.w3.org/2001/XMLSchema#decimal">0</time:years>
        <rdfs:label xml:lang="en">Minute (unit of temporal duration)</rdfs:label>
        <skos:prefLabel xml:lang="de">Minute</skos:prefLabel>
        <skos:prefLabel xml:lang="pl">minuta</skos:prefLabel>
        <skos:prefLabel xml:lang="en">minute</skos:prefLabel>
        <skos:prefLabel xml:lang="fr">minute</skos:prefLabel>
        <skos:prefLabel xml:lang="es">minuto</skos:prefLabel>
        <skos:prefLabel xml:lang="it">minuto</skos:prefLabel>
        <skos:prefLabel xml:lang="pt">minuto</skos:prefLabel>
        <skos:prefLabel xml:lang="nl">minuut</skos:prefLabel>
        <skos:prefLabel xml:lang="ru">одна минута</skos:prefLabel>
        <skos:prefLabel xml:lang="ar">دقيقة واحدة</skos:prefLabel>
        <skos:prefLabel xml:lang="jp">一分</skos:prefLabel>
        <skos:prefLabel xml:lang="zh">等一下</skos:prefLabel>
        <skos:prefLabel xml:lang="kr">분</skos:prefLabel>
    </owl:NamedIndividual>
    


    <!-- http://www.w3.org/2006/time#unitMonth -->

    <owl:NamedIndividual rdf:about="http://www.w3.org/2006/time#unitMonth">
        <rdf:type rdf:resource="http://www.w3.org/2006/time#TemporalUnit"/>
        <time:days rdf:datatype="http://www.w3.org/2001/XMLSchema#decimal">0</time:days>
        <time:hours rdf:datatype="http://www.w3.org/2001/XMLSchema#decimal">0</time:hours>
        <time:minutes rdf:datatype="http://www.w3.org/2001/XMLSchema#decimal">0</time:minutes>
        <time:months rdf:datatype="http://www.w3.org/2001/XMLSchema#decimal">1</time:months>
        <time:seconds rdf:datatype="http://www.w3.org/2001/XMLSchema#decimal">0</time:seconds>
        <time:weeks rdf:datatype="http://www.w3.org/2001/XMLSchema#decimal">0</time:weeks>
        <time:years rdf:datatype="http://www.w3.org/2001/XMLSchema#decimal">0</time:years>
        <rdfs:label xml:lang="en">Month (unit of temporal duration)</rdfs:label>
        <skos:prefLabel xml:lang="nl">maand</skos:prefLabel>
        <skos:prefLabel xml:lang="es">mes</skos:prefLabel>
        <skos:prefLabel xml:lang="it">mese</skos:prefLabel>
        <skos:prefLabel xml:lang="pl">miesiąc</skos:prefLabel>
        <skos:prefLabel xml:lang="fr">mois</skos:prefLabel>
        <skos:prefLabel xml:lang="de">monat</skos:prefLabel>
        <skos:prefLabel xml:lang="en">month</skos:prefLabel>
        <skos:prefLabel xml:lang="ru">один месяц</skos:prefLabel>
        <skos:prefLabel xml:lang="ar">شهر واحد</skos:prefLabel>
        <skos:prefLabel xml:lang="jp">一か月</skos:prefLabel>
        <skos:prefLabel xml:lang="zh">一個月</skos:prefLabel>
        <skos:prefLabel xml:lang="kr">한달</skos:prefLabel>
    </owl:NamedIndividual>
    


    <!-- http://www.w3.org/2006/time#unitSecond -->

    <owl:NamedIndividual rdf:about="http://www.w3.org/2006/time#unitSecond">
        <rdf:type rdf:resource="http://www.w3.org/2006/time#TemporalUnit"/>
        <time:days rdf:datatype="http://www.w3.org/2001/XMLSchema#decimal">0</time:days>
        <time:hours rdf:datatype="http://www.w3.org/2001/XMLSchema#decimal">0</time:hours>
        <time:minutes rdf:datatype="http://www.w3.org/2001/XMLSchema#decimal">0</time:minutes>
        <time:months rdf:datatype="http://www.w3.org/2001/XMLSchema#decimal">0</time:months>
        <time:seconds rdf:datatype="http://www.w3.org/2001/XMLSchema#decimal">1</time:seconds>
        <time:weeks rdf:datatype="http://www.w3.org/2001/XMLSchema#decimal">0</time:weeks>
        <time:years rdf:datatype="http://www.w3.org/2001/XMLSchema#decimal">0</time:years>
        <rdfs:label xml:lang="en">Second (unit of temporal duration)</rdfs:label>
        <skos:prefLabel xml:lang="de">Sekunde</skos:prefLabel>
        <skos:prefLabel xml:lang="pl">Sekundę</skos:prefLabel>
        <skos:prefLabel xml:lang="en">second</skos:prefLabel>
        <skos:prefLabel xml:lang="fr">seconde</skos:prefLabel>
        <skos:prefLabel xml:lang="nl">seconde</skos:prefLabel>
        <skos:prefLabel xml:lang="it">secondo</skos:prefLabel>
        <skos:prefLabel xml:lang="es">segundo</skos:prefLabel>
        <skos:prefLabel xml:lang="pt">segundo</skos:prefLabel>
        <skos:prefLabel xml:lang="ar">ثانية واحدة</skos:prefLabel>
        <skos:prefLabel xml:lang="jp">一秒</skos:prefLabel>
        <skos:prefLabel xml:lang="zh">一秒</skos:prefLabel>
        <skos:prefLabel xml:lang="kr">일초</skos:prefLabel>
    </owl:NamedIndividual>
    


    <!-- http://www.w3.org/2006/time#unitWeek -->

    <owl:NamedIndividual rdf:about="http://www.w3.org/2006/time#unitWeek">
        <rdf:type rdf:resource="http://www.w3.org/2006/time#TemporalUnit"/>
        <time:days rdf:datatype="http://www.w3.org/2001/XMLSchema#decimal">0</time:days>
        <time:hours rdf:datatype="http://www.w3.org/2001/XMLSchema#decimal">0</time:hours>
        <time:minutes rdf:datatype="http://www.w3.org/2001/XMLSchema#decimal">0</time:minutes>
        <time:months rdf:datatype="http://www.w3.org/2001/XMLSchema#decimal">0</time:months>
        <time:seconds rdf:datatype="http://www.w3.org/2001/XMLSchema#decimal">0</time:seconds>
        <time:weeks rdf:datatype="http://www.w3.org/2001/XMLSchema#decimal">1</time:weeks>
        <time:years rdf:datatype="http://www.w3.org/2001/XMLSchema#decimal">0</time:years>
        <rdfs:label xml:lang="en">Week (unit of temporal duration)</rdfs:label>
        <skos:prefLabel xml:lang="de">Woche</skos:prefLabel>
        <skos:prefLabel xml:lang="fr">semaine</skos:prefLabel>
        <skos:prefLabel xml:lang="es">semana</skos:prefLabel>
        <skos:prefLabel xml:lang="pt">semana</skos:prefLabel>
        <skos:prefLabel xml:lang="it">settimana</skos:prefLabel>
        <skos:prefLabel xml:lang="pl">tydzień</skos:prefLabel>
        <skos:prefLabel xml:lang="en">week</skos:prefLabel>
        <skos:prefLabel xml:lang="nl">week</skos:prefLabel>
        <skos:prefLabel xml:lang="ru">одна неделя</skos:prefLabel>
        <skos:prefLabel xml:lang="ar">سبوع واحد</skos:prefLabel>
        <skos:prefLabel xml:lang="zh">一周</skos:prefLabel>
        <skos:prefLabel xml:lang="jp">一週間</skos:prefLabel>
        <skos:prefLabel xml:lang="kr">일주일</skos:prefLabel>
    </owl:NamedIndividual>
    


    <!-- http://www.w3.org/2006/time#unitYear -->

    <owl:NamedIndividual rdf:about="http://www.w3.org/2006/time#unitYear">
        <rdf:type rdf:resource="http://www.w3.org/2006/time#TemporalUnit"/>
        <time:days rdf:datatype="http://www.w3.org/2001/XMLSchema#decimal">0</time:days>
        <time:hours rdf:datatype="http://www.w3.org/2001/XMLSchema#decimal">0</time:hours>
        <time:minutes rdf:datatype="http://www.w3.org/2001/XMLSchema#decimal">0</time:minutes>
        <time:months rdf:datatype="http://www.w3.org/2001/XMLSchema#decimal">0</time:months>
        <time:seconds rdf:datatype="http://www.w3.org/2001/XMLSchema#decimal">0</time:seconds>
        <time:weeks rdf:datatype="http://www.w3.org/2001/XMLSchema#decimal">0</time:weeks>
        <time:years rdf:datatype="http://www.w3.org/2001/XMLSchema#decimal">1</time:years>
        <rdfs:label xml:lang="en">Year (unit of temporal duration)</rdfs:label>
        <skos:prefLabel xml:lang="kr">1 년</skos:prefLabel>
        <skos:prefLabel xml:lang="jp">1年</skos:prefLabel>
        <skos:prefLabel xml:lang="de">Jahr</skos:prefLabel>
        <skos:prefLabel xml:lang="pl">Rok</skos:prefLabel>
        <skos:prefLabel xml:lang="fr">an</skos:prefLabel>
        <skos:prefLabel xml:lang="it">anno</skos:prefLabel>
        <skos:prefLabel xml:lang="pt">ano</skos:prefLabel>
        <skos:prefLabel xml:lang="nl">jaar</skos:prefLabel>
        <skos:prefLabel xml:lang="es">un año</skos:prefLabel>
        <skos:prefLabel xml:lang="en">year</skos:prefLabel>
        <skos:prefLabel xml:lang="ru">один год</skos:prefLabel>
        <skos:prefLabel xml:lang="ar">سنة واحدة</skos:prefLabel>
        <skos:prefLabel xml:lang="zh">一年</skos:prefLabel>
    </owl:NamedIndividual>
    


    <!-- http://www.w3.org/ns/org#Head -->

    <owl:NamedIndividual rdf:about="http://www.w3.org/ns/org#Head">
        <rdf:type rdf:resource="http://www.w3.org/ns/org#Role"/>
        <rdfs:comment xml:lang="en">A role corresponding to the `org:headOf` property</rdfs:comment>
        <rdfs:comment xml:lang="es">Actividad correspondiente a la propiedad `org:headOf`.</rdfs:comment>
        <rdfs:comment xml:lang="it">Un ruolo corrispondente alla proprietà `org:headOf`.</rdfs:comment>
        <rdfs:comment xml:lang="fr">Un rôle correspondant à la propriété `org:headOf`</rdfs:comment>
        <rdfs:isDefinedBy rdf:resource="http://www.w3.org/ns/org"/>
        <rdfs:label xml:lang="es">director ejecutivo</rdfs:label>
        <rdfs:label xml:lang="es">directora ejecutiva</rdfs:label>
        <rdfs:label xml:lang="en">head</rdfs:label>
        <rdfs:label xml:lang="it">responsabile</rdfs:label>
        <rdfs:label xml:lang="fr">responsable</rdfs:label>
        <skos:prefLabel xml:lang="en">head</skos:prefLabel>
        <skos:prefLabel xml:lang="it">responsabile</skos:prefLabel>
        <skos:prefLabel xml:lang="fr">responsable</skos:prefLabel>
        <org:roleProperty rdf:resource="http://www.w3.org/ns/org#headOf"/>
    </owl:NamedIndividual>
    <rdf:Description>
        <www:subClassOfInverted rdf:resource="http://www.w3.org/2006/time#DurationDescription"/>
    </rdf:Description>
    <rdf:Description>
        <www:subClassOfInverted rdf:resource="http://www.w3.org/2006/time#TimePosition"/>
        <rdfs:comment xml:lang="en">A temporal position described using either a (nominal) value from an ordinal reference system, or a (numeric) value in a temporal coordinate system. </rdfs:comment>
        <rdfs:label xml:lang="en">Time position</rdfs:label>
        <skos:definition xml:lang="en">A temporal position described using either a (nominal) value from an ordinal reference system, or a (numeric) value in a temporal coordinate system. </skos:definition>
    </rdf:Description>
    <rdf:Description>
        <www:subClassOfInverted rdf:resource="http://www.w3.org/2006/time#DateTimeDescription"/>
    </rdf:Description>
    <rdf:Description>
        <www:subClassOfInverted rdf:resource="http://people.aifb.kit.edu/mu2771/step#UnplannedWorkOrder"/>
    </rdf:Description>
    <rdf:Description>
        <www:subClassOfInverted rdf:resource="http://www.w3.org/2006/time#MonthOfYear"/>
    </rdf:Description>
    <rdf:Description>
        <www:subClassOfInverted>
            <rdf:Description rdf:nodeID="_:genid309">
                <dc:source>skos:exactMatch &apos;feature&apos; [O&amp;M] 
		                    http://www.opengeospatial.org/standards/om</dc:source>
                <www:subClassOfInverted rdf:resource="http://purl.oclc.org/NET/ssnx/ssn#FeatureOfInterest"/>
                <rdfs:comment>A feature is an abstraction of real world phenomena (thing, person, event, etc).</rdfs:comment>
                <rdfs:isDefinedBy>http://purl.oclc.org/NET/ssnx/ssn</rdfs:isDefinedBy>
                <rdfs:label>Feature of Interest</rdfs:label>
                <rdfs:seeAlso>http://www.w3.org/2005/Incubator/ssn/wiki/SSN_Skeleton#Skeleton</rdfs:seeAlso>
            </rdf:Description>
        </www:subClassOfInverted>
    </rdf:Description>
    <rdf:Description>
        <www:subClassOfInverted rdf:resource="http://purl.oclc.org/NET/ssnx/ssn#Observation"/>
    </rdf:Description>
    <rdf:Description>
        <www:subClassOfInverted rdf:resource="http://www.w3.org/2006/time#GeneralDateTimeDescription"/>
    </rdf:Description>
    <rdf:Description>
        <www:subClassOfInverted>
            <rdf:Description rdf:nodeID="_:genid313">
                <www:subClassOfInverted rdf:resource="http://people.aifb.kit.edu/mu2771/step#Technician"/>
                <rdfs:comment xml:lang="en">a technician is any person who can install/maintain/repair a technical system</rdfs:comment>
                <rdfs:label xml:lang="en">Technician</rdfs:label>
                <rdfs:label xml:lang="de">Techniker</rdfs:label>
            </rdf:Description>
        </www:subClassOfInverted>
    </rdf:Description>
    <rdf:Description>
        <www:subClassOfInverted rdf:resource="http://purl.oclc.org/NET/ssnx/ssn#System"/>
    </rdf:Description>
    <rdf:Description>
        <www:subClassOfInverted rdf:resource="http://www.w3.org/2006/time#GeneralDateTimeDescription"/>
    </rdf:Description>
    <rdf:Description>
        <www:subClassOfInverted rdf:resource="http://www.w3.org/2006/time#MonthOfYear"/>
    </rdf:Description>
    <rdf:Description>
        <www:subClassOfInverted rdf:resource="http://www.w3.org/2006/time#GeneralDurationDescription"/>
    </rdf:Description>
    <rdf:Description>
        <www:subClassOfInverted rdf:resource="http://www.w3.org/2006/time#Year"/>
    </rdf:Description>
    <rdf:Description>
        <www:subClassOfInverted rdf:resource="http://www.w3.org/2006/time#DurationDescription"/>
    </rdf:Description>
    <rdf:Description>
        <www:subClassOfInverted rdf:resource="http://purl.oclc.org/NET/ssnx/ssn#Observation"/>
    </rdf:Description>
    <rdf:Description>
        <www:subClassOfInverted rdf:resource="http://purl.oclc.org/NET/ssnx/ssn#MeasurementCapability"/>
    </rdf:Description>
    <rdf:Description>
        <www:subClassOfInverted rdf:resource="http://www.w3.org/2006/time#DurationDescription"/>
    </rdf:Description>
    <rdf:Description>
        <www:subClassOfInverted rdf:resource="http://www.w3.org/2006/time#DurationDescription"/>
    </rdf:Description>
    <rdf:Description>
        <www:subClassOfInverted rdf:resource="http://www.w3.org/2006/time#GeneralDateTimeDescription"/>
    </rdf:Description>
    <rdf:Description>
        <www:subClassOfInverted rdf:resource="http://people.aifb.kit.edu/mu2771/step#Report"/>
    </rdf:Description>
    <rdf:Description>
        <www:subClassOfInverted rdf:resource="http://purl.oclc.org/NET/ssnx/ssn#SensorInput"/>
    </rdf:Description>
    <rdf:Description>
        <www:subClassOfInverted rdf:resource="http://purl.oclc.org/NET/ssnx/ssn#System"/>
    </rdf:Description>
    <rdf:Description>
        <www:subClassOfInverted rdf:resource="http://people.aifb.kit.edu/mu2771/step#NewWorkOrder"/>
    </rdf:Description>
    <rdf:Description>
        <www:subClassOfInverted rdf:resource="http://purl.oclc.org/NET/ssnx/ssn#ObservationValue"/>
    </rdf:Description>
    <rdf:Description>
        <www:subClassOfInverted rdf:resource="http://www.w3.org/2006/time#MonthOfYear"/>
    </rdf:Description>
    <rdf:Description>
        <www:subClassOfInverted rdf:resource="http://www.w3.org/2006/time#Year"/>
    </rdf:Description>
    <rdf:Description>
        <www:subClassOfInverted rdf:resource="http://purl.oclc.org/NET/ssnx/ssn#DeploymentRelatedProcess"/>
    </rdf:Description>
    <rdf:Description>
        <www:subClassOfInverted rdf:resource="http://purl.oclc.org/NET/ssnx/ssn#MeasurementCapability"/>
    </rdf:Description>
    <rdf:Description>
        <www:subClassOfInverted rdf:resource="http://www.w3.org/2006/time#MonthOfYear"/>
    </rdf:Description>
    <rdf:Description>
        <www:subClassOfInverted rdf:resource="http://people.aifb.kit.edu/mu2771/step#WorkOrder"/>
        <rdfs:comment xml:lang="en">a work order represents a customer&apos;s potential problem, which can or can not result in an action of a technician</rdfs:comment>
        <rdfs:label xml:lang="de">Auftrag</rdfs:label>
        <rdfs:label xml:lang="de">Servicefall</rdfs:label>
        <rdfs:label xml:lang="en">work order</rdfs:label>
    </rdf:Description>
    <rdf:Description>
        <rdfs:comment xml:lang="en">To specify the birth date of the object</rdfs:comment>
        <rdfs:isDefinedBy rdf:resource="http://www.w3.org/2006/vcard/ns"/>
        <rdfs:label xml:lang="en">birth date</rdfs:label>
    </rdf:Description>
    <rdf:Description>
        <foaf:homepage rdf:resource="http://www.asahi-net.or.jp/~ax2s-kmtn/"/>
        <foaf:name>Shuji Kamitsuna</foaf:name>
    </rdf:Description>
    <rdf:Description>
        <www:subClassOfInverted rdf:resource="http://www.w3.org/2006/time#Year"/>
    </rdf:Description>
    <rdf:Description>
        <www:subClassOfInverted rdf:resource="http://purl.oclc.org/NET/ssnx/ssn#Observation"/>
    </rdf:Description>
    <rdf:Description>
        <www:subClassOfInverted rdf:resource="http://purl.oclc.org/NET/ssnx/ssn#Sensor"/>
    </rdf:Description>
    <rdf:Description>
        <www:subClassOfInverted rdf:resource="http://www.w3.org/2006/time#MonthOfYear"/>
    </rdf:Description>
    <rdf:Description>
        <www:subClassOfInverted rdf:resource="http://purl.oclc.org/NET/ssnx/ssn#Observation"/>
    </rdf:Description>
    <rdf:Description>
        <www:subClassOfInverted rdf:resource="http://www.w3.org/2006/time#DurationDescription"/>
    </rdf:Description>
    <rdf:Description>
        <www:subClassOfInverted rdf:resource="http://www.w3.org/2006/time#Year"/>
    </rdf:Description>
    <rdf:Description>
        <www:subClassOfInverted rdf:resource="http://purl.oclc.org/NET/ssnx/ssn#Process"/>
    </rdf:Description>
    <rdf:Description>
        <www:subClassOfInverted rdf:resource="http://www.w3.org/2006/time#GeneralDateTimeDescription"/>
    </rdf:Description>
    <rdf:Description>
        <www:subClassOfInverted rdf:resource="http://purl.oclc.org/NET/ssnx/ssn#Observation"/>
    </rdf:Description>
    <rdf:Description>
        <www:subClassOfInverted rdf:resource="http://www.w3.org/2006/time#Year"/>
    </rdf:Description>
    <rdf:Description>
        <www:subClassOfInverted rdf:resource="http://www.w3.org/2006/time#January"/>
    </rdf:Description>
    <rdf:Description>
        <www:subClassOfInverted rdf:resource="http://people.aifb.kit.edu/mu2771/step#SpatialTemporalEntity"/>
    </rdf:Description>
    <rdf:Description>
        <www:subClassOfInverted>
            <rdf:Description rdf:nodeID="_:genid352">
                <www:subClassOfInverted rdf:resource="http://people.aifb.kit.edu/mu2771/step#Technician"/>
                <rdfs:comment xml:lang="en">a technician is any person who can install/maintain/repair a technical system</rdfs:comment>
                <rdfs:label xml:lang="en">Technician</rdfs:label>
                <rdfs:label xml:lang="de">Techniker</rdfs:label>
            </rdf:Description>
        </www:subClassOfInverted>
    </rdf:Description>
    <rdf:Description>
        <www:subClassOfInverted rdf:resource="http://purl.oclc.org/NET/ssnx/ssn#SurvivalRange"/>
    </rdf:Description>
    <rdf:Description>
        <www:subClassOfInverted rdf:resource="http://www.w3.org/2006/time#GeneralDurationDescription"/>
    </rdf:Description>
    <rdf:Description>
        <www:subClassOfInverted rdf:resource="http://purl.oclc.org/NET/ssnx/ssn#Platform"/>
    </rdf:Description>
    <rdf:Description>
        <www:subClassOfInverted rdf:resource="http://purl.oclc.org/NET/ssnx/ssn#Observation"/>
    </rdf:Description>
    <rdf:Description>
        <www:subClassOfInverted rdf:resource="http://www.w3.org/2006/time#DurationDescription"/>
    </rdf:Description>
    <rdf:Description>
        <www:subClassOfInverted rdf:resource="http://purl.oclc.org/NET/ssnx/ssn#OperatingRange"/>
    </rdf:Description>
    <rdf:Description>
        <www:subClassOfInverted rdf:resource="http://purl.oclc.org/NET/ssnx/ssn#Deployment"/>
    </rdf:Description>
    <rdf:Description>
        <www:subClassOfInverted rdf:resource="http://www.w3.org/2006/time#GeneralDateTimeDescription"/>
    </rdf:Description>
    <rdf:Description>
        <www:subClassOfInverted rdf:resource="http://purl.oclc.org/NET/ssnx/ssn#ObservationValue"/>
    </rdf:Description>
    <rdf:Description>
        <www:subClassOfInverted rdf:resource="http://purl.oclc.org/NET/ssnx/ssn#ObservationValue"/>
    </rdf:Description>
    <rdf:Description>
        <www:subClassOfInverted rdf:resource="http://www.w3.org/2006/time#GeneralDurationDescription"/>
    </rdf:Description>
    <rdf:Description>
        <www:subClassOfInverted rdf:resource="http://www.w3.org/2006/time#DurationDescription"/>
    </rdf:Description>
    <rdf:Description>
        <rdfs:comment xml:lang="es">Actividad que el agente desempeña en una relación de pertenencia a una organización.</rdfs:comment>
        <rdfs:comment xml:lang="it">Indica il Role che un Agent ricopre in una relazione di Membership con una Organization</rdfs:comment>
        <rdfs:comment xml:lang="en">Indicates the Role that the Agent plays in a Membership relationship with an Organization.</rdfs:comment>
        <rdfs:comment xml:lang="fr">Indique le Rôle de l&apos;Agent dans son Engagement avec l&apos;Organisation.</rdfs:comment>
        <rdfs:comment xml:lang="ja">エージェントが組織との構成員関係において担う役割を示します。ポストの保持者が担う役割を示すためにorg:Postで用いることもできます。</rdfs:comment>
        <rdfs:isDefinedBy rdf:resource="http://www.w3.org/ns/org"/>
        <rdfs:label xml:lang="es">desempeña la actividad de</rdfs:label>
        <rdfs:label xml:lang="en">role</rdfs:label>
        <rdfs:label xml:lang="it">ruolo</rdfs:label>
        <rdfs:label xml:lang="fr">rôle</rdfs:label>
    </rdf:Description>
    <rdf:Description>
        <www:subClassOfInverted rdf:resource="http://purl.oclc.org/NET/ssnx/ssn#Sensor"/>
    </rdf:Description>
    <rdf:Description>
        <www:subClassOfInverted rdf:resource="http://www.w3.org/2006/time#GeneralDateTimeDescription"/>
    </rdf:Description>
    <rdf:Description>
        <www:subClassOfInverted rdf:resource="http://purl.oclc.org/NET/ssnx/ssn#System"/>
    </rdf:Description>
    <rdf:Description>
        <www:subClassOfInverted rdf:resource="http://www.w3.org/2006/time#GeneralDurationDescription"/>
    </rdf:Description>
    <rdf:Description>
        <rdfs:comment xml:lang="en">The date of marriage, or equivalent, of the object</rdfs:comment>
        <rdfs:isDefinedBy rdf:resource="http://www.w3.org/2006/vcard/ns"/>
        <rdfs:label xml:lang="en">anniversary</rdfs:label>
    </rdf:Description>
    <rdf:Description>
        <www:subClassOfInverted rdf:resource="http://www.w3.org/2006/time#DateTimeDescription"/>
    </rdf:Description>
    <rdf:Description>
        <www:subClassOfInverted rdf:resource="http://www.w3.org/2006/time#GeneralDurationDescription"/>
    </rdf:Description>
    <rdf:Description>
        <www:subClassOfInverted rdf:resource="http://purl.oclc.org/NET/ssnx/ssn#Observation"/>
    </rdf:Description>
    <rdf:Description>
        <www:subClassOfInverted>
            <rdf:Description rdf:nodeID="_:genid375">
                <dc:source>skos:exactMatch &apos;feature&apos; [O&amp;M] 
		                    http://www.opengeospatial.org/standards/om</dc:source>
                <www:subClassOfInverted rdf:resource="http://purl.oclc.org/NET/ssnx/ssn#FeatureOfInterest"/>
                <rdfs:comment>A feature is an abstraction of real world phenomena (thing, person, event, etc).</rdfs:comment>
                <rdfs:isDefinedBy>http://purl.oclc.org/NET/ssnx/ssn</rdfs:isDefinedBy>
                <rdfs:label>Feature of Interest</rdfs:label>
                <rdfs:seeAlso>http://www.w3.org/2005/Incubator/ssn/wiki/SSN_Skeleton#Skeleton</rdfs:seeAlso>
            </rdf:Description>
        </www:subClassOfInverted>
    </rdf:Description>
    <rdf:Description>
        <www:subClassOfInverted rdf:resource="http://www.w3.org/2006/time#DurationDescription"/>
    </rdf:Description>
    <rdf:Description>
        <www:subClassOfInverted rdf:resource="http://purl.oclc.org/NET/ssnx/ssn#Observation"/>
    </rdf:Description>
    <rdf:Description>
        <www:subClassOfInverted rdf:resource="http://purl.oclc.org/NET/ssnx/ssn#System"/>
    </rdf:Description>
    <rdf:Description>
        <www:subClassOfInverted rdf:resource="http://www.w3.org/2006/time#MonthOfYear"/>
    </rdf:Description>
    <rdf:Description>
        <www:subClassOfInverted rdf:resource="http://purl.oclc.org/NET/ssnx/ssn#Deployment"/>
    </rdf:Description>
    <rdf:Description>
        <www:subClassOfInverted rdf:resource="http://www.w3.org/2006/time#DurationDescription"/>
    </rdf:Description>
    <rdf:Description>
        <www:subClassOfInverted rdf:resource="http://purl.oclc.org/NET/ssnx/ssn#Observation"/>
    </rdf:Description>
    <rdf:Description>
        <www:subClassOfInverted rdf:resource="http://www.w3.org/2006/time#Duration"/>
    </rdf:Description>
    <rdf:Description>
        <www:subClassOfInverted rdf:resource="http://purl.oclc.org/NET/ssnx/ssn#Sensor"/>
    </rdf:Description>
    <rdf:Description>
        <www:subClassOfInverted rdf:resource="http://purl.oclc.org/NET/ssnx/ssn#SensorOutput"/>
    </rdf:Description>
    <rdf:Description>
        <www:subClassOfInverted rdf:resource="http://purl.oclc.org/NET/ssnx/ssn#Process"/>
    </rdf:Description>
    <rdf:Description>
        <rdfs:comment xml:lang="it">Indica una relazione di subordinazione all&apos;interno dell&apos;organigramma. La semantica precisa può variare a seconda dell&apos;organizzazione, per esempio può essere usata per rappresentare la proprietà di supervisione oppure per le relazioni di rendicontazione.</rdfs:comment>
        <rdfs:comment xml:lang="en">Indicates a reporting relationship as might be depicted on an organizational chart. The precise semantics of the reporting relationship will vary by organization but is intended to encompass both direct supervisory relationships (e.g. carrying objective and salary setting authority) and more general reporting or accountability relationships (e.g. so called _dotted line_ reporting).</rdfs:comment>
        <rdfs:comment xml:lang="fr">Indique une relation de subordination comme elle pourrait figurer dans un organigramme. La sémantique précise de cette subordination pourra varier selon l&apos;Organisation mais vise à englober aussi bien les relations hiérarchiques directes (définition d&apos;objectifs, montant du salaire) que des relations plus générales ou organisationnelles (les liens en pointillés dans les organigrammes).</rdfs:comment>
        <rdfs:comment xml:lang="es">Relación de subordinación que se representa en los organigramas de las organizaciones. La semántica de la relación de subordinación varía según las organizaciones, pero su intención es abarcar tanto a las relaciones de supervisión directa (por ejemplo, aquellas en las que la autoridad determina los objetivos o el salario) como a las relaciones de subordinación más generales (por ejemplo, las llamadas líneas de autoridad o de mando (y responsabilidad) (http://www.promonegocios.net/organigramas/tipos-de-organigramas.html)).</rdfs:comment>
        <rdfs:comment xml:lang="ja">組織図で描かれるかもしれないような上下関係を示します。エージェント間またはエージェントが就くことができるポスト間の上下関係を直接的に示すために使用できます。</rdfs:comment>
        <rdfs:isDefinedBy rdf:resource="http://www.w3.org/ns/org"/>
        <rdfs:label xml:lang="fr">est subordonné à</rdfs:label>
        <rdfs:label xml:lang="en">reports to</rdfs:label>
        <rdfs:label xml:lang="es">responde ante</rdfs:label>
        <rdfs:label xml:lang="it">riporta a</rdfs:label>
    </rdf:Description>
    <rdf:Description>
        <www:subClassOfInverted rdf:resource="http://people.aifb.kit.edu/mu2771/step#Route"/>
        <rdfs:comment xml:lang="en">a step:Route is set of spatial-temporal points (step:SpatialTemporalEntity) to define a route for a navigation system</rdfs:comment>
        <rdfs:label xml:lang="en">Route</rdfs:label>
    </rdf:Description>
    <rdf:Description>
        <www:subClassOfInverted rdf:resource="http://people.aifb.kit.edu/mu2771/step#Report"/>
    </rdf:Description>
    <rdf:Description>
        <www:subClassOfInverted rdf:resource="http://www.w3.org/2006/time#GeneralDurationDescription"/>
    </rdf:Description>
    <rdf:Description>
        <rdfs:comment xml:lang="en">To specify the components of the name of the object</rdfs:comment>
        <rdfs:isDefinedBy rdf:resource="http://www.w3.org/2006/vcard/ns"/>
        <rdfs:label xml:lang="en">Name</rdfs:label>
    </rdf:Description>
    <rdf:Description>
        <www:subClassOfInverted rdf:resource="http://purl.oclc.org/NET/ssnx/ssn#Observation"/>
    </rdf:Description>
    <rdf:Description>
        <www:subClassOfInverted rdf:resource="http://www.w3.org/2006/time#MonthOfYear"/>
    </rdf:Description>
    <rdf:Description>
        <www:subClassOfInverted rdf:resource="http://www.w3.org/2006/time#Year"/>
    </rdf:Description>
    <rdf:Description>
        <www:subClassOfInverted rdf:resource="http://purl.oclc.org/NET/ssnx/ssn#Platform"/>
    </rdf:Description>
    <rdf:Description>
        <www:subClassOfInverted rdf:resource="http://www.w3.org/2006/time#Duration"/>
    </rdf:Description>
    <rdf:Description>
        <www:subClassOfInverted rdf:resource="http://people.aifb.kit.edu/mu2771/step#ScheduledWorkOrder"/>
        <rdfs:label xml:lang="de">Geplanter Auftrag</rdfs:label>
        <rdfs:label xml:lang="en">scheduled work order</rdfs:label>
    </rdf:Description>
    <rdf:Description>
        <www:subClassOfInverted rdf:resource="http://www.w3.org/2006/time#DurationDescription"/>
    </rdf:Description>
    <rdf:Description>
        <www:subClassOfInverted rdf:resource="http://purl.oclc.org/NET/ssnx/ssn#System"/>
    </rdf:Description>
    <rdf:Description>
        <www:subClassOfInverted rdf:resource="http://www.w3.org/2006/time#DurationDescription"/>
    </rdf:Description>
    <rdf:Description>
        <www:subClassOfInverted rdf:resource="http://purl.oclc.org/NET/ssnx/ssn#OperatingRange"/>
    </rdf:Description>
    <rdf:Description>
        <www:subClassOfInverted rdf:resource="http://www.w3.org/2006/time#DurationDescription"/>
    </rdf:Description>
    <rdf:Description>
        <www:subClassOfInverted rdf:resource="http://people.aifb.kit.edu/mu2771/step#FinishedWorkOrder"/>
        <rdfs:label xml:lang="de">beendeter Auftrag</rdfs:label>
        <rdfs:label xml:lang="en">finished work order</rdfs:label>
    </rdf:Description>
    <rdf:Description>
        <www:subClassOfInverted rdf:resource="http://www.w3.org/2006/time#MonthOfYear"/>
    </rdf:Description>
    <rdf:Description>
        <www:subClassOfInverted rdf:resource="http://purl.oclc.org/NET/ssnx/ssn#System"/>
    </rdf:Description>
    <rdf:Description>
        <www:subClassOfInverted rdf:resource="http://www.w3.org/2006/time#TemporalPosition"/>
    </rdf:Description>
    <rdf:Description>
        <www:subClassOfInverted rdf:resource="http://purl.oclc.org/NET/ssnx/ssn#Observation"/>
    </rdf:Description>
    <rdf:Description>
        <www:subClassOfInverted rdf:resource="http://www.w3.org/2006/time#January"/>
    </rdf:Description>
    <rdf:Description>
        <www:subClassOfInverted rdf:resource="http://purl.oclc.org/NET/ssnx/ssn#MeasurementCapability"/>
    </rdf:Description>
    <rdf:Description>
        <www:subClassOfInverted rdf:resource="http://www.w3.org/2006/time#DateTimeDescription"/>
    </rdf:Description>
    <rdf:Description>
        <www:subClassOfInverted rdf:resource="http://www.w3.org/2006/time#GeneralDateTimeDescription"/>
    </rdf:Description>
    <rdf:Description>
        <www:subClassOfInverted rdf:resource="http://purl.oclc.org/NET/ssnx/ssn#Observation"/>
    </rdf:Description>
    <rdf:Description>
        <www:subClassOfInverted rdf:resource="http://www.w3.org/2006/time#GeneralDurationDescription"/>
    </rdf:Description>
    <rdf:Description>
        <foaf:homepage rdf:resource="http://www.asahi-net.or.jp/~ax2s-kmtn/"/>
        <foaf:name>Shuji Kamitsuna</foaf:name>
    </rdf:Description>
    <rdf:Description>
        <www:subClassOfInverted rdf:resource="http://www.w3.org/2006/time#GeneralDateTimeDescription"/>
    </rdf:Description>
    <rdf:Description>
        <www:subClassOfInverted rdf:resource="http://purl.oclc.org/NET/ssnx/ssn#Observation"/>
    </rdf:Description>
    <rdf:Description>
        <www:subClassOfInverted rdf:resource="http://purl.oclc.org/NET/ssnx/ssn#Property"/>
    </rdf:Description>
    <rdf:Description>
        <www:subClassOfInverted>
            <rdf:Description rdf:nodeID="_:genid419">
                <www:subClassOfInverted rdf:resource="http://people.aifb.kit.edu/mu2771/step#Technician"/>
                <rdfs:comment xml:lang="en">a technician is any person who can install/maintain/repair a technical system</rdfs:comment>
                <rdfs:label xml:lang="en">Technician</rdfs:label>
                <rdfs:label xml:lang="de">Techniker</rdfs:label>
            </rdf:Description>
        </www:subClassOfInverted>
    </rdf:Description>
    <rdf:Description>
        <www:subClassOfInverted rdf:resource="http://www.w3.org/2006/time#Year"/>
    </rdf:Description>
    <rdf:Description>
        <www:subClassOfInverted rdf:resource="http://purl.oclc.org/NET/ssnx/ssn#Sensor"/>
    </rdf:Description>
    <rdf:Description>
        <www:subClassOfInverted rdf:resource="http://people.aifb.kit.edu/mu2771/step#SpatialTemporalEntity"/>
    </rdf:Description>
    <rdf:Description>
        <www:subClassOfInverted rdf:resource="http://www.w3.org/2006/time#GeneralDurationDescription"/>
    </rdf:Description>
    <rdf:Description>
        <foaf:mbox>dguardiola@quinode.fr</foaf:mbox>
        <foaf:name>Dominique Guardiola</foaf:name>
    </rdf:Description>
    <rdf:Description>
        <foaf:mbox>giorgia.lodi@agid.gov.it</foaf:mbox>
        <foaf:name>Giorgia Lodi</foaf:name>
    </rdf:Description>
    <rdf:Description>
        <foaf:mbox>antonio.maccioni@agid.gov.it</foaf:mbox>
        <foaf:name>Antonio Maccioni</foaf:name>
    </rdf:Description>
    <rdf:Description>
        <foaf:mbox>mpoveda@fi.upm.es</foaf:mbox>
        <foaf:name>María Poveda Villalón</foaf:name>
    </rdf:Description>
    <rdf:Description>
        <foaf:mbox>ogiraldo@fi.upm.es</foaf:mbox>
        <foaf:name>Olga Ximena Giraldo</foaf:name>
    </rdf:Description>
    <rdf:Description>
        <foaf:mbox>dave@epimorphics.com</foaf:mbox>
        <foaf:name>Dave Reynolds</foaf:name>
    </rdf:Description>
    <rdf:Description>
        <foaf:mbox>lupe@fi.upm.es</foaf:mbox>
        <foaf:name>Guadalupe Aguado de Cea</foaf:name>
    </rdf:Description>
    <rdf:Description>
        <foaf:mbox>emontiel@fi.upm.es</foaf:mbox>
        <foaf:name>Elena Montiel Ponsoda</foaf:name>
    </rdf:Description>
    <rdf:Description>
        <www:subClassOfInverted rdf:resource="http://www.w3.org/2006/time#DurationDescription"/>
    </rdf:Description>
    <rdf:Description>
        <www:subClassOfInverted rdf:resource="http://purl.oclc.org/NET/ssnx/ssn#SurvivalRange"/>
    </rdf:Description>
    <rdf:Description>
        <www:subClassOfInverted rdf:resource="http://www.w3.org/2006/time#DateTimeDescription"/>
    </rdf:Description>
    <rdf:Description>
        <www:subClassOfInverted rdf:resource="http://www.w3.org/2006/time#GeneralDateTimeDescription"/>
    </rdf:Description>
    <rdf:Description>
        <www:subClassOfInverted rdf:resource="http://purl.oclc.org/NET/ssnx/ssn#SensorOutput"/>
    </rdf:Description>
    <rdf:Description>
        <www:subClassOfInverted rdf:resource="http://www.w3.org/2006/time#DurationDescription"/>
    </rdf:Description>
    <rdf:Description>
        <www:subClassOfInverted rdf:resource="http://www.w3.org/2006/time#GeneralDateTimeDescription"/>
    </rdf:Description>
    <rdf:Description>
        <www:subClassOfInverted rdf:resource="http://purl.oclc.org/NET/ssnx/ssn#System"/>
    </rdf:Description>
    <rdf:Description>
        <www:subClassOfInverted rdf:resource="http://purl.oclc.org/NET/ssnx/ssn#Process"/>
    </rdf:Description>
    <rdf:Description>
        <www:subClassOfInverted rdf:resource="http://www.w3.org/2006/time#GeneralDateTimeDescription"/>
    </rdf:Description>
    <rdf:Description>
        <www:subClassOfInverted rdf:resource="http://www.w3.org/2006/time#GeneralDateTimeDescription"/>
    </rdf:Description>
    <rdf:Description>
        <rdfs:comment xml:lang="en">The temporal unit which provides the precision of a date-time value or scale of a temporal extent</rdfs:comment>
        <rdfs:label xml:lang="en">temporal unit type</rdfs:label>
    </rdf:Description>
    <rdf:Description>
        <foaf:mbox>antonio.maccioni@agid.gov.it</foaf:mbox>
        <foaf:name>Antonio Maccioni</foaf:name>
    </rdf:Description>
    <rdf:Description>
        <foaf:mbox>mpoveda@fi.upm.es</foaf:mbox>
        <foaf:name>María Poveda Villalón</foaf:name>
    </rdf:Description>
    <rdf:Description>
        <foaf:mbox>dguardiola@quinode.fr</foaf:mbox>
        <foaf:name>Dominique Guardiola</foaf:name>
    </rdf:Description>
    <rdf:Description>
        <foaf:mbox>dave@epimorphics.com</foaf:mbox>
        <foaf:name>Dave Reynolds</foaf:name>
    </rdf:Description>
    <rdf:Description>
        <foaf:mbox>ogiraldo@fi.upm.es</foaf:mbox>
        <foaf:name>Olga Ximena Giraldo</foaf:name>
    </rdf:Description>
    <rdf:Description>
        <rdfs:comment xml:lang="en">The temporal reference system used by a temporal position or extent description. </rdfs:comment>
        <rdfs:label xml:lang="en">Temporal reference system used</rdfs:label>
        <skos:definition xml:lang="en">The temporal reference system used by a temporal position or extent description. </skos:definition>
    </rdf:Description>
    <rdf:Description>
        <foaf:mbox>lupe@fi.upm.es</foaf:mbox>
        <foaf:name>Guadalupe Aguado de Cea</foaf:name>
    </rdf:Description>
    <rdf:Description>
        <foaf:mbox>emontiel@fi.upm.es</foaf:mbox>
        <foaf:name>Elena Montiel Ponsoda</foaf:name>
    </rdf:Description>
    <rdf:Description>
        <foaf:mbox>giorgia.lodi@agid.gov.it</foaf:mbox>
        <foaf:name>Giorgia Lodi</foaf:name>
    </rdf:Description>
    <rdf:Description>
        <rdfs:comment>The relation between something and the point, 
 or other geometrical thing in space, where it is.  For example, the realtionship between
 a radio tower and a Point with a given lat and long.
 Or a relationship between a park and its outline as a closed arc of points, or a road and
 its location as a arc (a sequence of points).
 Clearly in practice there will be limit to the accuracy of any such statement, but one would expect
 an accuracy appropriate for the size of the object and uses such as mapping .
 </rdfs:comment>
        <rdfs:label>location</rdfs:label>
    </rdf:Description>
    <rdf:Description>
        <owl:minQualifiedCardinality rdf:datatype="http://www.w3.org/2001/XMLSchema#nonNegativeInteger">1</owl:minQualifiedCardinality>
    </rdf:Description>
    <rdf:Description>
        <xsd:pattern>---(0[1-9]|[1-9][0-9])(Z|(\+|-)((0[0-9]|1[0-3]):[0-5][0-9]|14:00))?</xsd:pattern>
    </rdf:Description>
    <rdf:Description>
        <owl:minQualifiedCardinality rdf:datatype="http://www.w3.org/2001/XMLSchema#nonNegativeInteger">1</owl:minQualifiedCardinality>
    </rdf:Description>
    <rdf:Description>
        <owl:minQualifiedCardinality rdf:datatype="http://www.w3.org/2001/XMLSchema#nonNegativeInteger">1</owl:minQualifiedCardinality>
    </rdf:Description>
    <rdf:Description>
        <owl:minQualifiedCardinality rdf:datatype="http://www.w3.org/2001/XMLSchema#nonNegativeInteger">1</owl:minQualifiedCardinality>
    </rdf:Description>
    <rdf:Description>
        <xsd:pattern>-?([1-9][0-9]{3,}|0[0-9]{3})(Z|(\+|-)((0[0-9]|1[0-3]):[0-5][0-9]|14:00))?</xsd:pattern>
    </rdf:Description>
    <rdf:Description>
        <xsd:pattern>--(0[1-9]|1[0-9]|20)(Z|(\+|-)((0[0-9]|1[0-3]):[0-5][0-9]|14:00))?</xsd:pattern>
    </rdf:Description>
    


    <!-- 
    ///////////////////////////////////////////////////////////////////////////////////////
    //
    // Annotations
    //
    ///////////////////////////////////////////////////////////////////////////////////////
     -->

    <rdf:Description rdf:about="http://iirds.tekom.de/iirds#Description">
        <rdfs:label xml:lang="en">Description</rdfs:label>
    </rdf:Description>
    <rdf:Description rdf:about="http://iirds.tekom.de/iirds#Document">
        <rdfs:label xml:lang="en">Document</rdfs:label>
        <rdfs:label xml:lang="de">Dokument</rdfs:label>
        <iirds:Description rdf:datatype="http://www.w3.org/2001/XMLSchema#string">A document consists of one or more files. It can be made up from topics. The resource is either a blank node (when there is not a file representing the document) or a file in the iiRDS package.</iirds:Description>
        <rdfs:comment xml:lang="en">A unit of information in an iiRDS package making up a complete document.</rdfs:comment>
    </rdf:Description>
    <rdf:Description rdf:about="http://iirds.tekom.de/iirds#DocumentType">
        <rdfs:label xml:lang="de">Dokumentart</rdfs:label>
        <rdfs:comment xml:lang="en">The type of a document.</rdfs:comment>
        <rdfs:label xml:lang="en">Document type</rdfs:label>
        <iirds:Description rdf:datatype="http://www.w3.org/2001/XMLSchema#string">Document types define the intended purpose of a document.</iirds:Description>
    </rdf:Description>
    <rdf:Description rdf:about="http://iirds.tekom.de/iirds#DocumentationMetadata">
        <iirds:Description rdf:datatype="http://www.w3.org/2001/XMLSchema#string">ClassDescription</iirds:Description>
        <www:subClassOfInverted rdf:resource="http://iirds.tekom.de/iirds#ProductMetadata"/>
        <rdfs:label xml:lang="de">Metadaten der Dokumentation</rdfs:label>
        <www:subClassOfInverted rdf:resource="http://iirds.tekom.de/iirds#FunctionalMetadata"/>
        <rdfs:label xml:lang="en">Documentation metadata</rdfs:label>
    </rdf:Description>
    <rdf:Description rdf:about="http://iirds.tekom.de/iirds#Format">
        <rdfs:label xml:lang="de">Format</rdfs:label>
    </rdf:Description>
    <rdf:Description rdf:about="http://iirds.tekom.de/iirds#Fragment">
        <rdfs:label xml:lang="de">Fragment</rdfs:label>
        <iirds:Description rdf:datatype="http://www.w3.org/2001/XMLSchema#string">Sections, tables, lists, paragraphs and hazard statement are examples of fragments. Fragments are usually parts of topic or document files in an iiRDS package identified by a fragment identifier in the IRI.</iirds:Description>
        <rdfs:comment xml:lang="en">A piece of information within a document of topic.</rdfs:comment>
        <rdfs:label xml:lang="en">Fragment</rdfs:label>
    </rdf:Description>
    <rdf:Description rdf:about="http://iirds.tekom.de/iirds#Identifier">
        <rdfs:label xml:lang="de">Identifier</rdfs:label>
    </rdf:Description>
    <rdf:Description rdf:about="http://iirds.tekom.de/iirds#InformationType">
        <rdfs:label xml:lang="en">Information type</rdfs:label>
        <rdfs:comment xml:lang="en">Type of information. Abstract base class of document and topic type.</rdfs:comment>
        <www:subClassOfInverted rdf:resource="http://iirds.tekom.de/iirds#InformationSubject"/>
        <iirds:Description rdf:datatype="http://www.w3.org/2001/XMLSchema#string">Not indented to be used directly.</iirds:Description>
        <rdfs:label xml:lang="de">Informationsart</rdfs:label>
        <www:subClassOfInverted rdf:resource="http://iirds.tekom.de/iirds#TopicType"/>
        <www:subClassOfInverted rdf:resource="http://iirds.tekom.de/iirds#DocumentType"/>
    </rdf:Description>
    <rdf:Description rdf:about="http://iirds.tekom.de/iirds#InformationUnit">
        <iirds:Description rdf:datatype="http://www.w3.org/2001/XMLSchema#string">Not intended to be used directly. Use the subclasses Package, Document, Topic, and Fragment instead.</iirds:Description>
        <rdfs:label xml:lang="de">Informationseinheit</rdfs:label>
        <www:subClassOfInverted rdf:resource="http://iirds.tekom.de/iirds#Fragment"/>
        <rdfs:comment xml:lang="en">A unit of information. An Information unit is the abstract base class of information units, such as packages, documents, topics, and fragments.</rdfs:comment>
        <www:subClassOfInverted rdf:resource="http://iirds.tekom.de/iirds#Document"/>
        <www:subClassOfInverted rdf:resource="http://iirds.tekom.de/iirds#Topic"/>
        <rdfs:label xml:lang="en">Information unit</rdfs:label>
        <www:subClassOfInverted rdf:resource="http://iirds.tekom.de/iirds#Package"/>
    </rdf:Description>
    <rdf:Description rdf:about="http://iirds.tekom.de/iirds#Language">
        <rdfs:label xml:lang="en">Language</rdfs:label>
        <rdfs:label xml:lang="de">Sprache</rdfs:label>
    </rdf:Description>
    <rdf:Description rdf:about="http://iirds.tekom.de/iirds#Package">
        <rdfs:label xml:lang="de">Paket</rdfs:label>
        <rdfs:comment xml:lang="en">A set of information in terms of documents and topics with its metadata</rdfs:comment>
        <rdfs:label xml:lang="en">Package</rdfs:label>
        <iirds:Description rdf:datatype="http://www.w3.org/2001/XMLSchema#string">There is exactly one Package instance within an iiRDS package. It holds general metadata on the overall iiRDS package.  A blank node or the relative resource IRI “#” must be used for the package.</iirds:Description>
    </rdf:Description>
    <rdf:Description rdf:about="http://iirds.tekom.de/iirds#Product">
        <rdfs:comment xml:lang="de">Beabsichtigtes oder erreichtes Ergebnis einer Arbeit oder eines natürlichen oder künstlichen Vorgangs, das eine Ware oder eine Dienstleistung sein kann.</rdfs:comment>
        <rdfs:label xml:lang="en">Product</rdfs:label>
        <rdfs:label xml:lang="de">Produkt</rdfs:label>
        <iirds:Description rdf:datatype="http://www.w3.org/2001/XMLSchema#string">iiRDS provides product as a docking point for a customer-specific product taxonomy.</iirds:Description>
        <rdfs:comment xml:lang="en">Intended or accomplished result of labour, or of a natural or artificial process, which could be a good or service.</rdfs:comment>
    </rdf:Description>
    <rdf:Description rdf:about="http://iirds.tekom.de/iirds#Title">
        <rdfs:label xml:lang="en">Title</rdfs:label>
        <rdfs:label xml:lang="de">Titel</rdfs:label>
    </rdf:Description>
    <rdf:Description rdf:about="http://iirds.tekom.de/iirds#Topic">
        <iirds:Description rdf:datatype="http://www.w3.org/2001/XMLSchema#string">The resource of a topic is a file in the iiRDS package.</iirds:Description>
        <rdfs:label xml:lang="de">Topic</rdfs:label>
        <rdfs:comment xml:lang="en">A topic is a unit of information covering a single subject.</rdfs:comment>
        <rdfs:label xml:lang="en">Topic</rdfs:label>
    </rdf:Description>
    <rdf:Description rdf:about="http://iirds.tekom.de/iirds#TopicType">
        <rdfs:comment xml:lang="en">Defines the information type of an iiRDS topic.</rdfs:comment>
        <rdfs:label xml:lang="en">Topic type</rdfs:label>
        <rdfs:label xml:lang="de">Topictyp</rdfs:label>
        <iirds:Description rdf:datatype="http://www.w3.org/2001/XMLSchema#string">Possible types include task, learning, and concept. InformationUnits that represent topics may have one or more has-topic-type properties that define the topic&apos;s information type. Topics without a has-topic-type property are generic topics, with no specific type.</iirds:Description>
    </rdf:Description>
    <rdf:Description rdf:about="http://iirds.tekom.de/iirds#has-author">
        <rdfs:label xml:lang="de">hat Autor</rdfs:label>
        <rdfs:label xml:lang="en">has author</rdfs:label>
    </rdf:Description>
    <rdf:Description rdf:about="http://iirds.tekom.de/iirds#has-contributor">
        <iirds:Description rdf:datatype="http://www.w3.org/2001/XMLSchema#string">Organisations and persons are examples of contributors.</iirds:Description>
        <rdfs:label xml:lang="en">has contributor</rdfs:label>
        <rdfs:label xml:lang="de">hat Mitwirkenden</rdfs:label>
        <rdfs:comment xml:lang="en">An entity having made contributions to an information unit.</rdfs:comment>
    </rdf:Description>
    <rdf:Description rdf:about="http://iirds.tekom.de/iirds#has-document-type">
        <rdfs:label xml:lang="de">hat Dokumentart</rdfs:label>
        <rdfs:comment xml:lang="de">Hier fehlt Text</rdfs:comment>
        <rdfs:label xml:lang="en">has document type</rdfs:label>
        <rdfs:comment xml:lang="en">The type of a document.</rdfs:comment>
        <iirds:Description rdf:datatype="http://www.w3.org/2001/XMLSchema#string">Documents have one or more document types. Documents without document types are unspecific documents.</iirds:Description>
    </rdf:Description>
    <rdf:Description rdf:about="http://iirds.tekom.de/iirds#has-information-type">
        <rdfs:comment xml:lang="en">The nature of an information unit.</rdfs:comment>
        <rdfs:label xml:lang="en">has information type</rdfs:label>
        <rdfs:comment xml:lang="de">Hier fehlt Text</rdfs:comment>
        <rdfs:label xml:lang="de">hat Informationsart</rdfs:label>
        <iirds:Description rdf:datatype="http://www.w3.org/2001/XMLSchema#string">Not intended to be used directly. Use has-document-type for documents and has-topic-type for topics.</iirds:Description>
    </rdf:Description>
    <rdf:Description rdf:about="http://iirds.tekom.de/iirds#has-subject">
        <rdfs:label xml:lang="en">has subject</rdfs:label>
        <rdfs:label xml:lang="de">hat Thema</rdfs:label>
    </rdf:Description>
    <rdf:Description rdf:about="http://iirds.tekom.de/iirds#has-topic-type">
        <iirds:Description rdf:datatype="http://www.w3.org/2001/XMLSchema#string">Not intended to be used directly. Use has-document-type for documents and has-topic-type for topics.</iirds:Description>
        <rdfs:label xml:lang="en">has topic type</rdfs:label>
        <rdfs:comment xml:lang="de">Hier fehlt Text</rdfs:comment>
        <rdfs:comment xml:lang="en">The nature of an information unit.</rdfs:comment>
        <rdfs:label xml:lang="de">hat Topictyp</rdfs:label>
    </rdf:Description>
    <rdf:Description rdf:about="http://iirds.tekom.de/iirds#has-version">
        <rdfs:label xml:lang="en">has version</rdfs:label>
        <iirds:Description rdf:datatype="http://www.w3.org/2001/XMLSchema#string">Relates an information unit to another resource. The other resource is another version of the information unit.</iirds:Description>
        <rdfs:comment xml:lang="de">Hier fehlt Text</rdfs:comment>
        <rdfs:comment xml:lang="en">A related resource that is a version, edition, or adaptation of the described resource.</rdfs:comment>
        <rdfs:label xml:lang="de">hat Version</rdfs:label>
    </rdf:Description>
    <rdf:Description rdf:about="http://iirds.tekom.de/iirds#is-version-of">
        <iirds:Description rdf:datatype="http://www.w3.org/2001/XMLSchema#string">Relates an information unit to another resource. The information unit is another version of the resource.</iirds:Description>
        <rdfs:comment xml:lang="en">A related resource of which the described resource is a version, edition, or adaptation.</rdfs:comment>
        <rdfs:label xml:lang="en">is version of</rdfs:label>
        <rdfs:comment xml:lang="de">Hier fehlt Text</rdfs:comment>
        <rdfs:label xml:lang="de">ist Version von</rdfs:label>
    </rdf:Description>
    <rdf:Description rdf:about="http://people.aifb.kit.edu/mu2771/step#hasExpertise">
        <rdfs:comment xml:lang="en">relates the experties to any possible entity. Describes that a person is experienced in a domain/with a product/a process etc.</rdfs:comment>
        <rdfs:label xml:lang="en">has expertise</rdfs:label>
    </rdf:Description>
    <rdf:Description rdf:about="http://www.w3.org/2000/01/rdf-schema#Literal">
        <www:subClassOfInverted rdf:resource="http://www.w3.org/2001/XMLSchema#dateTimeStamp"/>
    </rdf:Description>
    <rdf:Description rdf:about="http://www.w3.org/2001/XMLSchema#dateTimeStamp">
        <rdfs:label>dateTimeStamp</rdfs:label>
    </rdf:Description>
    <rdf:Description rdf:about="http://www.w3.org/2003/01/geo/wgs84_pos#">
        <dc:date>$Date: 2009/04/20 15:00:30 $</dc:date>
        <rdfs:label>geo</rdfs:label>
        <dc:description>A vocabulary for representing latitude, longitude and 
 altitude information in the WGS84 geodetic reference datum. 
 Version $Id: wgs84_pos.rdf,v 1.22 2009/04/20 15:00:30 timbl Exp $. See http://www.w3.org/2003/01/geo/ for more details.</dc:description>
        <rdfs:comment>
Recent changes to this namespace:
$Log: wgs84_pos.rdf,v $
Revision 1.22  2009/04/20 15:00:30  timbl
Remove the time bits which have been deal with elsewhere eg in iCal.

Revision 1.21  2009/04/20 12:52:47  timbl
try again

Revision 1.20  2009/04/20 12:42:11  timbl
Add Event (edited ages ago and never checked in), and location (following discussion http://chatlogs.planetrdf.com/swig/2009-04-20#T12-36-09)

Revision 1.19  2009/04/20 12:36:31  timbl
Add Event (edited ages ago and never checked in), and location (following discussion http://chatlogs.planetrdf.com/swig/2009-04-20#T12-36-09)

Revision 1.18  2006/02/01 22:01:04  danbri
Clarified that lat and long are decimal degrees, and that alt is decimal metres about local reference ellipsoid

Revision 1.17  2004/02/06 17:38:12  danbri
Fixed a bad commit screwup

Revision 1.15  2003/04/19 11:24:08  danbri
Fixed the typo even more.

Revision 1.14  2003/04/19 11:16:56  danbri
fixed a typo

Revision 1.13  2003/02/19 22:27:27  connolly
relaxed domain constraints on lat/long/alt from Point to SpatialThing

Revision 1.12  2003/01/12 01:41:41  danbri
Trying local copy of XSLT doc.

Revision 1.11  2003/01/12 01:20:18  danbri
added a link to morten&apos;s xslt rdfs viewer.

Revision 1.10  2003/01/11 18:56:49  danbri
Removed datatype range from lat and long properties, since they would
have required each occurance of the property to mention the datatype.

Revision 1.9  2003/01/11 11:41:31  danbri
Another typo; repaired rdfs:Property to rdf:Property x4

Revision 1.8  2003/01/11 11:05:02  danbri
Added an rdfs:range for each lat/long/alt property,
http://www.w3.org/2001/XMLSchema#float

Revision 1.7  2003/01/10 20:25:16  danbri
Longer rdfs:comment for Point, trying to be Earth-centric and neutral about
coordinate system(s) at the same time. Feedback welcomed.

Revision 1.6  2003/01/10 20:18:30  danbri
Added CVS log comments into the RDF/XML as an rdfs:comment property of the
vocabulary. Note that this is not common practice (but seems both harmless
and potentially useful).


revision 1.5
date: 2003/01/10 20:14:31;  author: danbri;  state: Exp;  lines: +16 -5
Updated schema:
Added a dc:date, added url for more info. Changed the rdfs:label of the
namespace from gp to geo. Added a class Point, set as the rdfs:domain of
each property. Added XML comment on the lat_long property suggesting that
we might not need it (based on #rdfig commentary from implementors).

revision 1.4
date: 2003/01/10 20:01:07;  author: danbri;  state: Exp;  lines: +6 -5
Fixed typo; several rdfs:about attributes are now rdf:about. Thanks to MortenF in
#rdfig for catching this error.

revision 1.3
date: 2003/01/10 11:59:03;  author: danbri;  state: Exp;  lines: +4 -3
fixed buglet in vocab, added more wgs links

revision 1.2
date: 2003/01/10 11:01:11;  author: danbri;  state: Exp;  lines: +4 -4
Removed alt from the as-a-flat-string property, and switched from
space separated to comma separated.

revision 1.1
date: 2003/01/10 10:53:23;  author: danbri;  state: Exp;
basic geo vocab

</rdfs:comment>
        <dc:title>WGS84 Geo Positioning: an RDF vocabulary</dc:title>
    </rdf:Description>
    <rdf:Description rdf:about="http://www.w3.org/2003/01/geo/wgs84_pos#lat_long">
        <rdfs:comment>A comma-separated representation of a latitude, longitude coordinate.</rdfs:comment>
        <rdfs:label>lat/long</rdfs:label>
    </rdf:Description>
    <rdf:Description rdf:about="http://www.w3.org/2006/time#generalYear">
        <rdfs:label xml:lang="en">Generalized year</rdfs:label>
        <rdfs:comment xml:lang="en">Year number - formulated as a text string with a pattern constraint to reproduce the same lexical form as gYear, but not restricted to values from the Gregorian calendar. 
Note that the value-space is not defined, so a generic OWL2 processor cannot compute ordering relationships of values of this type.</rdfs:comment>
        <skos:definition xml:lang="en">Year number - generalization of xsd:gYear, formulated as a text string with a pattern constraint to reproduce the same lexical form as gYear. Note that the value-space is not defined, so a generic OWL2 processor cannot compute ordering relationships of values of this type.</skos:definition>
    </rdf:Description>
    


    <!-- 
    ///////////////////////////////////////////////////////////////////////////////////////
    //
    // General axioms
    //
    ///////////////////////////////////////////////////////////////////////////////////////
     -->

    <owl:Class>
        <owl:intersectionOf rdf:parseType="Collection">
            <rdf:Description rdf:about="http://www.w3.org/ns/org#Organization"/>
            <owl:Restriction>
                <owl:onProperty rdf:resource="http://www.w3.org/ns/org#hasMember"/>
                <owl:allValuesFrom rdf:resource="http://www.w3.org/ns/org#Organization"/>
            </owl:Restriction>
        </owl:intersectionOf>
        <rdfs:subClassOf rdf:resource="http://www.w3.org/ns/org#Organization"/>
    </owl:Class>
    <owl:Class>
        <owl:intersectionOf rdf:parseType="Collection">
            <owl:Restriction>
                <owl:onProperty rdf:resource="http://www.w3.org/2006/vcard/ns#hasMember"/>
                <owl:someValuesFrom rdf:resource="http://www.w3.org/2006/vcard/ns#Kind"/>
            </owl:Restriction>
            <owl:Restriction>
                <owl:onProperty rdf:resource="http://www.w3.org/2006/vcard/ns#hasMember"/>
                <owl:minQualifiedCardinality rdf:datatype="http://www.w3.org/2001/XMLSchema#nonNegativeInteger">1</owl:minQualifiedCardinality>
                <owl:onClass rdf:resource="http://www.w3.org/2006/vcard/ns#Kind"/>
            </owl:Restriction>
        </owl:intersectionOf>
        <rdfs:subClassOf rdf:resource="http://www.w3.org/2006/vcard/ns#Kind"/>
    </owl:Class>
    <owl:Class>
        <owl:intersectionOf rdf:parseType="Collection">
            <owl:Restriction>
                <owl:onProperty rdf:resource="http://www.w3.org/2006/vcard/ns#region"/>
                <owl:someValuesFrom rdf:resource="http://www.w3.org/2001/XMLSchema#string"/>
            </owl:Restriction>
            <owl:Restriction>
                <owl:onProperty rdf:resource="http://www.w3.org/2006/vcard/ns#region"/>
                <owl:maxCardinality rdf:datatype="http://www.w3.org/2001/XMLSchema#nonNegativeInteger">1</owl:maxCardinality>
            </owl:Restriction>
        </owl:intersectionOf>
        <rdfs:subClassOf rdf:resource="http://www.w3.org/2003/01/geo/wgs84_pos#SpatialThing"/>
    </owl:Class>
    <owl:Class>
        <owl:unionOf rdf:parseType="Collection">
            <rdf:Description rdf:about="http://www.loa-cnr.it/ontologies/DUL.owl#Event"/>
            <rdf:Description rdf:about="http://www.loa-cnr.it/ontologies/DUL.owl#Object"/>
        </owl:unionOf>
        <rdfs:subClassOf>
            <owl:Restriction>
                <owl:onProperty rdf:resource="http://purl.oclc.org/NET/ssnx/ssn#hasProperty"/>
                <owl:someValuesFrom rdf:resource="http://purl.oclc.org/NET/ssnx/ssn#Property"/>
            </owl:Restriction>
        </rdfs:subClassOf>
    </owl:Class>
    <owl:Class>
        <owl:unionOf rdf:parseType="Collection">
            <rdf:Description rdf:about="http://www.loa-cnr.it/ontologies/DUL.owl#Event"/>
            <rdf:Description rdf:about="http://www.loa-cnr.it/ontologies/DUL.owl#Object"/>
        </owl:unionOf>
        <rdfs:subClassOf>
            <owl:Restriction>
                <owl:onProperty rdf:resource="http://purl.oclc.org/NET/ssnx/ssn#hasProperty"/>
                <owl:allValuesFrom rdf:resource="http://purl.oclc.org/NET/ssnx/ssn#Property"/>
            </owl:Restriction>
        </rdfs:subClassOf>
    </owl:Class>
    <owl:Class>
        <owl:unionOf rdf:parseType="Collection">
            <rdf:Description rdf:about="http://www.w3.org/2006/time#Instant"/>
            <rdf:Description rdf:about="http://www.w3.org/2006/time#Interval"/>
        </owl:unionOf>
        <rdfs:subClassOf rdf:resource="http://www.w3.org/2002/07/owl#Thing"/>
    </owl:Class>
    <owl:Class>
        <owl:unionOf rdf:parseType="Collection">
            <owl:Restriction>
                <owl:onProperty rdf:resource="http://people.aifb.kit.edu/mu2771/step#isAvailableAt"/>
                <owl:minQualifiedCardinality rdf:datatype="http://www.w3.org/2001/XMLSchema#nonNegativeInteger">1</owl:minQualifiedCardinality>
                <owl:onClass rdf:resource="http://www.w3.org/2003/01/geo/wgs84_pos#SpatialThing"/>
            </owl:Restriction>
            <owl:Restriction>
                <owl:onProperty rdf:resource="http://www.w3.org/2006/vcard/ns#hasAddress"/>
                <owl:minQualifiedCardinality rdf:datatype="http://www.w3.org/2001/XMLSchema#nonNegativeInteger">1</owl:minQualifiedCardinality>
                <owl:onClass rdf:resource="http://www.w3.org/2006/vcard/ns#Address"/>
            </owl:Restriction>
        </owl:unionOf>
        <rdfs:subClassOf>
            <owl:Restriction>
                <owl:onProperty rdf:resource="http://people.aifb.kit.edu/mu2771/step#hasExpertise"/>
                <owl:someValuesFrom rdf:resource="http://people.aifb.kit.edu/mu2771/step#Expertise"/>
            </owl:Restriction>
        </rdfs:subClassOf>
    </owl:Class>
    <owl:Class>
        <owl:unionOf rdf:parseType="Collection">
            <owl:Restriction>
                <owl:onProperty rdf:resource="http://people.aifb.kit.edu/mu2771/step#isAvailableAt"/>
                <owl:minQualifiedCardinality rdf:datatype="http://www.w3.org/2001/XMLSchema#nonNegativeInteger">1</owl:minQualifiedCardinality>
                <owl:onClass rdf:resource="http://www.w3.org/2003/01/geo/wgs84_pos#SpatialThing"/>
            </owl:Restriction>
            <owl:Restriction>
                <owl:onProperty rdf:resource="http://www.w3.org/2006/vcard/ns#hasAddress"/>
                <owl:minQualifiedCardinality rdf:datatype="http://www.w3.org/2001/XMLSchema#nonNegativeInteger">1</owl:minQualifiedCardinality>
                <owl:onClass rdf:resource="http://www.w3.org/2006/vcard/ns#Address"/>
            </owl:Restriction>
        </owl:unionOf>
        <rdfs:subClassOf>
            <owl:Restriction>
                <owl:onProperty rdf:resource="http://www.w3.org/ns/org#memberOf"/>
                <owl:someValuesFrom rdf:resource="http://www.w3.org/ns/org#Organization"/>
            </owl:Restriction>
        </rdfs:subClassOf>
    </owl:Class>
    <owl:Class>
        <owl:unionOf rdf:parseType="Collection">
            <owl:Restriction>
                <owl:onProperty rdf:resource="http://people.aifb.kit.edu/mu2771/step#isAvailableAt"/>
                <owl:minQualifiedCardinality rdf:datatype="http://www.w3.org/2001/XMLSchema#nonNegativeInteger">1</owl:minQualifiedCardinality>
                <owl:onClass rdf:resource="http://www.w3.org/2003/01/geo/wgs84_pos#SpatialThing"/>
            </owl:Restriction>
            <owl:Restriction>
                <owl:onProperty rdf:resource="http://www.w3.org/2006/vcard/ns#hasAddress"/>
                <owl:minQualifiedCardinality rdf:datatype="http://www.w3.org/2001/XMLSchema#nonNegativeInteger">1</owl:minQualifiedCardinality>
                <owl:onClass rdf:resource="http://www.w3.org/2006/vcard/ns#Address"/>
            </owl:Restriction>
        </owl:unionOf>
        <rdfs:subClassOf>
            <owl:Restriction>
                <owl:onProperty rdf:resource="http://people.aifb.kit.edu/mu2771/step#hasWorktimeAt"/>
                <owl:minQualifiedCardinality rdf:datatype="http://www.w3.org/2001/XMLSchema#nonNegativeInteger">1</owl:minQualifiedCardinality>
                <owl:onClass rdf:resource="http://www.w3.org/2006/time#Interval"/>
            </owl:Restriction>
        </rdfs:subClassOf>
    </owl:Class>
    <owl:Class>
        <owl:oneOf rdf:parseType="Collection">
            <rdf:Description rdf:about="http://www.w3.org/2006/time#unitDay"/>
            <rdf:Description rdf:about="http://www.w3.org/2006/time#unitHour"/>
            <rdf:Description rdf:about="http://www.w3.org/2006/time#unitMinute"/>
            <rdf:Description rdf:about="http://www.w3.org/2006/time#unitMonth"/>
            <rdf:Description rdf:about="http://www.w3.org/2006/time#unitSecond"/>
            <rdf:Description rdf:about="http://www.w3.org/2006/time#unitWeek"/>
            <rdf:Description rdf:about="http://www.w3.org/2006/time#unitYear"/>
        </owl:oneOf>
        <rdfs:subClassOf rdf:resource="http://qudt.org/schema/qudt#Unit"/>
    </owl:Class>
    <owl:Class>
        <owl:oneOf rdf:parseType="Collection">
            <rdf:Description rdf:about="http://www.w3.org/2006/time#unitDay"/>
            <rdf:Description rdf:about="http://www.w3.org/2006/time#unitHour"/>
            <rdf:Description rdf:about="http://www.w3.org/2006/time#unitMinute"/>
            <rdf:Description rdf:about="http://www.w3.org/2006/time#unitMonth"/>
            <rdf:Description rdf:about="http://www.w3.org/2006/time#unitSecond"/>
            <rdf:Description rdf:about="http://www.w3.org/2006/time#unitWeek"/>
            <rdf:Description rdf:about="http://www.w3.org/2006/time#unitYear"/>
        </owl:oneOf>
        <rdfs:subClassOf rdf:resource="http://www.w3.org/2006/time#TemporalDuration"/>
    </owl:Class>
</rdf:RDF>



<!-- Generated by the OWL API (version 4.2.8.20170104-2310) https://github.com/owlcs/owlapi -->

